{"@context":{"rdf":"http://www.w3.org/1999/02/22-rdf-syntax-ns#","owl":"http://www.w3.org/2002/07/owl#","rdfs":"http://www.w3.org/2000/01/rdf-schema#","unece":"https://vocabulary.uncefact.org/"},"@graph":[{"rdfs:label":"AcknowledgementCodeList","@type":"rdfs:Class","@id":"unece:AcknowledgementCodeList","rdfs:comment":"A character string used to represent a type of acknowledgment."},{"@id":"unece:AcknowledgementCodeList#5","@type":"unece:AcknowledgementCodeList","rdf:value":"5","rdfs:comment":"Replace"},{"@id":"unece:AcknowledgementCodeList#6","@type":"unece:AcknowledgementCodeList","rdf:value":"6","rdfs:comment":"Confirmation"},{"@id":"unece:AcknowledgementCodeList#7","@type":"unece:AcknowledgementCodeList","rdf:value":"7","rdfs:comment":"Duplicate"},{"@id":"unece:AcknowledgementCodeList#9","@type":"unece:AcknowledgementCodeList","rdf:value":"9","rdfs:comment":"Original"},{"@id":"unece:AcknowledgementCodeList#18","@type":"unece:AcknowledgementCodeList","rdf:value":"18","rdfs:comment":"Reissue"},{"@id":"unece:AcknowledgementCodeList#31","@type":"unece:AcknowledgementCodeList","rdf:value":"31","rdfs:comment":"Copy"},{"@id":"unece:AcknowledgementCodeList#35","@type":"unece:AcknowledgementCodeList","rdf:value":"35","rdfs:comment":"Retransmission"},{"@id":"unece:AcknowledgementCodeList#43","@type":"unece:AcknowledgementCodeList","rdf:value":"43","rdfs:comment":"Additional transmission"},{"rdfs:label":"CommitmentLevelCodeList","@type":"rdfs:Class","@id":"unece:CommitmentLevelCodeList","rdfs:comment":"A character string used to represent a commitment level."},{"@id":"unece:CommitmentLevelCodeList#1","@type":"unece:CommitmentLevelCodeList","rdf:value":"1","rdfs:comment":"Firm"},{"@id":"unece:CommitmentLevelCodeList#2","@type":"unece:CommitmentLevelCodeList","rdf:value":"2","rdfs:comment":"Commitment for manufacturing and material"},{"@id":"unece:CommitmentLevelCodeList#3","@type":"unece:CommitmentLevelCodeList","rdf:value":"3","rdfs:comment":"Commitment for material"},{"@id":"unece:CommitmentLevelCodeList#4","@type":"unece:CommitmentLevelCodeList","rdf:value":"4","rdfs:comment":"Planning/forecast"},{"@id":"unece:CommitmentLevelCodeList#5","@type":"unece:CommitmentLevelCodeList","rdf:value":"5","rdfs:comment":"Short delivered on previous delivery"},{"@id":"unece:CommitmentLevelCodeList#6","@type":"unece:CommitmentLevelCodeList","rdf:value":"6","rdfs:comment":"Capacity available"},{"@id":"unece:CommitmentLevelCodeList#7","@type":"unece:CommitmentLevelCodeList","rdf:value":"7","rdfs:comment":"Promotion"},{"@id":"unece:CommitmentLevelCodeList#8","@type":"unece:CommitmentLevelCodeList","rdf:value":"8","rdfs:comment":"Special demand"},{"@id":"unece:CommitmentLevelCodeList#9","@type":"unece:CommitmentLevelCodeList","rdf:value":"9","rdfs:comment":"User defined"},{"@id":"unece:CommitmentLevelCodeList#10","@type":"unece:CommitmentLevelCodeList","rdf:value":"10","rdfs:comment":"Immediate"},{"@id":"unece:CommitmentLevelCodeList#11","@type":"unece:CommitmentLevelCodeList","rdf:value":"11","rdfs:comment":"Pilot/Pre-volume"},{"@id":"unece:CommitmentLevelCodeList#12","@type":"unece:CommitmentLevelCodeList","rdf:value":"12","rdfs:comment":"Planning"},{"@id":"unece:CommitmentLevelCodeList#13","@type":"unece:CommitmentLevelCodeList","rdf:value":"13","rdfs:comment":"Potential order increase"},{"@id":"unece:CommitmentLevelCodeList#14","@type":"unece:CommitmentLevelCodeList","rdf:value":"14","rdfs:comment":"Average plant usage"},{"@id":"unece:CommitmentLevelCodeList#15","@type":"unece:CommitmentLevelCodeList","rdf:value":"15","rdfs:comment":"First time reported firm"},{"@id":"unece:CommitmentLevelCodeList#16","@type":"unece:CommitmentLevelCodeList","rdf:value":"16","rdfs:comment":"Maximum"},{"@id":"unece:CommitmentLevelCodeList#17","@type":"unece:CommitmentLevelCodeList","rdf:value":"17","rdfs:comment":"Tooling capacity"},{"@id":"unece:CommitmentLevelCodeList#18","@type":"unece:CommitmentLevelCodeList","rdf:value":"18","rdfs:comment":"Normal tooling capacity"},{"@id":"unece:CommitmentLevelCodeList#19","@type":"unece:CommitmentLevelCodeList","rdf:value":"19","rdfs:comment":"Prototype"},{"@id":"unece:CommitmentLevelCodeList#20","@type":"unece:CommitmentLevelCodeList","rdf:value":"20","rdfs:comment":"Strike protection"},{"@id":"unece:CommitmentLevelCodeList#21","@type":"unece:CommitmentLevelCodeList","rdf:value":"21","rdfs:comment":"Required tooling capacity"},{"@id":"unece:CommitmentLevelCodeList#22","@type":"unece:CommitmentLevelCodeList","rdf:value":"22","rdfs:comment":"Deliver to schedule"},{"@id":"unece:CommitmentLevelCodeList#23","@type":"unece:CommitmentLevelCodeList","rdf:value":"23","rdfs:comment":"Await manual pull"},{"@id":"unece:CommitmentLevelCodeList#24","@type":"unece:CommitmentLevelCodeList","rdf:value":"24","rdfs:comment":"Reference to commercial agreement between partners"},{"@id":"unece:CommitmentLevelCodeList#26","@type":"unece:CommitmentLevelCodeList","rdf:value":"26","rdfs:comment":"Proposed"},{"rdfs:label":"ContactTypeCodeList","@type":"rdfs:Class","@id":"unece:ContactTypeCodeList","rdfs:comment":"A character string used to represent a contact type."},{"@id":"unece:ContactTypeCodeList#AA","@type":"unece:ContactTypeCodeList","rdf:value":"AA","rdfs:comment":"Insurance contact"},{"@id":"unece:ContactTypeCodeList#AB","@type":"unece:ContactTypeCodeList","rdf:value":"AB","rdfs:comment":"Workshop contact"},{"@id":"unece:ContactTypeCodeList#AC","@type":"unece:ContactTypeCodeList","rdf:value":"AC","rdfs:comment":"Accepting contact"},{"@id":"unece:ContactTypeCodeList#AD","@type":"unece:ContactTypeCodeList","rdf:value":"AD","rdfs:comment":"Accounting contact"},{"@id":"unece:ContactTypeCodeList#AE","@type":"unece:ContactTypeCodeList","rdf:value":"AE","rdfs:comment":"Contract contact"},{"@id":"unece:ContactTypeCodeList#AF","@type":"unece:ContactTypeCodeList","rdf:value":"AF","rdfs:comment":"Land registry contact"},{"@id":"unece:ContactTypeCodeList#AG","@type":"unece:ContactTypeCodeList","rdf:value":"AG","rdfs:comment":"Agent"},{"@id":"unece:ContactTypeCodeList#AH","@type":"unece:ContactTypeCodeList","rdf:value":"AH","rdfs:comment":"Coordination contact"},{"@id":"unece:ContactTypeCodeList#AI","@type":"unece:ContactTypeCodeList","rdf:value":"AI","rdfs:comment":"Project management contact"},{"@id":"unece:ContactTypeCodeList#AJ","@type":"unece:ContactTypeCodeList","rdf:value":"AJ","rdfs:comment":"Investment contact"},{"@id":"unece:ContactTypeCodeList#AK","@type":"unece:ContactTypeCodeList","rdf:value":"AK","rdfs:comment":"Works management contact"},{"@id":"unece:ContactTypeCodeList#AL","@type":"unece:ContactTypeCodeList","rdf:value":"AL","rdfs:comment":"Personnel contact"},{"@id":"unece:ContactTypeCodeList#AM","@type":"unece:ContactTypeCodeList","rdf:value":"AM","rdfs:comment":"Claims contact"},{"@id":"unece:ContactTypeCodeList#AN","@type":"unece:ContactTypeCodeList","rdf:value":"AN","rdfs:comment":"Laboratory contact"},{"@id":"unece:ContactTypeCodeList#AO","@type":"unece:ContactTypeCodeList","rdf:value":"AO","rdfs:comment":"Plant/equipment contact"},{"@id":"unece:ContactTypeCodeList#AP","@type":"unece:ContactTypeCodeList","rdf:value":"AP","rdfs:comment":"Accounts payable contact"},{"@id":"unece:ContactTypeCodeList#AQ","@type":"unece:ContactTypeCodeList","rdf:value":"AQ","rdfs:comment":"Quantity surveyor contact"},{"@id":"unece:ContactTypeCodeList#AR","@type":"unece:ContactTypeCodeList","rdf:value":"AR","rdfs:comment":"Accounts receivable contact"},{"@id":"unece:ContactTypeCodeList#AS","@type":"unece:ContactTypeCodeList","rdf:value":"AS","rdfs:comment":"Public relations contact"},{"@id":"unece:ContactTypeCodeList#AT","@type":"unece:ContactTypeCodeList","rdf:value":"AT","rdfs:comment":"Technical contact"},{"@id":"unece:ContactTypeCodeList#AU","@type":"unece:ContactTypeCodeList","rdf:value":"AU","rdfs:comment":"City works authority contact"},{"@id":"unece:ContactTypeCodeList#AV","@type":"unece:ContactTypeCodeList","rdf:value":"AV","rdfs:comment":"Maintenance contact"},{"@id":"unece:ContactTypeCodeList#AW","@type":"unece:ContactTypeCodeList","rdf:value":"AW","rdfs:comment":"Town planning contact"},{"@id":"unece:ContactTypeCodeList#AX","@type":"unece:ContactTypeCodeList","rdf:value":"AX","rdfs:comment":"Traffic authority contact"},{"@id":"unece:ContactTypeCodeList#AY","@type":"unece:ContactTypeCodeList","rdf:value":"AY","rdfs:comment":"Electricity supply contact"},{"@id":"unece:ContactTypeCodeList#AZ","@type":"unece:ContactTypeCodeList","rdf:value":"AZ","rdfs:comment":"Gas supply contact"},{"@id":"unece:ContactTypeCodeList#BA","@type":"unece:ContactTypeCodeList","rdf:value":"BA","rdfs:comment":"Water supply contact"},{"@id":"unece:ContactTypeCodeList#BB","@type":"unece:ContactTypeCodeList","rdf:value":"BB","rdfs:comment":"Telecommunications network contact"},{"@id":"unece:ContactTypeCodeList#BC","@type":"unece:ContactTypeCodeList","rdf:value":"BC","rdfs:comment":"Banking contact"},{"@id":"unece:ContactTypeCodeList#BD","@type":"unece:ContactTypeCodeList","rdf:value":"BD","rdfs:comment":"New developments contact"},{"@id":"unece:ContactTypeCodeList#BE","@type":"unece:ContactTypeCodeList","rdf:value":"BE","rdfs:comment":"Transport infrastructure authority"},{"@id":"unece:ContactTypeCodeList#BF","@type":"unece:ContactTypeCodeList","rdf:value":"BF","rdfs:comment":"Service contact"},{"@id":"unece:ContactTypeCodeList#BG","@type":"unece:ContactTypeCodeList","rdf:value":"BG","rdfs:comment":"Auditing contact"},{"@id":"unece:ContactTypeCodeList#BH","@type":"unece:ContactTypeCodeList","rdf:value":"BH","rdfs:comment":"Legal auditing contact"},{"@id":"unece:ContactTypeCodeList#BI","@type":"unece:ContactTypeCodeList","rdf:value":"BI","rdfs:comment":"Software house contact"},{"@id":"unece:ContactTypeCodeList#BJ","@type":"unece:ContactTypeCodeList","rdf:value":"BJ","rdfs:comment":"Department or person responsible for processing purchase order"},{"@id":"unece:ContactTypeCodeList#BK","@type":"unece:ContactTypeCodeList","rdf:value":"BK","rdfs:comment":"Electronic data interchange coordinator"},{"@id":"unece:ContactTypeCodeList#BL","@type":"unece:ContactTypeCodeList","rdf:value":"BL","rdfs:comment":"Waiver contact"},{"@id":"unece:ContactTypeCodeList#BM","@type":"unece:ContactTypeCodeList","rdf:value":"BM","rdfs:comment":"Automated clearing house (ACH) contact"},{"@id":"unece:ContactTypeCodeList#BN","@type":"unece:ContactTypeCodeList","rdf:value":"BN","rdfs:comment":"Certification contact"},{"@id":"unece:ContactTypeCodeList#BO","@type":"unece:ContactTypeCodeList","rdf:value":"BO","rdfs:comment":"After business hours contact"},{"@id":"unece:ContactTypeCodeList#BP","@type":"unece:ContactTypeCodeList","rdf:value":"BP","rdfs:comment":"Company Security Officer’s 24-hour contact"},{"@id":"unece:ContactTypeCodeList#BQ","@type":"unece:ContactTypeCodeList","rdf:value":"BQ","rdfs:comment":"Agent of ship at the intended port of arrival"},{"@id":"unece:ContactTypeCodeList#BR","@type":"unece:ContactTypeCodeList","rdf:value":"BR","rdfs:comment":"Cook"},{"@id":"unece:ContactTypeCodeList#BS","@type":"unece:ContactTypeCodeList","rdf:value":"BS","rdfs:comment":"Customer contact"},{"@id":"unece:ContactTypeCodeList#BT","@type":"unece:ContactTypeCodeList","rdf:value":"BT","rdfs:comment":"Meter access contact"},{"@id":"unece:ContactTypeCodeList#BU","@type":"unece:ContactTypeCodeList","rdf:value":"BU","rdfs:comment":"Ultimate consignee"},{"@id":"unece:ContactTypeCodeList#CA","@type":"unece:ContactTypeCodeList","rdf:value":"CA","rdfs:comment":"Carrier"},{"@id":"unece:ContactTypeCodeList#CB","@type":"unece:ContactTypeCodeList","rdf:value":"CB","rdfs:comment":"Changed by"},{"@id":"unece:ContactTypeCodeList#CC","@type":"unece:ContactTypeCodeList","rdf:value":"CC","rdfs:comment":"Responsible person for information production"},{"@id":"unece:ContactTypeCodeList#CD","@type":"unece:ContactTypeCodeList","rdf:value":"CD","rdfs:comment":"Responsible person for information dissemination"},{"@id":"unece:ContactTypeCodeList#CE","@type":"unece:ContactTypeCodeList","rdf:value":"CE","rdfs:comment":"Head of unit for computer data processing"},{"@id":"unece:ContactTypeCodeList#CF","@type":"unece:ContactTypeCodeList","rdf:value":"CF","rdfs:comment":"Head of unit for information production"},{"@id":"unece:ContactTypeCodeList#CG","@type":"unece:ContactTypeCodeList","rdf:value":"CG","rdfs:comment":"Head of unit for information dissemination"},{"@id":"unece:ContactTypeCodeList#CN","@type":"unece:ContactTypeCodeList","rdf:value":"CN","rdfs:comment":"Consignee"},{"@id":"unece:ContactTypeCodeList#CO","@type":"unece:ContactTypeCodeList","rdf:value":"CO","rdfs:comment":"Consignor"},{"@id":"unece:ContactTypeCodeList#CP","@type":"unece:ContactTypeCodeList","rdf:value":"CP","rdfs:comment":"Responsible person for computer data processing"},{"@id":"unece:ContactTypeCodeList#CR","@type":"unece:ContactTypeCodeList","rdf:value":"CR","rdfs:comment":"Customer relations"},{"@id":"unece:ContactTypeCodeList#CW","@type":"unece:ContactTypeCodeList","rdf:value":"CW","rdfs:comment":"Confirmed with"},{"@id":"unece:ContactTypeCodeList#DE","@type":"unece:ContactTypeCodeList","rdf:value":"DE","rdfs:comment":"Department/employee to execute export procedures"},{"@id":"unece:ContactTypeCodeList#DI","@type":"unece:ContactTypeCodeList","rdf:value":"DI","rdfs:comment":"Department/employee to execute import procedures"},{"@id":"unece:ContactTypeCodeList#DL","@type":"unece:ContactTypeCodeList","rdf:value":"DL","rdfs:comment":"Delivery contact"},{"@id":"unece:ContactTypeCodeList#EB","@type":"unece:ContactTypeCodeList","rdf:value":"EB","rdfs:comment":"Entered by"},{"@id":"unece:ContactTypeCodeList#EC","@type":"unece:ContactTypeCodeList","rdf:value":"EC","rdfs:comment":"Education coordinator"},{"@id":"unece:ContactTypeCodeList#ED","@type":"unece:ContactTypeCodeList","rdf:value":"ED","rdfs:comment":"Engineering contact"},{"@id":"unece:ContactTypeCodeList#EX","@type":"unece:ContactTypeCodeList","rdf:value":"EX","rdfs:comment":"Expeditor"},{"@id":"unece:ContactTypeCodeList#GR","@type":"unece:ContactTypeCodeList","rdf:value":"GR","rdfs:comment":"Goods receiving contact"},{"@id":"unece:ContactTypeCodeList#HE","@type":"unece:ContactTypeCodeList","rdf:value":"HE","rdfs:comment":"Emergency dangerous goods contact"},{"@id":"unece:ContactTypeCodeList#HG","@type":"unece:ContactTypeCodeList","rdf:value":"HG","rdfs:comment":"Dangerous goods contact"},{"@id":"unece:ContactTypeCodeList#HM","@type":"unece:ContactTypeCodeList","rdf:value":"HM","rdfs:comment":"Hazardous material contact"},{"@id":"unece:ContactTypeCodeList#IC","@type":"unece:ContactTypeCodeList","rdf:value":"IC","rdfs:comment":"Information contact"},{"@id":"unece:ContactTypeCodeList#IN","@type":"unece:ContactTypeCodeList","rdf:value":"IN","rdfs:comment":"Insurer contact"},{"@id":"unece:ContactTypeCodeList#LB","@type":"unece:ContactTypeCodeList","rdf:value":"LB","rdfs:comment":"Place of delivery contact"},{"@id":"unece:ContactTypeCodeList#LO","@type":"unece:ContactTypeCodeList","rdf:value":"LO","rdfs:comment":"Place of collection contact"},{"@id":"unece:ContactTypeCodeList#MC","@type":"unece:ContactTypeCodeList","rdf:value":"MC","rdfs:comment":"Material control contact"},{"@id":"unece:ContactTypeCodeList#MD","@type":"unece:ContactTypeCodeList","rdf:value":"MD","rdfs:comment":"Material disposition contact"},{"@id":"unece:ContactTypeCodeList#MH","@type":"unece:ContactTypeCodeList","rdf:value":"MH","rdfs:comment":"Material handling contact"},{"@id":"unece:ContactTypeCodeList#MR","@type":"unece:ContactTypeCodeList","rdf:value":"MR","rdfs:comment":"Message recipient contact"},{"@id":"unece:ContactTypeCodeList#MS","@type":"unece:ContactTypeCodeList","rdf:value":"MS","rdfs:comment":"Message sender contact"},{"@id":"unece:ContactTypeCodeList#NT","@type":"unece:ContactTypeCodeList","rdf:value":"NT","rdfs:comment":"Notification contact"},{"@id":"unece:ContactTypeCodeList#OC","@type":"unece:ContactTypeCodeList","rdf:value":"OC","rdfs:comment":"Order contact"},{"@id":"unece:ContactTypeCodeList#PA","@type":"unece:ContactTypeCodeList","rdf:value":"PA","rdfs:comment":"Prototype coordinator"},{"@id":"unece:ContactTypeCodeList#PD","@type":"unece:ContactTypeCodeList","rdf:value":"PD","rdfs:comment":"Purchasing contact"},{"@id":"unece:ContactTypeCodeList#PE","@type":"unece:ContactTypeCodeList","rdf:value":"PE","rdfs:comment":"Payee contact"},{"@id":"unece:ContactTypeCodeList#PM","@type":"unece:ContactTypeCodeList","rdf:value":"PM","rdfs:comment":"Product management contact"},{"@id":"unece:ContactTypeCodeList#QA","@type":"unece:ContactTypeCodeList","rdf:value":"QA","rdfs:comment":"Quality assurance contact"},{"@id":"unece:ContactTypeCodeList#QC","@type":"unece:ContactTypeCodeList","rdf:value":"QC","rdfs:comment":"Quality coordinator contact"},{"@id":"unece:ContactTypeCodeList#RD","@type":"unece:ContactTypeCodeList","rdf:value":"RD","rdfs:comment":"Receiving dock contact"},{"@id":"unece:ContactTypeCodeList#RP","@type":"unece:ContactTypeCodeList","rdf:value":"RP","rdfs:comment":"Authorized responsible person"},{"@id":"unece:ContactTypeCodeList#SA","@type":"unece:ContactTypeCodeList","rdf:value":"SA","rdfs:comment":"Sales administration"},{"@id":"unece:ContactTypeCodeList#SC","@type":"unece:ContactTypeCodeList","rdf:value":"SC","rdfs:comment":"Schedule contact"},{"@id":"unece:ContactTypeCodeList#SD","@type":"unece:ContactTypeCodeList","rdf:value":"SD","rdfs:comment":"Shipping contact"},{"@id":"unece:ContactTypeCodeList#SR","@type":"unece:ContactTypeCodeList","rdf:value":"SR","rdfs:comment":"Sales representative or department"},{"@id":"unece:ContactTypeCodeList#SU","@type":"unece:ContactTypeCodeList","rdf:value":"SU","rdfs:comment":"Supplier contact"},{"@id":"unece:ContactTypeCodeList#TA","@type":"unece:ContactTypeCodeList","rdf:value":"TA","rdfs:comment":"Traffic administrator"},{"@id":"unece:ContactTypeCodeList#TD","@type":"unece:ContactTypeCodeList","rdf:value":"TD","rdfs:comment":"Test contact"},{"@id":"unece:ContactTypeCodeList#TI","@type":"unece:ContactTypeCodeList","rdf:value":"TI","rdfs:comment":"Technical documentation recipient"},{"@id":"unece:ContactTypeCodeList#TR","@type":"unece:ContactTypeCodeList","rdf:value":"TR","rdfs:comment":"Transport contact"},{"@id":"unece:ContactTypeCodeList#WH","@type":"unece:ContactTypeCodeList","rdf:value":"WH","rdfs:comment":"Warehouse"},{"@id":"unece:ContactTypeCodeList#WI","@type":"unece:ContactTypeCodeList","rdf:value":"WI","rdfs:comment":"Alternate contact"},{"@id":"unece:ContactTypeCodeList#WJ","@type":"unece:ContactTypeCodeList","rdf:value":"WJ","rdfs:comment":"Office Manager"},{"@id":"unece:ContactTypeCodeList#WK","@type":"unece:ContactTypeCodeList","rdf:value":"WK","rdfs:comment":"Chartered accountant contact"},{"@id":"unece:ContactTypeCodeList#ZZZ","@type":"unece:ContactTypeCodeList","rdf:value":"ZZZ","rdfs:comment":"Mutually defined"},{"rdfs:label":"LineStatusCodeList","@type":"rdfs:Class","@id":"unece:LineStatusCodeList","rdfs:comment":"A character string used to represent a line status."},{"@id":"unece:LineStatusCodeList#1","@type":"unece:LineStatusCodeList","rdf:value":"1","rdfs:comment":"Added"},{"@id":"unece:LineStatusCodeList#2","@type":"unece:LineStatusCodeList","rdf:value":"2","rdfs:comment":"Deleted"},{"@id":"unece:LineStatusCodeList#3","@type":"unece:LineStatusCodeList","rdf:value":"3","rdfs:comment":"Changed"},{"@id":"unece:LineStatusCodeList#4","@type":"unece:LineStatusCodeList","rdf:value":"4","rdfs:comment":"No action"},{"@id":"unece:LineStatusCodeList#5","@type":"unece:LineStatusCodeList","rdf:value":"5","rdfs:comment":"Accepted without amendment"},{"@id":"unece:LineStatusCodeList#6","@type":"unece:LineStatusCodeList","rdf:value":"6","rdfs:comment":"Accepted with amendment"},{"@id":"unece:LineStatusCodeList#7","@type":"unece:LineStatusCodeList","rdf:value":"7","rdfs:comment":"Not accepted"},{"@id":"unece:LineStatusCodeList#8","@type":"unece:LineStatusCodeList","rdf:value":"8","rdfs:comment":"Schedule only"},{"@id":"unece:LineStatusCodeList#9","@type":"unece:LineStatusCodeList","rdf:value":"9","rdfs:comment":"Amendments"},{"@id":"unece:LineStatusCodeList#10","@type":"unece:LineStatusCodeList","rdf:value":"10","rdfs:comment":"Not found"},{"@id":"unece:LineStatusCodeList#11","@type":"unece:LineStatusCodeList","rdf:value":"11","rdfs:comment":"Not amended"},{"@id":"unece:LineStatusCodeList#12","@type":"unece:LineStatusCodeList","rdf:value":"12","rdfs:comment":"Line item numbers changed"},{"@id":"unece:LineStatusCodeList#13","@type":"unece:LineStatusCodeList","rdf:value":"13","rdfs:comment":"Buyer has deducted amount"},{"@id":"unece:LineStatusCodeList#14","@type":"unece:LineStatusCodeList","rdf:value":"14","rdfs:comment":"Buyer claims against invoice"},{"@id":"unece:LineStatusCodeList#15","@type":"unece:LineStatusCodeList","rdf:value":"15","rdfs:comment":"Charge back by seller"},{"@id":"unece:LineStatusCodeList#16","@type":"unece:LineStatusCodeList","rdf:value":"16","rdfs:comment":"Seller will issue credit note"},{"@id":"unece:LineStatusCodeList#17","@type":"unece:LineStatusCodeList","rdf:value":"17","rdfs:comment":"Terms changed for new terms"},{"@id":"unece:LineStatusCodeList#18","@type":"unece:LineStatusCodeList","rdf:value":"18","rdfs:comment":"Abide outcome of negotiations"},{"@id":"unece:LineStatusCodeList#19","@type":"unece:LineStatusCodeList","rdf:value":"19","rdfs:comment":"Seller rejects dispute"},{"@id":"unece:LineStatusCodeList#20","@type":"unece:LineStatusCodeList","rdf:value":"20","rdfs:comment":"Settlement"},{"@id":"unece:LineStatusCodeList#21","@type":"unece:LineStatusCodeList","rdf:value":"21","rdfs:comment":"No delivery"},{"@id":"unece:LineStatusCodeList#22","@type":"unece:LineStatusCodeList","rdf:value":"22","rdfs:comment":"Call-off delivery"},{"@id":"unece:LineStatusCodeList#23","@type":"unece:LineStatusCodeList","rdf:value":"23","rdfs:comment":"Proposed amendment"},{"@id":"unece:LineStatusCodeList#24","@type":"unece:LineStatusCodeList","rdf:value":"24","rdfs:comment":"Accepted with amendment, no confirmation required"},{"@id":"unece:LineStatusCodeList#25","@type":"unece:LineStatusCodeList","rdf:value":"25","rdfs:comment":"Equipment provisionally repaired"},{"@id":"unece:LineStatusCodeList#26","@type":"unece:LineStatusCodeList","rdf:value":"26","rdfs:comment":"Included"},{"@id":"unece:LineStatusCodeList#27","@type":"unece:LineStatusCodeList","rdf:value":"27","rdfs:comment":"Upon receipt and verification of documents we shall cover you when due as per your instructions"},{"@id":"unece:LineStatusCodeList#28","@type":"unece:LineStatusCodeList","rdf:value":"28","rdfs:comment":"Upon receipt and verification of documents we shall authorize you to debit our account with you when due"},{"@id":"unece:LineStatusCodeList#29","@type":"unece:LineStatusCodeList","rdf:value":"29","rdfs:comment":"On receipt of your authenticated advice we shall cover you when due as per your instructions"},{"@id":"unece:LineStatusCodeList#30","@type":"unece:LineStatusCodeList","rdf:value":"30","rdfs:comment":"On receipt of your authenticated advice we shall authorize you to debit our account with you when due"},{"@id":"unece:LineStatusCodeList#31","@type":"unece:LineStatusCodeList","rdf:value":"31","rdfs:comment":"On receipt of your authenticated advice we shall credit your account with us when due"},{"@id":"unece:LineStatusCodeList#32","@type":"unece:LineStatusCodeList","rdf:value":"32","rdfs:comment":"Credit advice requested for direct debit"},{"@id":"unece:LineStatusCodeList#33","@type":"unece:LineStatusCodeList","rdf:value":"33","rdfs:comment":"Credit advice and acknowledgement for direct debit"},{"@id":"unece:LineStatusCodeList#34","@type":"unece:LineStatusCodeList","rdf:value":"34","rdfs:comment":"Inquiry"},{"@id":"unece:LineStatusCodeList#35","@type":"unece:LineStatusCodeList","rdf:value":"35","rdfs:comment":"Checked"},{"@id":"unece:LineStatusCodeList#36","@type":"unece:LineStatusCodeList","rdf:value":"36","rdfs:comment":"Not checked"},{"@id":"unece:LineStatusCodeList#37","@type":"unece:LineStatusCodeList","rdf:value":"37","rdfs:comment":"Cancelled"},{"@id":"unece:LineStatusCodeList#38","@type":"unece:LineStatusCodeList","rdf:value":"38","rdfs:comment":"Replaced"},{"@id":"unece:LineStatusCodeList#39","@type":"unece:LineStatusCodeList","rdf:value":"39","rdfs:comment":"New"},{"@id":"unece:LineStatusCodeList#40","@type":"unece:LineStatusCodeList","rdf:value":"40","rdfs:comment":"Agreed"},{"@id":"unece:LineStatusCodeList#41","@type":"unece:LineStatusCodeList","rdf:value":"41","rdfs:comment":"Proposed"},{"@id":"unece:LineStatusCodeList#42","@type":"unece:LineStatusCodeList","rdf:value":"42","rdfs:comment":"Already delivered"},{"@id":"unece:LineStatusCodeList#43","@type":"unece:LineStatusCodeList","rdf:value":"43","rdfs:comment":"Additional subordinate structures will follow"},{"@id":"unece:LineStatusCodeList#44","@type":"unece:LineStatusCodeList","rdf:value":"44","rdfs:comment":"Additional subordinate structures will not follow"},{"@id":"unece:LineStatusCodeList#45","@type":"unece:LineStatusCodeList","rdf:value":"45","rdfs:comment":"Result opposed"},{"@id":"unece:LineStatusCodeList#46","@type":"unece:LineStatusCodeList","rdf:value":"46","rdfs:comment":"Auction held"},{"@id":"unece:LineStatusCodeList#47","@type":"unece:LineStatusCodeList","rdf:value":"47","rdfs:comment":"Legal action pursued"},{"@id":"unece:LineStatusCodeList#48","@type":"unece:LineStatusCodeList","rdf:value":"48","rdfs:comment":"Meeting held"},{"@id":"unece:LineStatusCodeList#49","@type":"unece:LineStatusCodeList","rdf:value":"49","rdfs:comment":"Result set aside"},{"@id":"unece:LineStatusCodeList#50","@type":"unece:LineStatusCodeList","rdf:value":"50","rdfs:comment":"Result disputed"},{"@id":"unece:LineStatusCodeList#51","@type":"unece:LineStatusCodeList","rdf:value":"51","rdfs:comment":"Countersued"},{"@id":"unece:LineStatusCodeList#52","@type":"unece:LineStatusCodeList","rdf:value":"52","rdfs:comment":"Pending"},{"@id":"unece:LineStatusCodeList#53","@type":"unece:LineStatusCodeList","rdf:value":"53","rdfs:comment":"Court action dismissed"},{"@id":"unece:LineStatusCodeList#54","@type":"unece:LineStatusCodeList","rdf:value":"54","rdfs:comment":"Referred item, accepted"},{"@id":"unece:LineStatusCodeList#55","@type":"unece:LineStatusCodeList","rdf:value":"55","rdfs:comment":"Referred item, rejected"},{"@id":"unece:LineStatusCodeList#56","@type":"unece:LineStatusCodeList","rdf:value":"56","rdfs:comment":"Debit advice statement line"},{"@id":"unece:LineStatusCodeList#57","@type":"unece:LineStatusCodeList","rdf:value":"57","rdfs:comment":"Credit advice statement line"},{"@id":"unece:LineStatusCodeList#58","@type":"unece:LineStatusCodeList","rdf:value":"58","rdfs:comment":"Grouped credit advices"},{"@id":"unece:LineStatusCodeList#59","@type":"unece:LineStatusCodeList","rdf:value":"59","rdfs:comment":"Grouped debit advices"},{"@id":"unece:LineStatusCodeList#60","@type":"unece:LineStatusCodeList","rdf:value":"60","rdfs:comment":"Registered"},{"@id":"unece:LineStatusCodeList#61","@type":"unece:LineStatusCodeList","rdf:value":"61","rdfs:comment":"Payment denied"},{"@id":"unece:LineStatusCodeList#62","@type":"unece:LineStatusCodeList","rdf:value":"62","rdfs:comment":"Approved as amended"},{"@id":"unece:LineStatusCodeList#63","@type":"unece:LineStatusCodeList","rdf:value":"63","rdfs:comment":"Approved as submitted"},{"@id":"unece:LineStatusCodeList#64","@type":"unece:LineStatusCodeList","rdf:value":"64","rdfs:comment":"Cancelled, no activity"},{"@id":"unece:LineStatusCodeList#65","@type":"unece:LineStatusCodeList","rdf:value":"65","rdfs:comment":"Under investigation"},{"@id":"unece:LineStatusCodeList#66","@type":"unece:LineStatusCodeList","rdf:value":"66","rdfs:comment":"Initial claim received"},{"@id":"unece:LineStatusCodeList#67","@type":"unece:LineStatusCodeList","rdf:value":"67","rdfs:comment":"Not in process"},{"@id":"unece:LineStatusCodeList#68","@type":"unece:LineStatusCodeList","rdf:value":"68","rdfs:comment":"Rejected, duplicate"},{"@id":"unece:LineStatusCodeList#69","@type":"unece:LineStatusCodeList","rdf:value":"69","rdfs:comment":"Rejected, resubmit with corrections"},{"@id":"unece:LineStatusCodeList#70","@type":"unece:LineStatusCodeList","rdf:value":"70","rdfs:comment":"Pending, incomplete"},{"@id":"unece:LineStatusCodeList#71","@type":"unece:LineStatusCodeList","rdf:value":"71","rdfs:comment":"Under field office investigation"},{"@id":"unece:LineStatusCodeList#72","@type":"unece:LineStatusCodeList","rdf:value":"72","rdfs:comment":"Pending, awaiting additional material"},{"@id":"unece:LineStatusCodeList#73","@type":"unece:LineStatusCodeList","rdf:value":"73","rdfs:comment":"Pending, awaiting review"},{"@id":"unece:LineStatusCodeList#74","@type":"unece:LineStatusCodeList","rdf:value":"74","rdfs:comment":"Reopened"},{"@id":"unece:LineStatusCodeList#75","@type":"unece:LineStatusCodeList","rdf:value":"75","rdfs:comment":"Processed by primary, forwarded to additional payer(s)"},{"@id":"unece:LineStatusCodeList#76","@type":"unece:LineStatusCodeList","rdf:value":"76","rdfs:comment":"Processed by secondary, forwarded to additional payer(s)"},{"@id":"unece:LineStatusCodeList#77","@type":"unece:LineStatusCodeList","rdf:value":"77","rdfs:comment":"Processed by tertiary, forwarded to additional payer(s)"},{"@id":"unece:LineStatusCodeList#78","@type":"unece:LineStatusCodeList","rdf:value":"78","rdfs:comment":"Previous payment decision reversed"},{"@id":"unece:LineStatusCodeList#79","@type":"unece:LineStatusCodeList","rdf:value":"79","rdfs:comment":"Not our claim, forwarded to another payer(s)"},{"@id":"unece:LineStatusCodeList#80","@type":"unece:LineStatusCodeList","rdf:value":"80","rdfs:comment":"Transferred to correct insurance carrier"},{"@id":"unece:LineStatusCodeList#81","@type":"unece:LineStatusCodeList","rdf:value":"81","rdfs:comment":"Not paid, predetermination pricing only"},{"@id":"unece:LineStatusCodeList#82","@type":"unece:LineStatusCodeList","rdf:value":"82","rdfs:comment":"Documentation claim"},{"@id":"unece:LineStatusCodeList#83","@type":"unece:LineStatusCodeList","rdf:value":"83","rdfs:comment":"Reviewed"},{"@id":"unece:LineStatusCodeList#84","@type":"unece:LineStatusCodeList","rdf:value":"84","rdfs:comment":"Repriced"},{"@id":"unece:LineStatusCodeList#85","@type":"unece:LineStatusCodeList","rdf:value":"85","rdfs:comment":"Audited"},{"@id":"unece:LineStatusCodeList#86","@type":"unece:LineStatusCodeList","rdf:value":"86","rdfs:comment":"Conditionally paid"},{"@id":"unece:LineStatusCodeList#87","@type":"unece:LineStatusCodeList","rdf:value":"87","rdfs:comment":"On appeal"},{"@id":"unece:LineStatusCodeList#88","@type":"unece:LineStatusCodeList","rdf:value":"88","rdfs:comment":"Closed"},{"@id":"unece:LineStatusCodeList#89","@type":"unece:LineStatusCodeList","rdf:value":"89","rdfs:comment":"Reaudited"},{"@id":"unece:LineStatusCodeList#90","@type":"unece:LineStatusCodeList","rdf:value":"90","rdfs:comment":"Reissued"},{"@id":"unece:LineStatusCodeList#91","@type":"unece:LineStatusCodeList","rdf:value":"91","rdfs:comment":"Closed after reopening"},{"@id":"unece:LineStatusCodeList#92","@type":"unece:LineStatusCodeList","rdf:value":"92","rdfs:comment":"Redetermined"},{"@id":"unece:LineStatusCodeList#93","@type":"unece:LineStatusCodeList","rdf:value":"93","rdfs:comment":"Processed as primary"},{"@id":"unece:LineStatusCodeList#94","@type":"unece:LineStatusCodeList","rdf:value":"94","rdfs:comment":"Processed as secondary"},{"@id":"unece:LineStatusCodeList#95","@type":"unece:LineStatusCodeList","rdf:value":"95","rdfs:comment":"Processed as tertiary"},{"@id":"unece:LineStatusCodeList#96","@type":"unece:LineStatusCodeList","rdf:value":"96","rdfs:comment":"Correction of error"},{"@id":"unece:LineStatusCodeList#97","@type":"unece:LineStatusCodeList","rdf:value":"97","rdfs:comment":"Single credit item of a group"},{"@id":"unece:LineStatusCodeList#98","@type":"unece:LineStatusCodeList","rdf:value":"98","rdfs:comment":"Single debit item of a group"},{"@id":"unece:LineStatusCodeList#99","@type":"unece:LineStatusCodeList","rdf:value":"99","rdfs:comment":"Interim response"},{"@id":"unece:LineStatusCodeList#100","@type":"unece:LineStatusCodeList","rdf:value":"100","rdfs:comment":"Final response"},{"@id":"unece:LineStatusCodeList#101","@type":"unece:LineStatusCodeList","rdf:value":"101","rdfs:comment":"Debit advice requested"},{"@id":"unece:LineStatusCodeList#102","@type":"unece:LineStatusCodeList","rdf:value":"102","rdfs:comment":"Transaction not impacted"},{"@id":"unece:LineStatusCodeList#103","@type":"unece:LineStatusCodeList","rdf:value":"103","rdfs:comment":"Patient to be notified"},{"@id":"unece:LineStatusCodeList#104","@type":"unece:LineStatusCodeList","rdf:value":"104","rdfs:comment":"Healthcare provider to be notified"},{"@id":"unece:LineStatusCodeList#105","@type":"unece:LineStatusCodeList","rdf:value":"105","rdfs:comment":"Usual general practitioner to be notified"},{"@id":"unece:LineStatusCodeList#106","@type":"unece:LineStatusCodeList","rdf:value":"106","rdfs:comment":"Advice without details"},{"@id":"unece:LineStatusCodeList#107","@type":"unece:LineStatusCodeList","rdf:value":"107","rdfs:comment":"Advice with details"},{"@id":"unece:LineStatusCodeList#108","@type":"unece:LineStatusCodeList","rdf:value":"108","rdfs:comment":"Amendment requested"},{"@id":"unece:LineStatusCodeList#109","@type":"unece:LineStatusCodeList","rdf:value":"109","rdfs:comment":"For information"},{"@id":"unece:LineStatusCodeList#110","@type":"unece:LineStatusCodeList","rdf:value":"110","rdfs:comment":"Withdraw"},{"@id":"unece:LineStatusCodeList#111","@type":"unece:LineStatusCodeList","rdf:value":"111","rdfs:comment":"Delivery date change"},{"@id":"unece:LineStatusCodeList#112","@type":"unece:LineStatusCodeList","rdf:value":"112","rdfs:comment":"Quantity change"},{"@id":"unece:LineStatusCodeList#113","@type":"unece:LineStatusCodeList","rdf:value":"113","rdfs:comment":"Resale and claim"},{"@id":"unece:LineStatusCodeList#114","@type":"unece:LineStatusCodeList","rdf:value":"114","rdfs:comment":"Resale"},{"@id":"unece:LineStatusCodeList#115","@type":"unece:LineStatusCodeList","rdf:value":"115","rdfs:comment":"Prior addition"},{"@id":"unece:LineStatusCodeList#116","@type":"unece:LineStatusCodeList","rdf:value":"116","rdfs:comment":"Expired"},{"@id":"unece:LineStatusCodeList#117","@type":"unece:LineStatusCodeList","rdf:value":"117","rdfs:comment":"Hold"},{"@id":"unece:LineStatusCodeList#118","@type":"unece:LineStatusCodeList","rdf:value":"118","rdfs:comment":"Open"},{"rdfs:label":"PriorityDescriptionCodeList","@type":"rdfs:Class","@id":"unece:PriorityDescriptionCodeList","rdfs:comment":"A character string used to represent a priority."},{"@id":"unece:PriorityDescriptionCodeList#1","@type":"unece:PriorityDescriptionCodeList","rdf:value":"1","rdfs:comment":"Immediate"},{"@id":"unece:PriorityDescriptionCodeList#2","@type":"unece:PriorityDescriptionCodeList","rdf:value":"2","rdfs:comment":"Urgent"},{"@id":"unece:PriorityDescriptionCodeList#3","@type":"unece:PriorityDescriptionCodeList","rdf:value":"3","rdfs:comment":"Normal"},{"@id":"unece:PriorityDescriptionCodeList#4","@type":"unece:PriorityDescriptionCodeList","rdf:value":"4","rdfs:comment":"Scheduled"},{"@id":"unece:PriorityDescriptionCodeList#5","@type":"unece:PriorityDescriptionCodeList","rdf:value":"5","rdfs:comment":"Category A"},{"@id":"unece:PriorityDescriptionCodeList#6","@type":"unece:PriorityDescriptionCodeList","rdf:value":"6","rdfs:comment":"Category B"},{"rdfs:label":"ProcessTypeCodeList","@type":"rdfs:Class","@id":"unece:ProcessTypeCodeList","rdfs:comment":"A character string used to replace or represent a type of process."},{"@id":"unece:ProcessTypeCodeList#1","@type":"unece:ProcessTypeCodeList","rdf:value":"1","rdfs:comment":"Wood preparation"},{"@id":"unece:ProcessTypeCodeList#2","@type":"unece:ProcessTypeCodeList","rdf:value":"2","rdfs:comment":"Causticizing"},{"@id":"unece:ProcessTypeCodeList#3","@type":"unece:ProcessTypeCodeList","rdf:value":"3","rdfs:comment":"Digesting"},{"@id":"unece:ProcessTypeCodeList#4","@type":"unece:ProcessTypeCodeList","rdf:value":"4","rdfs:comment":"Brownstock washing"},{"@id":"unece:ProcessTypeCodeList#5","@type":"unece:ProcessTypeCodeList","rdf:value":"5","rdfs:comment":"Bleaching"},{"@id":"unece:ProcessTypeCodeList#6","@type":"unece:ProcessTypeCodeList","rdf:value":"6","rdfs:comment":"Pulp drying"},{"@id":"unece:ProcessTypeCodeList#7","@type":"unece:ProcessTypeCodeList","rdf:value":"7","rdfs:comment":"Freezing"},{"@id":"unece:ProcessTypeCodeList#8","@type":"unece:ProcessTypeCodeList","rdf:value":"8","rdfs:comment":"Processing of structured information"},{"@id":"unece:ProcessTypeCodeList#9","@type":"unece:ProcessTypeCodeList","rdf:value":"9","rdfs:comment":"Processing of identical information in structured and unstructured form"},{"@id":"unece:ProcessTypeCodeList#10","@type":"unece:ProcessTypeCodeList","rdf:value":"10","rdfs:comment":"Processing of different information in structured and unstructured form"},{"@id":"unece:ProcessTypeCodeList#11","@type":"unece:ProcessTypeCodeList","rdf:value":"11","rdfs:comment":"Processing of unstructured information"},{"@id":"unece:ProcessTypeCodeList#12","@type":"unece:ProcessTypeCodeList","rdf:value":"12","rdfs:comment":"Slaughter"},{"@id":"unece:ProcessTypeCodeList#13","@type":"unece:ProcessTypeCodeList","rdf:value":"13","rdfs:comment":"Packing"},{"@id":"unece:ProcessTypeCodeList#14","@type":"unece:ProcessTypeCodeList","rdf:value":"14","rdfs:comment":"Heat sterilisation"},{"@id":"unece:ProcessTypeCodeList#15","@type":"unece:ProcessTypeCodeList","rdf:value":"15","rdfs:comment":"Chemical sterilisation"},{"@id":"unece:ProcessTypeCodeList#16","@type":"unece:ProcessTypeCodeList","rdf:value":"16","rdfs:comment":"Fumigation"},{"@id":"unece:ProcessTypeCodeList#17","@type":"unece:ProcessTypeCodeList","rdf:value":"17","rdfs:comment":"Irradiation"},{"@id":"unece:ProcessTypeCodeList#18","@type":"unece:ProcessTypeCodeList","rdf:value":"18","rdfs:comment":"Fueling"},{"@id":"unece:ProcessTypeCodeList#19","@type":"unece:ProcessTypeCodeList","rdf:value":"19","rdfs:comment":"Acceptance of business conditions"},{"@id":"unece:ProcessTypeCodeList#20","@type":"unece:ProcessTypeCodeList","rdf:value":"20","rdfs:comment":"Pathology service"},{"@id":"unece:ProcessTypeCodeList#21","@type":"unece:ProcessTypeCodeList","rdf:value":"21","rdfs:comment":"Radiology service"},{"@id":"unece:ProcessTypeCodeList#22","@type":"unece:ProcessTypeCodeList","rdf:value":"22","rdfs:comment":"Contribution payment"},{"@id":"unece:ProcessTypeCodeList#23","@type":"unece:ProcessTypeCodeList","rdf:value":"23","rdfs:comment":"Clinical donation"},{"@id":"unece:ProcessTypeCodeList#24","@type":"unece:ProcessTypeCodeList","rdf:value":"24","rdfs:comment":"Medical general practice"},{"@id":"unece:ProcessTypeCodeList#25","@type":"unece:ProcessTypeCodeList","rdf:value":"25","rdfs:comment":"Specialist medical service"},{"@id":"unece:ProcessTypeCodeList#26","@type":"unece:ProcessTypeCodeList","rdf:value":"26","rdfs:comment":"Dispensing of medicine"},{"@id":"unece:ProcessTypeCodeList#27","@type":"unece:ProcessTypeCodeList","rdf:value":"27","rdfs:comment":"Planning"},{"@id":"unece:ProcessTypeCodeList#28","@type":"unece:ProcessTypeCodeList","rdf:value":"28","rdfs:comment":"Trading"},{"@id":"unece:ProcessTypeCodeList#29","@type":"unece:ProcessTypeCodeList","rdf:value":"29","rdfs:comment":"Operating"},{"@id":"unece:ProcessTypeCodeList#30","@type":"unece:ProcessTypeCodeList","rdf:value":"30","rdfs:comment":"Metering"},{"@id":"unece:ProcessTypeCodeList#31","@type":"unece:ProcessTypeCodeList","rdf:value":"31","rdfs:comment":"Settlement"},{"@id":"unece:ProcessTypeCodeList#32","@type":"unece:ProcessTypeCodeList","rdf:value":"32","rdfs:comment":"Chilling"},{"@id":"unece:ProcessTypeCodeList#33","@type":"unece:ProcessTypeCodeList","rdf:value":"33","rdfs:comment":"Collecting"},{"@id":"unece:ProcessTypeCodeList#34","@type":"unece:ProcessTypeCodeList","rdf:value":"34","rdfs:comment":"Cutting"},{"@id":"unece:ProcessTypeCodeList#35","@type":"unece:ProcessTypeCodeList","rdf:value":"35","rdfs:comment":"Harvesting"},{"@id":"unece:ProcessTypeCodeList#36","@type":"unece:ProcessTypeCodeList","rdf:value":"36","rdfs:comment":"Inspecting"},{"@id":"unece:ProcessTypeCodeList#37","@type":"unece:ProcessTypeCodeList","rdf:value":"37","rdfs:comment":"Manufacturing"},{"@id":"unece:ProcessTypeCodeList#38","@type":"unece:ProcessTypeCodeList","rdf:value":"38","rdfs:comment":"Preserving"},{"@id":"unece:ProcessTypeCodeList#39","@type":"unece:ProcessTypeCodeList","rdf:value":"39","rdfs:comment":"Processing"},{"@id":"unece:ProcessTypeCodeList#40","@type":"unece:ProcessTypeCodeList","rdf:value":"40","rdfs:comment":"Producing"},{"@id":"unece:ProcessTypeCodeList#41","@type":"unece:ProcessTypeCodeList","rdf:value":"41","rdfs:comment":"Rendering (agriculture)"},{"@id":"unece:ProcessTypeCodeList#42","@type":"unece:ProcessTypeCodeList","rdf:value":"42","rdfs:comment":"Sampling"},{"@id":"unece:ProcessTypeCodeList#43","@type":"unece:ProcessTypeCodeList","rdf:value":"43","rdfs:comment":"Storing"},{"@id":"unece:ProcessTypeCodeList#44","@type":"unece:ProcessTypeCodeList","rdf:value":"44","rdfs:comment":"Transferring"},{"@id":"unece:ProcessTypeCodeList#45","@type":"unece:ProcessTypeCodeList","rdf:value":"45","rdfs:comment":"Treating"},{"@id":"unece:ProcessTypeCodeList#46","@type":"unece:ProcessTypeCodeList","rdf:value":"46","rdfs:comment":"Grinding"},{"@id":"unece:ProcessTypeCodeList#47","@type":"unece:ProcessTypeCodeList","rdf:value":"47","rdfs:comment":"Addition of secondary inhibitors"},{"@id":"unece:ProcessTypeCodeList#48","@type":"unece:ProcessTypeCodeList","rdf:value":"48","rdfs:comment":"Metals recovery"},{"@id":"unece:ProcessTypeCodeList#49","@type":"unece:ProcessTypeCodeList","rdf:value":"49","rdfs:comment":"Solvents recovery"},{"@id":"unece:ProcessTypeCodeList#50","@type":"unece:ProcessTypeCodeList","rdf:value":"50","rdfs:comment":"Recovery for reuse"},{"@id":"unece:ProcessTypeCodeList#51","@type":"unece:ProcessTypeCodeList","rdf:value":"51","rdfs:comment":"Incineration"},{"@id":"unece:ProcessTypeCodeList#52","@type":"unece:ProcessTypeCodeList","rdf:value":"52","rdfs:comment":"On-site fuel recovery"},{"@id":"unece:ProcessTypeCodeList#53","@type":"unece:ProcessTypeCodeList","rdf:value":"53","rdfs:comment":"Fuel blending"},{"@id":"unece:ProcessTypeCodeList#54","@type":"unece:ProcessTypeCodeList","rdf:value":"54","rdfs:comment":"Chemical reduction"},{"@id":"unece:ProcessTypeCodeList#55","@type":"unece:ProcessTypeCodeList","rdf:value":"55","rdfs:comment":"Cyanide destruction"},{"@id":"unece:ProcessTypeCodeList#56","@type":"unece:ProcessTypeCodeList","rdf:value":"56","rdfs:comment":"Chemical oxidation"},{"@id":"unece:ProcessTypeCodeList#57","@type":"unece:ProcessTypeCodeList","rdf:value":"57","rdfs:comment":"Wet air oxidation"},{"@id":"unece:ProcessTypeCodeList#58","@type":"unece:ProcessTypeCodeList","rdf:value":"58","rdfs:comment":"Chemical precipitation"},{"@id":"unece:ProcessTypeCodeList#59","@type":"unece:ProcessTypeCodeList","rdf:value":"59","rdfs:comment":"Biological treatment"},{"@id":"unece:ProcessTypeCodeList#60","@type":"unece:ProcessTypeCodeList","rdf:value":"60","rdfs:comment":"Adsorption"},{"@id":"unece:ProcessTypeCodeList#61","@type":"unece:ProcessTypeCodeList","rdf:value":"61","rdfs:comment":"Air or steam stripping"},{"@id":"unece:ProcessTypeCodeList#62","@type":"unece:ProcessTypeCodeList","rdf:value":"62","rdfs:comment":"Dewatering"},{"@id":"unece:ProcessTypeCodeList#63","@type":"unece:ProcessTypeCodeList","rdf:value":"63","rdfs:comment":"Absorption"},{"@id":"unece:ProcessTypeCodeList#64","@type":"unece:ProcessTypeCodeList","rdf:value":"64","rdfs:comment":"Stabilization"},{"@id":"unece:ProcessTypeCodeList#65","@type":"unece:ProcessTypeCodeList","rdf:value":"65","rdfs:comment":"Macro-encapsulation"},{"@id":"unece:ProcessTypeCodeList#66","@type":"unece:ProcessTypeCodeList","rdf:value":"66","rdfs:comment":"Neutralization"},{"@id":"unece:ProcessTypeCodeList#67","@type":"unece:ProcessTypeCodeList","rdf:value":"67","rdfs:comment":"Evaporation"},{"@id":"unece:ProcessTypeCodeList#68","@type":"unece:ProcessTypeCodeList","rdf:value":"68","rdfs:comment":"Phase separation"},{"@id":"unece:ProcessTypeCodeList#69","@type":"unece:ProcessTypeCodeList","rdf:value":"69","rdfs:comment":"Unspecified treatment"},{"@id":"unece:ProcessTypeCodeList#70","@type":"unece:ProcessTypeCodeList","rdf:value":"70","rdfs:comment":"Landfill or surface impoundment disposal"},{"@id":"unece:ProcessTypeCodeList#71","@type":"unece:ProcessTypeCodeList","rdf:value":"71","rdfs:comment":"Deep well or underground injection"},{"@id":"unece:ProcessTypeCodeList#72","@type":"unece:ProcessTypeCodeList","rdf:value":"72","rdfs:comment":"Discharge to sewer"},{"@id":"unece:ProcessTypeCodeList#73","@type":"unece:ProcessTypeCodeList","rdf:value":"73","rdfs:comment":"Collection and storage, temporary"},{"@id":"unece:ProcessTypeCodeList#74","@type":"unece:ProcessTypeCodeList","rdf:value":"74","rdfs:comment":"Cold treatment"},{"@id":"unece:ProcessTypeCodeList#75","@type":"unece:ProcessTypeCodeList","rdf:value":"75","rdfs:comment":"Hot air treatment"},{"@id":"unece:ProcessTypeCodeList#76","@type":"unece:ProcessTypeCodeList","rdf:value":"76","rdfs:comment":"Hot water treatment"},{"@id":"unece:ProcessTypeCodeList#77","@type":"unece:ProcessTypeCodeList","rdf:value":"77","rdfs:comment":"Methyl bromide treatment"},{"@id":"unece:ProcessTypeCodeList#78","@type":"unece:ProcessTypeCodeList","rdf:value":"78","rdfs:comment":"Phosphine treatment"},{"@id":"unece:ProcessTypeCodeList#79","@type":"unece:ProcessTypeCodeList","rdf:value":"79","rdfs:comment":"Depulping"},{"@id":"unece:ProcessTypeCodeList#80","@type":"unece:ProcessTypeCodeList","rdf:value":"80","rdfs:comment":"Manual removal"},{"@id":"unece:ProcessTypeCodeList#81","@type":"unece:ProcessTypeCodeList","rdf:value":"81","rdfs:comment":"Sulfuryl fluoride fumigation"},{"@id":"unece:ProcessTypeCodeList#82","@type":"unece:ProcessTypeCodeList","rdf:value":"82","rdfs:comment":"Steam treatment"},{"@id":"unece:ProcessTypeCodeList#83","@type":"unece:ProcessTypeCodeList","rdf:value":"83","rdfs:comment":"Vapor heat"},{"@id":"unece:ProcessTypeCodeList#84","@type":"unece:ProcessTypeCodeList","rdf:value":"84","rdfs:comment":"Assembling"},{"@id":"unece:ProcessTypeCodeList#85","@type":"unece:ProcessTypeCodeList","rdf:value":"85","rdfs:comment":"Boiling"},{"@id":"unece:ProcessTypeCodeList#86","@type":"unece:ProcessTypeCodeList","rdf:value":"86","rdfs:comment":"Canning"},{"@id":"unece:ProcessTypeCodeList#87","@type":"unece:ProcessTypeCodeList","rdf:value":"87","rdfs:comment":"Chipping"},{"@id":"unece:ProcessTypeCodeList#88","@type":"unece:ProcessTypeCodeList","rdf:value":"88","rdfs:comment":"Cleaning"},{"@id":"unece:ProcessTypeCodeList#89","@type":"unece:ProcessTypeCodeList","rdf:value":"89","rdfs:comment":"Coating"},{"@id":"unece:ProcessTypeCodeList#90","@type":"unece:ProcessTypeCodeList","rdf:value":"90","rdfs:comment":"Dehydration"},{"@id":"unece:ProcessTypeCodeList#91","@type":"unece:ProcessTypeCodeList","rdf:value":"91","rdfs:comment":"Devitalization"},{"@id":"unece:ProcessTypeCodeList#92","@type":"unece:ProcessTypeCodeList","rdf:value":"92","rdfs:comment":"Disinfection"},{"@id":"unece:ProcessTypeCodeList#93","@type":"unece:ProcessTypeCodeList","rdf:value":"93","rdfs:comment":"Drying"},{"@id":"unece:ProcessTypeCodeList#94","@type":"unece:ProcessTypeCodeList","rdf:value":"94","rdfs:comment":"Dyeing"},{"@id":"unece:ProcessTypeCodeList#95","@type":"unece:ProcessTypeCodeList","rdf:value":"95","rdfs:comment":"Heat treatment"},{"@id":"unece:ProcessTypeCodeList#96","@type":"unece:ProcessTypeCodeList","rdf:value":"96","rdfs:comment":"Husking"},{"@id":"unece:ProcessTypeCodeList#97","@type":"unece:ProcessTypeCodeList","rdf:value":"97","rdfs:comment":"Liquification"},{"@id":"unece:ProcessTypeCodeList#98","@type":"unece:ProcessTypeCodeList","rdf:value":"98","rdfs:comment":"Shelling"},{"@id":"unece:ProcessTypeCodeList#99","@type":"unece:ProcessTypeCodeList","rdf:value":"99","rdfs:comment":"Washing"},{"@id":"unece:ProcessTypeCodeList#100","@type":"unece:ProcessTypeCodeList","rdf:value":"100","rdfs:comment":"Land treatment or application"},{"@id":"unece:ProcessTypeCodeList#101","@type":"unece:ProcessTypeCodeList","rdf:value":"101","rdfs:comment":"Pasteurization"},{"@id":"unece:ProcessTypeCodeList#102","@type":"unece:ProcessTypeCodeList","rdf:value":"102","rdfs:comment":"Biological recycling"},{"@id":"unece:ProcessTypeCodeList#103","@type":"unece:ProcessTypeCodeList","rdf:value":"103","rdfs:comment":"Biological refining"},{"@id":"unece:ProcessTypeCodeList#104","@type":"unece:ProcessTypeCodeList","rdf:value":"104","rdfs:comment":"Blending"},{"@id":"unece:ProcessTypeCodeList#105","@type":"unece:ProcessTypeCodeList","rdf:value":"105","rdfs:comment":"Breeding"},{"@id":"unece:ProcessTypeCodeList#106","@type":"unece:ProcessTypeCodeList","rdf:value":"106","rdfs:comment":"Chemical recycling"},{"@id":"unece:ProcessTypeCodeList#107","@type":"unece:ProcessTypeCodeList","rdf:value":"107","rdfs:comment":"Combing"},{"@id":"unece:ProcessTypeCodeList#108","@type":"unece:ProcessTypeCodeList","rdf:value":"108","rdfs:comment":"Agricultural cultivation"},{"@id":"unece:ProcessTypeCodeList#109","@type":"unece:ProcessTypeCodeList","rdf:value":"109","rdfs:comment":"Designing"},{"@id":"unece:ProcessTypeCodeList#110","@type":"unece:ProcessTypeCodeList","rdf:value":"110","rdfs:comment":"Disposing"},{"@id":"unece:ProcessTypeCodeList#111","@type":"unece:ProcessTypeCodeList","rdf:value":"111","rdfs:comment":"Extrusion"},{"@id":"unece:ProcessTypeCodeList#112","@type":"unece:ProcessTypeCodeList","rdf:value":"112","rdfs:comment":"Fatliquoring"},{"@id":"unece:ProcessTypeCodeList#113","@type":"unece:ProcessTypeCodeList","rdf:value":"113","rdfs:comment":"Product finishing"},{"@id":"unece:ProcessTypeCodeList#114","@type":"unece:ProcessTypeCodeList","rdf:value":"114","rdfs:comment":"Ginning"},{"@id":"unece:ProcessTypeCodeList#115","@type":"unece:ProcessTypeCodeList","rdf:value":"115","rdfs:comment":"Grading"},{"@id":"unece:ProcessTypeCodeList#116","@type":"unece:ProcessTypeCodeList","rdf:value":"116","rdfs:comment":"Hatching"},{"@id":"unece:ProcessTypeCodeList#117","@type":"unece:ProcessTypeCodeList","rdf:value":"117","rdfs:comment":"Marketing"},{"@id":"unece:ProcessTypeCodeList#118","@type":"unece:ProcessTypeCodeList","rdf:value":"118","rdfs:comment":"Mechanical recycling"},{"@id":"unece:ProcessTypeCodeList#119","@type":"unece:ProcessTypeCodeList","rdf:value":"119","rdfs:comment":"Polymerisation"},{"@id":"unece:ProcessTypeCodeList#120","@type":"unece:ProcessTypeCodeList","rdf:value":"120","rdfs:comment":"Pre-treatment"},{"@id":"unece:ProcessTypeCodeList#121","@type":"unece:ProcessTypeCodeList","rdf:value":"121","rdfs:comment":"Printing"},{"@id":"unece:ProcessTypeCodeList#122","@type":"unece:ProcessTypeCodeList","rdf:value":"122","rdfs:comment":"Pulp dissolving"},{"@id":"unece:ProcessTypeCodeList#123","@type":"unece:ProcessTypeCodeList","rdf:value":"123","rdfs:comment":"Quality checking"},{"@id":"unece:ProcessTypeCodeList#124","@type":"unece:ProcessTypeCodeList","rdf:value":"124","rdfs:comment":"Recycling"},{"@id":"unece:ProcessTypeCodeList#125","@type":"unece:ProcessTypeCodeList","rdf:value":"125","rdfs:comment":"Refining"},{"@id":"unece:ProcessTypeCodeList#126","@type":"unece:ProcessTypeCodeList","rdf:value":"126","rdfs:comment":"Retailing"},{"@id":"unece:ProcessTypeCodeList#127","@type":"unece:ProcessTypeCodeList","rdf:value":"127","rdfs:comment":"Retanning"},{"@id":"unece:ProcessTypeCodeList#128","@type":"unece:ProcessTypeCodeList","rdf:value":"128","rdfs:comment":"Retting"},{"@id":"unece:ProcessTypeCodeList#129","@type":"unece:ProcessTypeCodeList","rdf:value":"129","rdfs:comment":"Returns management"},{"@id":"unece:ProcessTypeCodeList#130","@type":"unece:ProcessTypeCodeList","rdf:value":"130","rdfs:comment":"Setting out leather"},{"@id":"unece:ProcessTypeCodeList#131","@type":"unece:ProcessTypeCodeList","rdf:value":"131","rdfs:comment":"Shaving hides"},{"@id":"unece:ProcessTypeCodeList#132","@type":"unece:ProcessTypeCodeList","rdf:value":"132","rdfs:comment":"Shearing"},{"@id":"unece:ProcessTypeCodeList#133","@type":"unece:ProcessTypeCodeList","rdf:value":"133","rdfs:comment":"Silk reeling"},{"@id":"unece:ProcessTypeCodeList#134","@type":"unece:ProcessTypeCodeList","rdf:value":"134","rdfs:comment":"Softening"},{"@id":"unece:ProcessTypeCodeList#135","@type":"unece:ProcessTypeCodeList","rdf:value":"135","rdfs:comment":"Sorting"},{"@id":"unece:ProcessTypeCodeList#136","@type":"unece:ProcessTypeCodeList","rdf:value":"136","rdfs:comment":"Spinning"},{"@id":"unece:ProcessTypeCodeList#137","@type":"unece:ProcessTypeCodeList","rdf:value":"137","rdfs:comment":"Splitting"},{"@id":"unece:ProcessTypeCodeList#138","@type":"unece:ProcessTypeCodeList","rdf:value":"138","rdfs:comment":"Tanning"},{"@id":"unece:ProcessTypeCodeList#139","@type":"unece:ProcessTypeCodeList","rdf:value":"139","rdfs:comment":"Thermo mechanical recycling"},{"@id":"unece:ProcessTypeCodeList#140","@type":"unece:ProcessTypeCodeList","rdf:value":"140","rdfs:comment":"Warehousing"},{"@id":"unece:ProcessTypeCodeList#141","@type":"unece:ProcessTypeCodeList","rdf:value":"141","rdfs:comment":"Weaving"},{"@id":"unece:ProcessTypeCodeList#ZZZ","@type":"unece:ProcessTypeCodeList","rdf:value":"ZZZ","rdfs:comment":"Mutually defined"},{"@id":"unece:HeaderTradeDelivery","@type":"rdfs:Class","rdfs:label":"HeaderTradeDelivery","schema:source":{"@id":"https://vocabulary.uncefact.org/HeaderTradeDelivery"},"rdfs:comment":"Shipping arrangements and movement of products and or services including despatch and delivery at a header level."},{"@id":"unece:LineTradeDelivery","@type":"rdfs:Class","rdfs:label":"LineTradeDelivery","schema:source":{"@id":"https://vocabulary.uncefact.org/LineTradeDelivery"},"rdfs:comment":"Shipping arrangements and movement of products and or services including despatch and delivery at a line level."},{"@id":"unece:TradeContact","@type":"rdfs:Class","rdfs:label":"TradeContact","schema:source":{"@id":"https://vocabulary.uncefact.org/TradeContact"},"rdfs:comment":"A person or a department that acts as a point of contact with another person or department in a trading relationship."},{"@id":"unece:SupplyChainTradeLineItem","@type":"rdfs:Class","rdfs:label":"SupplyChainTradeLineItem","schema:source":{"@id":"https://vocabulary.uncefact.org/SupplyChainTradeLineItem"},"rdfs:comment":"A collection of information specific to an item being used or reported on for supply chain trade purposes."},{"@id":"unece:AcknowledgementDocument","@type":"rdfs:Class","rdfs:label":"AcknowledgementDocument","schema:source":{"@id":"https://vocabulary.uncefact.org/AcknowledgementDocument"},"rdfs:comment":"A document exchanged between parties for a business application level acknowledgement of the receipt of information."},{"@id":"unece:TTAggregationEvent","@type":"rdfs:Class","rdfs:label":"TTAggregationEvent","schema:source":{"@id":"https://vocabulary.uncefact.org/TTAggregationEvent"},"rdfs:comment":"A Track and Trace (TT) event where objects or processes are grouped."},{"@id":"unece:TTObjectEvent","@type":"rdfs:Class","rdfs:label":"TTObjectEvent","schema:source":{"@id":"https://vocabulary.uncefact.org/TTObjectEvent"},"rdfs:comment":"Information about an event concerning one or more physical or digital Track and Trace (TT) objects identified by instance or class level identifiers."},{"@id":"unece:TTTransactionEvent","@type":"rdfs:Class","rdfs:label":"TTTransactionEvent","schema:source":{"@id":"https://vocabulary.uncefact.org/TTTransactionEvent"},"rdfs:comment":"Information about an event declaring that certain objects have been associated or disassociated with one or more Track and Trace (TT) trade transactions."},{"@id":"unece:SubordinateLineTradeDelivery","@type":"rdfs:Class","rdfs:label":"SubordinateLineTradeDelivery","schema:source":{"@id":"https://vocabulary.uncefact.org/SubordinateLineTradeDelivery"},"rdfs:comment":"Supply chain shipping arrangements and movement of products and or services including despatch and delivery."},{"@id":"unece:ProductInstance","@type":"rdfs:Class","rdfs:label":"ProductInstance","schema:source":{"@id":"https://vocabulary.uncefact.org/ProductInstance"},"rdfs:comment":"An individual trade product or batch of similar trade products produced by human or mechanical effort or by a natural process."},{"@id":"unece:SupplyPlan","@type":"rdfs:Class","rdfs:label":"SupplyPlan","schema:source":{"@id":"https://vocabulary.uncefact.org/SupplyPlan"},"rdfs:comment":"Specification of the delivery quantities and date/time values in a supply schedule."},{"@id":"unece:TradeProduct","@type":"rdfs:Class","rdfs:label":"TradeProduct","schema:source":{"@id":"https://vocabulary.uncefact.org/TradeProduct"},"rdfs:comment":"Any tangible output or service produced by human or mechanical effort or by a natural process for trade purposes."},{"@id":"unece:HeaderTradeAgreement","@type":"rdfs:Class","rdfs:label":"HeaderTradeAgreement","schema:source":{"@id":"https://vocabulary.uncefact.org/HeaderTradeAgreement"},"rdfs:comment":"The contractual terms of a header trade agreement."},{"@id":"unece:LineTradeAgreement","@type":"rdfs:Class","rdfs:label":"LineTradeAgreement","schema:source":{"@id":"https://vocabulary.uncefact.org/LineTradeAgreement"},"rdfs:comment":"The contractual terms of a line trade agreement."},{"@id":"unece:LineTradeSettlement","@type":"rdfs:Class","rdfs:label":"LineTradeSettlement","schema:source":{"@id":"https://vocabulary.uncefact.org/LineTradeSettlement"},"rdfs:comment":"The information, at a line level, that enables the reconciliation of a financial transaction with the item(s) that the financial transaction is intended to settle, for example a commercial invoice."},{"@id":"unece:SubordinateLineTradeAgreement","@type":"rdfs:Class","rdfs:label":"SubordinateLineTradeAgreement","schema:source":{"@id":"https://vocabulary.uncefact.org/SubordinateLineTradeAgreement"},"rdfs:comment":"The contractual terms of a subordinate line trade agreement."},{"@id":"unece:ProductionProcess","@type":"rdfs:Class","rdfs:label":"ProductionProcess","schema:source":{"@id":"https://vocabulary.uncefact.org/ProductionProcess"},"rdfs:comment":"A naturally occurring or designed sequence of operations or events in order to produce something."},{"@id":"unece:TradeAddress","@type":"rdfs:Class","rdfs:label":"TradeAddress","schema:source":{"@id":"https://vocabulary.uncefact.org/TradeAddress"},"rdfs:comment":"The location at which a particular trade related organization or person may be found or reached."},{"@id":"unece:TradeSettlementHeaderMonetarySummation","@type":"rdfs:Class","rdfs:label":"TradeSettlementHeaderMonetarySummation","schema:source":{"@id":"https://vocabulary.uncefact.org/TradeSettlementHeaderMonetarySummation"},"rdfs:comment":"A collection of monetary amount totals, specified at header level, for a trade settlement."},{"@id":"unece:TradeParty","@type":"rdfs:Class","rdfs:label":"TradeParty","schema:source":{"@id":"https://vocabulary.uncefact.org/TradeParty"},"rdfs:comment":"An individual, a group, or a body having a role in a trade business function."},{"@id":"unece:TradeTax","@type":"rdfs:Class","rdfs:label":"TradeTax","schema:source":{"@id":"https://vocabulary.uncefact.org/TradeTax"},"rdfs:comment":"A trade related fiscal levy or duty."},{"@id":"unece:TradeSettlementLineMonetarySummation","@type":"rdfs:Class","rdfs:label":"TradeSettlementLineMonetarySummation","schema:source":{"@id":"https://vocabulary.uncefact.org/TradeSettlementLineMonetarySummation"},"rdfs:comment":"A collection of monetary amount totals, specified at line level, for a trade settlement."},{"@id":"unece:SubordinateLineTradeSettlement","@type":"rdfs:Class","rdfs:label":"SubordinateLineTradeSettlement","schema:source":{"@id":"https://vocabulary.uncefact.org/SubordinateLineTradeSettlement"},"rdfs:comment":"The information, at a subordinate line level, that enables the reconciliation of a financial transaction with the item(s) that the financial transaction is intended to settle, for example a commercial invoice."},{"@id":"unece:ProductBatch","@type":"rdfs:Class","rdfs:label":"ProductBatch","schema:source":{"@id":"https://vocabulary.uncefact.org/ProductBatch"},"rdfs:comment":"A group of products considered or dealt with together."},{"@id":"unece:ProductionFacility","@type":"rdfs:Class","rdfs:label":"ProductionFacility","schema:source":{"@id":"https://vocabulary.uncefact.org/ProductionFacility"},"rdfs:comment":"A man made physical structure, such as a building, in which something is produced."},{"@id":"unece:SupplyChainTradeTransaction","@type":"rdfs:Class","rdfs:label":"SupplyChainTradeTransaction","schema:source":{"@id":"https://vocabulary.uncefact.org/SupplyChainTradeTransaction"},"rdfs:comment":"A group of supply chain trade line items, trade agreement, trade delivery and trade settlement details."},{"@id":"unece:LineTradeTransaction","@type":"rdfs:Class","rdfs:label":"LineTradeTransaction","schema:source":{"@id":"https://vocabulary.uncefact.org/LineTradeTransaction"},"rdfs:comment":"A group of trade line items, trade line agreement, trade line delivery and trade line settlement details."},{"@id":"unece:Colour","@type":"rdfs:Class","rdfs:label":"Colour","schema:source":{"@id":"https://vocabulary.uncefact.org/Colour"},"rdfs:comment":"A colour of a product."},{"@id":"unece:ProductionUnit","@type":"rdfs:Class","rdfs:label":"ProductionUnit","schema:source":{"@id":"https://vocabulary.uncefact.org/ProductionUnit"},"rdfs:comment":"A defined set of production processes under the single management of a facility."},{"@id":"unece:Print","@type":"rdfs:Class","rdfs:label":"Print","schema:source":{"@id":"https://vocabulary.uncefact.org/Print"},"rdfs:comment":"Any text or pattern put on the surface of a product using a specific material such as dye."},{"@id":"unece:ProductionDevice","@type":"rdfs:Class","rdfs:label":"ProductionDevice","schema:source":{"@id":"https://vocabulary.uncefact.org/ProductionDevice"},"rdfs:comment":"An object, especially a piece of mechanical or electronic equipment, made or adapted in order to perform a production activity."},{"@id":"unece:ProductFinishingTreatment","@type":"rdfs:Class","rdfs:label":"ProductFinishingTreatment","schema:source":{"@id":"https://vocabulary.uncefact.org/ProductFinishingTreatment"},"rdfs:comment":"Improving measures for manufactured components or products to meet end use requirements."},{"@id":"unece:ProductHandlingProcess","@type":"rdfs:Class","rdfs:label":"ProductHandlingProcess","schema:source":{"@id":"https://vocabulary.uncefact.org/ProductHandlingProcess"},"rdfs:comment":"A naturally occurring or designed sequence of operations or events that create, transform, or touch a product, such as manufacturing, treating, packaging, and storing."},{"@id":"unece:SubordinateTradeLineItem","@type":"rdfs:Class","rdfs:label":"SubordinateTradeLineItem","schema:source":{"@id":"https://vocabulary.uncefact.org/SubordinateTradeLineItem"},"rdfs:comment":"A collection of information specific to a subordinate item being used or reported on for trade purposes."},{"@id":"unece:ProductionCycle","@type":"rdfs:Class","rdfs:label":"ProductionCycle","schema:source":{"@id":"https://vocabulary.uncefact.org/ProductionCycle"},"rdfs:comment":"A series of activities associated with the processing of a product."},{"@id":"unece:SpecifiedChemicalTreatment","@type":"rdfs:Class","rdfs:label":"SpecifiedChemicalTreatment","schema:source":{"@id":"https://vocabulary.uncefact.org/SpecifiedChemicalTreatment"},"rdfs:comment":"Any substance such as dyestuffs, chrome oxide, acids, sulphate, surfactant or other chemicals applied to an agricultural field, substrate, plant, animal product, material or product."},{"@id":"unece:HeaderTradeSettlement","@type":"rdfs:Class","rdfs:label":"HeaderTradeSettlement","schema:source":{"@id":"https://vocabulary.uncefact.org/HeaderTradeSettlement"},"rdfs:comment":"The information, at a header level, that enables the reconciliation of a financial transaction, with the item(s) that the financial transaction is intended to settle, such as a commercial invoice."},{"@id":"unece:ProductLabel","@type":"rdfs:Class","rdfs:label":"ProductLabel","schema:source":{"@id":"https://vocabulary.uncefact.org/ProductLabel"},"rdfs:comment":"A label, such as a garment label or a radio frequency tag, used for identifying a product."},{"@id":"unece:Contract","@type":"rdfs:Class","rdfs:label":"Contract","schema:source":{"@id":"https://vocabulary.uncefact.org/Contract"},"rdfs:comment":"An agreement between two or more parties for trade purposes."},{"@id":"unece:SupplyChainInventory","@type":"rdfs:Class","rdfs:label":"SupplyChainInventory","schema:source":{"@id":"https://vocabulary.uncefact.org/SupplyChainInventory"},"rdfs:comment":"Supply chain goods and materials held in stock."},{"@id":"unece:TTTransformationEvent","@type":"rdfs:Class","rdfs:label":"TTTransformationEvent","schema:source":{"@id":"https://vocabulary.uncefact.org/TTTransformationEvent"},"rdfs:comment":"Information about an event that captures the relationship between one or more physical or digital objects identified by identifiers, such as an EPC (Electronic Product Code) or EPC class, that are fully or partially consumed as inputs or as outputs."},{"@id":"unece:Product","@type":"rdfs:Class","rdfs:label":"Product","schema:source":{"@id":"https://vocabulary.uncefact.org/Product"},"rdfs:comment":"A reference to a product or service produced by human or mechanical effort or by a natural process for trading purposes."},{"@id":"unece:TradeSettlementPayment","@type":"rdfs:Class","rdfs:label":"TradeSettlementPayment","schema:source":{"@id":"https://vocabulary.uncefact.org/TradeSettlementPayment"},"rdfs:comment":"The specific discharge obligations in respect of funds or securities transferred between two or more parties as part of a trade settlement."},{"@id":"unece:Machine","@type":"rdfs:Class","rdfs:label":"Machine","schema:source":{"@id":"https://vocabulary.uncefact.org/Machine"},"rdfs:comment":"An apparatus specified to be used to perform an activity to produce something."},{"@id":"unece:TradeLocation","@type":"rdfs:Class","rdfs:label":"TradeLocation","schema:source":{"@id":"https://vocabulary.uncefact.org/TradeLocation"},"rdfs:comment":"A physical location or place used or referenced for trade purposes."},{"@id":"unece:ForecastTerms","@type":"rdfs:Class","rdfs:label":"ForecastTerms","schema:source":{"@id":"https://vocabulary.uncefact.org/ForecastTerms"},"rdfs:comment":"A set of terms and conditions by which a supply chain forecast has been or will be made."},{"@id":"unece:TTExchangedDocument","@type":"rdfs:Class","rdfs:label":"TTExchangedDocument","schema:source":{"@id":"https://vocabulary.uncefact.org/TTExchangedDocument"},"rdfs:comment":"A collection of data for a piece of written, printed or electronic matter that is exchanged between two or more parties for Track and Trace (TT) purposes."},{"@id":"unece:TTLocation","@type":"rdfs:Class","rdfs:label":"TTLocation","schema:source":{"@id":"https://vocabulary.uncefact.org/TTLocation"},"rdfs:comment":"A physical place related to a Track and Trace (TT) process."},{"@id":"unece:TradeProductFeature","@type":"rdfs:Class","rdfs:label":"TradeProductFeature","schema:source":{"@id":"https://vocabulary.uncefact.org/TradeProductFeature"},"rdfs:comment":"Distinctive or characteristic parts of a trade product."},{"@id":"unece:TTAnimal","@type":"rdfs:Class","rdfs:label":"TTAnimal","schema:source":{"@id":"https://vocabulary.uncefact.org/TTAnimal"},"rdfs:comment":"A Track and Trace (TT) animal or a group of animals, such as those kept or raised on a farm, ranch."},{"@id":"unece:Marketplace","@type":"rdfs:Class","rdfs:label":"Marketplace","schema:source":{"@id":"https://vocabulary.uncefact.org/Marketplace"},"rdfs:comment":"An actual or virtual place where buyers and sellers interact, directly or through intermediaries, to trade goods or services."},{"@id":"unece:NegotiationContext","@type":"rdfs:Class","rdfs:label":"NegotiationContext","schema:source":{"@id":"https://vocabulary.uncefact.org/NegotiationContext"},"rdfs:comment":"The protocol and setting of a negotiation."},{"@id":"unece:ProductGroup","@type":"rdfs:Class","rdfs:label":"ProductGroup","schema:source":{"@id":"https://vocabulary.uncefact.org/ProductGroup"},"rdfs:comment":"A grouping of trade products."},{"@id":"unece:Production","@type":"rdfs:Class","rdfs:label":"Production","schema:source":{"@id":"https://vocabulary.uncefact.org/Production"},"rdfs:comment":"The making or manufacturing of goods, such as from components or raw materials."},{"@id":"unece:TTParty","@type":"rdfs:Class","rdfs:label":"TTParty","schema:source":{"@id":"https://vocabulary.uncefact.org/TTParty"},"rdfs:comment":"An individual, group, or body related to a Track and Trace (TT) process."},{"@id":"unece:TTTradeTransaction","@type":"rdfs:Class","rdfs:label":"TTTradeTransaction","schema:source":{"@id":"https://vocabulary.uncefact.org/TTTradeTransaction"},"rdfs:comment":"An agreement, contract, exchange, understanding, or transfer of cash or property related to a Track and Trace (TT) process."},{"@id":"unece:NegotiationExchange","@type":"rdfs:Class","rdfs:label":"NegotiationExchange","schema:source":{"@id":"https://vocabulary.uncefact.org/NegotiationExchange"},"rdfs:comment":"An offer exchanged between parties for an electronic negotiation."},{"@id":"unece:DeliverySchedule","@type":"rdfs:Class","rdfs:label":"DeliverySchedule","schema:source":{"@id":"https://vocabulary.uncefact.org/DeliverySchedule"},"rdfs:comment":"Specification of the forecasted delivery quantities and date/time values for a delivery schedule."},{"@id":"unece:ExchangedDeclaration","@type":"rdfs:Class","rdfs:label":"ExchangedDeclaration","schema:source":{"@id":"https://vocabulary.uncefact.org/ExchangedDeclaration"},"rdfs:comment":"A collection of data for a piece of written, printed or electronic matter that is exchanged between two parties as a formal declaration."},{"@id":"unece:Classification","@type":"rdfs:Class","rdfs:label":"Classification","schema:source":{"@id":"https://vocabulary.uncefact.org/Classification"},"rdfs:comment":"A systematic arrangement of products in classes or categories according to established criteria."},{"@id":"unece:DocumentLineDocument","@type":"rdfs:Class","rdfs:label":"DocumentLineDocument","schema:source":{"@id":"https://vocabulary.uncefact.org/DocumentLineDocument"},"rdfs:comment":"A collection of data for a line on a piece of written, printed or electronic matter that provides information or evidence."},{"@id":"unece:acceptanceEvent","@type":["rdf:Property","owl:ObjectProperty"],"rdfs:label":"acceptanceEvent","schema:rangeIncludes":{"@id":"unece:SupplyChainEvent"},"schema:domainIncludes":[{"@id":"unece:HeaderTradeDelivery"},{"@id":"unece:LineTradeDelivery"}],"rdfs:comment":"A significant occurrence or happening in a supply chain."},{"@id":"unece:actualDeliveryEvent","@type":["rdf:Property","owl:ObjectProperty"],"rdfs:label":"actualDeliveryEvent","schema:rangeIncludes":{"@id":"unece:SupplyChainEvent"},"schema:domainIncludes":[{"@id":"unece:HeaderTradeDelivery"},{"@id":"unece:LineTradeDelivery"},{"@id":"unece:SubordinateLineTradeDelivery"}],"rdfs:comment":"A significant occurrence or happening in a supply chain."},{"@id":"unece:actualDespatchEvent","@type":["rdf:Property","owl:ObjectProperty"],"rdfs:label":"actualDespatchEvent","schema:rangeIncludes":{"@id":"unece:SupplyChainEvent"},"schema:domainIncludes":[{"@id":"unece:HeaderTradeDelivery"},{"@id":"unece:LineTradeDelivery"}],"rdfs:comment":"A significant occurrence or happening in a supply chain."},{"@id":"unece:actualLoadingEvent","@type":["rdf:Property","owl:ObjectProperty"],"rdfs:label":"actualLoadingEvent","schema:rangeIncludes":{"@id":"unece:SupplyChainEvent"},"schema:domainIncludes":[{"@id":"unece:HeaderTradeDelivery"},{"@id":"unece:LineTradeDelivery"}],"rdfs:comment":"A significant occurrence or happening in a supply chain."},{"@id":"unece:actualPickUpEvent","@type":["rdf:Property","owl:ObjectProperty"],"rdfs:label":"actualPickUpEvent","schema:rangeIncludes":{"@id":"unece:SupplyChainEvent"},"schema:domainIncludes":[{"@id":"unece:HeaderTradeDelivery"},{"@id":"unece:LineTradeDelivery"}],"rdfs:comment":"A significant occurrence or happening in a supply chain."},{"@id":"unece:actualReceiptEvent","@type":["rdf:Property","owl:ObjectProperty"],"rdfs:label":"actualReceiptEvent","schema:rangeIncludes":{"@id":"unece:SupplyChainEvent"},"schema:domainIncludes":[{"@id":"unece:HeaderTradeDelivery"},{"@id":"unece:LineTradeDelivery"}],"rdfs:comment":"A significant occurrence or happening in a supply chain."},{"@id":"unece:actualUnloadingEvent","@type":["rdf:Property","owl:ObjectProperty"],"rdfs:label":"actualUnloadingEvent","schema:rangeIncludes":{"@id":"unece:SupplyChainEvent"},"schema:domainIncludes":[{"@id":"unece:HeaderTradeDelivery"},{"@id":"unece:LineTradeDelivery"}],"rdfs:comment":"A significant occurrence or happening in a supply chain."},{"@id":"unece:additionalDocument","@type":["rdf:Property","owl:ObjectProperty"],"rdfs:label":"additionalDocument","schema:rangeIncludes":{"@id":"unece:Document"},"schema:domainIncludes":[{"@id":"unece:HeaderTradeDelivery"},{"@id":"unece:LineTradeDelivery"},{"@id":"unece:HeaderTradeAgreement"},{"@id":"unece:LineTradeAgreement"},{"@id":"unece:LineTradeSettlement"},{"@id":"unece:SubordinateLineTradeAgreement"}],"rdfs:comment":"Written, printed or electronic matter that is referenced."},{"@id":"unece:agreedQuantity","@type":["rdf:Property","owl:ObjectProperty"],"rdfs:label":"agreedQuantity","schema:rangeIncludes":{"@id":"unece:QuantityType"},"schema:domainIncludes":[{"@id":"unece:HeaderTradeDelivery"},{"@id":"unece:LineTradeDelivery"}],"rdfs:comment":""},{"@id":"unece:buyerOrderDateTime","@type":["rdf:Property","owl:DatatypeProperty"],"rdfs:label":"buyerOrderDateTime","schema:rangeIncludes":{"@id":"schema:DateTime"},"schema:domainIncludes":[{"@id":"unece:HeaderTradeDelivery"},{"@id":"unece:LineTradeDelivery"}],"rdfs:comment":"The date, time, date time, or other date time value, at header level, for the buyer order for this trade delivery."},{"@id":"unece:classificationDocument","@type":["rdf:Property","owl:ObjectProperty"],"rdfs:label":"classificationDocument","schema:rangeIncludes":{"@id":"unece:Document"},"schema:domainIncludes":[{"@id":"unece:HeaderTradeDelivery"},{"@id":"unece:LineTradeDelivery"},{"@id":"unece:Consignment"},{"@id":"unece:ConsignmentItem"}],"rdfs:comment":"Written, printed or electronic matter that is referenced."},{"@id":"unece:confirmedDespatchEvent","@type":["rdf:Property","owl:ObjectProperty"],"rdfs:label":"confirmedDespatchEvent","schema:rangeIncludes":{"@id":"unece:SupplyChainEvent"},"schema:domainIncludes":[{"@id":"unece:HeaderTradeDelivery"},{"@id":"unece:LineTradeDelivery"}],"rdfs:comment":"A significant occurrence or happening in a supply chain."},{"@id":"unece:confirmedPickUpEvent","@type":["rdf:Property","owl:ObjectProperty"],"rdfs:label":"confirmedPickUpEvent","schema:rangeIncludes":{"@id":"unece:SupplyChainEvent"},"schema:domainIncludes":[{"@id":"unece:HeaderTradeDelivery"},{"@id":"unece:LineTradeDelivery"}],"rdfs:comment":"A significant occurrence or happening in a supply chain."},{"@id":"unece:confirmedReleaseEvent","@type":["rdf:Property","owl:ObjectProperty"],"rdfs:label":"confirmedReleaseEvent","schema:rangeIncludes":{"@id":"unece:SupplyChainEvent"},"schema:domainIncludes":[{"@id":"unece:HeaderTradeDelivery"},{"@id":"unece:LineTradeDelivery"}],"rdfs:comment":"A significant occurrence or happening in a supply chain."},{"@id":"unece:consumptionReportDocument","@type":["rdf:Property","owl:ObjectProperty"],"rdfs:label":"consumptionReportDocument","schema:rangeIncludes":{"@id":"unece:Document"},"schema:domainIncludes":[{"@id":"unece:HeaderTradeDelivery"},{"@id":"unece:LineTradeDelivery"}],"rdfs:comment":"Written, printed or electronic matter that is referenced."},{"@id":"unece:deliveryNoteDocument","@type":["rdf:Property","owl:ObjectProperty"],"rdfs:label":"deliveryNoteDocument","schema:rangeIncludes":{"@id":"unece:Document"},"schema:domainIncludes":[{"@id":"unece:HeaderTradeDelivery"},{"@id":"unece:LineTradeDelivery"},{"@id":"unece:SupplyPlan"}],"rdfs:comment":"Written, printed or electronic matter that is referenced."},{"@id":"unece:despatchAdviceDocument","@type":["rdf:Property","owl:ObjectProperty"],"rdfs:label":"despatchAdviceDocument","schema:rangeIncludes":{"@id":"unece:Document"},"schema:domainIncludes":[{"@id":"unece:HeaderTradeDelivery"},{"@id":"unece:LineTradeDelivery"}],"rdfs:comment":"Written, printed or electronic matter that is referenced."},{"@id":"unece:despatchedQuantity","@type":["rdf:Property","owl:ObjectProperty"],"rdfs:label":"despatchedQuantity","schema:rangeIncludes":{"@id":"unece:QuantityType"},"schema:domainIncludes":[{"@id":"unece:HeaderTradeDelivery"},{"@id":"unece:LineTradeDelivery"}],"rdfs:comment":""},{"@id":"unece:disposalParty","@type":["rdf:Property","owl:ObjectProperty"],"rdfs:label":"disposalParty","schema:rangeIncludes":{"@id":"unece:TradeParty"},"schema:domainIncludes":[{"@id":"unece:HeaderTradeDelivery"},{"@id":"unece:LineTradeDelivery"}],"rdfs:comment":"A disposal party, at header level, for this trade delivery."},{"@id":"unece:dueInAvailableQuantity","@type":["rdf:Property","owl:ObjectProperty"],"rdfs:label":"dueInAvailableQuantity","schema:rangeIncludes":{"@id":"unece:QuantityType"},"schema:domainIncludes":[{"@id":"unece:HeaderTradeDelivery"},{"@id":"unece:LineTradeDelivery"}],"rdfs:comment":""},{"@id":"unece:dueInForecastedQuantity","@type":["rdf:Property","owl:ObjectProperty"],"rdfs:label":"dueInForecastedQuantity","schema:rangeIncludes":{"@id":"unece:QuantityType"},"schema:domainIncludes":[{"@id":"unece:HeaderTradeDelivery"},{"@id":"unece:LineTradeDelivery"}],"rdfs:comment":""},{"@id":"unece:dueInRequestedQuantity","@type":["rdf:Property","owl:ObjectProperty"],"rdfs:label":"dueInRequestedQuantity","schema:rangeIncludes":{"@id":"unece:QuantityType"},"schema:domainIncludes":[{"@id":"unece:HeaderTradeDelivery"},{"@id":"unece:LineTradeDelivery"}],"rdfs:comment":""},{"@id":"unece:estimatedDeliveryEvent","@type":["rdf:Property","owl:ObjectProperty"],"rdfs:label":"estimatedDeliveryEvent","schema:rangeIncludes":{"@id":"unece:SupplyChainEvent"},"schema:domainIncludes":{"@id":"unece:HeaderTradeDelivery"},"rdfs:comment":"A significant occurrence or happening in a supply chain."},{"@id":"unece:finalDeliveryIndicator","@type":["rdf:Property","owl:DatatypeProperty"],"rdfs:label":"finalDeliveryIndicator","schema:rangeIncludes":{"@id":"schema:Boolean"},"schema:domainIncludes":[{"@id":"unece:HeaderTradeDelivery"},{"@id":"unece:LineTradeDelivery"}],"rdfs:comment":"The indication, at header level, of whether or not this trade delivery is the final delivery."},{"@id":"unece:finalDestinationCountry","@type":["rdf:Property","owl:ObjectProperty"],"rdfs:label":"finalDestinationCountry","schema:rangeIncludes":{"@id":"unece:Country"},"schema:domainIncludes":[{"@id":"unece:HeaderTradeDelivery"},{"@id":"unece:LineTradeDelivery"},{"@id":"unece:Consignment"}],"rdfs:comment":"The area of land that belongs to a nation together with its properties, such as population, political organization, etc., used or referenced for trade purposes."},{"@id":"unece:freightForwarderParty","@type":["rdf:Property","owl:ObjectProperty"],"rdfs:label":"freightForwarderParty","schema:rangeIncludes":{"@id":"unece:TradeParty"},"schema:domainIncludes":[{"@id":"unece:HeaderTradeDelivery"},{"@id":"unece:Consignment"}],"rdfs:comment":"A freight forwarder party, at header level, for this trade delivery."},{"@id":"unece:fullyDeliveredIndicator","@type":["rdf:Property","owl:DatatypeProperty"],"rdfs:label":"fullyDeliveredIndicator","schema:rangeIncludes":{"@id":"schema:Boolean"},"schema:domainIncludes":[{"@id":"unece:HeaderTradeDelivery"},{"@id":"unece:LineTradeDelivery"}],"rdfs:comment":"The indication, at header level, of whether or not this trade delivery is fully delivered."},{"@id":"unece:globalId","@type":["rdf:Property","owl:DatatypeProperty"],"rdfs:label":"globalId","schema:rangeIncludes":{"@id":"schema:Text"},"schema:domainIncludes":[{"@id":"unece:HeaderTradeDelivery"},{"@id":"unece:TradeProduct"},{"@id":"unece:TradeParty"},{"@id":"unece:ProductBatch"},{"@id":"unece:ProductionFacility"},{"@id":"unece:ProductionUnit"},{"@id":"unece:Product"},{"@id":"unece:Document"},{"@id":"unece:ExchangedDocument"},{"@id":"unece:Location"},{"@id":"unece:Package"},{"@id":"unece:Consignment"},{"@id":"unece:ConsignmentItem"}],"rdfs:comment":"A global identifier for this supply chain consignment item."},{"@id":"unece:goodsOwnershipChangeDateTime","@type":["rdf:Property","owl:DatatypeProperty"],"rdfs:label":"goodsOwnershipChangeDateTime","schema:rangeIncludes":{"@id":"schema:DateTime"},"schema:domainIncludes":[{"@id":"unece:HeaderTradeDelivery"},{"@id":"unece:LineTradeDelivery"}],"rdfs:comment":"The date, time, date time, or other date time value for the goods ownership change, at line level, for this trade delivery."},{"@id":"unece:goodsReceiptNoteDocument","@type":["rdf:Property","owl:ObjectProperty"],"rdfs:label":"goodsReceiptNoteDocument","schema:rangeIncludes":{"@id":"unece:Document"},"schema:domainIncludes":[{"@id":"unece:HeaderTradeDelivery"},{"@id":"unece:LineTradeDelivery"}],"rdfs:comment":"Written, printed or electronic matter that is referenced."},{"@id":"unece:headerTradeDeliveryGoodsPhysicalStateDescription","@type":["rdf:Property","owl:DatatypeProperty"],"rdfs:label":"headerTradeDeliveryGoodsPhysicalStateDescription","schema:rangeIncludes":{"@id":"schema:Text"},"schema:domainIncludes":{"@id":"unece:HeaderTradeDelivery"},"rdfs:comment":"A textual description for the physical state of the goods, at header level, for this trade delivery."},{"@id":"unece:headerTradeDeliveryGoodsPhysicalStateDescriptionCode","@type":["rdf:Property","owl:DatatypeProperty"],"rdfs:label":"headerTradeDeliveryGoodsPhysicalStateDescriptionCode","schema:rangeIncludes":{"@id":"schema:Text"},"schema:domainIncludes":{"@id":"unece:HeaderTradeDelivery"},"rdfs:comment":"The code specifying a description for the physical state of the goods, at header level, for this trade delivery."},{"@id":"unece:headerTradeDeliveryGoodsPhysicalStateType","@type":["rdf:Property","owl:DatatypeProperty"],"rdfs:label":"headerTradeDeliveryGoodsPhysicalStateType","schema:rangeIncludes":{"@id":"schema:Text"},"schema:domainIncludes":{"@id":"unece:HeaderTradeDelivery"},"rdfs:comment":"A type, expressed as text, for the physical state of the goods, at header level, for this trade delivery."},{"@id":"unece:headerTradeDeliveryGoodsPhysicalStateTypeCode","@type":["rdf:Property","owl:DatatypeProperty"],"rdfs:label":"headerTradeDeliveryGoodsPhysicalStateTypeCode","schema:rangeIncludes":{"@id":"schema:Text"},"schema:domainIncludes":{"@id":"unece:HeaderTradeDelivery"},"rdfs:comment":"The code specifying the type of physical state of the goods, at header level, for this trade delivery."},{"@id":"unece:identifier","@type":["rdf:Property","owl:DatatypeProperty"],"rdfs:label":"identifier","schema:rangeIncludes":{"@id":"schema:Text"},"schema:domainIncludes":[{"@id":"unece:HeaderTradeDelivery"},{"@id":"unece:LineTradeDelivery"},{"@id":"unece:TradeContact"},{"@id":"unece:SupplyChainTradeLineItem"},{"@id":"unece:AcknowledgementDocument"},{"@id":"unece:TTAggregationEvent"},{"@id":"unece:TTObjectEvent"},{"@id":"unece:TTTransactionEvent"},{"@id":"unece:ProductInstance"},{"@id":"unece:TradeProduct"},{"@id":"unece:HeaderTradeAgreement"},{"@id":"unece:LineTradeAgreement"},{"@id":"unece:ProductionProcess"},{"@id":"unece:TradeAddress"},{"@id":"unece:TradeParty"},{"@id":"unece:TradeTax"},{"@id":"unece:ProductBatch"},{"@id":"unece:ProductionFacility"},{"@id":"unece:SupplyChainTradeTransaction"},{"@id":"unece:Colour"},{"@id":"unece:ProductionUnit"},{"@id":"unece:Print"},{"@id":"unece:ProductionDevice"},{"@id":"unece:ProductFinishingTreatment"},{"@id":"unece:SubordinateTradeLineItem"},{"@id":"unece:ProductionCycle"},{"@id":"unece:SpecifiedChemicalTreatment"},{"@id":"unece:ProductLabel"},{"@id":"unece:Contract"},{"@id":"unece:TTTransformationEvent"},{"@id":"unece:Product"},{"@id":"unece:Machine"},{"@id":"unece:TradeLocation"},{"@id":"unece:TTExchangedDocument"},{"@id":"unece:TTLocation"},{"@id":"unece:TradeProductFeature"},{"@id":"unece:Marketplace"},{"@id":"unece:NegotiationContext"},{"@id":"unece:ProductGroup"},{"@id":"unece:Production"},{"@id":"unece:TTParty"},{"@id":"unece:TTTradeTransaction"},{"@id":"unece:ExchangedDeclaration"},{"@id":"unece:DocumentLineDocument"},{"@id":"unece:Document"},{"@id":"unece:ExchangedDocument"},{"@id":"unece:BinaryFile"},{"@id":"unece:GeographicalCoordinate"},{"@id":"unece:CountrySubDivision"},{"@id":"unece:QuantityAnalysis"},{"@id":"unece:Picture"},{"@id":"unece:SpecifiedMethod"},{"@id":"unece:Location"},{"@id":"unece:CommunicationEvent"},{"@id":"unece:GeographicalGrid"},{"@id":"unece:LegalOrganization"},{"@id":"unece:Object"},{"@id":"unece:GeographicalFeature"},{"@id":"unece:SpecifiedPeriod"},{"@id":"unece:WorkItemDimension"},{"@id":"unece:Project"},{"@id":"unece:Note"},{"@id":"unece:Response"},{"@id":"unece:SpecialQuery"},{"@id":"unece:SpecifiedNote"},{"@id":"unece:MetricCharacteristic"},{"@id":"unece:LegalRegistration"},{"@id":"unece:DocumentCharacteristic"},{"@id":"unece:GeographicalObjectCharacteristic"},{"@id":"unece:Membership"},{"@id":"unece:Schedule"},{"@id":"unece:SpatialDimension"},{"@id":"unece:SpecifiedParameter"},{"@id":"unece:ProprietaryIdentity"},{"@id":"unece:CoordinateReferenceSystem"},{"@id":"unece:CoordinateSourceSystem"},{"@id":"unece:DocumentContextParameter"},{"@id":"unece:EmployerIdentity"},{"@id":"unece:GeopoliticalRegion"},{"@id":"unece:Issue"},{"@id":"unece:Radionuclide"},{"@id":"unece:Section"},{"@id":"unece:Segment"},{"@id":"unece:SubordinateLocation"},{"@id":"unece:SubordinateSubordinateLocation"},{"@id":"unece:Version"},{"@id":"unece:WorkflowObject"},{"@id":"unece:Party"},{"@id":"unece:Authentication"},{"@id":"unece:Clause"},{"@id":"unece:Address"},{"@id":"unece:Event"},{"@id":"unece:SpecificationQuery"},{"@id":"unece:Person"},{"@id":"unece:PaymentFinancialAccount"},{"@id":"unece:AccountingAccount"},{"@id":"unece:Cheque"},{"@id":"unece:DigitalMethod"},{"@id":"unece:FinancialCard"},{"@id":"unece:PaymentFinancialInstitution"},{"@id":"unece:BreakdownStatement"},{"@id":"unece:HeaderBalanceOut"},{"@id":"unece:PaymentBalanceOut"},{"@id":"unece:BranchFinancialInstitution"},{"@id":"unece:RequestingParty"},{"@id":"unece:BasicWorkItem"},{"@id":"unece:GroupedWorkItem"},{"@id":"unece:Tax"},{"@id":"unece:Voucher"},{"@id":"unece:TradeAllowanceCharge"},{"@id":"unece:InspectionReference"},{"@id":"unece:LaboratoryObservationReference"},{"@id":"unece:Accreditation"},{"@id":"unece:OrganizationalCertificate"},{"@id":"unece:ProcessCertificate"},{"@id":"unece:ProductBatchCertificate"},{"@id":"unece:ProductCertificate"},{"@id":"unece:SpecifiedCertificate"},{"@id":"unece:ObservationResult"},{"@id":"unece:Standard"},{"@id":"unece:ProcessWorkItem"},{"@id":"unece:ProductCharacteristic"},{"@id":"unece:InspectionResult"},{"@id":"unece:ProductBatchCharacteristic"},{"@id":"unece:Chemical"},{"@id":"unece:SustainabilityCharacteristic"},{"@id":"unece:SustainabilityInspection"},{"@id":"unece:Observation"},{"@id":"unece:Assertion"},{"@id":"unece:Policy"},{"@id":"unece:ProcessCharacteristic"},{"@id":"unece:TechnicalCharacteristic"},{"@id":"unece:SpecifiedCertification"},{"@id":"unece:Licence"},{"@id":"unece:SpecifiedDeclaration"},{"@id":"unece:TaxRegistration"},{"@id":"unece:SpecifiedInspection"},{"@id":"unece:Source"},{"@id":"unece:GovernmentRegistration"},{"@id":"unece:ConformanceCertificate"},{"@id":"unece:LaboratoryObservationAnalysisMethod"},{"@id":"unece:ControlSettingParameter"},{"@id":"unece:OperationalParameter"},{"@id":"unece:LaboratoryObservationContact"},{"@id":"unece:InspectionInstructions"},{"@id":"unece:LaboratoryObservationInstructions"},{"@id":"unece:ObservationObjectiveParameter"},{"@id":"unece:CalibratedMeasurement"},{"@id":"unece:CorrectiveEvent"},{"@id":"unece:LaboratoryObservationParty"},{"@id":"unece:OrganizationCharacteristic"},{"@id":"unece:SpecifiedMaterial"},{"@id":"unece:Seal"},{"@id":"unece:GuestPerson"},{"@id":"unece:ExperienceItem"},{"@id":"unece:ExperienceProduct"},{"@id":"unece:ExperienceEvent"},{"@id":"unece:ExperienceFacility"},{"@id":"unece:AgriculturalCertificate"},{"@id":"unece:Area"},{"@id":"unece:Plot"},{"@id":"unece:AnimalCertificate"},{"@id":"unece:CropProtectionTreatment"},{"@id":"unece:AgriculturalApplication"},{"@id":"unece:CropProduceBatch"},{"@id":"unece:IndividualTTAnimal"},{"@id":"unece:AnimalBatch"},{"@id":"unece:Produce"},{"@id":"unece:AgriculturalCharacteristic"},{"@id":"unece:AnimalIdentity"},{"@id":"unece:LogisticsTransportEquipment"},{"@id":"unece:TransportEvent"},{"@id":"unece:Service"},{"@id":"unece:Package"},{"@id":"unece:TransportMovement"},{"@id":"unece:AssociatedTransportEquipment"},{"@id":"unece:LogisticsTransportMeans"},{"@id":"unece:Consignment"},{"@id":"unece:ConsignmentItem"},{"@id":"unece:LogisticsPackaging"},{"@id":"unece:HandlingInstructions"},{"@id":"unece:LogisticsLocation"},{"@id":"unece:IOTDevice"},{"@id":"unece:TransportPerson"},{"@id":"unece:AttachedTransportEquipment"},{"@id":"unece:TransportRoute"},{"@id":"unece:TransportMeans"},{"@id":"unece:LogisticsLabel"},{"@id":"unece:TransportServiceLocation"},{"@id":"unece:Sensor"},{"@id":"unece:LocationParty"},{"@id":"unece:SupplyChainReference"},{"@id":"unece:SupplyChainEvent"},{"@id":"unece:Equipment"}],"rdfs:comment":"A proprietary identifier."},{"@id":"unece:includedPackaging","@type":["rdf:Property","owl:ObjectProperty"],"rdfs:label":"includedPackaging","schema:rangeIncludes":{"@id":"unece:SupplyChainPackaging"},"schema:domainIncludes":[{"@id":"unece:HeaderTradeDelivery"},{"@id":"unece:LineTradeDelivery"},{"@id":"unece:SubordinateLineTradeDelivery"}],"rdfs:comment":"Any material with which supply chain goods are packaged, such as a box or bubble wrap."},{"@id":"unece:informationNote","@type":["rdf:Property","owl:ObjectProperty"],"rdfs:label":"informationNote","schema:rangeIncludes":{"@id":"unece:Note"},"schema:domainIncludes":[{"@id":"unece:HeaderTradeDelivery"},{"@id":"unece:LineTradeDelivery"},{"@id":"unece:TradeProduct"}],"rdfs:comment":"A textual or coded description, such as a remark or additional information."},{"@id":"unece:inventoryManagerParty","@type":["rdf:Property","owl:ObjectProperty"],"rdfs:label":"inventoryManagerParty","schema:rangeIncludes":{"@id":"unece:TradeParty"},"schema:domainIncludes":[{"@id":"unece:HeaderTradeDelivery"},{"@id":"unece:LineTradeDelivery"}],"rdfs:comment":"An inventory manager party, at header level, for this trade delivery."},{"@id":"unece:modificationForecastedQuantity","@type":["rdf:Property","owl:ObjectProperty"],"rdfs:label":"modificationForecastedQuantity","schema:rangeIncludes":{"@id":"unece:QuantityType"},"schema:domainIncludes":[{"@id":"unece:HeaderTradeDelivery"},{"@id":"unece:LineTradeDelivery"}],"rdfs:comment":""},{"@id":"unece:overDeliveryAllowedIndicator","@type":["rdf:Property","owl:DatatypeProperty"],"rdfs:label":"overDeliveryAllowedIndicator","schema:rangeIncludes":{"@id":"schema:Boolean"},"schema:domainIncludes":[{"@id":"unece:HeaderTradeDelivery"},{"@id":"unece:LineTradeDelivery"}],"rdfs:comment":"The indication, at header level, of whether or not over delivery is allowed for this trade delivery."},{"@id":"unece:packingListDocument","@type":["rdf:Property","owl:ObjectProperty"],"rdfs:label":"packingListDocument","schema:rangeIncludes":{"@id":"unece:Document"},"schema:domainIncludes":[{"@id":"unece:HeaderTradeDelivery"},{"@id":"unece:LineTradeDelivery"}],"rdfs:comment":"Written, printed or electronic matter that is referenced."},{"@id":"unece:partialDeliveryAllowedIndicator","@type":["rdf:Property","owl:DatatypeProperty"],"rdfs:label":"partialDeliveryAllowedIndicator","schema:rangeIncludes":{"@id":"schema:Boolean"},"schema:domainIncludes":[{"@id":"unece:HeaderTradeDelivery"},{"@id":"unece:LineTradeDelivery"},{"@id":"unece:DeliveryTerms"}],"rdfs:comment":"The indication of whether or not these trade delivery terms allow a partial delivery."},{"@id":"unece:pickUpAvailabilityDateTime","@type":["rdf:Property","owl:DatatypeProperty"],"rdfs:label":"pickUpAvailabilityDateTime","schema:rangeIncludes":{"@id":"schema:Text"},"schema:domainIncludes":[{"@id":"unece:HeaderTradeDelivery"},{"@id":"unece:LineTradeDelivery"}],"rdfs:comment":"The formatted date, time, date time, or other date time value, at header level, when this trade delivery is available for pick-up."},{"@id":"unece:plannedConsignment","@type":["rdf:Property","owl:ObjectProperty"],"rdfs:label":"plannedConsignment","schema:rangeIncludes":{"@id":"unece:Consignment"},"schema:domainIncludes":[{"@id":"unece:HeaderTradeDelivery"},{"@id":"unece:LineTradeDelivery"}],"rdfs:comment":"A separately identifiable collection of goods items to be transported or available to be transported from one consignor to one consignee in a supply chain via one or more modes of transport where each consignment is the subject of one single transport contract.,A referenced, separately identifiable collection of goods items to be transported or available to be transported from one consignor to one consignee via one or more modes of transport where each consignment is the subject of one single transport contract."},{"@id":"unece:plannedDeliveryEvent","@type":["rdf:Property","owl:ObjectProperty"],"rdfs:label":"plannedDeliveryEvent","schema:rangeIncludes":{"@id":"unece:SupplyChainEvent"},"schema:domainIncludes":[{"@id":"unece:HeaderTradeDelivery"},{"@id":"unece:LineTradeDelivery"}],"rdfs:comment":"A significant occurrence or happening in a supply chain."},{"@id":"unece:plannedDespatchEvent","@type":["rdf:Property","owl:ObjectProperty"],"rdfs:label":"plannedDespatchEvent","schema:rangeIncludes":{"@id":"unece:SupplyChainEvent"},"schema:domainIncludes":[{"@id":"unece:HeaderTradeDelivery"},{"@id":"unece:LineTradeDelivery"}],"rdfs:comment":"A significant occurrence or happening in a supply chain."},{"@id":"unece:plannedPickUpEvent","@type":["rdf:Property","owl:ObjectProperty"],"rdfs:label":"plannedPickUpEvent","schema:rangeIncludes":{"@id":"unece:SupplyChainEvent"},"schema:domainIncludes":[{"@id":"unece:HeaderTradeDelivery"},{"@id":"unece:LineTradeDelivery"}],"rdfs:comment":"A significant occurrence or happening in a supply chain."},{"@id":"unece:plannedReleaseEvent","@type":["rdf:Property","owl:ObjectProperty"],"rdfs:label":"plannedReleaseEvent","schema:rangeIncludes":{"@id":"unece:SupplyChainEvent"},"schema:domainIncludes":{"@id":"unece:HeaderTradeDelivery"},"rdfs:comment":"A significant occurrence or happening in a supply chain."},{"@id":"unece:plannedShipFromDeliveryEvent","@type":["rdf:Property","owl:ObjectProperty"],"rdfs:label":"plannedShipFromDeliveryEvent","schema:rangeIncludes":{"@id":"unece:SupplyChainEvent"},"schema:domainIncludes":{"@id":"unece:HeaderTradeDelivery"},"rdfs:comment":"A significant occurrence or happening in a supply chain."},{"@id":"unece:plannedShipToDeliveryEvent","@type":["rdf:Property","owl:ObjectProperty"],"rdfs:label":"plannedShipToDeliveryEvent","schema:rangeIncludes":{"@id":"unece:SupplyChainEvent"},"schema:domainIncludes":[{"@id":"unece:HeaderTradeDelivery"},{"@id":"unece:LineTradeDelivery"}],"rdfs:comment":"A significant occurrence or happening in a supply chain."},{"@id":"unece:previousDeliverySupplyChainEvent","@type":["rdf:Property","owl:ObjectProperty"],"rdfs:label":"previousDeliverySupplyChainEvent","schema:rangeIncludes":{"@id":"unece:SupplyChainEvent"},"schema:domainIncludes":{"@id":"unece:HeaderTradeDelivery"},"rdfs:comment":"A significant occurrence or happening in a supply chain."},{"@id":"unece:quantityCalculationMethodCode","@type":["rdf:Property","owl:DatatypeProperty"],"rdfs:label":"quantityCalculationMethodCode","schema:rangeIncludes":{"@id":"schema:Text"},"schema:domainIncludes":[{"@id":"unece:HeaderTradeDelivery"},{"@id":"unece:LineTradeDelivery"}],"rdfs:comment":"The code specifying the quantity calculation method of this header trade delivery."},{"@id":"unece:receivingAdviceDocument","@type":["rdf:Property","owl:ObjectProperty"],"rdfs:label":"receivingAdviceDocument","schema:rangeIncludes":{"@id":"unece:Document"},"schema:domainIncludes":[{"@id":"unece:HeaderTradeDelivery"},{"@id":"unece:LineTradeDelivery"}],"rdfs:comment":"Written, printed or electronic matter that is referenced."},{"@id":"unece:relatedConsignment","@type":["rdf:Property","owl:ObjectProperty"],"rdfs:label":"relatedConsignment","schema:rangeIncludes":{"@id":"unece:Consignment"},"schema:domainIncludes":[{"@id":"unece:HeaderTradeDelivery"},{"@id":"unece:LineTradeDelivery"}],"rdfs:comment":"A separately identifiable collection of goods items to be transported or available to be transported from one consignor to one consignee in a supply chain via one or more modes of transport where each consignment is the subject of one single transport contract.,A referenced, separately identifiable collection of goods items to be transported or available to be transported from one consignor to one consignee via one or more modes of transport where each consignment is the subject of one single transport contract."},{"@id":"unece:relatedParty","@type":["rdf:Property","owl:ObjectProperty"],"rdfs:label":"relatedParty","schema:rangeIncludes":{"@id":"unece:TradeParty"},"schema:domainIncludes":[{"@id":"unece:HeaderTradeDelivery"},{"@id":"unece:Colour"},{"@id":"unece:ProductionUnit"},{"@id":"unece:Print"}],"rdfs:comment":"A trade party related to this facility production unit."},{"@id":"unece:remainingRequestedQuantity","@type":["rdf:Property","owl:ObjectProperty"],"rdfs:label":"remainingRequestedQuantity","schema:rangeIncludes":{"@id":"unece:QuantityType"},"schema:domainIncludes":[{"@id":"unece:HeaderTradeDelivery"},{"@id":"unece:LineTradeDelivery"}],"rdfs:comment":""},{"@id":"unece:requestedDeliveryEvent","@type":["rdf:Property","owl:ObjectProperty"],"rdfs:label":"requestedDeliveryEvent","schema:rangeIncludes":{"@id":"unece:SupplyChainEvent"},"schema:domainIncludes":[{"@id":"unece:HeaderTradeDelivery"},{"@id":"unece:LineTradeDelivery"}],"rdfs:comment":"A significant occurrence or happening in a supply chain."},{"@id":"unece:requestedDespatchEvent","@type":["rdf:Property","owl:ObjectProperty"],"rdfs:label":"requestedDespatchEvent","schema:rangeIncludes":{"@id":"unece:SupplyChainEvent"},"schema:domainIncludes":[{"@id":"unece:HeaderTradeDelivery"},{"@id":"unece:LineTradeDelivery"}],"rdfs:comment":"A significant occurrence or happening in a supply chain."},{"@id":"unece:requestedQuantity","@type":["rdf:Property","owl:ObjectProperty"],"rdfs:label":"requestedQuantity","schema:rangeIncludes":{"@id":"unece:QuantityType"},"schema:domainIncludes":[{"@id":"unece:HeaderTradeDelivery"},{"@id":"unece:LineTradeDelivery"}],"rdfs:comment":""},{"@id":"unece:shipFromParty","@type":["rdf:Property","owl:ObjectProperty"],"rdfs:label":"shipFromParty","schema:rangeIncludes":{"@id":"unece:TradeParty"},"schema:domainIncludes":[{"@id":"unece:HeaderTradeDelivery"},{"@id":"unece:LineTradeDelivery"},{"@id":"unece:Consignment"}],"rdfs:comment":"The ship from party for this supply chain consignment."},{"@id":"unece:shipToParty","@type":["rdf:Property","owl:ObjectProperty"],"rdfs:label":"shipToParty","schema:rangeIncludes":{"@id":"unece:TradeParty"},"schema:domainIncludes":[{"@id":"unece:HeaderTradeDelivery"},{"@id":"unece:LineTradeDelivery"},{"@id":"unece:SupplyPlan"},{"@id":"unece:DeliverySchedule"},{"@id":"unece:Consignment"}],"rdfs:comment":"A ship to party for this forecast delivery schedule."},{"@id":"unece:shipmentScheduleDocument","@type":["rdf:Property","owl:ObjectProperty"],"rdfs:label":"shipmentScheduleDocument","schema:rangeIncludes":{"@id":"unece:Document"},"schema:domainIncludes":[{"@id":"unece:HeaderTradeDelivery"},{"@id":"unece:LineTradeDelivery"}],"rdfs:comment":"Written, printed or electronic matter that is referenced."},{"@id":"unece:specifiedDeliveryInstructions","@type":["rdf:Property","owl:ObjectProperty"],"rdfs:label":"specifiedDeliveryInstructions","schema:rangeIncludes":{"@id":"unece:DeliveryInstructions"},"schema:domainIncludes":[{"@id":"unece:HeaderTradeDelivery"},{"@id":"unece:LineTradeDelivery"}],"rdfs:comment":"Delivery information of an instructive nature."},{"@id":"unece:specifiedHandlingInstructions","@type":["rdf:Property","owl:ObjectProperty"],"rdfs:label":"specifiedHandlingInstructions","schema:rangeIncludes":{"@id":"unece:HandlingInstructions"},"schema:domainIncludes":[{"@id":"unece:HeaderTradeDelivery"},{"@id":"unece:LineTradeDelivery"},{"@id":"unece:TransportMovement"},{"@id":"unece:LogisticsTransportMeans"}],"rdfs:comment":"Handling information of an instructive nature."},{"@id":"unece:specifiedSchedule","@type":["rdf:Property","owl:ObjectProperty"],"rdfs:label":"specifiedSchedule","schema:rangeIncludes":{"@id":"unece:Schedule"},"schema:domainIncludes":[{"@id":"unece:HeaderTradeDelivery"},{"@id":"unece:LineTradeDelivery"}],"rdfs:comment":"A series of planned activities or things to be done in this supply chain."},{"@id":"unece:specifiedSupplyChainEvent","@type":["rdf:Property","owl:ObjectProperty"],"rdfs:label":"specifiedSupplyChainEvent","schema:rangeIncludes":{"@id":"unece:SupplyChainEvent"},"schema:domainIncludes":[{"@id":"unece:HeaderTradeDelivery"},{"@id":"unece:SupplyPlan"},{"@id":"unece:TradeProduct"},{"@id":"unece:ProductBatch"},{"@id":"unece:ProductionFacility"},{"@id":"unece:SupplyChainInventory"},{"@id":"unece:Location"},{"@id":"unece:SustainabilityCharacteristic"},{"@id":"unece:TechnicalCharacteristic"}],"rdfs:comment":"A significant occurrence or happening in a supply chain."},{"@id":"unece:statusCode","@type":["rdf:Property","owl:DatatypeProperty"],"rdfs:label":"statusCode","schema:rangeIncludes":{"@id":"schema:Text"},"schema:domainIncludes":[{"@id":"unece:HeaderTradeDelivery"},{"@id":"unece:LineTradeDelivery"},{"@id":"unece:TradeProduct"},{"@id":"unece:LineTradeSettlement"},{"@id":"unece:ProductionProcess"},{"@id":"unece:ProductBatch"},{"@id":"unece:SupplyChainInventory"},{"@id":"unece:Schedule"},{"@id":"unece:SpecifiedParameter"},{"@id":"unece:PaymentTradeSettlement"},{"@id":"unece:SpecifiedCertificate"},{"@id":"unece:InspectionResult"},{"@id":"unece:Assertion"},{"@id":"unece:Assessment"},{"@id":"unece:ControlSettingParameter"},{"@id":"unece:OperationalParameter"},{"@id":"unece:InspectionInstructions"},{"@id":"unece:LaboratoryObservationInstructions"},{"@id":"unece:ObservationObjectiveParameter"},{"@id":"unece:SpecifiedMaterial"},{"@id":"unece:ExperienceProgramAction"},{"@id":"unece:ExperienceItem"},{"@id":"unece:AgriculturalProcess"},{"@id":"unece:SpecifiedRoute"}],"rdfs:comment":"A code specifying a status for this trade product."},{"@id":"unece:subordinateId","@type":["rdf:Property","owl:DatatypeProperty"],"rdfs:label":"subordinateId","schema:rangeIncludes":{"@id":"schema:Text"},"schema:domainIncludes":[{"@id":"unece:HeaderTradeDelivery"},{"@id":"unece:LineTradeDelivery"}],"rdfs:comment":"A subordinate identifier, at header level, for this trade delivery."},{"@id":"unece:ultimateShipToDeliveryDateTime","@type":["rdf:Property","owl:DatatypeProperty"],"rdfs:label":"ultimateShipToDeliveryDateTime","schema:rangeIncludes":{"@id":"schema:DateTime"},"schema:domainIncludes":[{"@id":"unece:HeaderTradeDelivery"},{"@id":"unece:LineTradeDelivery"}],"rdfs:comment":"The date, time, date time, or other date time value, at header level, when this trade delivery is delivered to the ultimate ship to party."},{"@id":"unece:ultimateShipToDeliveryEvent","@type":["rdf:Property","owl:ObjectProperty"],"rdfs:label":"ultimateShipToDeliveryEvent","schema:rangeIncludes":{"@id":"unece:SupplyChainEvent"},"schema:domainIncludes":{"@id":"unece:HeaderTradeDelivery"},"rdfs:comment":"A significant occurrence or happening in a supply chain."},{"@id":"unece:ultimateShipToParty","@type":["rdf:Property","owl:ObjectProperty"],"rdfs:label":"ultimateShipToParty","schema:rangeIncludes":{"@id":"unece:TradeParty"},"schema:domainIncludes":[{"@id":"unece:HeaderTradeDelivery"},{"@id":"unece:LineTradeDelivery"}],"rdfs:comment":"The ultimate ship to party, at header level, for this trade delivery."},{"@id":"unece:utilizedTransportEquipment","@type":["rdf:Property","owl:ObjectProperty"],"rdfs:label":"utilizedTransportEquipment","schema:rangeIncludes":{"@id":"unece:LogisticsTransportEquipment"},"schema:domainIncludes":[{"@id":"unece:HeaderTradeDelivery"},{"@id":"unece:LineTradeDelivery"},{"@id":"unece:Consignment"}],"rdfs:comment":"A piece of equipment used to hold, protect or secure cargo for logistics purposes.,A referenced piece of equipment used to hold, protect or secure cargo for logistics purposes."},{"@id":"unece:applicableDangerousGoods","@type":["rdf:Property","owl:ObjectProperty"],"rdfs:label":"applicableDangerousGoods","schema:rangeIncludes":{"@id":"unece:DangerousGoods"},"schema:domainIncludes":[{"@id":"unece:LineTradeDelivery"},{"@id":"unece:TradeProduct"},{"@id":"unece:Consignment"},{"@id":"unece:ConsignmentItem"},{"@id":"unece:RegulatedGoods"}],"rdfs:comment":"Goods which may contain a substance which poses risks to people and/or the environment during transportation which is regulated by dangerous goods regulations."},{"@id":"unece:availableInventory","@type":["rdf:Property","owl:ObjectProperty"],"rdfs:label":"availableInventory","schema:rangeIncludes":{"@id":"unece:SupplyChainInventory"},"schema:domainIncludes":{"@id":"unece:LineTradeDelivery"},"rdfs:comment":"Inventory available, at line level, for this trade delivery."},{"@id":"unece:availableQuantity","@type":["rdf:Property","owl:ObjectProperty"],"rdfs:label":"availableQuantity","schema:rangeIncludes":{"@id":"unece:QuantityType"},"schema:domainIncludes":{"@id":"unece:LineTradeDelivery"},"rdfs:comment":""},{"@id":"unece:billedQuantity","@type":["rdf:Property","owl:ObjectProperty"],"rdfs:label":"billedQuantity","schema:rangeIncludes":{"@id":"unece:QuantityType"},"schema:domainIncludes":[{"@id":"unece:LineTradeDelivery"},{"@id":"unece:SubordinateLineTradeDelivery"}],"rdfs:comment":""},{"@id":"unece:cancelledQuantity","@type":["rdf:Property","owl:ObjectProperty"],"rdfs:label":"cancelledQuantity","schema:rangeIncludes":{"@id":"unece:QuantityType"},"schema:domainIncludes":{"@id":"unece:LineTradeDelivery"},"rdfs:comment":""},{"@id":"unece:chargeFreeQuantity","@type":["rdf:Property","owl:ObjectProperty"],"rdfs:label":"chargeFreeQuantity","schema:rangeIncludes":{"@id":"unece:QuantityType"},"schema:domainIncludes":{"@id":"unece:LineTradeDelivery"},"rdfs:comment":""},{"@id":"unece:confirmedDeliveryEvent","@type":["rdf:Property","owl:ObjectProperty"],"rdfs:label":"confirmedDeliveryEvent","schema:rangeIncludes":{"@id":"unece:SupplyChainEvent"},"schema:domainIncludes":[{"@id":"unece:LineTradeDelivery"},{"@id":"unece:SupplyPlan"}],"rdfs:comment":"A significant occurrence or happening in a supply chain."},{"@id":"unece:consignmentInventory","@type":["rdf:Property","owl:ObjectProperty"],"rdfs:label":"consignmentInventory","schema:rangeIncludes":{"@id":"unece:SupplyChainInventory"},"schema:domainIncludes":{"@id":"unece:LineTradeDelivery"},"rdfs:comment":"Supply chain consignment inventory, at line level, for this trade delivery."},{"@id":"unece:consumptionSchedule","@type":["rdf:Property","owl:ObjectProperty"],"rdfs:label":"consumptionSchedule","schema:rangeIncludes":{"@id":"unece:Schedule"},"schema:domainIncludes":{"@id":"unece:LineTradeDelivery"},"rdfs:comment":"A series of planned activities or things to be done in this supply chain."},{"@id":"unece:customerInventory","@type":["rdf:Property","owl:ObjectProperty"],"rdfs:label":"customerInventory","schema:rangeIncludes":{"@id":"unece:SupplyChainInventory"},"schema:domainIncludes":{"@id":"unece:LineTradeDelivery"},"rdfs:comment":"Supply chain customer inventory, at line level, for this trade delivery."},{"@id":"unece:deliverySchedule","@type":["rdf:Property","owl:ObjectProperty"],"rdfs:label":"deliverySchedule","schema:rangeIncludes":{"@id":"unece:Schedule"},"schema:domainIncludes":{"@id":"unece:LineTradeDelivery"},"rdfs:comment":"A series of planned activities or things to be done in this supply chain."},{"@id":"unece:despatchSchedule","@type":["rdf:Property","owl:ObjectProperty"],"rdfs:label":"despatchSchedule","schema:rangeIncludes":{"@id":"unece:Schedule"},"schema:domainIncludes":{"@id":"unece:LineTradeDelivery"},"rdfs:comment":"A series of planned activities or things to be done in this supply chain."},{"@id":"unece:destroyedQuantity","@type":["rdf:Property","owl:ObjectProperty"],"rdfs:label":"destroyedQuantity","schema:rangeIncludes":{"@id":"unece:QuantityType"},"schema:domainIncludes":{"@id":"unece:LineTradeDelivery"},"rdfs:comment":""},{"@id":"unece:dueInReturnedQuantity","@type":["rdf:Property","owl:ObjectProperty"],"rdfs:label":"dueInReturnedQuantity","schema:rangeIncludes":{"@id":"unece:QuantityType"},"schema:domainIncludes":{"@id":"unece:LineTradeDelivery"},"rdfs:comment":""},{"@id":"unece:economicOrderQuantity","@type":["rdf:Property","owl:ObjectProperty"],"rdfs:label":"economicOrderQuantity","schema:rangeIncludes":{"@id":"unece:QuantityType"},"schema:domainIncludes":[{"@id":"unece:LineTradeDelivery"},{"@id":"unece:LineTradeAgreement"}],"rdfs:comment":""},{"@id":"unece:gFMTransferRejectedQuantity","@type":["rdf:Property","owl:ObjectProperty"],"rdfs:label":"gFMTransferRejectedQuantity","schema:rangeIncludes":{"@id":"unece:QuantityType"},"schema:domainIncludes":{"@id":"unece:LineTradeDelivery"},"rdfs:comment":""},{"@id":"unece:individualPackageQuantity","@type":["rdf:Property","owl:ObjectProperty"],"rdfs:label":"individualPackageQuantity","schema:rangeIncludes":{"@id":"unece:QuantityType"},"schema:domainIncludes":{"@id":"unece:LineTradeDelivery"},"rdfs:comment":""},{"@id":"unece:latestDespatchedQuantity","@type":["rdf:Property","owl:ObjectProperty"],"rdfs:label":"latestDespatchedQuantity","schema:rangeIncludes":{"@id":"unece:QuantityType"},"schema:domainIncludes":{"@id":"unece:LineTradeDelivery"},"rdfs:comment":""},{"@id":"unece:lineTradeDeliveryQuantityDiscrepancyNatureCode","@type":["rdf:Property","owl:DatatypeProperty"],"rdfs:label":"lineTradeDeliveryQuantityDiscrepancyNatureCode","schema:rangeIncludes":{"@id":"schema:Text"},"schema:domainIncludes":{"@id":"unece:LineTradeDelivery"},"rdfs:comment":"The code specifying the nature of the discrepancy of the quantity, at line level, for this trade delivery."},{"@id":"unece:lineTradeDeliveryQuantityVariationTypeCode","@type":["rdf:Property","owl:DatatypeProperty"],"rdfs:label":"lineTradeDeliveryQuantityVariationTypeCode","schema:rangeIncludes":{"@id":"schema:Text"},"schema:domainIncludes":{"@id":"unece:LineTradeDelivery"},"rdfs:comment":"The code specifying the type of quantity variation, at line level, for this trade delivery."},{"@id":"unece:logisticsServiceProviderParty","@type":["rdf:Property","owl:ObjectProperty"],"rdfs:label":"logisticsServiceProviderParty","schema:rangeIncludes":{"@id":"unece:TradeParty"},"schema:domainIncludes":{"@id":"unece:LineTradeDelivery"},"rdfs:comment":"A logistics service provider party, at line level, for this trade delivery."},{"@id":"unece:orderQuantity","@type":["rdf:Property","owl:ObjectProperty"],"rdfs:label":"orderQuantity","schema:rangeIncludes":{"@id":"unece:QuantityType"},"schema:domainIncludes":{"@id":"unece:LineTradeDelivery"},"rdfs:comment":""},{"@id":"unece:orderSchedule","@type":["rdf:Property","owl:ObjectProperty"],"rdfs:label":"orderSchedule","schema:rangeIncludes":{"@id":"unece:Schedule"},"schema:domainIncludes":{"@id":"unece:LineTradeDelivery"},"rdfs:comment":"A series of planned activities or things to be done in this supply chain."},{"@id":"unece:packageQuantity","@type":["rdf:Property","owl:ObjectProperty"],"rdfs:label":"packageQuantity","schema:rangeIncludes":{"@id":"unece:QuantityType"},"schema:domainIncludes":[{"@id":"unece:LineTradeDelivery"},{"@id":"unece:SubordinateLineTradeDelivery"},{"@id":"unece:TransportMovement"},{"@id":"unece:Consignment"},{"@id":"unece:ConsignmentItem"}],"rdfs:comment":""},{"@id":"unece:perPackageUnitQuantity","@type":["rdf:Property","owl:ObjectProperty"],"rdfs:label":"perPackageUnitQuantity","schema:rangeIncludes":{"@id":"unece:QuantityType"},"schema:domainIncludes":[{"@id":"unece:LineTradeDelivery"},{"@id":"unece:SubordinateLineTradeDelivery"},{"@id":"unece:Package"}],"rdfs:comment":""},{"@id":"unece:productUnitQuantity","@type":["rdf:Property","owl:ObjectProperty"],"rdfs:label":"productUnitQuantity","schema:rangeIncludes":{"@id":"unece:QuantityType"},"schema:domainIncludes":[{"@id":"unece:LineTradeDelivery"},{"@id":"unece:SubordinateLineTradeDelivery"}],"rdfs:comment":""},{"@id":"unece:projectedSupplyPlan","@type":["rdf:Property","owl:ObjectProperty"],"rdfs:label":"projectedSupplyPlan","schema:rangeIncludes":{"@id":"unece:SupplyPlan"},"schema:domainIncludes":{"@id":"unece:LineTradeDelivery"},"rdfs:comment":"A supply plan, at line level, projected for this trade delivery."},{"@id":"unece:quantityVariationReason","@type":["rdf:Property","owl:DatatypeProperty"],"rdfs:label":"quantityVariationReason","schema:rangeIncludes":{"@id":"schema:Text"},"schema:domainIncludes":{"@id":"unece:LineTradeDelivery"},"rdfs:comment":"A reason, expressed as text, for a quantity variation, at line level, for this trade delivery."},{"@id":"unece:quantityVariationReasonCode","@type":["rdf:Property","owl:DatatypeProperty"],"rdfs:label":"quantityVariationReasonCode","schema:rangeIncludes":{"@id":"schema:Text"},"schema:domainIncludes":{"@id":"unece:LineTradeDelivery"},"rdfs:comment":"The code specifying the reason for the quantity variation, at line level, for this trade delivery."},{"@id":"unece:receiptSchedule","@type":["rdf:Property","owl:ObjectProperty"],"rdfs:label":"receiptSchedule","schema:rangeIncludes":{"@id":"unece:Schedule"},"schema:domainIncludes":{"@id":"unece:LineTradeDelivery"},"rdfs:comment":"A series of planned activities or things to be done in this supply chain."},{"@id":"unece:receivedQuantity","@type":["rdf:Property","owl:ObjectProperty"],"rdfs:label":"receivedQuantity","schema:rangeIncludes":{"@id":"unece:QuantityType"},"schema:domainIncludes":{"@id":"unece:LineTradeDelivery"},"rdfs:comment":""},{"@id":"unece:rejectedQuantity","@type":["rdf:Property","owl:ObjectProperty"],"rdfs:label":"rejectedQuantity","schema:rangeIncludes":{"@id":"unece:QuantityType"},"schema:domainIncludes":{"@id":"unece:LineTradeDelivery"},"rdfs:comment":""},{"@id":"unece:returnedQuantity","@type":["rdf:Property","owl:ObjectProperty"],"rdfs:label":"returnedQuantity","schema:rangeIncludes":{"@id":"unece:QuantityType"},"schema:domainIncludes":{"@id":"unece:LineTradeDelivery"},"rdfs:comment":""},{"@id":"unece:reverseBilledQuantity","@type":["rdf:Property","owl:ObjectProperty"],"rdfs:label":"reverseBilledQuantity","schema:rangeIncludes":{"@id":"unece:QuantityType"},"schema:domainIncludes":{"@id":"unece:LineTradeDelivery"},"rdfs:comment":""},{"@id":"unece:specifiedDeliveryAdjustment","@type":["rdf:Property","owl:ObjectProperty"],"rdfs:label":"specifiedDeliveryAdjustment","schema:rangeIncludes":{"@id":"unece:DeliveryAdjustment"},"schema:domainIncludes":{"@id":"unece:LineTradeDelivery"},"rdfs:comment":"A correction or modification to reflect actual delivery conditions."},{"@id":"unece:specifiedPackage","@type":["rdf:Property","owl:ObjectProperty"],"rdfs:label":"specifiedPackage","schema:rangeIncludes":{"@id":"unece:Package"},"schema:domainIncludes":[{"@id":"unece:LineTradeDelivery"},{"@id":"unece:SupplyChainTradeTransaction"},{"@id":"unece:DangerousGoods"}],"rdfs:comment":"A self-contained wrapping or container within which goods can be contained for logistics purposes, such as a box or a barrel which can be filled, partially filled or empty.,A referenced self-contained wrapping or container within which goods can be contained for logistics purposes."},{"@id":"unece:supplySpecifiedSchedule","@type":["rdf:Property","owl:ObjectProperty"],"rdfs:label":"supplySpecifiedSchedule","schema:rangeIncludes":{"@id":"unece:Schedule"},"schema:domainIncludes":{"@id":"unece:LineTradeDelivery"},"rdfs:comment":"A series of planned activities or things to be done in this supply chain."},{"@id":"unece:turnInReceivedQuantity","@type":["rdf:Property","owl:ObjectProperty"],"rdfs:label":"turnInReceivedQuantity","schema:rangeIncludes":{"@id":"unece:QuantityType"},"schema:domainIncludes":{"@id":"unece:LineTradeDelivery"},"rdfs:comment":""},{"@id":"unece:unavailableQuantity","@type":["rdf:Property","owl:ObjectProperty"],"rdfs:label":"unavailableQuantity","schema:rangeIncludes":{"@id":"unece:QuantityType"},"schema:domainIncludes":{"@id":"unece:LineTradeDelivery"},"rdfs:comment":""},{"@id":"unece:usedLabel","@type":["rdf:Property","owl:ObjectProperty"],"rdfs:label":"usedLabel","schema:rangeIncludes":{"@id":"unece:LogisticsLabel"},"schema:domainIncludes":{"@id":"unece:LineTradeDelivery"},"rdfs:comment":"A label used for identifying goods for logistics purposes, such as a barcode, a radio frequency tag or a Vehicle Identification Number (VIN)."},{"@id":"unece:volumeUnitGrossVolumeMeasure","@type":["rdf:Property","owl:ObjectProperty"],"rdfs:label":"volumeUnitGrossVolumeMeasure","schema:rangeIncludes":{"@id":"unece:VolumeUnitMeasureType"},"schema:domainIncludes":[{"@id":"unece:LineTradeDelivery"},{"@id":"unece:LogisticsTransportEquipment"},{"@id":"unece:DangerousGoods"},{"@id":"unece:Package"},{"@id":"unece:Consignment"},{"@id":"unece:ConsignmentItem"}],"rdfs:comment":""},{"@id":"unece:volumeUnitNetVolumeMeasure","@type":["rdf:Property","owl:ObjectProperty"],"rdfs:label":"volumeUnitNetVolumeMeasure","schema:rangeIncludes":{"@id":"unece:VolumeUnitMeasureType"},"schema:domainIncludes":[{"@id":"unece:LineTradeDelivery"},{"@id":"unece:Consignment"}],"rdfs:comment":""},{"@id":"unece:weightUnitChargeableWeightMeasure","@type":["rdf:Property","owl:ObjectProperty"],"rdfs:label":"weightUnitChargeableWeightMeasure","schema:rangeIncludes":{"@id":"unece:WeightUnitMeasureType"},"schema:domainIncludes":[{"@id":"unece:LineTradeDelivery"},{"@id":"unece:Consignment"},{"@id":"unece:ConsignmentItem"}],"rdfs:comment":""},{"@id":"unece:weightUnitGrossWeightMeasure","@type":["rdf:Property","owl:ObjectProperty"],"rdfs:label":"weightUnitGrossWeightMeasure","schema:rangeIncludes":{"@id":"unece:WeightUnitMeasureType"},"schema:domainIncludes":[{"@id":"unece:LineTradeDelivery"},{"@id":"unece:LogisticsTransportEquipment"},{"@id":"unece:DangerousGoods"},{"@id":"unece:Package"},{"@id":"unece:LogisticsTransportMeans"},{"@id":"unece:Consignment"},{"@id":"unece:ConsignmentItem"}],"rdfs:comment":""},{"@id":"unece:weightUnitNetWeightMeasure","@type":["rdf:Property","owl:ObjectProperty"],"rdfs:label":"weightUnitNetWeightMeasure","schema:rangeIncludes":{"@id":"unece:WeightUnitMeasureType"},"schema:domainIncludes":[{"@id":"unece:LineTradeDelivery"},{"@id":"unece:LogisticsTransportEquipment"},{"@id":"unece:DangerousGoods"},{"@id":"unece:Package"},{"@id":"unece:LogisticsTransportMeans"},{"@id":"unece:Consignment"},{"@id":"unece:ConsignmentItem"}],"rdfs:comment":""},{"@id":"unece:weightUnitTheoreticalWeightMeasure","@type":["rdf:Property","owl:ObjectProperty"],"rdfs:label":"weightUnitTheoreticalWeightMeasure","schema:rangeIncludes":{"@id":"unece:WeightUnitMeasureType"},"schema:domainIncludes":{"@id":"unece:LineTradeDelivery"},"rdfs:comment":""},{"@id":"unece:accessibleLocation","@type":["rdf:Property","owl:ObjectProperty"],"rdfs:label":"accessibleLocation","schema:rangeIncludes":{"@id":"unece:SpecifiedLocation"},"schema:domainIncludes":{"@id":"unece:TradeContact"},"rdfs:comment":"A specified physical location or place."},{"@id":"unece:authorizedPersonName","@type":["rdf:Property","owl:DatatypeProperty"],"rdfs:label":"authorizedPersonName","schema:rangeIncludes":{"@id":"schema:Text"},"schema:domainIncludes":{"@id":"unece:TradeContact"},"rdfs:comment":"The name, expressed as text, of the authorized person for this trade contact."},{"@id":"unece:contactTypeCode","@type":["rdf:Property","owl:DatatypeProperty"],"rdfs:label":"contactTypeCode","schema:rangeIncludes":{"@id":"unece:ContactTypeCodeList"},"schema:domainIncludes":{"@id":"unece:TradeContact"},"rdfs:comment":"The code specifying the type of trade contact."},{"@id":"unece:departmentName","@type":["rdf:Property","owl:DatatypeProperty"],"rdfs:label":"departmentName","schema:rangeIncludes":{"@id":"schema:Text"},"schema:domainIncludes":[{"@id":"unece:TradeContact"},{"@id":"unece:TradeAddress"},{"@id":"unece:Address"},{"@id":"unece:FinancialInstitutionAddress"},{"@id":"unece:LaboratoryObservationContact"}],"rdfs:comment":"The name, expressed as text, of a department for this trade address."},{"@id":"unece:description","@type":["rdf:Property","owl:DatatypeProperty"],"rdfs:label":"description","schema:rangeIncludes":{"@id":"schema:Text"},"schema:domainIncludes":[{"@id":"unece:TradeContact"},{"@id":"unece:TradeProduct"},{"@id":"unece:ProductionProcess"},{"@id":"unece:TradeAddress"},{"@id":"unece:TradeParty"},{"@id":"unece:TradeTax"},{"@id":"unece:ProductBatch"},{"@id":"unece:ProductionFacility"},{"@id":"unece:Colour"},{"@id":"unece:ProductionUnit"},{"@id":"unece:Print"},{"@id":"unece:ProductFinishingTreatment"},{"@id":"unece:SpecifiedChemicalTreatment"},{"@id":"unece:HeaderTradeSettlement"},{"@id":"unece:Contract"},{"@id":"unece:Product"},{"@id":"unece:TTExchangedDocument"},{"@id":"unece:TTLocation"},{"@id":"unece:TradeProductFeature"},{"@id":"unece:Classification"},{"@id":"unece:Document"},{"@id":"unece:ExchangedDocument"},{"@id":"unece:BinaryFile"},{"@id":"unece:SpecifiedAction"},{"@id":"unece:Measurement"},{"@id":"unece:QuantityAnalysis"},{"@id":"unece:SpecifiedFault"},{"@id":"unece:Picture"},{"@id":"unece:UsageCondition"},{"@id":"unece:Location"},{"@id":"unece:CommunicationEvent"},{"@id":"unece:CustomerClass"},{"@id":"unece:InformationSource"},{"@id":"unece:GeographicalFeature"},{"@id":"unece:Communication"},{"@id":"unece:SpecifiedPeriod"},{"@id":"unece:WorkItemDimension"},{"@id":"unece:DocumentStatus"},{"@id":"unece:Project"},{"@id":"unece:SpecifiedNote"},{"@id":"unece:MetricCharacteristic"},{"@id":"unece:AvailablePeriod"},{"@id":"unece:DocumentCharacteristic"},{"@id":"unece:GeographicalObjectCharacteristic"},{"@id":"unece:IdentifiedFault"},{"@id":"unece:Membership"},{"@id":"unece:Schedule"},{"@id":"unece:SpatialDimension"},{"@id":"unece:SpecifiedFeature"},{"@id":"unece:SpecifiedLocation"},{"@id":"unece:SpecifiedParameter"},{"@id":"unece:Address"},{"@id":"unece:Event"},{"@id":"unece:AppliedAllowanceCharge"},{"@id":"unece:Cash"},{"@id":"unece:Cheque"},{"@id":"unece:DigitalMethod"},{"@id":"unece:FinancialCard"},{"@id":"unece:PaymentTerms"},{"@id":"unece:BreakdownStatement"},{"@id":"unece:HeaderBalanceOut"},{"@id":"unece:PaymentBalanceOut"},{"@id":"unece:Guarantee"},{"@id":"unece:RegisteredTax"},{"@id":"unece:RequestingParty"},{"@id":"unece:Tax"},{"@id":"unece:Voucher"},{"@id":"unece:TradeAllowanceCharge"},{"@id":"unece:TradePrice"},{"@id":"unece:InspectionReference"},{"@id":"unece:LaboratoryObservationReference"},{"@id":"unece:ProtectionMeans"},{"@id":"unece:Accreditation"},{"@id":"unece:CorrectiveAction"},{"@id":"unece:PreventiveAction"},{"@id":"unece:OrganizationalCertificate"},{"@id":"unece:ProcessCertificate"},{"@id":"unece:ProductBatchCertificate"},{"@id":"unece:ProductCertificate"},{"@id":"unece:SpecifiedCertificate"},{"@id":"unece:Standard"},{"@id":"unece:ProcessWorkItem"},{"@id":"unece:ProductCharacteristic"},{"@id":"unece:ProductBatchCharacteristic"},{"@id":"unece:SustainabilityCharacteristic"},{"@id":"unece:SustainabilityInspection"},{"@id":"unece:Observation"},{"@id":"unece:HazardousMaterial"},{"@id":"unece:Assertion"},{"@id":"unece:Policy"},{"@id":"unece:ProcessCharacteristic"},{"@id":"unece:TechnicalCharacteristic"},{"@id":"unece:Licence"},{"@id":"unece:SpecifiedDeclaration"},{"@id":"unece:SpecifiedInspection"},{"@id":"unece:Source"},{"@id":"unece:RiskAnalysisResult"},{"@id":"unece:ControlSettingParameter"},{"@id":"unece:OperationalParameter"},{"@id":"unece:InspectionStatus"},{"@id":"unece:DisposalInstructions"},{"@id":"unece:InspectionEvent"},{"@id":"unece:InspectionInstructions"},{"@id":"unece:LaboratoryObservationInstructions"},{"@id":"unece:ObservationObjectiveParameter"},{"@id":"unece:QuarantineInstructions"},{"@id":"unece:Requirement"},{"@id":"unece:TemperatureSettingInstructions"},{"@id":"unece:OrganizationCharacteristic"},{"@id":"unece:GoodsCharacteristic"},{"@id":"unece:SpecifiedMaterial"},{"@id":"unece:WasteMaterialRecoveryDisposalProcess"},{"@id":"unece:TransportInstructions"},{"@id":"unece:IngredientRangeMeasurement"},{"@id":"unece:ProductionWasteMaterialComponent"},{"@id":"unece:ProductionWasteRecoveryDisposalProcess"},{"@id":"unece:GuestPerson"},{"@id":"unece:ExperienceProgramAction"},{"@id":"unece:PetAnimal"},{"@id":"unece:ExperienceItem"},{"@id":"unece:ExperienceProduct"},{"@id":"unece:ExperienceEvent"},{"@id":"unece:ExperienceFacility"},{"@id":"unece:Allergy"},{"@id":"unece:CarriedEquipment"},{"@id":"unece:Disability"},{"@id":"unece:FoodChoice"},{"@id":"unece:GuestHealthIndication"},{"@id":"unece:PersonalEffects"},{"@id":"unece:Preference"},{"@id":"unece:AgriculturalCertificate"},{"@id":"unece:AgriculturalProcess"},{"@id":"unece:FieldCrop"},{"@id":"unece:CropProtectionTreatment"},{"@id":"unece:AgriculturalCharacteristic"},{"@id":"unece:TransportEvent"},{"@id":"unece:Service"},{"@id":"unece:Package"},{"@id":"unece:ServiceCharge"},{"@id":"unece:LogisticsPackaging"},{"@id":"unece:TransportationWasteMaterialComponent"},{"@id":"unece:HandlingInstructions"},{"@id":"unece:SanitaryMeasure"},{"@id":"unece:MDHHealthIndication"},{"@id":"unece:LogisticsStatus"},{"@id":"unece:LogisticsLocation"},{"@id":"unece:SpecifiedRoute"},{"@id":"unece:TransportRoute"},{"@id":"unece:HaulageInstructions"},{"@id":"unece:PackagingInstructions"},{"@id":"unece:StoresItemInventory"},{"@id":"unece:TransportationWasteRecoveryDisposalProcess"},{"@id":"unece:SupplyChainReference"},{"@id":"unece:SupplyChainPackaging"},{"@id":"unece:SupplyChainEvent"},{"@id":"unece:DeliveryTerms"},{"@id":"unece:DeliveryInstructions"}],"rdfs:comment":"A textual description for the type of transportation waste recovery disposal process."},{"@id":"unece:directTelephoneCommunication","@type":["rdf:Property","owl:ObjectProperty"],"rdfs:label":"directTelephoneCommunication","schema:rangeIncludes":{"@id":"unece:Communication"},"schema:domainIncludes":{"@id":"unece:TradeContact"},"rdfs:comment":"The exchange of thoughts, messages, or information, as universally exchanged by speech, signals, writing, or behaviour between persons and/or organizations."},{"@id":"unece:emailURICommunication","@type":["rdf:Property","owl:ObjectProperty"],"rdfs:label":"emailURICommunication","schema:rangeIncludes":{"@id":"unece:Communication"},"schema:domainIncludes":[{"@id":"unece:TradeContact"},{"@id":"unece:Person"},{"@id":"unece:Contact"},{"@id":"unece:TransportPerson"}],"rdfs:comment":"The exchange of thoughts, messages, or information, as universally exchanged by speech, signals, writing, or behaviour between persons and/or organizations."},{"@id":"unece:faxCommunication","@type":["rdf:Property","owl:ObjectProperty"],"rdfs:label":"faxCommunication","schema:rangeIncludes":{"@id":"unece:Communication"},"schema:domainIncludes":[{"@id":"unece:TradeContact"},{"@id":"unece:Contact"},{"@id":"unece:LaboratoryObservationContact"},{"@id":"unece:LocationParty"}],"rdfs:comment":"The exchange of thoughts, messages, or information, as universally exchanged by speech, signals, writing, or behaviour between persons and/or organizations."},{"@id":"unece:instantMessagingCommunication","@type":["rdf:Property","owl:ObjectProperty"],"rdfs:label":"instantMessagingCommunication","schema:rangeIncludes":{"@id":"unece:Communication"},"schema:domainIncludes":[{"@id":"unece:TradeContact"},{"@id":"unece:Contact"}],"rdfs:comment":"The exchange of thoughts, messages, or information, as universally exchanged by speech, signals, writing, or behaviour between persons and/or organizations."},{"@id":"unece:jobTitle","@type":["rdf:Property","owl:DatatypeProperty"],"rdfs:label":"jobTitle","schema:rangeIncludes":{"@id":"schema:Text"},"schema:domainIncludes":{"@id":"unece:TradeContact"},"rdfs:comment":"The job title, position or designation, expressed as text, of this trade contact within an organization, such as Director, Software Engineer, Purchasing Manager."},{"@id":"unece:mobileTelephoneCommunication","@type":["rdf:Property","owl:ObjectProperty"],"rdfs:label":"mobileTelephoneCommunication","schema:rangeIncludes":{"@id":"unece:Communication"},"schema:domainIncludes":[{"@id":"unece:TradeContact"},{"@id":"unece:Person"},{"@id":"unece:LaboratoryObservationContact"},{"@id":"unece:TransportPerson"}],"rdfs:comment":"The exchange of thoughts, messages, or information, as universally exchanged by speech, signals, writing, or behaviour between persons and/or organizations."},{"@id":"unece:personId","@type":["rdf:Property","owl:DatatypeProperty"],"rdfs:label":"personId","schema:rangeIncludes":{"@id":"schema:Text"},"schema:domainIncludes":{"@id":"unece:TradeContact"},"rdfs:comment":"A unique identifier for this trade contact person."},{"@id":"unece:personName","@type":["rdf:Property","owl:DatatypeProperty"],"rdfs:label":"personName","schema:rangeIncludes":{"@id":"schema:Text"},"schema:domainIncludes":[{"@id":"unece:TradeContact"},{"@id":"unece:LaboratoryObservationContact"}],"rdfs:comment":"The name, expressed as text, of the person for this laboratory observation contact."},{"@id":"unece:postalAddress","@type":["rdf:Property","owl:ObjectProperty"],"rdfs:label":"postalAddress","schema:rangeIncludes":{"@id":"unece:TradeAddress"},"schema:domainIncludes":[{"@id":"unece:TradeContact"},{"@id":"unece:TradeParty"},{"@id":"unece:Location"},{"@id":"unece:LegalOrganization"},{"@id":"unece:LaboratoryObservationParty"},{"@id":"unece:LogisticsLocation"},{"@id":"unece:LocationParty"}],"rdfs:comment":"A postal address for this legally set up organization."},{"@id":"unece:responsibility","@type":["rdf:Property","owl:DatatypeProperty"],"rdfs:label":"responsibility","schema:rangeIncludes":{"@id":"schema:Text"},"schema:domainIncludes":{"@id":"unece:TradeContact"},"rdfs:comment":"A responsibility, expressed as text, of this trade contact."},{"@id":"unece:specifiedContactPerson","@type":["rdf:Property","owl:ObjectProperty"],"rdfs:label":"specifiedContactPerson","schema:rangeIncludes":{"@id":"unece:Contact"},"schema:domainIncludes":[{"@id":"unece:TradeContact"},{"@id":"unece:TradeParty"}],"rdfs:comment":"An individual human being in a position to give assistance or information."},{"@id":"unece:specifiedNote","@type":["rdf:Property","owl:ObjectProperty"],"rdfs:label":"specifiedNote","schema:rangeIncludes":{"@id":"unece:Note"},"schema:domainIncludes":[{"@id":"unece:TradeContact"},{"@id":"unece:ProductBatch"},{"@id":"unece:Picture"}],"rdfs:comment":"A textual or coded description, such as a remark or additional information."},{"@id":"unece:telephoneCommunication","@type":["rdf:Property","owl:ObjectProperty"],"rdfs:label":"telephoneCommunication","schema:rangeIncludes":{"@id":"unece:Communication"},"schema:domainIncludes":[{"@id":"unece:TradeContact"},{"@id":"unece:TradeParty"},{"@id":"unece:Contact"},{"@id":"unece:LaboratoryObservationContact"},{"@id":"unece:LocationParty"}],"rdfs:comment":"The exchange of thoughts, messages, or information, as universally exchanged by speech, signals, writing, or behaviour between persons and/or organizations."},{"@id":"unece:telexCommunication","@type":["rdf:Property","owl:ObjectProperty"],"rdfs:label":"telexCommunication","schema:rangeIncludes":{"@id":"unece:Communication"},"schema:domainIncludes":{"@id":"unece:TradeContact"},"rdfs:comment":"The exchange of thoughts, messages, or information, as universally exchanged by speech, signals, writing, or behaviour between persons and/or organizations."},{"@id":"unece:usedCommunication","@type":["rdf:Property","owl:ObjectProperty"],"rdfs:label":"usedCommunication","schema:rangeIncludes":{"@id":"unece:Communication"},"schema:domainIncludes":[{"@id":"unece:TradeContact"},{"@id":"unece:GuestPerson"}],"rdfs:comment":"The exchange of thoughts, messages, or information, as universally exchanged by speech, signals, writing, or behaviour between persons and/or organizations."},{"@id":"unece:vOIPCommunication","@type":["rdf:Property","owl:ObjectProperty"],"rdfs:label":"vOIPCommunication","schema:rangeIncludes":{"@id":"unece:Communication"},"schema:domainIncludes":{"@id":"unece:TradeContact"},"rdfs:comment":"The exchange of thoughts, messages, or information, as universally exchanged by speech, signals, writing, or behaviour between persons and/or organizations."},{"@id":"unece:accessoryApplicableProduct","@type":["rdf:Property","owl:ObjectProperty"],"rdfs:label":"accessoryApplicableProduct","schema:rangeIncludes":{"@id":"unece:Product"},"schema:domainIncludes":{"@id":"unece:SupplyChainTradeLineItem"},"rdfs:comment":"A referenced accessory product applicable for this supply chain trade line item."},{"@id":"unece:additionalApplicableProduct","@type":["rdf:Property","owl:ObjectProperty"],"rdfs:label":"additionalApplicableProduct","schema:rangeIncludes":{"@id":"unece:Product"},"schema:domainIncludes":{"@id":"unece:SupplyChainTradeLineItem"},"rdfs:comment":"A referenced product additionally applicable with this supply chain trade line item."},{"@id":"unece:additionalId","@type":["rdf:Property","owl:DatatypeProperty"],"rdfs:label":"additionalId","schema:rangeIncludes":{"@id":"schema:Text"},"schema:domainIncludes":{"@id":"unece:SupplyChainTradeLineItem"},"rdfs:comment":"An additional unique identifier for this supply chain trade line item."},{"@id":"unece:additionalInformationNote","@type":["rdf:Property","owl:ObjectProperty"],"rdfs:label":"additionalInformationNote","schema:rangeIncludes":{"@id":"unece:Note"},"schema:domainIncludes":[{"@id":"unece:SupplyChainTradeLineItem"},{"@id":"unece:ProductionProcess"}],"rdfs:comment":"A textual or coded description, such as a remark or additional information."},{"@id":"unece:applicableBatch","@type":["rdf:Property","owl:ObjectProperty"],"rdfs:label":"applicableBatch","schema:rangeIncludes":{"@id":"unece:ProductBatch"},"schema:domainIncludes":{"@id":"unece:SupplyChainTradeLineItem"},"rdfs:comment":"A product batch applicable to this supply chain trade line item."},{"@id":"unece:applicableMaterial","@type":["rdf:Property","owl:ObjectProperty"],"rdfs:label":"applicableMaterial","schema:rangeIncludes":{"@id":"unece:SpecifiedMaterial"},"schema:domainIncludes":[{"@id":"unece:SupplyChainTradeLineItem"},{"@id":"unece:Colour"},{"@id":"unece:Print"}],"rdfs:comment":"A substance from which something is or could be made."},{"@id":"unece:appliedProcess","@type":["rdf:Property","owl:ObjectProperty"],"rdfs:label":"appliedProcess","schema:rangeIncludes":{"@id":"unece:ProductHandlingProcess"},"schema:domainIncludes":[{"@id":"unece:SupplyChainTradeLineItem"},{"@id":"unece:ProductInstance"}],"rdfs:comment":"A product handling process applied to this supply chain trade line item, such as manufacturing, treatment or storage."},{"@id":"unece:assertedAuthentication","@type":["rdf:Property","owl:ObjectProperty"],"rdfs:label":"assertedAuthentication","schema:rangeIncludes":{"@id":"unece:Authentication"},"schema:domainIncludes":{"@id":"unece:SupplyChainTradeLineItem"},"rdfs:comment":"A proof that a document is genuine."},{"@id":"unece:associatedDocumentLineDocument","@type":["rdf:Property","owl:ObjectProperty"],"rdfs:label":"associatedDocumentLineDocument","schema:rangeIncludes":{"@id":"unece:DocumentLineDocument"},"schema:domainIncludes":[{"@id":"unece:SupplyChainTradeLineItem"},{"@id":"unece:LineTradeSettlement"},{"@id":"unece:SupplyChainTradeTransaction"}],"rdfs:comment":"A document line associated with this line trade settlement."},{"@id":"unece:associatedTransportEquipment","@type":["rdf:Property","owl:ObjectProperty"],"rdfs:label":"associatedTransportEquipment","schema:rangeIncludes":{"@id":"unece:LogisticsTransportEquipment"},"schema:domainIncludes":[{"@id":"unece:SupplyChainTradeLineItem"},{"@id":"unece:DangerousGoods"},{"@id":"unece:ConsignmentItem"}],"rdfs:comment":"A piece of equipment used to hold, protect or secure cargo for logistics purposes.,A referenced piece of equipment used to hold, protect or secure cargo for logistics purposes."},{"@id":"unece:barcodeId","@type":["rdf:Property","owl:DatatypeProperty"],"rdfs:label":"barcodeId","schema:rangeIncludes":{"@id":"schema:Text"},"schema:domainIncludes":[{"@id":"unece:SupplyChainTradeLineItem"},{"@id":"unece:ProductLabel"}],"rdfs:comment":"A unique barcode identifier for this supply chain trade line item."},{"@id":"unece:complementaryApplicableProduct","@type":["rdf:Property","owl:ObjectProperty"],"rdfs:label":"complementaryApplicableProduct","schema:rangeIncludes":{"@id":"unece:Product"},"schema:domainIncludes":{"@id":"unece:SupplyChainTradeLineItem"},"rdfs:comment":"A referenced complementary product applicable for this supply chain trade line item."},{"@id":"unece:componentApplicableProduct","@type":["rdf:Property","owl:ObjectProperty"],"rdfs:label":"componentApplicableProduct","schema:rangeIncludes":{"@id":"unece:Product"},"schema:domainIncludes":{"@id":"unece:SupplyChainTradeLineItem"},"rdfs:comment":"A referenced component product applicable for this supply chain trade line item."},{"@id":"unece:descriptionCode","@type":["rdf:Property","owl:DatatypeProperty"],"rdfs:label":"descriptionCode","schema:rangeIncludes":{"@id":"schema:Text"},"schema:domainIncludes":[{"@id":"unece:SupplyChainTradeLineItem"},{"@id":"unece:TradeProduct"},{"@id":"unece:ProductBatch"},{"@id":"unece:Assertion"},{"@id":"unece:TechnicalCharacteristic"},{"@id":"unece:InspectionInstructions"},{"@id":"unece:SpecifiedMaterial"}],"rdfs:comment":"A code specifying a description of this technical characteristic."},{"@id":"unece:generalInformationDescription","@type":["rdf:Property","owl:DatatypeProperty"],"rdfs:label":"generalInformationDescription","schema:rangeIncludes":{"@id":"schema:Text"},"schema:domainIncludes":{"@id":"unece:SupplyChainTradeLineItem"},"rdfs:comment":"A textual description providing general information for this supply chain trade line item."},{"@id":"unece:includedSubordinateTradeLineItem","@type":["rdf:Property","owl:ObjectProperty"],"rdfs:label":"includedSubordinateTradeLineItem","schema:rangeIncludes":{"@id":"unece:SubordinateTradeLineItem"},"schema:domainIncludes":{"@id":"unece:SupplyChainTradeLineItem"},"rdfs:comment":"A subordinate trade line item included in this supply chain trade line item."},{"@id":"unece:includedWithinConsignmentItem","@type":["rdf:Property","owl:ObjectProperty"],"rdfs:label":"includedWithinConsignmentItem","schema:rangeIncludes":{"@id":"unece:ConsignmentItem"},"schema:domainIncludes":{"@id":"unece:SupplyChainTradeLineItem"},"rdfs:comment":"A reference to an item within a supply chain consignment of goods separately identified for transport and customs purposes.,An item within a supply chain consignment of goods separately identified for transport and customs purposes."},{"@id":"unece:invoiceAssociatedDocument","@type":["rdf:Property","owl:ObjectProperty"],"rdfs:label":"invoiceAssociatedDocument","schema:rangeIncludes":{"@id":"unece:Document"},"schema:domainIncludes":{"@id":"unece:SupplyChainTradeLineItem"},"rdfs:comment":"Written, printed or electronic matter that is referenced."},{"@id":"unece:package","@type":["rdf:Property","owl:ObjectProperty"],"rdfs:label":"package","schema:rangeIncludes":{"@id":"unece:Package"},"schema:domainIncludes":{"@id":"unece:SupplyChainTradeLineItem"},"rdfs:comment":"A self-contained wrapping or container within which goods can be contained for logistics purposes, such as a box or a barrel which can be filled, partially filled or empty.,A referenced self-contained wrapping or container within which goods can be contained for logistics purposes."},{"@id":"unece:physicalPackage","@type":["rdf:Property","owl:ObjectProperty"],"rdfs:label":"physicalPackage","schema:rangeIncludes":{"@id":"unece:Package"},"schema:domainIncludes":{"@id":"unece:SupplyChainTradeLineItem"},"rdfs:comment":"A self-contained wrapping or container within which goods can be contained for logistics purposes, such as a box or a barrel which can be filled, partially filled or empty.,A referenced self-contained wrapping or container within which goods can be contained for logistics purposes."},{"@id":"unece:referenceDocument","@type":["rdf:Property","owl:ObjectProperty"],"rdfs:label":"referenceDocument","schema:rangeIncludes":{"@id":"unece:Document"},"schema:domainIncludes":[{"@id":"unece:SupplyChainTradeLineItem"},{"@id":"unece:AcknowledgementDocument"},{"@id":"unece:DocumentLineDocument"},{"@id":"unece:ExchangedDocument"}],"rdfs:comment":"Written, printed or electronic matter that is referenced."},{"@id":"unece:requiredApplicableProduct","@type":["rdf:Property","owl:ObjectProperty"],"rdfs:label":"requiredApplicableProduct","schema:rangeIncludes":{"@id":"unece:Product"},"schema:domainIncludes":{"@id":"unece:SupplyChainTradeLineItem"},"rdfs:comment":"A required product applicable for this supply chain trade line item."},{"@id":"unece:requisitionerSpecifiedProduct","@type":["rdf:Property","owl:ObjectProperty"],"rdfs:label":"requisitionerSpecifiedProduct","schema:rangeIncludes":{"@id":"unece:TradeProduct"},"schema:domainIncludes":{"@id":"unece:SupplyChainTradeLineItem"},"rdfs:comment":"The product specified by the requisitioner for this supply chain trade line item."},{"@id":"unece:sequenceNumeric","@type":["rdf:Property","owl:DatatypeProperty"],"rdfs:label":"sequenceNumeric","schema:rangeIncludes":{"@id":"schema:Text"},"schema:domainIncludes":[{"@id":"unece:SupplyChainTradeLineItem"},{"@id":"unece:ProductionCycle"},{"@id":"unece:NegotiationExchange"},{"@id":"unece:SpecifiedPeriod"},{"@id":"unece:DocumentStatus"},{"@id":"unece:TradeAllowanceCharge"},{"@id":"unece:SpecifiedCertificate"},{"@id":"unece:InspectionInstructions"},{"@id":"unece:LaboratoryObservationInstructions"},{"@id":"unece:PersonalEffects"},{"@id":"unece:LogisticsTransportEquipment"},{"@id":"unece:Package"},{"@id":"unece:LogisticsTransportMeans"},{"@id":"unece:Consignment"},{"@id":"unece:ConsignmentItem"},{"@id":"unece:LogisticsPackaging"},{"@id":"unece:LogisticsStatus"},{"@id":"unece:StoresItemInventory"}],"rdfs:comment":"A sequence number for these specified personal effects."},{"@id":"unece:specifiedLineTradeAgreement","@type":["rdf:Property","owl:ObjectProperty"],"rdfs:label":"specifiedLineTradeAgreement","schema:rangeIncludes":{"@id":"unece:LineTradeAgreement"},"schema:domainIncludes":{"@id":"unece:SupplyChainTradeLineItem"},"rdfs:comment":"The line trade agreement specified for this supply chain trade line item."},{"@id":"unece:specifiedLineTradeDelivery","@type":["rdf:Property","owl:ObjectProperty"],"rdfs:label":"specifiedLineTradeDelivery","schema:rangeIncludes":{"@id":"unece:LineTradeDelivery"},"schema:domainIncludes":{"@id":"unece:SupplyChainTradeLineItem"},"rdfs:comment":"The line trade delivery specified for this supply chain trade line item."},{"@id":"unece:specifiedLineTradeSettlement","@type":["rdf:Property","owl:ObjectProperty"],"rdfs:label":"specifiedLineTradeSettlement","schema:rangeIncludes":{"@id":"unece:LineTradeSettlement"},"schema:domainIncludes":{"@id":"unece:SupplyChainTradeLineItem"},"rdfs:comment":"A line trade settlement specified for this supply chain trade line item."},{"@id":"unece:specifiedProduction","@type":["rdf:Property","owl:ObjectProperty"],"rdfs:label":"specifiedProduction","schema:rangeIncludes":{"@id":"unece:Production"},"schema:domainIncludes":{"@id":"unece:SupplyChainTradeLineItem"},"rdfs:comment":"A production of goods specified for this supply chain trade line Item."},{"@id":"unece:specifiedTradeProduct","@type":["rdf:Property","owl:ObjectProperty"],"rdfs:label":"specifiedTradeProduct","schema:rangeIncludes":{"@id":"unece:TradeProduct"},"schema:domainIncludes":[{"@id":"unece:SupplyChainTradeLineItem"},{"@id":"unece:TradeParty"}],"rdfs:comment":"A product specified for this supply chain trade line item."},{"@id":"unece:substituteApplicableBatch","@type":["rdf:Property","owl:ObjectProperty"],"rdfs:label":"substituteApplicableBatch","schema:rangeIncludes":{"@id":"unece:ProductBatch"},"schema:domainIncludes":{"@id":"unece:SupplyChainTradeLineItem"},"rdfs:comment":"A substitute product batch applicable to this supply chain trade line item."},{"@id":"unece:substituteApplicableMaterial","@type":["rdf:Property","owl:ObjectProperty"],"rdfs:label":"substituteApplicableMaterial","schema:rangeIncludes":{"@id":"unece:SpecifiedMaterial"},"schema:domainIncludes":{"@id":"unece:SupplyChainTradeLineItem"},"rdfs:comment":"A substance from which something is or could be made."},{"@id":"unece:substituteApplicableProduct","@type":["rdf:Property","owl:ObjectProperty"],"rdfs:label":"substituteApplicableProduct","schema:rangeIncludes":{"@id":"unece:Product"},"schema:domainIncludes":{"@id":"unece:SupplyChainTradeLineItem"},"rdfs:comment":"A referenced substitute product applicable for this supply chain trade line item."},{"@id":"unece:substitutedApplicableBatch","@type":["rdf:Property","owl:ObjectProperty"],"rdfs:label":"substitutedApplicableBatch","schema:rangeIncludes":{"@id":"unece:ProductBatch"},"schema:domainIncludes":{"@id":"unece:SupplyChainTradeLineItem"},"rdfs:comment":"A substituted product batch applicable to this supply chain trade line item."},{"@id":"unece:substitutedApplicableMaterial","@type":["rdf:Property","owl:ObjectProperty"],"rdfs:label":"substitutedApplicableMaterial","schema:rangeIncludes":{"@id":"unece:SpecifiedMaterial"},"schema:domainIncludes":{"@id":"unece:SupplyChainTradeLineItem"},"rdfs:comment":"A substance from which something is or could be made."},{"@id":"unece:substitutedProduct","@type":["rdf:Property","owl:ObjectProperty"],"rdfs:label":"substitutedProduct","schema:rangeIncludes":{"@id":"unece:Product"},"schema:domainIncludes":[{"@id":"unece:SupplyChainTradeLineItem"},{"@id":"unece:TradeProduct"}],"rdfs:comment":"A referenced product substituted for this supply chain trade line item."},{"@id":"unece:typeCode","@type":["rdf:Property","owl:DatatypeProperty"],"rdfs:label":"typeCode","schema:rangeIncludes":{"@id":"schema:Text"},"schema:domainIncludes":[{"@id":"unece:SupplyChainTradeLineItem"},{"@id":"unece:TradeProduct"},{"@id":"unece:ProductionProcess"},{"@id":"unece:ProductBatch"},{"@id":"unece:ProductionFacility"},{"@id":"unece:SupplyChainTradeTransaction"},{"@id":"unece:Colour"},{"@id":"unece:ProductionUnit"},{"@id":"unece:Print"},{"@id":"unece:ProductionDevice"},{"@id":"unece:ProductFinishingTreatment"},{"@id":"unece:SpecifiedChemicalTreatment"},{"@id":"unece:Machine"},{"@id":"unece:TradeProductFeature"},{"@id":"unece:NegotiationContext"},{"@id":"unece:NegotiationExchange"},{"@id":"unece:Classification"},{"@id":"unece:SpecifiedAction"},{"@id":"unece:CountrySubDivision"},{"@id":"unece:Measurement"},{"@id":"unece:QuantityAnalysis"},{"@id":"unece:SpecifiedFault"},{"@id":"unece:RadioactiveMaterial"},{"@id":"unece:CommunicationEvent"},{"@id":"unece:LegalOrganization"},{"@id":"unece:Object"},{"@id":"unece:SpecifiedPeriod"},{"@id":"unece:Project"},{"@id":"unece:MetricCharacteristic"},{"@id":"unece:LegalRegistration"},{"@id":"unece:DocumentCharacteristic"},{"@id":"unece:Schedule"},{"@id":"unece:SpecifiedFeature"},{"@id":"unece:SpecifiedParameter"},{"@id":"unece:Range"},{"@id":"unece:GeopoliticalRegion"},{"@id":"unece:Issue"},{"@id":"unece:Segment"},{"@id":"unece:SecurityTag"},{"@id":"unece:SpecificationQuery"},{"@id":"unece:PaymentTradeSettlement"},{"@id":"unece:PaymentFinancialAccount"},{"@id":"unece:Cash"},{"@id":"unece:Cheque"},{"@id":"unece:DigitalMethod"},{"@id":"unece:FinancialCard"},{"@id":"unece:PaymentFinancialInstitution"},{"@id":"unece:BreakdownStatement"},{"@id":"unece:BasicWorkItem"},{"@id":"unece:GroupedWorkItem"},{"@id":"unece:Voucher"},{"@id":"unece:CustomsValuation"},{"@id":"unece:Accreditation"},{"@id":"unece:CorrectiveAction"},{"@id":"unece:PreventiveAction"},{"@id":"unece:Standard"},{"@id":"unece:ProcessWorkItem"},{"@id":"unece:ProductCharacteristic"},{"@id":"unece:ProductBatchCharacteristic"},{"@id":"unece:Chemical"},{"@id":"unece:SustainabilityCharacteristic"},{"@id":"unece:SustainabilityInspection"},{"@id":"unece:Assessment"},{"@id":"unece:TechnicalCharacteristic"},{"@id":"unece:Licence"},{"@id":"unece:SpecifiedDeclaration"},{"@id":"unece:SpecifiedInspection"},{"@id":"unece:GovernmentRegistration"},{"@id":"unece:ControlSettingParameter"},{"@id":"unece:OperationalParameter"},{"@id":"unece:InspectionEvent"},{"@id":"unece:ObservationObjectiveParameter"},{"@id":"unece:Requirement"},{"@id":"unece:ProductCharacteristicCondition"},{"@id":"unece:OrganizationCharacteristic"},{"@id":"unece:GoodsCharacteristic"},{"@id":"unece:SpecifiedMaterial"},{"@id":"unece:WasteMaterialRecoveryDisposalProcess"},{"@id":"unece:ProductionWasteMaterial"},{"@id":"unece:ProductionWasteMaterialComponent"},{"@id":"unece:ProductionWasteRecoveryDisposalProcess"},{"@id":"unece:ExperienceProgramAction"},{"@id":"unece:ExperienceFacility"},{"@id":"unece:Allergy"},{"@id":"unece:CarriedEquipment"},{"@id":"unece:Disability"},{"@id":"unece:FoodChoice"},{"@id":"unece:GuestHealthIndication"},{"@id":"unece:PersonalEffects"},{"@id":"unece:AgriculturalProcess"},{"@id":"unece:CropProtectionTreatment"},{"@id":"unece:CropProduceBatch"},{"@id":"unece:Produce"},{"@id":"unece:AgriculturalCharacteristic"},{"@id":"unece:AnimalHoldingEvent"},{"@id":"unece:TransportEvent"},{"@id":"unece:Emission"},{"@id":"unece:LogisticsPackaging"},{"@id":"unece:TransportationWasteMaterial"},{"@id":"unece:TransportationWasteMaterialComponent"},{"@id":"unece:SanitaryMeasure"},{"@id":"unece:MDHHealthIndication"},{"@id":"unece:IOTDevice"},{"@id":"unece:StoresItemInventory"},{"@id":"unece:TransportationWasteRecoveryDisposalProcess"},{"@id":"unece:Sensor"},{"@id":"unece:SupplyChainReference"},{"@id":"unece:SupplyChainEvent"},{"@id":"unece:Equipment"}],"rdfs:comment":"A code specifying a type of MDH health indication."},{"@id":"unece:typeExtensionCode","@type":["rdf:Property","owl:DatatypeProperty"],"rdfs:label":"typeExtensionCode","schema:rangeIncludes":{"@id":"schema:Text"},"schema:domainIncludes":{"@id":"unece:SupplyChainTradeLineItem"},"rdfs:comment":"The code used as an extension to the type code for further specifying a type of supply chain trade line item."},{"@id":"unece:acknowledgementDocumentReasonInformation","@type":["rdf:Property","owl:DatatypeProperty"],"rdfs:label":"acknowledgementDocumentReasonInformation","schema:rangeIncludes":{"@id":"schema:Text"},"schema:domainIncludes":{"@id":"unece:AcknowledgementDocument"},"rdfs:comment":"Reason information, expressed as text, for this acknowledgement document."},{"@id":"unece:acknowledgementDocumentStatusCode","@type":["rdf:Property","owl:DatatypeProperty"],"rdfs:label":"acknowledgementDocumentStatusCode","schema:rangeIncludes":{"@id":"unece:StatusCodeList"},"schema:domainIncludes":{"@id":"unece:AcknowledgementDocument"},"rdfs:comment":"A code specifying a status for this acknowledgement document."},{"@id":"unece:acknowledgementStatusCode","@type":["rdf:Property","owl:DatatypeProperty"],"rdfs:label":"acknowledgementStatusCode","schema:rangeIncludes":{"@id":"unece:AcknowledgementCodeList"},"schema:domainIncludes":{"@id":"unece:AcknowledgementDocument"},"rdfs:comment":"A code specifying an acknowledgment status for this acknowledgement document."},{"@id":"unece:channelCode","@type":["rdf:Property","owl:DatatypeProperty"],"rdfs:label":"channelCode","schema:rangeIncludes":{"@id":"schema:Text"},"schema:domainIncludes":{"@id":"unece:AcknowledgementDocument"},"rdfs:comment":"The code specifying the channel by which this acknowledgement document is sent, such as mail, email, fax."},{"@id":"unece:controlRequirementIndicator","@type":["rdf:Property","owl:DatatypeProperty"],"rdfs:label":"controlRequirementIndicator","schema:rangeIncludes":{"@id":"schema:Boolean"},"schema:domainIncludes":[{"@id":"unece:AcknowledgementDocument"},{"@id":"unece:ExchangedDocument"},{"@id":"unece:RegulatoryProcedure"}],"rdfs:comment":"The indication of whether or not a control is required for this cross-border regulatory procedure."},{"@id":"unece:creationDateTime","@type":["rdf:Property","owl:DatatypeProperty"],"rdfs:label":"creationDateTime","schema:rangeIncludes":{"@id":"schema:Text"},"schema:domainIncludes":[{"@id":"unece:AcknowledgementDocument"},{"@id":"unece:ProductBatch"},{"@id":"unece:ExchangedDocument"},{"@id":"unece:SpecifiedNote"},{"@id":"unece:PaymentTradeSettlement"},{"@id":"unece:FinancingRequestDocument"},{"@id":"unece:BreakdownStatement"},{"@id":"unece:CropProduceBatch"},{"@id":"unece:AnimalBatch"}],"rdfs:comment":"The creation date, time, date time, or other date time value for this payment trade settlement."},{"@id":"unece:documentTypeCode","@type":["rdf:Property","owl:DatatypeProperty"],"rdfs:label":"documentTypeCode","schema:rangeIncludes":{"@id":"unece:DocumentCodeList"},"schema:domainIncludes":[{"@id":"unece:AcknowledgementDocument"},{"@id":"unece:ExchangedDeclaration"},{"@id":"unece:Document"},{"@id":"unece:ExchangedDocument"}],"rdfs:comment":"A code specifying a type of acknowledgement document."},{"@id":"unece:issueDateTime","@type":["rdf:Property","owl:DatatypeProperty"],"rdfs:label":"issueDateTime","schema:rangeIncludes":{"@id":"schema:Text"},"schema:domainIncludes":[{"@id":"unece:AcknowledgementDocument"},{"@id":"unece:SupplyChainTradeTransaction"},{"@id":"unece:Contract"},{"@id":"unece:TTExchangedDocument"},{"@id":"unece:ExchangedDeclaration"},{"@id":"unece:DocumentLineDocument"},{"@id":"unece:Document"},{"@id":"unece:ExchangedDocument"},{"@id":"unece:Error"},{"@id":"unece:Version"},{"@id":"unece:Voucher"},{"@id":"unece:OrganizationalCertificate"},{"@id":"unece:ProcessCertificate"},{"@id":"unece:ProductBatchCertificate"},{"@id":"unece:ProductCertificate"},{"@id":"unece:SpecifiedCertificate"},{"@id":"unece:Licence"},{"@id":"unece:SpecifiedDeclaration"},{"@id":"unece:ConformanceCertificate"},{"@id":"unece:AgriculturalCertificate"}],"rdfs:comment":"An issue date, time, date time or other date time value for this declared error."},{"@id":"unece:itemIdentificationId","@type":["rdf:Property","owl:DatatypeProperty"],"rdfs:label":"itemIdentificationId","schema:rangeIncludes":{"@id":"schema:Text"},"schema:domainIncludes":{"@id":"unece:AcknowledgementDocument"},"rdfs:comment":"The unique identifier of an item in this acknowledgement document."},{"@id":"unece:multipleReferencesIndicator","@type":["rdf:Property","owl:DatatypeProperty"],"rdfs:label":"multipleReferencesIndicator","schema:rangeIncludes":{"@id":"schema:Boolean"},"schema:domainIncludes":{"@id":"unece:AcknowledgementDocument"},"rdfs:comment":"The indication of whether or not this acknowledgement document has multiple references."},{"@id":"unece:name","@type":["rdf:Property","owl:DatatypeProperty"],"rdfs:label":"name","schema:rangeIncludes":{"@id":"schema:Text"},"schema:domainIncludes":[{"@id":"unece:AcknowledgementDocument"},{"@id":"unece:TradeProduct"},{"@id":"unece:ProductionProcess"},{"@id":"unece:TradeParty"},{"@id":"unece:ProductBatch"},{"@id":"unece:ProductionFacility"},{"@id":"unece:Colour"},{"@id":"unece:ProductionUnit"},{"@id":"unece:Print"},{"@id":"unece:ProductionCycle"},{"@id":"unece:ProductLabel"},{"@id":"unece:Contract"},{"@id":"unece:Product"},{"@id":"unece:TradeLocation"},{"@id":"unece:TTLocation"},{"@id":"unece:TradeProductFeature"},{"@id":"unece:Marketplace"},{"@id":"unece:ProductGroup"},{"@id":"unece:TTParty"},{"@id":"unece:Document"},{"@id":"unece:ExchangedDocument"},{"@id":"unece:CountrySubDivision"},{"@id":"unece:RadioactiveIsotope"},{"@id":"unece:SpecifiedMethod"},{"@id":"unece:Location"},{"@id":"unece:LegalOrganization"},{"@id":"unece:DirectPosition"},{"@id":"unece:DirectPositionList"},{"@id":"unece:InformationSource"},{"@id":"unece:GeographicalFeature"},{"@id":"unece:SpecifiedPeriod"},{"@id":"unece:Project"},{"@id":"unece:SpecifiedNote"},{"@id":"unece:Country"},{"@id":"unece:DocumentCharacteristic"},{"@id":"unece:GeographicalObjectCharacteristic"},{"@id":"unece:Membership"},{"@id":"unece:SpecifiedLocation"},{"@id":"unece:SpecifiedParameter"},{"@id":"unece:CoordinateReferenceSystem"},{"@id":"unece:GeopoliticalRegion"},{"@id":"unece:Radionuclide"},{"@id":"unece:SubordinateLocation"},{"@id":"unece:SubordinateSubordinateLocation"},{"@id":"unece:Version"},{"@id":"unece:CooperatingOrganization"},{"@id":"unece:Keyword"},{"@id":"unece:AccountingAccount"},{"@id":"unece:CreditorFinancialInstitution"},{"@id":"unece:DebtorFinancialInstitution"},{"@id":"unece:PaymentFinancialInstitution"},{"@id":"unece:BreakdownStatement"},{"@id":"unece:BranchFinancialInstitution"},{"@id":"unece:RequestingParty"},{"@id":"unece:AcademicQualification"},{"@id":"unece:SpecifiedCertificate"},{"@id":"unece:Standard"},{"@id":"unece:SustainabilityInspection"},{"@id":"unece:AppliedChemicalTreatment"},{"@id":"unece:Assessment"},{"@id":"unece:Licence"},{"@id":"unece:SpecifiedDeclaration"},{"@id":"unece:SpecifiedInspection"},{"@id":"unece:AuthoritativeSignatoryPerson"},{"@id":"unece:Source"},{"@id":"unece:LaboratoryObservationAnalysisMethod"},{"@id":"unece:ControlSettingParameter"},{"@id":"unece:OperationalParameter"},{"@id":"unece:ObservationObjectiveParameter"},{"@id":"unece:LaboratoryObservationParty"},{"@id":"unece:ProductCharacteristicCondition"},{"@id":"unece:SpecifiedQualification"},{"@id":"unece:SpecifiedMaterial"},{"@id":"unece:GuestPerson"},{"@id":"unece:ExperienceItem"},{"@id":"unece:ExperienceProduct"},{"@id":"unece:ExperienceEvent"},{"@id":"unece:ExperienceFacility"},{"@id":"unece:Allergy"},{"@id":"unece:CarriedEquipment"},{"@id":"unece:Disability"},{"@id":"unece:FoodChoice"},{"@id":"unece:Area"},{"@id":"unece:Produce"},{"@id":"unece:Service"},{"@id":"unece:TransportMovement"},{"@id":"unece:LogisticsTransportMeans"},{"@id":"unece:LogisticsLocation"},{"@id":"unece:TransportMeans"},{"@id":"unece:TransportServiceLocation"},{"@id":"unece:SpecifiedCondition"},{"@id":"unece:LocationParty"}],"rdfs:comment":"A name or symbol, expressed as text, of a radioactive radionuclide."},{"@id":"unece:processCondition","@type":["rdf:Property","owl:DatatypeProperty"],"rdfs:label":"processCondition","schema:rangeIncludes":{"@id":"schema:Text"},"schema:domainIncludes":[{"@id":"unece:AcknowledgementDocument"},{"@id":"unece:Document"},{"@id":"unece:DocumentStatus"}],"rdfs:comment":"A process condition, expressed as text, for this acknowledgement document."},{"@id":"unece:processConditionCode","@type":["rdf:Property","owl:DatatypeProperty"],"rdfs:label":"processConditionCode","schema:rangeIncludes":{"@id":"schema:Text"},"schema:domainIncludes":[{"@id":"unece:AcknowledgementDocument"},{"@id":"unece:Document"},{"@id":"unece:DocumentStatus"}],"rdfs:comment":"The code specifying the process condition for this acknowledgement document."},{"@id":"unece:reportReceiptDateTime","@type":["rdf:Property","owl:DatatypeProperty"],"rdfs:label":"reportReceiptDateTime","schema:rangeIncludes":{"@id":"schema:Text"},"schema:domainIncludes":{"@id":"unece:AcknowledgementDocument"},"rdfs:comment":"The date, time, date time or other date time value of the receipt of the report being acknowledged by this acknowledgment document."},{"@id":"unece:reportSubmissionDateTime","@type":["rdf:Property","owl:DatatypeProperty"],"rdfs:label":"reportSubmissionDateTime","schema:rangeIncludes":{"@id":"schema:Text"},"schema:domainIncludes":{"@id":"unece:AcknowledgementDocument"},"rdfs:comment":"The date, time, date time or other date time value of the submission of the report being acknowledged by this acknowledgment document."},{"@id":"unece:status","@type":["rdf:Property","owl:DatatypeProperty"],"rdfs:label":"status","schema:rangeIncludes":{"@id":"schema:Text"},"schema:domainIncludes":[{"@id":"unece:AcknowledgementDocument"},{"@id":"unece:ProductionProcess"},{"@id":"unece:Document"},{"@id":"unece:InspectionReference"},{"@id":"unece:LaboratoryObservationReference"},{"@id":"unece:GuestHealthIndication"},{"@id":"unece:SupplyChainReference"}],"rdfs:comment":"A status, expressed as text, for this acknowledgement document."},{"@id":"unece:actionCode","@type":["rdf:Property","owl:DatatypeProperty"],"rdfs:label":"actionCode","schema:rangeIncludes":{"@id":"schema:Text"},"schema:domainIncludes":[{"@id":"unece:TTAggregationEvent"},{"@id":"unece:TTObjectEvent"},{"@id":"unece:TTTransactionEvent"},{"@id":"unece:SpecifiedCondition"}],"rdfs:comment":"A code specifying an action for this specified condition."},{"@id":"unece:businessStepCode","@type":["rdf:Property","owl:DatatypeProperty"],"rdfs:label":"businessStepCode","schema:rangeIncludes":{"@id":"schema:Text"},"schema:domainIncludes":[{"@id":"unece:TTAggregationEvent"},{"@id":"unece:TTObjectEvent"},{"@id":"unece:TTTransactionEvent"},{"@id":"unece:TTTransformationEvent"}],"rdfs:comment":"The code specifying the business step for this TT aggregation event."},{"@id":"unece:childObjectInstanceId","@type":["rdf:Property","owl:DatatypeProperty"],"rdfs:label":"childObjectInstanceId","schema:rangeIncludes":{"@id":"schema:Text"},"schema:domainIncludes":{"@id":"unece:TTAggregationEvent"},"rdfs:comment":"An instance identifier for a child object of this TT aggregation event."},{"@id":"unece:childQuantitySpecifiedEventElement","@type":["rdf:Property","owl:ObjectProperty"],"rdfs:label":"childQuantitySpecifiedEventElement","schema:rangeIncludes":{"@id":"unece:EventElement"},"schema:domainIncludes":{"@id":"unece:TTAggregationEvent"},"rdfs:comment":"Information about an event in which a Track and Trace (TT) element of one of more physical or digital objects is identified by a specific object class identifier (such as an electronic product class), either a specific quantity or an unspecified quantity."},{"@id":"unece:destinationRelatedParty","@type":["rdf:Property","owl:ObjectProperty"],"rdfs:label":"destinationRelatedParty","schema:rangeIncludes":{"@id":"unece:TTParty"},"schema:domainIncludes":[{"@id":"unece:TTAggregationEvent"},{"@id":"unece:TTObjectEvent"},{"@id":"unece:TTTransactionEvent"},{"@id":"unece:TTTransformationEvent"}],"rdfs:comment":"A destination related party for this TT aggregation event."},{"@id":"unece:dispositionCode","@type":["rdf:Property","owl:DatatypeProperty"],"rdfs:label":"dispositionCode","schema:rangeIncludes":{"@id":"schema:Text"},"schema:domainIncludes":[{"@id":"unece:TTAggregationEvent"},{"@id":"unece:TTObjectEvent"},{"@id":"unece:TTTransactionEvent"},{"@id":"unece:TTTransformationEvent"}],"rdfs:comment":"The code specifying the disposition related to this TT aggregation event."},{"@id":"unece:occurrenceDateTime","@type":["rdf:Property","owl:DatatypeProperty"],"rdfs:label":"occurrenceDateTime","schema:rangeIncludes":{"@id":"schema:Text"},"schema:domainIncludes":[{"@id":"unece:TTAggregationEvent"},{"@id":"unece:TTObjectEvent"},{"@id":"unece:TTTransactionEvent"},{"@id":"unece:ProductionProcess"},{"@id":"unece:TTTransformationEvent"},{"@id":"unece:CommunicationEvent"},{"@id":"unece:Schedule"},{"@id":"unece:HeaderBalanceOut"},{"@id":"unece:PaymentBalanceOut"},{"@id":"unece:AppliedChemicalTreatment"},{"@id":"unece:InspectionEvent"},{"@id":"unece:AnimalHoldingEvent"},{"@id":"unece:SupplyChainEvent"}],"rdfs:comment":"A date, time, date time, or other date time of an occurrence in this supply chain schedule."},{"@id":"unece:parentObjectId","@type":["rdf:Property","owl:DatatypeProperty"],"rdfs:label":"parentObjectId","schema:rangeIncludes":{"@id":"schema:Text"},"schema:domainIncludes":[{"@id":"unece:TTAggregationEvent"},{"@id":"unece:TTTransactionEvent"}],"rdfs:comment":"The identifier of the parent object for this TT aggregation event."},{"@id":"unece:readPointRelatedLocation","@type":["rdf:Property","owl:ObjectProperty"],"rdfs:label":"readPointRelatedLocation","schema:rangeIncludes":{"@id":"unece:TTLocation"},"schema:domainIncludes":[{"@id":"unece:TTAggregationEvent"},{"@id":"unece:TTObjectEvent"},{"@id":"unece:TTTransactionEvent"},{"@id":"unece:TTTransformationEvent"}],"rdfs:comment":"The read point related location of this TT aggregation event."},{"@id":"unece:recordedDateTime","@type":["rdf:Property","owl:DatatypeProperty"],"rdfs:label":"recordedDateTime","schema:rangeIncludes":{"@id":"schema:Text"},"schema:domainIncludes":[{"@id":"unece:TTAggregationEvent"},{"@id":"unece:TTObjectEvent"},{"@id":"unece:TTTransactionEvent"},{"@id":"unece:TTTransformationEvent"}],"rdfs:comment":"The date, time, date time, or other date time value at which this TT aggregation event was recorded."},{"@id":"unece:relatedCertification","@type":["rdf:Property","owl:ObjectProperty"],"rdfs:label":"relatedCertification","schema:rangeIncludes":{"@id":"unece:SpecifiedCertification"},"schema:domainIncludes":[{"@id":"unece:TTAggregationEvent"},{"@id":"unece:TTObjectEvent"},{"@id":"unece:TTTransactionEvent"},{"@id":"unece:TTTransformationEvent"}],"rdfs:comment":"The process of certifying that a certain product, process or organization has passed performance tests, or qualification requirements stipulated in a standard or regulation."},{"@id":"unece:relatedTTLocation","@type":["rdf:Property","owl:ObjectProperty"],"rdfs:label":"relatedTTLocation","schema:rangeIncludes":{"@id":"unece:TTLocation"},"schema:domainIncludes":[{"@id":"unece:TTAggregationEvent"},{"@id":"unece:TTAnimal"}],"rdfs:comment":"A location related to this TT animal."},{"@id":"unece:sourceRelatedParty","@type":["rdf:Property","owl:ObjectProperty"],"rdfs:label":"sourceRelatedParty","schema:rangeIncludes":{"@id":"unece:TTParty"},"schema:domainIncludes":[{"@id":"unece:TTAggregationEvent"},{"@id":"unece:TTObjectEvent"},{"@id":"unece:TTTransactionEvent"},{"@id":"unece:TTTransformationEvent"}],"rdfs:comment":"A source related party for this TT aggregation event."},{"@id":"unece:specifiedError","@type":["rdf:Property","owl:ObjectProperty"],"rdfs:label":"specifiedError","schema:rangeIncludes":{"@id":"unece:Error"},"schema:domainIncludes":[{"@id":"unece:TTAggregationEvent"},{"@id":"unece:TTObjectEvent"},{"@id":"unece:TTTransactionEvent"},{"@id":"unece:TTTransformationEvent"}],"rdfs:comment":"A notification that an error has occurred."},{"@id":"unece:specifiedTradeTransaction","@type":["rdf:Property","owl:ObjectProperty"],"rdfs:label":"specifiedTradeTransaction","schema:rangeIncludes":{"@id":"unece:TTTradeTransaction"},"schema:domainIncludes":[{"@id":"unece:TTAggregationEvent"},{"@id":"unece:TTObjectEvent"},{"@id":"unece:TTTransactionEvent"},{"@id":"unece:TTTransformationEvent"}],"rdfs:comment":"A trade transaction specified for this TT aggregation event."},{"@id":"unece:businessRelatedLocation","@type":["rdf:Property","owl:ObjectProperty"],"rdfs:label":"businessRelatedLocation","schema:rangeIncludes":{"@id":"unece:TTLocation"},"schema:domainIncludes":[{"@id":"unece:TTObjectEvent"},{"@id":"unece:TTTransactionEvent"},{"@id":"unece:TTTransformationEvent"}],"rdfs:comment":"The business location related to this TT object event."},{"@id":"unece:objectInstanceId","@type":["rdf:Property","owl:DatatypeProperty"],"rdfs:label":"objectInstanceId","schema:rangeIncludes":{"@id":"schema:Text"},"schema:domainIncludes":[{"@id":"unece:TTObjectEvent"},{"@id":"unece:TTTransactionEvent"}],"rdfs:comment":"An instance identifier for an object of this TT object event."},{"@id":"unece:quantitySpecifiedEventElement","@type":["rdf:Property","owl:ObjectProperty"],"rdfs:label":"quantitySpecifiedEventElement","schema:rangeIncludes":{"@id":"unece:EventElement"},"schema:domainIncludes":[{"@id":"unece:TTObjectEvent"},{"@id":"unece:TTTransactionEvent"}],"rdfs:comment":"Information about an event in which a Track and Trace (TT) element of one of more physical or digital objects is identified by a specific object class identifier (such as an electronic product class), either a specific quantity or an unspecified quantity."},{"@id":"unece:actualQuantity","@type":["rdf:Property","owl:ObjectProperty"],"rdfs:label":"actualQuantity","schema:rangeIncludes":{"@id":"unece:QuantityType"},"schema:domainIncludes":[{"@id":"unece:ProductInstance"},{"@id":"unece:SupplyPlan"},{"@id":"unece:QuantityAnalysis"},{"@id":"unece:FinancialAdjustment"},{"@id":"unece:DeliveryAdjustment"}],"rdfs:comment":""},{"@id":"unece:applicableGoodsCharacteristic","@type":["rdf:Property","owl:ObjectProperty"],"rdfs:label":"applicableGoodsCharacteristic","schema:rangeIncludes":{"@id":"unece:GoodsCharacteristic"},"schema:domainIncludes":[{"@id":"unece:ProductInstance"},{"@id":"unece:TradeProduct"},{"@id":"unece:SpecifiedMaterial"},{"@id":"unece:SupplyChainPackaging"}],"rdfs:comment":"A distinctive feature of a material contained within physical goods."},{"@id":"unece:applicableProductCharacteristic","@type":["rdf:Property","owl:ObjectProperty"],"rdfs:label":"applicableProductCharacteristic","schema:rangeIncludes":{"@id":"unece:ProductCharacteristic"},"schema:domainIncludes":[{"@id":"unece:ProductInstance"},{"@id":"unece:TradeProduct"},{"@id":"unece:ProductBatchCertificate"},{"@id":"unece:ProductCertificate"},{"@id":"unece:Chemical"},{"@id":"unece:HazardousMaterial"},{"@id":"unece:SpecifiedMaterial"}],"rdfs:comment":"A prominent attribute or aspect of a product."},{"@id":"unece:batchId","@type":["rdf:Property","owl:DatatypeProperty"],"rdfs:label":"batchId","schema:rangeIncludes":{"@id":"schema:Text"},"schema:domainIncludes":[{"@id":"unece:ProductInstance"},{"@id":"unece:TradeProduct"}],"rdfs:comment":"A batch identifier for this trade product."},{"@id":"unece:bestBeforeDateTime","@type":["rdf:Property","owl:DatatypeProperty"],"rdfs:label":"bestBeforeDateTime","schema:rangeIncludes":{"@id":"schema:Text"},"schema:domainIncludes":{"@id":"unece:ProductInstance"},"rdfs:comment":"The date, time, date time, or other date time value before which it is best to consume the items contained in this trade product instance."},{"@id":"unece:ceramicCapacitorId","@type":["rdf:Property","owl:DatatypeProperty"],"rdfs:label":"ceramicCapacitorId","schema:rangeIncludes":{"@id":"schema:Text"},"schema:domainIncludes":{"@id":"unece:ProductInstance"},"rdfs:comment":"The ceramic capacitor identifier of this trade product instance."},{"@id":"unece:dNAMarkerId","@type":["rdf:Property","owl:DatatypeProperty"],"rdfs:label":"dNAMarkerId","schema:rangeIncludes":{"@id":"schema:Text"},"schema:domainIncludes":[{"@id":"unece:ProductInstance"},{"@id":"unece:TradeProduct"},{"@id":"unece:ProductBatch"}],"rdfs:comment":"The DNA marker identifier of this product batch."},{"@id":"unece:ePCId","@type":["rdf:Property","owl:DatatypeProperty"],"rdfs:label":"ePCId","schema:rangeIncludes":{"@id":"schema:Text"},"schema:domainIncludes":[{"@id":"unece:ProductInstance"},{"@id":"unece:TradeProduct"}],"rdfs:comment":"The EPC (Electronic Product Code) identifier of this trade product instance."},{"@id":"unece:expiryDateTime","@type":["rdf:Property","owl:DatatypeProperty"],"rdfs:label":"expiryDateTime","schema:rangeIncludes":{"@id":"schema:Text"},"schema:domainIncludes":[{"@id":"unece:ProductInstance"},{"@id":"unece:DigitalMethod"},{"@id":"unece:FinancialCard"},{"@id":"unece:TradePrice"},{"@id":"unece:Accreditation"},{"@id":"unece:OrganizationalCertificate"},{"@id":"unece:ProcessCertificate"},{"@id":"unece:ProductBatchCertificate"},{"@id":"unece:ProductCertificate"},{"@id":"unece:SpecifiedCertificate"},{"@id":"unece:Licence"},{"@id":"unece:AgriculturalCertificate"}],"rdfs:comment":"An expiry date, time, date time or other date time value for this specified licence."},{"@id":"unece:globalSerialId","@type":["rdf:Property","owl:DatatypeProperty"],"rdfs:label":"globalSerialId","schema:rangeIncludes":{"@id":"schema:Text"},"schema:domainIncludes":{"@id":"unece:ProductInstance"},"rdfs:comment":"The unique global serial identifier for this trade product instance."},{"@id":"unece:inspectionEvent","@type":["rdf:Property","owl:ObjectProperty"],"rdfs:label":"inspectionEvent","schema:rangeIncludes":{"@id":"unece:SupplyChainEvent"},"schema:domainIncludes":[{"@id":"unece:ProductInstance"},{"@id":"unece:LogisticsLocation"}],"rdfs:comment":"A significant occurrence or happening in a supply chain."},{"@id":"unece:kanbanId","@type":["rdf:Property","owl:DatatypeProperty"],"rdfs:label":"kanbanId","schema:rangeIncludes":{"@id":"schema:Text"},"schema:domainIncludes":{"@id":"unece:ProductInstance"},"rdfs:comment":"The unique kanban identifier for this trade product instance."},{"@id":"unece:lotId","@type":["rdf:Property","owl:DatatypeProperty"],"rdfs:label":"lotId","schema:rangeIncludes":{"@id":"schema:Text"},"schema:domainIncludes":{"@id":"unece:ProductInstance"},"rdfs:comment":"The unique lot identifier for this trade product instance."},{"@id":"unece:manufacturerAssignedSerialId","@type":["rdf:Property","owl:DatatypeProperty"],"rdfs:label":"manufacturerAssignedSerialId","schema:rangeIncludes":{"@id":"schema:Text"},"schema:domainIncludes":{"@id":"unece:ProductInstance"},"rdfs:comment":"The unique manufacturer assigned serial identifier for this trade product instance."},{"@id":"unece:originLocation","@type":["rdf:Property","owl:ObjectProperty"],"rdfs:label":"originLocation","schema:rangeIncludes":{"@id":"unece:LogisticsLocation"},"schema:domainIncludes":[{"@id":"unece:ProductInstance"},{"@id":"unece:TradeProduct"}],"rdfs:comment":"A logistics related physical location or place."},{"@id":"unece:packagingEvent","@type":["rdf:Property","owl:ObjectProperty"],"rdfs:label":"packagingEvent","schema:rangeIncludes":{"@id":"unece:SupplyChainEvent"},"schema:domainIncludes":{"@id":"unece:ProductInstance"},"rdfs:comment":"A significant occurrence or happening in a supply chain."},{"@id":"unece:productionEvent","@type":["rdf:Property","owl:ObjectProperty"],"rdfs:label":"productionEvent","schema:rangeIncludes":{"@id":"unece:SupplyChainEvent"},"schema:domainIncludes":{"@id":"unece:ProductInstance"},"rdfs:comment":"A significant occurrence or happening in a supply chain."},{"@id":"unece:registrationId","@type":["rdf:Property","owl:DatatypeProperty"],"rdfs:label":"registrationId","schema:rangeIncludes":{"@id":"schema:Text"},"schema:domainIncludes":{"@id":"unece:ProductInstance"},"rdfs:comment":"A unique registration identifier, such as a vehicle licence plate identification, for this trade product instance."},{"@id":"unece:sellByDateTime","@type":["rdf:Property","owl:DatatypeProperty"],"rdfs:label":"sellByDateTime","schema:rangeIncludes":{"@id":"schema:Text"},"schema:domainIncludes":{"@id":"unece:ProductInstance"},"rdfs:comment":"The date, time, date time, or other date time value by after which the items contained in the trade product instance should not be sold."},{"@id":"unece:serialId","@type":["rdf:Property","owl:DatatypeProperty"],"rdfs:label":"serialId","schema:rangeIncludes":{"@id":"schema:Text"},"schema:domainIncludes":{"@id":"unece:ProductInstance"},"rdfs:comment":"A unique serial identifier for this trade product instance."},{"@id":"unece:supplierAssignedSerialId","@type":["rdf:Property","owl:DatatypeProperty"],"rdfs:label":"supplierAssignedSerialId","schema:rangeIncludes":{"@id":"schema:Text"},"schema:domainIncludes":{"@id":"unece:ProductInstance"},"rdfs:comment":"The unique supplier assigned serial identifier for this trade product instance."},{"@id":"unece:applicablePeriod","@type":["rdf:Property","owl:ObjectProperty"],"rdfs:label":"applicablePeriod","schema:rangeIncludes":{"@id":"unece:SpecifiedPeriod"},"schema:domainIncludes":[{"@id":"unece:SupplyPlan"},{"@id":"unece:TradeProduct"},{"@id":"unece:ProductionProcess"},{"@id":"unece:ProductBatch"},{"@id":"unece:SupplyChainTradeTransaction"},{"@id":"unece:RegulatoryProcedure"},{"@id":"unece:ExperienceItem"}],"rdfs:comment":"A specified period of time."},{"@id":"unece:contractDocument","@type":["rdf:Property","owl:ObjectProperty"],"rdfs:label":"contractDocument","schema:rangeIncludes":{"@id":"unece:Document"},"schema:domainIncludes":[{"@id":"unece:SupplyPlan"},{"@id":"unece:HeaderTradeAgreement"},{"@id":"unece:LineTradeAgreement"}],"rdfs:comment":"Written, printed or electronic matter that is referenced."},{"@id":"unece:deliverySupplyChainEvent","@type":["rdf:Property","owl:ObjectProperty"],"rdfs:label":"deliverySupplyChainEvent","schema:rangeIncludes":{"@id":"unece:SupplyChainEvent"},"schema:domainIncludes":{"@id":"unece:SupplyPlan"},"rdfs:comment":"A significant occurrence or happening in a supply chain."},{"@id":"unece:minusToleranceQuantity","@type":["rdf:Property","owl:ObjectProperty"],"rdfs:label":"minusToleranceQuantity","schema:rangeIncludes":{"@id":"unece:QuantityType"},"schema:domainIncludes":{"@id":"unece:SupplyPlan"},"rdfs:comment":""},{"@id":"unece:plannedQuantity","@type":["rdf:Property","owl:ObjectProperty"],"rdfs:label":"plannedQuantity","schema:rangeIncludes":{"@id":"unece:QuantityType"},"schema:domainIncludes":{"@id":"unece:SupplyPlan"},"rdfs:comment":""},{"@id":"unece:plusToleranceQuantity","@type":["rdf:Property","owl:ObjectProperty"],"rdfs:label":"plusToleranceQuantity","schema:rangeIncludes":{"@id":"unece:QuantityType"},"schema:domainIncludes":{"@id":"unece:SupplyPlan"},"rdfs:comment":""},{"@id":"unece:scheduledDeliveryEvent","@type":["rdf:Property","owl:ObjectProperty"],"rdfs:label":"scheduledDeliveryEvent","schema:rangeIncludes":{"@id":"unece:SupplyChainEvent"},"schema:domainIncludes":{"@id":"unece:SupplyPlan"},"rdfs:comment":"A significant occurrence or happening in a supply chain."},{"@id":"unece:specifiedLogisticsLocation","@type":["rdf:Property","owl:ObjectProperty"],"rdfs:label":"specifiedLogisticsLocation","schema:rangeIncludes":{"@id":"unece:LogisticsLocation"},"schema:domainIncludes":[{"@id":"unece:SupplyPlan"},{"@id":"unece:TradeParty"},{"@id":"unece:SupplyChainInventory"},{"@id":"unece:LogisticsStatus"},{"@id":"unece:StoresItemInventory"}],"rdfs:comment":"A logistics related physical location or place."},{"@id":"unece:supplyChainSupplyPlanCommitmentLevelCode","@type":["rdf:Property","owl:DatatypeProperty"],"rdfs:label":"supplyChainSupplyPlanCommitmentLevelCode","schema:rangeIncludes":{"@id":"unece:CommitmentLevelCodeList"},"schema:domainIncludes":{"@id":"unece:SupplyPlan"},"rdfs:comment":"The code specifying the commitment level for this supply chain supply plan, such as fabrication or raw material."},{"@id":"unece:synchronizationDateTime","@type":["rdf:Property","owl:DatatypeProperty"],"rdfs:label":"synchronizationDateTime","schema:rangeIncludes":{"@id":"schema:Text"},"schema:domainIncludes":{"@id":"unece:SupplyPlan"},"rdfs:comment":"A date, time, date time, or other date time value of a synchronization of the supply chain supply plan."},{"@id":"unece:synchronizationQuantity","@type":["rdf:Property","owl:ObjectProperty"],"rdfs:label":"synchronizationQuantity","schema:rangeIncludes":{"@id":"unece:QuantityType"},"schema:domainIncludes":{"@id":"unece:SupplyPlan"},"rdfs:comment":""},{"@id":"unece:toleranceQuantity","@type":["rdf:Property","owl:ObjectProperty"],"rdfs:label":"toleranceQuantity","schema:rangeIncludes":{"@id":"unece:QuantityType"},"schema:domainIncludes":{"@id":"unece:SupplyPlan"},"rdfs:comment":""},{"@id":"unece:additionalDescription","@type":["rdf:Property","owl:DatatypeProperty"],"rdfs:label":"additionalDescription","schema:rangeIncludes":{"@id":"schema:Text"},"schema:domainIncludes":[{"@id":"unece:TradeProduct"},{"@id":"unece:Picture"},{"@id":"unece:PaymentTradeSettlement"}],"rdfs:comment":"An additional textual description for this trade product."},{"@id":"unece:additionalReferenceDocument","@type":["rdf:Property","owl:ObjectProperty"],"rdfs:label":"additionalReferenceDocument","schema:rangeIncludes":{"@id":"unece:Document"},"schema:domainIncludes":{"@id":"unece:TradeProduct"},"rdfs:comment":"Written, printed or electronic matter that is referenced."},{"@id":"unece:applicableAssessment","@type":["rdf:Property","owl:ObjectProperty"],"rdfs:label":"applicableAssessment","schema:rangeIncludes":{"@id":"unece:Assessment"},"schema:domainIncludes":[{"@id":"unece:TradeProduct"},{"@id":"unece:ProductionProcess"},{"@id":"unece:TradeParty"},{"@id":"unece:ProductBatch"},{"@id":"unece:ProductionFacility"},{"@id":"unece:Standard"},{"@id":"unece:SpecifiedMaterial"}],"rdfs:comment":"The evaluation of an object, such as a product, process, or organization, with respect to the object's worth or condition."},{"@id":"unece:applicableDeclaration","@type":["rdf:Property","owl:ObjectProperty"],"rdfs:label":"applicableDeclaration","schema:rangeIncludes":{"@id":"unece:SpecifiedDeclaration"},"schema:domainIncludes":[{"@id":"unece:TradeProduct"},{"@id":"unece:ProductionProcess"},{"@id":"unece:TradeParty"},{"@id":"unece:Standard"}],"rdfs:comment":"An act of notification by formal documentation or action, in any form prescribed or accepted, such as a self-declaration."},{"@id":"unece:applicableDisposalInstructions","@type":["rdf:Property","owl:ObjectProperty"],"rdfs:label":"applicableDisposalInstructions","schema:rangeIncludes":{"@id":"unece:DisposalInstructions"},"schema:domainIncludes":[{"@id":"unece:TradeProduct"},{"@id":"unece:ProductBatch"},{"@id":"unece:SupplyChainPackaging"}],"rdfs:comment":"A set of instructions detailing how to properly dispose of a material."},{"@id":"unece:applicableFault","@type":["rdf:Property","owl:ObjectProperty"],"rdfs:label":"applicableFault","schema:rangeIncludes":{"@id":"unece:SpecifiedFault"},"schema:domainIncludes":[{"@id":"unece:TradeProduct"},{"@id":"unece:ProductionProcess"},{"@id":"unece:ProductBatch"}],"rdfs:comment":"An unattractive or unsatisfactory characteristic."},{"@id":"unece:applicableKeyword","@type":["rdf:Property","owl:ObjectProperty"],"rdfs:label":"applicableKeyword","schema:rangeIncludes":{"@id":"unece:Keyword"},"schema:domainIncludes":{"@id":"unece:TradeProduct"},"rdfs:comment":"A significant word, part of word or phrase that is used to enable indexing of or searching within a textual repository, such as a product catalogue or library."},{"@id":"unece:applicableLicence","@type":["rdf:Property","owl:ObjectProperty"],"rdfs:label":"applicableLicence","schema:rangeIncludes":{"@id":"unece:Licence"},"schema:domainIncludes":[{"@id":"unece:TradeProduct"},{"@id":"unece:ProductionProcess"},{"@id":"unece:TradeParty"},{"@id":"unece:Standard"}],"rdfs:comment":"A permit from an authority to own or use something, do a particular thing, or to conduct a trade."},{"@id":"unece:applicableLogisticsPackaging","@type":["rdf:Property","owl:ObjectProperty"],"rdfs:label":"applicableLogisticsPackaging","schema:rangeIncludes":{"@id":"unece:LogisticsPackaging"},"schema:domainIncludes":{"@id":"unece:TradeProduct"},"rdfs:comment":"Any wrapping or containment, such as a box or a barrel, whether or not any goods are contained within."},{"@id":"unece:applicableProductionProcess","@type":["rdf:Property","owl:ObjectProperty"],"rdfs:label":"applicableProductionProcess","schema:rangeIncludes":{"@id":"unece:ProductionProcess"},"schema:domainIncludes":[{"@id":"unece:TradeProduct"},{"@id":"unece:ProductionUnit"},{"@id":"unece:ProductionCycle"}],"rdfs:comment":"A process applicable to this specified production cycle."},{"@id":"unece:applicableSpecifiedCertificate","@type":["rdf:Property","owl:ObjectProperty"],"rdfs:label":"applicableSpecifiedCertificate","schema:rangeIncludes":{"@id":"unece:SpecifiedCertificate"},"schema:domainIncludes":[{"@id":"unece:TradeProduct"},{"@id":"unece:ProductionProcess"},{"@id":"unece:TradeParty"},{"@id":"unece:ProductBatch"},{"@id":"unece:ProductionFacility"},{"@id":"unece:Standard"},{"@id":"unece:SpecifiedMaterial"}],"rdfs:comment":"A document issued by a government, public organization or association to certify a property of a person, entity, process or object."},{"@id":"unece:applicableSpecifiedInspection","@type":["rdf:Property","owl:ObjectProperty"],"rdfs:label":"applicableSpecifiedInspection","schema:rangeIncludes":{"@id":"unece:SpecifiedInspection"},"schema:domainIncludes":[{"@id":"unece:TradeProduct"},{"@id":"unece:ProductionProcess"},{"@id":"unece:TradeParty"},{"@id":"unece:ProductBatch"},{"@id":"unece:ProductionFacility"},{"@id":"unece:TransportMovement"}],"rdfs:comment":"The process of performing documented checks, such as on materials or processes, with a focus on discovering deviations, errors or faults related to documented requirements."},{"@id":"unece:applicableSupplyChainPackaging","@type":["rdf:Property","owl:ObjectProperty"],"rdfs:label":"applicableSupplyChainPackaging","schema:rangeIncludes":{"@id":"unece:SupplyChainPackaging"},"schema:domainIncludes":[{"@id":"unece:TradeProduct"},{"@id":"unece:ProductBatch"}],"rdfs:comment":"Any material with which supply chain goods are packaged, such as a box or bubble wrap."},{"@id":"unece:applicableSustainabilityCharacteristic","@type":["rdf:Property","owl:ObjectProperty"],"rdfs:label":"applicableSustainabilityCharacteristic","schema:rangeIncludes":{"@id":"unece:SustainabilityCharacteristic"},"schema:domainIncludes":[{"@id":"unece:TradeProduct"},{"@id":"unece:ProductionProcess"},{"@id":"unece:TradeParty"},{"@id":"unece:ProductionFacility"},{"@id":"unece:ProductionUnit"},{"@id":"unece:ProductFinishingTreatment"},{"@id":"unece:SpecifiedChemicalTreatment"},{"@id":"unece:OrganizationalCertificate"},{"@id":"unece:ProcessCertificate"},{"@id":"unece:ProductBatchCertificate"},{"@id":"unece:ProductCertificate"},{"@id":"unece:SpecifiedCertificate"},{"@id":"unece:ProductCharacteristic"},{"@id":"unece:Chemical"},{"@id":"unece:SustainabilityInspection"},{"@id":"unece:HazardousMaterial"},{"@id":"unece:Assessment"},{"@id":"unece:ProcessCharacteristic"},{"@id":"unece:OrganizationCharacteristic"},{"@id":"unece:SpecifiedMaterial"},{"@id":"unece:ProductionWasteMaterial"},{"@id":"unece:ProductionWasteMaterialComponent"},{"@id":"unece:AgriculturalCertificate"},{"@id":"unece:AnimalCertificate"},{"@id":"unece:CropProtectionTreatment"},{"@id":"unece:AgriculturalApplication"},{"@id":"unece:TransportMovement"},{"@id":"unece:LogisticsTransportMeans"},{"@id":"unece:TransportationWasteMaterial"},{"@id":"unece:TransportationWasteMaterialComponent"}],"rdfs:comment":"A prominent attribute or aspect of an object, such as recyclability of a product, which can meet customer needs without compromising the ability of future generations to meet their own needs."},{"@id":"unece:applicableSustainabilityInspection","@type":["rdf:Property","owl:ObjectProperty"],"rdfs:label":"applicableSustainabilityInspection","schema:rangeIncludes":{"@id":"unece:SustainabilityInspection"},"schema:domainIncludes":[{"@id":"unece:TradeProduct"},{"@id":"unece:ProductionProcess"},{"@id":"unece:TradeParty"},{"@id":"unece:ProductBatch"},{"@id":"unece:ProductionFacility"},{"@id":"unece:TransportMovement"}],"rdfs:comment":"The process of performing documented checks of sustainability characteristics, with a focus on discovering deviations, related to documented sustainability requirements."},{"@id":"unece:applicableTechnicalCharacteristic","@type":["rdf:Property","owl:ObjectProperty"],"rdfs:label":"applicableTechnicalCharacteristic","schema:rangeIncludes":{"@id":"unece:TechnicalCharacteristic"},"schema:domainIncludes":[{"@id":"unece:TradeProduct"},{"@id":"unece:TradeParty"},{"@id":"unece:Colour"},{"@id":"unece:Print"}],"rdfs:comment":"A prominent technical attribute or aspect."},{"@id":"unece:applicableTradeProductCertification","@type":["rdf:Property","owl:ObjectProperty"],"rdfs:label":"applicableTradeProductCertification","schema:rangeIncludes":{"@id":"unece:TradeProductCertification"},"schema:domainIncludes":[{"@id":"unece:TradeProduct"},{"@id":"unece:ProductBatchCertificate"},{"@id":"unece:ProductCertificate"},{"@id":"unece:SpecifiedMaterial"}],"rdfs:comment":"The process of certifying that a certain product has passed performance and quality assurance tests, or qualification requirements stipulated in regulations."},{"@id":"unece:appliedChemicalTreatment","@type":["rdf:Property","owl:ObjectProperty"],"rdfs:label":"appliedChemicalTreatment","schema:rangeIncludes":{"@id":"unece:SpecifiedChemicalTreatment"},"schema:domainIncludes":[{"@id":"unece:TradeProduct"},{"@id":"unece:ProductionProcess"},{"@id":"unece:ProductBatch"}],"rdfs:comment":"A chemical treatment applied during this production process."},{"@id":"unece:appliedProductFinishingTreatment","@type":["rdf:Property","owl:ObjectProperty"],"rdfs:label":"appliedProductFinishingTreatment","schema:rangeIncludes":{"@id":"unece:ProductFinishingTreatment"},"schema:domainIncludes":[{"@id":"unece:TradeProduct"},{"@id":"unece:ProductionProcess"},{"@id":"unece:ProductBatch"}],"rdfs:comment":"A product finishing treatment applied during this production process."},{"@id":"unece:areaDensityMeasure","@type":["rdf:Property","owl:ObjectProperty"],"rdfs:label":"areaDensityMeasure","schema:rangeIncludes":{"@id":"unece:MeasureType"},"schema:domainIncludes":{"@id":"unece:TradeProduct"},"rdfs:comment":""},{"@id":"unece:attachedSecurityTag","@type":["rdf:Property","owl:ObjectProperty"],"rdfs:label":"attachedSecurityTag","schema:rangeIncludes":{"@id":"unece:SecurityTag"},"schema:domainIncludes":{"@id":"unece:TradeProduct"},"rdfs:comment":"A product tag device to provide protection from a peril such as theft."},{"@id":"unece:biologicallyBasedIndicator","@type":["rdf:Property","owl:DatatypeProperty"],"rdfs:label":"biologicallyBasedIndicator","schema:rangeIncludes":{"@id":"schema:Boolean"},"schema:domainIncludes":{"@id":"unece:TradeProduct"},"rdfs:comment":"The indication of whether or not this trade product is biologically based."},{"@id":"unece:brandName","@type":["rdf:Property","owl:DatatypeProperty"],"rdfs:label":"brandName","schema:rangeIncludes":{"@id":"schema:Text"},"schema:domainIncludes":[{"@id":"unece:TradeProduct"},{"@id":"unece:TradeParty"},{"@id":"unece:ProductLabel"},{"@id":"unece:ExperienceItem"},{"@id":"unece:ExperienceProduct"}],"rdfs:comment":"A brand name, expressed as text, for this experience product."},{"@id":"unece:brandOwnerParty","@type":["rdf:Property","owl:ObjectProperty"],"rdfs:label":"brandOwnerParty","schema:rangeIncludes":{"@id":"unece:TradeParty"},"schema:domainIncludes":{"@id":"unece:TradeProduct"},"rdfs:comment":"The party that owns the brand of this trade product."},{"@id":"unece:brandRangeName","@type":["rdf:Property","owl:DatatypeProperty"],"rdfs:label":"brandRangeName","schema:rangeIncludes":{"@id":"schema:Text"},"schema:domainIncludes":{"@id":"unece:TradeProduct"},"rdfs:comment":"The brand range name, expressed as text, for this trade product."},{"@id":"unece:buyerAssignedId","@type":["rdf:Property","owl:DatatypeProperty"],"rdfs:label":"buyerAssignedId","schema:rangeIncludes":{"@id":"schema:Text"},"schema:domainIncludes":[{"@id":"unece:TradeProduct"},{"@id":"unece:ProductBatch"},{"@id":"unece:Product"}],"rdfs:comment":"A buyer assigned identifier of this product batch."},{"@id":"unece:buyerSuppliedPartsReferenceDocument","@type":["rdf:Property","owl:ObjectProperty"],"rdfs:label":"buyerSuppliedPartsReferenceDocument","schema:rangeIncludes":{"@id":"unece:Document"},"schema:domainIncludes":{"@id":"unece:TradeProduct"},"rdfs:comment":"Written, printed or electronic matter that is referenced."},{"@id":"unece:cITESSpeciesCode","@type":["rdf:Property","owl:DatatypeProperty"],"rdfs:label":"cITESSpeciesCode","schema:rangeIncludes":{"@id":"schema:Text"},"schema:domainIncludes":{"@id":"unece:TradeProduct"},"rdfs:comment":"The CITES (Convention on International Trade in Endangered Species) code for this trade product."},{"@id":"unece:cancellationAnnouncedLaunchDateTime","@type":["rdf:Property","owl:DatatypeProperty"],"rdfs:label":"cancellationAnnouncedLaunchDateTime","schema:rangeIncludes":{"@id":"schema:DateTime"},"schema:domainIncludes":{"@id":"unece:TradeProduct"},"rdfs:comment":"The formatted date, time, date time, or other date time value of the cancellation of the announced launch of this trade product."},{"@id":"unece:careSpecifiedLabel","@type":["rdf:Property","owl:ObjectProperty"],"rdfs:label":"careSpecifiedLabel","schema:rangeIncludes":{"@id":"unece:ProductLabel"},"schema:domainIncludes":{"@id":"unece:TradeProduct"},"rdfs:comment":"A product care label specified for this trade product."},{"@id":"unece:certificationEvidenceReferenceDocument","@type":["rdf:Property","owl:ObjectProperty"],"rdfs:label":"certificationEvidenceReferenceDocument","schema:rangeIncludes":{"@id":"unece:Document"},"schema:domainIncludes":{"@id":"unece:TradeProduct"},"rdfs:comment":"Written, printed or electronic matter that is referenced."},{"@id":"unece:collectionId","@type":["rdf:Property","owl:DatatypeProperty"],"rdfs:label":"collectionId","schema:rangeIncludes":{"@id":"schema:Text"},"schema:domainIncludes":{"@id":"unece:TradeProduct"},"rdfs:comment":"A collection identifier of this trade product."},{"@id":"unece:collectionStatusCode","@type":["rdf:Property","owl:DatatypeProperty"],"rdfs:label":"collectionStatusCode","schema:rangeIncludes":{"@id":"schema:Text"},"schema:domainIncludes":{"@id":"unece:TradeProduct"},"rdfs:comment":"The code specifying the collection status of this trade product."},{"@id":"unece:colourCode","@type":["rdf:Property","owl:DatatypeProperty"],"rdfs:label":"colourCode","schema:rangeIncludes":{"@id":"schema:Text"},"schema:domainIncludes":[{"@id":"unece:TradeProduct"},{"@id":"unece:Package"}],"rdfs:comment":"The code specifying the colour for this trade product."},{"@id":"unece:colourDescription","@type":["rdf:Property","owl:DatatypeProperty"],"rdfs:label":"colourDescription","schema:rangeIncludes":{"@id":"schema:Text"},"schema:domainIncludes":{"@id":"unece:TradeProduct"},"rdfs:comment":"A textual description of the colour of this trade product."},{"@id":"unece:colourMatchingLightSourceCode","@type":["rdf:Property","owl:DatatypeProperty"],"rdfs:label":"colourMatchingLightSourceCode","schema:rangeIncludes":{"@id":"schema:Text"},"schema:domainIncludes":{"@id":"unece:TradeProduct"},"rdfs:comment":"The code specifying the light source used for colour matching of this trade product."},{"@id":"unece:colourMatchingSampleId","@type":["rdf:Property","owl:DatatypeProperty"],"rdfs:label":"colourMatchingSampleId","schema:rangeIncludes":{"@id":"schema:Text"},"schema:domainIncludes":{"@id":"unece:TradeProduct"},"rdfs:comment":"An identifier of the colour matching sample for this trade product."},{"@id":"unece:commonName","@type":["rdf:Property","owl:DatatypeProperty"],"rdfs:label":"commonName","schema:rangeIncludes":{"@id":"schema:Text"},"schema:domainIncludes":[{"@id":"unece:TradeProduct"},{"@id":"unece:Chemical"}],"rdfs:comment":"A common name, expressed as text, for this distinct chemical."},{"@id":"unece:componentMaterial","@type":["rdf:Property","owl:ObjectProperty"],"rdfs:label":"componentMaterial","schema:rangeIncludes":{"@id":"unece:SpecifiedMaterial"},"schema:domainIncludes":[{"@id":"unece:TradeProduct"},{"@id":"unece:ProductBatch"},{"@id":"unece:TechnicalCharacteristic"},{"@id":"unece:SpecifiedMaterial"}],"rdfs:comment":"A substance from which something is or could be made."},{"@id":"unece:conciseDescription","@type":["rdf:Property","owl:DatatypeProperty"],"rdfs:label":"conciseDescription","schema:rangeIncludes":{"@id":"schema:Text"},"schema:domainIncludes":{"@id":"unece:TradeProduct"},"rdfs:comment":"A concise textual description for this trade product, such as the description used on a shelf or printed on a receipt."},{"@id":"unece:configurableIndicator","@type":["rdf:Property","owl:DatatypeProperty"],"rdfs:label":"configurableIndicator","schema:rangeIncludes":{"@id":"schema:Boolean"},"schema:domainIncludes":{"@id":"unece:TradeProduct"},"rdfs:comment":"The indication of whether or not this trade product is configurable."},{"@id":"unece:consumerAgeDescription","@type":["rdf:Property","owl:DatatypeProperty"],"rdfs:label":"consumerAgeDescription","schema:rangeIncludes":{"@id":"schema:Text"},"schema:domainIncludes":{"@id":"unece:TradeProduct"},"rdfs:comment":"A consumer age description, expressed as text, for this trade product."},{"@id":"unece:consumerGenderCode","@type":["rdf:Property","owl:DatatypeProperty"],"rdfs:label":"consumerGenderCode","schema:rangeIncludes":{"@id":"schema:Text"},"schema:domainIncludes":{"@id":"unece:TradeProduct"},"rdfs:comment":"The code specifying the gender of the consumer of this trade product."},{"@id":"unece:consumerGenderDescription","@type":["rdf:Property","owl:DatatypeProperty"],"rdfs:label":"consumerGenderDescription","schema:rangeIncludes":{"@id":"schema:Text"},"schema:domainIncludes":{"@id":"unece:TradeProduct"},"rdfs:comment":"A consumer gender description, expressed as text, for this trade product."},{"@id":"unece:contentUnitQuantity","@type":["rdf:Property","owl:ObjectProperty"],"rdfs:label":"contentUnitQuantity","schema:rangeIncludes":{"@id":"unece:QuantityType"},"schema:domainIncludes":{"@id":"unece:TradeProduct"},"rdfs:comment":""},{"@id":"unece:contentVariableMeasureIndicator","@type":["rdf:Property","owl:DatatypeProperty"],"rdfs:label":"contentVariableMeasureIndicator","schema:rangeIncludes":{"@id":"schema:Boolean"},"schema:domainIncludes":{"@id":"unece:TradeProduct"},"rdfs:comment":"The indication of whether or not instances of this trade product have a content variable measure, such as weight, length or volume."},{"@id":"unece:customerAssignedId","@type":["rdf:Property","owl:DatatypeProperty"],"rdfs:label":"customerAssignedId","schema:rangeIncludes":{"@id":"schema:Text"},"schema:domainIncludes":{"@id":"unece:TradeProduct"},"rdfs:comment":"A unique customer assigned identifier for this trade product."},{"@id":"unece:customsStatisticalClassificationCode","@type":["rdf:Property","owl:DatatypeProperty"],"rdfs:label":"customsStatisticalClassificationCode","schema:rangeIncludes":{"@id":"schema:Text"},"schema:domainIncludes":{"@id":"unece:TradeProduct"},"rdfs:comment":"The code specifying the customs statistical classification for this trade product."},{"@id":"unece:designatedClassification","@type":["rdf:Property","owl:ObjectProperty"],"rdfs:label":"designatedClassification","schema:rangeIncludes":{"@id":"unece:Classification"},"schema:domainIncludes":{"@id":"unece:TradeProduct"},"rdfs:comment":"A product classification designated for this trade product."},{"@id":"unece:designation","@type":["rdf:Property","owl:DatatypeProperty"],"rdfs:label":"designation","schema:rangeIncludes":{"@id":"schema:Text"},"schema:domainIncludes":{"@id":"unece:TradeProduct"},"rdfs:comment":"A designation, expressed as text, for this trade product."},{"@id":"unece:digitalPlatformAssignedId","@type":["rdf:Property","owl:DatatypeProperty"],"rdfs:label":"digitalPlatformAssignedId","schema:rangeIncludes":{"@id":"schema:Text"},"schema:domainIncludes":[{"@id":"unece:TradeProduct"},{"@id":"unece:ProductionFacility"}],"rdfs:comment":"The digital platform assigned identifier for this production facility."},{"@id":"unece:drainedNetWeightMeasure","@type":["rdf:Property","owl:ObjectProperty"],"rdfs:label":"drainedNetWeightMeasure","schema:rangeIncludes":{"@id":"unece:MeasureType"},"schema:domainIncludes":{"@id":"unece:TradeProduct"},"rdfs:comment":""},{"@id":"unece:endItemName","@type":["rdf:Property","owl:DatatypeProperty"],"rdfs:label":"endItemName","schema:rangeIncludes":{"@id":"schema:Text"},"schema:domainIncludes":{"@id":"unece:TradeProduct"},"rdfs:comment":"An end item name, expressed as text, for this trade product."},{"@id":"unece:endItemTypeCode","@type":["rdf:Property","owl:DatatypeProperty"],"rdfs:label":"endItemTypeCode","schema:rangeIncludes":{"@id":"schema:Text"},"schema:domainIncludes":{"@id":"unece:TradeProduct"},"rdfs:comment":"A code specifying a type of end item for this trade product."},{"@id":"unece:endUseProductGroup","@type":["rdf:Property","owl:ObjectProperty"],"rdfs:label":"endUseProductGroup","schema:rangeIncludes":{"@id":"unece:ProductGroup"},"schema:domainIncludes":{"@id":"unece:TradeProduct"},"rdfs:comment":"An end use product group for this trade product."},{"@id":"unece:endUserParty","@type":["rdf:Property","owl:ObjectProperty"],"rdfs:label":"endUserParty","schema:rangeIncludes":{"@id":"unece:TradeParty"},"schema:domainIncludes":{"@id":"unece:TradeProduct"},"rdfs:comment":"An end user party for this trade product."},{"@id":"unece:exportIndicator","@type":["rdf:Property","owl:DatatypeProperty"],"rdfs:label":"exportIndicator","schema:rangeIncludes":{"@id":"schema:Boolean"},"schema:domainIncludes":{"@id":"unece:TradeProduct"},"rdfs:comment":"The indication of whether or not this trade product is for export."},{"@id":"unece:finalAssemblyCountry","@type":["rdf:Property","owl:ObjectProperty"],"rdfs:label":"finalAssemblyCountry","schema:rangeIncludes":{"@id":"unece:Country"},"schema:domainIncludes":{"@id":"unece:TradeProduct"},"rdfs:comment":"The area of land that belongs to a nation together with its properties, such as population, political organization, etc., used or referenced for trade purposes."},{"@id":"unece:fromDeliveryLifeSpanMeasure","@type":["rdf:Property","owl:ObjectProperty"],"rdfs:label":"fromDeliveryLifeSpanMeasure","schema:rangeIncludes":{"@id":"unece:DurationUnitMeasureType"},"schema:domainIncludes":{"@id":"unece:TradeProduct"},"rdfs:comment":""},{"@id":"unece:fromOpeningLifeSpanMeasure","@type":["rdf:Property","owl:ObjectProperty"],"rdfs:label":"fromOpeningLifeSpanMeasure","schema:rangeIncludes":{"@id":"unece:DurationUnitMeasureType"},"schema:domainIncludes":{"@id":"unece:TradeProduct"},"rdfs:comment":""},{"@id":"unece:fromProductionLifeSpanMeasure","@type":["rdf:Property","owl:ObjectProperty"],"rdfs:label":"fromProductionLifeSpanMeasure","schema:rangeIncludes":{"@id":"unece:DurationUnitMeasureType"},"schema:domainIncludes":{"@id":"unece:TradeProduct"},"rdfs:comment":""},{"@id":"unece:functionDescription","@type":["rdf:Property","owl:DatatypeProperty"],"rdfs:label":"functionDescription","schema:rangeIncludes":{"@id":"schema:Text"},"schema:domainIncludes":[{"@id":"unece:TradeProduct"},{"@id":"unece:ProductionDevice"},{"@id":"unece:Machine"}],"rdfs:comment":"A textual description of a function for this trade product."},{"@id":"unece:functionTypeCode","@type":["rdf:Property","owl:DatatypeProperty"],"rdfs:label":"functionTypeCode","schema:rangeIncludes":{"@id":"schema:Text"},"schema:domainIncludes":{"@id":"unece:TradeProduct"},"rdfs:comment":"The code specifying the type of function for this trade product."},{"@id":"unece:geneticModificationExtentCode","@type":["rdf:Property","owl:DatatypeProperty"],"rdfs:label":"geneticModificationExtentCode","schema:rangeIncludes":{"@id":"schema:Text"},"schema:domainIncludes":{"@id":"unece:TradeProduct"},"rdfs:comment":"The code specifying the extent of a genetic modification to this trade product."},{"@id":"unece:globalExtensionId","@type":["rdf:Property","owl:DatatypeProperty"],"rdfs:label":"globalExtensionId","schema:rangeIncludes":{"@id":"schema:Text"},"schema:domainIncludes":{"@id":"unece:TradeProduct"},"rdfs:comment":"A global extension identifier for this trade product, such as a prefix or a suffix."},{"@id":"unece:grossVolumeMeasure","@type":["rdf:Property","owl:ObjectProperty"],"rdfs:label":"grossVolumeMeasure","schema:rangeIncludes":{"@id":"unece:MeasureType"},"schema:domainIncludes":[{"@id":"unece:TradeProduct"},{"@id":"unece:ProductBatch"},{"@id":"unece:Package"},{"@id":"unece:AssociatedTransportEquipment"}],"rdfs:comment":""},{"@id":"unece:grossWeightMeasure","@type":["rdf:Property","owl:ObjectProperty"],"rdfs:label":"grossWeightMeasure","schema:rangeIncludes":{"@id":"unece:MeasureType"},"schema:domainIncludes":[{"@id":"unece:TradeProduct"},{"@id":"unece:ProductBatch"},{"@id":"unece:Package"},{"@id":"unece:AssociatedTransportEquipment"}],"rdfs:comment":""},{"@id":"unece:includedProduct","@type":["rdf:Property","owl:ObjectProperty"],"rdfs:label":"includedProduct","schema:rangeIncludes":{"@id":"unece:Product"},"schema:domainIncludes":{"@id":"unece:TradeProduct"},"rdfs:comment":"An included product referenced from this trade product."},{"@id":"unece:includedProductContentUnitQuantity","@type":["rdf:Property","owl:ObjectProperty"],"rdfs:label":"includedProductContentUnitQuantity","schema:rangeIncludes":{"@id":"unece:QuantityType"},"schema:domainIncludes":{"@id":"unece:TradeProduct"},"rdfs:comment":""},{"@id":"unece:includedProductTypeQuantity","@type":["rdf:Property","owl:ObjectProperty"],"rdfs:label":"includedProductTypeQuantity","schema:rangeIncludes":{"@id":"unece:QuantityType"},"schema:domainIncludes":{"@id":"unece:TradeProduct"},"rdfs:comment":""},{"@id":"unece:individualProductInstance","@type":["rdf:Property","owl:ObjectProperty"],"rdfs:label":"individualProductInstance","schema:rangeIncludes":{"@id":"unece:ProductInstance"},"schema:domainIncludes":{"@id":"unece:TradeProduct"},"rdfs:comment":"An individual instance of this trade product."},{"@id":"unece:industryAssignedId","@type":["rdf:Property","owl:DatatypeProperty"],"rdfs:label":"industryAssignedId","schema:rangeIncludes":{"@id":"schema:Text"},"schema:domainIncludes":[{"@id":"unece:TradeProduct"},{"@id":"unece:Product"}],"rdfs:comment":"A unique industry assigned identifier for this product."},{"@id":"unece:innerPackContentUnitQuantity","@type":["rdf:Property","owl:ObjectProperty"],"rdfs:label":"innerPackContentUnitQuantity","schema:rangeIncludes":{"@id":"unece:QuantityType"},"schema:domainIncludes":{"@id":"unece:TradeProduct"},"rdfs:comment":""},{"@id":"unece:innerPackQuantity","@type":["rdf:Property","owl:ObjectProperty"],"rdfs:label":"innerPackQuantity","schema:rangeIncludes":{"@id":"unece:QuantityType"},"schema:domainIncludes":{"@id":"unece:TradeProduct"},"rdfs:comment":""},{"@id":"unece:inspectionReferenceDocument","@type":["rdf:Property","owl:ObjectProperty"],"rdfs:label":"inspectionReferenceDocument","schema:rangeIncludes":{"@id":"unece:Document"},"schema:domainIncludes":{"@id":"unece:TradeProduct"},"rdfs:comment":"Written, printed or electronic matter that is referenced."},{"@id":"unece:intendedUse","@type":["rdf:Property","owl:DatatypeProperty"],"rdfs:label":"intendedUse","schema:rangeIncludes":{"@id":"schema:Text"},"schema:domainIncludes":[{"@id":"unece:TradeProduct"},{"@id":"unece:Picture"}],"rdfs:comment":"An intended use, expressed as text, for this photographic picture."},{"@id":"unece:latestProductDataChangeDateTime","@type":["rdf:Property","owl:DatatypeProperty"],"rdfs:label":"latestProductDataChangeDateTime","schema:rangeIncludes":{"@id":"schema:DateTime"},"schema:domainIncludes":{"@id":"unece:TradeProduct"},"rdfs:comment":"The formatted date, time, date time, or other date time value of the latest change in the product data for this trade product."},{"@id":"unece:legalRightsOwnerParty","@type":["rdf:Property","owl:ObjectProperty"],"rdfs:label":"legalRightsOwnerParty","schema:rangeIncludes":{"@id":"unece:TradeParty"},"schema:domainIncludes":{"@id":"unece:TradeProduct"},"rdfs:comment":"The party that owns the legal rights for this trade product."},{"@id":"unece:lifeCycleStageCode","@type":["rdf:Property","owl:DatatypeProperty"],"rdfs:label":"lifeCycleStageCode","schema:rangeIncludes":{"@id":"schema:Text"},"schema:domainIncludes":{"@id":"unece:TradeProduct"},"rdfs:comment":"The code specifying the life cycle stage for this trade product."},{"@id":"unece:line","@type":["rdf:Property","owl:DatatypeProperty"],"rdfs:label":"line","schema:rangeIncludes":{"@id":"schema:Text"},"schema:domainIncludes":{"@id":"unece:TradeProduct"},"rdfs:comment":"A product line, such as a fashion product line, expressed as text, for this trade product."},{"@id":"unece:linearDimension","@type":["rdf:Property","owl:ObjectProperty"],"rdfs:label":"linearDimension","schema:rangeIncludes":{"@id":"unece:SpatialDimension"},"schema:domainIncludes":[{"@id":"unece:TradeProduct"},{"@id":"unece:Picture"},{"@id":"unece:LogisticsTransportEquipment"},{"@id":"unece:Package"},{"@id":"unece:ConsignmentItem"},{"@id":"unece:LogisticsPackaging"},{"@id":"unece:SupplyChainPackaging"}],"rdfs:comment":"A measure of spatial extent of an object, such as the length, breadth or height of a shipping container."},{"@id":"unece:mSDSReferenceDocument","@type":["rdf:Property","owl:ObjectProperty"],"rdfs:label":"mSDSReferenceDocument","schema:rangeIncludes":{"@id":"unece:Document"},"schema:domainIncludes":{"@id":"unece:TradeProduct"},"rdfs:comment":"Written, printed or electronic matter that is referenced."},{"@id":"unece:mSRPPrice","@type":["rdf:Property","owl:ObjectProperty"],"rdfs:label":"mSRPPrice","schema:rangeIncludes":{"@id":"unece:TradePrice"},"schema:domainIncludes":{"@id":"unece:TradeProduct"},"rdfs:comment":"A sum of money for which something is or may be bought or sold for trade purposes."},{"@id":"unece:manufactureCountry","@type":["rdf:Property","owl:ObjectProperty"],"rdfs:label":"manufactureCountry","schema:rangeIncludes":{"@id":"unece:Country"},"schema:domainIncludes":{"@id":"unece:TradeProduct"},"rdfs:comment":"The area of land that belongs to a nation together with its properties, such as population, political organization, etc., used or referenced for trade purposes."},{"@id":"unece:manufacturerAssignedId","@type":["rdf:Property","owl:DatatypeProperty"],"rdfs:label":"manufacturerAssignedId","schema:rangeIncludes":{"@id":"schema:Text"},"schema:domainIncludes":[{"@id":"unece:TradeProduct"},{"@id":"unece:ProductBatch"},{"@id":"unece:Product"}],"rdfs:comment":"A manufacturer assigned identifier of this product batch."},{"@id":"unece:manufacturerParty","@type":["rdf:Property","owl:ObjectProperty"],"rdfs:label":"manufacturerParty","schema:rangeIncludes":{"@id":"unece:TradeParty"},"schema:domainIncludes":[{"@id":"unece:TradeProduct"},{"@id":"unece:LineTradeAgreement"},{"@id":"unece:ProductionProcess"},{"@id":"unece:ProductionUnit"},{"@id":"unece:SpecifiedMaterial"},{"@id":"unece:LogisticsTransportEquipment"},{"@id":"unece:LogisticsTransportMeans"},{"@id":"unece:ConsignmentItem"},{"@id":"unece:IOTDevice"},{"@id":"unece:Sensor"},{"@id":"unece:Equipment"}],"rdfs:comment":"A manufacturer party for this production process."},{"@id":"unece:markedSerialNumberIndicator","@type":["rdf:Property","owl:DatatypeProperty"],"rdfs:label":"markedSerialNumberIndicator","schema:rangeIncludes":{"@id":"schema:Boolean"},"schema:domainIncludes":{"@id":"unece:TradeProduct"},"rdfs:comment":"The indication of whether or not this trade product is marked with a serial number."},{"@id":"unece:marketingCampaignReferenceDocument","@type":["rdf:Property","owl:ObjectProperty"],"rdfs:label":"marketingCampaignReferenceDocument","schema:rangeIncludes":{"@id":"unece:Document"},"schema:domainIncludes":{"@id":"unece:TradeProduct"},"rdfs:comment":"Written, printed or electronic matter that is referenced."},{"@id":"unece:marketingDescription","@type":["rdf:Property","owl:DatatypeProperty"],"rdfs:label":"marketingDescription","schema:rangeIncludes":{"@id":"schema:Text"},"schema:domainIncludes":{"@id":"unece:TradeProduct"},"rdfs:comment":"A marketing description, expressed as text, for this trade product."},{"@id":"unece:marketingFeature","@type":["rdf:Property","owl:ObjectProperty"],"rdfs:label":"marketingFeature","schema:rangeIncludes":{"@id":"unece:TradeProductFeature"},"schema:domainIncludes":{"@id":"unece:TradeProduct"},"rdfs:comment":"A marketing feature of this trade product."},{"@id":"unece:maximumLinearDimension","@type":["rdf:Property","owl:ObjectProperty"],"rdfs:label":"maximumLinearDimension","schema:rangeIncludes":{"@id":"unece:SpatialDimension"},"schema:domainIncludes":[{"@id":"unece:TradeProduct"},{"@id":"unece:SupplyChainPackaging"}],"rdfs:comment":"A measure of spatial extent of an object, such as the length, breadth or height of a shipping container."},{"@id":"unece:minimumLinearDimension","@type":["rdf:Property","owl:ObjectProperty"],"rdfs:label":"minimumLinearDimension","schema:rangeIncludes":{"@id":"unece:SpatialDimension"},"schema:domainIncludes":[{"@id":"unece:TradeProduct"},{"@id":"unece:SupplyChainPackaging"}],"rdfs:comment":"A measure of spatial extent of an object, such as the length, breadth or height of a shipping container."},{"@id":"unece:modelId","@type":["rdf:Property","owl:DatatypeProperty"],"rdfs:label":"modelId","schema:rangeIncludes":{"@id":"schema:Text"},"schema:domainIncludes":[{"@id":"unece:TradeProduct"},{"@id":"unece:IOTDevice"}],"rdfs:comment":"A model identifier for this monitoring IOT device."},{"@id":"unece:modelName","@type":["rdf:Property","owl:DatatypeProperty"],"rdfs:label":"modelName","schema:rangeIncludes":{"@id":"schema:Text"},"schema:domainIncludes":{"@id":"unece:TradeProduct"},"rdfs:comment":"The model name, expressed as text, for this trade product."},{"@id":"unece:netVolumeMeasure","@type":["rdf:Property","owl:ObjectProperty"],"rdfs:label":"netVolumeMeasure","schema:rangeIncludes":{"@id":"unece:MeasureType"},"schema:domainIncludes":[{"@id":"unece:TradeProduct"},{"@id":"unece:ProductBatch"},{"@id":"unece:Package"}],"rdfs:comment":""},{"@id":"unece:netWeightMeasure","@type":["rdf:Property","owl:ObjectProperty"],"rdfs:label":"netWeightMeasure","schema:rangeIncludes":{"@id":"unece:MeasureType"},"schema:domainIncludes":[{"@id":"unece:TradeProduct"},{"@id":"unece:ProductBatch"},{"@id":"unece:Package"}],"rdfs:comment":""},{"@id":"unece:originCountry","@type":["rdf:Property","owl:ObjectProperty"],"rdfs:label":"originCountry","schema:rangeIncludes":{"@id":"unece:Country"},"schema:domainIncludes":[{"@id":"unece:TradeProduct"},{"@id":"unece:Consignment"},{"@id":"unece:ConsignmentItem"}],"rdfs:comment":"The area of land that belongs to a nation together with its properties, such as population, political organization, etc., used or referenced for trade purposes."},{"@id":"unece:physicalFormDescription","@type":["rdf:Property","owl:DatatypeProperty"],"rdfs:label":"physicalFormDescription","schema:rangeIncludes":{"@id":"schema:Text"},"schema:domainIncludes":{"@id":"unece:TradeProduct"},"rdfs:comment":"A textual description of the physical form of this trade product."},{"@id":"unece:pieceIndicator","@type":["rdf:Property","owl:DatatypeProperty"],"rdfs:label":"pieceIndicator","schema:rangeIncludes":{"@id":"schema:Boolean"},"schema:domainIncludes":{"@id":"unece:TradeProduct"},"rdfs:comment":"The indication of whether or not this trade product is a piece, such as a piece of fabric."},{"@id":"unece:prePackagedIndicator","@type":["rdf:Property","owl:DatatypeProperty"],"rdfs:label":"prePackagedIndicator","schema:rangeIncludes":{"@id":"schema:Boolean"},"schema:domainIncludes":{"@id":"unece:TradeProduct"},"rdfs:comment":"The indication of whether or not this trade product is pre-packaged."},{"@id":"unece:presentationBinaryFile","@type":["rdf:Property","owl:ObjectProperty"],"rdfs:label":"presentationBinaryFile","schema:rangeIncludes":{"@id":"unece:BinaryFile"},"schema:domainIncludes":{"@id":"unece:TradeProduct"},"rdfs:comment":"A specified computer file or program stored in a binary format."},{"@id":"unece:preservationAppliedMethod","@type":["rdf:Property","owl:ObjectProperty"],"rdfs:label":"preservationAppliedMethod","schema:rangeIncludes":{"@id":"unece:SpecifiedMethod"},"schema:domainIncludes":{"@id":"unece:TradeProduct"},"rdfs:comment":"A defined way of performing something."},{"@id":"unece:printDesignDescription","@type":["rdf:Property","owl:DatatypeProperty"],"rdfs:label":"printDesignDescription","schema:rangeIncludes":{"@id":"schema:Text"},"schema:domainIncludes":{"@id":"unece:TradeProduct"},"rdfs:comment":"A textual description of the print design for this trade product."},{"@id":"unece:printDesignId","@type":["rdf:Property","owl:DatatypeProperty"],"rdfs:label":"printDesignId","schema:rangeIncludes":{"@id":"schema:Text"},"schema:domainIncludes":{"@id":"unece:TradeProduct"},"rdfs:comment":"An identifier of the print design for this trade product."},{"@id":"unece:productGroupId","@type":["rdf:Property","owl:DatatypeProperty"],"rdfs:label":"productGroupId","schema:rangeIncludes":{"@id":"schema:Text"},"schema:domainIncludes":{"@id":"unece:TradeProduct"},"rdfs:comment":"A unique identifier for a product group for this trade product."},{"@id":"unece:productionDiscontinuedDateTime","@type":["rdf:Property","owl:DatatypeProperty"],"rdfs:label":"productionDiscontinuedDateTime","schema:rangeIncludes":{"@id":"schema:Text"},"schema:domainIncludes":{"@id":"unece:TradeProduct"},"rdfs:comment":"The date, time, date time, or other date time value of the discontinuation of the production of this trade product."},{"@id":"unece:promotionalVariantId","@type":["rdf:Property","owl:DatatypeProperty"],"rdfs:label":"promotionalVariantId","schema:rangeIncludes":{"@id":"schema:Text"},"schema:domainIncludes":{"@id":"unece:TradeProduct"},"rdfs:comment":"The promotional variant identifier for this trade product."},{"@id":"unece:qualityLevelCode","@type":["rdf:Property","owl:DatatypeProperty"],"rdfs:label":"qualityLevelCode","schema:rangeIncludes":{"@id":"schema:Text"},"schema:domainIncludes":{"@id":"unece:TradeProduct"},"rdfs:comment":"The code specifying the quality level for this trade product."},{"@id":"unece:qualityParameter","@type":["rdf:Property","owl:ObjectProperty"],"rdfs:label":"qualityParameter","schema:rangeIncludes":{"@id":"unece:SpecifiedParameter"},"schema:domainIncludes":{"@id":"unece:TradeProduct"},"rdfs:comment":"A specified feature that is fixed for the case in question but may be different in other cases."},{"@id":"unece:recyclableIndicator","@type":["rdf:Property","owl:DatatypeProperty"],"rdfs:label":"recyclableIndicator","schema:rangeIncludes":{"@id":"schema:Boolean"},"schema:domainIncludes":[{"@id":"unece:TradeProduct"},{"@id":"unece:SupplyChainPackaging"}],"rdfs:comment":"The indication of whether or not this supply chain packaging is recyclable."},{"@id":"unece:recycledMaterialIndicator","@type":["rdf:Property","owl:DatatypeProperty"],"rdfs:label":"recycledMaterialIndicator","schema:rangeIncludes":{"@id":"schema:Boolean"},"schema:domainIncludes":[{"@id":"unece:TradeProduct"},{"@id":"unece:SupplyChainPackaging"}],"rdfs:comment":"The indication of whether or not this supply chain packaging is made of recycled material."},{"@id":"unece:recycledMaterialPercent","@type":["rdf:Property","owl:DatatypeProperty"],"rdfs:label":"recycledMaterialPercent","schema:rangeIncludes":{"@id":"schema:Text"},"schema:domainIncludes":[{"@id":"unece:TradeProduct"},{"@id":"unece:SupplyChainPackaging"}],"rdfs:comment":"The percentage of recycled material in this supply chain packaging."},{"@id":"unece:recyclingTypeCode","@type":["rdf:Property","owl:DatatypeProperty"],"rdfs:label":"recyclingTypeCode","schema:rangeIncludes":{"@id":"schema:Text"},"schema:domainIncludes":{"@id":"unece:TradeProduct"},"rdfs:comment":"The code specifying the type of recycling for this trade product."},{"@id":"unece:regulationConformityId","@type":["rdf:Property","owl:DatatypeProperty"],"rdfs:label":"regulationConformityId","schema:rangeIncludes":{"@id":"schema:Text"},"schema:domainIncludes":{"@id":"unece:TradeProduct"},"rdfs:comment":"An identifier assigned to indicate conformity with a regulation or standard for this trade product, such as \"CE\" which declares that the product conforms with the essential requirements of the applicable EC directives."},{"@id":"unece:relatedAnimal","@type":["rdf:Property","owl:ObjectProperty"],"rdfs:label":"relatedAnimal","schema:rangeIncludes":{"@id":"unece:TTAnimal"},"schema:domainIncludes":{"@id":"unece:TradeProduct"},"rdfs:comment":"A TT (Track and Trace) animal, such as one kept or raised on a farm or ranch, related to this trade product."},{"@id":"unece:relatedLocation","@type":["rdf:Property","owl:ObjectProperty"],"rdfs:label":"relatedLocation","schema:rangeIncludes":{"@id":"unece:Location"},"schema:domainIncludes":[{"@id":"unece:TradeProduct"},{"@id":"unece:OrganizationalCertification"},{"@id":"unece:ProcessCertification"},{"@id":"unece:ProductBatchCertification"},{"@id":"unece:SpecifiedCertification"},{"@id":"unece:TradeProductCertification"},{"@id":"unece:AnimalCertification"}],"rdfs:comment":"A reference to a physical location or place."},{"@id":"unece:relatedPackage","@type":["rdf:Property","owl:ObjectProperty"],"rdfs:label":"relatedPackage","schema:rangeIncludes":{"@id":"unece:Package"},"schema:domainIncludes":{"@id":"unece:TradeProduct"},"rdfs:comment":"A self-contained wrapping or container within which goods can be contained for logistics purposes, such as a box or a barrel which can be filled, partially filled or empty.,A referenced self-contained wrapping or container within which goods can be contained for logistics purposes."},{"@id":"unece:relatedTradeTransaction","@type":["rdf:Property","owl:ObjectProperty"],"rdfs:label":"relatedTradeTransaction","schema:rangeIncludes":{"@id":"unece:SupplyChainTradeTransaction"},"schema:domainIncludes":{"@id":"unece:TradeProduct"},"rdfs:comment":"A supply chain trade transaction related to this specified assessment."},{"@id":"unece:responsibleParty","@type":["rdf:Property","owl:ObjectProperty"],"rdfs:label":"responsibleParty","schema:rangeIncludes":{"@id":"unece:TradeParty"},"schema:domainIncludes":[{"@id":"unece:TradeProduct"},{"@id":"unece:Service"}],"rdfs:comment":"A party responsible for providing this referenced transport service."},{"@id":"unece:reusableIndicator","@type":["rdf:Property","owl:DatatypeProperty"],"rdfs:label":"reusableIndicator","schema:rangeIncludes":{"@id":"schema:Boolean"},"schema:domainIncludes":{"@id":"unece:TradeProduct"},"rdfs:comment":"The indication of whether or not this trade product is reusable."},{"@id":"unece:salesCountry","@type":["rdf:Property","owl:ObjectProperty"],"rdfs:label":"salesCountry","schema:rangeIncludes":{"@id":"unece:Country"},"schema:domainIncludes":{"@id":"unece:TradeProduct"},"rdfs:comment":"The area of land that belongs to a nation together with its properties, such as population, political organization, etc., used or referenced for trade purposes."},{"@id":"unece:scientificName","@type":["rdf:Property","owl:DatatypeProperty"],"rdfs:label":"scientificName","schema:rangeIncludes":{"@id":"schema:Text"},"schema:domainIncludes":[{"@id":"unece:TradeProduct"},{"@id":"unece:Chemical"}],"rdfs:comment":"A scientific name, expressed as text, for this trade product."},{"@id":"unece:seasonCode","@type":["rdf:Property","owl:DatatypeProperty"],"rdfs:label":"seasonCode","schema:rangeIncludes":{"@id":"schema:Text"},"schema:domainIncludes":[{"@id":"unece:TradeProduct"},{"@id":"unece:SpecifiedPeriod"}],"rdfs:comment":"A code specifying a season for this trade product."},{"@id":"unece:seasonDescription","@type":["rdf:Property","owl:DatatypeProperty"],"rdfs:label":"seasonDescription","schema:rangeIncludes":{"@id":"schema:Text"},"schema:domainIncludes":{"@id":"unece:TradeProduct"},"rdfs:comment":"A season description, expressed as text, for this trade product."},{"@id":"unece:sectionCode","@type":["rdf:Property","owl:DatatypeProperty"],"rdfs:label":"sectionCode","schema:rangeIncludes":{"@id":"schema:Text"},"schema:domainIncludes":[{"@id":"unece:TradeProduct"},{"@id":"unece:Print"}],"rdfs:comment":"The code specifying the section for this product print."},{"@id":"unece:securityInformationNote","@type":["rdf:Property","owl:ObjectProperty"],"rdfs:label":"securityInformationNote","schema:rangeIncludes":{"@id":"unece:Note"},"schema:domainIncludes":{"@id":"unece:TradeProduct"},"rdfs:comment":"A textual or coded description, such as a remark or additional information."},{"@id":"unece:sellerAssignedId","@type":["rdf:Property","owl:DatatypeProperty"],"rdfs:label":"sellerAssignedId","schema:rangeIncludes":{"@id":"schema:Text"},"schema:domainIncludes":[{"@id":"unece:TradeProduct"},{"@id":"unece:ProductBatch"},{"@id":"unece:Product"}],"rdfs:comment":"A seller assigned identifier of this product batch."},{"@id":"unece:sizeCode","@type":["rdf:Property","owl:DatatypeProperty"],"rdfs:label":"sizeCode","schema:rangeIncludes":{"@id":"schema:Text"},"schema:domainIncludes":[{"@id":"unece:TradeProduct"},{"@id":"unece:ProductLabel"},{"@id":"unece:LogisticsLabel"}],"rdfs:comment":"The code specifying the size of this logistics label."},{"@id":"unece:sizeDescription","@type":["rdf:Property","owl:DatatypeProperty"],"rdfs:label":"sizeDescription","schema:rangeIncludes":{"@id":"schema:Text"},"schema:domainIncludes":{"@id":"unece:TradeProduct"},"rdfs:comment":"A size description, expressed as text, for this trade product."},{"@id":"unece:speciesCode","@type":["rdf:Property","owl:DatatypeProperty"],"rdfs:label":"speciesCode","schema:rangeIncludes":{"@id":"schema:Text"},"schema:domainIncludes":{"@id":"unece:TradeProduct"},"rdfs:comment":"The code specifying the species, such as for a plant or animal, of this trade product."},{"@id":"unece:specifiedAssertion","@type":["rdf:Property","owl:ObjectProperty"],"rdfs:label":"specifiedAssertion","schema:rangeIncludes":{"@id":"unece:Assertion"},"schema:domainIncludes":[{"@id":"unece:TradeProduct"},{"@id":"unece:ProductionProcess"},{"@id":"unece:TradeParty"},{"@id":"unece:ProductBatch"},{"@id":"unece:Standard"},{"@id":"unece:OrganizationalCertification"},{"@id":"unece:ProcessCertification"},{"@id":"unece:ProductBatchCertification"},{"@id":"unece:SpecifiedCertification"},{"@id":"unece:TradeProductCertification"},{"@id":"unece:AnimalCertification"}],"rdfs:comment":"A statement that user needs of the present are met without compromising the needs of future generations."},{"@id":"unece:specifiedColour","@type":["rdf:Property","owl:ObjectProperty"],"rdfs:label":"specifiedColour","schema:rangeIncludes":{"@id":"unece:Colour"},"schema:domainIncludes":{"@id":"unece:TradeProduct"},"rdfs:comment":"A colour specified for this trade product."},{"@id":"unece:specifiedFacility","@type":["rdf:Property","owl:ObjectProperty"],"rdfs:label":"specifiedFacility","schema:rangeIncludes":{"@id":"unece:ProductionFacility"},"schema:domainIncludes":[{"@id":"unece:TradeProduct"},{"@id":"unece:ProductionProcess"},{"@id":"unece:TradeParty"}],"rdfs:comment":"A production facility specified for this production process."},{"@id":"unece:specifiedLabel","@type":["rdf:Property","owl:ObjectProperty"],"rdfs:label":"specifiedLabel","schema:rangeIncludes":{"@id":"unece:ProductLabel"},"schema:domainIncludes":{"@id":"unece:TradeProduct"},"rdfs:comment":"A product label specified for this trade product."},{"@id":"unece:specifiedPicture","@type":["rdf:Property","owl:ObjectProperty"],"rdfs:label":"specifiedPicture","schema:rangeIncludes":{"@id":"unece:Picture"},"schema:domainIncludes":[{"@id":"unece:TradeProduct"},{"@id":"unece:ProductBatch"}],"rdfs:comment":"A photograph or video still represented as a digital image for electronic sharing."},{"@id":"unece:specifiedPrint","@type":["rdf:Property","owl:ObjectProperty"],"rdfs:label":"specifiedPrint","schema:rangeIncludes":{"@id":"unece:Print"},"schema:domainIncludes":{"@id":"unece:TradeProduct"},"rdfs:comment":"A product print specified for this trade product."},{"@id":"unece:specifiedProductCertificate","@type":["rdf:Property","owl:ObjectProperty"],"rdfs:label":"specifiedProductCertificate","schema:rangeIncludes":{"@id":"unece:ProductCertificate"},"schema:domainIncludes":[{"@id":"unece:TradeProduct"},{"@id":"unece:ProductionFacility"},{"@id":"unece:ProductionUnit"},{"@id":"unece:Chemical"}],"rdfs:comment":"A collection of data for a piece of written, printed or electronic matter that provides information or evidence about the product."},{"@id":"unece:specifiedProductGroup","@type":["rdf:Property","owl:ObjectProperty"],"rdfs:label":"specifiedProductGroup","schema:rangeIncludes":{"@id":"unece:ProductGroup"},"schema:domainIncludes":{"@id":"unece:TradeProduct"},"rdfs:comment":"A product group specified for this trade product."},{"@id":"unece:specifiedSupplyPlan","@type":["rdf:Property","owl:ObjectProperty"],"rdfs:label":"specifiedSupplyPlan","schema:rangeIncludes":{"@id":"unece:SupplyPlan"},"schema:domainIncludes":{"@id":"unece:TradeProduct"},"rdfs:comment":"The specification of the delivery quantities and delivery date/time values in a supply plan for this trade product."},{"@id":"unece:storageInformationNote","@type":["rdf:Property","owl:ObjectProperty"],"rdfs:label":"storageInformationNote","schema:rangeIncludes":{"@id":"unece:Note"},"schema:domainIncludes":{"@id":"unece:TradeProduct"},"rdfs:comment":"A textual or coded description, such as a remark or additional information."},{"@id":"unece:subBrandName","@type":["rdf:Property","owl:DatatypeProperty"],"rdfs:label":"subBrandName","schema:rangeIncludes":{"@id":"schema:Text"},"schema:domainIncludes":{"@id":"unece:TradeProduct"},"rdfs:comment":"The sub-brand name, expressed as text, for this trade product."},{"@id":"unece:subcontractorParty","@type":["rdf:Property","owl:ObjectProperty"],"rdfs:label":"subcontractorParty","schema:rangeIncludes":{"@id":"unece:TradeParty"},"schema:domainIncludes":[{"@id":"unece:TradeProduct"},{"@id":"unece:ProductionProcess"},{"@id":"unece:TradeParty"},{"@id":"unece:ProductionUnit"}],"rdfs:comment":"A subcontractor for this trade party."},{"@id":"unece:subordinateTypeCode","@type":["rdf:Property","owl:DatatypeProperty"],"rdfs:label":"subordinateTypeCode","schema:rangeIncludes":{"@id":"schema:Text"},"schema:domainIncludes":[{"@id":"unece:TradeProduct"},{"@id":"unece:ProductionProcess"},{"@id":"unece:ProductionFacility"},{"@id":"unece:ProductionDevice"},{"@id":"unece:Machine"},{"@id":"unece:SustainabilityCharacteristic"},{"@id":"unece:TechnicalCharacteristic"},{"@id":"unece:AgriculturalProcess"},{"@id":"unece:Produce"}],"rdfs:comment":"The code specifying the subordinate type for this production device."},{"@id":"unece:subordinateTypeDescription","@type":["rdf:Property","owl:DatatypeProperty"],"rdfs:label":"subordinateTypeDescription","schema:rangeIncludes":{"@id":"schema:Text"},"schema:domainIncludes":{"@id":"unece:TradeProduct"},"rdfs:comment":"A textual description of the subordinate type for this trade product."},{"@id":"unece:substituteProduct","@type":["rdf:Property","owl:ObjectProperty"],"rdfs:label":"substituteProduct","schema:rangeIncludes":{"@id":"unece:Product"},"schema:domainIncludes":{"@id":"unece:TradeProduct"},"rdfs:comment":"A referenced product that may substitute for this trade product."},{"@id":"unece:suppliedFromCountry","@type":["rdf:Property","owl:ObjectProperty"],"rdfs:label":"suppliedFromCountry","schema:rangeIncludes":{"@id":"unece:Country"},"schema:domainIncludes":{"@id":"unece:TradeProduct"},"rdfs:comment":"The area of land that belongs to a nation together with its properties, such as population, political organization, etc., used or referenced for trade purposes."},{"@id":"unece:trackingSystemId","@type":["rdf:Property","owl:DatatypeProperty"],"rdfs:label":"trackingSystemId","schema:rangeIncludes":{"@id":"schema:Text"},"schema:domainIncludes":{"@id":"unece:TradeProduct"},"rdfs:comment":"An identifier for a tracking system of this trade product."},{"@id":"unece:tradeName","@type":["rdf:Property","owl:DatatypeProperty"],"rdfs:label":"tradeName","schema:rangeIncludes":{"@id":"schema:Text"},"schema:domainIncludes":{"@id":"unece:TradeProduct"},"rdfs:comment":"A trade name, expressed as text, for this trade product."},{"@id":"unece:transportInformationNote","@type":["rdf:Property","owl:ObjectProperty"],"rdfs:label":"transportInformationNote","schema:rangeIncludes":{"@id":"unece:Note"},"schema:domainIncludes":{"@id":"unece:TradeProduct"},"rdfs:comment":"A textual or coded description, such as a remark or additional information."},{"@id":"unece:typeDescription","@type":["rdf:Property","owl:DatatypeProperty"],"rdfs:label":"typeDescription","schema:rangeIncludes":{"@id":"schema:Text"},"schema:domainIncludes":{"@id":"unece:TradeProduct"},"rdfs:comment":"A textual description of the type for this trade product."},{"@id":"unece:uRIId","@type":["rdf:Property","owl:DatatypeProperty"],"rdfs:label":"uRIId","schema:rangeIncludes":{"@id":"schema:Text"},"schema:domainIncludes":[{"@id":"unece:TradeProduct"},{"@id":"unece:TTTradeTransaction"},{"@id":"unece:Document"},{"@id":"unece:BinaryFile"},{"@id":"unece:Picture"},{"@id":"unece:Communication"},{"@id":"unece:Standard"},{"@id":"unece:SpecifiedCertification"}],"rdfs:comment":"A Uniform Resource Identifier (URI) for this specified certification."},{"@id":"unece:ultimateCustomerAssignedExtensionId","@type":["rdf:Property","owl:DatatypeProperty"],"rdfs:label":"ultimateCustomerAssignedExtensionId","schema:rangeIncludes":{"@id":"schema:Text"},"schema:domainIncludes":{"@id":"unece:TradeProduct"},"rdfs:comment":"An ultimate customer assigned extension identifier for this trade product."},{"@id":"unece:unitTypeCode","@type":["rdf:Property","owl:DatatypeProperty"],"rdfs:label":"unitTypeCode","schema:rangeIncludes":{"@id":"schema:Text"},"schema:domainIncludes":{"@id":"unece:TradeProduct"},"rdfs:comment":"A code specifying a type of unit for this trade product."},{"@id":"unece:useDescription","@type":["rdf:Property","owl:DatatypeProperty"],"rdfs:label":"useDescription","schema:rangeIncludes":{"@id":"schema:Text"},"schema:domainIncludes":{"@id":"unece:TradeProduct"},"rdfs:comment":"A textual description of a use of this trade product."},{"@id":"unece:variableMeasureIndicator","@type":["rdf:Property","owl:DatatypeProperty"],"rdfs:label":"variableMeasureIndicator","schema:rangeIncludes":{"@id":"schema:Boolean"},"schema:domainIncludes":{"@id":"unece:TradeProduct"},"rdfs:comment":"The indication of whether or not instances of this trade product have a variable measure, such as weight, length or volume."},{"@id":"unece:variantDescription","@type":["rdf:Property","owl:DatatypeProperty"],"rdfs:label":"variantDescription","schema:rangeIncludes":{"@id":"schema:Text"},"schema:domainIncludes":{"@id":"unece:TradeProduct"},"rdfs:comment":"A textual description of a variant of this trade product."},{"@id":"unece:variantId","@type":["rdf:Property","owl:DatatypeProperty"],"rdfs:label":"variantId","schema:rangeIncludes":{"@id":"schema:Text"},"schema:domainIncludes":{"@id":"unece:TradeProduct"},"rdfs:comment":"A variant identifier of this trade product."},{"@id":"unece:applicableDeliveryTerms","@type":["rdf:Property","owl:ObjectProperty"],"rdfs:label":"applicableDeliveryTerms","schema:rangeIncludes":{"@id":"unece:DeliveryTerms"},"schema:domainIncludes":[{"@id":"unece:HeaderTradeAgreement"},{"@id":"unece:LineTradeAgreement"}],"rdfs:comment":"Conditions agreed upon between the parties with regard to the delivery of goods and or services for trade purposes."},{"@id":"unece:applicableForecastTerms","@type":["rdf:Property","owl:ObjectProperty"],"rdfs:label":"applicableForecastTerms","schema:rangeIncludes":{"@id":"unece:ForecastTerms"},"schema:domainIncludes":[{"@id":"unece:HeaderTradeAgreement"},{"@id":"unece:LineTradeAgreement"}],"rdfs:comment":"The supply chain forecast terms applicable to this header trade agreement."},{"@id":"unece:applicableLocation","@type":["rdf:Property","owl:ObjectProperty"],"rdfs:label":"applicableLocation","schema:rangeIncludes":{"@id":"unece:LogisticsLocation"},"schema:domainIncludes":{"@id":"unece:HeaderTradeAgreement"},"rdfs:comment":"A logistics related physical location or place."},{"@id":"unece:applicablePaymentTerms","@type":["rdf:Property","owl:ObjectProperty"],"rdfs:label":"applicablePaymentTerms","schema:rangeIncludes":{"@id":"unece:PaymentTerms"},"schema:domainIncludes":{"@id":"unece:HeaderTradeAgreement"},"rdfs:comment":"Terms and conditions by which payment has been or will be made for trade purposes."},{"@id":"unece:applicableRegulatoryProcedure","@type":["rdf:Property","owl:ObjectProperty"],"rdfs:label":"applicableRegulatoryProcedure","schema:rangeIncludes":{"@id":"unece:RegulatoryProcedure"},"schema:domainIncludes":[{"@id":"unece:HeaderTradeAgreement"},{"@id":"unece:TransportMovement"},{"@id":"unece:Consignment"},{"@id":"unece:ConsignmentItem"}],"rdfs:comment":"A set of formal steps to satisfy a cross-border regulation, law or convention."},{"@id":"unece:blanketOrderDocument","@type":["rdf:Property","owl:ObjectProperty"],"rdfs:label":"blanketOrderDocument","schema:rangeIncludes":{"@id":"unece:Document"},"schema:domainIncludes":[{"@id":"unece:HeaderTradeAgreement"},{"@id":"unece:LineTradeAgreement"}],"rdfs:comment":"Written, printed or electronic matter that is referenced."},{"@id":"unece:buyerAgentParty","@type":["rdf:Property","owl:ObjectProperty"],"rdfs:label":"buyerAgentParty","schema:rangeIncludes":{"@id":"unece:TradeParty"},"schema:domainIncludes":{"@id":"unece:HeaderTradeAgreement"},"rdfs:comment":"The buyer agent party for this header trade agreement."},{"@id":"unece:buyerApprovedDateTime","@type":["rdf:Property","owl:DatatypeProperty"],"rdfs:label":"buyerApprovedDateTime","schema:rangeIncludes":{"@id":"schema:DateTime"},"schema:domainIncludes":[{"@id":"unece:HeaderTradeAgreement"},{"@id":"unece:LineTradeAgreement"}],"rdfs:comment":"The date, time, date time, or other date time value of approval by the buyer for this header trade agreement."},{"@id":"unece:buyerAssignedAccountantParty","@type":["rdf:Property","owl:ObjectProperty"],"rdfs:label":"buyerAssignedAccountantParty","schema:rangeIncludes":{"@id":"unece:TradeParty"},"schema:domainIncludes":{"@id":"unece:HeaderTradeAgreement"},"rdfs:comment":"The party assigned as an accountant by the buyer for this header trade agreement."},{"@id":"unece:buyerOrderDocument","@type":["rdf:Property","owl:ObjectProperty"],"rdfs:label":"buyerOrderDocument","schema:rangeIncludes":{"@id":"unece:Document"},"schema:domainIncludes":[{"@id":"unece:HeaderTradeAgreement"},{"@id":"unece:LineTradeAgreement"},{"@id":"unece:SubordinateLineTradeAgreement"}],"rdfs:comment":"Written, printed or electronic matter that is referenced."},{"@id":"unece:buyerParty","@type":["rdf:Property","owl:ObjectProperty"],"rdfs:label":"buyerParty","schema:rangeIncludes":{"@id":"unece:TradeParty"},"schema:domainIncludes":[{"@id":"unece:HeaderTradeAgreement"},{"@id":"unece:LineTradeAgreement"}],"rdfs:comment":"The buyer party for this header trade agreement."},{"@id":"unece:buyerReference","@type":["rdf:Property","owl:DatatypeProperty"],"rdfs:label":"buyerReference","schema:rangeIncludes":{"@id":"schema:Text"},"schema:domainIncludes":[{"@id":"unece:HeaderTradeAgreement"},{"@id":"unece:LineTradeAgreement"}],"rdfs:comment":"A buyer reference, expressed as text, for this header trade agreement."},{"@id":"unece:buyerRequisitionerParty","@type":["rdf:Property","owl:ObjectProperty"],"rdfs:label":"buyerRequisitionerParty","schema:rangeIncludes":{"@id":"unece:TradeParty"},"schema:domainIncludes":[{"@id":"unece:HeaderTradeAgreement"},{"@id":"unece:LineTradeAgreement"}],"rdfs:comment":"A party who is a buyer requisitioner in this header trade agreement."},{"@id":"unece:buyerTaxRepresentativeParty","@type":["rdf:Property","owl:ObjectProperty"],"rdfs:label":"buyerTaxRepresentativeParty","schema:rangeIncludes":{"@id":"unece:TradeParty"},"schema:domainIncludes":{"@id":"unece:HeaderTradeAgreement"},"rdfs:comment":"The party acting as a tax representative for the buyer for this header trade agreement."},{"@id":"unece:carrierParty","@type":["rdf:Property","owl:ObjectProperty"],"rdfs:label":"carrierParty","schema:rangeIncludes":{"@id":"unece:TradeParty"},"schema:domainIncludes":[{"@id":"unece:HeaderTradeAgreement"},{"@id":"unece:LineTradeAgreement"},{"@id":"unece:LogisticsTransportEquipment"},{"@id":"unece:TransportMovement"},{"@id":"unece:Consignment"}],"rdfs:comment":"A carrier party for this line trade agreement."},{"@id":"unece:catalogueDocument","@type":["rdf:Property","owl:ObjectProperty"],"rdfs:label":"catalogueDocument","schema:rangeIncludes":{"@id":"unece:Document"},"schema:domainIncludes":[{"@id":"unece:HeaderTradeAgreement"},{"@id":"unece:LineTradeAgreement"}],"rdfs:comment":"Written, printed or electronic matter that is referenced."},{"@id":"unece:catalogueInformationProviderParty","@type":["rdf:Property","owl:ObjectProperty"],"rdfs:label":"catalogueInformationProviderParty","schema:rangeIncludes":{"@id":"unece:TradeParty"},"schema:domainIncludes":[{"@id":"unece:HeaderTradeAgreement"},{"@id":"unece:LineTradeAgreement"}],"rdfs:comment":"The party that provides catalogue information for this header trade agreement."},{"@id":"unece:catalogueInformationReceiverParty","@type":["rdf:Property","owl:ObjectProperty"],"rdfs:label":"catalogueInformationReceiverParty","schema:rangeIncludes":{"@id":"unece:TradeParty"},"schema:domainIncludes":{"@id":"unece:HeaderTradeAgreement"},"rdfs:comment":"The party that receives catalogue information for this header trade agreement."},{"@id":"unece:catalogueRequestDocument","@type":["rdf:Property","owl:ObjectProperty"],"rdfs:label":"catalogueRequestDocument","schema:rangeIncludes":{"@id":"unece:Document"},"schema:domainIncludes":{"@id":"unece:HeaderTradeAgreement"},"rdfs:comment":"Written, printed or electronic matter that is referenced."},{"@id":"unece:catalogueSubscriptionDocument","@type":["rdf:Property","owl:ObjectProperty"],"rdfs:label":"catalogueSubscriptionDocument","schema:rangeIncludes":{"@id":"unece:Document"},"schema:domainIncludes":{"@id":"unece:HeaderTradeAgreement"},"rdfs:comment":"Written, printed or electronic matter that is referenced."},{"@id":"unece:demandForecastDocument","@type":["rdf:Property","owl:ObjectProperty"],"rdfs:label":"demandForecastDocument","schema:rangeIncludes":{"@id":"unece:Document"},"schema:domainIncludes":[{"@id":"unece:HeaderTradeAgreement"},{"@id":"unece:LineTradeAgreement"}],"rdfs:comment":"Written, printed or electronic matter that is referenced."},{"@id":"unece:engineeringChangeDocument","@type":["rdf:Property","owl:ObjectProperty"],"rdfs:label":"engineeringChangeDocument","schema:rangeIncludes":{"@id":"unece:Document"},"schema:domainIncludes":[{"@id":"unece:HeaderTradeAgreement"},{"@id":"unece:LineTradeAgreement"}],"rdfs:comment":"Written, printed or electronic matter that is referenced."},{"@id":"unece:exportLicenceDocument","@type":["rdf:Property","owl:ObjectProperty"],"rdfs:label":"exportLicenceDocument","schema:rangeIncludes":{"@id":"unece:Document"},"schema:domainIncludes":[{"@id":"unece:HeaderTradeAgreement"},{"@id":"unece:LineTradeAgreement"}],"rdfs:comment":"Written, printed or electronic matter that is referenced."},{"@id":"unece:impactCode","@type":["rdf:Property","owl:DatatypeProperty"],"rdfs:label":"impactCode","schema:rangeIncludes":{"@id":"schema:Text"},"schema:domainIncludes":[{"@id":"unece:HeaderTradeAgreement"},{"@id":"unece:LineTradeAgreement"}],"rdfs:comment":"The code specifying the impact for this header trade agreement."},{"@id":"unece:importLicenceDocument","@type":["rdf:Property","owl:ObjectProperty"],"rdfs:label":"importLicenceDocument","schema:rangeIncludes":{"@id":"unece:Document"},"schema:domainIncludes":[{"@id":"unece:HeaderTradeAgreement"},{"@id":"unece:LineTradeAgreement"}],"rdfs:comment":"Written, printed or electronic matter that is referenced."},{"@id":"unece:letterOfCreditDocument","@type":["rdf:Property","owl:ObjectProperty"],"rdfs:label":"letterOfCreditDocument","schema:rangeIncludes":{"@id":"unece:Document"},"schema:domainIncludes":[{"@id":"unece:HeaderTradeAgreement"},{"@id":"unece:LineTradeAgreement"},{"@id":"unece:HeaderTradeSettlement"}],"rdfs:comment":"Written, printed or electronic matter that is referenced."},{"@id":"unece:marketplaceOrderDocument","@type":["rdf:Property","owl:ObjectProperty"],"rdfs:label":"marketplaceOrderDocument","schema:rangeIncludes":{"@id":"unece:Document"},"schema:domainIncludes":[{"@id":"unece:HeaderTradeAgreement"},{"@id":"unece:LineTradeAgreement"}],"rdfs:comment":"Written, printed or electronic matter that is referenced."},{"@id":"unece:orderResponseDocument","@type":["rdf:Property","owl:ObjectProperty"],"rdfs:label":"orderResponseDocument","schema:rangeIncludes":{"@id":"unece:Document"},"schema:domainIncludes":{"@id":"unece:HeaderTradeAgreement"},"rdfs:comment":"Written, printed or electronic matter that is referenced."},{"@id":"unece:originalOrderDocument","@type":["rdf:Property","owl:ObjectProperty"],"rdfs:label":"originalOrderDocument","schema:rangeIncludes":{"@id":"unece:Document"},"schema:domainIncludes":[{"@id":"unece:HeaderTradeAgreement"},{"@id":"unece:LineTradeAgreement"}],"rdfs:comment":"Written, printed or electronic matter that is referenced."},{"@id":"unece:previousOrderChangeDocument","@type":["rdf:Property","owl:ObjectProperty"],"rdfs:label":"previousOrderChangeDocument","schema:rangeIncludes":{"@id":"unece:Document"},"schema:domainIncludes":{"@id":"unece:HeaderTradeAgreement"},"rdfs:comment":"Written, printed or electronic matter that is referenced."},{"@id":"unece:previousOrderDocument","@type":["rdf:Property","owl:ObjectProperty"],"rdfs:label":"previousOrderDocument","schema:rangeIncludes":{"@id":"unece:Document"},"schema:domainIncludes":[{"@id":"unece:HeaderTradeAgreement"},{"@id":"unece:LineTradeAgreement"}],"rdfs:comment":"Written, printed or electronic matter that is referenced."},{"@id":"unece:previousOrderResponseDocument","@type":["rdf:Property","owl:ObjectProperty"],"rdfs:label":"previousOrderResponseDocument","schema:rangeIncludes":{"@id":"unece:Document"},"schema:domainIncludes":{"@id":"unece:HeaderTradeAgreement"},"rdfs:comment":"Written, printed or electronic matter that is referenced."},{"@id":"unece:priceListDocument","@type":["rdf:Property","owl:ObjectProperty"],"rdfs:label":"priceListDocument","schema:rangeIncludes":{"@id":"unece:Document"},"schema:domainIncludes":[{"@id":"unece:HeaderTradeAgreement"},{"@id":"unece:LineTradeAgreement"}],"rdfs:comment":"Written, printed or electronic matter that is referenced."},{"@id":"unece:pricingBaseApplicableLocation","@type":["rdf:Property","owl:ObjectProperty"],"rdfs:label":"pricingBaseApplicableLocation","schema:rangeIncludes":{"@id":"unece:LogisticsLocation"},"schema:domainIncludes":{"@id":"unece:HeaderTradeAgreement"},"rdfs:comment":"A logistics related physical location or place."},{"@id":"unece:primeContractSellerParty","@type":["rdf:Property","owl:ObjectProperty"],"rdfs:label":"primeContractSellerParty","schema:rangeIncludes":{"@id":"unece:TradeParty"},"schema:domainIncludes":[{"@id":"unece:HeaderTradeAgreement"},{"@id":"unece:LineTradeAgreement"}],"rdfs:comment":"The seller party acting as the prime contractor for this header trade agreement."},{"@id":"unece:priorityCode","@type":["rdf:Property","owl:DatatypeProperty"],"rdfs:label":"priorityCode","schema:rangeIncludes":{"@id":"schema:Text"},"schema:domainIncludes":[{"@id":"unece:HeaderTradeAgreement"},{"@id":"unece:LineTradeAgreement"},{"@id":"unece:PaymentTradeSettlement"}],"rdfs:comment":"The code specifying the priority for this header trade agreement."},{"@id":"unece:priorityDescriptionCode","@type":["rdf:Property","owl:DatatypeProperty"],"rdfs:label":"priorityDescriptionCode","schema:rangeIncludes":{"@id":"unece:PriorityDescriptionCodeList"},"schema:domainIncludes":[{"@id":"unece:HeaderTradeAgreement"},{"@id":"unece:LineTradeAgreement"}],"rdfs:comment":"The code specifying the delivery priority for this header trade agreement."},{"@id":"unece:procurementParty","@type":["rdf:Property","owl:ObjectProperty"],"rdfs:label":"procurementParty","schema:rangeIncludes":{"@id":"unece:TradeParty"},"schema:domainIncludes":[{"@id":"unece:HeaderTradeAgreement"},{"@id":"unece:LineTradeAgreement"}],"rdfs:comment":"The procurement party for this header trade agreement."},{"@id":"unece:productEndUserParty","@type":["rdf:Property","owl:ObjectProperty"],"rdfs:label":"productEndUserParty","schema:rangeIncludes":{"@id":"unece:TradeParty"},"schema:domainIncludes":[{"@id":"unece:HeaderTradeAgreement"},{"@id":"unece:LineTradeAgreement"}],"rdfs:comment":"The party acting as the end user for the products in this header trade agreement."},{"@id":"unece:promotionalDealDocument","@type":["rdf:Property","owl:ObjectProperty"],"rdfs:label":"promotionalDealDocument","schema:rangeIncludes":{"@id":"unece:Document"},"schema:domainIncludes":[{"@id":"unece:HeaderTradeAgreement"},{"@id":"unece:LineTradeAgreement"}],"rdfs:comment":"Written, printed or electronic matter that is referenced."},{"@id":"unece:purchaseConditionsDocument","@type":["rdf:Property","owl:ObjectProperty"],"rdfs:label":"purchaseConditionsDocument","schema:rangeIncludes":{"@id":"unece:Document"},"schema:domainIncludes":{"@id":"unece:HeaderTradeAgreement"},"rdfs:comment":"Written, printed or electronic matter that is referenced."},{"@id":"unece:quotationDocument","@type":["rdf:Property","owl:ObjectProperty"],"rdfs:label":"quotationDocument","schema:rangeIncludes":{"@id":"unece:Document"},"schema:domainIncludes":[{"@id":"unece:HeaderTradeAgreement"},{"@id":"unece:LineTradeAgreement"}],"rdfs:comment":"Written, printed or electronic matter that is referenced."},{"@id":"unece:quotationProposalDocument","@type":["rdf:Property","owl:ObjectProperty"],"rdfs:label":"quotationProposalDocument","schema:rangeIncludes":{"@id":"unece:Document"},"schema:domainIncludes":[{"@id":"unece:HeaderTradeAgreement"},{"@id":"unece:LineTradeAgreement"}],"rdfs:comment":"Written, printed or electronic matter that is referenced."},{"@id":"unece:quotationProposalResponseDocument","@type":["rdf:Property","owl:ObjectProperty"],"rdfs:label":"quotationProposalResponseDocument","schema:rangeIncludes":{"@id":"unece:Document"},"schema:domainIncludes":[{"@id":"unece:HeaderTradeAgreement"},{"@id":"unece:LineTradeAgreement"}],"rdfs:comment":"Written, printed or electronic matter that is referenced."},{"@id":"unece:quotationRequestDocument","@type":["rdf:Property","owl:ObjectProperty"],"rdfs:label":"quotationRequestDocument","schema:rangeIncludes":{"@id":"unece:Document"},"schema:domainIncludes":[{"@id":"unece:HeaderTradeAgreement"},{"@id":"unece:LineTradeAgreement"}],"rdfs:comment":"Written, printed or electronic matter that is referenced."},{"@id":"unece:quotationRequestResponseDocument","@type":["rdf:Property","owl:ObjectProperty"],"rdfs:label":"quotationRequestResponseDocument","schema:rangeIncludes":{"@id":"unece:Document"},"schema:domainIncludes":[{"@id":"unece:HeaderTradeAgreement"},{"@id":"unece:LineTradeAgreement"}],"rdfs:comment":"Written, printed or electronic matter that is referenced."},{"@id":"unece:quoteReferencedWorkflowObject","@type":["rdf:Property","owl:ObjectProperty"],"rdfs:label":"quoteReferencedWorkflowObject","schema:rangeIncludes":{"@id":"unece:WorkflowObject"},"schema:domainIncludes":{"@id":"unece:HeaderTradeAgreement"},"rdfs:comment":"An object used in the management of the status changes in a business process."},{"@id":"unece:reference","@type":["rdf:Property","owl:DatatypeProperty"],"rdfs:label":"reference","schema:rangeIncludes":{"@id":"schema:Text"},"schema:domainIncludes":[{"@id":"unece:HeaderTradeAgreement"},{"@id":"unece:LineTradeAgreement"},{"@id":"unece:Picture"}],"rdfs:comment":"A reference, expressed as text, for this header trade agreement."},{"@id":"unece:relevantParty","@type":["rdf:Property","owl:ObjectProperty"],"rdfs:label":"relevantParty","schema:rangeIncludes":{"@id":"unece:TradeParty"},"schema:domainIncludes":[{"@id":"unece:HeaderTradeAgreement"},{"@id":"unece:LineTradeAgreement"},{"@id":"unece:HeaderTradeSettlement"}],"rdfs:comment":"A party relevant for this line trade agreement."},{"@id":"unece:requisitionDocument","@type":["rdf:Property","owl:ObjectProperty"],"rdfs:label":"requisitionDocument","schema:rangeIncludes":{"@id":"unece:Document"},"schema:domainIncludes":[{"@id":"unece:HeaderTradeAgreement"},{"@id":"unece:LineTradeAgreement"}],"rdfs:comment":"Written, printed or electronic matter that is referenced."},{"@id":"unece:requisitionerDocument","@type":["rdf:Property","owl:ObjectProperty"],"rdfs:label":"requisitionerDocument","schema:rangeIncludes":{"@id":"unece:Document"},"schema:domainIncludes":[{"@id":"unece:HeaderTradeAgreement"},{"@id":"unece:LineTradeAgreement"}],"rdfs:comment":"Written, printed or electronic matter that is referenced."},{"@id":"unece:revisionId","@type":["rdf:Property","owl:DatatypeProperty"],"rdfs:label":"revisionId","schema:rangeIncludes":{"@id":"schema:Text"},"schema:domainIncludes":[{"@id":"unece:HeaderTradeAgreement"},{"@id":"unece:LineTradeAgreement"},{"@id":"unece:Document"},{"@id":"unece:ExchangedDocument"}],"rdfs:comment":"A unique identifier for a revision of this referenced document."},{"@id":"unece:salesAgentParty","@type":["rdf:Property","owl:ObjectProperty"],"rdfs:label":"salesAgentParty","schema:rangeIncludes":{"@id":"unece:TradeParty"},"schema:domainIncludes":{"@id":"unece:HeaderTradeAgreement"},"rdfs:comment":"The agent party representing the seller for this header trade agreement."},{"@id":"unece:salesConditionsDocument","@type":["rdf:Property","owl:ObjectProperty"],"rdfs:label":"salesConditionsDocument","schema:rangeIncludes":{"@id":"unece:Document"},"schema:domainIncludes":[{"@id":"unece:HeaderTradeAgreement"},{"@id":"unece:LineTradeAgreement"}],"rdfs:comment":"Written, printed or electronic matter that is referenced."},{"@id":"unece:salesReportDocument","@type":["rdf:Property","owl:ObjectProperty"],"rdfs:label":"salesReportDocument","schema:rangeIncludes":{"@id":"unece:Document"},"schema:domainIncludes":[{"@id":"unece:HeaderTradeAgreement"},{"@id":"unece:LineTradeAgreement"}],"rdfs:comment":"Written, printed or electronic matter that is referenced."},{"@id":"unece:sellerAssignedAccountantParty","@type":["rdf:Property","owl:ObjectProperty"],"rdfs:label":"sellerAssignedAccountantParty","schema:rangeIncludes":{"@id":"unece:TradeParty"},"schema:domainIncludes":{"@id":"unece:HeaderTradeAgreement"},"rdfs:comment":"The party assigned as an accountant by the seller for this header trade agreement."},{"@id":"unece:sellerOrderDocument","@type":["rdf:Property","owl:ObjectProperty"],"rdfs:label":"sellerOrderDocument","schema:rangeIncludes":{"@id":"unece:Document"},"schema:domainIncludes":[{"@id":"unece:HeaderTradeAgreement"},{"@id":"unece:LineTradeAgreement"},{"@id":"unece:SubordinateLineTradeAgreement"}],"rdfs:comment":"Written, printed or electronic matter that is referenced."},{"@id":"unece:sellerParty","@type":["rdf:Property","owl:ObjectProperty"],"rdfs:label":"sellerParty","schema:rangeIncludes":{"@id":"unece:TradeParty"},"schema:domainIncludes":[{"@id":"unece:HeaderTradeAgreement"},{"@id":"unece:LineTradeAgreement"}],"rdfs:comment":"The seller party for this header trade agreement."},{"@id":"unece:sellerReference","@type":["rdf:Property","owl:DatatypeProperty"],"rdfs:label":"sellerReference","schema:rangeIncludes":{"@id":"schema:Text"},"schema:domainIncludes":[{"@id":"unece:HeaderTradeAgreement"},{"@id":"unece:LineTradeAgreement"}],"rdfs:comment":"A seller reference, expressed as text, for this header trade agreement."},{"@id":"unece:sellerTaxRepresentativeParty","@type":["rdf:Property","owl:ObjectProperty"],"rdfs:label":"sellerTaxRepresentativeParty","schema:rangeIncludes":{"@id":"unece:TradeParty"},"schema:domainIncludes":{"@id":"unece:HeaderTradeAgreement"},"rdfs:comment":"The party acting as a tax representative for the seller for this header trade agreement."},{"@id":"unece:shippingPeriod","@type":["rdf:Property","owl:ObjectProperty"],"rdfs:label":"shippingPeriod","schema:rangeIncludes":{"@id":"unece:SpecifiedPeriod"},"schema:domainIncludes":{"@id":"unece:HeaderTradeAgreement"},"rdfs:comment":"A specified period of time."},{"@id":"unece:specifiedProject","@type":["rdf:Property","owl:ObjectProperty"],"rdfs:label":"specifiedProject","schema:rangeIncludes":{"@id":"unece:Project"},"schema:domainIncludes":{"@id":"unece:HeaderTradeAgreement"},"rdfs:comment":"An endeavour carefully planned to achieve a procurement of goods, works and service."},{"@id":"unece:supplyInstructionDocument","@type":["rdf:Property","owl:ObjectProperty"],"rdfs:label":"supplyInstructionDocument","schema:rangeIncludes":{"@id":"unece:Document"},"schema:domainIncludes":[{"@id":"unece:HeaderTradeAgreement"},{"@id":"unece:LineTradeAgreement"}],"rdfs:comment":"Written, printed or electronic matter that is referenced."},{"@id":"unece:targetMarketCountry","@type":["rdf:Property","owl:ObjectProperty"],"rdfs:label":"targetMarketCountry","schema:rangeIncludes":{"@id":"unece:Country"},"schema:domainIncludes":[{"@id":"unece:HeaderTradeAgreement"},{"@id":"unece:LineTradeAgreement"}],"rdfs:comment":"The area of land that belongs to a nation together with its properties, such as population, political organization, etc., used or referenced for trade purposes."},{"@id":"unece:ultimateCustomerOrderDocument","@type":["rdf:Property","owl:ObjectProperty"],"rdfs:label":"ultimateCustomerOrderDocument","schema:rangeIncludes":{"@id":"unece:Document"},"schema:domainIncludes":[{"@id":"unece:HeaderTradeAgreement"},{"@id":"unece:LineTradeAgreement"}],"rdfs:comment":"Written, printed or electronic matter that is referenced."},{"@id":"unece:agreedPriceProductPrice","@type":["rdf:Property","owl:ObjectProperty"],"rdfs:label":"agreedPriceProductPrice","schema:rangeIncludes":{"@id":"unece:TradePrice"},"schema:domainIncludes":{"@id":"unece:LineTradeAgreement"},"rdfs:comment":"A sum of money for which something is or may be bought or sold for trade purposes."},{"@id":"unece:deliveryOrderFulfilmentLeadTimeMeasure","@type":["rdf:Property","owl:ObjectProperty"],"rdfs:label":"deliveryOrderFulfilmentLeadTimeMeasure","schema:rangeIncludes":{"@id":"unece:DurationUnitMeasureType"},"schema:domainIncludes":{"@id":"unece:LineTradeAgreement"},"rdfs:comment":""},{"@id":"unece:exclusivityPeriod","@type":["rdf:Property","owl:ObjectProperty"],"rdfs:label":"exclusivityPeriod","schema:rangeIncludes":{"@id":"unece:SpecifiedPeriod"},"schema:domainIncludes":{"@id":"unece:LineTradeAgreement"},"rdfs:comment":"A specified period of time."},{"@id":"unece:grossPriceProductPrice","@type":["rdf:Property","owl:ObjectProperty"],"rdfs:label":"grossPriceProductPrice","schema:rangeIncludes":{"@id":"unece:TradePrice"},"schema:domainIncludes":[{"@id":"unece:LineTradeAgreement"},{"@id":"unece:SubordinateLineTradeAgreement"}],"rdfs:comment":"A sum of money for which something is or may be bought or sold for trade purposes."},{"@id":"unece:guaranteedProductLifeSpanPeriod","@type":["rdf:Property","owl:ObjectProperty"],"rdfs:label":"guaranteedProductLifeSpanPeriod","schema:rangeIncludes":{"@id":"unece:SpecifiedPeriod"},"schema:domainIncludes":{"@id":"unece:LineTradeAgreement"},"rdfs:comment":"A specified period of time."},{"@id":"unece:immediatePreviousPriceListDocument","@type":["rdf:Property","owl:ObjectProperty"],"rdfs:label":"immediatePreviousPriceListDocument","schema:rangeIncludes":{"@id":"unece:Document"},"schema:domainIncludes":{"@id":"unece:LineTradeAgreement"},"rdfs:comment":"Written, printed or electronic matter that is referenced."},{"@id":"unece:includedMarketplace","@type":["rdf:Property","owl:ObjectProperty"],"rdfs:label":"includedMarketplace","schema:rangeIncludes":{"@id":"unece:Marketplace"},"schema:domainIncludes":{"@id":"unece:LineTradeAgreement"},"rdfs:comment":"A marketplace included in this line trade agreement."},{"@id":"unece:incrementalProductOrderableQuantity","@type":["rdf:Property","owl:ObjectProperty"],"rdfs:label":"incrementalProductOrderableQuantity","schema:rangeIncludes":{"@id":"unece:QuantityType"},"schema:domainIncludes":{"@id":"unece:LineTradeAgreement"},"rdfs:comment":""},{"@id":"unece:informationUseRestrictionIndicator","@type":["rdf:Property","owl:DatatypeProperty"],"rdfs:label":"informationUseRestrictionIndicator","schema:rangeIncludes":{"@id":"schema:Boolean"},"schema:domainIncludes":{"@id":"unece:LineTradeAgreement"},"rdfs:comment":"The indication of whether or not the use of the information provided in this line trade agreement is restricted."},{"@id":"unece:itemBuyerParty","@type":["rdf:Property","owl:ObjectProperty"],"rdfs:label":"itemBuyerParty","schema:rangeIncludes":{"@id":"unece:TradeParty"},"schema:domainIncludes":{"@id":"unece:LineTradeAgreement"},"rdfs:comment":"The item buyer party for this line trade agreement."},{"@id":"unece:itemSellerParty","@type":["rdf:Property","owl:ObjectProperty"],"rdfs:label":"itemSellerParty","schema:rangeIncludes":{"@id":"unece:TradeParty"},"schema:domainIncludes":{"@id":"unece:LineTradeAgreement"},"rdfs:comment":"The item seller party for this line trade agreement."},{"@id":"unece:maximumOrderQuantityOrderingPeriod","@type":["rdf:Property","owl:ObjectProperty"],"rdfs:label":"maximumOrderQuantityOrderingPeriod","schema:rangeIncludes":{"@id":"unece:SpecifiedPeriod"},"schema:domainIncludes":{"@id":"unece:LineTradeAgreement"},"rdfs:comment":"A specified period of time."},{"@id":"unece:maximumProductOrderableQuantity","@type":["rdf:Property","owl:ObjectProperty"],"rdfs:label":"maximumProductOrderableQuantity","schema:rangeIncludes":{"@id":"unece:QuantityType"},"schema:domainIncludes":{"@id":"unece:LineTradeAgreement"},"rdfs:comment":""},{"@id":"unece:minimumOrderQuantityOrderingPeriod","@type":["rdf:Property","owl:ObjectProperty"],"rdfs:label":"minimumOrderQuantityOrderingPeriod","schema:rangeIncludes":{"@id":"unece:SpecifiedPeriod"},"schema:domainIncludes":{"@id":"unece:LineTradeAgreement"},"rdfs:comment":"A specified period of time."},{"@id":"unece:minimumProductOrderableQuantity","@type":["rdf:Property","owl:ObjectProperty"],"rdfs:label":"minimumProductOrderableQuantity","schema:rangeIncludes":{"@id":"unece:QuantityType"},"schema:domainIncludes":{"@id":"unece:LineTradeAgreement"},"rdfs:comment":""},{"@id":"unece:netPriceProductPrice","@type":["rdf:Property","owl:ObjectProperty"],"rdfs:label":"netPriceProductPrice","schema:rangeIncludes":{"@id":"unece:TradePrice"},"schema:domainIncludes":[{"@id":"unece:LineTradeAgreement"},{"@id":"unece:SubordinateLineTradeAgreement"}],"rdfs:comment":"A sum of money for which something is or may be bought or sold for trade purposes."},{"@id":"unece:orderPriceProductPrice","@type":["rdf:Property","owl:ObjectProperty"],"rdfs:label":"orderPriceProductPrice","schema:rangeIncludes":{"@id":"unece:TradePrice"},"schema:domainIncludes":{"@id":"unece:LineTradeAgreement"},"rdfs:comment":"A sum of money for which something is or may be bought or sold for trade purposes."},{"@id":"unece:orderProductUnitMeasureCode","@type":["rdf:Property","owl:DatatypeProperty"],"rdfs:label":"orderProductUnitMeasureCode","schema:rangeIncludes":{"@id":"schema:Text"},"schema:domainIncludes":{"@id":"unece:LineTradeAgreement"},"rdfs:comment":"The code specifying the order product unit of measure, such as kilogram or litre, for this line trade agreement."},{"@id":"unece:orderingSpecifiedPeriod","@type":["rdf:Property","owl:ObjectProperty"],"rdfs:label":"orderingSpecifiedPeriod","schema:rangeIncludes":{"@id":"unece:SpecifiedPeriod"},"schema:domainIncludes":{"@id":"unece:LineTradeAgreement"},"rdfs:comment":"A specified period of time."},{"@id":"unece:pickUpOrderFulfilmentLeadTimeMeasure","@type":["rdf:Property","owl:ObjectProperty"],"rdfs:label":"pickUpOrderFulfilmentLeadTimeMeasure","schema:rangeIncludes":{"@id":"unece:DurationUnitMeasureType"},"schema:domainIncludes":{"@id":"unece:LineTradeAgreement"},"rdfs:comment":""},{"@id":"unece:productAvailabilityCode","@type":["rdf:Property","owl:DatatypeProperty"],"rdfs:label":"productAvailabilityCode","schema:rangeIncludes":{"@id":"schema:Text"},"schema:domainIncludes":{"@id":"unece:LineTradeAgreement"},"rdfs:comment":"The code specifying the product availability according to this line trade agreement."},{"@id":"unece:productMadeToOrderIndicator","@type":["rdf:Property","owl:DatatypeProperty"],"rdfs:label":"productMadeToOrderIndicator","schema:rangeIncludes":{"@id":"schema:Boolean"},"schema:domainIncludes":{"@id":"unece:LineTradeAgreement"},"rdfs:comment":"The indication of whether or not, according to this line trade agreement, the product is manufactured, built or customized only after receipt of order."},{"@id":"unece:productOrderableIndicator","@type":["rdf:Property","owl:DatatypeProperty"],"rdfs:label":"productOrderableIndicator","schema:rangeIncludes":{"@id":"schema:Boolean"},"schema:domainIncludes":{"@id":"unece:LineTradeAgreement"},"rdfs:comment":"The indication of whether or not the product can be ordered according to this line trade agreement."},{"@id":"unece:productReorderableIndicator","@type":["rdf:Property","owl:DatatypeProperty"],"rdfs:label":"productReorderableIndicator","schema:rangeIncludes":{"@id":"schema:Boolean"},"schema:domainIncludes":{"@id":"unece:LineTradeAgreement"},"rdfs:comment":"The indication of whether or not the product can be reordered according to this line trade agreement."},{"@id":"unece:resalePeriod","@type":["rdf:Property","owl:ObjectProperty"],"rdfs:label":"resalePeriod","schema:rangeIncludes":{"@id":"unece:SpecifiedPeriod"},"schema:domainIncludes":{"@id":"unece:LineTradeAgreement"},"rdfs:comment":"A specified period of time."},{"@id":"unece:resaleProductUnitMeasureCode","@type":["rdf:Property","owl:DatatypeProperty"],"rdfs:label":"resaleProductUnitMeasureCode","schema:rangeIncludes":{"@id":"schema:Text"},"schema:domainIncludes":{"@id":"unece:LineTradeAgreement"},"rdfs:comment":"The code specifying the resale product unit of measure, such as kilogram or litre, for this trade line agreement."},{"@id":"unece:supportCentreParty","@type":["rdf:Property","owl:ObjectProperty"],"rdfs:label":"supportCentreParty","schema:rangeIncludes":{"@id":"unece:TradeParty"},"schema:domainIncludes":{"@id":"unece:LineTradeAgreement"},"rdfs:comment":"The support centre party for this line trade agreement."},{"@id":"unece:amountDirectionCode","@type":["rdf:Property","owl:DatatypeProperty"],"rdfs:label":"amountDirectionCode","schema:rangeIncludes":{"@id":"schema:Text"},"schema:domainIncludes":[{"@id":"unece:LineTradeSettlement"},{"@id":"unece:SubordinateLineTradeSettlement"}],"rdfs:comment":"The code, specifying the direction, either an addition or subtraction, for the amount of this line trade settlement."},{"@id":"unece:applicableTax","@type":["rdf:Property","owl:ObjectProperty"],"rdfs:label":"applicableTax","schema:rangeIncludes":{"@id":"unece:TradeTax"},"schema:domainIncludes":[{"@id":"unece:LineTradeSettlement"},{"@id":"unece:SubordinateLineTradeSettlement"},{"@id":"unece:HeaderTradeSettlement"},{"@id":"unece:PaymentTradeSettlement"},{"@id":"unece:RegulatoryProcedure"}],"rdfs:comment":"A tax applicable to this header trade settlement."},{"@id":"unece:associatedDocument","@type":["rdf:Property","owl:ObjectProperty"],"rdfs:label":"associatedDocument","schema:rangeIncludes":{"@id":"unece:Document"},"schema:domainIncludes":[{"@id":"unece:LineTradeSettlement"},{"@id":"unece:SupplyChainTradeTransaction"},{"@id":"unece:ExchangedDeclaration"},{"@id":"unece:CurrencyExchange"},{"@id":"unece:TradePrice"},{"@id":"unece:LogisticsTransportEquipment"},{"@id":"unece:Consignment"},{"@id":"unece:ConsignmentItem"}],"rdfs:comment":"Written, printed or electronic matter that is referenced."},{"@id":"unece:billingPeriod","@type":["rdf:Property","owl:ObjectProperty"],"rdfs:label":"billingPeriod","schema:rangeIncludes":{"@id":"unece:SpecifiedPeriod"},"schema:domainIncludes":[{"@id":"unece:LineTradeSettlement"},{"@id":"unece:HeaderTradeSettlement"}],"rdfs:comment":"A specified period of time."},{"@id":"unece:creditorReferenceTypeCode","@type":["rdf:Property","owl:DatatypeProperty"],"rdfs:label":"creditorReferenceTypeCode","schema:rangeIncludes":{"@id":"schema:Text"},"schema:domainIncludes":[{"@id":"unece:LineTradeSettlement"},{"@id":"unece:HeaderTradeSettlement"}],"rdfs:comment":"A code specifying a type of creditor reference for this line trade settlement."},{"@id":"unece:discountIndicator","@type":["rdf:Property","owl:DatatypeProperty"],"rdfs:label":"discountIndicator","schema:rangeIncludes":{"@id":"schema:Boolean"},"schema:domainIncludes":[{"@id":"unece:LineTradeSettlement"},{"@id":"unece:HeaderTradeSettlement"}],"rdfs:comment":"The indication of whether or not a discount applies to the item in this line trade settlement."},{"@id":"unece:invoiceDateTime","@type":["rdf:Property","owl:DatatypeProperty"],"rdfs:label":"invoiceDateTime","schema:rangeIncludes":{"@id":"schema:Text"},"schema:domainIncludes":[{"@id":"unece:LineTradeSettlement"},{"@id":"unece:HeaderTradeSettlement"}],"rdfs:comment":"The date, time, date time or other date time value of the invoice in this header trade settlement."},{"@id":"unece:invoiceDocument","@type":["rdf:Property","owl:ObjectProperty"],"rdfs:label":"invoiceDocument","schema:rangeIncludes":{"@id":"unece:Document"},"schema:domainIncludes":[{"@id":"unece:LineTradeSettlement"},{"@id":"unece:HeaderTradeSettlement"}],"rdfs:comment":"Written, printed or electronic matter that is referenced."},{"@id":"unece:invoiceIssuerReference","@type":["rdf:Property","owl:DatatypeProperty"],"rdfs:label":"invoiceIssuerReference","schema:rangeIncludes":{"@id":"schema:Text"},"schema:domainIncludes":[{"@id":"unece:LineTradeSettlement"},{"@id":"unece:HeaderTradeSettlement"}],"rdfs:comment":"The invoice issuer reference, expressed as text, for this header trade settlement."},{"@id":"unece:invoiceeParty","@type":["rdf:Property","owl:ObjectProperty"],"rdfs:label":"invoiceeParty","schema:rangeIncludes":{"@id":"unece:TradeParty"},"schema:domainIncludes":[{"@id":"unece:LineTradeSettlement"},{"@id":"unece:HeaderTradeSettlement"}],"rdfs:comment":"The party to whom an invoice is issued for this header trade settlement."},{"@id":"unece:payableSpecifiedAccountingAccount","@type":["rdf:Property","owl:ObjectProperty"],"rdfs:label":"payableSpecifiedAccountingAccount","schema:rangeIncludes":{"@id":"unece:AccountingAccount"},"schema:domainIncludes":[{"@id":"unece:LineTradeSettlement"},{"@id":"unece:HeaderTradeSettlement"}],"rdfs:comment":"A specific trade account for recording debits and credits to general accounting, cost accounting or budget accounting."},{"@id":"unece:payerParty","@type":["rdf:Property","owl:ObjectProperty"],"rdfs:label":"payerParty","schema:rangeIncludes":{"@id":"unece:TradeParty"},"schema:domainIncludes":[{"@id":"unece:LineTradeSettlement"},{"@id":"unece:HeaderTradeSettlement"},{"@id":"unece:PaymentTradeSettlement"}],"rdfs:comment":"The payer party for this header trade settlement."},{"@id":"unece:payerReference","@type":["rdf:Property","owl:DatatypeProperty"],"rdfs:label":"payerReference","schema:rangeIncludes":{"@id":"schema:Text"},"schema:domainIncludes":[{"@id":"unece:LineTradeSettlement"},{"@id":"unece:HeaderTradeSettlement"}],"rdfs:comment":"The payer reference, expressed as text, for this header trade settlement."},{"@id":"unece:paymentAmount","@type":["rdf:Property","owl:ObjectProperty"],"rdfs:label":"paymentAmount","schema:rangeIncludes":{"@id":"unece:AmountType"},"schema:domainIncludes":[{"@id":"unece:LineTradeSettlement"},{"@id":"unece:HeaderTradeSettlement"},{"@id":"unece:PaymentTradeSettlement"}],"rdfs:comment":""},{"@id":"unece:paymentReference","@type":["rdf:Property","owl:DatatypeProperty"],"rdfs:label":"paymentReference","schema:rangeIncludes":{"@id":"schema:Text"},"schema:domainIncludes":[{"@id":"unece:LineTradeSettlement"},{"@id":"unece:HeaderTradeSettlement"}],"rdfs:comment":"A payment reference, expressed as text, for this header trade settlement."},{"@id":"unece:priceCurrencyCode","@type":["rdf:Property","owl:DatatypeProperty"],"rdfs:label":"priceCurrencyCode","schema:rangeIncludes":{"@id":"schema:Text"},"schema:domainIncludes":[{"@id":"unece:LineTradeSettlement"},{"@id":"unece:HeaderTradeSettlement"}],"rdfs:comment":"The code specifying the price currency for this header trade settlement."},{"@id":"unece:purchaseSpecifiedAccountingAccount","@type":["rdf:Property","owl:ObjectProperty"],"rdfs:label":"purchaseSpecifiedAccountingAccount","schema:rangeIncludes":{"@id":"unece:AccountingAccount"},"schema:domainIncludes":[{"@id":"unece:LineTradeSettlement"},{"@id":"unece:HeaderTradeSettlement"}],"rdfs:comment":"A specific trade account for recording debits and credits to general accounting, cost accounting or budget accounting."},{"@id":"unece:receivableSpecifiedAccountingAccount","@type":["rdf:Property","owl:ObjectProperty"],"rdfs:label":"receivableSpecifiedAccountingAccount","schema:rangeIncludes":{"@id":"unece:AccountingAccount"},"schema:domainIncludes":[{"@id":"unece:LineTradeSettlement"},{"@id":"unece:HeaderTradeSettlement"}],"rdfs:comment":"A specific trade account for recording debits and credits to general accounting, cost accounting or budget accounting."},{"@id":"unece:salesSpecifiedAccountingAccount","@type":["rdf:Property","owl:ObjectProperty"],"rdfs:label":"salesSpecifiedAccountingAccount","schema:rangeIncludes":{"@id":"unece:AccountingAccount"},"schema:domainIncludes":[{"@id":"unece:LineTradeSettlement"},{"@id":"unece:HeaderTradeSettlement"}],"rdfs:comment":"A specific trade account for recording debits and credits to general accounting, cost accounting or budget accounting."},{"@id":"unece:specifiedAllowanceCharge","@type":["rdf:Property","owl:ObjectProperty"],"rdfs:label":"specifiedAllowanceCharge","schema:rangeIncludes":{"@id":"unece:TradeAllowanceCharge"},"schema:domainIncludes":[{"@id":"unece:LineTradeSettlement"},{"@id":"unece:SubordinateLineTradeSettlement"},{"@id":"unece:HeaderTradeSettlement"}],"rdfs:comment":"A component of pricing, such as an allowance or charge for trade purposes."},{"@id":"unece:specifiedFinancialAdjustment","@type":["rdf:Property","owl:ObjectProperty"],"rdfs:label":"specifiedFinancialAdjustment","schema:rangeIncludes":{"@id":"unece:FinancialAdjustment"},"schema:domainIncludes":[{"@id":"unece:LineTradeSettlement"},{"@id":"unece:SubordinateLineTradeSettlement"},{"@id":"unece:HeaderTradeSettlement"}],"rdfs:comment":"A correction or modification to reflect actual financial conditions."},{"@id":"unece:specifiedFinancialCard","@type":["rdf:Property","owl:ObjectProperty"],"rdfs:label":"specifiedFinancialCard","schema:rangeIncludes":{"@id":"unece:FinancialCard"},"schema:domainIncludes":[{"@id":"unece:LineTradeSettlement"},{"@id":"unece:HeaderTradeSettlement"}],"rdfs:comment":"A card used to represent a financial account for a trade settlement."},{"@id":"unece:specifiedPaymentTerms","@type":["rdf:Property","owl:ObjectProperty"],"rdfs:label":"specifiedPaymentTerms","schema:rangeIncludes":{"@id":"unece:PaymentTerms"},"schema:domainIncludes":[{"@id":"unece:LineTradeSettlement"},{"@id":"unece:HeaderTradeSettlement"}],"rdfs:comment":"Terms and conditions by which payment has been or will be made for trade purposes."},{"@id":"unece:specifiedServiceCharge","@type":["rdf:Property","owl:ObjectProperty"],"rdfs:label":"specifiedServiceCharge","schema:rangeIncludes":{"@id":"unece:ServiceCharge"},"schema:domainIncludes":[{"@id":"unece:LineTradeSettlement"},{"@id":"unece:HeaderTradeSettlement"}],"rdfs:comment":"A charge made for a logistics related service."},{"@id":"unece:specifiedTradeSettlementLineMonetarySummation","@type":["rdf:Property","owl:ObjectProperty"],"rdfs:label":"specifiedTradeSettlementLineMonetarySummation","schema:rangeIncludes":{"@id":"unece:TradeSettlementLineMonetarySummation"},"schema:domainIncludes":{"@id":"unece:LineTradeSettlement"},"rdfs:comment":"The monetary summation totals specified for this line trade settlement."},{"@id":"unece:subtotalCalculatedTax","@type":["rdf:Property","owl:ObjectProperty"],"rdfs:label":"subtotalCalculatedTax","schema:rangeIncludes":{"@id":"unece:TradeTax"},"schema:domainIncludes":[{"@id":"unece:LineTradeSettlement"},{"@id":"unece:HeaderTradeSettlement"}],"rdfs:comment":"A tax subtotal calculated for this header trade settlement."},{"@id":"unece:totalAdjustmentAmount","@type":["rdf:Property","owl:ObjectProperty"],"rdfs:label":"totalAdjustmentAmount","schema:rangeIncludes":{"@id":"unece:AmountType"},"schema:domainIncludes":[{"@id":"unece:LineTradeSettlement"},{"@id":"unece:HeaderTradeSettlement"}],"rdfs:comment":""},{"@id":"unece:tradeTransaction","@type":["rdf:Property","owl:ObjectProperty"],"rdfs:label":"tradeTransaction","schema:rangeIncludes":{"@id":"unece:LineTradeTransaction"},"schema:domainIncludes":{"@id":"unece:LineTradeSettlement"},"rdfs:comment":"A trade transaction referenced in this line trade settlement."},{"@id":"unece:allocatedMachine","@type":["rdf:Property","owl:ObjectProperty"],"rdfs:label":"allocatedMachine","schema:rangeIncludes":{"@id":"unece:Machine"},"schema:domainIncludes":{"@id":"unece:ProductionProcess"},"rdfs:comment":"A machine allocated to this production process."},{"@id":"unece:allocatedProductionDevice","@type":["rdf:Property","owl:ObjectProperty"],"rdfs:label":"allocatedProductionDevice","schema:rangeIncludes":{"@id":"unece:ProductionDevice"},"schema:domainIncludes":{"@id":"unece:ProductionProcess"},"rdfs:comment":"A production device allocated to this production process."},{"@id":"unece:applicableParameter","@type":["rdf:Property","owl:ObjectProperty"],"rdfs:label":"applicableParameter","schema:rangeIncludes":{"@id":"unece:SpecifiedParameter"},"schema:domainIncludes":[{"@id":"unece:ProductionProcess"},{"@id":"unece:ProductionDevice"},{"@id":"unece:SpecifiedMethod"}],"rdfs:comment":"A specified feature that is fixed for the case in question but may be different in other cases."},{"@id":"unece:applicableProductionCycle","@type":["rdf:Property","owl:ObjectProperty"],"rdfs:label":"applicableProductionCycle","schema:rangeIncludes":{"@id":"unece:ProductionCycle"},"schema:domainIncludes":{"@id":"unece:ProductionProcess"},"rdfs:comment":"A specified production cycle applicable to this production process."},{"@id":"unece:appliedCropProtectionTreatment","@type":["rdf:Property","owl:ObjectProperty"],"rdfs:label":"appliedCropProtectionTreatment","schema:rangeIncludes":{"@id":"unece:CropProtectionTreatment"},"schema:domainIncludes":{"@id":"unece:ProductionProcess"},"rdfs:comment":"A method or substance, such as chemical fertilizers and crop protection products, applied to plant growth whilst managing and controlling diseases and pests."},{"@id":"unece:associatedStandard","@type":["rdf:Property","owl:ObjectProperty"],"rdfs:label":"associatedStandard","schema:rangeIncludes":{"@id":"unece:Standard"},"schema:domainIncludes":[{"@id":"unece:ProductionProcess"},{"@id":"unece:SupplyChainTradeTransaction"},{"@id":"unece:Licence"},{"@id":"unece:SpecifiedDeclaration"}],"rdfs:comment":"A referenced norm or requirement that establishes uniform criteria, methods, processes and practices, such as in engineering or technical areas."},{"@id":"unece:criticalIndicator","@type":["rdf:Property","owl:DatatypeProperty"],"rdfs:label":"criticalIndicator","schema:rangeIncludes":{"@id":"schema:Boolean"},"schema:domainIncludes":{"@id":"unece:ProductionProcess"},"rdfs:comment":"The indication of whether or not this production process is critical."},{"@id":"unece:disclosureLevelCode","@type":["rdf:Property","owl:DatatypeProperty"],"rdfs:label":"disclosureLevelCode","schema:rangeIncludes":{"@id":"schema:Text"},"schema:domainIncludes":[{"@id":"unece:ProductionProcess"},{"@id":"unece:TradeParty"}],"rdfs:comment":"A code specifying a disclosure level for this production process."},{"@id":"unece:finalIndicator","@type":["rdf:Property","owl:DatatypeProperty"],"rdfs:label":"finalIndicator","schema:rangeIncludes":{"@id":"schema:Boolean"},"schema:domainIncludes":{"@id":"unece:ProductionProcess"},"rdfs:comment":"The indication of whether or not this production process is a final one."},{"@id":"unece:inputApplicableBatch","@type":["rdf:Property","owl:ObjectProperty"],"rdfs:label":"inputApplicableBatch","schema:rangeIncludes":{"@id":"unece:ProductBatch"},"schema:domainIncludes":[{"@id":"unece:ProductionProcess"},{"@id":"unece:ProductionUnit"},{"@id":"unece:ProductionDevice"},{"@id":"unece:Machine"}],"rdfs:comment":"An input batch applicable to this production machine."},{"@id":"unece:inputApplicableMaterial","@type":["rdf:Property","owl:ObjectProperty"],"rdfs:label":"inputApplicableMaterial","schema:rangeIncludes":{"@id":"unece:SpecifiedMaterial"},"schema:domainIncludes":[{"@id":"unece:ProductionProcess"},{"@id":"unece:ProductionUnit"},{"@id":"unece:ProductionDevice"},{"@id":"unece:Machine"}],"rdfs:comment":"A substance from which something is or could be made."},{"@id":"unece:inputApplicableProduct","@type":["rdf:Property","owl:ObjectProperty"],"rdfs:label":"inputApplicableProduct","schema:rangeIncludes":{"@id":"unece:TradeProduct"},"schema:domainIncludes":[{"@id":"unece:ProductionProcess"},{"@id":"unece:ProductionUnit"},{"@id":"unece:ProductionDevice"},{"@id":"unece:Machine"}],"rdfs:comment":"An input product applicable to this facility production unit."},{"@id":"unece:inventoryTypeCode","@type":["rdf:Property","owl:DatatypeProperty"],"rdfs:label":"inventoryTypeCode","schema:rangeIncludes":{"@id":"schema:Text"},"schema:domainIncludes":{"@id":"unece:ProductionProcess"},"rdfs:comment":"The code specifying the inventory type for this production process."},{"@id":"unece:occurrenceEvent","@type":["rdf:Property","owl:ObjectProperty"],"rdfs:label":"occurrenceEvent","schema:rangeIncludes":{"@id":"unece:SupplyChainEvent"},"schema:domainIncludes":{"@id":"unece:ProductionProcess"},"rdfs:comment":"A significant occurrence or happening in a supply chain."},{"@id":"unece:operationReferenceCode","@type":["rdf:Property","owl:DatatypeProperty"],"rdfs:label":"operationReferenceCode","schema:rangeIncludes":{"@id":"schema:Text"},"schema:domainIncludes":{"@id":"unece:ProductionProcess"},"rdfs:comment":"The code specifying the operation reference for this production process."},{"@id":"unece:operationTechnologyCode","@type":["rdf:Property","owl:DatatypeProperty"],"rdfs:label":"operationTechnologyCode","schema:rangeIncludes":{"@id":"schema:Text"},"schema:domainIncludes":{"@id":"unece:ProductionProcess"},"rdfs:comment":"The code specifying the operation technology for this production process."},{"@id":"unece:outputApplicableBatch","@type":["rdf:Property","owl:ObjectProperty"],"rdfs:label":"outputApplicableBatch","schema:rangeIncludes":{"@id":"unece:ProductBatch"},"schema:domainIncludes":[{"@id":"unece:ProductionProcess"},{"@id":"unece:ProductionUnit"},{"@id":"unece:ProductionDevice"},{"@id":"unece:Machine"}],"rdfs:comment":"An output batch applicable to this specified production device."},{"@id":"unece:outputApplicableMaterial","@type":["rdf:Property","owl:ObjectProperty"],"rdfs:label":"outputApplicableMaterial","schema:rangeIncludes":{"@id":"unece:SpecifiedMaterial"},"schema:domainIncludes":[{"@id":"unece:ProductionProcess"},{"@id":"unece:ProductionUnit"},{"@id":"unece:ProductionDevice"},{"@id":"unece:Machine"}],"rdfs:comment":"A substance from which something is or could be made."},{"@id":"unece:outputApplicableProduct","@type":["rdf:Property","owl:ObjectProperty"],"rdfs:label":"outputApplicableProduct","schema:rangeIncludes":{"@id":"unece:TradeProduct"},"schema:domainIncludes":[{"@id":"unece:ProductionProcess"},{"@id":"unece:ProductionUnit"},{"@id":"unece:ProductionDevice"},{"@id":"unece:Machine"}],"rdfs:comment":"An output product applicable to this facility production unit."},{"@id":"unece:performedWorkItem","@type":["rdf:Property","owl:ObjectProperty"],"rdfs:label":"performedWorkItem","schema:rangeIncludes":{"@id":"unece:ProcessWorkItem"},"schema:domainIncludes":{"@id":"unece:ProductionProcess"},"rdfs:comment":"A distinct operation or task that is part of a process."},{"@id":"unece:productionWasteInstructions","@type":["rdf:Property","owl:ObjectProperty"],"rdfs:label":"productionWasteInstructions","schema:rangeIncludes":{"@id":"unece:DisposalInstructions"},"schema:domainIncludes":[{"@id":"unece:ProductionProcess"},{"@id":"unece:AgriculturalProcess"}],"rdfs:comment":"A set of instructions detailing how to properly dispose of a material."},{"@id":"unece:recyclingIndicator","@type":["rdf:Property","owl:DatatypeProperty"],"rdfs:label":"recyclingIndicator","schema:rangeIncludes":{"@id":"schema:Boolean"},"schema:domainIncludes":{"@id":"unece:ProductionProcess"},"rdfs:comment":"The indication of whether or not this is a recycling production process."},{"@id":"unece:relatedBinaryFile","@type":["rdf:Property","owl:ObjectProperty"],"rdfs:label":"relatedBinaryFile","schema:rangeIncludes":{"@id":"unece:BinaryFile"},"schema:domainIncludes":[{"@id":"unece:ProductionProcess"},{"@id":"unece:ProductionCycle"},{"@id":"unece:Observation"}],"rdfs:comment":"A specified computer file or program stored in a binary format."},{"@id":"unece:reportedProductionWasteMaterial","@type":["rdf:Property","owl:ObjectProperty"],"rdfs:label":"reportedProductionWasteMaterial","schema:rangeIncludes":{"@id":"unece:ProductionWasteMaterial"},"schema:domainIncludes":[{"@id":"unece:ProductionProcess"},{"@id":"unece:AgriculturalProcess"}],"rdfs:comment":"Any materials unused and rejected as unwanted during a production process."},{"@id":"unece:specificationDocument","@type":["rdf:Property","owl:ObjectProperty"],"rdfs:label":"specificationDocument","schema:rangeIncludes":{"@id":"unece:Document"},"schema:domainIncludes":{"@id":"unece:ProductionProcess"},"rdfs:comment":"Written, printed or electronic matter that is referenced."},{"@id":"unece:specifiedDocument","@type":["rdf:Property","owl:ObjectProperty"],"rdfs:label":"specifiedDocument","schema:rangeIncludes":{"@id":"unece:Document"},"schema:domainIncludes":[{"@id":"unece:ProductionProcess"},{"@id":"unece:ProductBatch"},{"@id":"unece:Colour"},{"@id":"unece:Print"},{"@id":"unece:ProductGroup"},{"@id":"unece:Standard"},{"@id":"unece:SustainabilityInspection"},{"@id":"unece:SpecifiedInspection"}],"rdfs:comment":"Written, printed or electronic matter that is referenced."},{"@id":"unece:specifiedOrganizationalCertificate","@type":["rdf:Property","owl:ObjectProperty"],"rdfs:label":"specifiedOrganizationalCertificate","schema:rangeIncludes":{"@id":"unece:OrganizationalCertificate"},"schema:domainIncludes":[{"@id":"unece:ProductionProcess"},{"@id":"unece:ProductionFacility"},{"@id":"unece:ProductionUnit"},{"@id":"unece:TransportMovement"}],"rdfs:comment":"A piece of written, printed or electronic matter that provides information or evidence that an organization has met required organizational criteria."},{"@id":"unece:specifiedOrganizationalCertification","@type":["rdf:Property","owl:ObjectProperty"],"rdfs:label":"specifiedOrganizationalCertification","schema:rangeIncludes":{"@id":"unece:OrganizationalCertification"},"schema:domainIncludes":[{"@id":"unece:ProductionProcess"},{"@id":"unece:ProductionFacility"}],"rdfs:comment":"The process of certifying organizational performance or qualification requirements as stipulated in regulations."},{"@id":"unece:specifiedProcessCertificate","@type":["rdf:Property","owl:ObjectProperty"],"rdfs:label":"specifiedProcessCertificate","schema:rangeIncludes":{"@id":"unece:ProcessCertificate"},"schema:domainIncludes":[{"@id":"unece:ProductionProcess"},{"@id":"unece:ProductionFacility"},{"@id":"unece:ProductionUnit"},{"@id":"unece:SpecifiedChemicalTreatment"},{"@id":"unece:ProductionWasteRecoveryDisposalProcess"},{"@id":"unece:TransportMovement"},{"@id":"unece:TransportationWasteRecoveryDisposalProcess"}],"rdfs:comment":"A piece of written, printed or electronic matter that provides information or evidence that a process has met required criteria."},{"@id":"unece:specifiedProcessCertification","@type":["rdf:Property","owl:ObjectProperty"],"rdfs:label":"specifiedProcessCertification","schema:rangeIncludes":{"@id":"unece:ProcessCertification"},"schema:domainIncludes":[{"@id":"unece:ProductionProcess"},{"@id":"unece:ProductionFacility"}],"rdfs:comment":"The process of certifying that a process has met performance and quality assurance tests, or qualification requirements."},{"@id":"unece:specifiedProductBatchCertification","@type":["rdf:Property","owl:ObjectProperty"],"rdfs:label":"specifiedProductBatchCertification","schema:rangeIncludes":{"@id":"unece:ProductBatchCertification"},"schema:domainIncludes":[{"@id":"unece:ProductionProcess"},{"@id":"unece:ProductionFacility"}],"rdfs:comment":"The process of certifying that a certain product batch has passed performance and quality assurance tests, or qualification requirements stipulated in regulations."},{"@id":"unece:specifiedTradeProductCertification","@type":["rdf:Property","owl:ObjectProperty"],"rdfs:label":"specifiedTradeProductCertification","schema:rangeIncludes":{"@id":"unece:TradeProductCertification"},"schema:domainIncludes":[{"@id":"unece:ProductionProcess"},{"@id":"unece:ProductionFacility"}],"rdfs:comment":"The process of certifying that a certain product has passed performance and quality assurance tests, or qualification requirements stipulated in regulations."},{"@id":"unece:stepCode","@type":["rdf:Property","owl:DatatypeProperty"],"rdfs:label":"stepCode","schema:rangeIncludes":{"@id":"schema:Text"},"schema:domainIncludes":{"@id":"unece:ProductionProcess"},"rdfs:comment":"The code specifying the step in this production process."},{"@id":"unece:subordinateProcess","@type":["rdf:Property","owl:ObjectProperty"],"rdfs:label":"subordinateProcess","schema:rangeIncludes":{"@id":"unece:ProductionProcess"},"schema:domainIncludes":{"@id":"unece:ProductionProcess"},"rdfs:comment":"A subordinate process of this production process."},{"@id":"unece:additionalStreetName","@type":["rdf:Property","owl:DatatypeProperty"],"rdfs:label":"additionalStreetName","schema:rangeIncludes":{"@id":"schema:Text"},"schema:domainIncludes":[{"@id":"unece:TradeAddress"},{"@id":"unece:Address"}],"rdfs:comment":"The additional name of a street, expressed as text, for this trade address."},{"@id":"unece:addressTypeCode","@type":["rdf:Property","owl:DatatypeProperty"],"rdfs:label":"addressTypeCode","schema:rangeIncludes":{"@id":"unece:AddressTypeCodeList"},"schema:domainIncludes":[{"@id":"unece:TradeAddress"},{"@id":"unece:Address"}],"rdfs:comment":"A code specifying the type of this trade address, such as business address or home address."},{"@id":"unece:attentionOf","@type":["rdf:Property","owl:DatatypeProperty"],"rdfs:label":"attentionOf","schema:rangeIncludes":{"@id":"schema:Text"},"schema:domainIncludes":[{"@id":"unece:TradeAddress"},{"@id":"unece:Address"}],"rdfs:comment":"The name, expressed as text, of a person or department in the organization to whom incoming mail is marked with words such as 'for the attention of' or 'FAO' or 'ATTN' for this trade address."},{"@id":"unece:buildingName","@type":["rdf:Property","owl:DatatypeProperty"],"rdfs:label":"buildingName","schema:rangeIncludes":{"@id":"schema:Text"},"schema:domainIncludes":[{"@id":"unece:TradeAddress"},{"@id":"unece:Address"}],"rdfs:comment":"The name, expressed as text, of a building, a house or other structure on a street at this trade address."},{"@id":"unece:buildingNumber","@type":["rdf:Property","owl:DatatypeProperty"],"rdfs:label":"buildingNumber","schema:rangeIncludes":{"@id":"schema:Text"},"schema:domainIncludes":[{"@id":"unece:TradeAddress"},{"@id":"unece:Address"},{"@id":"unece:FinancialInstitutionAddress"}],"rdfs:comment":"The building number, expressed as text, in this trade address."},{"@id":"unece:careOf","@type":["rdf:Property","owl:DatatypeProperty"],"rdfs:label":"careOf","schema:rangeIncludes":{"@id":"schema:Text"},"schema:domainIncludes":[{"@id":"unece:TradeAddress"},{"@id":"unece:Address"}],"rdfs:comment":"The name, expressed as text, of a person or organization at this trade address to whom incoming mail is marked with words such as 'care of' or 'C/O'."},{"@id":"unece:cityId","@type":["rdf:Property","owl:DatatypeProperty"],"rdfs:label":"cityId","schema:rangeIncludes":{"@id":"schema:Text"},"schema:domainIncludes":[{"@id":"unece:TradeAddress"},{"@id":"unece:Address"},{"@id":"unece:FinancialInstitutionAddress"}],"rdfs:comment":"The identifier of the city for this trade address, such as United Nations Location Code (UNLOCODE)."},{"@id":"unece:cityName","@type":["rdf:Property","owl:DatatypeProperty"],"rdfs:label":"cityName","schema:rangeIncludes":{"@id":"schema:Text"},"schema:domainIncludes":[{"@id":"unece:TradeAddress"},{"@id":"unece:BirthAddress"},{"@id":"unece:Address"},{"@id":"unece:FinancialInstitutionAddress"}],"rdfs:comment":"The name, expressed as text, of the city, town or village of this birth address."},{"@id":"unece:citySubDivisionName","@type":["rdf:Property","owl:DatatypeProperty"],"rdfs:label":"citySubDivisionName","schema:rangeIncludes":{"@id":"schema:Text"},"schema:domainIncludes":[{"@id":"unece:TradeAddress"},{"@id":"unece:Address"}],"rdfs:comment":"A name, expressed as text, of a sub-division of a city for this trade address, for example a district or borough."},{"@id":"unece:countryName","@type":["rdf:Property","owl:DatatypeProperty"],"rdfs:label":"countryName","schema:rangeIncludes":{"@id":"schema:Text"},"schema:domainIncludes":[{"@id":"unece:TradeAddress"},{"@id":"unece:TradeLocation"},{"@id":"unece:Location"},{"@id":"unece:Address"},{"@id":"unece:FinancialInstitutionAddress"},{"@id":"unece:LogisticsLocation"}],"rdfs:comment":"A name, expressed as text, of the country for this trade address."},{"@id":"unece:countrySubDivisionId","@type":["rdf:Property","owl:DatatypeProperty"],"rdfs:label":"countrySubDivisionId","schema:rangeIncludes":{"@id":"schema:Text"},"schema:domainIncludes":[{"@id":"unece:TradeAddress"},{"@id":"unece:Location"},{"@id":"unece:Address"},{"@id":"unece:FinancialInstitutionAddress"},{"@id":"unece:GovernmentRegistration"},{"@id":"unece:LogisticsLocation"}],"rdfs:comment":"A unique identifier of the country sub-division for this trade address."},{"@id":"unece:countrySubDivisionName","@type":["rdf:Property","owl:DatatypeProperty"],"rdfs:label":"countrySubDivisionName","schema:rangeIncludes":{"@id":"schema:Text"},"schema:domainIncludes":[{"@id":"unece:TradeAddress"},{"@id":"unece:BirthAddress"},{"@id":"unece:Address"},{"@id":"unece:FinancialInstitutionAddress"}],"rdfs:comment":"A name, expressed as text, of the sub-division of a country for this trade address."},{"@id":"unece:freeForm","@type":["rdf:Property","owl:DatatypeProperty"],"rdfs:label":"freeForm","schema:rangeIncludes":{"@id":"schema:Text"},"schema:domainIncludes":[{"@id":"unece:TradeAddress"},{"@id":"unece:Address"}],"rdfs:comment":"A free form representation, expressed as text, of this trade address."},{"@id":"unece:geoCoordinateIdentificationGeographicalCoordinate","@type":["rdf:Property","owl:ObjectProperty"],"rdfs:label":"geoCoordinateIdentificationGeographicalCoordinate","schema:rangeIncludes":{"@id":"unece:GeographicalCoordinate"},"schema:domainIncludes":[{"@id":"unece:TradeAddress"},{"@id":"unece:Address"}],"rdfs:comment":"A set of geographical coordinates of a specific point such as the longitude, latitude and altitude."},{"@id":"unece:invalidIndicator","@type":["rdf:Property","owl:DatatypeProperty"],"rdfs:label":"invalidIndicator","schema:rangeIncludes":{"@id":"schema:Boolean"},"schema:domainIncludes":[{"@id":"unece:TradeAddress"},{"@id":"unece:Communication"},{"@id":"unece:Address"}],"rdfs:comment":"The indication of whether or not this trade address is invalid."},{"@id":"unece:lineFive","@type":["rdf:Property","owl:DatatypeProperty"],"rdfs:label":"lineFive","schema:rangeIncludes":{"@id":"schema:Text"},"schema:domainIncludes":[{"@id":"unece:TradeAddress"},{"@id":"unece:Address"},{"@id":"unece:FinancialInstitutionAddress"}],"rdfs:comment":"The fifth free form line, expressed as text, of this financial institution address."},{"@id":"unece:lineFour","@type":["rdf:Property","owl:DatatypeProperty"],"rdfs:label":"lineFour","schema:rangeIncludes":{"@id":"schema:Text"},"schema:domainIncludes":[{"@id":"unece:TradeAddress"},{"@id":"unece:Address"},{"@id":"unece:FinancialInstitutionAddress"}],"rdfs:comment":"The fourth free form line, expressed as text, of this financial institution address."},{"@id":"unece:lineOne","@type":["rdf:Property","owl:DatatypeProperty"],"rdfs:label":"lineOne","schema:rangeIncludes":{"@id":"schema:Text"},"schema:domainIncludes":[{"@id":"unece:TradeAddress"},{"@id":"unece:Address"},{"@id":"unece:FinancialInstitutionAddress"}],"rdfs:comment":"The first free form line, expressed as text, of this financial institution address."},{"@id":"unece:lineThree","@type":["rdf:Property","owl:DatatypeProperty"],"rdfs:label":"lineThree","schema:rangeIncludes":{"@id":"schema:Text"},"schema:domainIncludes":[{"@id":"unece:TradeAddress"},{"@id":"unece:Address"},{"@id":"unece:FinancialInstitutionAddress"}],"rdfs:comment":"The third free form line, expressed as text, of this financial institution address."},{"@id":"unece:lineTwo","@type":["rdf:Property","owl:DatatypeProperty"],"rdfs:label":"lineTwo","schema:rangeIncludes":{"@id":"schema:Text"},"schema:domainIncludes":[{"@id":"unece:TradeAddress"},{"@id":"unece:Address"},{"@id":"unece:FinancialInstitutionAddress"}],"rdfs:comment":"The second free form line, expressed as text, of this financial institution address."},{"@id":"unece:postOfficeBox","@type":["rdf:Property","owl:DatatypeProperty"],"rdfs:label":"postOfficeBox","schema:rangeIncludes":{"@id":"schema:Text"},"schema:domainIncludes":[{"@id":"unece:TradeAddress"},{"@id":"unece:Address"},{"@id":"unece:FinancialInstitutionAddress"}],"rdfs:comment":"The post office box, expressed as text, for this financial institution address."},{"@id":"unece:postcodeCode","@type":["rdf:Property","owl:DatatypeProperty"],"rdfs:label":"postcodeCode","schema:rangeIncludes":{"@id":"schema:Text"},"schema:domainIncludes":[{"@id":"unece:TradeAddress"},{"@id":"unece:Address"},{"@id":"unece:FinancialInstitutionAddress"}],"rdfs:comment":"A code specifying the postcode of this trade address."},{"@id":"unece:streetName","@type":["rdf:Property","owl:DatatypeProperty"],"rdfs:label":"streetName","schema:rangeIncludes":{"@id":"schema:Text"},"schema:domainIncludes":[{"@id":"unece:TradeAddress"},{"@id":"unece:Address"},{"@id":"unece:FinancialInstitutionAddress"}],"rdfs:comment":"A name, expressed as text, of a street or thoroughfare for this trade address."},{"@id":"unece:tradeAddressCountryId","@type":["rdf:Property","owl:DatatypeProperty"],"rdfs:label":"tradeAddressCountryId","schema:rangeIncludes":{"@id":"unece:CountryId"},"schema:domainIncludes":{"@id":"unece:TradeAddress"},"rdfs:comment":"The unique identifier of a country for this trade address."},{"@id":"unece:adjustedBalanceOutAmount","@type":["rdf:Property","owl:ObjectProperty"],"rdfs:label":"adjustedBalanceOutAmount","schema:rangeIncludes":{"@id":"unece:AmountType"},"schema:domainIncludes":[{"@id":"unece:TradeSettlementHeaderMonetarySummation"},{"@id":"unece:TradeSettlementPaymentMonetarySummation"}],"rdfs:comment":""},{"@id":"unece:allowanceTotalAmount","@type":["rdf:Property","owl:ObjectProperty"],"rdfs:label":"allowanceTotalAmount","schema:rangeIncludes":{"@id":"unece:AmountType"},"schema:domainIncludes":[{"@id":"unece:TradeSettlementHeaderMonetarySummation"},{"@id":"unece:TradeSettlementLineMonetarySummation"}],"rdfs:comment":""},{"@id":"unece:applicableHeaderBalanceOut","@type":["rdf:Property","owl:ObjectProperty"],"rdfs:label":"applicableHeaderBalanceOut","schema:rangeIncludes":{"@id":"unece:HeaderBalanceOut"},"schema:domainIncludes":{"@id":"unece:TradeSettlementHeaderMonetarySummation"},"rdfs:comment":"Offset header information to ensure that debits and credits are equal for a transaction."},{"@id":"unece:balanceOutAmount","@type":["rdf:Property","owl:ObjectProperty"],"rdfs:label":"balanceOutAmount","schema:rangeIncludes":{"@id":"unece:AmountType"},"schema:domainIncludes":[{"@id":"unece:TradeSettlementHeaderMonetarySummation"},{"@id":"unece:TradeSettlementPaymentMonetarySummation"}],"rdfs:comment":""},{"@id":"unece:chargeTotalAmount","@type":["rdf:Property","owl:ObjectProperty"],"rdfs:label":"chargeTotalAmount","schema:rangeIncludes":{"@id":"unece:AmountType"},"schema:domainIncludes":[{"@id":"unece:TradeSettlementHeaderMonetarySummation"},{"@id":"unece:TradeSettlementLineMonetarySummation"}],"rdfs:comment":""},{"@id":"unece:duePayableAmount","@type":["rdf:Property","owl:ObjectProperty"],"rdfs:label":"duePayableAmount","schema:rangeIncludes":{"@id":"unece:AmountType"},"schema:domainIncludes":[{"@id":"unece:TradeSettlementHeaderMonetarySummation"},{"@id":"unece:TradeSettlementLineMonetarySummation"},{"@id":"unece:HeaderTradeSettlement"}],"rdfs:comment":""},{"@id":"unece:excludingTaxesLineTotalAmount","@type":["rdf:Property","owl:ObjectProperty"],"rdfs:label":"excludingTaxesLineTotalAmount","schema:rangeIncludes":{"@id":"unece:AmountType"},"schema:domainIncludes":{"@id":"unece:TradeSettlementHeaderMonetarySummation"},"rdfs:comment":""},{"@id":"unece:grandTotalAmount","@type":["rdf:Property","owl:ObjectProperty"],"rdfs:label":"grandTotalAmount","schema:rangeIncludes":{"@id":"unece:AmountType"},"schema:domainIncludes":[{"@id":"unece:TradeSettlementHeaderMonetarySummation"},{"@id":"unece:TradeTax"},{"@id":"unece:TradeSettlementLineMonetarySummation"},{"@id":"unece:Tax"},{"@id":"unece:TradeSettlementPaymentMonetarySummation"}],"rdfs:comment":""},{"@id":"unece:grandTotalSpecifiedAdjustment","@type":["rdf:Property","owl:ObjectProperty"],"rdfs:label":"grandTotalSpecifiedAdjustment","schema:rangeIncludes":{"@id":"unece:FinancialAdjustment"},"schema:domainIncludes":{"@id":"unece:TradeSettlementHeaderMonetarySummation"},"rdfs:comment":"A correction or modification to reflect actual financial conditions."},{"@id":"unece:grossLineTotalAmount","@type":["rdf:Property","owl:ObjectProperty"],"rdfs:label":"grossLineTotalAmount","schema:rangeIncludes":{"@id":"unece:AmountType"},"schema:domainIncludes":[{"@id":"unece:TradeSettlementHeaderMonetarySummation"},{"@id":"unece:TradeSettlementLineMonetarySummation"}],"rdfs:comment":""},{"@id":"unece:includingTaxesLineTotalAmount","@type":["rdf:Property","owl:ObjectProperty"],"rdfs:label":"includingTaxesLineTotalAmount","schema:rangeIncludes":{"@id":"unece:AmountType"},"schema:domainIncludes":[{"@id":"unece:TradeSettlementHeaderMonetarySummation"},{"@id":"unece:TradeSettlementLineMonetarySummation"},{"@id":"unece:TradeSettlementPaymentMonetarySummation"}],"rdfs:comment":""},{"@id":"unece:informationAmount","@type":["rdf:Property","owl:ObjectProperty"],"rdfs:label":"informationAmount","schema:rangeIncludes":{"@id":"unece:AmountType"},"schema:domainIncludes":[{"@id":"unece:TradeSettlementHeaderMonetarySummation"},{"@id":"unece:TradeTax"},{"@id":"unece:TradeSettlementLineMonetarySummation"},{"@id":"unece:Tax"}],"rdfs:comment":""},{"@id":"unece:insuranceChargeTotalAmount","@type":["rdf:Property","owl:ObjectProperty"],"rdfs:label":"insuranceChargeTotalAmount","schema:rangeIncludes":{"@id":"unece:AmountType"},"schema:domainIncludes":{"@id":"unece:TradeSettlementHeaderMonetarySummation"},"rdfs:comment":""},{"@id":"unece:lineTotalAmount","@type":["rdf:Property","owl:ObjectProperty"],"rdfs:label":"lineTotalAmount","schema:rangeIncludes":{"@id":"unece:AmountType"},"schema:domainIncludes":[{"@id":"unece:TradeSettlementHeaderMonetarySummation"},{"@id":"unece:TradeSettlementLineMonetarySummation"}],"rdfs:comment":""},{"@id":"unece:netIncludingTaxesLineTotalAmount","@type":["rdf:Property","owl:ObjectProperty"],"rdfs:label":"netIncludingTaxesLineTotalAmount","schema:rangeIncludes":{"@id":"unece:AmountType"},"schema:domainIncludes":[{"@id":"unece:TradeSettlementHeaderMonetarySummation"},{"@id":"unece:TradeSettlementLineMonetarySummation"}],"rdfs:comment":""},{"@id":"unece:netLineTotalAmount","@type":["rdf:Property","owl:ObjectProperty"],"rdfs:label":"netLineTotalAmount","schema:rangeIncludes":{"@id":"unece:AmountType"},"schema:domainIncludes":[{"@id":"unece:TradeSettlementHeaderMonetarySummation"},{"@id":"unece:TradeSettlementLineMonetarySummation"},{"@id":"unece:TradeSettlementPaymentMonetarySummation"}],"rdfs:comment":""},{"@id":"unece:paymentTotalAmount","@type":["rdf:Property","owl:ObjectProperty"],"rdfs:label":"paymentTotalAmount","schema:rangeIncludes":{"@id":"unece:AmountType"},"schema:domainIncludes":[{"@id":"unece:TradeSettlementHeaderMonetarySummation"},{"@id":"unece:TradeSettlementLineMonetarySummation"},{"@id":"unece:TradeSettlementPaymentMonetarySummation"}],"rdfs:comment":""},{"@id":"unece:productValueExcludingTobaccoTaxInformationAmount","@type":["rdf:Property","owl:ObjectProperty"],"rdfs:label":"productValueExcludingTobaccoTaxInformationAmount","schema:rangeIncludes":{"@id":"unece:AmountType"},"schema:domainIncludes":{"@id":"unece:TradeSettlementHeaderMonetarySummation"},"rdfs:comment":""},{"@id":"unece:retailValueExcludingTaxInformationAmount","@type":["rdf:Property","owl:ObjectProperty"],"rdfs:label":"retailValueExcludingTaxInformationAmount","schema:rangeIncludes":{"@id":"unece:AmountType"},"schema:domainIncludes":{"@id":"unece:TradeSettlementHeaderMonetarySummation"},"rdfs:comment":""},{"@id":"unece:roundingAmount","@type":["rdf:Property","owl:ObjectProperty"],"rdfs:label":"roundingAmount","schema:rangeIncludes":{"@id":"unece:AmountType"},"schema:domainIncludes":{"@id":"unece:TradeSettlementHeaderMonetarySummation"},"rdfs:comment":""},{"@id":"unece:taxBasisTotalAmount","@type":["rdf:Property","owl:ObjectProperty"],"rdfs:label":"taxBasisTotalAmount","schema:rangeIncludes":{"@id":"unece:AmountType"},"schema:domainIncludes":[{"@id":"unece:TradeSettlementHeaderMonetarySummation"},{"@id":"unece:TradeSettlementLineMonetarySummation"}],"rdfs:comment":""},{"@id":"unece:taxTotalAmount","@type":["rdf:Property","owl:ObjectProperty"],"rdfs:label":"taxTotalAmount","schema:rangeIncludes":{"@id":"unece:AmountType"},"schema:domainIncludes":[{"@id":"unece:TradeSettlementHeaderMonetarySummation"},{"@id":"unece:TradeSettlementLineMonetarySummation"},{"@id":"unece:TradeSettlementPaymentMonetarySummation"}],"rdfs:comment":""},{"@id":"unece:totalAllowanceChargeAmount","@type":["rdf:Property","owl:ObjectProperty"],"rdfs:label":"totalAllowanceChargeAmount","schema:rangeIncludes":{"@id":"unece:AmountType"},"schema:domainIncludes":[{"@id":"unece:TradeSettlementHeaderMonetarySummation"},{"@id":"unece:TradeSettlementLineMonetarySummation"},{"@id":"unece:Consignment"}],"rdfs:comment":""},{"@id":"unece:totalDepositFeeInformationAmount","@type":["rdf:Property","owl:ObjectProperty"],"rdfs:label":"totalDepositFeeInformationAmount","schema:rangeIncludes":{"@id":"unece:AmountType"},"schema:domainIncludes":{"@id":"unece:TradeSettlementHeaderMonetarySummation"},"rdfs:comment":""},{"@id":"unece:totalDiscountAmount","@type":["rdf:Property","owl:ObjectProperty"],"rdfs:label":"totalDiscountAmount","schema:rangeIncludes":{"@id":"unece:AmountType"},"schema:domainIncludes":{"@id":"unece:TradeSettlementHeaderMonetarySummation"},"rdfs:comment":""},{"@id":"unece:totalDiscountBasisAmount","@type":["rdf:Property","owl:ObjectProperty"],"rdfs:label":"totalDiscountBasisAmount","schema:rangeIncludes":{"@id":"unece:AmountType"},"schema:domainIncludes":{"@id":"unece:TradeSettlementHeaderMonetarySummation"},"rdfs:comment":""},{"@id":"unece:totalPrepaidAmount","@type":["rdf:Property","owl:ObjectProperty"],"rdfs:label":"totalPrepaidAmount","schema:rangeIncludes":{"@id":"unece:AmountType"},"schema:domainIncludes":{"@id":"unece:TradeSettlementHeaderMonetarySummation"},"rdfs:comment":""},{"@id":"unece:totalRetailValueInformationAmount","@type":["rdf:Property","owl:ObjectProperty"],"rdfs:label":"totalRetailValueInformationAmount","schema:rangeIncludes":{"@id":"unece:AmountType"},"schema:domainIncludes":[{"@id":"unece:TradeSettlementHeaderMonetarySummation"},{"@id":"unece:TradeSettlementLineMonetarySummation"}],"rdfs:comment":""},{"@id":"unece:agreedContract","@type":["rdf:Property","owl:ObjectProperty"],"rdfs:label":"agreedContract","schema:rangeIncludes":{"@id":"unece:Contract"},"schema:domainIncludes":{"@id":"unece:TradeParty"},"rdfs:comment":"A trade contract agreed with this trade party."},{"@id":"unece:allianceName","@type":["rdf:Property","owl:DatatypeProperty"],"rdfs:label":"allianceName","schema:rangeIncludes":{"@id":"schema:Text"},"schema:domainIncludes":{"@id":"unece:TradeParty"},"rdfs:comment":"An alliance name, expressed as text, for this trade party."},{"@id":"unece:applicableOrganizationalCertificate","@type":["rdf:Property","owl:ObjectProperty"],"rdfs:label":"applicableOrganizationalCertificate","schema:rangeIncludes":{"@id":"unece:OrganizationalCertificate"},"schema:domainIncludes":{"@id":"unece:TradeParty"},"rdfs:comment":"A piece of written, printed or electronic matter that provides information or evidence that an organization has met required organizational criteria."},{"@id":"unece:applicableOrganizationalCertification","@type":["rdf:Property","owl:ObjectProperty"],"rdfs:label":"applicableOrganizationalCertification","schema:rangeIncludes":{"@id":"unece:OrganizationalCertification"},"schema:domainIncludes":[{"@id":"unece:TradeParty"},{"@id":"unece:OrganizationalCertificate"}],"rdfs:comment":"The process of certifying organizational performance or qualification requirements as stipulated in regulations."},{"@id":"unece:applicableProcessCertificate","@type":["rdf:Property","owl:ObjectProperty"],"rdfs:label":"applicableProcessCertificate","schema:rangeIncludes":{"@id":"unece:ProcessCertificate"},"schema:domainIncludes":[{"@id":"unece:TradeParty"},{"@id":"unece:ProductFinishingTreatment"},{"@id":"unece:WasteMaterialRecoveryDisposalProcess"},{"@id":"unece:CropProtectionTreatment"}],"rdfs:comment":"A piece of written, printed or electronic matter that provides information or evidence that a process has met required criteria."},{"@id":"unece:applicableProductBatchCertificate","@type":["rdf:Property","owl:ObjectProperty"],"rdfs:label":"applicableProductBatchCertificate","schema:rangeIncludes":{"@id":"unece:ProductBatchCertificate"},"schema:domainIncludes":{"@id":"unece:TradeParty"},"rdfs:comment":"A piece of written, printed or electronic matter that provides information or evidence that a product batch has met required criteria."},{"@id":"unece:applicableProductCertificate","@type":["rdf:Property","owl:ObjectProperty"],"rdfs:label":"applicableProductCertificate","schema:rangeIncludes":{"@id":"unece:ProductCertificate"},"schema:domainIncludes":[{"@id":"unece:TradeParty"},{"@id":"unece:HazardousMaterial"},{"@id":"unece:SpecifiedMaterial"},{"@id":"unece:ProductionWasteMaterial"},{"@id":"unece:ProductionWasteMaterialComponent"},{"@id":"unece:TransportationWasteMaterial"},{"@id":"unece:TransportationWasteMaterialComponent"}],"rdfs:comment":"A collection of data for a piece of written, printed or electronic matter that provides information or evidence about the product."},{"@id":"unece:applicableServiceCharge","@type":["rdf:Property","owl:ObjectProperty"],"rdfs:label":"applicableServiceCharge","schema:rangeIncludes":{"@id":"unece:ServiceCharge"},"schema:domainIncludes":[{"@id":"unece:TradeParty"},{"@id":"unece:LogisticsTransportEquipment"},{"@id":"unece:TransportMovement"},{"@id":"unece:LogisticsTransportMeans"},{"@id":"unece:Consignment"},{"@id":"unece:ConsignmentItem"}],"rdfs:comment":"A charge made for a logistics related service."},{"@id":"unece:associatedMembership","@type":["rdf:Property","owl:ObjectProperty"],"rdfs:label":"associatedMembership","schema:rangeIncludes":{"@id":"unece:Membership"},"schema:domainIncludes":{"@id":"unece:TradeParty"},"rdfs:comment":"The state of belonging to a group, such as a club or trade association."},{"@id":"unece:associatedParty","@type":["rdf:Property","owl:ObjectProperty"],"rdfs:label":"associatedParty","schema:rangeIncludes":{"@id":"unece:TradeParty"},"schema:domainIncludes":[{"@id":"unece:TradeParty"},{"@id":"unece:Consignment"}],"rdfs:comment":"A party associated with this trade party, such as a local agent of a shipping line."},{"@id":"unece:availableExperienceItem","@type":["rdf:Property","owl:ObjectProperty"],"rdfs:label":"availableExperienceItem","schema:rangeIncludes":{"@id":"unece:ExperienceItem"},"schema:domainIncludes":{"@id":"unece:TradeParty"},"rdfs:comment":"A collection of information specific to the involvement of a person or persons in a happening, such as a theme park, a guided tour being used or reported on for trade purposes."},{"@id":"unece:availableFacility","@type":["rdf:Property","owl:ObjectProperty"],"rdfs:label":"availableFacility","schema:rangeIncludes":{"@id":"unece:ExperienceFacility"},"schema:domainIncludes":{"@id":"unece:TradeParty"},"rdfs:comment":"A structure or place, such as a restaurant, hotel, theme park, hot spring bathing pool, parking lot, or meeting room, that provides a particular experience."},{"@id":"unece:businessTypeCode","@type":["rdf:Property","owl:DatatypeProperty"],"rdfs:label":"businessTypeCode","schema:rangeIncludes":{"@id":"schema:Text"},"schema:domainIncludes":[{"@id":"unece:TradeParty"},{"@id":"unece:LegalOrganization"}],"rdfs:comment":"A code specifying the type of business of this legally set up organization."},{"@id":"unece:chainName","@type":["rdf:Property","owl:DatatypeProperty"],"rdfs:label":"chainName","schema:rangeIncludes":{"@id":"schema:Text"},"schema:domainIncludes":{"@id":"unece:TradeParty"},"rdfs:comment":"A chain name, expressed as text, for this trade party."},{"@id":"unece:claimedLanguageProficiency","@type":["rdf:Property","owl:ObjectProperty"],"rdfs:label":"claimedLanguageProficiency","schema:rangeIncludes":{"@id":"unece:LanguageProficiency"},"schema:domainIncludes":[{"@id":"unece:TradeParty"},{"@id":"unece:GuestPerson"},{"@id":"unece:Stowaway"}],"rdfs:comment":"Skills in any principal method of human communication, consisting of words used in a structured and conventional way and conveyed by speech, writing, or gesture."},{"@id":"unece:commentedReviewNote","@type":["rdf:Property","owl:ObjectProperty"],"rdfs:label":"commentedReviewNote","schema:rangeIncludes":{"@id":"unece:SpecifiedNote"},"schema:domainIncludes":{"@id":"unece:TradeParty"},"rdfs:comment":"A specified textual or coded description, such as a remark or additional information."},{"@id":"unece:cooperativeInformationSource","@type":["rdf:Property","owl:ObjectProperty"],"rdfs:label":"cooperativeInformationSource","schema:rangeIncludes":{"@id":"unece:InformationSource"},"schema:domainIncludes":{"@id":"unece:TradeParty"},"rdfs:comment":"A person, organization, thing or place from which information comes, arises or is obtained."},{"@id":"unece:dUNSId","@type":["rdf:Property","owl:DatatypeProperty"],"rdfs:label":"dUNSId","schema:rangeIncludes":{"@id":"schema:Text"},"schema:domainIncludes":{"@id":"unece:TradeParty"},"rdfs:comment":"The unique nine-digit Data Universal Numbering System (DUNS) identifier for this trade party."},{"@id":"unece:definedContact","@type":["rdf:Property","owl:ObjectProperty"],"rdfs:label":"definedContact","schema:rangeIncludes":{"@id":"unece:TradeContact"},"schema:domainIncludes":[{"@id":"unece:TradeParty"},{"@id":"unece:LocationParty"}],"rdfs:comment":"A trade contact defined for this location party."},{"@id":"unece:endPointURICommunication","@type":["rdf:Property","owl:ObjectProperty"],"rdfs:label":"endPointURICommunication","schema:rangeIncludes":{"@id":"unece:Communication"},"schema:domainIncludes":{"@id":"unece:TradeParty"},"rdfs:comment":"The exchange of thoughts, messages, or information, as universally exchanged by speech, signals, writing, or behaviour between persons and/or organizations."},{"@id":"unece:gLNId","@type":["rdf:Property","owl:DatatypeProperty"],"rdfs:label":"gLNId","schema:rangeIncludes":{"@id":"schema:Text"},"schema:domainIncludes":[{"@id":"unece:TradeParty"},{"@id":"unece:PaymentFinancialInstitution"}],"rdfs:comment":"A Global Location Number (GLN) identifier for this trade party."},{"@id":"unece:logoAssociatedBinaryFile","@type":["rdf:Property","owl:ObjectProperty"],"rdfs:label":"logoAssociatedBinaryFile","schema:rangeIncludes":{"@id":"unece:BinaryFile"},"schema:domainIncludes":{"@id":"unece:TradeParty"},"rdfs:comment":"A specified computer file or program stored in a binary format."},{"@id":"unece:ownedFinancialAccount","@type":["rdf:Property","owl:ObjectProperty"],"rdfs:label":"ownedFinancialAccount","schema:rangeIncludes":{"@id":"unece:CreditorFinancialAccount"},"schema:domainIncludes":{"@id":"unece:TradeParty"},"rdfs:comment":"A specific business arrangement whereby credits arising from transactions are recorded."},{"@id":"unece:partyRoleCode","@type":["rdf:Property","owl:DatatypeProperty"],"rdfs:label":"partyRoleCode","schema:rangeIncludes":{"@id":"unece:PartyRoleCodeList"},"schema:domainIncludes":[{"@id":"unece:TradeParty"},{"@id":"unece:TransportPerson"}],"rdfs:comment":"A code specifying a role of this transport person."},{"@id":"unece:partyTypeCode","@type":["rdf:Property","owl:DatatypeProperty"],"rdfs:label":"partyTypeCode","schema:rangeIncludes":{"@id":"unece:PartyTypeCodeList"},"schema:domainIncludes":[{"@id":"unece:TradeParty"},{"@id":"unece:TTParty"},{"@id":"unece:RequestingParty"}],"rdfs:comment":"A code specifying the type of TT party."},{"@id":"unece:providedProcess","@type":["rdf:Property","owl:ObjectProperty"],"rdfs:label":"providedProcess","schema:rangeIncludes":{"@id":"unece:ProductionProcess"},"schema:domainIncludes":{"@id":"unece:TradeParty"},"rdfs:comment":"A production process provided by this trade party."},{"@id":"unece:providedService","@type":["rdf:Property","owl:ObjectProperty"],"rdfs:label":"providedService","schema:rangeIncludes":{"@id":"unece:Service"},"schema:domainIncludes":[{"@id":"unece:TradeParty"},{"@id":"unece:LocationParty"}],"rdfs:comment":"A service associated with a transport movement.,A referenced service associated with a specified event during transport movement."},{"@id":"unece:qualityAssuranceIndicator","@type":["rdf:Property","owl:DatatypeProperty"],"rdfs:label":"qualityAssuranceIndicator","schema:rangeIncludes":{"@id":"schema:Boolean"},"schema:domainIncludes":{"@id":"unece:TradeParty"},"rdfs:comment":"The indication of whether or not this trade party is quality assured."},{"@id":"unece:registeredId","@type":["rdf:Property","owl:DatatypeProperty"],"rdfs:label":"registeredId","schema:rangeIncludes":{"@id":"schema:Text"},"schema:domainIncludes":{"@id":"unece:TradeParty"},"rdfs:comment":"A registered identifier of this trade party."},{"@id":"unece:relatedBatch","@type":["rdf:Property","owl:ObjectProperty"],"rdfs:label":"relatedBatch","schema:rangeIncludes":{"@id":"unece:ProductBatch"},"schema:domainIncludes":{"@id":"unece:TradeParty"},"rdfs:comment":"A product batch related to this trade party."},{"@id":"unece:relatedMaterial","@type":["rdf:Property","owl:ObjectProperty"],"rdfs:label":"relatedMaterial","schema:rangeIncludes":{"@id":"unece:SpecifiedMaterial"},"schema:domainIncludes":{"@id":"unece:TradeParty"},"rdfs:comment":"A substance from which something is or could be made."},{"@id":"unece:requestedExperienceItem","@type":["rdf:Property","owl:ObjectProperty"],"rdfs:label":"requestedExperienceItem","schema:rangeIncludes":{"@id":"unece:ExperienceItem"},"schema:domainIncludes":{"@id":"unece:TradeParty"},"rdfs:comment":"A collection of information specific to the involvement of a person or persons in a happening, such as a theme park, a guided tour being used or reported on for trade purposes."},{"@id":"unece:reservedExperienceItem","@type":["rdf:Property","owl:ObjectProperty"],"rdfs:label":"reservedExperienceItem","schema:rangeIncludes":{"@id":"unece:ExperienceItem"},"schema:domainIncludes":{"@id":"unece:TradeParty"},"rdfs:comment":"A collection of information specific to the involvement of a person or persons in a happening, such as a theme park, a guided tour being used or reported on for trade purposes."},{"@id":"unece:role","@type":["rdf:Property","owl:DatatypeProperty"],"rdfs:label":"role","schema:rangeIncludes":{"@id":"schema:Text"},"schema:domainIncludes":[{"@id":"unece:TradeParty"},{"@id":"unece:Contact"},{"@id":"unece:TransportPerson"}],"rdfs:comment":"A role, expressed as text, for this contact person."},{"@id":"unece:salesManagerName","@type":["rdf:Property","owl:DatatypeProperty"],"rdfs:label":"salesManagerName","schema:rangeIncludes":{"@id":"schema:Text"},"schema:domainIncludes":{"@id":"unece:TradeParty"},"rdfs:comment":"A name of a sales manager, expressed as text, for this trade party."},{"@id":"unece:searchedWishListExperienceItem","@type":["rdf:Property","owl:ObjectProperty"],"rdfs:label":"searchedWishListExperienceItem","schema:rangeIncludes":{"@id":"unece:ExperienceItem"},"schema:domainIncludes":{"@id":"unece:TradeParty"},"rdfs:comment":"A collection of information specific to the involvement of a person or persons in a happening, such as a theme park, a guided tour being used or reported on for trade purposes."},{"@id":"unece:specifiedAuthoritativeSignatoryPerson","@type":["rdf:Property","owl:ObjectProperty"],"rdfs:label":"specifiedAuthoritativeSignatoryPerson","schema:rangeIncludes":{"@id":"unece:AuthoritativeSignatoryPerson"},"schema:domainIncludes":{"@id":"unece:TradeParty"},"rdfs:comment":"A person who is authorized to sign a document, such as a customs officer or other government official."},{"@id":"unece:specifiedCooperatingOrganization","@type":["rdf:Property","owl:ObjectProperty"],"rdfs:label":"specifiedCooperatingOrganization","schema:rangeIncludes":{"@id":"unece:CooperatingOrganization"},"schema:domainIncludes":{"@id":"unece:TradeParty"},"rdfs:comment":"An organized structure set up for a particular purpose, such as a business, government body, department, charity, or financial institution that is working together with another organization, business, or person."},{"@id":"unece:specifiedCreditorFinancialInstitution","@type":["rdf:Property","owl:ObjectProperty"],"rdfs:label":"specifiedCreditorFinancialInstitution","schema:rangeIncludes":{"@id":"unece:CreditorFinancialInstitution"},"schema:domainIncludes":{"@id":"unece:TradeParty"},"rdfs:comment":"A bank, building society, credit union, stock brokerage, or similar business of the party that receives money."},{"@id":"unece:specifiedFinancialIdentity","@type":["rdf:Property","owl:ObjectProperty"],"rdfs:label":"specifiedFinancialIdentity","schema:rangeIncludes":{"@id":"unece:FinancialIdentity"},"schema:domainIncludes":{"@id":"unece:TradeParty"},"rdfs:comment":"A financial identification for an organization."},{"@id":"unece:specifiedGovernmentRegistration","@type":["rdf:Property","owl:ObjectProperty"],"rdfs:label":"specifiedGovernmentRegistration","schema:rangeIncludes":{"@id":"unece:GovernmentRegistration"},"schema:domainIncludes":{"@id":"unece:TradeParty"},"rdfs:comment":"The recording of items or details for a governmental purpose."},{"@id":"unece:specifiedGuestPerson","@type":["rdf:Property","owl:ObjectProperty"],"rdfs:label":"specifiedGuestPerson","schema:rangeIncludes":{"@id":"unece:GuestPerson"},"schema:domainIncludes":{"@id":"unece:TradeParty"},"rdfs:comment":"An individual guest."},{"@id":"unece:specifiedLegalOrganization","@type":["rdf:Property","owl:ObjectProperty"],"rdfs:label":"specifiedLegalOrganization","schema:rangeIncludes":{"@id":"unece:LegalOrganization"},"schema:domainIncludes":{"@id":"unece:TradeParty"},"rdfs:comment":"An organization set up on a legal basis as a business, government body, department, charity, or financial institution."},{"@id":"unece:specifiedProprietaryIdentity","@type":["rdf:Property","owl:ObjectProperty"],"rdfs:label":"specifiedProprietaryIdentity","schema:rangeIncludes":{"@id":"unece:ProprietaryIdentity"},"schema:domainIncludes":[{"@id":"unece:TradeParty"},{"@id":"unece:PersonIdentity"},{"@id":"unece:CreditorFinancialInstitution"},{"@id":"unece:RequestingParty"}],"rdfs:comment":"Proprietary information which uniquely identifies a person or organization."},{"@id":"unece:specifiedRiskAnalysisResult","@type":["rdf:Property","owl:ObjectProperty"],"rdfs:label":"specifiedRiskAnalysisResult","schema:rangeIncludes":{"@id":"unece:RiskAnalysisResult"},"schema:domainIncludes":[{"@id":"unece:TradeParty"},{"@id":"unece:LogisticsTransportEquipment"},{"@id":"unece:TransportMovement"},{"@id":"unece:Consignment"},{"@id":"unece:ConsignmentItem"}],"rdfs:comment":"The result of a logistics risk analysis calculation."},{"@id":"unece:specifiedTaxRegistration","@type":["rdf:Property","owl:ObjectProperty"],"rdfs:label":"specifiedTaxRegistration","schema:rangeIncludes":{"@id":"unece:TaxRegistration"},"schema:domainIncludes":{"@id":"unece:TradeParty"},"rdfs:comment":"Registration with a specific tax authority."},{"@id":"unece:tradePartyLanguageCode","@type":["rdf:Property","owl:DatatypeProperty"],"rdfs:label":"tradePartyLanguageCode","schema:rangeIncludes":{"@id":"unece:LanguageCodeList"},"schema:domainIncludes":{"@id":"unece:TradeParty"},"rdfs:comment":"A code specifying a language for this trade party."},{"@id":"unece:uRICommunication","@type":["rdf:Property","owl:ObjectProperty"],"rdfs:label":"uRICommunication","schema:rangeIncludes":{"@id":"unece:Communication"},"schema:domainIncludes":[{"@id":"unece:TradeParty"},{"@id":"unece:Service"},{"@id":"unece:LocationParty"}],"rdfs:comment":"The exchange of thoughts, messages, or information, as universally exchanged by speech, signals, writing, or behaviour between persons and/or organizations."},{"@id":"unece:allowanceChargeBasisAmount","@type":["rdf:Property","owl:ObjectProperty"],"rdfs:label":"allowanceChargeBasisAmount","schema:rangeIncludes":{"@id":"unece:AmountType"},"schema:domainIncludes":[{"@id":"unece:TradeTax"},{"@id":"unece:Tax"}],"rdfs:comment":""},{"@id":"unece:applicablePercent","@type":["rdf:Property","owl:DatatypeProperty"],"rdfs:label":"applicablePercent","schema:rangeIncludes":{"@id":"schema:Text"},"schema:domainIncludes":[{"@id":"unece:TradeTax"},{"@id":"unece:Tax"}],"rdfs:comment":"The percent of trade tax applicable, such as to an object or an activity."},{"@id":"unece:basisAmount","@type":["rdf:Property","owl:ObjectProperty"],"rdfs:label":"basisAmount","schema:rangeIncludes":{"@id":"unece:AmountType"},"schema:domainIncludes":[{"@id":"unece:TradeTax"},{"@id":"unece:AppliedAllowanceCharge"},{"@id":"unece:PaymentDiscountTerms"},{"@id":"unece:PaymentPenaltyTerms"},{"@id":"unece:AppliedTax"},{"@id":"unece:Tax"},{"@id":"unece:TradeAllowanceCharge"}],"rdfs:comment":""},{"@id":"unece:basisQuantity","@type":["rdf:Property","owl:ObjectProperty"],"rdfs:label":"basisQuantity","schema:rangeIncludes":{"@id":"unece:QuantityType"},"schema:domainIncludes":[{"@id":"unece:TradeTax"},{"@id":"unece:Tax"},{"@id":"unece:TradeAllowanceCharge"},{"@id":"unece:TradePrice"},{"@id":"unece:ReferencePrice"}],"rdfs:comment":""},{"@id":"unece:buyerDeductibleTaxSpecifiedAccountingAccount","@type":["rdf:Property","owl:ObjectProperty"],"rdfs:label":"buyerDeductibleTaxSpecifiedAccountingAccount","schema:rangeIncludes":{"@id":"unece:AccountingAccount"},"schema:domainIncludes":[{"@id":"unece:TradeTax"},{"@id":"unece:Tax"}],"rdfs:comment":"A specific trade account for recording debits and credits to general accounting, cost accounting or budget accounting."},{"@id":"unece:buyerNonDeductibleTaxSpecifiedAccountingAccount","@type":["rdf:Property","owl:ObjectProperty"],"rdfs:label":"buyerNonDeductibleTaxSpecifiedAccountingAccount","schema:rangeIncludes":{"@id":"unece:AccountingAccount"},"schema:domainIncludes":[{"@id":"unece:TradeTax"},{"@id":"unece:Tax"}],"rdfs:comment":"A specific trade account for recording debits and credits to general accounting, cost accounting or budget accounting."},{"@id":"unece:buyerRepayableTaxSpecifiedAccountingAccount","@type":["rdf:Property","owl:ObjectProperty"],"rdfs:label":"buyerRepayableTaxSpecifiedAccountingAccount","schema:rangeIncludes":{"@id":"unece:AccountingAccount"},"schema:domainIncludes":[{"@id":"unece:TradeTax"},{"@id":"unece:Tax"}],"rdfs:comment":"A specific trade account for recording debits and credits to general accounting, cost accounting or budget accounting."},{"@id":"unece:calculatedAmount","@type":["rdf:Property","owl:ObjectProperty"],"rdfs:label":"calculatedAmount","schema:rangeIncludes":{"@id":"unece:AmountType"},"schema:domainIncludes":[{"@id":"unece:TradeTax"},{"@id":"unece:AppliedTax"},{"@id":"unece:HeaderBalanceOut"},{"@id":"unece:PaymentBalanceOut"},{"@id":"unece:Tax"}],"rdfs:comment":""},{"@id":"unece:calculatedRate","@type":["rdf:Property","owl:DatatypeProperty"],"rdfs:label":"calculatedRate","schema:rangeIncludes":{"@id":"schema:Text"},"schema:domainIncludes":[{"@id":"unece:TradeTax"},{"@id":"unece:AppliedTax"},{"@id":"unece:Tax"}],"rdfs:comment":"The rate used to calculate the amount of this trade related tax, levy or duty."},{"@id":"unece:calculationMethodCode","@type":["rdf:Property","owl:DatatypeProperty"],"rdfs:label":"calculationMethodCode","schema:rangeIncludes":{"@id":"schema:Text"},"schema:domainIncludes":[{"@id":"unece:TradeTax"},{"@id":"unece:Tax"}],"rdfs:comment":"The code specifying the method by which this trade related tax, levy or duty is calculated, such as codes for \"tax calculated after line total summation\", \"tax calculated before line total summation\", \"tax back calculated based on grand total\"."},{"@id":"unece:calculationSequenceNumeric","@type":["rdf:Property","owl:DatatypeProperty"],"rdfs:label":"calculationSequenceNumeric","schema:rangeIncludes":{"@id":"schema:Text"},"schema:domainIncludes":[{"@id":"unece:TradeTax"},{"@id":"unece:Tax"}],"rdfs:comment":"A numeric expression of the sequence in which this trade related tax is to be or has been applied when multiple taxes are applicable per calculation, such as first \"Value Added Tax (VAT)\", second \"Transfer\"."},{"@id":"unece:categoryName","@type":["rdf:Property","owl:DatatypeProperty"],"rdfs:label":"categoryName","schema:rangeIncludes":{"@id":"schema:Text"},"schema:domainIncludes":[{"@id":"unece:TradeTax"},{"@id":"unece:CustomerClass"},{"@id":"unece:Tax"}],"rdfs:comment":"A category name, expressed as text, of this specified customer class."},{"@id":"unece:customsDutyIndicator","@type":["rdf:Property","owl:DatatypeProperty"],"rdfs:label":"customsDutyIndicator","schema:rangeIncludes":{"@id":"schema:Boolean"},"schema:domainIncludes":[{"@id":"unece:TradeTax"},{"@id":"unece:RegisteredTax"},{"@id":"unece:Tax"}],"rdfs:comment":"The indication of whether or not this registered tax is a customs duty."},{"@id":"unece:customsDutyRegimeTypeCode","@type":["rdf:Property","owl:DatatypeProperty"],"rdfs:label":"customsDutyRegimeTypeCode","schema:rangeIncludes":{"@id":"unece:CustomsDutyRegimeTypeCodeList"},"schema:domainIncludes":[{"@id":"unece:TradeTax"},{"@id":"unece:Tax"}],"rdfs:comment":"The code specifying a type of regime applicable to the assessment or calculation of this trade related tax, levy or duty, such as a preferential duty rate."},{"@id":"unece:customsProcedureGuaranteeCode","@type":["rdf:Property","owl:DatatypeProperty"],"rdfs:label":"customsProcedureGuaranteeCode","schema:rangeIncludes":{"@id":"unece:CustomsProcedureGuaranteeCodeList"},"schema:domainIncludes":[{"@id":"unece:TradeTax"},{"@id":"unece:Tax"},{"@id":"unece:RegulatoryProcedure"}],"rdfs:comment":"The code specifying an undertaking given in cash, bond or as a written guarantee to ensure that an obligation will be fulfilled for this cross-border regulatory procedure."},{"@id":"unece:deductionAmount","@type":["rdf:Property","owl:ObjectProperty"],"rdfs:label":"deductionAmount","schema:rangeIncludes":{"@id":"unece:AmountType"},"schema:domainIncludes":[{"@id":"unece:TradeTax"},{"@id":"unece:Tax"}],"rdfs:comment":""},{"@id":"unece:exemptionAuthorizationId","@type":["rdf:Property","owl:DatatypeProperty"],"rdfs:label":"exemptionAuthorizationId","schema:rangeIncludes":{"@id":"schema:Text"},"schema:domainIncludes":[{"@id":"unece:TradeTax"},{"@id":"unece:Tax"}],"rdfs:comment":"The unique identifier of the exemption authorization for this trade tax."},{"@id":"unece:exemptionIndicator","@type":["rdf:Property","owl:DatatypeProperty"],"rdfs:label":"exemptionIndicator","schema:rangeIncludes":{"@id":"schema:Boolean"},"schema:domainIncludes":[{"@id":"unece:TradeTax"},{"@id":"unece:Tax"}],"rdfs:comment":"The indication of whether or not there is an exemption from this trade tax."},{"@id":"unece:exemptionReason","@type":["rdf:Property","owl:DatatypeProperty"],"rdfs:label":"exemptionReason","schema:rangeIncludes":{"@id":"schema:Text"},"schema:domainIncludes":[{"@id":"unece:TradeTax"},{"@id":"unece:RegisteredTax"},{"@id":"unece:Tax"}],"rdfs:comment":"A reason, expressed as text, for exemption from this registered tax."},{"@id":"unece:guarantee","@type":["rdf:Property","owl:DatatypeProperty"],"rdfs:label":"guarantee","schema:rangeIncludes":{"@id":"schema:Text"},"schema:domainIncludes":[{"@id":"unece:TradeTax"},{"@id":"unece:Tax"},{"@id":"unece:RegulatoryProcedure"}],"rdfs:comment":"The undertaking, expressed as text, given in cash, bond or as a written guarantee to ensure that an obligation will be fulfilled for this cross-border regulatory procedure."},{"@id":"unece:jurisdiction","@type":["rdf:Property","owl:DatatypeProperty"],"rdfs:label":"jurisdiction","schema:rangeIncludes":{"@id":"schema:Text"},"schema:domainIncludes":[{"@id":"unece:TradeTax"},{"@id":"unece:RegisteredTax"},{"@id":"unece:Tax"}],"rdfs:comment":"A jurisdiction, expressed as text, for this registered tax."},{"@id":"unece:lineTotalBasisAmount","@type":["rdf:Property","owl:ObjectProperty"],"rdfs:label":"lineTotalBasisAmount","schema:rangeIncludes":{"@id":"unece:AmountType"},"schema:domainIncludes":[{"@id":"unece:TradeTax"},{"@id":"unece:Tax"}],"rdfs:comment":""},{"@id":"unece:localTaxSystemId","@type":["rdf:Property","owl:DatatypeProperty"],"rdfs:label":"localTaxSystemId","schema:rangeIncludes":{"@id":"schema:Text"},"schema:domainIncludes":[{"@id":"unece:TradeTax"},{"@id":"unece:Tax"}],"rdfs:comment":"The identifier of the local tax system for this trade tax."},{"@id":"unece:paymentId","@type":["rdf:Property","owl:DatatypeProperty"],"rdfs:label":"paymentId","schema:rangeIncludes":{"@id":"schema:Text"},"schema:domainIncludes":[{"@id":"unece:TradeTax"},{"@id":"unece:Tax"}],"rdfs:comment":"The unique identifier of the payment of this trade related tax, levy or duty."},{"@id":"unece:placeApplicableLocation","@type":["rdf:Property","owl:ObjectProperty"],"rdfs:label":"placeApplicableLocation","schema:rangeIncludes":{"@id":"unece:TradeLocation"},"schema:domainIncludes":[{"@id":"unece:TradeTax"},{"@id":"unece:Tax"}],"rdfs:comment":"A location where this trade tax is applicable."},{"@id":"unece:rateApplicablePercent","@type":["rdf:Property","owl:DatatypeProperty"],"rdfs:label":"rateApplicablePercent","schema:rangeIncludes":{"@id":"schema:Text"},"schema:domainIncludes":[{"@id":"unece:TradeTax"},{"@id":"unece:Tax"}],"rdfs:comment":"The applicable rate, expressed as a percentage, for this trade tax, levy or duty."},{"@id":"unece:rateCode","@type":["rdf:Property","owl:DatatypeProperty"],"rdfs:label":"rateCode","schema:rangeIncludes":{"@id":"schema:Text"},"schema:domainIncludes":[{"@id":"unece:TradeTax"},{"@id":"unece:Tax"}],"rdfs:comment":"The code specifying the rate for this trade related tax, levy or duty."},{"@id":"unece:refundAmount","@type":["rdf:Property","owl:ObjectProperty"],"rdfs:label":"refundAmount","schema:rangeIncludes":{"@id":"unece:AmountType"},"schema:domainIncludes":[{"@id":"unece:TradeTax"},{"@id":"unece:PaymentTradeSettlement"},{"@id":"unece:Tax"}],"rdfs:comment":""},{"@id":"unece:selfAssessedBasisAmount","@type":["rdf:Property","owl:ObjectProperty"],"rdfs:label":"selfAssessedBasisAmount","schema:rangeIncludes":{"@id":"unece:AmountType"},"schema:domainIncludes":[{"@id":"unece:TradeTax"},{"@id":"unece:Tax"}],"rdfs:comment":""},{"@id":"unece:selfAssessedBasisQuantity","@type":["rdf:Property","owl:ObjectProperty"],"rdfs:label":"selfAssessedBasisQuantity","schema:rangeIncludes":{"@id":"unece:QuantityType"},"schema:domainIncludes":[{"@id":"unece:TradeTax"},{"@id":"unece:Tax"}],"rdfs:comment":""},{"@id":"unece:selfAssessedCalculatedAmount","@type":["rdf:Property","owl:ObjectProperty"],"rdfs:label":"selfAssessedCalculatedAmount","schema:rangeIncludes":{"@id":"unece:AmountType"},"schema:domainIncludes":[{"@id":"unece:TradeTax"},{"@id":"unece:Tax"}],"rdfs:comment":""},{"@id":"unece:sellerPayableTaxSpecifiedAccountingAccount","@type":["rdf:Property","owl:ObjectProperty"],"rdfs:label":"sellerPayableTaxSpecifiedAccountingAccount","schema:rangeIncludes":{"@id":"unece:AccountingAccount"},"schema:domainIncludes":[{"@id":"unece:TradeTax"},{"@id":"unece:Tax"}],"rdfs:comment":"A specific trade account for recording debits and credits to general accounting, cost accounting or budget accounting."},{"@id":"unece:sellerRefundableTaxSpecifiedAccountingAccount","@type":["rdf:Property","owl:ObjectProperty"],"rdfs:label":"sellerRefundableTaxSpecifiedAccountingAccount","schema:rangeIncludes":{"@id":"unece:AccountingAccount"},"schema:domainIncludes":[{"@id":"unece:TradeTax"},{"@id":"unece:Tax"}],"rdfs:comment":"A specific trade account for recording debits and credits to general accounting, cost accounting or budget accounting."},{"@id":"unece:serviceSupplyCountry","@type":["rdf:Property","owl:ObjectProperty"],"rdfs:label":"serviceSupplyCountry","schema:rangeIncludes":{"@id":"unece:Country"},"schema:domainIncludes":[{"@id":"unece:TradeTax"},{"@id":"unece:Tax"}],"rdfs:comment":"The area of land that belongs to a nation together with its properties, such as population, political organization, etc., used or referenced for trade purposes."},{"@id":"unece:specifiedAccountingAccount","@type":["rdf:Property","owl:ObjectProperty"],"rdfs:label":"specifiedAccountingAccount","schema:rangeIncludes":{"@id":"unece:AccountingAccount"},"schema:domainIncludes":[{"@id":"unece:TradeTax"},{"@id":"unece:Tax"}],"rdfs:comment":"A specific trade account for recording debits and credits to general accounting, cost accounting or budget accounting."},{"@id":"unece:tariffDeductionQuantity","@type":["rdf:Property","owl:ObjectProperty"],"rdfs:label":"tariffDeductionQuantity","schema:rangeIncludes":{"@id":"unece:QuantityType"},"schema:domainIncludes":[{"@id":"unece:TradeTax"},{"@id":"unece:Tax"},{"@id":"unece:RegulatoryProcedure"}],"rdfs:comment":""},{"@id":"unece:taxBasisAllowanceRate","@type":["rdf:Property","owl:DatatypeProperty"],"rdfs:label":"taxBasisAllowanceRate","schema:rangeIncludes":{"@id":"schema:Text"},"schema:domainIncludes":[{"@id":"unece:TradeTax"},{"@id":"unece:Tax"}],"rdfs:comment":"The rate of the tax basis allowance (deduction or discount) used to calculate the trade related tax, levy or duty."},{"@id":"unece:taxCategoryCode","@type":["rdf:Property","owl:DatatypeProperty"],"rdfs:label":"taxCategoryCode","schema:rangeIncludes":{"@id":"unece:TaxCategoryCodeList"},"schema:domainIncludes":[{"@id":"unece:TradeTax"},{"@id":"unece:Tax"}],"rdfs:comment":"The code specifying the category to which this trade related tax, levy or duty applies, such as codes for \"Exempt from Tax\", \"Standard Rate\", \"Free Export Item - Tax Not Charged\" [Reference United Nations Code List (UNCL) 5305]."},{"@id":"unece:taxExemptionAuthorityId","@type":["rdf:Property","owl:DatatypeProperty"],"rdfs:label":"taxExemptionAuthorityId","schema:rangeIncludes":{"@id":"schema:Text"},"schema:domainIncludes":[{"@id":"unece:TradeTax"},{"@id":"unece:Tax"}],"rdfs:comment":"The unique tax exemption authority identifier for this trade tax."},{"@id":"unece:taxExemptionReasonExemptionReasonCode","@type":["rdf:Property","owl:DatatypeProperty"],"rdfs:label":"taxExemptionReasonExemptionReasonCode","schema:rangeIncludes":{"@id":"unece:TaxExemptionReasonCodeList"},"schema:domainIncludes":[{"@id":"unece:TradeTax"},{"@id":"unece:Tax"}],"rdfs:comment":"A code specifying a reason for exemption from this trade related tax, levy or duty."},{"@id":"unece:taxPointDate","@type":["rdf:Property","owl:DatatypeProperty"],"rdfs:label":"taxPointDate","schema:rangeIncludes":{"@id":"schema:Text"},"schema:domainIncludes":[{"@id":"unece:TradeTax"},{"@id":"unece:AppliedTax"},{"@id":"unece:Tax"}],"rdfs:comment":"The date of the tax point when taxes, such as VAT, are to be applied."},{"@id":"unece:taxType","@type":["rdf:Property","owl:DatatypeProperty"],"rdfs:label":"taxType","schema:rangeIncludes":{"@id":"schema:Text"},"schema:domainIncludes":[{"@id":"unece:TradeTax"},{"@id":"unece:Tax"}],"rdfs:comment":"The type, expressed as text, of this trade related tax, levy or duty."},{"@id":"unece:taxTypeCode","@type":["rdf:Property","owl:DatatypeProperty"],"rdfs:label":"taxTypeCode","schema:rangeIncludes":{"@id":"unece:TaxTypeCodeList"},"schema:domainIncludes":[{"@id":"unece:TradeTax"},{"@id":"unece:Tax"}],"rdfs:comment":"The code specifying the type of trade related tax, levy or duty, such as a code for a Value Added Tax (VAT) [Reference United Nations Code List (UNCL) 5153]."},{"@id":"unece:timeReferenceDueDateTypeCode","@type":["rdf:Property","owl:DatatypeProperty"],"rdfs:label":"timeReferenceDueDateTypeCode","schema:rangeIncludes":{"@id":"unece:TimeReferenceCodeList"},"schema:domainIncludes":[{"@id":"unece:TradeTax"},{"@id":"unece:Tax"}],"rdfs:comment":"The code specifying a type of due date for this trade tax."},{"@id":"unece:tradeTaxCurrencyCode","@type":["rdf:Property","owl:DatatypeProperty"],"rdfs:label":"tradeTaxCurrencyCode","schema:rangeIncludes":{"@id":"unece:CurrencyCodeList"},"schema:domainIncludes":[{"@id":"unece:TradeTax"},{"@id":"unece:Tax"}],"rdfs:comment":"The code specifying the currency for this trade related tax, levy or duty [UNCL 6345]."},{"@id":"unece:tradeTaxPaymentMethodCode","@type":["rdf:Property","owl:DatatypeProperty"],"rdfs:label":"tradeTaxPaymentMethodCode","schema:rangeIncludes":{"@id":"unece:PaymentMethodCodeList"},"schema:domainIncludes":[{"@id":"unece:TradeTax"},{"@id":"unece:Tax"}],"rdfs:comment":"The code specifying the payment method for this trade related tax, levy or duty."},{"@id":"unece:unitBasisAmount","@type":["rdf:Property","owl:ObjectProperty"],"rdfs:label":"unitBasisAmount","schema:rangeIncludes":{"@id":"unece:AmountType"},"schema:domainIncludes":[{"@id":"unece:TradeTax"},{"@id":"unece:Tax"},{"@id":"unece:TradeAllowanceCharge"}],"rdfs:comment":""},{"@id":"unece:productWeightLossInformationAmount","@type":["rdf:Property","owl:ObjectProperty"],"rdfs:label":"productWeightLossInformationAmount","schema:rangeIncludes":{"@id":"unece:AmountType"},"schema:domainIncludes":{"@id":"unece:TradeSettlementLineMonetarySummation"},"rdfs:comment":""},{"@id":"unece:invoiceReferencedDocument","@type":["rdf:Property","owl:ObjectProperty"],"rdfs:label":"invoiceReferencedDocument","schema:rangeIncludes":{"@id":"unece:Document"},"schema:domainIncludes":{"@id":"unece:SubordinateLineTradeSettlement"},"rdfs:comment":"Written, printed or electronic matter that is referenced."},{"@id":"unece:applicableProductBatchCertification","@type":["rdf:Property","owl:ObjectProperty"],"rdfs:label":"applicableProductBatchCertification","schema:rangeIncludes":{"@id":"unece:ProductBatchCertification"},"schema:domainIncludes":{"@id":"unece:ProductBatch"},"rdfs:comment":"The process of certifying that a certain product batch has passed performance and quality assurance tests, or qualification requirements stipulated in regulations."},{"@id":"unece:applicableProductBatchCharacteristic","@type":["rdf:Property","owl:ObjectProperty"],"rdfs:label":"applicableProductBatchCharacteristic","schema:rangeIncludes":{"@id":"unece:ProductBatchCharacteristic"},"schema:domainIncludes":{"@id":"unece:ProductBatch"},"rdfs:comment":"A prominent attribute or aspect of a group of products considered or dealt with together."},{"@id":"unece:appliedAgriculturalApplication","@type":["rdf:Property","owl:ObjectProperty"],"rdfs:label":"appliedAgriculturalApplication","schema:rangeIncludes":{"@id":"unece:AgriculturalApplication"},"schema:domainIncludes":[{"@id":"unece:ProductBatch"},{"@id":"unece:AgriculturalProcess"},{"@id":"unece:Area"},{"@id":"unece:FieldCrop"},{"@id":"unece:Plot"}],"rdfs:comment":"Any substance such as seed, fertilizer, water, gas or chemical applied to an agricultural field, substrate, construction, plant, animal or product."},{"@id":"unece:appliedTreatment","@type":["rdf:Property","owl:DatatypeProperty"],"rdfs:label":"appliedTreatment","schema:rangeIncludes":{"@id":"schema:Text"},"schema:domainIncludes":[{"@id":"unece:ProductBatch"},{"@id":"unece:CropProduceBatch"}],"rdfs:comment":"A treatment, expressed as text, applied to this crop produce batch."},{"@id":"unece:componentProduct","@type":["rdf:Property","owl:ObjectProperty"],"rdfs:label":"componentProduct","schema:rangeIncludes":{"@id":"unece:TradeProduct"},"schema:domainIncludes":{"@id":"unece:ProductBatch"},"rdfs:comment":"A trade product component of this product batch."},{"@id":"unece:massMeasure","@type":["rdf:Property","owl:ObjectProperty"],"rdfs:label":"massMeasure","schema:rangeIncludes":{"@id":"unece:MeasureType"},"schema:domainIncludes":[{"@id":"unece:ProductBatch"},{"@id":"unece:Chemical"},{"@id":"unece:SpecifiedMaterial"}],"rdfs:comment":""},{"@id":"unece:massRatioMeasure","@type":["rdf:Property","owl:ObjectProperty"],"rdfs:label":"massRatioMeasure","schema:rangeIncludes":{"@id":"unece:MeasureType"},"schema:domainIncludes":[{"@id":"unece:ProductBatch"},{"@id":"unece:Chemical"},{"@id":"unece:SpecifiedMaterial"}],"rdfs:comment":""},{"@id":"unece:maximumSizeMeasure","@type":["rdf:Property","owl:ObjectProperty"],"rdfs:label":"maximumSizeMeasure","schema:rangeIncludes":{"@id":"unece:MeasureType"},"schema:domainIncludes":[{"@id":"unece:ProductBatch"},{"@id":"unece:AnimalBatch"}],"rdfs:comment":""},{"@id":"unece:minimumSizeMeasure","@type":["rdf:Property","owl:ObjectProperty"],"rdfs:label":"minimumSizeMeasure","schema:rangeIncludes":{"@id":"unece:MeasureType"},"schema:domainIncludes":[{"@id":"unece:ProductBatch"},{"@id":"unece:AnimalBatch"}],"rdfs:comment":""},{"@id":"unece:productName","@type":["rdf:Property","owl:DatatypeProperty"],"rdfs:label":"productName","schema:rangeIncludes":{"@id":"schema:Text"},"schema:domainIncludes":[{"@id":"unece:ProductBatch"},{"@id":"unece:CropProduceBatch"}],"rdfs:comment":"The product name, expressed as text, for this crop produce batch."},{"@id":"unece:productionModeCode","@type":["rdf:Property","owl:DatatypeProperty"],"rdfs:label":"productionModeCode","schema:rangeIncludes":{"@id":"schema:Text"},"schema:domainIncludes":{"@id":"unece:ProductBatch"},"rdfs:comment":"The code specifying the production mode for this product batch."},{"@id":"unece:sizeMeasure","@type":["rdf:Property","owl:ObjectProperty"],"rdfs:label":"sizeMeasure","schema:rangeIncludes":{"@id":"unece:MeasureType"},"schema:domainIncludes":[{"@id":"unece:ProductBatch"},{"@id":"unece:BinaryFile"},{"@id":"unece:CropProduceBatch"}],"rdfs:comment":""},{"@id":"unece:specifiedAgriculturalCertificate","@type":["rdf:Property","owl:ObjectProperty"],"rdfs:label":"specifiedAgriculturalCertificate","schema:rangeIncludes":{"@id":"unece:AgriculturalCertificate"},"schema:domainIncludes":[{"@id":"unece:ProductBatch"},{"@id":"unece:Plot"},{"@id":"unece:CropProduceBatch"}],"rdfs:comment":"A legal proof of ownership, worthiness or qualification to operate an agricultural item."},{"@id":"unece:specifiedAgriculturalCharacteristic","@type":["rdf:Property","owl:ObjectProperty"],"rdfs:label":"specifiedAgriculturalCharacteristic","schema:rangeIncludes":{"@id":"unece:AgriculturalCharacteristic"},"schema:domainIncludes":[{"@id":"unece:ProductBatch"},{"@id":"unece:FieldCrop"},{"@id":"unece:Plot"},{"@id":"unece:CropProduceBatch"}],"rdfs:comment":"A prominent attribute or aspect of an agricultural object."},{"@id":"unece:specifiedLocation","@type":["rdf:Property","owl:ObjectProperty"],"rdfs:label":"specifiedLocation","schema:rangeIncludes":{"@id":"unece:Location"},"schema:domainIncludes":[{"@id":"unece:ProductBatch"},{"@id":"unece:ProductionDevice"},{"@id":"unece:Machine"},{"@id":"unece:SpecifiedMaterial"},{"@id":"unece:Area"},{"@id":"unece:Plot"},{"@id":"unece:AgriculturalApplication"}],"rdfs:comment":"A reference to a physical location or place."},{"@id":"unece:specifiedProcess","@type":["rdf:Property","owl:ObjectProperty"],"rdfs:label":"specifiedProcess","schema:rangeIncludes":{"@id":"unece:ProductionProcess"},"schema:domainIncludes":[{"@id":"unece:ProductBatch"},{"@id":"unece:ProductionFacility"}],"rdfs:comment":"A production process specified for this product batch."},{"@id":"unece:specifiedProductBatchCertificate","@type":["rdf:Property","owl:ObjectProperty"],"rdfs:label":"specifiedProductBatchCertificate","schema:rangeIncludes":{"@id":"unece:ProductBatchCertificate"},"schema:domainIncludes":[{"@id":"unece:ProductBatch"},{"@id":"unece:ProductionFacility"},{"@id":"unece:ProductionUnit"}],"rdfs:comment":"A piece of written, printed or electronic matter that provides information or evidence that a product batch has met required criteria."},{"@id":"unece:specifiedProductBatchCharacteristic","@type":["rdf:Property","owl:ObjectProperty"],"rdfs:label":"specifiedProductBatchCharacteristic","schema:rangeIncludes":{"@id":"unece:ProductBatchCharacteristic"},"schema:domainIncludes":{"@id":"unece:ProductBatch"},"rdfs:comment":"A prominent attribute or aspect of a group of products considered or dealt with together."},{"@id":"unece:unitQuantity","@type":["rdf:Property","owl:ObjectProperty"],"rdfs:label":"unitQuantity","schema:rangeIncludes":{"@id":"unece:QuantityType"},"schema:domainIncludes":[{"@id":"unece:ProductBatch"},{"@id":"unece:Product"},{"@id":"unece:CommunicationEvent"},{"@id":"unece:EventElement"},{"@id":"unece:ExperienceItem"},{"@id":"unece:CropProduceBatch"},{"@id":"unece:AnimalBatch"},{"@id":"unece:LogisticsTransportEquipment"},{"@id":"unece:TransportEvent"},{"@id":"unece:AssociatedTransportEquipment"},{"@id":"unece:AttachedTransportEquipment"},{"@id":"unece:SupplyChainEvent"}],"rdfs:comment":""},{"@id":"unece:weightMeasure","@type":["rdf:Property","owl:ObjectProperty"],"rdfs:label":"weightMeasure","schema:rangeIncludes":{"@id":"unece:MeasureType"},"schema:domainIncludes":[{"@id":"unece:ProductBatch"},{"@id":"unece:Chemical"},{"@id":"unece:SpecifiedMaterial"},{"@id":"unece:ProductionWasteMaterial"},{"@id":"unece:AnimalBatch"},{"@id":"unece:LogisticsPackaging"},{"@id":"unece:TransportationWasteMaterial"},{"@id":"unece:SupplyChainPackaging"}],"rdfs:comment":""},{"@id":"unece:bufferCapacityMeasure","@type":["rdf:Property","owl:ObjectProperty"],"rdfs:label":"bufferCapacityMeasure","schema:rangeIncludes":{"@id":"unece:MeasureType"},"schema:domainIncludes":{"@id":"unece:ProductionFacility"},"rdfs:comment":""},{"@id":"unece:capacityMeasure","@type":["rdf:Property","owl:ObjectProperty"],"rdfs:label":"capacityMeasure","schema:rangeIncludes":{"@id":"unece:MeasureType"},"schema:domainIncludes":[{"@id":"unece:ProductionFacility"},{"@id":"unece:LogisticsPackaging"}],"rdfs:comment":""},{"@id":"unece:certificationTypeCode","@type":["rdf:Property","owl:DatatypeProperty"],"rdfs:label":"certificationTypeCode","schema:rangeIncludes":{"@id":"schema:Text"},"schema:domainIncludes":[{"@id":"unece:ProductionFacility"},{"@id":"unece:SpecifiedMethod"},{"@id":"unece:LaboratoryObservationAnalysisMethod"}],"rdfs:comment":"The code specifying the certification type of this method."},{"@id":"unece:completionDate","@type":["rdf:Property","owl:DatatypeProperty"],"rdfs:label":"completionDate","schema:rangeIncludes":{"@id":"schema:Text"},"schema:domainIncludes":[{"@id":"unece:ProductionFacility"},{"@id":"unece:ProductionUnit"}],"rdfs:comment":"The completion date of this production facility."},{"@id":"unece:constructionDate","@type":["rdf:Property","owl:DatatypeProperty"],"rdfs:label":"constructionDate","schema:rangeIncludes":{"@id":"schema:Text"},"schema:domainIncludes":[{"@id":"unece:ProductionFacility"},{"@id":"unece:ProductionUnit"}],"rdfs:comment":"The construction date for this production facility."},{"@id":"unece:functionCode","@type":["rdf:Property","owl:DatatypeProperty"],"rdfs:label":"functionCode","schema:rangeIncludes":{"@id":"schema:Text"},"schema:domainIncludes":{"@id":"unece:ProductionFacility"},"rdfs:comment":"The code specifying the function of this production facility."},{"@id":"unece:inputCapacityMeasure","@type":["rdf:Property","owl:ObjectProperty"],"rdfs:label":"inputCapacityMeasure","schema:rangeIncludes":{"@id":"unece:MeasureType"},"schema:domainIncludes":[{"@id":"unece:ProductionFacility"},{"@id":"unece:ProductionDevice"},{"@id":"unece:Machine"}],"rdfs:comment":""},{"@id":"unece:licence","@type":["rdf:Property","owl:DatatypeProperty"],"rdfs:label":"licence","schema:rangeIncludes":{"@id":"schema:Text"},"schema:domainIncludes":[{"@id":"unece:ProductionFacility"},{"@id":"unece:TechnicalCharacteristic"}],"rdfs:comment":"A licence, expressed as text, for this production facility."},{"@id":"unece:outputCapacityMeasure","@type":["rdf:Property","owl:ObjectProperty"],"rdfs:label":"outputCapacityMeasure","schema:rangeIncludes":{"@id":"unece:MeasureType"},"schema:domainIncludes":[{"@id":"unece:ProductionFacility"},{"@id":"unece:ProductionDevice"},{"@id":"unece:Machine"}],"rdfs:comment":""},{"@id":"unece:physicalLocation","@type":["rdf:Property","owl:ObjectProperty"],"rdfs:label":"physicalLocation","schema:rangeIncludes":{"@id":"unece:Location"},"schema:domainIncludes":[{"@id":"unece:ProductionFacility"},{"@id":"unece:ProductionUnit"}],"rdfs:comment":"A reference to a physical location or place."},{"@id":"unece:relatedProductionUnit","@type":["rdf:Property","owl:ObjectProperty"],"rdfs:label":"relatedProductionUnit","schema:rangeIncludes":{"@id":"unece:ProductionUnit"},"schema:domainIncludes":{"@id":"unece:ProductionFacility"},"rdfs:comment":"A facility production unit related to this referenced location."},{"@id":"unece:renovationDate","@type":["rdf:Property","owl:DatatypeProperty"],"rdfs:label":"renovationDate","schema:rangeIncludes":{"@id":"schema:Text"},"schema:domainIncludes":{"@id":"unece:ProductionFacility"},"rdfs:comment":"The renovation date of this production facility."},{"@id":"unece:roofTypeCode","@type":["rdf:Property","owl:DatatypeProperty"],"rdfs:label":"roofTypeCode","schema:rangeIncludes":{"@id":"schema:Text"},"schema:domainIncludes":{"@id":"unece:ProductionFacility"},"rdfs:comment":"The code specifying the type of roof, such as a glass roof, for this production facility."},{"@id":"unece:specifiedAnimalCertificate","@type":["rdf:Property","owl:ObjectProperty"],"rdfs:label":"specifiedAnimalCertificate","schema:rangeIncludes":{"@id":"unece:AnimalCertificate"},"schema:domainIncludes":[{"@id":"unece:ProductionFacility"},{"@id":"unece:TTAnimal"}],"rdfs:comment":"A collection of data for a piece of written, printed or electronic matter that provides information or evidence about the identity of an animal or a batch of animals."},{"@id":"unece:specifiedAnimalCertification","@type":["rdf:Property","owl:ObjectProperty"],"rdfs:label":"specifiedAnimalCertification","schema:rangeIncludes":{"@id":"unece:AnimalCertification"},"schema:domainIncludes":{"@id":"unece:ProductionFacility"},"rdfs:comment":"The process of certifying that a certain animal has met performance and quality assurance requirements, or qualification requirements as stipulated in regulations."},{"@id":"unece:subordinateFacility","@type":["rdf:Property","owl:ObjectProperty"],"rdfs:label":"subordinateFacility","schema:rangeIncludes":{"@id":"unece:ProductionFacility"},"schema:domainIncludes":{"@id":"unece:ProductionFacility"},"rdfs:comment":"A production facility subordinate to this production facility."},{"@id":"unece:applicableHeaderTradeAgreement","@type":["rdf:Property","owl:ObjectProperty"],"rdfs:label":"applicableHeaderTradeAgreement","schema:rangeIncludes":{"@id":"unece:HeaderTradeAgreement"},"schema:domainIncludes":{"@id":"unece:SupplyChainTradeTransaction"},"rdfs:comment":"A trade agreement header applicable to this supply chain trade transaction, such as payment or delivery terms."},{"@id":"unece:applicableHeaderTradeDelivery","@type":["rdf:Property","owl:ObjectProperty"],"rdfs:label":"applicableHeaderTradeDelivery","schema:rangeIncludes":{"@id":"unece:HeaderTradeDelivery"},"schema:domainIncludes":{"@id":"unece:SupplyChainTradeTransaction"},"rdfs:comment":"A trade delivery header applicable to this supply chain trade transaction."},{"@id":"unece:applicableTradeSettlement","@type":["rdf:Property","owl:ObjectProperty"],"rdfs:label":"applicableTradeSettlement","schema:rangeIncludes":{"@id":"unece:HeaderTradeSettlement"},"schema:domainIncludes":{"@id":"unece:SupplyChainTradeTransaction"},"rdfs:comment":"The trade settlement header applicable to this supply chain trade transaction."},{"@id":"unece:associatedFinancingRequestResultDocument","@type":["rdf:Property","owl:ObjectProperty"],"rdfs:label":"associatedFinancingRequestResultDocument","schema:rangeIncludes":{"@id":"unece:FinancingRequestResultDocument"},"schema:domainIncludes":{"@id":"unece:SupplyChainTradeTransaction"},"rdfs:comment":"A collection of data that reports the result of a financing request."},{"@id":"unece:documentURLId","@type":["rdf:Property","owl:DatatypeProperty"],"rdfs:label":"documentURLId","schema:rangeIncludes":{"@id":"schema:Text"},"schema:domainIncludes":{"@id":"unece:SupplyChainTradeTransaction"},"rdfs:comment":"The Uniform Resource Locator (URL) of the web location of the document for this supply chain trade transaction."},{"@id":"unece:includedDeliverySchedule","@type":["rdf:Property","owl:ObjectProperty"],"rdfs:label":"includedDeliverySchedule","schema:rangeIncludes":{"@id":"unece:DeliverySchedule"},"schema:domainIncludes":{"@id":"unece:SupplyChainTradeTransaction"},"rdfs:comment":"Delivery scheduling details included in a defined forecast period for this supply chain trade transaction."},{"@id":"unece:includedNote","@type":["rdf:Property","owl:ObjectProperty"],"rdfs:label":"includedNote","schema:rangeIncludes":{"@id":"unece:Note"},"schema:domainIncludes":[{"@id":"unece:SupplyChainTradeTransaction"},{"@id":"unece:DocumentLineDocument"},{"@id":"unece:Document"},{"@id":"unece:ExchangedDocument"},{"@id":"unece:DocumentStatus"}],"rdfs:comment":"A textual or coded description, such as a remark or additional information."},{"@id":"unece:includedProductGroup","@type":["rdf:Property","owl:ObjectProperty"],"rdfs:label":"includedProductGroup","schema:rangeIncludes":{"@id":"unece:ProductGroup"},"schema:domainIncludes":{"@id":"unece:SupplyChainTradeTransaction"},"rdfs:comment":"A product group included in this supply chain trade transaction."},{"@id":"unece:includedSupplyChainTradeLineItem","@type":["rdf:Property","owl:ObjectProperty"],"rdfs:label":"includedSupplyChainTradeLineItem","schema:rangeIncludes":{"@id":"unece:SupplyChainTradeLineItem"},"schema:domainIncludes":[{"@id":"unece:SupplyChainTradeTransaction"},{"@id":"unece:ProductGroup"}],"rdfs:comment":"A supply chain trade line item included in this logistics package."},{"@id":"unece:information","@type":["rdf:Property","owl:DatatypeProperty"],"rdfs:label":"information","schema:rangeIncludes":{"@id":"schema:Text"},"schema:domainIncludes":[{"@id":"unece:SupplyChainTradeTransaction"},{"@id":"unece:Document"},{"@id":"unece:ExchangedDocument"},{"@id":"unece:SpecifiedMethod"},{"@id":"unece:DocumentStatus"},{"@id":"unece:Segment"},{"@id":"unece:Tolerance"},{"@id":"unece:Authentication"},{"@id":"unece:PaymentMeans"},{"@id":"unece:TradePrice"},{"@id":"unece:LaboratoryObservationAnalysisMethod"},{"@id":"unece:SpecifiedMaterial"},{"@id":"unece:LogisticsTransportEquipment"},{"@id":"unece:Service"},{"@id":"unece:DangerousGoods"},{"@id":"unece:Package"},{"@id":"unece:TransportMovement"},{"@id":"unece:Consignment"},{"@id":"unece:ConsignmentItem"},{"@id":"unece:LogisticsPackaging"}],"rdfs:comment":"Information, expressed as text, concerning the transport of these dangerous goods."},{"@id":"unece:lineItemQuantity","@type":["rdf:Property","owl:ObjectProperty"],"rdfs:label":"lineItemQuantity","schema:rangeIncludes":{"@id":"unece:QuantityType"},"schema:domainIncludes":[{"@id":"unece:SupplyChainTradeTransaction"},{"@id":"unece:ExchangedDocument"}],"rdfs:comment":""},{"@id":"unece:salesAgentAssignedId","@type":["rdf:Property","owl:DatatypeProperty"],"rdfs:label":"salesAgentAssignedId","schema:rangeIncludes":{"@id":"schema:Text"},"schema:domainIncludes":{"@id":"unece:SupplyChainTradeTransaction"},"rdfs:comment":"The unique identifier assigned by the sales agent to identify this supply chain trade transaction."},{"@id":"unece:senderRecipientSequenceId","@type":["rdf:Property","owl:DatatypeProperty"],"rdfs:label":"senderRecipientSequenceId","schema:rangeIncludes":{"@id":"schema:Text"},"schema:domainIncludes":{"@id":"unece:SupplyChainTradeTransaction"},"rdfs:comment":"The sender-recipient sequence identifier for this supply chain trade transaction."},{"@id":"unece:shipmentId","@type":["rdf:Property","owl:DatatypeProperty"],"rdfs:label":"shipmentId","schema:rangeIncludes":{"@id":"schema:Text"},"schema:domainIncludes":{"@id":"unece:SupplyChainTradeTransaction"},"rdfs:comment":"An identifier, such as the Unique Consignment Reference (UCR), for the shipment which is the subject of this supply chain trade transaction."},{"@id":"unece:applicableLineTradeAgreement","@type":["rdf:Property","owl:ObjectProperty"],"rdfs:label":"applicableLineTradeAgreement","schema:rangeIncludes":{"@id":"unece:LineTradeAgreement"},"schema:domainIncludes":{"@id":"unece:LineTradeTransaction"},"rdfs:comment":"A trade agreement applicable to this line trade transaction, such as payment or delivery terms."},{"@id":"unece:applicableLineTradeDelivery","@type":["rdf:Property","owl:ObjectProperty"],"rdfs:label":"applicableLineTradeDelivery","schema:rangeIncludes":{"@id":"unece:LineTradeDelivery"},"schema:domainIncludes":{"@id":"unece:LineTradeTransaction"},"rdfs:comment":"A trade delivery applicable to this line trade transaction."},{"@id":"unece:includedTradeProduct","@type":["rdf:Property","owl:ObjectProperty"],"rdfs:label":"includedTradeProduct","schema:rangeIncludes":{"@id":"unece:TradeProduct"},"schema:domainIncludes":[{"@id":"unece:LineTradeTransaction"},{"@id":"unece:SupplyChainInventory"},{"@id":"unece:ProductGroup"}],"rdfs:comment":"A product included in this supply chain inventory."},{"@id":"unece:applicableMachine","@type":["rdf:Property","owl:ObjectProperty"],"rdfs:label":"applicableMachine","schema:rangeIncludes":{"@id":"unece:Machine"},"schema:domainIncludes":[{"@id":"unece:Colour"},{"@id":"unece:ProductionUnit"}],"rdfs:comment":"A production machine applicable to this facility production unit."},{"@id":"unece:applicableMethod","@type":["rdf:Property","owl:ObjectProperty"],"rdfs:label":"applicableMethod","schema:rangeIncludes":{"@id":"unece:SpecifiedMethod"},"schema:domainIncludes":[{"@id":"unece:Colour"},{"@id":"unece:Print"},{"@id":"unece:ObservationResult"},{"@id":"unece:InspectionResult"},{"@id":"unece:InspectionResultCharacteristic"}],"rdfs:comment":"A defined way of performing something."},{"@id":"unece:applicableProductionDevice","@type":["rdf:Property","owl:ObjectProperty"],"rdfs:label":"applicableProductionDevice","schema:rangeIncludes":{"@id":"unece:ProductionDevice"},"schema:domainIncludes":[{"@id":"unece:Colour"},{"@id":"unece:Print"}],"rdfs:comment":"A production device applicable to this product colour."},{"@id":"unece:applicableStandard","@type":["rdf:Property","owl:ObjectProperty"],"rdfs:label":"applicableStandard","schema:rangeIncludes":{"@id":"unece:Standard"},"schema:domainIncludes":[{"@id":"unece:Colour"},{"@id":"unece:Classification"},{"@id":"unece:OrganizationalCertificate"},{"@id":"unece:ProcessCertificate"},{"@id":"unece:ProductBatchCertificate"},{"@id":"unece:ProductCertificate"},{"@id":"unece:SpecifiedCertificate"},{"@id":"unece:ProductCharacteristic"},{"@id":"unece:ProductBatchCharacteristic"},{"@id":"unece:SustainabilityCharacteristic"},{"@id":"unece:SustainabilityInspection"},{"@id":"unece:Assertion"},{"@id":"unece:Assessment"},{"@id":"unece:OrganizationalCertification"},{"@id":"unece:Policy"},{"@id":"unece:ProcessCertification"},{"@id":"unece:ProcessCharacteristic"},{"@id":"unece:ProductBatchCertification"},{"@id":"unece:TechnicalCharacteristic"},{"@id":"unece:OrganizationCharacteristic"},{"@id":"unece:TradeProductCertification"},{"@id":"unece:AgriculturalCertificate"},{"@id":"unece:AnimalCertificate"}],"rdfs:comment":"A referenced norm or requirement that establishes uniform criteria, methods, processes and practices, such as in engineering or technical areas."},{"@id":"unece:presencePercent","@type":["rdf:Property","owl:DatatypeProperty"],"rdfs:label":"presencePercent","schema:rangeIncludes":{"@id":"schema:Text"},"schema:domainIncludes":[{"@id":"unece:Colour"},{"@id":"unece:Chemical"},{"@id":"unece:SpecifiedMaterial"}],"rdfs:comment":"The percentage of the presence for this specified material."},{"@id":"unece:testIndicator","@type":["rdf:Property","owl:DatatypeProperty"],"rdfs:label":"testIndicator","schema:rangeIncludes":{"@id":"schema:Boolean"},"schema:domainIncludes":[{"@id":"unece:Colour"},{"@id":"unece:Print"},{"@id":"unece:ExchangedDocumentContext"}],"rdfs:comment":"The indication of whether or not this XHE document is a test ."},{"@id":"unece:usedLightSourceCode","@type":["rdf:Property","owl:DatatypeProperty"],"rdfs:label":"usedLightSourceCode","schema:rangeIncludes":{"@id":"schema:Text"},"schema:domainIncludes":{"@id":"unece:Colour"},"rdfs:comment":"The code specifying the light source used for this product colour."},{"@id":"unece:variationMeasureCoefficientNumeric","@type":["rdf:Property","owl:DatatypeProperty"],"rdfs:label":"variationMeasureCoefficientNumeric","schema:rangeIncludes":{"@id":"schema:Text"},"schema:domainIncludes":{"@id":"unece:Colour"},"rdfs:comment":"The measure of the variation coefficient number for this product colour."},{"@id":"unece:dedicatedFacility","@type":["rdf:Property","owl:ObjectProperty"],"rdfs:label":"dedicatedFacility","schema:rangeIncludes":{"@id":"unece:ProductionFacility"},"schema:domainIncludes":{"@id":"unece:ProductionUnit"},"rdfs:comment":"A dedicated production facility for this production unit."},{"@id":"unece:subordinateProductionUnit","@type":["rdf:Property","owl:ObjectProperty"],"rdfs:label":"subordinateProductionUnit","schema:rangeIncludes":{"@id":"unece:ProductionUnit"},"schema:domainIncludes":{"@id":"unece:ProductionUnit"},"rdfs:comment":"A production unit subordinate to this facility production unit."},{"@id":"unece:backgroundColourCode","@type":["rdf:Property","owl:DatatypeProperty"],"rdfs:label":"backgroundColourCode","schema:rangeIncludes":{"@id":"schema:Text"},"schema:domainIncludes":{"@id":"unece:Print"},"rdfs:comment":"The code specifying the background colour for this product print."},{"@id":"unece:design","@type":["rdf:Property","owl:DatatypeProperty"],"rdfs:label":"design","schema:rangeIncludes":{"@id":"schema:Text"},"schema:domainIncludes":{"@id":"unece:Print"},"rdfs:comment":"A textual description of a design for this product print."},{"@id":"unece:designCode","@type":["rdf:Property","owl:DatatypeProperty"],"rdfs:label":"designCode","schema:rangeIncludes":{"@id":"schema:Text"},"schema:domainIncludes":{"@id":"unece:Print"},"rdfs:comment":"The code specifying the design for this product print."},{"@id":"unece:section","@type":["rdf:Property","owl:DatatypeProperty"],"rdfs:label":"section","schema:rangeIncludes":{"@id":"schema:Text"},"schema:domainIncludes":{"@id":"unece:Print"},"rdfs:comment":"A section, expressed as text, of this product print."},{"@id":"unece:specifiedMachine","@type":["rdf:Property","owl:ObjectProperty"],"rdfs:label":"specifiedMachine","schema:rangeIncludes":{"@id":"unece:Machine"},"schema:domainIncludes":{"@id":"unece:Print"},"rdfs:comment":"A production machine specified for this product print."},{"@id":"unece:textContent","@type":["rdf:Property","owl:DatatypeProperty"],"rdfs:label":"textContent","schema:rangeIncludes":{"@id":"schema:Text"},"schema:domainIncludes":{"@id":"unece:Print"},"rdfs:comment":"A textual description of the content for this product print."},{"@id":"unece:combinedMachine","@type":["rdf:Property","owl:ObjectProperty"],"rdfs:label":"combinedMachine","schema:rangeIncludes":{"@id":"unece:Machine"},"schema:domainIncludes":[{"@id":"unece:ProductionDevice"},{"@id":"unece:Machine"}],"rdfs:comment":"A production machine combined with this production machine."},{"@id":"unece:combinedProductionDevice","@type":["rdf:Property","owl:ObjectProperty"],"rdfs:label":"combinedProductionDevice","schema:rangeIncludes":{"@id":"unece:ProductionDevice"},"schema:domainIncludes":[{"@id":"unece:ProductionDevice"},{"@id":"unece:Machine"}],"rdfs:comment":"A production device combined with this production machine."},{"@id":"unece:productionDeviceType","@type":["rdf:Property","owl:DatatypeProperty"],"rdfs:label":"productionDeviceType","schema:rangeIncludes":{"@id":"schema:Text"},"schema:domainIncludes":{"@id":"unece:ProductionDevice"},"rdfs:comment":"A type, expressed as text, for this specified production device."},{"@id":"unece:reportingIOTDeviceSupplyChainEvent","@type":["rdf:Property","owl:ObjectProperty"],"rdfs:label":"reportingIOTDeviceSupplyChainEvent","schema:rangeIncludes":{"@id":"unece:SupplyChainEvent"},"schema:domainIncludes":[{"@id":"unece:ProductionDevice"},{"@id":"unece:Machine"}],"rdfs:comment":"A significant occurrence or happening in a supply chain."},{"@id":"unece:requestedOperationalApplicableParameter","@type":["rdf:Property","owl:ObjectProperty"],"rdfs:label":"requestedOperationalApplicableParameter","schema:rangeIncludes":{"@id":"unece:SpecifiedParameter"},"schema:domainIncludes":[{"@id":"unece:ProductionDevice"},{"@id":"unece:Machine"}],"rdfs:comment":"A specified feature that is fixed for the case in question but may be different in other cases."},{"@id":"unece:specifiedProductionUnit","@type":["rdf:Property","owl:ObjectProperty"],"rdfs:label":"specifiedProductionUnit","schema:rangeIncludes":{"@id":"unece:ProductionUnit"},"schema:domainIncludes":[{"@id":"unece:ProductionDevice"},{"@id":"unece:Machine"}],"rdfs:comment":"A facility production unit for this specified production device."},{"@id":"unece:usedMaterial","@type":["rdf:Property","owl:ObjectProperty"],"rdfs:label":"usedMaterial","schema:rangeIncludes":{"@id":"unece:SpecifiedMaterial"},"schema:domainIncludes":[{"@id":"unece:ProductFinishingTreatment"},{"@id":"unece:CropProtectionTreatment"}],"rdfs:comment":"A substance from which something is or could be made."},{"@id":"unece:applicableProcessCharacteristic","@type":["rdf:Property","owl:ObjectProperty"],"rdfs:label":"applicableProcessCharacteristic","schema:rangeIncludes":{"@id":"unece:ProcessCharacteristic"},"schema:domainIncludes":[{"@id":"unece:ProductHandlingProcess"},{"@id":"unece:ProcessCertificate"}],"rdfs:comment":"A prominent attribute or aspect of a process."},{"@id":"unece:completionPeriod","@type":["rdf:Property","owl:ObjectProperty"],"rdfs:label":"completionPeriod","schema:rangeIncludes":{"@id":"unece:SpecifiedPeriod"},"schema:domainIncludes":{"@id":"unece:ProductHandlingProcess"},"rdfs:comment":"A specified period of time."},{"@id":"unece:operationCountry","@type":["rdf:Property","owl:ObjectProperty"],"rdfs:label":"operationCountry","schema:rangeIncludes":{"@id":"unece:Country"},"schema:domainIncludes":{"@id":"unece:ProductHandlingProcess"},"rdfs:comment":"The area of land that belongs to a nation together with its properties, such as population, political organization, etc., used or referenced for trade purposes."},{"@id":"unece:operatorParty","@type":["rdf:Property","owl:ObjectProperty"],"rdfs:label":"operatorParty","schema:rangeIncludes":{"@id":"unece:TradeParty"},"schema:domainIncludes":[{"@id":"unece:ProductHandlingProcess"},{"@id":"unece:LogisticsTransportMeans"},{"@id":"unece:IOTDevice"}],"rdfs:comment":"A trade party who is an operator of this product handling process."},{"@id":"unece:processTypeCode","@type":["rdf:Property","owl:DatatypeProperty"],"rdfs:label":"processTypeCode","schema:rangeIncludes":{"@id":"unece:ProcessTypeCodeList"},"schema:domainIncludes":{"@id":"unece:ProductHandlingProcess"},"rdfs:comment":"The code specifying the type of product handling process."},{"@id":"unece:applicableProduct","@type":["rdf:Property","owl:ObjectProperty"],"rdfs:label":"applicableProduct","schema:rangeIncludes":{"@id":"unece:TradeProduct"},"schema:domainIncludes":{"@id":"unece:SubordinateTradeLineItem"},"rdfs:comment":"A product applicable for this subordinate trade line item."},{"@id":"unece:categoryCode","@type":["rdf:Property","owl:DatatypeProperty"],"rdfs:label":"categoryCode","schema:rangeIncludes":{"@id":"schema:Text"},"schema:domainIncludes":[{"@id":"unece:SubordinateTradeLineItem"},{"@id":"unece:ProductLabel"},{"@id":"unece:DocumentLineDocument"},{"@id":"unece:Document"},{"@id":"unece:ExchangedDocument"},{"@id":"unece:SpecifiedFault"},{"@id":"unece:Object"},{"@id":"unece:CustomerClass"},{"@id":"unece:InformationSource"},{"@id":"unece:Authentication"},{"@id":"unece:ProtectionMeans"},{"@id":"unece:Accreditation"},{"@id":"unece:RegulatoryProcedure"},{"@id":"unece:SpecifiedCertificate"},{"@id":"unece:SustainabilityCharacteristic"},{"@id":"unece:Assessment"},{"@id":"unece:Source"},{"@id":"unece:GovernmentRegistration"},{"@id":"unece:RiskAnalysisResult"},{"@id":"unece:PetAnimal"},{"@id":"unece:ExperienceItem"},{"@id":"unece:ExperienceProduct"},{"@id":"unece:TransportPerson"}],"rdfs:comment":"A code specifying a category for this cross-border regulatory procedure, such as the appendices of the CITES Convention."},{"@id":"unece:responseReasonCode","@type":["rdf:Property","owl:DatatypeProperty"],"rdfs:label":"responseReasonCode","schema:rangeIncludes":{"@id":"schema:Text"},"schema:domainIncludes":[{"@id":"unece:SubordinateTradeLineItem"},{"@id":"unece:DocumentLineDocument"},{"@id":"unece:ExchangedDocument"}],"rdfs:comment":"A code specifying a response reason for this exchanged document."},{"@id":"unece:specifiedProduct","@type":["rdf:Property","owl:ObjectProperty"],"rdfs:label":"specifiedProduct","schema:rangeIncludes":{"@id":"unece:Product"},"schema:domainIncludes":{"@id":"unece:SubordinateTradeLineItem"},"rdfs:comment":"The referenced product specified for this subordinate trade line item."},{"@id":"unece:specifiedSubordinateLineTradeAgreement","@type":["rdf:Property","owl:ObjectProperty"],"rdfs:label":"specifiedSubordinateLineTradeAgreement","schema:rangeIncludes":{"@id":"unece:SubordinateLineTradeAgreement"},"schema:domainIncludes":{"@id":"unece:SubordinateTradeLineItem"},"rdfs:comment":"The trade agreement specified for this subordinate trade line item."},{"@id":"unece:specifiedSubordinateLineTradeDelivery","@type":["rdf:Property","owl:ObjectProperty"],"rdfs:label":"specifiedSubordinateLineTradeDelivery","schema:rangeIncludes":{"@id":"unece:SubordinateLineTradeDelivery"},"schema:domainIncludes":{"@id":"unece:SubordinateTradeLineItem"},"rdfs:comment":"The delivery specified for this subordinate trade line item."},{"@id":"unece:specifiedSubordinateLineTradeSettlement","@type":["rdf:Property","owl:ObjectProperty"],"rdfs:label":"specifiedSubordinateLineTradeSettlement","schema:rangeIncludes":{"@id":"unece:SubordinateLineTradeSettlement"},"schema:domainIncludes":{"@id":"unece:SubordinateTradeLineItem"},"rdfs:comment":"A trade settlement specified for this subordinate trade line item."},{"@id":"unece:endDateTime","@type":["rdf:Property","owl:DatatypeProperty"],"rdfs:label":"endDateTime","schema:rangeIncludes":{"@id":"schema:Text"},"schema:domainIncludes":[{"@id":"unece:ProductionCycle"},{"@id":"unece:SpecifiedPeriod"},{"@id":"unece:AvailablePeriod"},{"@id":"unece:Membership"},{"@id":"unece:DelimitedPeriod"},{"@id":"unece:Assessment"},{"@id":"unece:SpecifiedCertification"},{"@id":"unece:Plot"}],"rdfs:comment":"The date, time, date time or other date time value for the end of this available period of time."},{"@id":"unece:processSpecifiedDocument","@type":["rdf:Property","owl:ObjectProperty"],"rdfs:label":"processSpecifiedDocument","schema:rangeIncludes":{"@id":"unece:Document"},"schema:domainIncludes":{"@id":"unece:ProductionCycle"},"rdfs:comment":"Written, printed or electronic matter that is referenced."},{"@id":"unece:productionYearDateTime","@type":["rdf:Property","owl:DatatypeProperty"],"rdfs:label":"productionYearDateTime","schema:rangeIncludes":{"@id":"schema:Text"},"schema:domainIncludes":{"@id":"unece:ProductionCycle"},"rdfs:comment":"The production year for this specified production cycle."},{"@id":"unece:startDateTime","@type":["rdf:Property","owl:DatatypeProperty"],"rdfs:label":"startDateTime","schema:rangeIncludes":{"@id":"schema:Text"},"schema:domainIncludes":[{"@id":"unece:ProductionCycle"},{"@id":"unece:SpecifiedPeriod"},{"@id":"unece:AvailablePeriod"},{"@id":"unece:Membership"},{"@id":"unece:DelimitedPeriod"},{"@id":"unece:Assessment"},{"@id":"unece:SpecifiedCertification"},{"@id":"unece:Plot"}],"rdfs:comment":"The date, time, date time or other date time value for the start of this available period of time."},{"@id":"unece:usedChemical","@type":["rdf:Property","owl:ObjectProperty"],"rdfs:label":"usedChemical","schema:rangeIncludes":{"@id":"unece:Chemical"},"schema:domainIncludes":[{"@id":"unece:SpecifiedChemicalTreatment"},{"@id":"unece:AppliedChemicalTreatment"},{"@id":"unece:SpecifiedMaterial"}],"rdfs:comment":"Any clearly defined substance having a defined molecular composition."},{"@id":"unece:closingBookDueDateTime","@type":["rdf:Property","owl:DatatypeProperty"],"rdfs:label":"closingBookDueDateTime","schema:rangeIncludes":{"@id":"schema:Text"},"schema:domainIncludes":[{"@id":"unece:HeaderTradeSettlement"},{"@id":"unece:TradeSettlementPayment"}],"rdfs:comment":"A date, time, date time or other date time value of a closing book due date for this trade settlement payment."},{"@id":"unece:creditNoteAmount","@type":["rdf:Property","owl:ObjectProperty"],"rdfs:label":"creditNoteAmount","schema:rangeIncludes":{"@id":"unece:AmountType"},"schema:domainIncludes":{"@id":"unece:HeaderTradeSettlement"},"rdfs:comment":""},{"@id":"unece:creditReason","@type":["rdf:Property","owl:DatatypeProperty"],"rdfs:label":"creditReason","schema:rangeIncludes":{"@id":"schema:Text"},"schema:domainIncludes":{"@id":"unece:HeaderTradeSettlement"},"rdfs:comment":"A textual description of the reason for a credit being given in this header trade settlement."},{"@id":"unece:creditReasonCode","@type":["rdf:Property","owl:DatatypeProperty"],"rdfs:label":"creditReasonCode","schema:rangeIncludes":{"@id":"schema:Text"},"schema:domainIncludes":{"@id":"unece:HeaderTradeSettlement"},"rdfs:comment":"The code specifying the reason for a credit being given in this header trade settlement."},{"@id":"unece:creditorReferenceId","@type":["rdf:Property","owl:DatatypeProperty"],"rdfs:label":"creditorReferenceId","schema:rangeIncludes":{"@id":"schema:Text"},"schema:domainIncludes":{"@id":"unece:HeaderTradeSettlement"},"rdfs:comment":"The identifier of the creditor reference for this header trade settlement, such as a specific identifier assigned by the creditor to reference the financial transaction."},{"@id":"unece:creditorReferenceIssuerId","@type":["rdf:Property","owl:DatatypeProperty"],"rdfs:label":"creditorReferenceIssuerId","schema:rangeIncludes":{"@id":"schema:Text"},"schema:domainIncludes":{"@id":"unece:HeaderTradeSettlement"},"rdfs:comment":"An identifier of the creditor reference issuer for this header trade settlement."},{"@id":"unece:creditorReferenceType","@type":["rdf:Property","owl:DatatypeProperty"],"rdfs:label":"creditorReferenceType","schema:rangeIncludes":{"@id":"schema:Text"},"schema:domainIncludes":{"@id":"unece:HeaderTradeSettlement"},"rdfs:comment":"A creditor reference type, expressed as text, for this header trade settlement."},{"@id":"unece:debitNoteAmount","@type":["rdf:Property","owl:ObjectProperty"],"rdfs:label":"debitNoteAmount","schema:rangeIncludes":{"@id":"unece:AmountType"},"schema:domainIncludes":{"@id":"unece:HeaderTradeSettlement"},"rdfs:comment":""},{"@id":"unece:factoringAgreementDocument","@type":["rdf:Property","owl:ObjectProperty"],"rdfs:label":"factoringAgreementDocument","schema:rangeIncludes":{"@id":"unece:Document"},"schema:domainIncludes":{"@id":"unece:HeaderTradeSettlement"},"rdfs:comment":"Written, printed or electronic matter that is referenced."},{"@id":"unece:factoringListDocument","@type":["rdf:Property","owl:ObjectProperty"],"rdfs:label":"factoringListDocument","schema:rangeIncludes":{"@id":"unece:Document"},"schema:domainIncludes":{"@id":"unece:HeaderTradeSettlement"},"rdfs:comment":"Written, printed or electronic matter that is referenced."},{"@id":"unece:invoiceApplicableCurrencyExchange","@type":["rdf:Property","owl:ObjectProperty"],"rdfs:label":"invoiceApplicableCurrencyExchange","schema:rangeIncludes":{"@id":"unece:CurrencyExchange"},"schema:domainIncludes":[{"@id":"unece:HeaderTradeSettlement"},{"@id":"unece:Consignment"}],"rdfs:comment":"The conversion of one currency to another for trade purposes."},{"@id":"unece:invoiceCurrencyCode","@type":["rdf:Property","owl:DatatypeProperty"],"rdfs:label":"invoiceCurrencyCode","schema:rangeIncludes":{"@id":"unece:CurrencyCodeList"},"schema:domainIncludes":{"@id":"unece:HeaderTradeSettlement"},"rdfs:comment":"The code specifying the invoice currency for this header trade settlement."},{"@id":"unece:invoicerParty","@type":["rdf:Property","owl:ObjectProperty"],"rdfs:label":"invoicerParty","schema:rangeIncludes":{"@id":"unece:TradeParty"},"schema:domainIncludes":{"@id":"unece:HeaderTradeSettlement"},"rdfs:comment":"The party issuing the invoice for this header trade settlement."},{"@id":"unece:nextInvoiceDateTime","@type":["rdf:Property","owl:DatatypeProperty"],"rdfs:label":"nextInvoiceDateTime","schema:rangeIncludes":{"@id":"schema:Text"},"schema:domainIncludes":{"@id":"unece:HeaderTradeSettlement"},"rdfs:comment":"A date, time, date time or other date time value of a next invoice or invoices in this header trade settlement."},{"@id":"unece:orderApplicableCurrencyExchange","@type":["rdf:Property","owl:ObjectProperty"],"rdfs:label":"orderApplicableCurrencyExchange","schema:rangeIncludes":{"@id":"unece:CurrencyExchange"},"schema:domainIncludes":{"@id":"unece:HeaderTradeSettlement"},"rdfs:comment":"The conversion of one currency to another for trade purposes."},{"@id":"unece:orderCurrencyCode","@type":["rdf:Property","owl:DatatypeProperty"],"rdfs:label":"orderCurrencyCode","schema:rangeIncludes":{"@id":"unece:CurrencyCodeList"},"schema:domainIncludes":{"@id":"unece:HeaderTradeSettlement"},"rdfs:comment":"The code specifying the currency of the order for this header trade settlement."},{"@id":"unece:payeeParty","@type":["rdf:Property","owl:ObjectProperty"],"rdfs:label":"payeeParty","schema:rangeIncludes":{"@id":"unece:TradeParty"},"schema:domainIncludes":[{"@id":"unece:HeaderTradeSettlement"},{"@id":"unece:PaymentTradeSettlement"},{"@id":"unece:PaymentTerms"}],"rdfs:comment":"A payee party for this header trade settlement."},{"@id":"unece:paymentApplicableCurrencyExchange","@type":["rdf:Property","owl:ObjectProperty"],"rdfs:label":"paymentApplicableCurrencyExchange","schema:rangeIncludes":{"@id":"unece:CurrencyExchange"},"schema:domainIncludes":[{"@id":"unece:HeaderTradeSettlement"},{"@id":"unece:PaymentTradeSettlement"}],"rdfs:comment":"The conversion of one currency to another for trade purposes."},{"@id":"unece:paymentCurrencyCode","@type":["rdf:Property","owl:DatatypeProperty"],"rdfs:label":"paymentCurrencyCode","schema:rangeIncludes":{"@id":"unece:CurrencyCodeList"},"schema:domainIncludes":[{"@id":"unece:HeaderTradeSettlement"},{"@id":"unece:PaymentTradeSettlement"}],"rdfs:comment":"The code specifying the currency for this payment trade settlement."},{"@id":"unece:priceApplicableCurrencyExchange","@type":["rdf:Property","owl:ObjectProperty"],"rdfs:label":"priceApplicableCurrencyExchange","schema:rangeIncludes":{"@id":"unece:CurrencyExchange"},"schema:domainIncludes":{"@id":"unece:HeaderTradeSettlement"},"rdfs:comment":"The conversion of one currency to another for trade purposes."},{"@id":"unece:proFormaInvoiceDocument","@type":["rdf:Property","owl:ObjectProperty"],"rdfs:label":"proFormaInvoiceDocument","schema:rangeIncludes":{"@id":"unece:Document"},"schema:domainIncludes":{"@id":"unece:HeaderTradeSettlement"},"rdfs:comment":"Written, printed or electronic matter that is referenced."},{"@id":"unece:quotationApplicableCurrencyExchange","@type":["rdf:Property","owl:ObjectProperty"],"rdfs:label":"quotationApplicableCurrencyExchange","schema:rangeIncludes":{"@id":"unece:CurrencyExchange"},"schema:domainIncludes":{"@id":"unece:HeaderTradeSettlement"},"rdfs:comment":"The conversion of one currency to another for trade purposes."},{"@id":"unece:quotationCurrencyCode","@type":["rdf:Property","owl:DatatypeProperty"],"rdfs:label":"quotationCurrencyCode","schema:rangeIncludes":{"@id":"unece:CurrencyCodeList"},"schema:domainIncludes":{"@id":"unece:HeaderTradeSettlement"},"rdfs:comment":"The code specifying the quotation currency for this header trade settlement."},{"@id":"unece:requestedFinancingAmount","@type":["rdf:Property","owl:ObjectProperty"],"rdfs:label":"requestedFinancingAmount","schema:rangeIncludes":{"@id":"unece:AmountType"},"schema:domainIncludes":{"@id":"unece:HeaderTradeSettlement"},"rdfs:comment":""},{"@id":"unece:requestedFinancingRatePercent","@type":["rdf:Property","owl:DatatypeProperty"],"rdfs:label":"requestedFinancingRatePercent","schema:rangeIncludes":{"@id":"schema:Text"},"schema:domainIncludes":{"@id":"unece:HeaderTradeSettlement"},"rdfs:comment":"The financing rate, expressed as a percentage, requested for this header trade settlement."},{"@id":"unece:scheduledPaymentDateTime","@type":["rdf:Property","owl:DatatypeProperty"],"rdfs:label":"scheduledPaymentDateTime","schema:rangeIncludes":{"@id":"schema:Text"},"schema:domainIncludes":{"@id":"unece:HeaderTradeSettlement"},"rdfs:comment":"The date, time, date time or other date time value of the scheduled payment of this header trade settlement."},{"@id":"unece:specifiedAdvancePayment","@type":["rdf:Property","owl:ObjectProperty"],"rdfs:label":"specifiedAdvancePayment","schema:rangeIncludes":{"@id":"unece:AdvancePayment"},"schema:domainIncludes":{"@id":"unece:HeaderTradeSettlement"},"rdfs:comment":"A prepaid discharge of obligations in respect of funds or securities transferred between two or more parties."},{"@id":"unece:specifiedInstalmentPlan","@type":["rdf:Property","owl:ObjectProperty"],"rdfs:label":"specifiedInstalmentPlan","schema:rangeIncludes":{"@id":"unece:InstalmentPlan"},"schema:domainIncludes":{"@id":"unece:HeaderTradeSettlement"},"rdfs:comment":"A plan for paying a total sum of money by several payments made over a period of time."},{"@id":"unece:specifiedPaymentMeans","@type":["rdf:Property","owl:ObjectProperty"],"rdfs:label":"specifiedPaymentMeans","schema:rangeIncludes":{"@id":"unece:PaymentMeans"},"schema:domainIncludes":[{"@id":"unece:HeaderTradeSettlement"},{"@id":"unece:PaymentTradeSettlement"},{"@id":"unece:GuestPerson"},{"@id":"unece:ServiceCharge"}],"rdfs:comment":"The means by which a payment will be or has been made for trade settlement purposes."},{"@id":"unece:specifiedTradeSettlementHeaderMonetarySummation","@type":["rdf:Property","owl:ObjectProperty"],"rdfs:label":"specifiedTradeSettlementHeaderMonetarySummation","schema:rangeIncludes":{"@id":"unece:TradeSettlementHeaderMonetarySummation"},"schema:domainIncludes":{"@id":"unece:HeaderTradeSettlement"},"rdfs:comment":"The monetary summation totals specified for this header trade settlement."},{"@id":"unece:taxApplicableCurrencyExchange","@type":["rdf:Property","owl:ObjectProperty"],"rdfs:label":"taxApplicableCurrencyExchange","schema:rangeIncludes":{"@id":"unece:CurrencyExchange"},"schema:domainIncludes":{"@id":"unece:HeaderTradeSettlement"},"rdfs:comment":"The conversion of one currency to another for trade purposes."},{"@id":"unece:taxCurrencyCode","@type":["rdf:Property","owl:DatatypeProperty"],"rdfs:label":"taxCurrencyCode","schema:rangeIncludes":{"@id":"unece:CurrencyCodeList"},"schema:domainIncludes":{"@id":"unece:HeaderTradeSettlement"},"rdfs:comment":"The code specifying the tax currency for this header trade settlement."},{"@id":"unece:totalInvoiceAmount","@type":["rdf:Property","owl:ObjectProperty"],"rdfs:label":"totalInvoiceAmount","schema:rangeIncludes":{"@id":"unece:AmountType"},"schema:domainIncludes":{"@id":"unece:HeaderTradeSettlement"},"rdfs:comment":""},{"@id":"unece:ultimatePayeeParty","@type":["rdf:Property","owl:ObjectProperty"],"rdfs:label":"ultimatePayeeParty","schema:rangeIncludes":{"@id":"unece:TradeParty"},"schema:domainIncludes":{"@id":"unece:HeaderTradeSettlement"},"rdfs:comment":"An ultimate payee party in this header trade settlement."},{"@id":"unece:attachmentDateTime","@type":["rdf:Property","owl:DatatypeProperty"],"rdfs:label":"attachmentDateTime","schema:rangeIncludes":{"@id":"schema:Text"},"schema:domainIncludes":{"@id":"unece:ProductLabel"},"rdfs:comment":"The date, time, date time, or other date time value, for the attachment of this product label."},{"@id":"unece:includedAssertion","@type":["rdf:Property","owl:ObjectProperty"],"rdfs:label":"includedAssertion","schema:rangeIncludes":{"@id":"unece:Assertion"},"schema:domainIncludes":{"@id":"unece:ProductLabel"},"rdfs:comment":"A statement that user needs of the present are met without compromising the needs of future generations."},{"@id":"unece:layoutTypeCode","@type":["rdf:Property","owl:DatatypeProperty"],"rdfs:label":"layoutTypeCode","schema:rangeIncludes":{"@id":"schema:Text"},"schema:domainIncludes":[{"@id":"unece:ProductLabel"},{"@id":"unece:LogisticsLabel"}],"rdfs:comment":"The code specifying the layout type of this logistics label."},{"@id":"unece:seriesEndId","@type":["rdf:Property","owl:DatatypeProperty"],"rdfs:label":"seriesEndId","schema:rangeIncludes":{"@id":"schema:Text"},"schema:domainIncludes":[{"@id":"unece:ProductLabel"},{"@id":"unece:Package"},{"@id":"unece:LogisticsLabel"}],"rdfs:comment":"The identifier of the end of a series of packages within this referenced logistics package."},{"@id":"unece:seriesStartId","@type":["rdf:Property","owl:DatatypeProperty"],"rdfs:label":"seriesStartId","schema:rangeIncludes":{"@id":"schema:Text"},"schema:domainIncludes":[{"@id":"unece:ProductLabel"},{"@id":"unece:Package"},{"@id":"unece:LogisticsLabel"}],"rdfs:comment":"The identifier of the start of a series of packages within this referenced logistics package."},{"@id":"unece:tagTypeCode","@type":["rdf:Property","owl:DatatypeProperty"],"rdfs:label":"tagTypeCode","schema:rangeIncludes":{"@id":"schema:Text"},"schema:domainIncludes":{"@id":"unece:ProductLabel"},"rdfs:comment":"The code specifying the type of tag for this product label."},{"@id":"unece:automaticExtensionDateTime","@type":["rdf:Property","owl:DatatypeProperty"],"rdfs:label":"automaticExtensionDateTime","schema:rangeIncludes":{"@id":"schema:DateTime"},"schema:domainIncludes":{"@id":"unece:Contract"},"rdfs:comment":"The date, time, date time, or other date time value of automatic extension for this trade contract."},{"@id":"unece:automaticExtensionDurationMeasure","@type":["rdf:Property","owl:ObjectProperty"],"rdfs:label":"automaticExtensionDurationMeasure","schema:rangeIncludes":{"@id":"unece:DurationUnitMeasureType"},"schema:domainIncludes":{"@id":"unece:Contract"},"rdfs:comment":""},{"@id":"unece:signatureName","@type":["rdf:Property","owl:DatatypeProperty"],"rdfs:label":"signatureName","schema:rangeIncludes":{"@id":"schema:Text"},"schema:domainIncludes":{"@id":"unece:Contract"},"rdfs:comment":"A signature name, expressed as text, for this trade contract."},{"@id":"unece:signedDateTime","@type":["rdf:Property","owl:DatatypeProperty"],"rdfs:label":"signedDateTime","schema:rangeIncludes":{"@id":"schema:DateTime"},"schema:domainIncludes":{"@id":"unece:Contract"},"rdfs:comment":"The date, time, date time or other date time value when this trade contract was signed."},{"@id":"unece:signedLocation","@type":["rdf:Property","owl:ObjectProperty"],"rdfs:label":"signedLocation","schema:rangeIncludes":{"@id":"unece:SpecifiedLocation"},"schema:domainIncludes":{"@id":"unece:Contract"},"rdfs:comment":"A specified physical location or place."},{"@id":"unece:signeeJobTitle","@type":["rdf:Property","owl:DatatypeProperty"],"rdfs:label":"signeeJobTitle","schema:rangeIncludes":{"@id":"schema:Text"},"schema:domainIncludes":{"@id":"unece:Contract"},"rdfs:comment":"A job title of the signee, expressed as text, for this trade contract."},{"@id":"unece:averageDemandQuantity","@type":["rdf:Property","owl:ObjectProperty"],"rdfs:label":"averageDemandQuantity","schema:rangeIncludes":{"@id":"unece:QuantityType"},"schema:domainIncludes":{"@id":"unece:SupplyChainInventory"},"rdfs:comment":""},{"@id":"unece:averageDurationDateTime","@type":["rdf:Property","owl:DatatypeProperty"],"rdfs:label":"averageDurationDateTime","schema:rangeIncludes":{"@id":"schema:Text"},"schema:domainIncludes":{"@id":"unece:SupplyChainInventory"},"rdfs:comment":"The date, time, date time, or other date time of the average duration for this supply chain inventory."},{"@id":"unece:calculationDateTime","@type":["rdf:Property","owl:DatatypeProperty"],"rdfs:label":"calculationDateTime","schema:rangeIncludes":{"@id":"schema:Text"},"schema:domainIncludes":{"@id":"unece:SupplyChainInventory"},"rdfs:comment":"The date, time, date time, or other date time value of the calculation of this supply chain inventory."},{"@id":"unece:dispositionDocument","@type":["rdf:Property","owl:ObjectProperty"],"rdfs:label":"dispositionDocument","schema:rangeIncludes":{"@id":"unece:Document"},"schema:domainIncludes":{"@id":"unece:SupplyChainInventory"},"rdfs:comment":"Written, printed or electronic matter that is referenced."},{"@id":"unece:includedBatch","@type":["rdf:Property","owl:ObjectProperty"],"rdfs:label":"includedBatch","schema:rangeIncludes":{"@id":"unece:ProductBatch"},"schema:domainIncludes":{"@id":"unece:SupplyChainInventory"},"rdfs:comment":"A product batch included in this supply chain inventory."},{"@id":"unece:includedMaterial","@type":["rdf:Property","owl:ObjectProperty"],"rdfs:label":"includedMaterial","schema:rangeIncludes":{"@id":"unece:SpecifiedMaterial"},"schema:domainIncludes":{"@id":"unece:SupplyChainInventory"},"rdfs:comment":"A substance from which something is or could be made."},{"@id":"unece:maximumStockLevelMeasure","@type":["rdf:Property","owl:ObjectProperty"],"rdfs:label":"maximumStockLevelMeasure","schema:rangeIncludes":{"@id":"unece:MeasureType"},"schema:domainIncludes":{"@id":"unece:SupplyChainInventory"},"rdfs:comment":""},{"@id":"unece:maximumStockQuantity","@type":["rdf:Property","owl:ObjectProperty"],"rdfs:label":"maximumStockQuantity","schema:rangeIncludes":{"@id":"unece:QuantityType"},"schema:domainIncludes":{"@id":"unece:SupplyChainInventory"},"rdfs:comment":""},{"@id":"unece:minimumStockLevelMeasure","@type":["rdf:Property","owl:ObjectProperty"],"rdfs:label":"minimumStockLevelMeasure","schema:rangeIncludes":{"@id":"unece:MeasureType"},"schema:domainIncludes":{"@id":"unece:SupplyChainInventory"},"rdfs:comment":""},{"@id":"unece:minimumStockQuantity","@type":["rdf:Property","owl:ObjectProperty"],"rdfs:label":"minimumStockQuantity","schema:rangeIncludes":{"@id":"unece:QuantityType"},"schema:domainIncludes":{"@id":"unece:SupplyChainInventory"},"rdfs:comment":""},{"@id":"unece:plannedStockCalculationDateTime","@type":["rdf:Property","owl:DatatypeProperty"],"rdfs:label":"plannedStockCalculationDateTime","schema:rangeIncludes":{"@id":"schema:Text"},"schema:domainIncludes":{"@id":"unece:SupplyChainInventory"},"rdfs:comment":"The date, time, date time, or other date time value of the planned stock calculation of this supply chain inventory."},{"@id":"unece:plannedStockQuantity","@type":["rdf:Property","owl:ObjectProperty"],"rdfs:label":"plannedStockQuantity","schema:rangeIncludes":{"@id":"unece:QuantityType"},"schema:domainIncludes":{"@id":"unece:SupplyChainInventory"},"rdfs:comment":""},{"@id":"unece:remarkNote","@type":["rdf:Property","owl:ObjectProperty"],"rdfs:label":"remarkNote","schema:rangeIncludes":{"@id":"unece:Note"},"schema:domainIncludes":{"@id":"unece:SupplyChainInventory"},"rdfs:comment":"A textual or coded description, such as a remark or additional information."},{"@id":"unece:stockQuantity","@type":["rdf:Property","owl:ObjectProperty"],"rdfs:label":"stockQuantity","schema:rangeIncludes":{"@id":"unece:QuantityType"},"schema:domainIncludes":{"@id":"unece:SupplyChainInventory"},"rdfs:comment":""},{"@id":"unece:inputObjectInstanceId","@type":["rdf:Property","owl:DatatypeProperty"],"rdfs:label":"inputObjectInstanceId","schema:rangeIncludes":{"@id":"schema:Text"},"schema:domainIncludes":{"@id":"unece:TTTransformationEvent"},"rdfs:comment":"An instance identifier for an input object of this TT transformation event."},{"@id":"unece:inputQuantitySpecifiedEventElement","@type":["rdf:Property","owl:ObjectProperty"],"rdfs:label":"inputQuantitySpecifiedEventElement","schema:rangeIncludes":{"@id":"unece:EventElement"},"schema:domainIncludes":{"@id":"unece:TTTransformationEvent"},"rdfs:comment":"Information about an event in which a Track and Trace (TT) element of one of more physical or digital objects is identified by a specific object class identifier (such as an electronic product class), either a specific quantity or an unspecified quantity."},{"@id":"unece:outputObjectInstanceId","@type":["rdf:Property","owl:DatatypeProperty"],"rdfs:label":"outputObjectInstanceId","schema:rangeIncludes":{"@id":"schema:Text"},"schema:domainIncludes":{"@id":"unece:TTTransformationEvent"},"rdfs:comment":"An instance identifier for an output object of this TT transformation event."},{"@id":"unece:outputQuantitySpecifiedEventElement","@type":["rdf:Property","owl:ObjectProperty"],"rdfs:label":"outputQuantitySpecifiedEventElement","schema:rangeIncludes":{"@id":"unece:EventElement"},"schema:domainIncludes":{"@id":"unece:TTTransformationEvent"},"rdfs:comment":"Information about an event in which a Track and Trace (TT) element of one of more physical or digital objects is identified by a specific object class identifier (such as an electronic product class), either a specific quantity or an unspecified quantity."},{"@id":"unece:relationshipTypeCode","@type":["rdf:Property","owl:DatatypeProperty"],"rdfs:label":"relationshipTypeCode","schema:rangeIncludes":{"@id":"schema:Text"},"schema:domainIncludes":{"@id":"unece:Product"},"rdfs:comment":"A code specifying a type of relationship for this referenced product."},{"@id":"unece:endToEndId","@type":["rdf:Property","owl:DatatypeProperty"],"rdfs:label":"endToEndId","schema:rangeIncludes":{"@id":"schema:Text"},"schema:domainIncludes":{"@id":"unece:TradeSettlementPayment"},"rdfs:comment":"The unique identifier for the end-to-end processing of this trade settlement payment, such as an identifier assigned by an initiating party to unambiguously identify the transaction."},{"@id":"unece:instructionId","@type":["rdf:Property","owl:DatatypeProperty"],"rdfs:label":"instructionId","schema:rangeIncludes":{"@id":"schema:Text"},"schema:domainIncludes":{"@id":"unece:TradeSettlementPayment"},"rdfs:comment":"The unique identifier of the instruction for this trade settlement payment."},{"@id":"unece:requestedExecutionDateTime","@type":["rdf:Property","owl:DatatypeProperty"],"rdfs:label":"requestedExecutionDateTime","schema:rangeIncludes":{"@id":"schema:Text"},"schema:domainIncludes":{"@id":"unece:TradeSettlementPayment"},"rdfs:comment":"The date, time, date time or other date time value of the requested execution of this trade settlement payment."},{"@id":"unece:specifiedPaymentTradeSettlement","@type":["rdf:Property","owl:ObjectProperty"],"rdfs:label":"specifiedPaymentTradeSettlement","schema:rangeIncludes":{"@id":"unece:PaymentTradeSettlement"},"schema:domainIncludes":[{"@id":"unece:TradeSettlementPayment"},{"@id":"unece:TradePrice"},{"@id":"unece:Requirement"}],"rdfs:comment":"The information that enables the reconciliation of a payment with the item(s) that the payment is intended to settle, for example a commercial invoice."},{"@id":"unece:machineType","@type":["rdf:Property","owl:DatatypeProperty"],"rdfs:label":"machineType","schema:rangeIncludes":{"@id":"schema:Text"},"schema:domainIncludes":{"@id":"unece:Machine"},"rdfs:comment":"A type, expressed as text, for this production machine."},{"@id":"unece:operationalApplicableParameter","@type":["rdf:Property","owl:ObjectProperty"],"rdfs:label":"operationalApplicableParameter","schema:rangeIncludes":{"@id":"unece:SpecifiedParameter"},"schema:domainIncludes":{"@id":"unece:Machine"},"rdfs:comment":"A specified feature that is fixed for the case in question but may be different in other cases."},{"@id":"unece:tradeLocationCountryId","@type":["rdf:Property","owl:DatatypeProperty"],"rdfs:label":"tradeLocationCountryId","schema:rangeIncludes":{"@id":"unece:CountryId"},"schema:domainIncludes":{"@id":"unece:TradeLocation"},"rdfs:comment":"The unique identifier of a country location used or referenced in trade."},{"@id":"unece:dateTypeCode","@type":["rdf:Property","owl:DatatypeProperty"],"rdfs:label":"dateTypeCode","schema:rangeIncludes":{"@id":"schema:Text"},"schema:domainIncludes":{"@id":"unece:ForecastTerms"},"rdfs:comment":"A code specifying a type of date in these supply chain forecast terms."},{"@id":"unece:forecastTypeCode","@type":["rdf:Property","owl:DatatypeProperty"],"rdfs:label":"forecastTypeCode","schema:rangeIncludes":{"@id":"schema:Text"},"schema:domainIncludes":{"@id":"unece:ForecastTerms"},"rdfs:comment":"The code specifying the forecast type in these supply chain forecast terms."},{"@id":"unece:supplyChainForecastTermsCommitmentLevelCode","@type":["rdf:Property","owl:DatatypeProperty"],"rdfs:label":"supplyChainForecastTermsCommitmentLevelCode","schema:rangeIncludes":{"@id":"unece:CommitmentLevelCodeList"},"schema:domainIncludes":{"@id":"unece:ForecastTerms"},"rdfs:comment":"A code specifying a commitment level in these supply chain forecast terms."},{"@id":"unece:supplyChainForecastTermsFrequencyCode","@type":["rdf:Property","owl:DatatypeProperty"],"rdfs:label":"supplyChainForecastTermsFrequencyCode","schema:rangeIncludes":{"@id":"schema:Text"},"schema:domainIncludes":{"@id":"unece:ForecastTerms"},"rdfs:comment":"A code specifying a frequency in these supply chain forecast terms."},{"@id":"unece:receiverSpecifiedParty","@type":["rdf:Property","owl:ObjectProperty"],"rdfs:label":"receiverSpecifiedParty","schema:rangeIncludes":{"@id":"unece:TTParty"},"schema:domainIncludes":{"@id":"unece:TTExchangedDocument"},"rdfs:comment":"The receiving party specified for this TT exchanged document."},{"@id":"unece:senderSpecifiedParty","@type":["rdf:Property","owl:ObjectProperty"],"rdfs:label":"senderSpecifiedParty","schema:rangeIncludes":{"@id":"unece:TTParty"},"schema:domainIncludes":{"@id":"unece:TTExchangedDocument"},"rdfs:comment":"The sending party specified for this TT exchanged document."},{"@id":"unece:tTExchangedDocumentPurposeCode","@type":["rdf:Property","owl:DatatypeProperty"],"rdfs:label":"tTExchangedDocumentPurposeCode","schema:rangeIncludes":{"@id":"schema:Text"},"schema:domainIncludes":{"@id":"unece:TTExchangedDocument"},"rdfs:comment":"The code specifying a purpose of this TT exchanged document."},{"@id":"unece:tTExchangedDocumentStatusCode","@type":["rdf:Property","owl:DatatypeProperty"],"rdfs:label":"tTExchangedDocumentStatusCode","schema:rangeIncludes":{"@id":"schema:Text"},"schema:domainIncludes":{"@id":"unece:TTExchangedDocument"},"rdfs:comment":"The code specifying the status of this TT exchanged document."},{"@id":"unece:tTExchangedDocumentTypeCode","@type":["rdf:Property","owl:DatatypeProperty"],"rdfs:label":"tTExchangedDocumentTypeCode","schema:rangeIncludes":{"@id":"schema:Text"},"schema:domainIncludes":{"@id":"unece:TTExchangedDocument"},"rdfs:comment":"The code specifying the type of TT exchanged document."},{"@id":"unece:locationFunctionTypeCode","@type":["rdf:Property","owl:DatatypeProperty"],"rdfs:label":"locationFunctionTypeCode","schema:rangeIncludes":{"@id":"unece:LocationFunctionCodeList"},"schema:domainIncludes":[{"@id":"unece:TTLocation"},{"@id":"unece:CountrySubDivision"},{"@id":"unece:SubordinateLocation"},{"@id":"unece:SubordinateSubordinateLocation"},{"@id":"unece:LogisticsLocation"},{"@id":"unece:TransportServiceLocation"}],"rdfs:comment":"A code specifying the type of this logistics related location."},{"@id":"unece:marketingMeasure","@type":["rdf:Property","owl:ObjectProperty"],"rdfs:label":"marketingMeasure","schema:rangeIncludes":{"@id":"unece:MeasureType"},"schema:domainIncludes":{"@id":"unece:TradeProductFeature"},"rdfs:comment":""},{"@id":"unece:marketingPhrase","@type":["rdf:Property","owl:DatatypeProperty"],"rdfs:label":"marketingPhrase","schema:rangeIncludes":{"@id":"schema:Text"},"schema:domainIncludes":[{"@id":"unece:TradeProductFeature"},{"@id":"unece:SpecifiedFeature"},{"@id":"unece:Source"}],"rdfs:comment":"A catch phrase, expressed as text, for marketing of this trade product feature."},{"@id":"unece:holderResponsibleParty","@type":["rdf:Property","owl:ObjectProperty"],"rdfs:label":"holderResponsibleParty","schema:rangeIncludes":{"@id":"unece:TTParty"},"schema:domainIncludes":{"@id":"unece:TTAnimal"},"rdfs:comment":"The holder responsible party for this TT animal."},{"@id":"unece:speciesTypeCode","@type":["rdf:Property","owl:DatatypeProperty"],"rdfs:label":"speciesTypeCode","schema:rangeIncludes":{"@id":"schema:Text"},"schema:domainIncludes":[{"@id":"unece:TTAnimal"},{"@id":"unece:SpeciesTTAnimal"}],"rdfs:comment":"A code specifying the species type of this TT animal."},{"@id":"unece:specifiedAnimalBatch","@type":["rdf:Property","owl:ObjectProperty"],"rdfs:label":"specifiedAnimalBatch","schema:rangeIncludes":{"@id":"unece:AnimalBatch"},"schema:domainIncludes":{"@id":"unece:TTAnimal"},"rdfs:comment":"A group of animals dealt with together."},{"@id":"unece:specifiedAnimalHoldingEvent","@type":["rdf:Property","owl:ObjectProperty"],"rdfs:label":"specifiedAnimalHoldingEvent","schema:rangeIncludes":{"@id":"unece:AnimalHoldingEvent"},"schema:domainIncludes":[{"@id":"unece:TTAnimal"},{"@id":"unece:TechnicalCharacteristic"}],"rdfs:comment":"The keeping of an animal in a particular location."},{"@id":"unece:specifiedAnimalIdentity","@type":["rdf:Property","owl:ObjectProperty"],"rdfs:label":"specifiedAnimalIdentity","schema:rangeIncludes":{"@id":"unece:AnimalIdentity"},"schema:domainIncludes":{"@id":"unece:TTAnimal"},"rdfs:comment":"Information about an animal which uniquely identifies it."},{"@id":"unece:specifiedIndividualTTAnimal","@type":["rdf:Property","owl:ObjectProperty"],"rdfs:label":"specifiedIndividualTTAnimal","schema:rangeIncludes":{"@id":"unece:IndividualTTAnimal"},"schema:domainIncludes":{"@id":"unece:TTAnimal"},"rdfs:comment":"A Track and Trace (TT) animal, such as one kept or raised on a farm, ranch."},{"@id":"unece:specifiedPeriod","@type":["rdf:Property","owl:ObjectProperty"],"rdfs:label":"specifiedPeriod","schema:rangeIncludes":{"@id":"unece:DelimitedPeriod"},"schema:domainIncludes":[{"@id":"unece:TTAnimal"},{"@id":"unece:CoordinateReferenceSystem"},{"@id":"unece:IndividualTTAnimal"},{"@id":"unece:AnimalBatch"}],"rdfs:comment":"A period of time from a start date time onwards up to an end date time."},{"@id":"unece:specifiedSpeciesTTAnimal","@type":["rdf:Property","owl:ObjectProperty"],"rdfs:label":"specifiedSpeciesTTAnimal","schema:rangeIncludes":{"@id":"unece:SpeciesTTAnimal"},"schema:domainIncludes":{"@id":"unece:TTAnimal"},"rdfs:comment":"The species of a Track and Trace (TT) animal or batch of animals."},{"@id":"unece:orderingAvailablePeriod","@type":["rdf:Property","owl:ObjectProperty"],"rdfs:label":"orderingAvailablePeriod","schema:rangeIncludes":{"@id":"unece:AvailablePeriod"},"schema:domainIncludes":{"@id":"unece:Marketplace"},"rdfs:comment":"A specific period of time such as the length of time between two known date/time points, from a start date onwards, or up to an end date for which something is available."},{"@id":"unece:salesMethodCode","@type":["rdf:Property","owl:DatatypeProperty"],"rdfs:label":"salesMethodCode","schema:rangeIncludes":{"@id":"schema:Text"},"schema:domainIncludes":{"@id":"unece:Marketplace"},"rdfs:comment":"The code specifying a sales method, such as an auction clock or mediation, for this specified marketplace."},{"@id":"unece:virtualIndicator","@type":["rdf:Property","owl:DatatypeProperty"],"rdfs:label":"virtualIndicator","schema:rangeIncludes":{"@id":"schema:Boolean"},"schema:domainIncludes":{"@id":"unece:Marketplace"},"rdfs:comment":"The indication of whether or not this specified marketplace is virtual, such as a web-based marketplace."},{"@id":"unece:websiteURIId","@type":["rdf:Property","owl:DatatypeProperty"],"rdfs:label":"websiteURIId","schema:rangeIncludes":{"@id":"schema:Text"},"schema:domainIncludes":[{"@id":"unece:Marketplace"},{"@id":"unece:InformationSource"},{"@id":"unece:Communication"}],"rdfs:comment":"A website Uniform Resource Identifier (URI) for this specified marketplace."},{"@id":"unece:subordinateProductGroup","@type":["rdf:Property","owl:ObjectProperty"],"rdfs:label":"subordinateProductGroup","schema:rangeIncludes":{"@id":"unece:ProductGroup"},"schema:domainIncludes":{"@id":"unece:ProductGroup"},"rdfs:comment":"A product group subordinate to this trade product group."},{"@id":"unece:manufacturingProcessDescription","@type":["rdf:Property","owl:DatatypeProperty"],"rdfs:label":"manufacturingProcessDescription","schema:rangeIncludes":{"@id":"schema:Text"},"schema:domainIncludes":{"@id":"unece:Production"},"rdfs:comment":"A textual description of the manufacturing process for this goods production."},{"@id":"unece:residenceCountryId","@type":["rdf:Property","owl:DatatypeProperty"],"rdfs:label":"residenceCountryId","schema:rangeIncludes":{"@id":"schema:Text"},"schema:domainIncludes":[{"@id":"unece:TTParty"},{"@id":"unece:GuestPerson"}],"rdfs:comment":"The identifier for the country of residence for this TT party, such as the country in which a person lives or in which a corporation has its place of incorporation."},{"@id":"unece:tTPartyRoleCode","@type":["rdf:Property","owl:DatatypeProperty"],"rdfs:label":"tTPartyRoleCode","schema:rangeIncludes":{"@id":"schema:Text"},"schema:domainIncludes":{"@id":"unece:TTParty"},"rdfs:comment":"A code specifying the role of this TT party."},{"@id":"unece:typeId","@type":["rdf:Property","owl:DatatypeProperty"],"rdfs:label":"typeId","schema:rangeIncludes":{"@id":"schema:Text"},"schema:domainIncludes":[{"@id":"unece:TTParty"},{"@id":"unece:TTTradeTransaction"}],"rdfs:comment":"An identifier of the type for this TT party."},{"@id":"unece:protocolTypeCode","@type":["rdf:Property","owl:DatatypeProperty"],"rdfs:label":"protocolTypeCode","schema:rangeIncludes":{"@id":"schema:Text"},"schema:domainIncludes":{"@id":"unece:NegotiationExchange"},"rdfs:comment":"The code specifying the type of the protocol for this electronic negotiation exchange, such as Alternating Offer Protocol, Continuous Offer Protocol, Withdrawable Alternating Offer Protocol, Withdrawable Continuous Offer Protocol."},{"@id":"unece:responseDueDateTime","@type":["rdf:Property","owl:DatatypeProperty"],"rdfs:label":"responseDueDateTime","schema:rangeIncludes":{"@id":"schema:Text"},"schema:domainIncludes":{"@id":"unece:NegotiationExchange"},"rdfs:comment":"The date or date time value when the response is due for this electronic negotiation exchange."},{"@id":"unece:sessionId","@type":["rdf:Property","owl:DatatypeProperty"],"rdfs:label":"sessionId","schema:rangeIncludes":{"@id":"schema:Text"},"schema:domainIncludes":{"@id":"unece:NegotiationExchange"},"rdfs:comment":"The identifier of the session for this electronic negotiation exchange."},{"@id":"unece:specifiedContext","@type":["rdf:Property","owl:ObjectProperty"],"rdfs:label":"specifiedContext","schema:rangeIncludes":{"@id":"unece:NegotiationContext"},"schema:domainIncludes":{"@id":"unece:NegotiationExchange"},"rdfs:comment":"A context specified for this electronic negotiation exchange."},{"@id":"unece:specifiedIssue","@type":["rdf:Property","owl:ObjectProperty"],"rdfs:label":"specifiedIssue","schema:rangeIncludes":{"@id":"unece:Issue"},"schema:domainIncludes":{"@id":"unece:NegotiationExchange"},"rdfs:comment":"A targeted topic for debate or resolution."},{"@id":"unece:scopeCode","@type":["rdf:Property","owl:DatatypeProperty"],"rdfs:label":"scopeCode","schema:rangeIncludes":{"@id":"schema:Text"},"schema:domainIncludes":{"@id":"unece:DeliverySchedule"},"rdfs:comment":"The code indicating the scope of a forecast delivery schedule."},{"@id":"unece:specifiedTradeLineItem","@type":["rdf:Property","owl:ObjectProperty"],"rdfs:label":"specifiedTradeLineItem","schema:rangeIncludes":{"@id":"unece:SupplyChainTradeLineItem"},"schema:domainIncludes":{"@id":"unece:DeliverySchedule"},"rdfs:comment":"A trade line item specified for this forecast delivery schedule."},{"@id":"unece:additionalStatementNote","@type":["rdf:Property","owl:ObjectProperty"],"rdfs:label":"additionalStatementNote","schema:rangeIncludes":{"@id":"unece:Note"},"schema:domainIncludes":{"@id":"unece:ExchangedDeclaration"},"rdfs:comment":"A textual or coded description, such as a remark or additional information."},{"@id":"unece:applicableCustomsValuation","@type":["rdf:Property","owl:ObjectProperty"],"rdfs:label":"applicableCustomsValuation","schema:rangeIncludes":{"@id":"unece:CustomsValuation"},"schema:domainIncludes":[{"@id":"unece:ExchangedDeclaration"},{"@id":"unece:Consignment"},{"@id":"unece:ConsignmentItem"}],"rdfs:comment":"A cross-border trade related assessment of the worth of an object, such as its monetary value, for customs purposes."},{"@id":"unece:currencyExchangeRate","@type":["rdf:Property","owl:DatatypeProperty"],"rdfs:label":"currencyExchangeRate","schema:rangeIncludes":{"@id":"schema:Text"},"schema:domainIncludes":{"@id":"unece:ExchangedDeclaration"},"rdfs:comment":"The rate of currency exchange in this exchanged declaration."},{"@id":"unece:customsValueSpecifiedAmount","@type":["rdf:Property","owl:ObjectProperty"],"rdfs:label":"customsValueSpecifiedAmount","schema:rangeIncludes":{"@id":"unece:AmountType"},"schema:domainIncludes":{"@id":"unece:ExchangedDeclaration"},"rdfs:comment":""},{"@id":"unece:declarantAgentParty","@type":["rdf:Property","owl:ObjectProperty"],"rdfs:label":"declarantAgentParty","schema:rangeIncludes":{"@id":"unece:TradeParty"},"schema:domainIncludes":{"@id":"unece:ExchangedDeclaration"},"rdfs:comment":"The trade party acting as an agent for the declarant for this exchanged declaration."},{"@id":"unece:declarantParty","@type":["rdf:Property","owl:ObjectProperty"],"rdfs:label":"declarantParty","schema:rangeIncludes":{"@id":"unece:TradeParty"},"schema:domainIncludes":{"@id":"unece:ExchangedDeclaration"},"rdfs:comment":"The trade party acting as the declarant for this exchanged declaration."},{"@id":"unece:grossWeightSpecifiedMeasure","@type":["rdf:Property","owl:ObjectProperty"],"rdfs:label":"grossWeightSpecifiedMeasure","schema:rangeIncludes":{"@id":"unece:WeightUnitMeasureType"},"schema:domainIncludes":{"@id":"unece:ExchangedDeclaration"},"rdfs:comment":""},{"@id":"unece:jurisdictionEntryDateTime","@type":["rdf:Property","owl:DatatypeProperty"],"rdfs:label":"jurisdictionEntryDateTime","schema:rangeIncludes":{"@id":"schema:DateTime"},"schema:domainIncludes":{"@id":"unece:ExchangedDeclaration"},"rdfs:comment":"The date, time, date time or other date time value when the items which are a subject of this exchanged declaration enter a jurisdiction, such as the actual date of arrival of a means of transport."},{"@id":"unece:previousDocument","@type":["rdf:Property","owl:ObjectProperty"],"rdfs:label":"previousDocument","schema:rangeIncludes":{"@id":"unece:Document"},"schema:domainIncludes":[{"@id":"unece:ExchangedDeclaration"},{"@id":"unece:RegulatoryProcedure"}],"rdfs:comment":"Written, printed or electronic matter that is referenced."},{"@id":"unece:principalAssociatedParty","@type":["rdf:Property","owl:ObjectProperty"],"rdfs:label":"principalAssociatedParty","schema:rangeIncludes":{"@id":"unece:TradeParty"},"schema:domainIncludes":{"@id":"unece:ExchangedDeclaration"},"rdfs:comment":"A principal trade party associated with this exchanged declaration."},{"@id":"unece:procedureCode","@type":["rdf:Property","owl:DatatypeProperty"],"rdfs:label":"procedureCode","schema:rangeIncludes":{"@id":"schema:Text"},"schema:domainIncludes":{"@id":"unece:ExchangedDeclaration"},"rdfs:comment":"A code specifying a procedure for this exchanged declaration."},{"@id":"unece:specificCircumstanceCode","@type":["rdf:Property","owl:DatatypeProperty"],"rdfs:label":"specificCircumstanceCode","schema:rangeIncludes":{"@id":"schema:Text"},"schema:domainIncludes":{"@id":"unece:ExchangedDeclaration"},"rdfs:comment":"The code specifying a specific circumstance in this exchanged declaration."},{"@id":"unece:statisticalValueSpecifiedAmount","@type":["rdf:Property","owl:ObjectProperty"],"rdfs:label":"statisticalValueSpecifiedAmount","schema:rangeIncludes":{"@id":"unece:AmountType"},"schema:domainIncludes":{"@id":"unece:ExchangedDeclaration"},"rdfs:comment":""},{"@id":"unece:submissionLocation","@type":["rdf:Property","owl:ObjectProperty"],"rdfs:label":"submissionLocation","schema:rangeIncludes":{"@id":"unece:LogisticsLocation"},"schema:domainIncludes":{"@id":"unece:ExchangedDeclaration"},"rdfs:comment":"A logistics related physical location or place."},{"@id":"unece:totalInvoiceSpecifiedAmount","@type":["rdf:Property","owl:ObjectProperty"],"rdfs:label":"totalInvoiceSpecifiedAmount","schema:rangeIncludes":{"@id":"unece:AmountType"},"schema:domainIncludes":{"@id":"unece:ExchangedDeclaration"},"rdfs:comment":""},{"@id":"unece:totalPackageSpecifiedQuantity","@type":["rdf:Property","owl:ObjectProperty"],"rdfs:label":"totalPackageSpecifiedQuantity","schema:rangeIncludes":{"@id":"unece:QuantityType"},"schema:domainIncludes":{"@id":"unece:ExchangedDeclaration"},"rdfs:comment":""},{"@id":"unece:versionId","@type":["rdf:Property","owl:DatatypeProperty"],"rdfs:label":"versionId","schema:rangeIncludes":{"@id":"schema:Text"},"schema:domainIncludes":[{"@id":"unece:ExchangedDeclaration"},{"@id":"unece:Document"},{"@id":"unece:ExchangedDocument"},{"@id":"unece:BinaryFile"},{"@id":"unece:SpecialQuery"},{"@id":"unece:Standard"},{"@id":"unece:GovernmentRegistration"},{"@id":"unece:CalibratedMeasurement"}],"rdfs:comment":"The identifier for the version of this exchanged declaration."},{"@id":"unece:classCharacteristic","@type":["rdf:Property","owl:ObjectProperty"],"rdfs:label":"classCharacteristic","schema:rangeIncludes":{"@id":"unece:ProductCharacteristic"},"schema:domainIncludes":{"@id":"unece:Classification"},"rdfs:comment":"A prominent attribute or aspect of a product."},{"@id":"unece:classCode","@type":["rdf:Property","owl:DatatypeProperty"],"rdfs:label":"classCode","schema:rangeIncludes":{"@id":"schema:Text"},"schema:domainIncludes":{"@id":"unece:Classification"},"rdfs:comment":"The code specifying the class for this product classification."},{"@id":"unece:classContentTypeDescription","@type":["rdf:Property","owl:DatatypeProperty"],"rdfs:label":"classContentTypeDescription","schema:rangeIncludes":{"@id":"schema:Text"},"schema:domainIncludes":{"@id":"unece:Classification"},"rdfs:comment":"The textual description for the class content type of this product classification."},{"@id":"unece:classContentTypeDescriptionCode","@type":["rdf:Property","owl:DatatypeProperty"],"rdfs:label":"classContentTypeDescriptionCode","schema:rangeIncludes":{"@id":"schema:Text"},"schema:domainIncludes":{"@id":"unece:Classification"},"rdfs:comment":"The code specifying the description of the class content type of this product classification."},{"@id":"unece:className","@type":["rdf:Property","owl:DatatypeProperty"],"rdfs:label":"className","schema:rangeIncludes":{"@id":"schema:Text"},"schema:domainIncludes":[{"@id":"unece:Classification"},{"@id":"unece:FieldCrop"}],"rdfs:comment":"A class name, expressed as text, for this product classification."},{"@id":"unece:subClassCode","@type":["rdf:Property","owl:DatatypeProperty"],"rdfs:label":"subClassCode","schema:rangeIncludes":{"@id":"schema:Text"},"schema:domainIncludes":{"@id":"unece:Classification"},"rdfs:comment":"The code specifying the sub class for this product classification."},{"@id":"unece:systemId","@type":["rdf:Property","owl:DatatypeProperty"],"rdfs:label":"systemId","schema:rangeIncludes":{"@id":"schema:Text"},"schema:domainIncludes":[{"@id":"unece:Classification"},{"@id":"unece:GeographicalCoordinate"}],"rdfs:comment":"The unique identifier of the classification system for this product classification."},{"@id":"unece:systemName","@type":["rdf:Property","owl:DatatypeProperty"],"rdfs:label":"systemName","schema:rangeIncludes":{"@id":"schema:Text"},"schema:domainIncludes":{"@id":"unece:Classification"},"rdfs:comment":"A name, expressed as text, of the classification system for this product classification."},{"@id":"unece:buyerAssignedCategoryCode","@type":["rdf:Property","owl:DatatypeProperty"],"rdfs:label":"buyerAssignedCategoryCode","schema:rangeIncludes":{"@id":"schema:Text"},"schema:domainIncludes":{"@id":"unece:DocumentLineDocument"},"rdfs:comment":"The code specifying the category assigned by the buyer for this document line."},{"@id":"unece:documentLineStatusCode","@type":["rdf:Property","owl:DatatypeProperty"],"rdfs:label":"documentLineStatusCode","schema:rangeIncludes":{"@id":"unece:LineStatusCodeList"},"schema:domainIncludes":{"@id":"unece:DocumentLineDocument"},"rdfs:comment":"The code specifying the status of this document line."},{"@id":"unece:effectiveSpecifiedPeriod","@type":["rdf:Property","owl:ObjectProperty"],"rdfs:label":"effectiveSpecifiedPeriod","schema:rangeIncludes":{"@id":"unece:SpecifiedPeriod"},"schema:domainIncludes":[{"@id":"unece:DocumentLineDocument"},{"@id":"unece:Document"},{"@id":"unece:ExchangedDocument"},{"@id":"unece:Service"}],"rdfs:comment":"A specified period of time."},{"@id":"unece:latestRevisionDateTime","@type":["rdf:Property","owl:DatatypeProperty"],"rdfs:label":"latestRevisionDateTime","schema:rangeIncludes":{"@id":"schema:Text"},"schema:domainIncludes":{"@id":"unece:DocumentLineDocument"},"rdfs:comment":"The date, time, date time, or other date time value for the latest revision of this document line."},{"@id":"unece:lineId","@type":["rdf:Property","owl:DatatypeProperty"],"rdfs:label":"lineId","schema:rangeIncludes":{"@id":"schema:Text"},"schema:domainIncludes":[{"@id":"unece:DocumentLineDocument"},{"@id":"unece:Document"}],"rdfs:comment":"The unique identifier of a line in this referenced document."},{"@id":"unece:lineStatusReason","@type":["rdf:Property","owl:DatatypeProperty"],"rdfs:label":"lineStatusReason","schema:rangeIncludes":{"@id":"schema:Text"},"schema:domainIncludes":{"@id":"unece:DocumentLineDocument"},"rdfs:comment":"A reason, expressed as text, for the line status in this document line."},{"@id":"unece:lineStatusReasonCode","@type":["rdf:Property","owl:DatatypeProperty"],"rdfs:label":"lineStatusReasonCode","schema:rangeIncludes":{"@id":"schema:Text"},"schema:domainIncludes":{"@id":"unece:DocumentLineDocument"},"rdfs:comment":"The code specifying the line status reason for this document line."},{"@id":"unece:parentLineId","@type":["rdf:Property","owl:DatatypeProperty"],"rdfs:label":"parentLineId","schema:rangeIncludes":{"@id":"schema:Text"},"schema:domainIncludes":{"@id":"unece:DocumentLineDocument"},"rdfs:comment":"The unique identifier of the parent line to this document line."},{"@id":"unece:publicationDateTime","@type":["rdf:Property","owl:DatatypeProperty"],"rdfs:label":"publicationDateTime","schema:rangeIncludes":{"@id":"schema:Text"},"schema:domainIncludes":{"@id":"unece:DocumentLineDocument"},"rdfs:comment":"The date, time, date time, or other date time value of the publication of this document line."},{"@id":"unece:referenceAcknowledgementDocument","@type":["rdf:Property","owl:ObjectProperty"],"rdfs:label":"referenceAcknowledgementDocument","schema:rangeIncludes":{"@id":"unece:AcknowledgementDocument"},"schema:domainIncludes":{"@id":"unece:DocumentLineDocument"},"rdfs:comment":"The acknowledgement document referenced in this document line."},{"@id":"unece:subordinateLineId","@type":["rdf:Property","owl:DatatypeProperty"],"rdfs:label":"subordinateLineId","schema:rangeIncludes":{"@id":"schema:Text"},"schema:domainIncludes":[{"@id":"unece:DocumentLineDocument"},{"@id":"unece:Document"}],"rdfs:comment":"An identifier of a subordinate line of this document line."},{"@id":"unece:uUIDLineId","@type":["rdf:Property","owl:DatatypeProperty"],"rdfs:label":"uUIDLineId","schema:rangeIncludes":{"@id":"schema:Text"},"schema:domainIncludes":{"@id":"unece:DocumentLineDocument"},"rdfs:comment":"The universally unique identifier (UUID) of this document line."},{"@id":"unece:abstract","@type":["rdf:Property","owl:DatatypeProperty"],"rdfs:label":"abstract","schema:rangeIncludes":{"@id":"schema:Text"},"schema:domainIncludes":{"@id":"unece:ComplexDescription"},"rdfs:comment":"A textual abstract of the content of the work item complex description."},{"@id":"unece:content","@type":["rdf:Property","owl:DatatypeProperty"],"rdfs:label":"content","schema:rangeIncludes":{"@id":"schema:Text"},"schema:domainIncludes":[{"@id":"unece:ComplexDescription"},{"@id":"unece:InformationSource"},{"@id":"unece:Note"},{"@id":"unece:Response"},{"@id":"unece:SpecialQuery"},{"@id":"unece:SpecifiedNote"},{"@id":"unece:Clause"},{"@id":"unece:SpecificationQuery"},{"@id":"unece:InspectionNote"},{"@id":"unece:LaboratoryObservationNote"},{"@id":"unece:Marking"}],"rdfs:comment":"A content, expressed as text, of this note."},{"@id":"unece:contractualLanguageCode","@type":["rdf:Property","owl:DatatypeProperty"],"rdfs:label":"contractualLanguageCode","schema:rangeIncludes":{"@id":"schema:Text"},"schema:domainIncludes":[{"@id":"unece:ComplexDescription"},{"@id":"unece:QuantityAnalysis"},{"@id":"unece:WorkItemDimension"},{"@id":"unece:Response"},{"@id":"unece:SpecificationQuery"},{"@id":"unece:BreakdownStatement"},{"@id":"unece:BasicWorkItem"},{"@id":"unece:GroupedWorkItem"}],"rdfs:comment":"The code specifying the contractual language for this basic work item."},{"@id":"unece:requestingQuery","@type":["rdf:Property","owl:ObjectProperty"],"rdfs:label":"requestingQuery","schema:rangeIncludes":{"@id":"unece:SpecificationQuery"},"schema:domainIncludes":{"@id":"unece:ComplexDescription"},"rdfs:comment":"A requesting specification query for this work item complex description."},{"@id":"unece:respondingResponse","@type":["rdf:Property","owl:ObjectProperty"],"rdfs:label":"respondingResponse","schema:rangeIncludes":{"@id":"unece:Response"},"schema:domainIncludes":{"@id":"unece:ComplexDescription"},"rdfs:comment":"A responding specification response for this work item complex description."},{"@id":"unece:subsetComplexDescription","@type":["rdf:Property","owl:ObjectProperty"],"rdfs:label":"subsetComplexDescription","schema:rangeIncludes":{"@id":"unece:ComplexDescription"},"schema:domainIncludes":{"@id":"unece:ComplexDescription"},"rdfs:comment":"The complex description subset for this work item complex description."},{"@id":"unece:acceptablePeriod","@type":["rdf:Property","owl:ObjectProperty"],"rdfs:label":"acceptablePeriod","schema:rangeIncludes":{"@id":"unece:SpecifiedPeriod"},"schema:domainIncludes":{"@id":"unece:Document"},"rdfs:comment":"The specified period within which this referenced document may be accepted."},{"@id":"unece:acceptanceDateTime","@type":["rdf:Property","owl:DatatypeProperty"],"rdfs:label":"acceptanceDateTime","schema:rangeIncludes":{"@id":"schema:Text"},"schema:domainIncludes":[{"@id":"unece:Document"},{"@id":"unece:ExchangedDocument"}],"rdfs:comment":"The date, time, date time, or other date time value for the acceptance of this exchanged document."},{"@id":"unece:attachedBinaryFile","@type":["rdf:Property","owl:ObjectProperty"],"rdfs:label":"attachedBinaryFile","schema:rangeIncludes":{"@id":"unece:BinaryFile"},"schema:domainIncludes":[{"@id":"unece:Document"},{"@id":"unece:ExchangedDocument"},{"@id":"unece:Picture"},{"@id":"unece:OrganizationalCertificate"},{"@id":"unece:ProcessCertificate"},{"@id":"unece:ProductBatchCertificate"},{"@id":"unece:ProductCertificate"},{"@id":"unece:SpecifiedCertificate"},{"@id":"unece:Standard"},{"@id":"unece:InspectionResult"},{"@id":"unece:SustainabilityInspection"},{"@id":"unece:SpecifiedInspection"},{"@id":"unece:AgriculturalCertificate"}],"rdfs:comment":"A binary file attached for this sustainability inspection."},{"@id":"unece:attachmentBinaryObject","@type":["rdf:Property","owl:DatatypeProperty"],"rdfs:label":"attachmentBinaryObject","schema:rangeIncludes":{"@id":"schema:Text"},"schema:domainIncludes":{"@id":"unece:Document"},"rdfs:comment":"A binary object that is attached or otherwise appended to this referenced document."},{"@id":"unece:authenticatedOriginalIndicator","@type":["rdf:Property","owl:DatatypeProperty"],"rdfs:label":"authenticatedOriginalIndicator","schema:rangeIncludes":{"@id":"schema:Boolean"},"schema:domainIncludes":{"@id":"unece:Document"},"rdfs:comment":"The indication of whether or not this referenced document is an authenticated original."},{"@id":"unece:contractualClause","@type":["rdf:Property","owl:ObjectProperty"],"rdfs:label":"contractualClause","schema:rangeIncludes":{"@id":"unece:Clause"},"schema:domainIncludes":[{"@id":"unece:Document"},{"@id":"unece:ExchangedDocument"},{"@id":"unece:FinancingRequestDocument"}],"rdfs:comment":"A contractual clause of this exchanged document."},{"@id":"unece:copyIndicator","@type":["rdf:Property","owl:DatatypeProperty"],"rdfs:label":"copyIndicator","schema:rangeIncludes":{"@id":"schema:Boolean"},"schema:domainIncludes":[{"@id":"unece:Document"},{"@id":"unece:ExchangedDocument"},{"@id":"unece:FinancingRequestDocument"}],"rdfs:comment":"The indication of whether or not the referenced document is a copy."},{"@id":"unece:documentLanguageId","@type":["rdf:Property","owl:DatatypeProperty"],"rdfs:label":"documentLanguageId","schema:rangeIncludes":{"@id":"unece:LanguageId"},"schema:domainIncludes":{"@id":"unece:Document"},"rdfs:comment":"An identifier for a language used in this referenced document."},{"@id":"unece:documentStatusCode","@type":["rdf:Property","owl:DatatypeProperty"],"rdfs:label":"documentStatusCode","schema:rangeIncludes":{"@id":"unece:DocumentStatusCodeList"},"schema:domainIncludes":[{"@id":"unece:Document"},{"@id":"unece:ExchangedDocument"}],"rdfs:comment":"The code specifying the status for this referenced document."},{"@id":"unece:documentType","@type":["rdf:Property","owl:DatatypeProperty"],"rdfs:label":"documentType","schema:rangeIncludes":{"@id":"schema:Text"},"schema:domainIncludes":{"@id":"unece:Document"},"rdfs:comment":"A type, expressed as text, for this referenced document."},{"@id":"unece:electronicPresentationIndicator","@type":["rdf:Property","owl:DatatypeProperty"],"rdfs:label":"electronicPresentationIndicator","schema:rangeIncludes":{"@id":"schema:Boolean"},"schema:domainIncludes":[{"@id":"unece:Document"},{"@id":"unece:ExchangedDocument"}],"rdfs:comment":"The indication of whether or not this exchanged document is presented in an electronic format."},{"@id":"unece:includedAmount","@type":["rdf:Property","owl:ObjectProperty"],"rdfs:label":"includedAmount","schema:rangeIncludes":{"@id":"unece:AmountType"},"schema:domainIncludes":{"@id":"unece:Document"},"rdfs:comment":"A monetary value included in this referenced document."},{"@id":"unece:issueLocation","@type":["rdf:Property","owl:ObjectProperty"],"rdfs:label":"issueLocation","schema:rangeIncludes":{"@id":"unece:Location"},"schema:domainIncludes":[{"@id":"unece:Document"},{"@id":"unece:ExchangedDocument"},{"@id":"unece:Authentication"}],"rdfs:comment":"The issue location for this document authentication."},{"@id":"unece:issuerAssignedId","@type":["rdf:Property","owl:DatatypeProperty"],"rdfs:label":"issuerAssignedId","schema:rangeIncludes":{"@id":"schema:Text"},"schema:domainIncludes":{"@id":"unece:Document"},"rdfs:comment":"The unique issuer assigned identifier for this referenced document."},{"@id":"unece:issuerParty","@type":["rdf:Property","owl:ObjectProperty"],"rdfs:label":"issuerParty","schema:rangeIncludes":{"@id":"unece:Party"},"schema:domainIncludes":[{"@id":"unece:Document"},{"@id":"unece:ExchangedDocument"},{"@id":"unece:SpecifiedCertificate"},{"@id":"unece:Licence"},{"@id":"unece:SpecifiedDeclaration"}],"rdfs:comment":"A party that issues this specified declaration."},{"@id":"unece:issuerSpecifiedInstructions","@type":["rdf:Property","owl:ObjectProperty"],"rdfs:label":"issuerSpecifiedInstructions","schema:rangeIncludes":{"@id":"unece:DocumentHandlingInstructions"},"schema:domainIncludes":{"@id":"unece:Document"},"rdfs:comment":"Handling instructions specified by the issuer for this referenced document."},{"@id":"unece:lodgementLocation","@type":["rdf:Property","owl:ObjectProperty"],"rdfs:label":"lodgementLocation","schema:rangeIncludes":{"@id":"unece:Location"},"schema:domainIncludes":[{"@id":"unece:Document"},{"@id":"unece:ExchangedDocument"}],"rdfs:comment":"The location where this exchanged document has been lodged."},{"@id":"unece:pageId","@type":["rdf:Property","owl:DatatypeProperty"],"rdfs:label":"pageId","schema:rangeIncludes":{"@id":"schema:Text"},"schema:domainIncludes":{"@id":"unece:Document"},"rdfs:comment":"The identifier of the page for this referenced document."},{"@id":"unece:previousRevisionId","@type":["rdf:Property","owl:DatatypeProperty"],"rdfs:label":"previousRevisionId","schema:rangeIncludes":{"@id":"schema:Text"},"schema:domainIncludes":[{"@id":"unece:Document"},{"@id":"unece:ExchangedDocument"}],"rdfs:comment":"An identifier for a previous revision of this referenced document."},{"@id":"unece:proprietaryType","@type":["rdf:Property","owl:DatatypeProperty"],"rdfs:label":"proprietaryType","schema:rangeIncludes":{"@id":"schema:Text"},"schema:domainIncludes":[{"@id":"unece:Document"},{"@id":"unece:CreditorFinancialAccount"},{"@id":"unece:DebtorFinancialAccount"},{"@id":"unece:FinancingFinancialAccount"}],"rdfs:comment":"A proprietary type, expressed as text, for this referenced document."},{"@id":"unece:receiptDateTime","@type":["rdf:Property","owl:DatatypeProperty"],"rdfs:label":"receiptDateTime","schema:rangeIncludes":{"@id":"schema:Text"},"schema:domainIncludes":[{"@id":"unece:Document"},{"@id":"unece:PaymentTradeSettlement"}],"rdfs:comment":"The date, time, date time, or other date time value for the formal receipt of this referenced document."},{"@id":"unece:recipientTradeParty","@type":["rdf:Property","owl:ObjectProperty"],"rdfs:label":"recipientTradeParty","schema:rangeIncludes":{"@id":"unece:Party"},"schema:domainIncludes":[{"@id":"unece:Document"},{"@id":"unece:ExchangedDocument"}],"rdfs:comment":"A trade party that receives this exchanged document."},{"@id":"unece:referenceDateTime","@type":["rdf:Property","owl:DatatypeProperty"],"rdfs:label":"referenceDateTime","schema:rangeIncludes":{"@id":"schema:Text"},"schema:domainIncludes":[{"@id":"unece:Document"},{"@id":"unece:DocumentStatus"},{"@id":"unece:LogisticsStatus"}],"rdfs:comment":"The reference date or date time for this referenced document."},{"@id":"unece:referenceRelationshipTypeCode","@type":["rdf:Property","owl:DatatypeProperty"],"rdfs:label":"referenceRelationshipTypeCode","schema:rangeIncludes":{"@id":"unece:ReferenceCodeList"},"schema:domainIncludes":{"@id":"unece:Document"},"rdfs:comment":"The code specifying the type of relationship between this referenced document and another artefact, such as a replacement of an original document."},{"@id":"unece:referenceTypeCode","@type":["rdf:Property","owl:DatatypeProperty"],"rdfs:label":"referenceTypeCode","schema:rangeIncludes":{"@id":"unece:ReferenceCodeList"},"schema:domainIncludes":[{"@id":"unece:Document"},{"@id":"unece:Location"}],"rdfs:comment":"The code specifying the reference type of this referenced document."},{"@id":"unece:remarks","@type":["rdf:Property","owl:DatatypeProperty"],"rdfs:label":"remarks","schema:rangeIncludes":{"@id":"schema:Text"},"schema:domainIncludes":[{"@id":"unece:Document"},{"@id":"unece:ExchangedDocument"}],"rdfs:comment":"A remark, expressed as text, regarding this exchanged document."},{"@id":"unece:sectionName","@type":["rdf:Property","owl:DatatypeProperty"],"rdfs:label":"sectionName","schema:rangeIncludes":{"@id":"schema:Text"},"schema:domainIncludes":{"@id":"unece:Document"},"rdfs:comment":"A section name, expressed as text, for this referenced document."},{"@id":"unece:senderTradeParty","@type":["rdf:Property","owl:ObjectProperty"],"rdfs:label":"senderTradeParty","schema:rangeIncludes":{"@id":"unece:Party"},"schema:domainIncludes":[{"@id":"unece:Document"},{"@id":"unece:ExchangedDocument"}],"rdfs:comment":"The party that sends this exchanged document."},{"@id":"unece:signatoryAuthentication","@type":["rdf:Property","owl:ObjectProperty"],"rdfs:label":"signatoryAuthentication","schema:rangeIncludes":{"@id":"unece:Authentication"},"schema:domainIncludes":[{"@id":"unece:Document"},{"@id":"unece:ExchangedDocument"}],"rdfs:comment":"A signatory authentication for this referenced document."},{"@id":"unece:specifiedDocumentStatus","@type":["rdf:Property","owl:ObjectProperty"],"rdfs:label":"specifiedDocumentStatus","schema:rangeIncludes":{"@id":"unece:DocumentStatus"},"schema:domainIncludes":{"@id":"unece:Document"},"rdfs:comment":"Status information specified for this referenced document."},{"@id":"unece:subtypeCode","@type":["rdf:Property","owl:DatatypeProperty"],"rdfs:label":"subtypeCode","schema:rangeIncludes":{"@id":"schema:Text"},"schema:domainIncludes":[{"@id":"unece:Document"},{"@id":"unece:ExchangedDocument"}],"rdfs:comment":"A code specifying a subtype of this referenced document."},{"@id":"unece:totalIssueCountNumeric","@type":["rdf:Property","owl:DatatypeProperty"],"rdfs:label":"totalIssueCountNumeric","schema:rangeIncludes":{"@id":"schema:Text"},"schema:domainIncludes":{"@id":"unece:Document"},"rdfs:comment":"The total issue count for this referenced document."},{"@id":"unece:validityPeriod","@type":["rdf:Property","owl:ObjectProperty"],"rdfs:label":"validityPeriod","schema:rangeIncludes":{"@id":"unece:SpecifiedPeriod"},"schema:domainIncludes":[{"@id":"unece:Document"},{"@id":"unece:BinaryFile"},{"@id":"unece:DocumentStatus"},{"@id":"unece:TradePrice"},{"@id":"unece:GovernmentRegistration"},{"@id":"unece:LogisticsStatus"}],"rdfs:comment":"A period of validity specified for this referenced document."},{"@id":"unece:agentParty","@type":["rdf:Property","owl:ObjectProperty"],"rdfs:label":"agentParty","schema:rangeIncludes":{"@id":"unece:Party"},"schema:domainIncludes":{"@id":"unece:ExchangedDocument"},"rdfs:comment":"A party representing another party for this exchanged document."},{"@id":"unece:amendmentPurpose","@type":["rdf:Property","owl:DatatypeProperty"],"rdfs:label":"amendmentPurpose","schema:rangeIncludes":{"@id":"schema:Text"},"schema:domainIncludes":{"@id":"unece:ExchangedDocument"},"rdfs:comment":"An amendment purpose, expressed in text, for this exchanged document."},{"@id":"unece:approverSignatoryAuthentication","@type":["rdf:Property","owl:ObjectProperty"],"rdfs:label":"approverSignatoryAuthentication","schema:rangeIncludes":{"@id":"unece:Authentication"},"schema:domainIncludes":{"@id":"unece:ExchangedDocument"},"rdfs:comment":"The approver signature that authenticates this exchanged document."},{"@id":"unece:buyerSignatoryAuthentication","@type":["rdf:Property","owl:ObjectProperty"],"rdfs:label":"buyerSignatoryAuthentication","schema:rangeIncludes":{"@id":"unece:Authentication"},"schema:domainIncludes":{"@id":"unece:ExchangedDocument"},"rdfs:comment":"The buyer signature that authenticates this exchanged document."},{"@id":"unece:cancellationDateTime","@type":["rdf:Property","owl:DatatypeProperty"],"rdfs:label":"cancellationDateTime","schema:rangeIncludes":{"@id":"schema:Text"},"schema:domainIncludes":{"@id":"unece:ExchangedDocument"},"rdfs:comment":"The date, time, date time, or other date time value of a cancellation of the exchanged document."},{"@id":"unece:copyIssuedQuantity","@type":["rdf:Property","owl:ObjectProperty"],"rdfs:label":"copyIssuedQuantity","schema:rangeIncludes":{"@id":"unece:QuantityType"},"schema:domainIncludes":{"@id":"unece:ExchangedDocument"},"rdfs:comment":"The number of copies issued of this exchanged document."},{"@id":"unece:copyRequiredQuantity","@type":["rdf:Property","owl:ObjectProperty"],"rdfs:label":"copyRequiredQuantity","schema:rangeIncludes":{"@id":"unece:QuantityType"},"schema:domainIncludes":{"@id":"unece:ExchangedDocument"},"rdfs:comment":"The number of copies required of this exchanged document."},{"@id":"unece:customsId","@type":["rdf:Property","owl:DatatypeProperty"],"rdfs:label":"customsId","schema:rangeIncludes":{"@id":"schema:Text"},"schema:domainIncludes":[{"@id":"unece:ExchangedDocument"},{"@id":"unece:Consignment"}],"rdfs:comment":"A unique identifier, for customs purposes, for this consignment."},{"@id":"unece:exchangedDocumentAmendmentPurposeCode","@type":["rdf:Property","owl:DatatypeProperty"],"rdfs:label":"exchangedDocumentAmendmentPurposeCode","schema:rangeIncludes":{"@id":"schema:Text"},"schema:domainIncludes":{"@id":"unece:ExchangedDocument"},"rdfs:comment":"A code specifying a purpose of an amendment to this exchanged document."},{"@id":"unece:exchangedDocumentResponseTypeCode","@type":["rdf:Property","owl:DatatypeProperty"],"rdfs:label":"exchangedDocumentResponseTypeCode","schema:rangeIncludes":{"@id":"unece:ResponseTypeCodeList"},"schema:domainIncludes":{"@id":"unece:ExchangedDocument"},"rdfs:comment":"A code specifying a type of response requested for this exchanged document."},{"@id":"unece:firstSignatoryAuthentication","@type":["rdf:Property","owl:ObjectProperty"],"rdfs:label":"firstSignatoryAuthentication","schema:rangeIncludes":{"@id":"unece:Authentication"},"schema:domainIncludes":{"@id":"unece:ExchangedDocument"},"rdfs:comment":"The first or primary signature that authenticates this exchanged document."},{"@id":"unece:firstVersionIssueDateTime","@type":["rdf:Property","owl:DatatypeProperty"],"rdfs:label":"firstVersionIssueDateTime","schema:rangeIncludes":{"@id":"schema:Text"},"schema:domainIncludes":{"@id":"unece:ExchangedDocument"},"rdfs:comment":"The date, time, date time or other date time value when the first version of this exchanged document was issued."},{"@id":"unece:fourthSignatoryAuthentication","@type":["rdf:Property","owl:ObjectProperty"],"rdfs:label":"fourthSignatoryAuthentication","schema:rangeIncludes":{"@id":"unece:Authentication"},"schema:domainIncludes":{"@id":"unece:ExchangedDocument"},"rdfs:comment":"The fourth signature, also known as the third counter signature, that has been authenticated on this exchanged document indicating where appropriate the authentication party."},{"@id":"unece:languageId","@type":["rdf:Property","owl:DatatypeProperty"],"rdfs:label":"languageId","schema:rangeIncludes":{"@id":"schema:Text"},"schema:domainIncludes":[{"@id":"unece:ExchangedDocument"},{"@id":"unece:GuestPerson"}],"rdfs:comment":"A unique identifier for a language used in this exchanged document."},{"@id":"unece:lineCountNumeric","@type":["rdf:Property","owl:DatatypeProperty"],"rdfs:label":"lineCountNumeric","schema:rangeIncludes":{"@id":"schema:Text"},"schema:domainIncludes":{"@id":"unece:ExchangedDocument"},"rdfs:comment":"The count of the number of lines in this exchanged document."},{"@id":"unece:messageFunctionPurposeCode","@type":["rdf:Property","owl:DatatypeProperty"],"rdfs:label":"messageFunctionPurposeCode","schema:rangeIncludes":{"@id":"unece:MessageFunctionCodeList"},"schema:domainIncludes":{"@id":"unece:ExchangedDocument"},"rdfs:comment":"A code specifying the purpose of this exchanged document, such as request or reminder."},{"@id":"unece:offsetProcessingStatus","@type":["rdf:Property","owl:DatatypeProperty"],"rdfs:label":"offsetProcessingStatus","schema:rangeIncludes":{"@id":"schema:Text"},"schema:domainIncludes":{"@id":"unece:ExchangedDocument"},"rdfs:comment":"A status of an offset processing, expressed as text, for this exchanged document, such as the process offsetted by this document."},{"@id":"unece:originalIssuedQuantity","@type":["rdf:Property","owl:ObjectProperty"],"rdfs:label":"originalIssuedQuantity","schema:rangeIncludes":{"@id":"unece:QuantityType"},"schema:domainIncludes":{"@id":"unece:ExchangedDocument"},"rdfs:comment":"The number of originals issued of this exchanged document."},{"@id":"unece:originalRequiredQuantity","@type":["rdf:Property","owl:ObjectProperty"],"rdfs:label":"originalRequiredQuantity","schema:rangeIncludes":{"@id":"unece:QuantityType"},"schema:domainIncludes":{"@id":"unece:ExchangedDocument"},"rdfs:comment":"The number of originals required of this exchanged document."},{"@id":"unece:purpose","@type":["rdf:Property","owl:DatatypeProperty"],"rdfs:label":"purpose","schema:rangeIncludes":{"@id":"schema:Text"},"schema:domainIncludes":{"@id":"unece:ExchangedDocument"},"rdfs:comment":"The purpose, expressed as text, of this exchanged document."},{"@id":"unece:recipientAssignedId","@type":["rdf:Property","owl:DatatypeProperty"],"rdfs:label":"recipientAssignedId","schema:rangeIncludes":{"@id":"schema:Text"},"schema:domainIncludes":{"@id":"unece:ExchangedDocument"},"rdfs:comment":"A unique recipient assigned identifier for this exchanged document."},{"@id":"unece:rejectionResponseDateTime","@type":["rdf:Property","owl:DatatypeProperty"],"rdfs:label":"rejectionResponseDateTime","schema:rangeIncludes":{"@id":"schema:Text"},"schema:domainIncludes":{"@id":"unece:ExchangedDocument"},"rdfs:comment":"A date, time, date time, or other date time value of a rejection response of the exchanged document."},{"@id":"unece:responseDateTime","@type":["rdf:Property","owl:DatatypeProperty"],"rdfs:label":"responseDateTime","schema:rangeIncludes":{"@id":"schema:Text"},"schema:domainIncludes":[{"@id":"unece:ExchangedDocument"},{"@id":"unece:SpecialQuery"}],"rdfs:comment":"A date, time, date time, or other date time value of a response of the exchanged document."},{"@id":"unece:revisionDateTime","@type":["rdf:Property","owl:DatatypeProperty"],"rdfs:label":"revisionDateTime","schema:rangeIncludes":{"@id":"schema:Text"},"schema:domainIncludes":{"@id":"unece:ExchangedDocument"},"rdfs:comment":"The date, time, date time or other date time value for the revision of this exchanged document."},{"@id":"unece:secondSignatoryAuthentication","@type":["rdf:Property","owl:ObjectProperty"],"rdfs:label":"secondSignatoryAuthentication","schema:rangeIncludes":{"@id":"unece:Authentication"},"schema:domainIncludes":{"@id":"unece:ExchangedDocument"},"rdfs:comment":"The second signature, also known as the first counter signature, that has been authenticated on this exchanged document indicating where appropriate the authentication party."},{"@id":"unece:senderAssignedId","@type":["rdf:Property","owl:DatatypeProperty"],"rdfs:label":"senderAssignedId","schema:rangeIncludes":{"@id":"schema:Text"},"schema:domainIncludes":{"@id":"unece:ExchangedDocument"},"rdfs:comment":"A unique sender assigned identifier for this exchanged document."},{"@id":"unece:submissionDateTime","@type":["rdf:Property","owl:DatatypeProperty"],"rdfs:label":"submissionDateTime","schema:rangeIncludes":{"@id":"schema:Text"},"schema:domainIncludes":{"@id":"unece:ExchangedDocument"},"rdfs:comment":"The date, time, date time or other date time value for the formal submission of this exchanged document to a receiver by a sender."},{"@id":"unece:thirdSignatoryAuthentication","@type":["rdf:Property","owl:ObjectProperty"],"rdfs:label":"thirdSignatoryAuthentication","schema:rangeIncludes":{"@id":"unece:Authentication"},"schema:domainIncludes":{"@id":"unece:ExchangedDocument"},"rdfs:comment":"The third signature, also known as the second counter signature, that has been authenticated on this exchanged document indicating where appropriate the authentication party."},{"@id":"unece:traderAssignedId","@type":["rdf:Property","owl:DatatypeProperty"],"rdfs:label":"traderAssignedId","schema:rangeIncludes":{"@id":"schema:Text"},"schema:domainIncludes":{"@id":"unece:ExchangedDocument"},"rdfs:comment":"A unique trader assigned identifier for this exchanged document."},{"@id":"unece:urgency","@type":["rdf:Property","owl:DatatypeProperty"],"rdfs:label":"urgency","schema:rangeIncludes":{"@id":"schema:Text"},"schema:domainIncludes":{"@id":"unece:ExchangedDocument"},"rdfs:comment":"An urgency, expressed as text, of this exchanged document."},{"@id":"unece:urgencyCode","@type":["rdf:Property","owl:DatatypeProperty"],"rdfs:label":"urgencyCode","schema:rangeIncludes":{"@id":"schema:Text"},"schema:domainIncludes":{"@id":"unece:ExchangedDocument"},"rdfs:comment":"The code specifying the urgency for this exchanged document."},{"@id":"unece:access","@type":["rdf:Property","owl:DatatypeProperty"],"rdfs:label":"access","schema:rangeIncludes":{"@id":"schema:Text"},"schema:domainIncludes":{"@id":"unece:BinaryFile"},"rdfs:comment":"Access information, expressed as text, for this specified binary file, such as security and download parameters."},{"@id":"unece:accessAvailabilityPeriod","@type":["rdf:Property","owl:ObjectProperty"],"rdfs:label":"accessAvailabilityPeriod","schema:rangeIncludes":{"@id":"unece:SpecifiedPeriod"},"schema:domainIncludes":{"@id":"unece:BinaryFile"},"rdfs:comment":"The specified period when access to this binary file is available."},{"@id":"unece:authorName","@type":["rdf:Property","owl:DatatypeProperty"],"rdfs:label":"authorName","schema:rangeIncludes":{"@id":"schema:Text"},"schema:domainIncludes":{"@id":"unece:BinaryFile"},"rdfs:comment":"A name of an author, expressed as text, of this specified binary file."},{"@id":"unece:characterSetCode","@type":["rdf:Property","owl:DatatypeProperty"],"rdfs:label":"characterSetCode","schema:rangeIncludes":{"@id":"schema:Text"},"schema:domainIncludes":{"@id":"unece:BinaryFile"},"rdfs:comment":"The code specifying the character set for this specified binary file."},{"@id":"unece:encodingCode","@type":["rdf:Property","owl:DatatypeProperty"],"rdfs:label":"encodingCode","schema:rangeIncludes":{"@id":"schema:Text"},"schema:domainIncludes":{"@id":"unece:BinaryFile"},"rdfs:comment":"The code specifying the encoding of this specified binary file."},{"@id":"unece:fileName","@type":["rdf:Property","owl:DatatypeProperty"],"rdfs:label":"fileName","schema:rangeIncludes":{"@id":"schema:Text"},"schema:domainIncludes":{"@id":"unece:BinaryFile"},"rdfs:comment":"The file name, expressed as text, of this specified binary file."},{"@id":"unece:includedBinaryObject","@type":["rdf:Property","owl:DatatypeProperty"],"rdfs:label":"includedBinaryObject","schema:rangeIncludes":{"@id":"schema:Text"},"schema:domainIncludes":{"@id":"unece:BinaryFile"},"rdfs:comment":"A binary object included in this specified binary file."},{"@id":"unece:mIMECode","@type":["rdf:Property","owl:DatatypeProperty"],"rdfs:label":"mIMECode","schema:rangeIncludes":{"@id":"unece:MimeCodeList"},"schema:domainIncludes":{"@id":"unece:BinaryFile"},"rdfs:comment":"The code specifying the Multipurpose Internet Mail Extensions (MIME) type for this specified binary file."},{"@id":"unece:title","@type":["rdf:Property","owl:DatatypeProperty"],"rdfs:label":"title","schema:rangeIncludes":{"@id":"schema:Text"},"schema:domainIncludes":[{"@id":"unece:BinaryFile"},{"@id":"unece:GuestPerson"}],"rdfs:comment":"A title, expressed as text, for this specified binary file."},{"@id":"unece:acquisitionDateTime","@type":["rdf:Property","owl:DatatypeProperty"],"rdfs:label":"acquisitionDateTime","schema:rangeIncludes":{"@id":"schema:Text"},"schema:domainIncludes":[{"@id":"unece:GeographicalCoordinate"},{"@id":"unece:RegulatoryProcedure"}],"rdfs:comment":"The date, time, date time or other date time value of the acquisition of this geographical coordinate."},{"@id":"unece:alternativeSourceSystemId","@type":["rdf:Property","owl:DatatypeProperty"],"rdfs:label":"alternativeSourceSystemId","schema:rangeIncludes":{"@id":"schema:Text"},"schema:domainIncludes":{"@id":"unece:GeographicalCoordinate"},"rdfs:comment":"An alternative source system identifier for this geographical coordinate."},{"@id":"unece:altimetricSystemId","@type":["rdf:Property","owl:DatatypeProperty"],"rdfs:label":"altimetricSystemId","schema:rangeIncludes":{"@id":"schema:Text"},"schema:domainIncludes":{"@id":"unece:GeographicalCoordinate"},"rdfs:comment":"The unique identifier of the system used for measuring the altitude."},{"@id":"unece:altitudeMeasure","@type":["rdf:Property","owl:ObjectProperty"],"rdfs:label":"altitudeMeasure","schema:rangeIncludes":{"@id":"unece:MeasureType"},"schema:domainIncludes":{"@id":"unece:GeographicalCoordinate"},"rdfs:comment":"The measure of the altitude that reflects the vertical elevation of an object above a surface for this geographical coordinate (Reference ISO 6709)."},{"@id":"unece:latitudeDirectionIndicator","@type":["rdf:Property","owl:DatatypeProperty"],"rdfs:label":"latitudeDirectionIndicator","schema:rangeIncludes":{"@id":"schema:Boolean"},"schema:domainIncludes":{"@id":"unece:GeographicalCoordinate"},"rdfs:comment":"The indication of whether the latitude compass direction from the Equator meridian to the meridian of a specific place is North (+) or South (-)  (Reference ISO 6709)."},{"@id":"unece:latitudeMeasure","@type":["rdf:Property","owl:ObjectProperty"],"rdfs:label":"latitudeMeasure","schema:rangeIncludes":{"@id":"unece:MeasureType"},"schema:domainIncludes":{"@id":"unece:GeographicalCoordinate"},"rdfs:comment":"The measure of the latitude as an angular distance north or south from the Equator meridian to the meridian of a specific place for this geographical coordinate (Reference ISO 6709)."},{"@id":"unece:longitudeDirectionIndicator","@type":["rdf:Property","owl:DatatypeProperty"],"rdfs:label":"longitudeDirectionIndicator","schema:rangeIncludes":{"@id":"schema:Boolean"},"schema:domainIncludes":{"@id":"unece:GeographicalCoordinate"},"rdfs:comment":"The indication of whether the longitude as a compass direction from the Greenwich meridian to the meridian of a specific place is East (+) or West (-) for this geographical coordinate (Reference ISO 6709)."},{"@id":"unece:longitudeMeasure","@type":["rdf:Property","owl:ObjectProperty"],"rdfs:label":"longitudeMeasure","schema:rangeIncludes":{"@id":"unece:MeasureType"},"schema:domainIncludes":{"@id":"unece:GeographicalCoordinate"},"rdfs:comment":"The measure of the longitude as an angular distance east or west from the Greenwich meridian to the meridian of a specific place (Reference ISO 6709)."},{"@id":"unece:timeZone","@type":["rdf:Property","owl:DatatypeProperty"],"rdfs:label":"timeZone","schema:rangeIncludes":{"@id":"schema:Text"},"schema:domainIncludes":{"@id":"unece:GeographicalCoordinate"},"rdfs:comment":"The time zone, expressed as text, for this geographical coordinate."},{"@id":"unece:timeZoneCode","@type":["rdf:Property","owl:DatatypeProperty"],"rdfs:label":"timeZoneCode","schema:rangeIncludes":{"@id":"schema:Text"},"schema:domainIncludes":{"@id":"unece:GeographicalCoordinate"},"rdfs:comment":"The code specifying the time zone of this geographical coordinate."},{"@id":"unece:timeZoneDateTime","@type":["rdf:Property","owl:DatatypeProperty"],"rdfs:label":"timeZoneDateTime","schema:rangeIncludes":{"@id":"schema:DateTime"},"schema:domainIncludes":{"@id":"unece:GeographicalCoordinate"},"rdfs:comment":"The date, time, date time, or other date time value for the time zone of this geographical coordinate."},{"@id":"unece:usedCoordinateReferenceSystem","@type":["rdf:Property","owl:ObjectProperty"],"rdfs:label":"usedCoordinateReferenceSystem","schema:rangeIncludes":{"@id":"unece:CoordinateReferenceSystem"},"schema:domainIncludes":[{"@id":"unece:GeographicalCoordinate"},{"@id":"unece:GeographicalFeature"}],"rdfs:comment":"The CS (Coordinate System) engineering coordinate reference system used for this geographical coordinate."},{"@id":"unece:usedCoordinateSourceSystem","@type":["rdf:Property","owl:ObjectProperty"],"rdfs:label":"usedCoordinateSourceSystem","schema:rangeIncludes":{"@id":"unece:CoordinateSourceSystem"},"schema:domainIncludes":[{"@id":"unece:GeographicalCoordinate"},{"@id":"unece:GeographicalFeature"}],"rdfs:comment":"The geographical coordinate source system used for this geographical coordinate."},{"@id":"unece:actionType","@type":["rdf:Property","owl:DatatypeProperty"],"rdfs:label":"actionType","schema:rangeIncludes":{"@id":"schema:Text"},"schema:domainIncludes":[{"@id":"unece:SpecifiedAction"},{"@id":"unece:CorrectiveAction"},{"@id":"unece:PreventiveAction"},{"@id":"unece:ExperienceProgramAction"}],"rdfs:comment":"A type, expressed as text, for this corrective action."},{"@id":"unece:activityAuthorizedParty","@type":["rdf:Property","owl:ObjectProperty"],"rdfs:label":"activityAuthorizedParty","schema:rangeIncludes":{"@id":"unece:Party"},"schema:domainIncludes":{"@id":"unece:CountrySubDivision"},"rdfs:comment":"A party that is authorized to perform an activity in this trade country sub-division."},{"@id":"unece:hierarchicalLevelCode","@type":["rdf:Property","owl:DatatypeProperty"],"rdfs:label":"hierarchicalLevelCode","schema:rangeIncludes":{"@id":"schema:Text"},"schema:domainIncludes":{"@id":"unece:CountrySubDivision"},"rdfs:comment":"The code specifying the hierarchical level of this trade country sub-division."},{"@id":"unece:subordinateCountrySubDivision","@type":["rdf:Property","owl:ObjectProperty"],"rdfs:label":"subordinateCountrySubDivision","schema:rangeIncludes":{"@id":"unece:CountrySubDivision"},"schema:domainIncludes":[{"@id":"unece:CountrySubDivision"},{"@id":"unece:Country"}],"rdfs:comment":"A subordinate country sub-division within this trade country sub-division."},{"@id":"unece:superordinateCountrySubDivision","@type":["rdf:Property","owl:ObjectProperty"],"rdfs:label":"superordinateCountrySubDivision","schema:rangeIncludes":{"@id":"unece:CountrySubDivision"},"schema:domainIncludes":{"@id":"unece:CountrySubDivision"},"rdfs:comment":"A superordinate country sub-division for this trade country sub-division."},{"@id":"unece:activityLevelMeasure","@type":["rdf:Property","owl:ObjectProperty"],"rdfs:label":"activityLevelMeasure","schema:rangeIncludes":{"@id":"unece:MeasureType"},"schema:domainIncludes":{"@id":"unece:RadioactiveIsotope"},"rdfs:comment":"A measure of the activity level of this specified radioactive isotope."},{"@id":"unece:note","@type":["rdf:Property","owl:DatatypeProperty"],"rdfs:label":"note","schema:rangeIncludes":{"@id":"schema:Text"},"schema:domainIncludes":{"@id":"unece:RadioactiveIsotope"},"rdfs:comment":"A note, expressed as text, for this specified radioactive isotope."},{"@id":"unece:specifiedRadionuclide","@type":["rdf:Property","owl:ObjectProperty"],"rdfs:label":"specifiedRadionuclide","schema:rangeIncludes":{"@id":"unece:Radionuclide"},"schema:domainIncludes":{"@id":"unece:RadioactiveIsotope"},"rdfs:comment":"The radionuclide details specified for this radioactive isotope."},{"@id":"unece:actualMeasure","@type":["rdf:Property","owl:ObjectProperty"],"rdfs:label":"actualMeasure","schema:rangeIncludes":{"@id":"unece:MeasureType"},"schema:domainIncludes":{"@id":"unece:Measurement"},"rdfs:comment":"An actual measure for this measurement."},{"@id":"unece:comparisonOperatorCode","@type":["rdf:Property","owl:DatatypeProperty"],"rdfs:label":"comparisonOperatorCode","schema:rangeIncludes":{"@id":"schema:Text"},"schema:domainIncludes":[{"@id":"unece:Measurement"},{"@id":"unece:InspectionResultCharacteristic"},{"@id":"unece:ObservationResultCharacteristic"}],"rdfs:comment":"A code specifying the operator, such as, less than, greater than or equal to, for comparing two actual measures."},{"@id":"unece:conditionMeasure","@type":["rdf:Property","owl:ObjectProperty"],"rdfs:label":"conditionMeasure","schema:rangeIncludes":{"@id":"unece:MeasureType"},"schema:domainIncludes":{"@id":"unece:Measurement"},"rdfs:comment":"A measure of a condition for this measurement."},{"@id":"unece:method","@type":["rdf:Property","owl:DatatypeProperty"],"rdfs:label":"method","schema:rangeIncludes":{"@id":"schema:Text"},"schema:domainIncludes":{"@id":"unece:Measurement"},"rdfs:comment":"A measurement method expressed as text."},{"@id":"unece:actualQuantityDimension","@type":["rdf:Property","owl:ObjectProperty"],"rdfs:label":"actualQuantityDimension","schema:rangeIncludes":{"@id":"unece:WorkItemDimension"},"schema:domainIncludes":{"@id":"unece:QuantityAnalysis"},"rdfs:comment":"A work item dimension of the actual quantity in this work item quantity analysis."},{"@id":"unece:actualQuantityPercent","@type":["rdf:Property","owl:DatatypeProperty"],"rdfs:label":"actualQuantityPercent","schema:rangeIncludes":{"@id":"schema:Text"},"schema:domainIncludes":{"@id":"unece:QuantityAnalysis"},"rdfs:comment":"The percentage of a total quantity that the actual quantity of this work item quantity analysis represents."},{"@id":"unece:alternativeClassificationCode","@type":["rdf:Property","owl:DatatypeProperty"],"rdfs:label":"alternativeClassificationCode","schema:rangeIncludes":{"@id":"schema:Text"},"schema:domainIncludes":[{"@id":"unece:QuantityAnalysis"},{"@id":"unece:BasicWorkItem"},{"@id":"unece:GroupedWorkItem"},{"@id":"unece:ProcessWorkItem"}],"rdfs:comment":"A code specifying an alternative classification for this basic work item."},{"@id":"unece:breakdownQuantityAnalysis","@type":["rdf:Property","owl:ObjectProperty"],"rdfs:label":"breakdownQuantityAnalysis","schema:rangeIncludes":{"@id":"unece:QuantityAnalysis"},"schema:domainIncludes":{"@id":"unece:QuantityAnalysis"},"rdfs:comment":"A quantity analysis breakdown of this work item quantity analysis."},{"@id":"unece:changedStatus","@type":["rdf:Property","owl:ObjectProperty"],"rdfs:label":"changedStatus","schema:rangeIncludes":{"@id":"unece:RecordedStatus"},"schema:domainIncludes":[{"@id":"unece:QuantityAnalysis"},{"@id":"unece:BreakdownStatement"},{"@id":"unece:BasicWorkItem"},{"@id":"unece:GroupedWorkItem"}],"rdfs:comment":"A changed recorded status for this basic work item."},{"@id":"unece:primaryClassificationCode","@type":["rdf:Property","owl:DatatypeProperty"],"rdfs:label":"primaryClassificationCode","schema:rangeIncludes":{"@id":"schema:Text"},"schema:domainIncludes":[{"@id":"unece:QuantityAnalysis"},{"@id":"unece:BasicWorkItem"},{"@id":"unece:GroupedWorkItem"},{"@id":"unece:ProcessWorkItem"}],"rdfs:comment":"A code specifying a primary classification value for this work item quantity analysis."},{"@id":"unece:actualSpecifiedPercent","@type":["rdf:Property","owl:DatatypeProperty"],"rdfs:label":"actualSpecifiedPercent","schema:rangeIncludes":{"@id":"schema:Text"},"schema:domainIncludes":{"@id":"unece:SpecifiedFault"},"rdfs:comment":"The actual percentage of this specified fault."},{"@id":"unece:actualSpecifiedQuantity","@type":["rdf:Property","owl:ObjectProperty"],"rdfs:label":"actualSpecifiedQuantity","schema:rangeIncludes":{"@id":"unece:QuantityType"},"schema:domainIncludes":{"@id":"unece:SpecifiedFault"},"rdfs:comment":"The actual total quantity of this specified fault."},{"@id":"unece:classificationCode","@type":["rdf:Property","owl:DatatypeProperty"],"rdfs:label":"classificationCode","schema:rangeIncludes":{"@id":"schema:Text"},"schema:domainIncludes":[{"@id":"unece:SpecifiedFault"},{"@id":"unece:FieldCrop"}],"rdfs:comment":"A code specifying a classification for this field crop."},{"@id":"unece:estimatedSpecifiedPercent","@type":["rdf:Property","owl:DatatypeProperty"],"rdfs:label":"estimatedSpecifiedPercent","schema:rangeIncludes":{"@id":"schema:Text"},"schema:domainIncludes":{"@id":"unece:SpecifiedFault"},"rdfs:comment":"The estimated percentage of this specified fault."},{"@id":"unece:faultType","@type":["rdf:Property","owl:DatatypeProperty"],"rdfs:label":"faultType","schema:rangeIncludes":{"@id":"schema:Text"},"schema:domainIncludes":{"@id":"unece:SpecifiedFault"},"rdfs:comment":"A type, expressed as text, of this specified fault."},{"@id":"unece:operationalApplicableTolerance","@type":["rdf:Property","owl:ObjectProperty"],"rdfs:label":"operationalApplicableTolerance","schema:rangeIncludes":{"@id":"unece:Tolerance"},"schema:domainIncludes":{"@id":"unece:SpecifiedFault"},"rdfs:comment":"An applicable operational tolerance of this specified fault."},{"@id":"unece:areaIncluded","@type":["rdf:Property","owl:DatatypeProperty"],"rdfs:label":"areaIncluded","schema:rangeIncludes":{"@id":"schema:Text"},"schema:domainIncludes":{"@id":"unece:Picture"},"rdfs:comment":"The area or location, expressed as text, that is included in this photographic picture."},{"@id":"unece:copyrightOwnerName","@type":["rdf:Property","owl:DatatypeProperty"],"rdfs:label":"copyrightOwnerName","schema:rangeIncludes":{"@id":"schema:Text"},"schema:domainIncludes":{"@id":"unece:Picture"},"rdfs:comment":"The name of the copyright owner, expressed as text, for this photographic picture."},{"@id":"unece:digitalImageBinaryObject","@type":["rdf:Property","owl:DatatypeProperty"],"rdfs:label":"digitalImageBinaryObject","schema:rangeIncludes":{"@id":"schema:Text"},"schema:domainIncludes":{"@id":"unece:Picture"},"rdfs:comment":"Binary object data that is the actual digital image for this photographic picture."},{"@id":"unece:intendedUseCode","@type":["rdf:Property","owl:DatatypeProperty"],"rdfs:label":"intendedUseCode","schema:rangeIncludes":{"@id":"schema:Text"},"schema:domainIncludes":{"@id":"unece:Picture"},"rdfs:comment":"The code specifying the intended use of this photographic picture."},{"@id":"unece:pictureType","@type":["rdf:Property","owl:DatatypeProperty"],"rdfs:label":"pictureType","schema:rangeIncludes":{"@id":"schema:Text"},"schema:domainIncludes":{"@id":"unece:Picture"},"rdfs:comment":"The type, expressed as text, of this photographic picture."},{"@id":"unece:renderingInformation","@type":["rdf:Property","owl:DatatypeProperty"],"rdfs:label":"renderingInformation","schema:rangeIncludes":{"@id":"schema:Text"},"schema:domainIncludes":{"@id":"unece:Picture"},"rdfs:comment":"Rendering information, expressed as text, for this photographic picture."},{"@id":"unece:resolutionTypeCode","@type":["rdf:Property","owl:DatatypeProperty"],"rdfs:label":"resolutionTypeCode","schema:rangeIncludes":{"@id":"schema:Text"},"schema:domainIncludes":{"@id":"unece:Picture"},"rdfs:comment":"The code specifying the type of resolution for this photographic picture."},{"@id":"unece:resolutionValueNumeric","@type":["rdf:Property","owl:DatatypeProperty"],"rdfs:label":"resolutionValueNumeric","schema:rangeIncludes":{"@id":"schema:Text"},"schema:domainIncludes":{"@id":"unece:Picture"},"rdfs:comment":"The value, expressed as a number, for the resolution of this photographic picture."},{"@id":"unece:subject","@type":["rdf:Property","owl:DatatypeProperty"],"rdfs:label":"subject","schema:rangeIncludes":{"@id":"schema:Text"},"schema:domainIncludes":[{"@id":"unece:Picture"},{"@id":"unece:Note"},{"@id":"unece:SpecialQuery"},{"@id":"unece:SpecifiedNote"}],"rdfs:comment":"A subject, expressed as text, of this specified note."},{"@id":"unece:takenDateTime","@type":["rdf:Property","owl:DatatypeProperty"],"rdfs:label":"takenDateTime","schema:rangeIncludes":{"@id":"schema:Text"},"schema:domainIncludes":{"@id":"unece:Picture"},"rdfs:comment":"The date, time, date time, or other date value of when this photographic picture was created."},{"@id":"unece:titleName","@type":["rdf:Property","owl:DatatypeProperty"],"rdfs:label":"titleName","schema:rangeIncludes":{"@id":"schema:Text"},"schema:domainIncludes":{"@id":"unece:Picture"},"rdfs:comment":"The name, expressed as text, of the title for this photographic picture."},{"@id":"unece:additionalReason","@type":["rdf:Property","owl:DatatypeProperty"],"rdfs:label":"additionalReason","schema:rangeIncludes":{"@id":"schema:Text"},"schema:domainIncludes":{"@id":"unece:ValidationStatus"},"rdfs:comment":"Information, expressed as text, related to the reason for this validation status."},{"@id":"unece:reason","@type":["rdf:Property","owl:DatatypeProperty"],"rdfs:label":"reason","schema:rangeIncludes":{"@id":"schema:Text"},"schema:domainIncludes":[{"@id":"unece:ValidationStatus"},{"@id":"unece:CancellationStatus"},{"@id":"unece:DocumentStatus"},{"@id":"unece:FinancialAdjustment"},{"@id":"unece:FinancingStatus"},{"@id":"unece:TradeAllowanceCharge"},{"@id":"unece:LogisticsStatus"},{"@id":"unece:DeliveryAdjustment"}],"rdfs:comment":"A reason, expressed as text, for this cancellation status."},{"@id":"unece:reasonCode","@type":["rdf:Property","owl:DatatypeProperty"],"rdfs:label":"reasonCode","schema:rangeIncludes":{"@id":"schema:Text"},"schema:domainIncludes":[{"@id":"unece:ValidationStatus"},{"@id":"unece:Error"},{"@id":"unece:CommunicationEvent"},{"@id":"unece:CancellationStatus"},{"@id":"unece:HeaderBalanceOut"},{"@id":"unece:PaymentBalanceOut"},{"@id":"unece:TradePrice"},{"@id":"unece:Service"},{"@id":"unece:TransportMovement"}],"rdfs:comment":"A code specifying a reason for the declared error."},{"@id":"unece:validationDocumentStatusConditionCode","@type":["rdf:Property","owl:DatatypeProperty"],"rdfs:label":"validationDocumentStatusConditionCode","schema:rangeIncludes":{"@id":"unece:ValidationDocumentStatusCodeList"},"schema:domainIncludes":{"@id":"unece:ValidationStatus"},"rdfs:comment":"The code specifying the condition of this validation status."},{"@id":"unece:ageLimitation","@type":["rdf:Property","owl:DatatypeProperty"],"rdfs:label":"ageLimitation","schema:rangeIncludes":{"@id":"schema:Text"},"schema:domainIncludes":{"@id":"unece:UsageCondition"},"rdfs:comment":"An age limitation, expressed as text, for this specified usage condition."},{"@id":"unece:appropriateClothing","@type":["rdf:Property","owl:DatatypeProperty"],"rdfs:label":"appropriateClothing","schema:rangeIncludes":{"@id":"schema:Text"},"schema:domainIncludes":{"@id":"unece:UsageCondition"},"rdfs:comment":"Appropriate clothing, expressed as text, for this specified usage condition."},{"@id":"unece:duration","@type":["rdf:Property","owl:DatatypeProperty"],"rdfs:label":"duration","schema:rangeIncludes":{"@id":"schema:Text"},"schema:domainIncludes":[{"@id":"unece:UsageCondition"},{"@id":"unece:SpecifiedPeriod"}],"rdfs:comment":"A duration, expressed as text, for this specified period."},{"@id":"unece:genderLimitation","@type":["rdf:Property","owl:DatatypeProperty"],"rdfs:label":"genderLimitation","schema:rangeIncludes":{"@id":"schema:Text"},"schema:domainIncludes":{"@id":"unece:UsageCondition"},"rdfs:comment":"A gender limitation, expressed as text, for this specified usage condition."},{"@id":"unece:occupancy","@type":["rdf:Property","owl:DatatypeProperty"],"rdfs:label":"occupancy","schema:rangeIncludes":{"@id":"schema:Text"},"schema:domainIncludes":{"@id":"unece:UsageCondition"},"rdfs:comment":"Occupancy, expressed as text, for this specified usage condition."},{"@id":"unece:requiringParty","@type":["rdf:Property","owl:ObjectProperty"],"rdfs:label":"requiringParty","schema:rangeIncludes":{"@id":"unece:Party"},"schema:domainIncludes":{"@id":"unece:UsageCondition"},"rdfs:comment":"A party requiring this specified usage condition."},{"@id":"unece:alienRegistrationId","@type":["rdf:Property","owl:DatatypeProperty"],"rdfs:label":"alienRegistrationId","schema:rangeIncludes":{"@id":"schema:Text"},"schema:domainIncludes":{"@id":"unece:PersonIdentity"},"rdfs:comment":"The alien registration identifier for this person."},{"@id":"unece:driversLicenceId","@type":["rdf:Property","owl:DatatypeProperty"],"rdfs:label":"driversLicenceId","schema:rangeIncludes":{"@id":"schema:Text"},"schema:domainIncludes":{"@id":"unece:PersonIdentity"},"rdfs:comment":"The drivers licence identifier for this person."},{"@id":"unece:identityCardId","@type":["rdf:Property","owl:DatatypeProperty"],"rdfs:label":"identityCardId","schema:rangeIncludes":{"@id":"schema:Text"},"schema:domainIncludes":{"@id":"unece:PersonIdentity"},"rdfs:comment":"The identity card identifier for this person."},{"@id":"unece:passportId","@type":["rdf:Property","owl:DatatypeProperty"],"rdfs:label":"passportId","schema:rangeIncludes":{"@id":"schema:Text"},"schema:domainIncludes":[{"@id":"unece:PersonIdentity"},{"@id":"unece:GuestPerson"}],"rdfs:comment":"The identifier of the passport of this guest."},{"@id":"unece:socialSecurityId","@type":["rdf:Property","owl:DatatypeProperty"],"rdfs:label":"socialSecurityId","schema:rangeIncludes":{"@id":"schema:Text"},"schema:domainIncludes":{"@id":"unece:PersonIdentity"},"rdfs:comment":"The social security identifier for this person."},{"@id":"unece:certificationId","@type":["rdf:Property","owl:DatatypeProperty"],"rdfs:label":"certificationId","schema:rangeIncludes":{"@id":"schema:Text"},"schema:domainIncludes":[{"@id":"unece:SpecifiedMethod"},{"@id":"unece:LaboratoryObservationAnalysisMethod"}],"rdfs:comment":"A certification identifier of this specified method."},{"@id":"unece:externalReference","@type":["rdf:Property","owl:DatatypeProperty"],"rdfs:label":"externalReference","schema:rangeIncludes":{"@id":"schema:Text"},"schema:domainIncludes":[{"@id":"unece:SpecifiedMethod"},{"@id":"unece:LaboratoryObservationAnalysisMethod"}],"rdfs:comment":"An external reference, expressed as text, for this specified method."},{"@id":"unece:localTypeCode","@type":["rdf:Property","owl:DatatypeProperty"],"rdfs:label":"localTypeCode","schema:rangeIncludes":{"@id":"schema:Text"},"schema:domainIncludes":[{"@id":"unece:SpecifiedMethod"},{"@id":"unece:LaboratoryObservationAnalysisMethod"}],"rdfs:comment":"The code specifying the local type for this method."},{"@id":"unece:measurementCode","@type":["rdf:Property","owl:DatatypeProperty"],"rdfs:label":"measurementCode","schema:rangeIncludes":{"@id":"schema:Text"},"schema:domainIncludes":{"@id":"unece:SpecifiedMethod"},"rdfs:comment":"The code specifying the measurement for this method."},{"@id":"unece:obligatoryTypeCode","@type":["rdf:Property","owl:DatatypeProperty"],"rdfs:label":"obligatoryTypeCode","schema:rangeIncludes":{"@id":"schema:Text"},"schema:domainIncludes":[{"@id":"unece:SpecifiedMethod"},{"@id":"unece:LaboratoryObservationAnalysisMethod"}],"rdfs:comment":"The code specifying the obligatory type for this method."},{"@id":"unece:standardTypeCode","@type":["rdf:Property","owl:DatatypeProperty"],"rdfs:label":"standardTypeCode","schema:rangeIncludes":{"@id":"schema:Text"},"schema:domainIncludes":[{"@id":"unece:SpecifiedMethod"},{"@id":"unece:LaboratoryObservationAnalysisMethod"}],"rdfs:comment":"The code specifying the standard type for this method."},{"@id":"unece:usedTechnologyCode","@type":["rdf:Property","owl:DatatypeProperty"],"rdfs:label":"usedTechnologyCode","schema:rangeIncludes":{"@id":"schema:Text"},"schema:domainIncludes":{"@id":"unece:SpecifiedMethod"},"rdfs:comment":"The code specifying the technology used by this method."},{"@id":"unece:applicableRadioactiveIsotope","@type":["rdf:Property","owl:ObjectProperty"],"rdfs:label":"applicableRadioactiveIsotope","schema:rangeIncludes":{"@id":"unece:RadioactiveIsotope"},"schema:domainIncludes":{"@id":"unece:RadioactiveMaterial"},"rdfs:comment":"An isotope applicable to this radioactive material."},{"@id":"unece:compositionDescription","@type":["rdf:Property","owl:DatatypeProperty"],"rdfs:label":"compositionDescription","schema:rangeIncludes":{"@id":"schema:Text"},"schema:domainIncludes":{"@id":"unece:RadioactiveMaterial"},"rdfs:comment":"The textual description of the composition of this radioactive material."},{"@id":"unece:criticalitySafetyIndexNumeric","@type":["rdf:Property","owl:DatatypeProperty"],"rdfs:label":"criticalitySafetyIndexNumeric","schema:rangeIncludes":{"@id":"schema:Text"},"schema:domainIncludes":{"@id":"unece:RadioactiveMaterial"},"rdfs:comment":"The criticality safety index number of this radioactive material."},{"@id":"unece:fissileCriticalitySafetyIndexNumeric","@type":["rdf:Property","owl:DatatypeProperty"],"rdfs:label":"fissileCriticalitySafetyIndexNumeric","schema:rangeIncludes":{"@id":"schema:Text"},"schema:domainIncludes":{"@id":"unece:RadioactiveMaterial"},"rdfs:comment":"The number (rounded up to the next tenth) assigned to and placed on the label of a fissile radioactive material package, to designate the degree of control of accumulation of packages, overpacks or freight containers containing fissile material during transportation."},{"@id":"unece:fissileExceptionIndicator","@type":["rdf:Property","owl:DatatypeProperty"],"rdfs:label":"fissileExceptionIndicator","schema:rangeIncludes":{"@id":"schema:Boolean"},"schema:domainIncludes":{"@id":"unece:RadioactiveMaterial"},"rdfs:comment":"The indication of whether or not this radioactive material is a fissile exception."},{"@id":"unece:lowDispersibleInformation","@type":["rdf:Property","owl:DatatypeProperty"],"rdfs:label":"lowDispersibleInformation","schema:rangeIncludes":{"@id":"schema:Text"},"schema:domainIncludes":{"@id":"unece:RadioactiveMaterial"},"rdfs:comment":"Information, expressed as text, describing the low dispersion properties of this radioactive material."},{"@id":"unece:radioactivePackageTransportIndexCode","@type":["rdf:Property","owl:DatatypeProperty"],"rdfs:label":"radioactivePackageTransportIndexCode","schema:rangeIncludes":{"@id":"schema:Text"},"schema:domainIncludes":{"@id":"unece:RadioactiveMaterial"},"rdfs:comment":"A code specifying a package transport index for this radioactive material."},{"@id":"unece:radionuclideName","@type":["rdf:Property","owl:DatatypeProperty"],"rdfs:label":"radionuclideName","schema:rangeIncludes":{"@id":"schema:Text"},"schema:domainIncludes":{"@id":"unece:RadioactiveMaterial"},"rdfs:comment":"The name of the radionuclide, expressed as text, of this radioactive material."},{"@id":"unece:specialFormInformation","@type":["rdf:Property","owl:DatatypeProperty"],"rdfs:label":"specialFormInformation","schema:rangeIncludes":{"@id":"schema:Text"},"schema:domainIncludes":{"@id":"unece:RadioactiveMaterial"},"rdfs:comment":"Information, expressed as text, describing the special form for this radioactive material."},{"@id":"unece:transportIndexNumeric","@type":["rdf:Property","owl:DatatypeProperty"],"rdfs:label":"transportIndexNumeric","schema:rangeIncludes":{"@id":"schema:Text"},"schema:domainIncludes":{"@id":"unece:RadioactiveMaterial"},"rdfs:comment":"The transport index number of this radioactive material."},{"@id":"unece:associatedGeographicalFeature","@type":["rdf:Property","owl:ObjectProperty"],"rdfs:label":"associatedGeographicalFeature","schema:rangeIncludes":{"@id":"unece:GeographicalFeature"},"schema:domainIncludes":[{"@id":"unece:Location"},{"@id":"unece:CommunicationEvent"},{"@id":"unece:TransportEvent"},{"@id":"unece:LogisticsLocation"}],"rdfs:comment":"A geographical feature associated with this communication event."},{"@id":"unece:locationCountryId","@type":["rdf:Property","owl:DatatypeProperty"],"rdfs:label":"locationCountryId","schema:rangeIncludes":{"@id":"unece:CountryId"},"schema:domainIncludes":{"@id":"unece:Location"},"rdfs:comment":"The identifier of the country for this referenced location."},{"@id":"unece:locationTypeCode","@type":["rdf:Property","owl:DatatypeProperty"],"rdfs:label":"locationTypeCode","schema:rangeIncludes":{"@id":"schema:Text"},"schema:domainIncludes":{"@id":"unece:Location"},"rdfs:comment":"The code specifying the type of referenced location."},{"@id":"unece:specifiedTradeParty","@type":["rdf:Property","owl:ObjectProperty"],"rdfs:label":"specifiedTradeParty","schema:rangeIncludes":{"@id":"unece:Party"},"schema:domainIncludes":[{"@id":"unece:Location"},{"@id":"unece:ExperienceProgramAction"},{"@id":"unece:ExperienceItem"},{"@id":"unece:ExperienceProduct"},{"@id":"unece:ExperienceEvent"}],"rdfs:comment":"A party specified for this experience event."},{"@id":"unece:uTCOffsetNumeric","@type":["rdf:Property","owl:DatatypeProperty"],"rdfs:label":"uTCOffsetNumeric","schema:rangeIncludes":{"@id":"schema:Text"},"schema:domainIncludes":{"@id":"unece:Location"},"rdfs:comment":"The UTC (Universal Time Coordinate) time offset value for this referenced location."},{"@id":"unece:applicationSpecifiedParameter","@type":["rdf:Property","owl:ObjectProperty"],"rdfs:label":"applicationSpecifiedParameter","schema:rangeIncludes":{"@id":"unece:DocumentContextParameter"},"schema:domainIncludes":{"@id":"unece:ExchangedDocumentContext"},"rdfs:comment":"An application context parameter specified for this exchanged document context."},{"@id":"unece:bIMSpecifiedParameter","@type":["rdf:Property","owl:ObjectProperty"],"rdfs:label":"bIMSpecifiedParameter","schema:rangeIncludes":{"@id":"unece:DocumentContextParameter"},"schema:domainIncludes":{"@id":"unece:ExchangedDocumentContext"},"rdfs:comment":"A Business Information Master (BIM) context parameter specified for this exchanged document context."},{"@id":"unece:businessProcessSpecifiedParameter","@type":["rdf:Property","owl:ObjectProperty"],"rdfs:label":"businessProcessSpecifiedParameter","schema:rangeIncludes":{"@id":"unece:DocumentContextParameter"},"schema:domainIncludes":{"@id":"unece:ExchangedDocumentContext"},"rdfs:comment":"A business process context parameter specified for this exchanged document context."},{"@id":"unece:guidelineSpecifiedParameter","@type":["rdf:Property","owl:ObjectProperty"],"rdfs:label":"guidelineSpecifiedParameter","schema:rangeIncludes":{"@id":"unece:DocumentContextParameter"},"schema:domainIncludes":{"@id":"unece:ExchangedDocumentContext"},"rdfs:comment":"A guideline context parameter specified for this exchanged document context."},{"@id":"unece:messageStandardSpecifiedParameter","@type":["rdf:Property","owl:ObjectProperty"],"rdfs:label":"messageStandardSpecifiedParameter","schema:rangeIncludes":{"@id":"unece:DocumentContextParameter"},"schema:domainIncludes":{"@id":"unece:ExchangedDocumentContext"},"rdfs:comment":"The message standard document context parameter specified for this exchanged document context."},{"@id":"unece:processingTransactionDateTime","@type":["rdf:Property","owl:DatatypeProperty"],"rdfs:label":"processingTransactionDateTime","schema:rangeIncludes":{"@id":"schema:Text"},"schema:domainIncludes":{"@id":"unece:ExchangedDocumentContext"},"rdfs:comment":"The date, time, date time, or other date time value of the processing of a transaction for this exchanged document context."},{"@id":"unece:scenarioSpecifiedParameter","@type":["rdf:Property","owl:ObjectProperty"],"rdfs:label":"scenarioSpecifiedParameter","schema:rangeIncludes":{"@id":"unece:DocumentContextParameter"},"schema:domainIncludes":{"@id":"unece:ExchangedDocumentContext"},"rdfs:comment":"A scenario context parameter specified for this exchanged document context."},{"@id":"unece:specifiedTransactionId","@type":["rdf:Property","owl:DatatypeProperty"],"rdfs:label":"specifiedTransactionId","schema:rangeIncludes":{"@id":"schema:Text"},"schema:domainIncludes":{"@id":"unece:ExchangedDocumentContext"},"rdfs:comment":"The identifier of a specified transaction in this exchanged document context."},{"@id":"unece:subsetSpecifiedParameter","@type":["rdf:Property","owl:ObjectProperty"],"rdfs:label":"subsetSpecifiedParameter","schema:rangeIncludes":{"@id":"unece:DocumentContextParameter"},"schema:domainIncludes":{"@id":"unece:ExchangedDocumentContext"},"rdfs:comment":"A subset context parameter specified for this exchanged document context."},{"@id":"unece:userSpecifiedParameter","@type":["rdf:Property","owl:ObjectProperty"],"rdfs:label":"userSpecifiedParameter","schema:rangeIncludes":{"@id":"unece:DocumentContextParameter"},"schema:domainIncludes":{"@id":"unece:ExchangedDocumentContext"},"rdfs:comment":"A user specified document context parameter specified for this exchanged document context."},{"@id":"unece:associatedDirectPositionList","@type":["rdf:Property","owl:ObjectProperty"],"rdfs:label":"associatedDirectPositionList","schema:rangeIncludes":{"@id":"unece:DirectPositionList"},"schema:domainIncludes":[{"@id":"unece:GeographicalLine"},{"@id":"unece:GeographicalMultiCurve"},{"@id":"unece:GeographicalMultiPoint"},{"@id":"unece:GeographicalPoint"}],"rdfs:comment":"The direct position list associated with this geographical line."},{"@id":"unece:associatedGeographicalObjectCharacteristic","@type":["rdf:Property","owl:ObjectProperty"],"rdfs:label":"associatedGeographicalObjectCharacteristic","schema:rangeIncludes":{"@id":"unece:GeographicalObjectCharacteristic"},"schema:domainIncludes":[{"@id":"unece:GeographicalLine"},{"@id":"unece:GeographicalMultiCurve"},{"@id":"unece:GeographicalMultiPoint"},{"@id":"unece:GeographicalPoint"},{"@id":"unece:Circle"},{"@id":"unece:GeographicalGrid"},{"@id":"unece:GeographicalMultiSurface"},{"@id":"unece:GeographicalSurface"},{"@id":"unece:LinearRing"},{"@id":"unece:Polygon"}],"rdfs:comment":"The geographical object characteristic associated with this geographical grid."},{"@id":"unece:associatedLocation","@type":["rdf:Property","owl:ObjectProperty"],"rdfs:label":"associatedLocation","schema:rangeIncludes":{"@id":"unece:Location"},"schema:domainIncludes":[{"@id":"unece:GeographicalLine"},{"@id":"unece:GeographicalPoint"},{"@id":"unece:Circle"},{"@id":"unece:GeographicalGrid"},{"@id":"unece:Polygon"}],"rdfs:comment":"A logistics location associated with this specified circle."},{"@id":"unece:memberGeographicalLine","@type":["rdf:Property","owl:ObjectProperty"],"rdfs:label":"memberGeographicalLine","schema:rangeIncludes":{"@id":"unece:GeographicalLine"},"schema:domainIncludes":{"@id":"unece:GeographicalMultiCurve"},"rdfs:comment":"A geographical line member of this geographical multi-curve."},{"@id":"unece:memberGeographicalPoint","@type":["rdf:Property","owl:ObjectProperty"],"rdfs:label":"memberGeographicalPoint","schema:rangeIncludes":{"@id":"unece:GeographicalPoint"},"schema:domainIncludes":{"@id":"unece:GeographicalMultiPoint"},"rdfs:comment":"A geographical point member of this geographical multi-point feature."},{"@id":"unece:associatedEvent","@type":["rdf:Property","owl:ObjectProperty"],"rdfs:label":"associatedEvent","schema:rangeIncludes":{"@id":"unece:Event"},"schema:domainIncludes":{"@id":"unece:Error"},"rdfs:comment":"A corrective event associated with this declared error."},{"@id":"unece:occurrenceLogisticsLocation","@type":["rdf:Property","owl:ObjectProperty"],"rdfs:label":"occurrenceLogisticsLocation","schema:rangeIncludes":{"@id":"unece:Location"},"schema:domainIncludes":[{"@id":"unece:CommunicationEvent"},{"@id":"unece:TransportEvent"},{"@id":"unece:SupplyChainEvent"}],"rdfs:comment":"A logistics location where this supply chain event occurs."},{"@id":"unece:operationalResponsibleParty","@type":["rdf:Property","owl:ObjectProperty"],"rdfs:label":"operationalResponsibleParty","schema:rangeIncludes":{"@id":"unece:Party"},"schema:domainIncludes":{"@id":"unece:CommunicationEvent"},"rdfs:comment":"The operational responsible party for this communication event."},{"@id":"unece:valueMeasure","@type":["rdf:Property","owl:ObjectProperty"],"rdfs:label":"valueMeasure","schema:rangeIncludes":{"@id":"unece:MeasureType"},"schema:domainIncludes":[{"@id":"unece:CommunicationEvent"},{"@id":"unece:WorkItemDimension"},{"@id":"unece:MetricCharacteristic"},{"@id":"unece:DocumentCharacteristic"},{"@id":"unece:SpatialDimension"},{"@id":"unece:SpecifiedParameter"},{"@id":"unece:ProductCharacteristic"},{"@id":"unece:ProductBatchCharacteristic"},{"@id":"unece:SustainabilityCharacteristic"},{"@id":"unece:ProcessCharacteristic"},{"@id":"unece:TechnicalCharacteristic"},{"@id":"unece:ControlSettingParameter"},{"@id":"unece:OperationalParameter"},{"@id":"unece:ObservationObjectiveParameter"},{"@id":"unece:CalibratedMeasurement"},{"@id":"unece:ProductCharacteristicCondition"},{"@id":"unece:OrganizationCharacteristic"},{"@id":"unece:AgriculturalCharacteristic"},{"@id":"unece:Sensor"},{"@id":"unece:SpecifiedCondition"}],"rdfs:comment":"A measure of a value for this document characteristic."},{"@id":"unece:centreGeographicalPoint","@type":["rdf:Property","owl:ObjectProperty"],"rdfs:label":"centreGeographicalPoint","schema:rangeIncludes":{"@id":"unece:GeographicalPoint"},"schema:domainIncludes":{"@id":"unece:Circle"},"rdfs:comment":"The geographical point which defines the centre of this specified circle."},{"@id":"unece:radiusMeasure","@type":["rdf:Property","owl:ObjectProperty"],"rdfs:label":"radiusMeasure","schema:rangeIncludes":{"@id":"unece:MeasureType"},"schema:domainIncludes":{"@id":"unece:Circle"},"rdfs:comment":"The measure of the radius for this specified circle."},{"@id":"unece:axisName","@type":["rdf:Property","owl:DatatypeProperty"],"rdfs:label":"axisName","schema:rangeIncludes":{"@id":"schema:Text"},"schema:domainIncludes":{"@id":"unece:GeographicalGrid"},"rdfs:comment":"An axis name, expressed as text, for this geographical grid."},{"@id":"unece:cell","@type":["rdf:Property","owl:DatatypeProperty"],"rdfs:label":"cell","schema:rangeIncludes":{"@id":"schema:Text"},"schema:domainIncludes":{"@id":"unece:GeographicalGrid"},"rdfs:comment":"The cell value, expressed as text, for this geographical grid."},{"@id":"unece:dimensionNumeric","@type":["rdf:Property","owl:DatatypeProperty"],"rdfs:label":"dimensionNumeric","schema:rangeIncludes":{"@id":"schema:Text"},"schema:domainIncludes":{"@id":"unece:GeographicalGrid"},"rdfs:comment":"The dimension, expressed as a number, of this geographical grid."},{"@id":"unece:highLimit","@type":["rdf:Property","owl:DatatypeProperty"],"rdfs:label":"highLimit","schema:rangeIncludes":{"@id":"schema:Text"},"schema:domainIncludes":{"@id":"unece:GeographicalGrid"},"rdfs:comment":"The tuple of elements, expressed as text, indicating the high limit of this geographical grid specifying the diagonally opposing corner of each axis."},{"@id":"unece:lowLimit","@type":["rdf:Property","owl:DatatypeProperty"],"rdfs:label":"lowLimit","schema:rangeIncludes":{"@id":"schema:Text"},"schema:domainIncludes":{"@id":"unece:GeographicalGrid"},"rdfs:comment":"The tuple of elements, expressed as text, indicating the low limit of this geographical grid specifying the offset of each axis."},{"@id":"unece:offsetVectorNumeric","@type":["rdf:Property","owl:DatatypeProperty"],"rdfs:label":"offsetVectorNumeric","schema:rangeIncludes":{"@id":"schema:Text"},"schema:domainIncludes":{"@id":"unece:GeographicalGrid"},"rdfs:comment":"The offset vector, expressed as a number, which indicates the offset of cells along each axis for this geographical grid."},{"@id":"unece:originAssociatedDirectPositionList","@type":["rdf:Property","owl:ObjectProperty"],"rdfs:label":"originAssociatedDirectPositionList","schema:rangeIncludes":{"@id":"unece:DirectPositionList"},"schema:domainIncludes":{"@id":"unece:GeographicalGrid"},"rdfs:comment":"The direct position list associated with the origin of this geographical grid."},{"@id":"unece:includedPolygon","@type":["rdf:Property","owl:ObjectProperty"],"rdfs:label":"includedPolygon","schema:rangeIncludes":{"@id":"unece:Polygon"},"schema:domainIncludes":[{"@id":"unece:GeographicalMultiSurface"},{"@id":"unece:GeographicalSurface"},{"@id":"unece:GeographicalFeature"}],"rdfs:comment":"A polygon included in this geographical multi-surface."},{"@id":"unece:coordinate","@type":["rdf:Property","owl:DatatypeProperty"],"rdfs:label":"coordinate","schema:rangeIncludes":{"@id":"schema:Text"},"schema:domainIncludes":[{"@id":"unece:LinearRing"},{"@id":"unece:DirectPositionList"}],"rdfs:comment":"A coordinate, expressed as text, for this specified linear ring."},{"@id":"unece:coordinateDirectPosition","@type":["rdf:Property","owl:ObjectProperty"],"rdfs:label":"coordinateDirectPosition","schema:rangeIncludes":{"@id":"unece:DirectPosition"},"schema:domainIncludes":{"@id":"unece:LinearRing"},"rdfs:comment":"The specified direct position of a coordinate for this linear ring."},{"@id":"unece:exteriorLinearRing","@type":["rdf:Property","owl:ObjectProperty"],"rdfs:label":"exteriorLinearRing","schema:rangeIncludes":{"@id":"unece:LinearRing"},"schema:domainIncludes":{"@id":"unece:Polygon"},"rdfs:comment":"The exterior linear specified ring for this polygon."},{"@id":"unece:interiorLinearRing","@type":["rdf:Property","owl:ObjectProperty"],"rdfs:label":"interiorLinearRing","schema:rangeIncludes":{"@id":"unece:LinearRing"},"schema:domainIncludes":{"@id":"unece:Polygon"},"rdfs:comment":"An interior linear ring specified for this polygon."},{"@id":"unece:authorizedRegistration","@type":["rdf:Property","owl:ObjectProperty"],"rdfs:label":"authorizedRegistration","schema:rangeIncludes":{"@id":"unece:LegalRegistration"},"schema:domainIncludes":{"@id":"unece:LegalOrganization"},"rdfs:comment":"A legal registration authorized for this legally set up organization."},{"@id":"unece:establishedDateTime","@type":["rdf:Property","owl:DatatypeProperty"],"rdfs:label":"establishedDateTime","schema:rangeIncludes":{"@id":"schema:Text"},"schema:domainIncludes":{"@id":"unece:LegalOrganization"},"rdfs:comment":"The date, time, date time, or other date time value when this legally set up organization was established."},{"@id":"unece:legalClassificationCode","@type":["rdf:Property","owl:DatatypeProperty"],"rdfs:label":"legalClassificationCode","schema:rangeIncludes":{"@id":"schema:Text"},"schema:domainIncludes":{"@id":"unece:LegalOrganization"},"rdfs:comment":"The code specifying the legal classification of this organization, such as Incorporated (Inc), Limited Liability Corporation (LLC) or non-profit."},{"@id":"unece:tradingBusinessName","@type":["rdf:Property","owl:DatatypeProperty"],"rdfs:label":"tradingBusinessName","schema:rangeIncludes":{"@id":"schema:Text"},"schema:domainIncludes":{"@id":"unece:LegalOrganization"},"rdfs:comment":"The trading business name, expressed as text, of this legally set up organization."},{"@id":"unece:axisLabelList","@type":["rdf:Property","owl:DatatypeProperty"],"rdfs:label":"axisLabelList","schema:rangeIncludes":{"@id":"schema:Text"},"schema:domainIncludes":[{"@id":"unece:DirectPosition"},{"@id":"unece:DirectPositionList"}],"rdfs:comment":"An ordered list of axis labels, expressed as text, for this specified direct position list."},{"@id":"unece:coordinateReferenceDimension","@type":["rdf:Property","owl:DatatypeProperty"],"rdfs:label":"coordinateReferenceDimension","schema:rangeIncludes":{"@id":"schema:Text"},"schema:domainIncludes":[{"@id":"unece:DirectPosition"},{"@id":"unece:DirectPositionList"}],"rdfs:comment":"A coordinate reference dimension, expressed as text, for this specified direct position list."},{"@id":"unece:countNumeric","@type":["rdf:Property","owl:DatatypeProperty"],"rdfs:label":"countNumeric","schema:rangeIncludes":{"@id":"schema:Text"},"schema:domainIncludes":[{"@id":"unece:DirectPosition"},{"@id":"unece:DirectPositionList"}],"rdfs:comment":"A count for this specified direct position list."},{"@id":"unece:uOMLabelList","@type":["rdf:Property","owl:DatatypeProperty"],"rdfs:label":"uOMLabelList","schema:rangeIncludes":{"@id":"schema:Text"},"schema:domainIncludes":[{"@id":"unece:DirectPosition"},{"@id":"unece:DirectPositionList"}],"rdfs:comment":"An ordered list of Unit Of Measure (UOM) labels, expressed as text, for this specified direct position list."},{"@id":"unece:birthAddressCountryId","@type":["rdf:Property","owl:DatatypeProperty"],"rdfs:label":"birthAddressCountryId","schema:rangeIncludes":{"@id":"unece:CountryId"},"schema:domainIncludes":{"@id":"unece:BirthAddress"},"rdfs:comment":"The identifier of a country for this birth address."},{"@id":"unece:cancellationDocumentStatusConditionCode","@type":["rdf:Property","owl:DatatypeProperty"],"rdfs:label":"cancellationDocumentStatusConditionCode","schema:rangeIncludes":{"@id":"schema:Text"},"schema:domainIncludes":{"@id":"unece:CancellationStatus"},"rdfs:comment":"The code specifying the condition of this cancellation status."},{"@id":"unece:reasonInformation","@type":["rdf:Property","owl:DatatypeProperty"],"rdfs:label":"reasonInformation","schema:rangeIncludes":{"@id":"schema:Text"},"schema:domainIncludes":[{"@id":"unece:CancellationStatus"},{"@id":"unece:DocumentStatus"},{"@id":"unece:FinancingStatus"}],"rdfs:comment":"Information, expressed as text, related to the reason for this cancellation status."},{"@id":"unece:category","@type":["rdf:Property","owl:DatatypeProperty"],"rdfs:label":"category","schema:rangeIncludes":{"@id":"schema:Text"},"schema:domainIncludes":{"@id":"unece:Object"},"rdfs:comment":"A category, expressed as text, for this specified object."},{"@id":"unece:objectType","@type":["rdf:Property","owl:DatatypeProperty"],"rdfs:label":"objectType","schema:rangeIncludes":{"@id":"schema:Text"},"schema:domainIncludes":{"@id":"unece:Object"},"rdfs:comment":"A type, expressed as text, for this specified object."},{"@id":"unece:remark","@type":["rdf:Property","owl:DatatypeProperty"],"rdfs:label":"remark","schema:rangeIncludes":{"@id":"schema:Text"},"schema:domainIncludes":[{"@id":"unece:Object"},{"@id":"unece:RegulatoryProcedure"}],"rdfs:comment":"A remark, expressed as text, for this cross-border regulatory procedure."},{"@id":"unece:genderCode","@type":["rdf:Property","owl:DatatypeProperty"],"rdfs:label":"genderCode","schema:rangeIncludes":{"@id":"schema:Text"},"schema:domainIncludes":[{"@id":"unece:CustomerClass"},{"@id":"unece:Person"},{"@id":"unece:GuestPerson"},{"@id":"unece:TransportPerson"}],"rdfs:comment":"A code specifying the gender of this transport person."},{"@id":"unece:lowerAgeLimitNumeric","@type":["rdf:Property","owl:DatatypeProperty"],"rdfs:label":"lowerAgeLimitNumeric","schema:rangeIncludes":{"@id":"schema:Text"},"schema:domainIncludes":{"@id":"unece:CustomerClass"},"rdfs:comment":"The value, expressed as a number of years, for the lower age limit for the category of this specified customer class."},{"@id":"unece:mealServiceCategoryCode","@type":["rdf:Property","owl:DatatypeProperty"],"rdfs:label":"mealServiceCategoryCode","schema:rangeIncludes":{"@id":"schema:Text"},"schema:domainIncludes":{"@id":"unece:CustomerClass"},"rdfs:comment":"The code specifying the meal service category for this specified customer class."},{"@id":"unece:specialBeddingServiceOfferedIndicator","@type":["rdf:Property","owl:DatatypeProperty"],"rdfs:label":"specialBeddingServiceOfferedIndicator","schema:rangeIncludes":{"@id":"schema:Boolean"},"schema:domainIncludes":{"@id":"unece:CustomerClass"},"rdfs:comment":"The indication of whether or not special bedding service is offered for this specified customer class."},{"@id":"unece:upperAgeLimitNumeric","@type":["rdf:Property","owl:DatatypeProperty"],"rdfs:label":"upperAgeLimitNumeric","schema:rangeIncludes":{"@id":"schema:Text"},"schema:domainIncludes":{"@id":"unece:CustomerClass"},"rdfs:comment":"The value, expressed as a number of years, for the upper age limit for the category of this specified customer class."},{"@id":"unece:securityInformation","@type":["rdf:Property","owl:DatatypeProperty"],"rdfs:label":"securityInformation","schema:rangeIncludes":{"@id":"schema:Text"},"schema:domainIncludes":{"@id":"unece:InformationSource"},"rdfs:comment":"Security information, expressed as text, of this specified information source."},{"@id":"unece:changedDateTime","@type":["rdf:Property","owl:DatatypeProperty"],"rdfs:label":"changedDateTime","schema:rangeIncludes":{"@id":"schema:Text"},"schema:domainIncludes":{"@id":"unece:RecordedStatus"},"rdfs:comment":"The date, time, date time, or other date time value when this recorded status changed."},{"@id":"unece:changerName","@type":["rdf:Property","owl:DatatypeProperty"],"rdfs:label":"changerName","schema:rangeIncludes":{"@id":"schema:Text"},"schema:domainIncludes":{"@id":"unece:RecordedStatus"},"rdfs:comment":"The name of the person or system, expressed as text, that changed this recorded status."},{"@id":"unece:recordedStatusConditionCode","@type":["rdf:Property","owl:DatatypeProperty"],"rdfs:label":"recordedStatusConditionCode","schema:rangeIncludes":{"@id":"schema:Text"},"schema:domainIncludes":{"@id":"unece:RecordedStatus"},"rdfs:comment":"The code specifying the condition for this recorded status."},{"@id":"unece:collectionIndicator","@type":["rdf:Property","owl:DatatypeProperty"],"rdfs:label":"collectionIndicator","schema:rangeIncludes":{"@id":"schema:Boolean"},"schema:domainIncludes":{"@id":"unece:GeographicalFeature"},"rdfs:comment":"The indication of whether or not this specified geographical feature is a collection of features."},{"@id":"unece:coordinateReferenceSystemId","@type":["rdf:Property","owl:DatatypeProperty"],"rdfs:label":"coordinateReferenceSystemId","schema:rangeIncludes":{"@id":"schema:Text"},"schema:domainIncludes":{"@id":"unece:GeographicalFeature"},"rdfs:comment":"The identifier of the coordinate reference system for this geographical feature."},{"@id":"unece:includedCircle","@type":["rdf:Property","owl:ObjectProperty"],"rdfs:label":"includedCircle","schema:rangeIncludes":{"@id":"unece:Circle"},"schema:domainIncludes":{"@id":"unece:GeographicalFeature"},"rdfs:comment":"A circle included in this specified geographical feature."},{"@id":"unece:includedGeographicalGrid","@type":["rdf:Property","owl:ObjectProperty"],"rdfs:label":"includedGeographicalGrid","schema:rangeIncludes":{"@id":"unece:GeographicalGrid"},"schema:domainIncludes":{"@id":"unece:GeographicalFeature"},"rdfs:comment":"The geographical grid included in this geographical feature."},{"@id":"unece:includedGeographicalLine","@type":["rdf:Property","owl:ObjectProperty"],"rdfs:label":"includedGeographicalLine","schema:rangeIncludes":{"@id":"unece:GeographicalLine"},"schema:domainIncludes":{"@id":"unece:GeographicalFeature"},"rdfs:comment":"The geographical line included in this geographical feature."},{"@id":"unece:includedGeographicalMultiCurve","@type":["rdf:Property","owl:ObjectProperty"],"rdfs:label":"includedGeographicalMultiCurve","schema:rangeIncludes":{"@id":"unece:GeographicalMultiCurve"},"schema:domainIncludes":{"@id":"unece:GeographicalFeature"},"rdfs:comment":"The geographical multi-curve included in this geographical feature."},{"@id":"unece:includedGeographicalMultiPoint","@type":["rdf:Property","owl:ObjectProperty"],"rdfs:label":"includedGeographicalMultiPoint","schema:rangeIncludes":{"@id":"unece:GeographicalMultiPoint"},"schema:domainIncludes":{"@id":"unece:GeographicalFeature"},"rdfs:comment":"The geographical multi-point included in this geographical feature."},{"@id":"unece:includedGeographicalMultiSurface","@type":["rdf:Property","owl:ObjectProperty"],"rdfs:label":"includedGeographicalMultiSurface","schema:rangeIncludes":{"@id":"unece:GeographicalMultiSurface"},"schema:domainIncludes":{"@id":"unece:GeographicalFeature"},"rdfs:comment":"The geographical multi-surface included in this geographical feature."},{"@id":"unece:includedGeographicalPoint","@type":["rdf:Property","owl:ObjectProperty"],"rdfs:label":"includedGeographicalPoint","schema:rangeIncludes":{"@id":"unece:GeographicalPoint"},"schema:domainIncludes":{"@id":"unece:GeographicalFeature"},"rdfs:comment":"The geographical point included in this geographical feature."},{"@id":"unece:includedGeographicalSurface","@type":["rdf:Property","owl:ObjectProperty"],"rdfs:label":"includedGeographicalSurface","schema:rangeIncludes":{"@id":"unece:GeographicalSurface"},"schema:domainIncludes":{"@id":"unece:GeographicalFeature"},"rdfs:comment":"The geographical surface included in this geographical feature."},{"@id":"unece:communicationChannelCode","@type":["rdf:Property","owl:DatatypeProperty"],"rdfs:label":"communicationChannelCode","schema:rangeIncludes":{"@id":"unece:CommunicationChannelCodeList"},"schema:domainIncludes":{"@id":"unece:Communication"},"rdfs:comment":"The code specifying the channel or manner in which a universal communication can be made, such as telephone or email."},{"@id":"unece:completeNumber","@type":["rdf:Property","owl:DatatypeProperty"],"rdfs:label":"completeNumber","schema:rangeIncludes":{"@id":"schema:Text"},"schema:domainIncludes":{"@id":"unece:Communication"},"rdfs:comment":"The text string of characters that make up the complete number for this universal communication."},{"@id":"unece:emailURIId","@type":["rdf:Property","owl:DatatypeProperty"],"rdfs:label":"emailURIId","schema:rangeIncludes":{"@id":"schema:Text"},"schema:domainIncludes":{"@id":"unece:Communication"},"rdfs:comment":"The Uniform Resource Identifier (URI) of the email for this universal communication."},{"@id":"unece:completeDateTime","@type":["rdf:Property","owl:DatatypeProperty"],"rdfs:label":"completeDateTime","schema:rangeIncludes":{"@id":"schema:Text"},"schema:domainIncludes":{"@id":"unece:SpecifiedPeriod"},"rdfs:comment":"The date, time, date time or other date time value for a complete specified period of time expressed as a specific month, a specific week, etc."},{"@id":"unece:continuousIndicator","@type":["rdf:Property","owl:DatatypeProperty"],"rdfs:label":"continuousIndicator","schema:rangeIncludes":{"@id":"schema:Boolean"},"schema:domainIncludes":{"@id":"unece:SpecifiedPeriod"},"rdfs:comment":"The indication of whether or not this specified period is continuous."},{"@id":"unece:dayQuantity","@type":["rdf:Property","owl:ObjectProperty"],"rdfs:label":"dayQuantity","schema:rangeIncludes":{"@id":"unece:QuantityType"},"schema:domainIncludes":[{"@id":"unece:SpecifiedPeriod"},{"@id":"unece:TradePrice"}],"rdfs:comment":"The number of days in this specified period."},{"@id":"unece:durationMeasure","@type":["rdf:Property","owl:ObjectProperty"],"rdfs:label":"durationMeasure","schema:rangeIncludes":{"@id":"unece:MeasureType"},"schema:domainIncludes":[{"@id":"unece:SpecifiedPeriod"},{"@id":"unece:DelimitedPeriod"}],"rdfs:comment":"A measure of the length of time for this specified time period such as hours, days, weeks, months, years."},{"@id":"unece:endDayOfWeekCode","@type":["rdf:Property","owl:DatatypeProperty"],"rdfs:label":"endDayOfWeekCode","schema:rangeIncludes":{"@id":"schema:Text"},"schema:domainIncludes":{"@id":"unece:SpecifiedPeriod"},"rdfs:comment":"The code specifying the end day of the week for this specified period."},{"@id":"unece:inclusiveIndicator","@type":["rdf:Property","owl:DatatypeProperty"],"rdfs:label":"inclusiveIndicator","schema:rangeIncludes":{"@id":"schema:Boolean"},"schema:domainIncludes":{"@id":"unece:SpecifiedPeriod"},"rdfs:comment":"The indication of whether or not the start and end dates are included in this specified period."},{"@id":"unece:maximumDurationMeasure","@type":["rdf:Property","owl:ObjectProperty"],"rdfs:label":"maximumDurationMeasure","schema:rangeIncludes":{"@id":"unece:DurationUnitMeasureType"},"schema:domainIncludes":{"@id":"unece:SpecifiedPeriod"},"rdfs:comment":"The measure of the maximum length of time for this specified period, such as hours, days, weeks, months, years."},{"@id":"unece:minimumDurationMeasure","@type":["rdf:Property","owl:ObjectProperty"],"rdfs:label":"minimumDurationMeasure","schema:rangeIncludes":{"@id":"unece:DurationUnitMeasureType"},"schema:domainIncludes":{"@id":"unece:SpecifiedPeriod"},"rdfs:comment":"The measure of the minimum length of time for this specified period, such as hours, days, weeks, months, years."},{"@id":"unece:nightQuantity","@type":["rdf:Property","owl:ObjectProperty"],"rdfs:label":"nightQuantity","schema:rangeIncludes":{"@id":"unece:QuantityType"},"schema:domainIncludes":{"@id":"unece:SpecifiedPeriod"},"rdfs:comment":"The number of nights in this specified period."},{"@id":"unece:openIndicator","@type":["rdf:Property","owl:DatatypeProperty"],"rdfs:label":"openIndicator","schema:rangeIncludes":{"@id":"schema:Boolean"},"schema:domainIncludes":{"@id":"unece:SpecifiedPeriod"},"rdfs:comment":"The indication of whether or not an entity is open during this specified period."},{"@id":"unece:purposeCode","@type":["rdf:Property","owl:DatatypeProperty"],"rdfs:label":"purposeCode","schema:rangeIncludes":{"@id":"schema:Text"},"schema:domainIncludes":[{"@id":"unece:SpecifiedPeriod"},{"@id":"unece:OrganizationalCertificate"},{"@id":"unece:ProcessCertificate"},{"@id":"unece:ProductBatchCertificate"},{"@id":"unece:ProductCertificate"},{"@id":"unece:SpecifiedCertificate"},{"@id":"unece:AgriculturalCertificate"},{"@id":"unece:FieldCrop"}],"rdfs:comment":"A code specifying a purpose for this field crop."},{"@id":"unece:startDateFlexibilityCode","@type":["rdf:Property","owl:DatatypeProperty"],"rdfs:label":"startDateFlexibilityCode","schema:rangeIncludes":{"@id":"schema:Text"},"schema:domainIncludes":{"@id":"unece:SpecifiedPeriod"},"rdfs:comment":"The code specifying the flexibility of the start date of this specified period."},{"@id":"unece:startDayOfWeekCode","@type":["rdf:Property","owl:DatatypeProperty"],"rdfs:label":"startDayOfWeekCode","schema:rangeIncludes":{"@id":"schema:Text"},"schema:domainIncludes":{"@id":"unece:SpecifiedPeriod"},"rdfs:comment":"The code specifying the start day of the week for this specified period."},{"@id":"unece:componentDimension","@type":["rdf:Property","owl:ObjectProperty"],"rdfs:label":"componentDimension","schema:rangeIncludes":{"@id":"unece:WorkItemDimension"},"schema:domainIncludes":{"@id":"unece:WorkItemDimension"},"rdfs:comment":"A work item component dimension for this work item dimension."},{"@id":"unece:workItemDimensionTypeCode","@type":["rdf:Property","owl:DatatypeProperty"],"rdfs:label":"workItemDimensionTypeCode","schema:rangeIncludes":{"@id":"schema:Text"},"schema:domainIncludes":{"@id":"unece:WorkItemDimension"},"rdfs:comment":"The code specifying the type of this work item dimension."},{"@id":"unece:condition","@type":["rdf:Property","owl:DatatypeProperty"],"rdfs:label":"condition","schema:rangeIncludes":{"@id":"schema:Text"},"schema:domainIncludes":[{"@id":"unece:DocumentStatus"},{"@id":"unece:Guarantee"},{"@id":"unece:ProcessCharacteristic"},{"@id":"unece:OrganizationCharacteristic"}],"rdfs:comment":"A condition or status, expressed as text, for this process characteristic."},{"@id":"unece:documentStatusConditionCode","@type":["rdf:Property","owl:DatatypeProperty"],"rdfs:label":"documentStatusConditionCode","schema:rangeIncludes":{"@id":"unece:DocumentStatusCodeList"},"schema:domainIncludes":{"@id":"unece:DocumentStatus"},"rdfs:comment":"The code specifying the condition of this document status."},{"@id":"unece:documentStatusReasonCode","@type":["rdf:Property","owl:DatatypeProperty"],"rdfs:label":"documentStatusReasonCode","schema:rangeIncludes":{"@id":"schema:Text"},"schema:domainIncludes":{"@id":"unece:DocumentStatus"},"rdfs:comment":"A code specifying a reason for this document status."},{"@id":"unece:invalidInformation","@type":["rdf:Property","owl:DatatypeProperty"],"rdfs:label":"invalidInformation","schema:rangeIncludes":{"@id":"schema:Text"},"schema:domainIncludes":{"@id":"unece:DocumentStatus"},"rdfs:comment":"The invalid information, expressed as text, for this document status."},{"@id":"unece:reasonClassification","@type":["rdf:Property","owl:DatatypeProperty"],"rdfs:label":"reasonClassification","schema:rangeIncludes":{"@id":"schema:Text"},"schema:domainIncludes":{"@id":"unece:DocumentStatus"},"rdfs:comment":"A reason classification, expressed as text, for this document status."},{"@id":"unece:reasonClassificationCode","@type":["rdf:Property","owl:DatatypeProperty"],"rdfs:label":"reasonClassificationCode","schema:rangeIncludes":{"@id":"schema:Text"},"schema:domainIncludes":{"@id":"unece:DocumentStatus"},"rdfs:comment":"The code specifying the reason classification for this document status."},{"@id":"unece:reasonInformationCode","@type":["rdf:Property","owl:DatatypeProperty"],"rdfs:label":"reasonInformationCode","schema:rangeIncludes":{"@id":"schema:Text"},"schema:domainIncludes":{"@id":"unece:DocumentStatus"},"rdfs:comment":"The code specifying the reason for the information for this document status."},{"@id":"unece:requestedAction","@type":["rdf:Property","owl:DatatypeProperty"],"rdfs:label":"requestedAction","schema:rangeIncludes":{"@id":"schema:Text"},"schema:domainIncludes":{"@id":"unece:DocumentStatus"},"rdfs:comment":"A requested action, expressed as text, for this document status."},{"@id":"unece:requestedActionCode","@type":["rdf:Property","owl:DatatypeProperty"],"rdfs:label":"requestedActionCode","schema:rangeIncludes":{"@id":"schema:Text"},"schema:domainIncludes":[{"@id":"unece:DocumentStatus"},{"@id":"unece:BreakdownStatement"},{"@id":"unece:BasicWorkItem"},{"@id":"unece:GroupedWorkItem"}],"rdfs:comment":"A code specifying a requested action for this basic work item."},{"@id":"unece:specifiedDocumentCharacteristic","@type":["rdf:Property","owl:ObjectProperty"],"rdfs:label":"specifiedDocumentCharacteristic","schema:rangeIncludes":{"@id":"unece:DocumentCharacteristic"},"schema:domainIncludes":{"@id":"unece:DocumentStatus"},"rdfs:comment":"A document characteristic specified for this document status."},{"@id":"unece:validInformation","@type":["rdf:Property","owl:DatatypeProperty"],"rdfs:label":"validInformation","schema:rangeIncludes":{"@id":"schema:Text"},"schema:domainIncludes":{"@id":"unece:DocumentStatus"},"rdfs:comment":"The valid information, expressed as text, for this document status."},{"@id":"unece:constraintIndicator","@type":["rdf:Property","owl:DatatypeProperty"],"rdfs:label":"constraintIndicator","schema:rangeIncludes":{"@id":"schema:Boolean"},"schema:domainIncludes":{"@id":"unece:Project"},"rdfs:comment":"The indication of whether or not the project is constrained by an authority such as the World Trade Organization (WTO) for this procuring project."},{"@id":"unece:netBudgetAmount","@type":["rdf:Property","owl:ObjectProperty"],"rdfs:label":"netBudgetAmount","schema:rangeIncludes":{"@id":"unece:AmountType"},"schema:domainIncludes":{"@id":"unece:Project"},"rdfs:comment":"The monetary value of the net budget for this procuring project."},{"@id":"unece:subWorksTypeCode","@type":["rdf:Property","owl:DatatypeProperty"],"rdfs:label":"subWorksTypeCode","schema:rangeIncludes":{"@id":"schema:Text"},"schema:domainIncludes":{"@id":"unece:Project"},"rdfs:comment":"A code specifying the type of sub works, such as land surveying or information technology consulting, for this procuring project."},{"@id":"unece:totalBudgetAmount","@type":["rdf:Property","owl:ObjectProperty"],"rdfs:label":"totalBudgetAmount","schema:rangeIncludes":{"@id":"unece:AmountType"},"schema:domainIncludes":{"@id":"unece:Project"},"rdfs:comment":"The monetary value of the total budget which includes net amount, taxes, and material and instalment costs for this procuring project."},{"@id":"unece:worksTypeCode","@type":["rdf:Property","owl:DatatypeProperty"],"rdfs:label":"worksTypeCode","schema:rangeIncludes":{"@id":"schema:Text"},"schema:domainIncludes":{"@id":"unece:Project"},"rdfs:comment":"A code specifying the type of work, such as surveying or consulting, for this procuring project."},{"@id":"unece:contentCode","@type":["rdf:Property","owl:DatatypeProperty"],"rdfs:label":"contentCode","schema:rangeIncludes":{"@id":"schema:Text"},"schema:domainIncludes":[{"@id":"unece:Note"},{"@id":"unece:Marking"}],"rdfs:comment":"A code specifying the content of this note."},{"@id":"unece:noteSubjectCode","@type":["rdf:Property","owl:DatatypeProperty"],"rdfs:label":"noteSubjectCode","schema:rangeIncludes":{"@id":"schema:Text"},"schema:domainIncludes":{"@id":"unece:Note"},"rdfs:comment":"A code specifying the subject of this note."},{"@id":"unece:queryId","@type":["rdf:Property","owl:DatatypeProperty"],"rdfs:label":"queryId","schema:rangeIncludes":{"@id":"schema:Text"},"schema:domainIncludes":{"@id":"unece:Response"},"rdfs:comment":"The unique identifier for the query to which this response refers."},{"@id":"unece:responseTypeCode","@type":["rdf:Property","owl:DatatypeProperty"],"rdfs:label":"responseTypeCode","schema:rangeIncludes":{"@id":"unece:ResponseTypeCodeList"},"schema:domainIncludes":{"@id":"unece:Response"},"rdfs:comment":"The code specifying the type of this specification response."},{"@id":"unece:latestResponseDateTime","@type":["rdf:Property","owl:DatatypeProperty"],"rdfs:label":"latestResponseDateTime","schema:rangeIncludes":{"@id":"schema:DateTime"},"schema:domainIncludes":{"@id":"unece:SpecialQuery"},"rdfs:comment":"The date, time, date time, or other date time value for the latest response to this special query."},{"@id":"unece:responseStatusCode","@type":["rdf:Property","owl:DatatypeProperty"],"rdfs:label":"responseStatusCode","schema:rangeIncludes":{"@id":"schema:Text"},"schema:domainIncludes":[{"@id":"unece:SpecialQuery"},{"@id":"unece:ExperienceItem"}],"rdfs:comment":"The code specifying the response status for this special query."},{"@id":"unece:submittedDateTime","@type":["rdf:Property","owl:DatatypeProperty"],"rdfs:label":"submittedDateTime","schema:rangeIncludes":{"@id":"schema:DateTime"},"schema:domainIncludes":{"@id":"unece:SpecialQuery"},"rdfs:comment":"The date, time, date time, or other date time value when this special query was submitted."},{"@id":"unece:submittingPersonName","@type":["rdf:Property","owl:DatatypeProperty"],"rdfs:label":"submittingPersonName","schema:rangeIncludes":{"@id":"schema:Text"},"schema:domainIncludes":{"@id":"unece:SpecialQuery"},"rdfs:comment":"The name, expressed as text, of the person submitting this special query."},{"@id":"unece:subjectCode","@type":["rdf:Property","owl:DatatypeProperty"],"rdfs:label":"subjectCode","schema:rangeIncludes":{"@id":"schema:Text"},"schema:domainIncludes":{"@id":"unece:SpecifiedNote"},"rdfs:comment":"The code specifying the subject of this specified note."},{"@id":"unece:contentTypeCode","@type":["rdf:Property","owl:DatatypeProperty"],"rdfs:label":"contentTypeCode","schema:rangeIncludes":{"@id":"schema:Text"},"schema:domainIncludes":[{"@id":"unece:MetricCharacteristic"},{"@id":"unece:ProductCharacteristic"},{"@id":"unece:SustainabilityCharacteristic"}],"rdfs:comment":"A code specifying the content type of this product characteristic."},{"@id":"unece:value","@type":["rdf:Property","owl:DatatypeProperty"],"rdfs:label":"value","schema:rangeIncludes":{"@id":"schema:Text"},"schema:domainIncludes":[{"@id":"unece:MetricCharacteristic"},{"@id":"unece:DocumentCharacteristic"},{"@id":"unece:SpecifiedParameter"},{"@id":"unece:Range"},{"@id":"unece:DocumentContextParameter"},{"@id":"unece:InspectionReference"},{"@id":"unece:LaboratoryObservationReference"},{"@id":"unece:ProductCharacteristic"},{"@id":"unece:ProductBatchCharacteristic"},{"@id":"unece:SustainabilityCharacteristic"},{"@id":"unece:ProcessCharacteristic"},{"@id":"unece:TechnicalCharacteristic"},{"@id":"unece:ControlSettingParameter"},{"@id":"unece:OperationalParameter"},{"@id":"unece:ObservationObjectiveParameter"},{"@id":"unece:OrganizationCharacteristic"},{"@id":"unece:AgriculturalCharacteristic"},{"@id":"unece:SupplyChainReference"}],"rdfs:comment":"A value, expressed as text, for this document characteristic."},{"@id":"unece:valueAmount","@type":["rdf:Property","owl:ObjectProperty"],"rdfs:label":"valueAmount","schema:rangeIncludes":{"@id":"unece:AmountType"},"schema:domainIncludes":[{"@id":"unece:MetricCharacteristic"},{"@id":"unece:DocumentCharacteristic"},{"@id":"unece:ProductCharacteristic"},{"@id":"unece:ProductBatchCharacteristic"},{"@id":"unece:SustainabilityCharacteristic"},{"@id":"unece:ProcessCharacteristic"},{"@id":"unece:TechnicalCharacteristic"},{"@id":"unece:OrganizationCharacteristic"},{"@id":"unece:AgriculturalCharacteristic"}],"rdfs:comment":"A value, expressed as a monetary value, for this document characteristic."},{"@id":"unece:valueCode","@type":["rdf:Property","owl:DatatypeProperty"],"rdfs:label":"valueCode","schema:rangeIncludes":{"@id":"schema:Text"},"schema:domainIncludes":[{"@id":"unece:MetricCharacteristic"},{"@id":"unece:DocumentCharacteristic"},{"@id":"unece:Range"},{"@id":"unece:InspectionReference"},{"@id":"unece:LaboratoryObservationReference"},{"@id":"unece:ProductBatchCharacteristic"},{"@id":"unece:SustainabilityCharacteristic"},{"@id":"unece:ProcessCharacteristic"},{"@id":"unece:TechnicalCharacteristic"},{"@id":"unece:CalibratedMeasurement"},{"@id":"unece:OrganizationCharacteristic"},{"@id":"unece:AgriculturalCharacteristic"},{"@id":"unece:SupplyChainReference"}],"rdfs:comment":"A code specifying a value for this specified range."},{"@id":"unece:valueDateTime","@type":["rdf:Property","owl:DatatypeProperty"],"rdfs:label":"valueDateTime","schema:rangeIncludes":{"@id":"schema:Text"},"schema:domainIncludes":[{"@id":"unece:MetricCharacteristic"},{"@id":"unece:DocumentCharacteristic"},{"@id":"unece:ProductCharacteristic"},{"@id":"unece:ProductBatchCharacteristic"},{"@id":"unece:SustainabilityCharacteristic"},{"@id":"unece:ProcessCharacteristic"},{"@id":"unece:TechnicalCharacteristic"},{"@id":"unece:OrganizationCharacteristic"},{"@id":"unece:AgriculturalCharacteristic"}],"rdfs:comment":"A date, time, date time or other date time value for this document characteristic."},{"@id":"unece:valueIndicator","@type":["rdf:Property","owl:DatatypeProperty"],"rdfs:label":"valueIndicator","schema:rangeIncludes":{"@id":"schema:Boolean"},"schema:domainIncludes":[{"@id":"unece:MetricCharacteristic"},{"@id":"unece:ProductCharacteristic"},{"@id":"unece:ProductBatchCharacteristic"},{"@id":"unece:SustainabilityCharacteristic"},{"@id":"unece:ProcessCharacteristic"},{"@id":"unece:TechnicalCharacteristic"},{"@id":"unece:OrganizationCharacteristic"},{"@id":"unece:AgriculturalCharacteristic"}],"rdfs:comment":"The value for this metric characteristic expressed as an indicator."},{"@id":"unece:valueMethod","@type":["rdf:Property","owl:ObjectProperty"],"rdfs:label":"valueMethod","schema:rangeIncludes":{"@id":"unece:SpecifiedMethod"},"schema:domainIncludes":[{"@id":"unece:MetricCharacteristic"},{"@id":"unece:ProductCharacteristic"},{"@id":"unece:ProductBatchCharacteristic"},{"@id":"unece:ProcessCharacteristic"},{"@id":"unece:OrganizationCharacteristic"},{"@id":"unece:AgriculturalCharacteristic"}],"rdfs:comment":"A method specified for a value of this metric characteristic."},{"@id":"unece:valueNumeric","@type":["rdf:Property","owl:DatatypeProperty"],"rdfs:label":"valueNumeric","schema:rangeIncludes":{"@id":"schema:Text"},"schema:domainIncludes":[{"@id":"unece:MetricCharacteristic"},{"@id":"unece:DocumentCharacteristic"},{"@id":"unece:ProductCharacteristic"},{"@id":"unece:ProductBatchCharacteristic"},{"@id":"unece:SustainabilityCharacteristic"},{"@id":"unece:ProcessCharacteristic"},{"@id":"unece:TechnicalCharacteristic"},{"@id":"unece:OrganizationCharacteristic"},{"@id":"unece:AgriculturalCharacteristic"}],"rdfs:comment":"A value, expressed as a number, for this document characteristic."},{"@id":"unece:valueParameter","@type":["rdf:Property","owl:ObjectProperty"],"rdfs:label":"valueParameter","schema:rangeIncludes":{"@id":"unece:SpecifiedParameter"},"schema:domainIncludes":[{"@id":"unece:MetricCharacteristic"},{"@id":"unece:ProductCharacteristic"},{"@id":"unece:ProductBatchCharacteristic"},{"@id":"unece:SustainabilityCharacteristic"},{"@id":"unece:ProcessCharacteristic"},{"@id":"unece:TechnicalCharacteristic"},{"@id":"unece:OrganizationCharacteristic"},{"@id":"unece:AgriculturalCharacteristic"}],"rdfs:comment":"A parameter specified for a value for this metric characteristic."},{"@id":"unece:valueQuantity","@type":["rdf:Property","owl:ObjectProperty"],"rdfs:label":"valueQuantity","schema:rangeIncludes":{"@id":"unece:QuantityType"},"schema:domainIncludes":[{"@id":"unece:MetricCharacteristic"},{"@id":"unece:DocumentCharacteristic"}],"rdfs:comment":"A value, expressed as a quantity, for this document characteristic."},{"@id":"unece:valueRange","@type":["rdf:Property","owl:ObjectProperty"],"rdfs:label":"valueRange","schema:rangeIncludes":{"@id":"unece:Range"},"schema:domainIncludes":[{"@id":"unece:MetricCharacteristic"},{"@id":"unece:ProductCharacteristic"},{"@id":"unece:ProductBatchCharacteristic"},{"@id":"unece:SustainabilityCharacteristic"},{"@id":"unece:ProcessCharacteristic"},{"@id":"unece:TechnicalCharacteristic"},{"@id":"unece:OrganizationCharacteristic"},{"@id":"unece:AgriculturalCharacteristic"}],"rdfs:comment":"A range specified for a value of this metric characteristic."},{"@id":"unece:valueTolerance","@type":["rdf:Property","owl:ObjectProperty"],"rdfs:label":"valueTolerance","schema:rangeIncludes":{"@id":"unece:Tolerance"},"schema:domainIncludes":[{"@id":"unece:MetricCharacteristic"},{"@id":"unece:SpecifiedParameter"},{"@id":"unece:ProductCharacteristic"},{"@id":"unece:ProductBatchCharacteristic"},{"@id":"unece:SustainabilityCharacteristic"},{"@id":"unece:ProcessCharacteristic"},{"@id":"unece:TechnicalCharacteristic"},{"@id":"unece:OrganizationCharacteristic"},{"@id":"unece:AgriculturalCharacteristic"}],"rdfs:comment":"A tolerance specified for a value of this metric characteristic."},{"@id":"unece:countryId","@type":["rdf:Property","owl:DatatypeProperty"],"rdfs:label":"countryId","schema:rangeIncludes":{"@id":"schema:Text"},"schema:domainIncludes":[{"@id":"unece:Country"},{"@id":"unece:LegalRegistration"},{"@id":"unece:FinancialInstitutionAddress"},{"@id":"unece:GovernmentRegistration"},{"@id":"unece:LocationParty"}],"rdfs:comment":"A unique country identifier for this location party."},{"@id":"unece:lastRegisteredYearDateTime","@type":["rdf:Property","owl:DatatypeProperty"],"rdfs:label":"lastRegisteredYearDateTime","schema:rangeIncludes":{"@id":"schema:Text"},"schema:domainIncludes":[{"@id":"unece:LegalRegistration"},{"@id":"unece:GovernmentRegistration"}],"rdfs:comment":"The last registered year of this government registration."},{"@id":"unece:location","@type":["rdf:Property","owl:DatatypeProperty"],"rdfs:label":"location","schema:rangeIncludes":{"@id":"schema:Text"},"schema:domainIncludes":[{"@id":"unece:DocumentCharacteristic"},{"@id":"unece:ExperienceProduct"},{"@id":"unece:ExperienceEvent"},{"@id":"unece:SanitaryMeasure"}],"rdfs:comment":"A location, expressed as text, for this MDH sanitary measure."},{"@id":"unece:valueAdjustmentDirectionCode","@type":["rdf:Property","owl:DatatypeProperty"],"rdfs:label":"valueAdjustmentDirectionCode","schema:rangeIncludes":{"@id":"schema:Text"},"schema:domainIncludes":{"@id":"unece:DocumentCharacteristic"},"rdfs:comment":"The code specifying the adjustment direction for value of this document characteristic."},{"@id":"unece:valueChangedIndicator","@type":["rdf:Property","owl:DatatypeProperty"],"rdfs:label":"valueChangedIndicator","schema:rangeIncludes":{"@id":"schema:Boolean"},"schema:domainIncludes":{"@id":"unece:DocumentCharacteristic"},"rdfs:comment":"The indication of whether or not the value of this document characteristic is changed."},{"@id":"unece:valuePercent","@type":["rdf:Property","owl:DatatypeProperty"],"rdfs:label":"valuePercent","schema:rangeIncludes":{"@id":"schema:Text"},"schema:domainIncludes":{"@id":"unece:DocumentCharacteristic"},"rdfs:comment":"A value, expressed as a percentage, for this document characteristic."},{"@id":"unece:descriptionReference","@type":["rdf:Property","owl:DatatypeProperty"],"rdfs:label":"descriptionReference","schema:rangeIncludes":{"@id":"schema:Text"},"schema:domainIncludes":{"@id":"unece:GeographicalObjectCharacteristic"},"rdfs:comment":"The description reference, expressed as text, for this geographical object characteristic."},{"@id":"unece:geometryCollectionIndicator","@type":["rdf:Property","owl:DatatypeProperty"],"rdfs:label":"geometryCollectionIndicator","schema:rangeIncludes":{"@id":"schema:Boolean"},"schema:domainIncludes":{"@id":"unece:GeographicalObjectCharacteristic"},"rdfs:comment":"The indication of whether or not this geographical object can be characterized as a geometry collection."},{"@id":"unece:physicalIndicator","@type":["rdf:Property","owl:DatatypeProperty"],"rdfs:label":"physicalIndicator","schema:rangeIncludes":{"@id":"schema:Boolean"},"schema:domainIncludes":{"@id":"unece:GeographicalObjectCharacteristic"},"rdfs:comment":"The indication of whether or not this geographical object can be characterized as physical."},{"@id":"unece:relevantGeometryType","@type":["rdf:Property","owl:DatatypeProperty"],"rdfs:label":"relevantGeometryType","schema:rangeIncludes":{"@id":"schema:Text"},"schema:domainIncludes":{"@id":"unece:GeographicalObjectCharacteristic"},"rdfs:comment":"The type of geometry, expressed as text, relevant for this geographical object characteristic."},{"@id":"unece:shapeType","@type":["rdf:Property","owl:DatatypeProperty"],"rdfs:label":"shapeType","schema:rangeIncludes":{"@id":"schema:Text"},"schema:domainIncludes":{"@id":"unece:GeographicalObjectCharacteristic"},"rdfs:comment":"The type of shape, expressed as text, such as a semi-circle, for this geographical object characteristic."},{"@id":"unece:identificationCode","@type":["rdf:Property","owl:DatatypeProperty"],"rdfs:label":"identificationCode","schema:rangeIncludes":{"@id":"schema:Text"},"schema:domainIncludes":{"@id":"unece:IdentifiedFault"},"rdfs:comment":"A code specifying an identified fault."},{"@id":"unece:dimensionTypeCode","@type":["rdf:Property","owl:DatatypeProperty"],"rdfs:label":"dimensionTypeCode","schema:rangeIncludes":{"@id":"unece:DimensionTypeCodeList"},"schema:domainIncludes":{"@id":"unece:SpatialDimension"},"rdfs:comment":"The code specifying the type of spatial dimension, such as thickness, area, or volume."},{"@id":"unece:heightMeasure","@type":["rdf:Property","owl:ObjectProperty"],"rdfs:label":"heightMeasure","schema:rangeIncludes":{"@id":"unece:MeasureType"},"schema:domainIncludes":{"@id":"unece:SpatialDimension"},"rdfs:comment":"The measure of the height component of this spatial dimension."},{"@id":"unece:lengthMeasure","@type":["rdf:Property","owl:ObjectProperty"],"rdfs:label":"lengthMeasure","schema:rangeIncludes":{"@id":"unece:MeasureType"},"schema:domainIncludes":{"@id":"unece:SpatialDimension"},"rdfs:comment":"The measure of the length component of this spatial dimension."},{"@id":"unece:linearUnitDiameterMeasure","@type":["rdf:Property","owl:ObjectProperty"],"rdfs:label":"linearUnitDiameterMeasure","schema:rangeIncludes":{"@id":"unece:LinearUnitMeasureType"},"schema:domainIncludes":{"@id":"unece:SpatialDimension"},"rdfs:comment":"The measure of the diameter component for this spatial dimension."},{"@id":"unece:widthMeasure","@type":["rdf:Property","owl:ObjectProperty"],"rdfs:label":"widthMeasure","schema:rangeIncludes":{"@id":"unece:MeasureType"},"schema:domainIncludes":{"@id":"unece:SpatialDimension"},"rdfs:comment":"The measure of the width component of this spatial dimension."},{"@id":"unece:keywordMarketingPhrase","@type":["rdf:Property","owl:DatatypeProperty"],"rdfs:label":"keywordMarketingPhrase","schema:rangeIncludes":{"@id":"schema:Text"},"schema:domainIncludes":{"@id":"unece:SpecifiedFeature"},"rdfs:comment":"A keyword marketing phrase, expressed as text, for this feature."},{"@id":"unece:objective","@type":["rdf:Property","owl:DatatypeProperty"],"rdfs:label":"objective","schema:rangeIncludes":{"@id":"schema:Text"},"schema:domainIncludes":[{"@id":"unece:SpecifiedFeature"},{"@id":"unece:ExperienceProduct"}],"rdfs:comment":"An objective, expressed as text, for this experience product."},{"@id":"unece:usageCode","@type":["rdf:Property","owl:DatatypeProperty"],"rdfs:label":"usageCode","schema:rangeIncludes":{"@id":"schema:Text"},"schema:domainIncludes":{"@id":"unece:SpecifiedFeature"},"rdfs:comment":"The code specifying the usage for this specified feature."},{"@id":"unece:directions","@type":["rdf:Property","owl:DatatypeProperty"],"rdfs:label":"directions","schema:rangeIncludes":{"@id":"schema:Text"},"schema:domainIncludes":{"@id":"unece:SpecifiedLocation"},"rdfs:comment":"Directions, expressed as text, for this specified location."},{"@id":"unece:geopoliticalRegionCode","@type":["rdf:Property","owl:DatatypeProperty"],"rdfs:label":"geopoliticalRegionCode","schema:rangeIncludes":{"@id":"schema:Text"},"schema:domainIncludes":{"@id":"unece:SpecifiedLocation"},"rdfs:comment":"The code specifying the geopolitical region for this specified location."},{"@id":"unece:geopoliticalRegionName","@type":["rdf:Property","owl:DatatypeProperty"],"rdfs:label":"geopoliticalRegionName","schema:rangeIncludes":{"@id":"schema:Text"},"schema:domainIncludes":{"@id":"unece:SpecifiedLocation"},"rdfs:comment":"The name, expressed as text, of the geopolitical region for this specified location."},{"@id":"unece:mapURIId","@type":["rdf:Property","owl:DatatypeProperty"],"rdfs:label":"mapURIId","schema:rangeIncludes":{"@id":"schema:Text"},"schema:domainIncludes":[{"@id":"unece:SpecifiedLocation"},{"@id":"unece:SpecifiedRoute"}],"rdfs:comment":"The Uniform Resource Identifier (URI) of the map of this specified route."},{"@id":"unece:specifiedLocationTypeCode","@type":["rdf:Property","owl:DatatypeProperty"],"rdfs:label":"specifiedLocationTypeCode","schema:rangeIncludes":{"@id":"schema:Text"},"schema:domainIncludes":{"@id":"unece:SpecifiedLocation"},"rdfs:comment":"The code specifying the type of this specified location."},{"@id":"unece:specifiedTradeAddress","@type":["rdf:Property","owl:ObjectProperty"],"rdfs:label":"specifiedTradeAddress","schema:rangeIncludes":{"@id":"unece:Address"},"schema:domainIncludes":{"@id":"unece:SpecifiedLocation"},"rdfs:comment":"A address specified for this location."},{"@id":"unece:parameterType","@type":["rdf:Property","owl:DatatypeProperty"],"rdfs:label":"parameterType","schema:rangeIncludes":{"@id":"schema:Text"},"schema:domainIncludes":[{"@id":"unece:SpecifiedParameter"},{"@id":"unece:ObservationObjectiveParameter"}],"rdfs:comment":"A type, expressed as text, for this observation objective parameter."},{"@id":"unece:statusValueMeasure","@type":["rdf:Property","owl:ObjectProperty"],"rdfs:label":"statusValueMeasure","schema:rangeIncludes":{"@id":"unece:MeasureType"},"schema:domainIncludes":[{"@id":"unece:SpecifiedParameter"},{"@id":"unece:ObservationObjectiveParameter"}],"rdfs:comment":"A measure of a value of the status for this specified parameter."},{"@id":"unece:valueAllowedIndicator","@type":["rdf:Property","owl:DatatypeProperty"],"rdfs:label":"valueAllowedIndicator","schema:rangeIncludes":{"@id":"schema:Boolean"},"schema:domainIncludes":[{"@id":"unece:SpecifiedParameter"},{"@id":"unece:ControlSettingParameter"},{"@id":"unece:OperationalParameter"},{"@id":"unece:ObservationObjectiveParameter"}],"rdfs:comment":"The indication of whether or not the value for this specified parameter is allowed."},{"@id":"unece:endId","@type":["rdf:Property","owl:DatatypeProperty"],"rdfs:label":"endId","schema:rangeIncludes":{"@id":"schema:Text"},"schema:domainIncludes":{"@id":"unece:Range"},"rdfs:comment":"The identifier of the end of this specified range."},{"@id":"unece:maximumValueMeasure","@type":["rdf:Property","owl:ObjectProperty"],"rdfs:label":"maximumValueMeasure","schema:rangeIncludes":{"@id":"unece:MeasureType"},"schema:domainIncludes":[{"@id":"unece:Range"},{"@id":"unece:SpecifiedTemperature"},{"@id":"unece:SustainabilityCharacteristic"},{"@id":"unece:ProcessCharacteristic"},{"@id":"unece:InstructedTemperature"},{"@id":"unece:TransportSettingTemperature"}],"rdfs:comment":"A measure of a maximum value for this sustainability characteristic."},{"@id":"unece:minimumValueMeasure","@type":["rdf:Property","owl:ObjectProperty"],"rdfs:label":"minimumValueMeasure","schema:rangeIncludes":{"@id":"unece:MeasureType"},"schema:domainIncludes":[{"@id":"unece:Range"},{"@id":"unece:SpecifiedTemperature"},{"@id":"unece:SustainabilityCharacteristic"},{"@id":"unece:ProcessCharacteristic"},{"@id":"unece:InstructedTemperature"},{"@id":"unece:TransportSettingTemperature"}],"rdfs:comment":"A measure of a minimum value for this sustainability characteristic."},{"@id":"unece:startId","@type":["rdf:Property","owl:DatatypeProperty"],"rdfs:label":"startId","schema:rangeIncludes":{"@id":"schema:Text"},"schema:domainIncludes":{"@id":"unece:Range"},"rdfs:comment":"The identifier of the start of this specified range."},{"@id":"unece:totalItemQuantity","@type":["rdf:Property","owl:ObjectProperty"],"rdfs:label":"totalItemQuantity","schema:rangeIncludes":{"@id":"unece:QuantityType"},"schema:domainIncludes":{"@id":"unece:Range"},"rdfs:comment":"The total number of items in this specified range."},{"@id":"unece:valueBaseSystemCode","@type":["rdf:Property","owl:DatatypeProperty"],"rdfs:label":"valueBaseSystemCode","schema:rangeIncludes":{"@id":"schema:Text"},"schema:domainIncludes":{"@id":"unece:Range"},"rdfs:comment":"The code specifying the value base system, such as Arabic numerals, for this specified range."},{"@id":"unece:identificationType","@type":["rdf:Property","owl:DatatypeProperty"],"rdfs:label":"identificationType","schema:rangeIncludes":{"@id":"schema:Text"},"schema:domainIncludes":{"@id":"unece:ProprietaryIdentity"},"rdfs:comment":"An identifier type, expressed as text, for this proprietary identity."},{"@id":"unece:level","@type":["rdf:Property","owl:DatatypeProperty"],"rdfs:label":"level","schema:rangeIncludes":{"@id":"schema:Text"},"schema:domainIncludes":{"@id":"unece:CoordinateReferenceSystem"},"rdfs:comment":"The level, expressed as text, of this CS engineering coordinate reference system."},{"@id":"unece:subordinateCoordinateReferenceSystem","@type":["rdf:Property","owl:ObjectProperty"],"rdfs:label":"subordinateCoordinateReferenceSystem","schema:rangeIncludes":{"@id":"unece:CoordinateReferenceSystem"},"schema:domainIncludes":{"@id":"unece:CoordinateReferenceSystem"},"rdfs:comment":"A CS engineering coordinate reference system subordinate to this CS engineering coordinate reference system."},{"@id":"unece:signalSourceAvailableQuantity","@type":["rdf:Property","owl:ObjectProperty"],"rdfs:label":"signalSourceAvailableQuantity","schema:rangeIncludes":{"@id":"unece:QuantityType"},"schema:domainIncludes":{"@id":"unece:CoordinateSourceSystem"},"rdfs:comment":"The quantity of signal source available for this geographical coordinate source system."},{"@id":"unece:sourceTypeCode","@type":["rdf:Property","owl:DatatypeProperty"],"rdfs:label":"sourceTypeCode","schema:rangeIncludes":{"@id":"schema:Text"},"schema:domainIncludes":{"@id":"unece:CoordinateSourceSystem"},"rdfs:comment":"The code specifying a type of source for this geographical coordinate source system."},{"@id":"unece:toleranceMeasure","@type":["rdf:Property","owl:ObjectProperty"],"rdfs:label":"toleranceMeasure","schema:rangeIncludes":{"@id":"unece:MeasureType"},"schema:domainIncludes":[{"@id":"unece:CoordinateSourceSystem"},{"@id":"unece:CalibratedMeasurement"}],"rdfs:comment":"The measure of the tolerance of this calibrated measurement."},{"@id":"unece:usedSignalSourceQuantity","@type":["rdf:Property","owl:ObjectProperty"],"rdfs:label":"usedSignalSourceQuantity","schema:rangeIncludes":{"@id":"unece:QuantityType"},"schema:domainIncludes":{"@id":"unece:CoordinateSourceSystem"},"rdfs:comment":"The quantity of the used signal source of this geographical coordinate source system."},{"@id":"unece:specifiedVersion","@type":["rdf:Property","owl:ObjectProperty"],"rdfs:label":"specifiedVersion","schema:rangeIncludes":{"@id":"unece:Version"},"schema:domainIncludes":{"@id":"unece:DocumentContextParameter"},"rdfs:comment":"The document version specified for this document context parameter."},{"@id":"unece:includedCountry","@type":["rdf:Property","owl:ObjectProperty"],"rdfs:label":"includedCountry","schema:rangeIncludes":{"@id":"unece:Country"},"schema:domainIncludes":{"@id":"unece:GeopoliticalRegion"},"rdfs:comment":"A country included in this trade geopolitical region."},{"@id":"unece:maximumSpecifiedCharacteristic","@type":["rdf:Property","owl:ObjectProperty"],"rdfs:label":"maximumSpecifiedCharacteristic","schema:rangeIncludes":{"@id":"unece:MetricCharacteristic"},"schema:domainIncludes":{"@id":"unece:Issue"},"rdfs:comment":"The maximum metric characteristic specified for this target issue."},{"@id":"unece:minimumSpecifiedCharacteristic","@type":["rdf:Property","owl:ObjectProperty"],"rdfs:label":"minimumSpecifiedCharacteristic","schema:rangeIncludes":{"@id":"unece:MetricCharacteristic"},"schema:domainIncludes":{"@id":"unece:Issue"},"rdfs:comment":"The minimum metric characteristic specified for this target issue."},{"@id":"unece:specifiedMetricCharacteristic","@type":["rdf:Property","owl:ObjectProperty"],"rdfs:label":"specifiedMetricCharacteristic","schema:rangeIncludes":{"@id":"unece:MetricCharacteristic"},"schema:domainIncludes":{"@id":"unece:Issue"},"rdfs:comment":"The metric characteristic specified for this target issue."},{"@id":"unece:lowDispersibleStatusIndicator","@type":["rdf:Property","owl:DatatypeProperty"],"rdfs:label":"lowDispersibleStatusIndicator","schema:rangeIncludes":{"@id":"schema:Boolean"},"schema:domainIncludes":{"@id":"unece:Radionuclide"},"rdfs:comment":"The indication of whether or not this radioactive radionuclide has a low dispersible status."},{"@id":"unece:specialFormIndicator","@type":["rdf:Property","owl:DatatypeProperty"],"rdfs:label":"specialFormIndicator","schema:rangeIncludes":{"@id":"schema:Boolean"},"schema:domainIncludes":{"@id":"unece:Radionuclide"},"rdfs:comment":"The indication of whether or not this radioactive radionuclide has a special form."},{"@id":"unece:includedSegment","@type":["rdf:Property","owl:ObjectProperty"],"rdfs:label":"includedSegment","schema:rangeIncludes":{"@id":"unece:Segment"},"schema:domainIncludes":{"@id":"unece:Section"},"rdfs:comment":"A segment included in this label section."},{"@id":"unece:patternCode","@type":["rdf:Property","owl:DatatypeProperty"],"rdfs:label":"patternCode","schema:rangeIncludes":{"@id":"schema:Text"},"schema:domainIncludes":{"@id":"unece:Section"},"rdfs:comment":"The code specifying the pattern of this label section."},{"@id":"unece:imageBinaryObject","@type":["rdf:Property","owl:DatatypeProperty"],"rdfs:label":"imageBinaryObject","schema:rangeIncludes":{"@id":"schema:Text"},"schema:domainIncludes":{"@id":"unece:Segment"},"rdfs:comment":"The image, expressed as a binary object, for this section segment."},{"@id":"unece:physicalGeographicalCoordinate","@type":["rdf:Property","owl:ObjectProperty"],"rdfs:label":"physicalGeographicalCoordinate","schema:rangeIncludes":{"@id":"unece:GeographicalCoordinate"},"schema:domainIncludes":[{"@id":"unece:SubordinateLocation"},{"@id":"unece:SubordinateSubordinateLocation"},{"@id":"unece:LogisticsLocation"}],"rdfs:comment":"Geographical coordinate information for this logistics related location."},{"@id":"unece:subordinateSubordinateSubordinateLocation","@type":["rdf:Property","owl:ObjectProperty"],"rdfs:label":"subordinateSubordinateSubordinateLocation","schema:rangeIncludes":{"@id":"unece:SubordinateSubordinateLocation"},"schema:domainIncludes":{"@id":"unece:SubordinateLocation"},"rdfs:comment":"The location subordinate to this subordinate location."},{"@id":"unece:previousStatusCode","@type":["rdf:Property","owl:DatatypeProperty"],"rdfs:label":"previousStatusCode","schema:rangeIncludes":{"@id":"unece:WorkflowStatusCodeList"},"schema:domainIncludes":{"@id":"unece:WorkflowObject"},"rdfs:comment":"The code specifying the previous status of this trade workflow object."},{"@id":"unece:workflowStatusCode","@type":["rdf:Property","owl:DatatypeProperty"],"rdfs:label":"workflowStatusCode","schema:rangeIncludes":{"@id":"unece:WorkflowStatusCodeList"},"schema:domainIncludes":{"@id":"unece:WorkflowObject"},"rdfs:comment":"The code specifying the status of this trade workflow object."},{"@id":"unece:languageName","@type":["rdf:Property","owl:DatatypeProperty"],"rdfs:label":"languageName","schema:rangeIncludes":{"@id":"schema:Text"},"schema:domainIncludes":{"@id":"unece:LanguageProficiency"},"rdfs:comment":"A name, expressed as text, of the language for which this language proficiency is defined."},{"@id":"unece:personalLanguageProficiencyLanguageCode","@type":["rdf:Property","owl:DatatypeProperty"],"rdfs:label":"personalLanguageProficiencyLanguageCode","schema:rangeIncludes":{"@id":"unece:LanguageCodeList"},"schema:domainIncludes":{"@id":"unece:LanguageProficiency"},"rdfs:comment":"The code specifying the language for this personal language proficiency."},{"@id":"unece:personalLanguageProficiencyLanguageId","@type":["rdf:Property","owl:DatatypeProperty"],"rdfs:label":"personalLanguageProficiencyLanguageId","schema:rangeIncludes":{"@id":"unece:LanguageId"},"schema:domainIncludes":{"@id":"unece:LanguageProficiency"},"rdfs:comment":"The identifier of the language for which this personal language proficiency is defined."},{"@id":"unece:readingLevelCode","@type":["rdf:Property","owl:DatatypeProperty"],"rdfs:label":"readingLevelCode","schema:rangeIncludes":{"@id":"schema:Text"},"schema:domainIncludes":{"@id":"unece:LanguageProficiency"},"rdfs:comment":"The code specifying the personal reading proficiency level in this language."},{"@id":"unece:speakingLevelCode","@type":["rdf:Property","owl:DatatypeProperty"],"rdfs:label":"speakingLevelCode","schema:rangeIncludes":{"@id":"schema:Text"},"schema:domainIncludes":{"@id":"unece:LanguageProficiency"},"rdfs:comment":"The code specifying the personal speaking proficiency level in this language."},{"@id":"unece:writingLevelCode","@type":["rdf:Property","owl:DatatypeProperty"],"rdfs:label":"writingLevelCode","schema:rangeIncludes":{"@id":"schema:Text"},"schema:domainIncludes":{"@id":"unece:LanguageProficiency"},"rdfs:comment":"The code specifying the personal writing proficiency level in this language."},{"@id":"unece:locationCode","@type":["rdf:Property","owl:DatatypeProperty"],"rdfs:label":"locationCode","schema:rangeIncludes":{"@id":"schema:Text"},"schema:domainIncludes":{"@id":"unece:SecurityTag"},"rdfs:comment":"The code specifying the location of this product security tag."},{"@id":"unece:matchingEvent","@type":["rdf:Property","owl:ObjectProperty"],"rdfs:label":"matchingEvent","schema:rangeIncludes":{"@id":"unece:CommunicationEvent"},"schema:domainIncludes":{"@id":"unece:Pairing"},"rdfs:comment":"A matching event for this communication pairing."},{"@id":"unece:methodCode","@type":["rdf:Property","owl:DatatypeProperty"],"rdfs:label":"methodCode","schema:rangeIncludes":{"@id":"schema:Text"},"schema:domainIncludes":[{"@id":"unece:Pairing"},{"@id":"unece:CustomsValuation"}],"rdfs:comment":"The code specifying the method by which this cross-border customs valuation is determined."},{"@id":"unece:pairedIndicator","@type":["rdf:Property","owl:DatatypeProperty"],"rdfs:label":"pairedIndicator","schema:rangeIncludes":{"@id":"schema:Boolean"},"schema:domainIncludes":{"@id":"unece:Pairing"},"rdfs:comment":"The indication of whether or not the entity is paired in this communication pairing."},{"@id":"unece:targetEntityId","@type":["rdf:Property","owl:DatatypeProperty"],"rdfs:label":"targetEntityId","schema:rangeIncludes":{"@id":"schema:Text"},"schema:domainIncludes":{"@id":"unece:Pairing"},"rdfs:comment":"The identifier of the target entity for this communication pairing."},{"@id":"unece:temperatureUnitValueMeasure","@type":["rdf:Property","owl:ObjectProperty"],"rdfs:label":"temperatureUnitValueMeasure","schema:rangeIncludes":{"@id":"unece:TemperatureUnitMeasureType"},"schema:domainIncludes":[{"@id":"unece:SpecifiedTemperature"},{"@id":"unece:TransportSettingTemperature"}],"rdfs:comment":"The measure of the value of this specified temperature, such as a temperature value of ten degrees Celsius."},{"@id":"unece:roleCode","@type":["rdf:Property","owl:DatatypeProperty"],"rdfs:label":"roleCode","schema:rangeIncludes":{"@id":"schema:Text"},"schema:domainIncludes":[{"@id":"unece:CooperatingOrganization"},{"@id":"unece:PaymentFinancialInstitution"},{"@id":"unece:GuestPerson"}],"rdfs:comment":"The code specifying the role for this cooperating organization."},{"@id":"unece:usedInformationSource","@type":["rdf:Property","owl:ObjectProperty"],"rdfs:label":"usedInformationSource","schema:rangeIncludes":{"@id":"unece:InformationSource"},"schema:domainIncludes":{"@id":"unece:CooperatingOrganization"},"rdfs:comment":"A specified cooperative information source used for or from this cooperating organization."},{"@id":"unece:objectClassId","@type":["rdf:Property","owl:DatatypeProperty"],"rdfs:label":"objectClassId","schema:rangeIncludes":{"@id":"schema:Text"},"schema:domainIncludes":{"@id":"unece:EventElement"},"rdfs:comment":"The identifier of the object class for this TT event element."},{"@id":"unece:procedure","@type":["rdf:Property","owl:DatatypeProperty"],"rdfs:label":"procedure","schema:rangeIncludes":{"@id":"schema:Text"},"schema:domainIncludes":[{"@id":"unece:DocumentHandlingInstructions"},{"@id":"unece:InspectionInstructions"},{"@id":"unece:LaboratoryObservationInstructions"},{"@id":"unece:TemperatureSettingInstructions"},{"@id":"unece:HandlingInstructions"},{"@id":"unece:PackagingInstructions"}],"rdfs:comment":"A procedure, expressed as text, for a set of inspection instructions."},{"@id":"unece:requirementIndicator","@type":["rdf:Property","owl:DatatypeProperty"],"rdfs:label":"requirementIndicator","schema:rangeIncludes":{"@id":"schema:Boolean"},"schema:domainIncludes":[{"@id":"unece:DocumentHandlingInstructions"},{"@id":"unece:PackagingInstructions"}],"rdfs:comment":"The indication of whether or not a requirement exists for these document handling instructions."},{"@id":"unece:MeasureTypeValue","@type":["rdf:Property","owl:DatatypeProperty"],"rdfs:label":"MeasureTypeValue","schema:rangeIncludes":{"@id":"schema:Float"},"schema:domainIncludes":{"@id":"unece:MeasureType"},"rdfs:comment":"The numeric value."},{"@id":"unece:MeasureTypeCode","@type":["rdf:Property","owl:DatatypeProperty"],"rdfs:label":"MeasureTypeCode","schema:rangeIncludes":{"@id":"unece:MeasureCode"},"schema:domainIncludes":{"@id":"unece:MeasureType"},"rdfs:comment":"The unit code."},{"@id":"unece:TemperatureUnitMeasureTypeValue","@type":["rdf:Property","owl:DatatypeProperty"],"rdfs:label":"TemperatureUnitMeasureTypeValue","schema:rangeIncludes":{"@id":"schema:Float"},"schema:domainIncludes":{"@id":"unece:TemperatureUnitMeasureType"},"rdfs:comment":"The numeric value."},{"@id":"unece:TemperatureUnitMeasureTypeCode","@type":["rdf:Property","owl:DatatypeProperty"],"rdfs:label":"TemperatureUnitMeasureTypeCode","schema:rangeIncludes":{"@id":"unece:TemperatureUnitMeasureCode"},"schema:domainIncludes":{"@id":"unece:TemperatureUnitMeasureType"},"rdfs:comment":"The unit code."},{"@id":"unece:QuantityTypeValue","@type":["rdf:Property","owl:DatatypeProperty"],"rdfs:label":"QuantityTypeValue","schema:rangeIncludes":{"@id":"schema:Float"},"schema:domainIncludes":{"@id":"unece:QuantityType"},"rdfs:comment":"The numeric value."},{"@id":"unece:QuantityTypeCode","@type":["rdf:Property","owl:DatatypeProperty"],"rdfs:label":"QuantityTypeCode","schema:rangeIncludes":{"@id":"unece:QuantityCode"},"schema:domainIncludes":{"@id":"unece:QuantityType"},"rdfs:comment":"The unit code."},{"@id":"unece:AmountTypeValue","@type":["rdf:Property","owl:DatatypeProperty"],"rdfs:label":"AmountTypeValue","schema:rangeIncludes":{"@id":"schema:Float"},"schema:domainIncludes":{"@id":"unece:AmountType"},"rdfs:comment":"A number of monetary units."},{"@id":"unece:AmountTypeCurrency","@type":["rdf:Property","owl:DatatypeProperty"],"rdfs:label":"AmountTypeCurrency","schema:rangeIncludes":{"@id":"unece:AmountCurrency"},"schema:domainIncludes":{"@id":"unece:AmountType"},"rdfs:comment":"An amount currency code."},{"@id":"unece:DurationUnitMeasureTypeValue","@type":["rdf:Property","owl:DatatypeProperty"],"rdfs:label":"DurationUnitMeasureTypeValue","schema:rangeIncludes":{"@id":"schema:Float"},"schema:domainIncludes":{"@id":"unece:DurationUnitMeasureType"},"rdfs:comment":"The numeric value."},{"@id":"unece:DurationUnitMeasureTypeCode","@type":["rdf:Property","owl:DatatypeProperty"],"rdfs:label":"DurationUnitMeasureTypeCode","schema:rangeIncludes":{"@id":"unece:DurationUnitMeasureCode"},"schema:domainIncludes":{"@id":"unece:DurationUnitMeasureType"},"rdfs:comment":"The unit code."},{"@id":"unece:marginValueNumeric","@type":["rdf:Property","owl:DatatypeProperty"],"rdfs:label":"marginValueNumeric","schema:rangeIncludes":{"@id":"schema:Text"},"schema:domainIncludes":{"@id":"unece:Tolerance"},"rdfs:comment":"The margin numeric value of this specified tolerance."},{"@id":"unece:marginValuePercent","@type":["rdf:Property","owl:DatatypeProperty"],"rdfs:label":"marginValuePercent","schema:rangeIncludes":{"@id":"schema:Text"},"schema:domainIncludes":{"@id":"unece:Tolerance"},"rdfs:comment":"The margin percentage value of this specified tolerance."},{"@id":"unece:minusValuePercent","@type":["rdf:Property","owl:DatatypeProperty"],"rdfs:label":"minusValuePercent","schema:rangeIncludes":{"@id":"schema:Text"},"schema:domainIncludes":{"@id":"unece:Tolerance"},"rdfs:comment":"The minus percentage value of this specified tolerance."},{"@id":"unece:minusValueQuantity","@type":["rdf:Property","owl:ObjectProperty"],"rdfs:label":"minusValueQuantity","schema:rangeIncludes":{"@id":"unece:QuantityType"},"schema:domainIncludes":{"@id":"unece:Tolerance"},"rdfs:comment":"The minus quantity value of this specified tolerance."},{"@id":"unece:surplusValuePercent","@type":["rdf:Property","owl:DatatypeProperty"],"rdfs:label":"surplusValuePercent","schema:rangeIncludes":{"@id":"schema:Text"},"schema:domainIncludes":{"@id":"unece:Tolerance"},"rdfs:comment":"The surplus percentage value of this specified tolerance."},{"@id":"unece:surplusValueQuantity","@type":["rdf:Property","owl:ObjectProperty"],"rdfs:label":"surplusValueQuantity","schema:rangeIncludes":{"@id":"unece:QuantityType"},"schema:domainIncludes":{"@id":"unece:Tolerance"},"rdfs:comment":"The surplus quantity value of this specified tolerance."},{"@id":"unece:LinearUnitMeasureTypeValue","@type":["rdf:Property","owl:DatatypeProperty"],"rdfs:label":"LinearUnitMeasureTypeValue","schema:rangeIncludes":{"@id":"schema:Float"},"schema:domainIncludes":{"@id":"unece:LinearUnitMeasureType"},"rdfs:comment":"The numeric value."},{"@id":"unece:LinearUnitMeasureTypeCode","@type":["rdf:Property","owl:DatatypeProperty"],"rdfs:label":"LinearUnitMeasureTypeCode","schema:rangeIncludes":{"@id":"unece:LinearUnitMeasureCode"},"schema:domainIncludes":{"@id":"unece:LinearUnitMeasureType"},"rdfs:comment":"The unit code."},{"@id":"unece:actualDateTime","@type":["rdf:Property","owl:DatatypeProperty"],"rdfs:label":"actualDateTime","schema:rangeIncludes":{"@id":"schema:Text"},"schema:domainIncludes":[{"@id":"unece:Authentication"},{"@id":"unece:FinancialAdjustment"},{"@id":"unece:Booking"},{"@id":"unece:DeliveryAdjustment"}],"rdfs:comment":"An actual date, time, date time, or other date time value of this financial booking."},{"@id":"unece:governmentActionTypeCode","@type":["rdf:Property","owl:DatatypeProperty"],"rdfs:label":"governmentActionTypeCode","schema:rangeIncludes":{"@id":"unece:GovernmentActionCodeList"},"schema:domainIncludes":{"@id":"unece:Authentication"},"rdfs:comment":"The code specifying the type of document authentication."},{"@id":"unece:includedClause","@type":["rdf:Property","owl:ObjectProperty"],"rdfs:label":"includedClause","schema:rangeIncludes":{"@id":"unece:Clause"},"schema:domainIncludes":{"@id":"unece:Authentication"},"rdfs:comment":"A document clause included in this document authentication."},{"@id":"unece:locationProviderParty","@type":["rdf:Property","owl:ObjectProperty"],"rdfs:label":"locationProviderParty","schema:rangeIncludes":{"@id":"unece:Party"},"schema:domainIncludes":{"@id":"unece:Authentication"},"rdfs:comment":"The trade party providing the location for this document authentication."},{"@id":"unece:providerParty","@type":["rdf:Property","owl:ObjectProperty"],"rdfs:label":"providerParty","schema:rangeIncludes":{"@id":"unece:Party"},"schema:domainIncludes":[{"@id":"unece:Authentication"},{"@id":"unece:IOTDevice"}],"rdfs:comment":"The provider party for this monitoring IOT device."},{"@id":"unece:representationTypeCode","@type":["rdf:Property","owl:DatatypeProperty"],"rdfs:label":"representationTypeCode","schema:rangeIncludes":{"@id":"schema:Text"},"schema:domainIncludes":{"@id":"unece:Authentication"},"rdfs:comment":"The code specifying the type of representation of this document authentication, such as direct or indirect."},{"@id":"unece:signatory","@type":["rdf:Property","owl:DatatypeProperty"],"rdfs:label":"signatory","schema:rangeIncludes":{"@id":"schema:Text"},"schema:domainIncludes":{"@id":"unece:Authentication"},"rdfs:comment":"The signatory, expressed as text, for this document authentication."},{"@id":"unece:signatoryImageBinaryObject","@type":["rdf:Property","owl:DatatypeProperty"],"rdfs:label":"signatoryImageBinaryObject","schema:rangeIncludes":{"@id":"schema:Text"},"schema:domainIncludes":{"@id":"unece:Authentication"},"rdfs:comment":"The signatory image, expressed as a binary object, for this document authentication."},{"@id":"unece:statement","@type":["rdf:Property","owl:DatatypeProperty"],"rdfs:label":"statement","schema:rangeIncludes":{"@id":"schema:Text"},"schema:domainIncludes":[{"@id":"unece:Authentication"},{"@id":"unece:InspectionResult"}],"rdfs:comment":"A statement, expressed as text, for this specified inspection result."},{"@id":"unece:statementCode","@type":["rdf:Property","owl:DatatypeProperty"],"rdfs:label":"statementCode","schema:rangeIncludes":{"@id":"schema:Text"},"schema:domainIncludes":{"@id":"unece:Authentication"},"rdfs:comment":"The code specifying the statement for this document authentication."},{"@id":"unece:associatedMeasurement","@type":["rdf:Property","owl:ObjectProperty"],"rdfs:label":"associatedMeasurement","schema:rangeIncludes":{"@id":"unece:Measurement"},"schema:domainIncludes":{"@id":"unece:Clause"},"rdfs:comment":"A measurement associated with this document clause."},{"@id":"unece:associatedPeriod","@type":["rdf:Property","owl:ObjectProperty"],"rdfs:label":"associatedPeriod","schema:rangeIncludes":{"@id":"unece:SpecifiedPeriod"},"schema:domainIncludes":{"@id":"unece:Clause"},"rdfs:comment":"A period of time associated with this document clause."},{"@id":"unece:uRLId","@type":["rdf:Property","owl:DatatypeProperty"],"rdfs:label":"uRLId","schema:rangeIncludes":{"@id":"schema:Text"},"schema:domainIncludes":{"@id":"unece:Clause"},"rdfs:comment":"The Uniform Resource Locator (URL) for this document clause."},{"@id":"unece:actualOccurrenceDateTime","@type":["rdf:Property","owl:DatatypeProperty"],"rdfs:label":"actualOccurrenceDateTime","schema:rangeIncludes":{"@id":"schema:Text"},"schema:domainIncludes":[{"@id":"unece:Event"},{"@id":"unece:TransportEvent"}],"rdfs:comment":"The date, time, date time or other date time value of the actual arrival related to this transport event."},{"@id":"unece:actualOccurrencePeriod","@type":["rdf:Property","owl:ObjectProperty"],"rdfs:label":"actualOccurrencePeriod","schema:rangeIncludes":{"@id":"unece:SpecifiedPeriod"},"schema:domainIncludes":[{"@id":"unece:Event"},{"@id":"unece:TransportEvent"}],"rdfs:comment":"The actual period of time during which this transport event occurred."},{"@id":"unece:estimatedOccurrenceDateTime","@type":["rdf:Property","owl:DatatypeProperty"],"rdfs:label":"estimatedOccurrenceDateTime","schema:rangeIncludes":{"@id":"schema:Text"},"schema:domainIncludes":[{"@id":"unece:Event"},{"@id":"unece:TransportEvent"}],"rdfs:comment":"The estimated date, time, date time, or other date time value of the occurrence of this transport event."},{"@id":"unece:occurrencePeriod","@type":["rdf:Property","owl:ObjectProperty"],"rdfs:label":"occurrencePeriod","schema:rangeIncludes":{"@id":"unece:SpecifiedPeriod"},"schema:domainIncludes":[{"@id":"unece:Event"},{"@id":"unece:TransportEvent"},{"@id":"unece:SupplyChainEvent"}],"rdfs:comment":"The specified period of laycan time during which this transport event occurs."},{"@id":"unece:scheduledOccurrenceDateTime","@type":["rdf:Property","owl:DatatypeProperty"],"rdfs:label":"scheduledOccurrenceDateTime","schema:rangeIncludes":{"@id":"schema:Text"},"schema:domainIncludes":[{"@id":"unece:Event"},{"@id":"unece:TransportEvent"}],"rdfs:comment":"A pilot boarding place, expressed as text, for this transport event."},{"@id":"unece:scheduledOccurrencePeriod","@type":["rdf:Property","owl:ObjectProperty"],"rdfs:label":"scheduledOccurrencePeriod","schema:rangeIncludes":{"@id":"unece:SpecifiedPeriod"},"schema:domainIncludes":[{"@id":"unece:Event"},{"@id":"unece:TransportEvent"}],"rdfs:comment":"The scheduled period of time specified for the occurrence of this transport event."},{"@id":"unece:WeightUnitMeasureTypeValue","@type":["rdf:Property","owl:DatatypeProperty"],"rdfs:label":"WeightUnitMeasureTypeValue","schema:rangeIncludes":{"@id":"schema:Float"},"schema:domainIncludes":{"@id":"unece:WeightUnitMeasureType"},"rdfs:comment":"The numeric value."},{"@id":"unece:WeightUnitMeasureTypeCode","@type":["rdf:Property","owl:DatatypeProperty"],"rdfs:label":"WeightUnitMeasureTypeCode","schema:rangeIncludes":{"@id":"unece:WeightUnitMeasureCode"},"schema:domainIncludes":{"@id":"unece:WeightUnitMeasureType"},"rdfs:comment":"The unit code."},{"@id":"unece:UnitMeasureTypeValue","@type":["rdf:Property","owl:DatatypeProperty"],"rdfs:label":"UnitMeasureTypeValue","schema:rangeIncludes":{"@id":"schema:Float"},"schema:domainIncludes":{"@id":"unece:UnitMeasureType"},"rdfs:comment":"The numeric value."},{"@id":"unece:UnitMeasureTypeCode","@type":["rdf:Property","owl:DatatypeProperty"],"rdfs:label":"UnitMeasureTypeCode","schema:rangeIncludes":{"@id":"unece:UnitMeasureCode"},"schema:domainIncludes":{"@id":"unece:UnitMeasureType"},"rdfs:comment":"The unit code."},{"@id":"unece:VolumeUnitMeasureTypeValue","@type":["rdf:Property","owl:DatatypeProperty"],"rdfs:label":"VolumeUnitMeasureTypeValue","schema:rangeIncludes":{"@id":"schema:Float"},"schema:domainIncludes":{"@id":"unece:VolumeUnitMeasureType"},"rdfs:comment":"The numeric value."},{"@id":"unece:VolumeUnitMeasureTypeCode","@type":["rdf:Property","owl:DatatypeProperty"],"rdfs:label":"VolumeUnitMeasureTypeCode","schema:rangeIncludes":{"@id":"unece:VolumeUnitMeasureCode"},"schema:domainIncludes":{"@id":"unece:VolumeUnitMeasureType"},"rdfs:comment":"The unit code."},{"@id":"unece:AirFlowUnitMeasureTypeValue","@type":["rdf:Property","owl:DatatypeProperty"],"rdfs:label":"AirFlowUnitMeasureTypeValue","schema:rangeIncludes":{"@id":"schema:Float"},"schema:domainIncludes":{"@id":"unece:AirFlowUnitMeasureType"},"rdfs:comment":"The numeric value."},{"@id":"unece:AirFlowUnitMeasureTypeCode","@type":["rdf:Property","owl:DatatypeProperty"],"rdfs:label":"AirFlowUnitMeasureTypeCode","schema:rangeIncludes":{"@id":"unece:AirFlowUnitMeasureCode"},"schema:domainIncludes":{"@id":"unece:AirFlowUnitMeasureType"},"rdfs:comment":"The unit code."},{"@id":"unece:birthCountryId","@type":["rdf:Property","owl:DatatypeProperty"],"rdfs:label":"birthCountryId","schema:rangeIncludes":{"@id":"schema:Text"},"schema:domainIncludes":[{"@id":"unece:Person"},{"@id":"unece:TransportPerson"}],"rdfs:comment":"The identifier of the birth country of this transport person."},{"@id":"unece:birthDateTime","@type":["rdf:Property","owl:DatatypeProperty"],"rdfs:label":"birthDateTime","schema:rangeIncludes":{"@id":"schema:Text"},"schema:domainIncludes":[{"@id":"unece:Person"},{"@id":"unece:GuestPerson"},{"@id":"unece:IndividualTTAnimal"},{"@id":"unece:TransportPerson"}],"rdfs:comment":"The birth date for this individual TT animal."},{"@id":"unece:birthplaceName","@type":["rdf:Property","owl:DatatypeProperty"],"rdfs:label":"birthplaceName","schema:rangeIncludes":{"@id":"schema:Text"},"schema:domainIncludes":[{"@id":"unece:Person"},{"@id":"unece:TransportPerson"}],"rdfs:comment":"The name, expressed as text, of the place where this transport person was born."},{"@id":"unece:familyName","@type":["rdf:Property","owl:DatatypeProperty"],"rdfs:label":"familyName","schema:rangeIncludes":{"@id":"schema:Text"},"schema:domainIncludes":[{"@id":"unece:Person"},{"@id":"unece:Chemical"},{"@id":"unece:TransportPerson"}],"rdfs:comment":"A date, time, date time, or other date time value that this person embarked upon a means of transport."},{"@id":"unece:givenName","@type":["rdf:Property","owl:DatatypeProperty"],"rdfs:label":"givenName","schema:rangeIncludes":{"@id":"schema:Text"},"schema:domainIncludes":[{"@id":"unece:Person"},{"@id":"unece:TransportPerson"}],"rdfs:comment":"A given name, expressed as text, for this transport person."},{"@id":"unece:landlineTelephoneCommunication","@type":["rdf:Property","owl:ObjectProperty"],"rdfs:label":"landlineTelephoneCommunication","schema:rangeIncludes":{"@id":"unece:Communication"},"schema:domainIncludes":[{"@id":"unece:Person"},{"@id":"unece:TransportPerson"}],"rdfs:comment":"The indication of whether or not this transport person is in transit."},{"@id":"unece:nationalityCountry","@type":["rdf:Property","owl:ObjectProperty"],"rdfs:label":"nationalityCountry","schema:rangeIncludes":{"@id":"unece:Country"},"schema:domainIncludes":[{"@id":"unece:Person"},{"@id":"unece:TransportPerson"}],"rdfs:comment":"A country that constitutes a nationality by origin, birth, or naturalization for this transport person."},{"@id":"unece:contactPersonTitleCode","@type":["rdf:Property","owl:DatatypeProperty"],"rdfs:label":"contactPersonTitleCode","schema:rangeIncludes":{"@id":"unece:TitleCodeList"},"schema:domainIncludes":{"@id":"unece:Contact"},"rdfs:comment":"The code specifying the title of this contact person, such as Ms., Doctor, Mister."},{"@id":"unece:countryResidenceCountryId","@type":["rdf:Property","owl:DatatypeProperty"],"rdfs:label":"countryResidenceCountryId","schema:rangeIncludes":{"@id":"unece:CountryId"},"schema:domainIncludes":{"@id":"unece:Contact"},"rdfs:comment":"The identifier of the residence country of this contact person."},{"@id":"unece:specifiedBirthAddress","@type":["rdf:Property","owl:ObjectProperty"],"rdfs:label":"specifiedBirthAddress","schema:rangeIncludes":{"@id":"unece:BirthAddress"},"schema:domainIncludes":{"@id":"unece:Contact"},"rdfs:comment":"The birth address specified for this contact person."},{"@id":"unece:specifiedEmployerIdentity","@type":["rdf:Property","owl:ObjectProperty"],"rdfs:label":"specifiedEmployerIdentity","schema:rangeIncludes":{"@id":"unece:EmployerIdentity"},"schema:domainIncludes":{"@id":"unece:Contact"},"rdfs:comment":"An employer identity specified for this contact person."},{"@id":"unece:specifiedPersonIdentity","@type":["rdf:Property","owl:ObjectProperty"],"rdfs:label":"specifiedPersonIdentity","schema:rangeIncludes":{"@id":"unece:PersonIdentity"},"schema:domainIncludes":{"@id":"unece:Contact"},"rdfs:comment":"The person identity specified for this contact person."},{"@id":"unece:websiteURICommunication","@type":["rdf:Property","owl:ObjectProperty"],"rdfs:label":"websiteURICommunication","schema:rangeIncludes":{"@id":"unece:Communication"},"schema:domainIncludes":[{"@id":"unece:Contact"},{"@id":"unece:LaboratoryObservationParty"}],"rdfs:comment":"A website Uniform Resource Identifier (URI) communication for this contact person."},{"@id":"unece:acceptedAmount","@type":["rdf:Property","owl:ObjectProperty"],"rdfs:label":"acceptedAmount","schema:rangeIncludes":{"@id":"unece:AmountType"},"schema:domainIncludes":{"@id":"unece:PaymentTradeSettlement"},"rdfs:comment":""},{"@id":"unece:dueDateTime","@type":["rdf:Property","owl:DatatypeProperty"],"rdfs:label":"dueDateTime","schema:rangeIncludes":{"@id":"schema:Text"},"schema:domainIncludes":[{"@id":"unece:PaymentTradeSettlement"},{"@id":"unece:PaymentTerms"},{"@id":"unece:InstalmentPayment"},{"@id":"unece:SupplyChainEvent"}],"rdfs:comment":"The date, time, date time, or other date time value of the due date specified by these trade payment terms."},{"@id":"unece:identifiedGuarantee","@type":["rdf:Property","owl:ObjectProperty"],"rdfs:label":"identifiedGuarantee","schema:rangeIncludes":{"@id":"unece:Guarantee"},"schema:domainIncludes":{"@id":"unece:PaymentTradeSettlement"},"rdfs:comment":"The financial guarantee identified for this payment trade settlement."},{"@id":"unece:instruction","@type":["rdf:Property","owl:DatatypeProperty"],"rdfs:label":"instruction","schema:rangeIncludes":{"@id":"schema:Text"},"schema:domainIncludes":[{"@id":"unece:PaymentTradeSettlement"},{"@id":"unece:ExperienceItem"},{"@id":"unece:ExperienceProduct"},{"@id":"unece:ExperienceEvent"}],"rdfs:comment":"An instruction, expressed as text, for this experience event."},{"@id":"unece:invoicePayerAssignedReferenceId","@type":["rdf:Property","owl:DatatypeProperty"],"rdfs:label":"invoicePayerAssignedReferenceId","schema:rangeIncludes":{"@id":"schema:Text"},"schema:domainIncludes":{"@id":"unece:PaymentTradeSettlement"},"rdfs:comment":"The identifier of the invoice payer assigned reference of this payment trade settlement."},{"@id":"unece:penaltyPercent","@type":["rdf:Property","owl:DatatypeProperty"],"rdfs:label":"penaltyPercent","schema:rangeIncludes":{"@id":"schema:Text"},"schema:domainIncludes":{"@id":"unece:PaymentTradeSettlement"},"rdfs:comment":"The penalty percentage related to this payment trade settlement."},{"@id":"unece:requestedAmount","@type":["rdf:Property","owl:ObjectProperty"],"rdfs:label":"requestedAmount","schema:rangeIncludes":{"@id":"unece:AmountType"},"schema:domainIncludes":{"@id":"unece:PaymentTradeSettlement"},"rdfs:comment":""},{"@id":"unece:specifiedTradeSettlementPaymentMonetarySummation","@type":["rdf:Property","owl:ObjectProperty"],"rdfs:label":"specifiedTradeSettlementPaymentMonetarySummation","schema:rangeIncludes":{"@id":"unece:TradeSettlementPaymentMonetarySummation"},"schema:domainIncludes":{"@id":"unece:PaymentTradeSettlement"},"rdfs:comment":"The monetary summation totals specified for this payment trade settlement."},{"@id":"unece:taxAmount","@type":["rdf:Property","owl:ObjectProperty"],"rdfs:label":"taxAmount","schema:rangeIncludes":{"@id":"unece:AmountType"},"schema:domainIncludes":{"@id":"unece:PaymentTradeSettlement"},"rdfs:comment":""},{"@id":"unece:transferFeeInclusiveIndicator","@type":["rdf:Property","owl:DatatypeProperty"],"rdfs:label":"transferFeeInclusiveIndicator","schema:rangeIncludes":{"@id":"schema:Boolean"},"schema:domainIncludes":{"@id":"unece:PaymentTradeSettlement"},"rdfs:comment":"The indication of whether or not this payment trade settlement includes a transfer fee."},{"@id":"unece:acceptedTransactionOriginalTotalAmount","@type":["rdf:Property","owl:ObjectProperty"],"rdfs:label":"acceptedTransactionOriginalTotalAmount","schema:rangeIncludes":{"@id":"unece:AmountType"},"schema:domainIncludes":{"@id":"unece:FinancingSummaryDocument"},"rdfs:comment":""},{"@id":"unece:financedAppliedRatePercent","@type":["rdf:Property","owl:DatatypeProperty"],"rdfs:label":"financedAppliedRatePercent","schema:rangeIncludes":{"@id":"schema:Text"},"schema:domainIncludes":{"@id":"unece:FinancingSummaryDocument"},"rdfs:comment":"The financed applied rate, expressed as a percentage, in this financing summary document."},{"@id":"unece:financedTotalAmount","@type":["rdf:Property","owl:ObjectProperty"],"rdfs:label":"financedTotalAmount","schema:rangeIncludes":{"@id":"unece:AmountType"},"schema:domainIncludes":[{"@id":"unece:FinancingSummaryDocument"},{"@id":"unece:FinancingRequestResultDocument"}],"rdfs:comment":""},{"@id":"unece:financedTransactionSpecifiedQuantity","@type":["rdf:Property","owl:ObjectProperty"],"rdfs:label":"financedTransactionSpecifiedQuantity","schema:rangeIncludes":{"@id":"unece:QuantityType"},"schema:domainIncludes":{"@id":"unece:FinancingSummaryDocument"},"rdfs:comment":""},{"@id":"unece:lineOfCreditSpecifiedFinancialAccount","@type":["rdf:Property","owl:ObjectProperty"],"rdfs:label":"lineOfCreditSpecifiedFinancialAccount","schema:rangeIncludes":{"@id":"unece:FinancingFinancialAccount"},"schema:domainIncludes":[{"@id":"unece:FinancingSummaryDocument"},{"@id":"unece:RequestingParty"}],"rdfs:comment":"The financing financial account, used for managing the line of credit, specified for this financing summary document."},{"@id":"unece:relatedBooking","@type":["rdf:Property","owl:ObjectProperty"],"rdfs:label":"relatedBooking","schema:rangeIncludes":{"@id":"unece:Booking"},"schema:domainIncludes":{"@id":"unece:FinancingSummaryDocument"},"rdfs:comment":"The financial booking related to this financing summary document."},{"@id":"unece:specifiedCreditorFinancialAccount","@type":["rdf:Property","owl:ObjectProperty"],"rdfs:label":"specifiedCreditorFinancialAccount","schema:rangeIncludes":{"@id":"unece:CreditorFinancialAccount"},"schema:domainIncludes":[{"@id":"unece:FinancingSummaryDocument"},{"@id":"unece:PaymentMeans"},{"@id":"unece:RequestingParty"}],"rdfs:comment":"A creditor financial account specified for this trade settlement payment means."},{"@id":"unece:accountName","@type":["rdf:Property","owl:DatatypeProperty"],"rdfs:label":"accountName","schema:rangeIncludes":{"@id":"schema:Text"},"schema:domainIncludes":[{"@id":"unece:CreditorFinancialAccount"},{"@id":"unece:DebtorFinancialAccount"},{"@id":"unece:FinancingFinancialAccount"},{"@id":"unece:PaymentFinancialAccount"}],"rdfs:comment":"An account name, expressed as text, of this payment financial account."},{"@id":"unece:bBANId","@type":["rdf:Property","owl:DatatypeProperty"],"rdfs:label":"bBANId","schema:rangeIncludes":{"@id":"schema:Text"},"schema:domainIncludes":[{"@id":"unece:CreditorFinancialAccount"},{"@id":"unece:DebtorFinancialAccount"},{"@id":"unece:FinancingFinancialAccount"}],"rdfs:comment":"The unique Basic Bank Account Number (BBAN) identifier used as part of a National Account Numbering Scheme for this financing financial account."},{"@id":"unece:creditorFinancialAccountTypeCode","@type":["rdf:Property","owl:DatatypeProperty"],"rdfs:label":"creditorFinancialAccountTypeCode","schema:rangeIncludes":{"@id":"schema:Text"},"schema:domainIncludes":{"@id":"unece:CreditorFinancialAccount"},"rdfs:comment":"The code specifying the type of creditor financial account."},{"@id":"unece:currencyCode","@type":["rdf:Property","owl:DatatypeProperty"],"rdfs:label":"currencyCode","schema:rangeIncludes":{"@id":"schema:Text"},"schema:domainIncludes":[{"@id":"unece:CreditorFinancialAccount"},{"@id":"unece:DebtorFinancialAccount"},{"@id":"unece:Cash"},{"@id":"unece:RegisteredTax"}],"rdfs:comment":"The code specifying a currency of this cash used for payment."},{"@id":"unece:iBANId","@type":["rdf:Property","owl:DatatypeProperty"],"rdfs:label":"iBANId","schema:rangeIncludes":{"@id":"schema:Text"},"schema:domainIncludes":[{"@id":"unece:CreditorFinancialAccount"},{"@id":"unece:DebtorFinancialAccount"},{"@id":"unece:FinancingFinancialAccount"},{"@id":"unece:PaymentFinancialAccount"}],"rdfs:comment":"The unique International Bank Account Number (IBAN) identifier for this creditor financial account."},{"@id":"unece:proprietaryId","@type":["rdf:Property","owl:DatatypeProperty"],"rdfs:label":"proprietaryId","schema:rangeIncludes":{"@id":"schema:Text"},"schema:domainIncludes":[{"@id":"unece:CreditorFinancialAccount"},{"@id":"unece:DebtorFinancialAccount"},{"@id":"unece:FinancingFinancialAccount"}],"rdfs:comment":"The proprietary identifier for this financing financial account."},{"@id":"unece:uPICId","@type":["rdf:Property","owl:DatatypeProperty"],"rdfs:label":"uPICId","schema:rangeIncludes":{"@id":"schema:Text"},"schema:domainIncludes":[{"@id":"unece:CreditorFinancialAccount"},{"@id":"unece:DebtorFinancialAccount"},{"@id":"unece:FinancingFinancialAccount"}],"rdfs:comment":"The unique Universal Payment Identification Code (UPIC) identifier used by the New York Clearing House for this creditor financial account."},{"@id":"unece:debtorFinancialAccountTypeCode","@type":["rdf:Property","owl:DatatypeProperty"],"rdfs:label":"debtorFinancialAccountTypeCode","schema:rangeIncludes":{"@id":"schema:Text"},"schema:domainIncludes":{"@id":"unece:DebtorFinancialAccount"},"rdfs:comment":"The code specifying the type of debtor financial account."},{"@id":"unece:cashAccountTypeCode","@type":["rdf:Property","owl:DatatypeProperty"],"rdfs:label":"cashAccountTypeCode","schema:rangeIncludes":{"@id":"unece:CashAccountTypeCodeList"},"schema:domainIncludes":{"@id":"unece:FinancingFinancialAccount"},"rdfs:comment":"The code specifying the type of financing financial account."},{"@id":"unece:financingFinancialAccountCurrencyCode","@type":["rdf:Property","owl:DatatypeProperty"],"rdfs:label":"financingFinancialAccountCurrencyCode","schema:rangeIncludes":{"@id":"unece:CurrencyCodeList"},"schema:domainIncludes":{"@id":"unece:FinancingFinancialAccount"},"rdfs:comment":"The code specifying the currency of this financing financial account."},{"@id":"unece:paymentFinancialAccountCurrencyCode","@type":["rdf:Property","owl:DatatypeProperty"],"rdfs:label":"paymentFinancialAccountCurrencyCode","schema:rangeIncludes":{"@id":"unece:CurrencyCodeList"},"schema:domainIncludes":{"@id":"unece:PaymentFinancialAccount"},"rdfs:comment":"The code specifying the currency of this payment financial account."},{"@id":"unece:accountingAccountTypeCode","@type":["rdf:Property","owl:DatatypeProperty"],"rdfs:label":"accountingAccountTypeCode","schema:rangeIncludes":{"@id":"unece:AccountingAccountTypeCodeList"},"schema:domainIncludes":{"@id":"unece:AccountingAccount"},"rdfs:comment":"The code specifying the type of trade accounting account, such as general (main), secondary, cost accounting or budget account."},{"@id":"unece:accountingAmountTypeAmountTypeCode","@type":["rdf:Property","owl:DatatypeProperty"],"rdfs:label":"accountingAmountTypeAmountTypeCode","schema:rangeIncludes":{"@id":"unece:AccountingAmountTypeCodeList"},"schema:domainIncludes":{"@id":"unece:AccountingAccount"},"rdfs:comment":"The code specifying the amount type for this trade accounting account."},{"@id":"unece:accountingDocumentSetTriggerCode","@type":["rdf:Property","owl:DatatypeProperty"],"rdfs:label":"accountingDocumentSetTriggerCode","schema:rangeIncludes":{"@id":"unece:AccountingDocumentCodeList"},"schema:domainIncludes":{"@id":"unece:AccountingAccount"},"rdfs:comment":"A code specifying a set trigger for this trade accounting account to be used in response to a specific event or a set of events."},{"@id":"unece:costReferenceDimensionPattern","@type":["rdf:Property","owl:DatatypeProperty"],"rdfs:label":"costReferenceDimensionPattern","schema:rangeIncludes":{"@id":"schema:Text"},"schema:domainIncludes":{"@id":"unece:AccountingAccount"},"rdfs:comment":"The cost reference dimension pattern, expressed as text, for this trade accounting account."},{"@id":"unece:accountingDebitCreditStatusDirectionCode","@type":["rdf:Property","owl:DatatypeProperty"],"rdfs:label":"accountingDebitCreditStatusDirectionCode","schema:rangeIncludes":{"@id":"unece:AccountingDebitCreditStatusCodeList"},"schema:domainIncludes":{"@id":"unece:FinancialAdjustment"},"rdfs:comment":"The code specifying whether the financial adjustment must be subtracted or added."},{"@id":"unece:actualAmount","@type":["rdf:Property","owl:ObjectProperty"],"rdfs:label":"actualAmount","schema:rangeIncludes":{"@id":"unece:AmountType"},"schema:domainIncludes":[{"@id":"unece:FinancialAdjustment"},{"@id":"unece:AppliedAllowanceCharge"},{"@id":"unece:TradeAllowanceCharge"},{"@id":"unece:DeliveryAdjustment"}],"rdfs:comment":""},{"@id":"unece:claimRelatedParty","@type":["rdf:Property","owl:ObjectProperty"],"rdfs:label":"claimRelatedParty","schema:rangeIncludes":{"@id":"unece:Party"},"schema:domainIncludes":{"@id":"unece:FinancialAdjustment"},"rdfs:comment":""},{"@id":"unece:financialAdjustmentReasonCode","@type":["rdf:Property","owl:DatatypeProperty"],"rdfs:label":"financialAdjustmentReasonCode","schema:rangeIncludes":{"@id":"unece:FinancialAdjustmentReasonCodeList"},"schema:domainIncludes":{"@id":"unece:FinancialAdjustment"},"rdfs:comment":"A code specifying a reason for this financial adjustment."},{"@id":"unece:invoiceReferenceDocument","@type":["rdf:Property","owl:ObjectProperty"],"rdfs:label":"invoiceReferenceDocument","schema:rangeIncludes":{"@id":"unece:Document"},"schema:domainIncludes":{"@id":"unece:FinancialAdjustment"},"rdfs:comment":"Written, printed or electronic matter that is referenced."},{"@id":"unece:relatedTax","@type":["rdf:Property","owl:ObjectProperty"],"rdfs:label":"relatedTax","schema:rangeIncludes":{"@id":"unece:Tax"},"schema:domainIncludes":{"@id":"unece:FinancialAdjustment"},"rdfs:comment":"A trade tax related to this financial adjustment."},{"@id":"unece:appliedAllowanceChargeReasonCode","@type":["rdf:Property","owl:DatatypeProperty"],"rdfs:label":"appliedAllowanceChargeReasonCode","schema:rangeIncludes":{"@id":"schema:Text"},"schema:domainIncludes":{"@id":"unece:AppliedAllowanceCharge"},"rdfs:comment":"The code specifying the reason for this applied allowance charge."},{"@id":"unece:calculationPercent","@type":["rdf:Property","owl:DatatypeProperty"],"rdfs:label":"calculationPercent","schema:rangeIncludes":{"@id":"schema:Text"},"schema:domainIncludes":[{"@id":"unece:AppliedAllowanceCharge"},{"@id":"unece:PaymentDiscountTerms"},{"@id":"unece:PaymentPenaltyTerms"},{"@id":"unece:TradeAllowanceCharge"},{"@id":"unece:TradePrice"}],"rdfs:comment":"The calculation percentage for this trade price."},{"@id":"unece:categoryAppliedTax","@type":["rdf:Property","owl:ObjectProperty"],"rdfs:label":"categoryAppliedTax","schema:rangeIncludes":{"@id":"unece:AppliedTax"},"schema:domainIncludes":{"@id":"unece:AppliedAllowanceCharge"},"rdfs:comment":"The applied tax category of this applied allowance charge."},{"@id":"unece:chargeIndicator","@type":["rdf:Property","owl:DatatypeProperty"],"rdfs:label":"chargeIndicator","schema:rangeIncludes":{"@id":"schema:Boolean"},"schema:domainIncludes":[{"@id":"unece:AppliedAllowanceCharge"},{"@id":"unece:TradeAllowanceCharge"}],"rdfs:comment":"The indication of whether or not the applied allowance charge is a charge."},{"@id":"unece:creditDateTime","@type":["rdf:Property","owl:DatatypeProperty"],"rdfs:label":"creditDateTime","schema:rangeIncludes":{"@id":"schema:DateTime"},"schema:domainIncludes":{"@id":"unece:Booking"},"rdfs:comment":"The credit date, time, date time, or other date time value of this financial booking."},{"@id":"unece:debitDateTime","@type":["rdf:Property","owl:DatatypeProperty"],"rdfs:label":"debitDateTime","schema:rangeIncludes":{"@id":"schema:DateTime"},"schema:domainIncludes":{"@id":"unece:Booking"},"rdfs:comment":"The debit date, time, date time, or other date time value of this financial booking."},{"@id":"unece:actualDiscountAmount","@type":["rdf:Property","owl:ObjectProperty"],"rdfs:label":"actualDiscountAmount","schema:rangeIncludes":{"@id":"unece:AmountType"},"schema:domainIncludes":{"@id":"unece:PaymentDiscountTerms"},"rdfs:comment":""},{"@id":"unece:basisDateTime","@type":["rdf:Property","owl:DatatypeProperty"],"rdfs:label":"basisDateTime","schema:rangeIncludes":{"@id":"schema:Text"},"schema:domainIncludes":[{"@id":"unece:PaymentDiscountTerms"},{"@id":"unece:PaymentPenaltyTerms"},{"@id":"unece:TradePrice"}],"rdfs:comment":"The date, time, date time, or other date time value used as the basis for this trade price."},{"@id":"unece:basisPeriodMeasure","@type":["rdf:Property","owl:ObjectProperty"],"rdfs:label":"basisPeriodMeasure","schema:rangeIncludes":{"@id":"unece:MeasureType"},"schema:domainIncludes":[{"@id":"unece:PaymentDiscountTerms"},{"@id":"unece:PaymentPenaltyTerms"}],"rdfs:comment":""},{"@id":"unece:actualPenaltyAmount","@type":["rdf:Property","owl:ObjectProperty"],"rdfs:label":"actualPenaltyAmount","schema:rangeIncludes":{"@id":"unece:AmountType"},"schema:domainIncludes":{"@id":"unece:PaymentPenaltyTerms"},"rdfs:comment":""},{"@id":"unece:additionalClearingSystemId","@type":["rdf:Property","owl:DatatypeProperty"],"rdfs:label":"additionalClearingSystemId","schema:rangeIncludes":{"@id":"schema:Text"},"schema:domainIncludes":{"@id":"unece:CreditorFinancialInstitution"},"rdfs:comment":"An additional clearing system identifier for this creditor financial institution."},{"@id":"unece:australianBSBId","@type":["rdf:Property","owl:DatatypeProperty"],"rdfs:label":"australianBSBId","schema:rangeIncludes":{"@id":"schema:Text"},"schema:domainIncludes":[{"@id":"unece:CreditorFinancialInstitution"},{"@id":"unece:DebtorFinancialInstitution"}],"rdfs:comment":"The unique Australian Bank State Branch (BSB) Code identifier as assigned by the Australian Payments Clearing Association (APCA) for this creditor financial institution."},{"@id":"unece:australianSNId","@type":["rdf:Property","owl:DatatypeProperty"],"rdfs:label":"australianSNId","schema:rangeIncludes":{"@id":"schema:Text"},"schema:domainIncludes":{"@id":"unece:CreditorFinancialInstitution"},"rdfs:comment":"The Australian Small Network (SN) identifier as assigned by the Australian Payments Clearing Association (APCA) for this creditor financial institution."},{"@id":"unece:austrianBankleitzahlId","@type":["rdf:Property","owl:DatatypeProperty"],"rdfs:label":"austrianBankleitzahlId","schema:rangeIncludes":{"@id":"schema:Text"},"schema:domainIncludes":[{"@id":"unece:CreditorFinancialInstitution"},{"@id":"unece:DebtorFinancialInstitution"}],"rdfs:comment":"The unique Austrian Bankleitzahl identifier for this creditor financial institution."},{"@id":"unece:bICId","@type":["rdf:Property","owl:DatatypeProperty"],"rdfs:label":"bICId","schema:rangeIncludes":{"@id":"schema:Text"},"schema:domainIncludes":[{"@id":"unece:CreditorFinancialInstitution"},{"@id":"unece:FinancialIdentity"},{"@id":"unece:DebtorFinancialInstitution"},{"@id":"unece:PaymentFinancialInstitution"}],"rdfs:comment":"The Bank Identifier Code (BIC) as defined by ISO 9362 (Banking telecommunication messages, Bank Identifier Codes) for this financial identity."},{"@id":"unece:cHIPSParticipantId","@type":["rdf:Property","owl:DatatypeProperty"],"rdfs:label":"cHIPSParticipantId","schema:rangeIncludes":{"@id":"schema:Text"},"schema:domainIncludes":[{"@id":"unece:CreditorFinancialInstitution"},{"@id":"unece:DebtorFinancialInstitution"}],"rdfs:comment":"The unique (United States) Clearing House Interbank Payment System (CHIPS) Participant Identifier (ID) as assigned by the New York Clearing House for this creditor financial institution."},{"@id":"unece:cHIPSUniversalId","@type":["rdf:Property","owl:DatatypeProperty"],"rdfs:label":"cHIPSUniversalId","schema:rangeIncludes":{"@id":"schema:Text"},"schema:domainIncludes":[{"@id":"unece:CreditorFinancialInstitution"},{"@id":"unece:FinancialIdentity"},{"@id":"unece:DebtorFinancialInstitution"}],"rdfs:comment":"The (United States) Clearing House Interbank Payments System (CHIPS) Universal Identification (UID) as assigned by the New York Clearing House for this financial identity."},{"@id":"unece:canadianPaymentsAssociationId","@type":["rdf:Property","owl:DatatypeProperty"],"rdfs:label":"canadianPaymentsAssociationId","schema:rangeIncludes":{"@id":"schema:Text"},"schema:domainIncludes":[{"@id":"unece:CreditorFinancialInstitution"},{"@id":"unece:DebtorFinancialInstitution"}],"rdfs:comment":"The unique Canadian Payments Association Routing Number identifier for this creditor financial institution."},{"@id":"unece:clearingSystemName","@type":["rdf:Property","owl:DatatypeProperty"],"rdfs:label":"clearingSystemName","schema:rangeIncludes":{"@id":"schema:Text"},"schema:domainIncludes":[{"@id":"unece:CreditorFinancialInstitution"},{"@id":"unece:DebtorFinancialInstitution"}],"rdfs:comment":"The clearing system name, expressed as text, for this creditor financial institution."},{"@id":"unece:fedwireRoutingNumberId","@type":["rdf:Property","owl:DatatypeProperty"],"rdfs:label":"fedwireRoutingNumberId","schema:rangeIncludes":{"@id":"schema:Text"},"schema:domainIncludes":[{"@id":"unece:CreditorFinancialInstitution"},{"@id":"unece:DebtorFinancialInstitution"}],"rdfs:comment":"The unique Fedwire Routing Number identifier as assigned by the American Bankers Association (ABA) for this creditor financial institution."},{"@id":"unece:germanBankleitzahlId","@type":["rdf:Property","owl:DatatypeProperty"],"rdfs:label":"germanBankleitzahlId","schema:rangeIncludes":{"@id":"schema:Text"},"schema:domainIncludes":[{"@id":"unece:CreditorFinancialInstitution"},{"@id":"unece:DebtorFinancialInstitution"}],"rdfs:comment":"The unique German Bankleitzahl identifier for this creditor financial institution."},{"@id":"unece:hellenicBankId","@type":["rdf:Property","owl:DatatypeProperty"],"rdfs:label":"hellenicBankId","schema:rangeIncludes":{"@id":"schema:Text"},"schema:domainIncludes":[{"@id":"unece:CreditorFinancialInstitution"},{"@id":"unece:DebtorFinancialInstitution"}],"rdfs:comment":"The unique Hellenic Bank Identification Code identifier for this creditor financial institution."},{"@id":"unece:hongKongBankId","@type":["rdf:Property","owl:DatatypeProperty"],"rdfs:label":"hongKongBankId","schema:rangeIncludes":{"@id":"schema:Text"},"schema:domainIncludes":[{"@id":"unece:CreditorFinancialInstitution"},{"@id":"unece:DebtorFinancialInstitution"}],"rdfs:comment":"The unique Hong Kong Bank Code identifier for this creditor financial institution."},{"@id":"unece:indianFinancialSystemId","@type":["rdf:Property","owl:DatatypeProperty"],"rdfs:label":"indianFinancialSystemId","schema:rangeIncludes":{"@id":"schema:Text"},"schema:domainIncludes":[{"@id":"unece:CreditorFinancialInstitution"},{"@id":"unece:DebtorFinancialInstitution"}],"rdfs:comment":"The unique Indian Financial System Code identifier for this creditor financial institution."},{"@id":"unece:irishNSCId","@type":["rdf:Property","owl:DatatypeProperty"],"rdfs:label":"irishNSCId","schema:rangeIncludes":{"@id":"schema:Text"},"schema:domainIncludes":[{"@id":"unece:CreditorFinancialInstitution"},{"@id":"unece:DebtorFinancialInstitution"}],"rdfs:comment":"The unique Irish National Sorting Code (NSC) identifier as assigned by the Irish Payments Services Organisation (IPSO) for this creditor financial institution."},{"@id":"unece:italianDomesticId","@type":["rdf:Property","owl:DatatypeProperty"],"rdfs:label":"italianDomesticId","schema:rangeIncludes":{"@id":"schema:Text"},"schema:domainIncludes":[{"@id":"unece:CreditorFinancialInstitution"},{"@id":"unece:DebtorFinancialInstitution"}],"rdfs:comment":"The unique Italian Domestic Identification Code identifier as assigned by the Associazione Bancaria Italiana (ABI) for this creditor financial institution."},{"@id":"unece:japanFinancialInstitutionCommonId","@type":["rdf:Property","owl:DatatypeProperty"],"rdfs:label":"japanFinancialInstitutionCommonId","schema:rangeIncludes":{"@id":"schema:Text"},"schema:domainIncludes":[{"@id":"unece:CreditorFinancialInstitution"},{"@id":"unece:DebtorFinancialInstitution"}],"rdfs:comment":"The Japan Financial Institution Common identifier as assigned by the Japanese Bankers Association for this creditor financial institution."},{"@id":"unece:locationAddress","@type":["rdf:Property","owl:ObjectProperty"],"rdfs:label":"locationAddress","schema:rangeIncludes":{"@id":"unece:FinancialInstitutionAddress"},"schema:domainIncludes":[{"@id":"unece:CreditorFinancialInstitution"},{"@id":"unece:DebtorFinancialInstitution"},{"@id":"unece:BranchFinancialInstitution"}],"rdfs:comment":"The location address for this branch of a financial institution."},{"@id":"unece:newZealandNCCId","@type":["rdf:Property","owl:DatatypeProperty"],"rdfs:label":"newZealandNCCId","schema:rangeIncludes":{"@id":"schema:Text"},"schema:domainIncludes":[{"@id":"unece:CreditorFinancialInstitution"},{"@id":"unece:DebtorFinancialInstitution"}],"rdfs:comment":"The unique New Zealand National Clearing Code (NCC) identifier as assigned by the New Zealand Bankers' Association (NZBA) for this creditor financial institution."},{"@id":"unece:polishNationalClearingId","@type":["rdf:Property","owl:DatatypeProperty"],"rdfs:label":"polishNationalClearingId","schema:rangeIncludes":{"@id":"schema:Text"},"schema:domainIncludes":[{"@id":"unece:CreditorFinancialInstitution"},{"@id":"unece:DebtorFinancialInstitution"}],"rdfs:comment":"The unique Polish National Clearing Code identifier for this creditor financial institution."},{"@id":"unece:portugueseNCCId","@type":["rdf:Property","owl:DatatypeProperty"],"rdfs:label":"portugueseNCCId","schema:rangeIncludes":{"@id":"schema:Text"},"schema:domainIncludes":[{"@id":"unece:CreditorFinancialInstitution"},{"@id":"unece:DebtorFinancialInstitution"}],"rdfs:comment":"The unique Portuguese National Clearing Code (NCC) identifier for this creditor financial institution."},{"@id":"unece:russianCentralBankId","@type":["rdf:Property","owl:DatatypeProperty"],"rdfs:label":"russianCentralBankId","schema:rangeIncludes":{"@id":"schema:Text"},"schema:domainIncludes":[{"@id":"unece:CreditorFinancialInstitution"},{"@id":"unece:DebtorFinancialInstitution"}],"rdfs:comment":"The unique Russian Central Bank Identification Code identifier for this creditor financial institution."},{"@id":"unece:sICId","@type":["rdf:Property","owl:DatatypeProperty"],"rdfs:label":"sICId","schema:rangeIncludes":{"@id":"schema:Text"},"schema:domainIncludes":[{"@id":"unece:CreditorFinancialInstitution"},{"@id":"unece:DebtorFinancialInstitution"}],"rdfs:comment":"The unique Swiss Interbank Clearing (SIC) Code identifier for this creditor financial institution."},{"@id":"unece:southAfricanNCCId","@type":["rdf:Property","owl:DatatypeProperty"],"rdfs:label":"southAfricanNCCId","schema:rangeIncludes":{"@id":"schema:Text"},"schema:domainIncludes":[{"@id":"unece:CreditorFinancialInstitution"},{"@id":"unece:DebtorFinancialInstitution"}],"rdfs:comment":"The unique South African National Clearing Code (NCC) identifier as assigned by the South African Bankers Services Company Ltd. (BankServ) for this creditor financial institution."},{"@id":"unece:spanishDomesticInterbankingId","@type":["rdf:Property","owl:DatatypeProperty"],"rdfs:label":"spanishDomesticInterbankingId","schema:rangeIncludes":{"@id":"schema:Text"},"schema:domainIncludes":[{"@id":"unece:CreditorFinancialInstitution"},{"@id":"unece:DebtorFinancialInstitution"}],"rdfs:comment":"The unique Spanish Domestic Interbanking Code identifier as assigned by the Centro de Cooperacion Interbancaria (CCI) for this creditor financial institution."},{"@id":"unece:subDivisionFinancialInstitution","@type":["rdf:Property","owl:ObjectProperty"],"rdfs:label":"subDivisionFinancialInstitution","schema:rangeIncludes":{"@id":"unece:BranchFinancialInstitution"},"schema:domainIncludes":[{"@id":"unece:CreditorFinancialInstitution"},{"@id":"unece:DebtorFinancialInstitution"}],"rdfs:comment":"The branch financial institution for this creditor financial institution."},{"@id":"unece:swissBCId","@type":["rdf:Property","owl:DatatypeProperty"],"rdfs:label":"swissBCId","schema:rangeIncludes":{"@id":"schema:Text"},"schema:domainIncludes":[{"@id":"unece:CreditorFinancialInstitution"},{"@id":"unece:DebtorFinancialInstitution"}],"rdfs:comment":"The unique Swiss Bank Code (BC) identifier for this creditor financial institution."},{"@id":"unece:uKSortCodeId","@type":["rdf:Property","owl:DatatypeProperty"],"rdfs:label":"uKSortCodeId","schema:rangeIncludes":{"@id":"schema:Text"},"schema:domainIncludes":[{"@id":"unece:CreditorFinancialInstitution"},{"@id":"unece:DebtorFinancialInstitution"}],"rdfs:comment":"The unique United Kingdom (UK) Sort Code identifier as assigned by the UK Payment Association (APACS) for this creditor financial institution."},{"@id":"unece:additionalInformationIncludedNote","@type":["rdf:Property","owl:ObjectProperty"],"rdfs:label":"additionalInformationIncludedNote","schema:rangeIncludes":{"@id":"unece:Note"},"schema:domainIncludes":{"@id":"unece:FinancingRequestDocument"},"rdfs:comment":"A textual or coded description, such as a remark or additional information."},{"@id":"unece:agreementInformation","@type":["rdf:Property","owl:DatatypeProperty"],"rdfs:label":"agreementInformation","schema:rangeIncludes":{"@id":"schema:Text"},"schema:domainIncludes":{"@id":"unece:FinancingRequestDocument"},"rdfs:comment":"Agreement information, expressed as text, in this financing request document, such as a collection mandate."},{"@id":"unece:authorization","@type":["rdf:Property","owl:DatatypeProperty"],"rdfs:label":"authorization","schema:rangeIncludes":{"@id":"schema:Text"},"schema:domainIncludes":{"@id":"unece:FinancingRequestDocument"},"rdfs:comment":"An authorization, expressed as text, for this financing request document."},{"@id":"unece:cancellationReason","@type":["rdf:Property","owl:DatatypeProperty"],"rdfs:label":"cancellationReason","schema:rangeIncludes":{"@id":"schema:Text"},"schema:domainIncludes":{"@id":"unece:FinancingRequestDocument"},"rdfs:comment":"A cancellation reason, expressed as text, in this financing request document."},{"@id":"unece:financingRequestDocumentCurrencyCode","@type":["rdf:Property","owl:DatatypeProperty"],"rdfs:label":"financingRequestDocumentCurrencyCode","schema:rangeIncludes":{"@id":"unece:CurrencyCodeList"},"schema:domainIncludes":{"@id":"unece:FinancingRequestDocument"},"rdfs:comment":"The code specifying the currency in this financing request document."},{"@id":"unece:firstAgentSpecifiedFinancialInstitution","@type":["rdf:Property","owl:ObjectProperty"],"rdfs:label":"firstAgentSpecifiedFinancialInstitution","schema:rangeIncludes":{"@id":"unece:CreditorFinancialInstitution"},"schema:domainIncludes":{"@id":"unece:FinancingRequestDocument"},"rdfs:comment":"The creditor financial institution specified as the first agent in this financing request document."},{"@id":"unece:groupId","@type":["rdf:Property","owl:DatatypeProperty"],"rdfs:label":"groupId","schema:rangeIncludes":{"@id":"schema:Text"},"schema:domainIncludes":{"@id":"unece:FinancingRequestDocument"},"rdfs:comment":"The group identifier in this financing request document."},{"@id":"unece:groupedTransactionSpecifiedQuantity","@type":["rdf:Property","owl:ObjectProperty"],"rdfs:label":"groupedTransactionSpecifiedQuantity","schema:rangeIncludes":{"@id":"unece:QuantityType"},"schema:domainIncludes":{"@id":"unece:FinancingRequestDocument"},"rdfs:comment":""},{"@id":"unece:groupedTransactionTotalAmount","@type":["rdf:Property","owl:ObjectProperty"],"rdfs:label":"groupedTransactionTotalAmount","schema:rangeIncludes":{"@id":"unece:AmountType"},"schema:domainIncludes":{"@id":"unece:FinancingRequestDocument"},"rdfs:comment":""},{"@id":"unece:intermediarySpecifiedFinancialInstitution","@type":["rdf:Property","owl:ObjectProperty"],"rdfs:label":"intermediarySpecifiedFinancialInstitution","schema:rangeIncludes":{"@id":"unece:CreditorFinancialInstitution"},"schema:domainIncludes":{"@id":"unece:FinancingRequestDocument"},"rdfs:comment":"The creditor financial institution specified as the intermediary in this financing request document."},{"@id":"unece:specifiedCancellationStatus","@type":["rdf:Property","owl:ObjectProperty"],"rdfs:label":"specifiedCancellationStatus","schema:rangeIncludes":{"@id":"unece:CancellationStatus"},"schema:domainIncludes":{"@id":"unece:FinancingRequestDocument"},"rdfs:comment":"Information relevant to a condition of a cancellation."},{"@id":"unece:specifiedRequestingParty","@type":["rdf:Property","owl:ObjectProperty"],"rdfs:label":"specifiedRequestingParty","schema:rangeIncludes":{"@id":"unece:RequestingParty"},"schema:domainIncludes":{"@id":"unece:FinancingRequestDocument"},"rdfs:comment":"The requesting party specified in this financing request document."},{"@id":"unece:specifiedValidationStatus","@type":["rdf:Property","owl:ObjectProperty"],"rdfs:label":"specifiedValidationStatus","schema:rangeIncludes":{"@id":"unece:ValidationStatus"},"schema:domainIncludes":{"@id":"unece:FinancingRequestDocument"},"rdfs:comment":"Information relevant to a condition of a validation."},{"@id":"unece:agentAssignedCustomerId","@type":["rdf:Property","owl:DatatypeProperty"],"rdfs:label":"agentAssignedCustomerId","schema:rangeIncludes":{"@id":"schema:Text"},"schema:domainIncludes":{"@id":"unece:FinancialIdentity"},"rdfs:comment":"The agent assigned customer identifier for this financial identity."},{"@id":"unece:bEIId","@type":["rdf:Property","owl:DatatypeProperty"],"rdfs:label":"bEIId","schema:rangeIncludes":{"@id":"schema:Text"},"schema:domainIncludes":[{"@id":"unece:FinancialIdentity"},{"@id":"unece:PaymentFinancialInstitution"},{"@id":"unece:RequestingParty"}],"rdfs:comment":"The Business Entity Identifier (BEI) as defined by ISO 9362 (Banking telecommunication messages, Bank Identifier Codes) for this financial identity."},{"@id":"unece:bankAssignedId","@type":["rdf:Property","owl:DatatypeProperty"],"rdfs:label":"bankAssignedId","schema:rangeIncludes":{"@id":"schema:Text"},"schema:domainIncludes":{"@id":"unece:FinancialIdentity"},"rdfs:comment":"The bank assigned identifier for this financial identity."},{"@id":"unece:iBEIId","@type":["rdf:Property","owl:DatatypeProperty"],"rdfs:label":"iBEIId","schema:rangeIncludes":{"@id":"schema:Text"},"schema:domainIncludes":{"@id":"unece:FinancialIdentity"},"rdfs:comment":"The International Business Entity Identifier (IBEI) for this financial identity."},{"@id":"unece:applicableFinancialCard","@type":["rdf:Property","owl:ObjectProperty"],"rdfs:label":"applicableFinancialCard","schema:rangeIncludes":{"@id":"unece:FinancialCard"},"schema:domainIncludes":{"@id":"unece:PaymentMeans"},"rdfs:comment":"A financial card applicable to this trade settlement payment means."},{"@id":"unece:creditorSpecifiedFinancialInstitution","@type":["rdf:Property","owl:ObjectProperty"],"rdfs:label":"creditorSpecifiedFinancialInstitution","schema:rangeIncludes":{"@id":"unece:PaymentFinancialInstitution"},"schema:domainIncludes":{"@id":"unece:PaymentMeans"},"rdfs:comment":"A creditor financial institution specified for this trade settlement payment means."},{"@id":"unece:debtorSpecifiedFinancialInstitution","@type":["rdf:Property","owl:ObjectProperty"],"rdfs:label":"debtorSpecifiedFinancialInstitution","schema:rangeIncludes":{"@id":"unece:PaymentFinancialInstitution"},"schema:domainIncludes":{"@id":"unece:PaymentMeans"},"rdfs:comment":"A debtor financial institution specified for this trade settlement payment means."},{"@id":"unece:identifiedCash","@type":["rdf:Property","owl:ObjectProperty"],"rdfs:label":"identifiedCash","schema:rangeIncludes":{"@id":"unece:Cash"},"schema:domainIncludes":{"@id":"unece:PaymentMeans"},"rdfs:comment":"A cash payment identified for this trade settlement payment means."},{"@id":"unece:identifiedCheque","@type":["rdf:Property","owl:ObjectProperty"],"rdfs:label":"identifiedCheque","schema:rangeIncludes":{"@id":"unece:Cheque"},"schema:domainIncludes":{"@id":"unece:PaymentMeans"},"rdfs:comment":"A cheque payment identified for this trade settlement payment means."},{"@id":"unece:identifiedDigitalMethod","@type":["rdf:Property","owl:ObjectProperty"],"rdfs:label":"identifiedDigitalMethod","schema:rangeIncludes":{"@id":"unece:DigitalMethod"},"schema:domainIncludes":{"@id":"unece:PaymentMeans"},"rdfs:comment":"A digital payment method identified for this trade settlement payment means."},{"@id":"unece:identifiedFinancialCard","@type":["rdf:Property","owl:ObjectProperty"],"rdfs:label":"identifiedFinancialCard","schema:rangeIncludes":{"@id":"unece:FinancialCard"},"schema:domainIncludes":{"@id":"unece:PaymentMeans"},"rdfs:comment":"A financial card identified for this trade settlement payment means."},{"@id":"unece:identifiedVoucher","@type":["rdf:Property","owl:ObjectProperty"],"rdfs:label":"identifiedVoucher","schema:rangeIncludes":{"@id":"unece:Voucher"},"schema:domainIncludes":{"@id":"unece:PaymentMeans"},"rdfs:comment":"An experience item voucher identified for this trade settlement payment means."},{"@id":"unece:payeePartyFinancialAccount","@type":["rdf:Property","owl:ObjectProperty"],"rdfs:label":"payeePartyFinancialAccount","schema:rangeIncludes":{"@id":"unece:CreditorFinancialAccount"},"schema:domainIncludes":{"@id":"unece:PaymentMeans"},"rdfs:comment":"A creditor financial account of the payee party for this trade settlement payment means."},{"@id":"unece:payeeSpecifiedFinancialInstitution","@type":["rdf:Property","owl:ObjectProperty"],"rdfs:label":"payeeSpecifiedFinancialInstitution","schema:rangeIncludes":{"@id":"unece:CreditorFinancialInstitution"},"schema:domainIncludes":{"@id":"unece:PaymentMeans"},"rdfs:comment":"The creditor financial institution of the payee party specified for this trade settlement payment means."},{"@id":"unece:payerPartyFinancialAccount","@type":["rdf:Property","owl:ObjectProperty"],"rdfs:label":"payerPartyFinancialAccount","schema:rangeIncludes":{"@id":"unece:DebtorFinancialAccount"},"schema:domainIncludes":{"@id":"unece:PaymentMeans"},"rdfs:comment":"The debtor financial account of the payer party for this trade settlement payment means."},{"@id":"unece:payerSpecifiedFinancialInstitution","@type":["rdf:Property","owl:ObjectProperty"],"rdfs:label":"payerSpecifiedFinancialInstitution","schema:rangeIncludes":{"@id":"unece:DebtorFinancialInstitution"},"schema:domainIncludes":{"@id":"unece:PaymentMeans"},"rdfs:comment":"The debtor financial institution of the payer party specified for this trade settlement payment means."},{"@id":"unece:paymentGuaranteeMeansGuaranteeMethodCode","@type":["rdf:Property","owl:DatatypeProperty"],"rdfs:label":"paymentGuaranteeMeansGuaranteeMethodCode","schema:rangeIncludes":{"@id":"unece:PaymentGuaranteeMeansCodeList"},"schema:domainIncludes":{"@id":"unece:PaymentMeans"},"rdfs:comment":"The code specifying the method of guarantee for this trade settlement payment means."},{"@id":"unece:paymentMeansChannelPaymentChannelCode","@type":["rdf:Property","owl:DatatypeProperty"],"rdfs:label":"paymentMeansChannelPaymentChannelCode","schema:rangeIncludes":{"@id":"unece:PaymentMeansChannelCodeList"},"schema:domainIncludes":{"@id":"unece:PaymentMeans"},"rdfs:comment":"The code specifying the payment channel through which this trade settlement payment is to be processed (Reference United Nations Code List (UNCL) 4435)."},{"@id":"unece:paymentMeansTypeCode","@type":["rdf:Property","owl:DatatypeProperty"],"rdfs:label":"paymentMeansTypeCode","schema:rangeIncludes":{"@id":"unece:PaymentMeansCodeList"},"schema:domainIncludes":{"@id":"unece:PaymentMeans"},"rdfs:comment":"The code specifying the type of trade settlement payment means, such as cash or check."},{"@id":"unece:paymentMethodCode","@type":["rdf:Property","owl:DatatypeProperty"],"rdfs:label":"paymentMethodCode","schema:rangeIncludes":{"@id":"schema:Text"},"schema:domainIncludes":{"@id":"unece:PaymentMeans"},"rdfs:comment":"The code specifying the method by which a payment may be made for this trade settlement payment means."},{"@id":"unece:specifiedPaymentFinancialInstitution","@type":["rdf:Property","owl:ObjectProperty"],"rdfs:label":"specifiedPaymentFinancialInstitution","schema:rangeIncludes":{"@id":"unece:PaymentFinancialInstitution"},"schema:domainIncludes":{"@id":"unece:PaymentMeans"},"rdfs:comment":"A financial institution specified for this trade settlement payment means."},{"@id":"unece:tradeSettlementPaymentMeansId","@type":["rdf:Property","owl:DatatypeProperty"],"rdfs:label":"tradeSettlementPaymentMeansId","schema:rangeIncludes":{"@id":"schema:Text"},"schema:domainIncludes":{"@id":"unece:PaymentMeans"},"rdfs:comment":"An identifier for this trade settlement payment means."},{"@id":"unece:applicableIndicator","@type":["rdf:Property","owl:DatatypeProperty"],"rdfs:label":"applicableIndicator","schema:rangeIncludes":{"@id":"schema:Boolean"},"schema:domainIncludes":[{"@id":"unece:Cash"},{"@id":"unece:Cheque"},{"@id":"unece:DigitalMethod"},{"@id":"unece:FinancialCard"},{"@id":"unece:Voucher"}],"rdfs:comment":"The indication of whether or not this cash used for payment. is applicable."},{"@id":"unece:clearingRegion","@type":["rdf:Property","owl:DatatypeProperty"],"rdfs:label":"clearingRegion","schema:rangeIncludes":{"@id":"schema:Text"},"schema:domainIncludes":{"@id":"unece:Cheque"},"rdfs:comment":"The clearing region, expressed as text, for this payment cheque."},{"@id":"unece:deliveryMethod","@type":["rdf:Property","owl:DatatypeProperty"],"rdfs:label":"deliveryMethod","schema:rangeIncludes":{"@id":"schema:Text"},"schema:domainIncludes":{"@id":"unece:Cheque"},"rdfs:comment":"The delivery method, expressed as text, for this payment cheque."},{"@id":"unece:deliveryMethodCode","@type":["rdf:Property","owl:DatatypeProperty"],"rdfs:label":"deliveryMethodCode","schema:rangeIncludes":{"@id":"schema:Text"},"schema:domainIncludes":{"@id":"unece:Cheque"},"rdfs:comment":"The code specifying the delivery method for this payment cheque."},{"@id":"unece:instructionPriorityCode","@type":["rdf:Property","owl:DatatypeProperty"],"rdfs:label":"instructionPriorityCode","schema:rangeIncludes":{"@id":"schema:Text"},"schema:domainIncludes":{"@id":"unece:Cheque"},"rdfs:comment":"The code specifying the instruction priority for this payment cheque, such as the urgency or order of importance for the processing of the payment cheque."},{"@id":"unece:layoutDescription","@type":["rdf:Property","owl:DatatypeProperty"],"rdfs:label":"layoutDescription","schema:rangeIncludes":{"@id":"schema:Text"},"schema:domainIncludes":{"@id":"unece:Cheque"},"rdfs:comment":"The textual description of the layout for this payment cheque, such as a description of the company logo and digitized signature printed on the cheque."},{"@id":"unece:maturityDateTime","@type":["rdf:Property","owl:DatatypeProperty"],"rdfs:label":"maturityDateTime","schema:rangeIncludes":{"@id":"schema:Text"},"schema:domainIncludes":{"@id":"unece:Cheque"},"rdfs:comment":"The date, time, date time, or other date time value when this payment cheque reaches maturity."},{"@id":"unece:memoField","@type":["rdf:Property","owl:DatatypeProperty"],"rdfs:label":"memoField","schema:rangeIncludes":{"@id":"schema:Text"},"schema:domainIncludes":{"@id":"unece:Cheque"},"rdfs:comment":"The memo field, expressed as text, on this payment check."},{"@id":"unece:number","@type":["rdf:Property","owl:DatatypeProperty"],"rdfs:label":"number","schema:rangeIncludes":{"@id":"schema:Text"},"schema:domainIncludes":{"@id":"unece:Cheque"},"rdfs:comment":"The number, expressed as text, of this payment cheque."},{"@id":"unece:printLocation","@type":["rdf:Property","owl:DatatypeProperty"],"rdfs:label":"printLocation","schema:rangeIncludes":{"@id":"schema:Text"},"schema:domainIncludes":{"@id":"unece:Cheque"},"rdfs:comment":"The print location, expressed as text, for this payment cheque."},{"@id":"unece:cardholderName","@type":["rdf:Property","owl:DatatypeProperty"],"rdfs:label":"cardholderName","schema:rangeIncludes":{"@id":"schema:Text"},"schema:domainIncludes":[{"@id":"unece:DigitalMethod"},{"@id":"unece:FinancialCard"}],"rdfs:comment":"A cardholder's name, expressed as text, for this digital method used for payment."},{"@id":"unece:issuingCompanyName","@type":["rdf:Property","owl:DatatypeProperty"],"rdfs:label":"issuingCompanyName","schema:rangeIncludes":{"@id":"schema:Text"},"schema:domainIncludes":[{"@id":"unece:DigitalMethod"},{"@id":"unece:FinancialCard"},{"@id":"unece:Voucher"}],"rdfs:comment":"A name, expressed as text, of the company issuing this experience item voucher."},{"@id":"unece:validFromDateTime","@type":["rdf:Property","owl:DatatypeProperty"],"rdfs:label":"validFromDateTime","schema:rangeIncludes":{"@id":"schema:Text"},"schema:domainIncludes":[{"@id":"unece:DigitalMethod"},{"@id":"unece:FinancialCard"}],"rdfs:comment":"The date from which this trade settlement financial card is valid."},{"@id":"unece:verificationNumeric","@type":["rdf:Property","owl:DatatypeProperty"],"rdfs:label":"verificationNumeric","schema:rangeIncludes":{"@id":"schema:Text"},"schema:domainIncludes":[{"@id":"unece:DigitalMethod"},{"@id":"unece:FinancialCard"}],"rdfs:comment":"The unique card verification number for security purposes to help verify the card user is in actual possession of this trade settlement financial card."},{"@id":"unece:creditAvailableAmount","@type":["rdf:Property","owl:ObjectProperty"],"rdfs:label":"creditAvailableAmount","schema:rangeIncludes":{"@id":"unece:AmountType"},"schema:domainIncludes":{"@id":"unece:FinancialCard"},"rdfs:comment":""},{"@id":"unece:creditLimitAmount","@type":["rdf:Property","owl:ObjectProperty"],"rdfs:label":"creditLimitAmount","schema:rangeIncludes":{"@id":"unece:AmountType"},"schema:domainIncludes":{"@id":"unece:FinancialCard"},"rdfs:comment":""},{"@id":"unece:expiryDate","@type":["rdf:Property","owl:DatatypeProperty"],"rdfs:label":"expiryDate","schema:rangeIncludes":{"@id":"schema:Text"},"schema:domainIncludes":{"@id":"unece:FinancialCard"},"rdfs:comment":"The date of expiry up to which this trade settlement financial card is valid."},{"@id":"unece:interestRatePercent","@type":["rdf:Property","owl:DatatypeProperty"],"rdfs:label":"interestRatePercent","schema:rangeIncludes":{"@id":"schema:Text"},"schema:domainIncludes":{"@id":"unece:FinancialCard"},"rdfs:comment":"The interest rate expressed as a percentage for this trade settlement financial card."},{"@id":"unece:microchipIndicator","@type":["rdf:Property","owl:DatatypeProperty"],"rdfs:label":"microchipIndicator","schema:rangeIncludes":{"@id":"schema:Boolean"},"schema:domainIncludes":{"@id":"unece:FinancialCard"},"rdfs:comment":"The indication of whether or not this trade settlement financial card has a microchip."},{"@id":"unece:applicablePaymentDiscountTerms","@type":["rdf:Property","owl:ObjectProperty"],"rdfs:label":"applicablePaymentDiscountTerms","schema:rangeIncludes":{"@id":"unece:PaymentDiscountTerms"},"schema:domainIncludes":{"@id":"unece:PaymentTerms"},"rdfs:comment":"Trade payment discount terms applicable to these trade payment terms."},{"@id":"unece:applicablePaymentPenaltyTerms","@type":["rdf:Property","owl:ObjectProperty"],"rdfs:label":"applicablePaymentPenaltyTerms","schema:rangeIncludes":{"@id":"unece:PaymentPenaltyTerms"},"schema:domainIncludes":{"@id":"unece:PaymentTerms"},"rdfs:comment":"Trade payment penalty terms applicable to these trade payment terms."},{"@id":"unece:billStartDateTime","@type":["rdf:Property","owl:DatatypeProperty"],"rdfs:label":"billStartDateTime","schema:rangeIncludes":{"@id":"schema:Text"},"schema:domainIncludes":{"@id":"unece:PaymentTerms"},"rdfs:comment":"The date, time, date time, or other date time value of the bill start specified by these trade payment terms."},{"@id":"unece:instructionCode","@type":["rdf:Property","owl:DatatypeProperty"],"rdfs:label":"instructionCode","schema:rangeIncludes":{"@id":"schema:Text"},"schema:domainIncludes":[{"@id":"unece:PaymentTerms"},{"@id":"unece:LogisticsPackaging"},{"@id":"unece:SupplyChainPackaging"}],"rdfs:comment":"A code specifying an instruction for these trade payment terms."},{"@id":"unece:partialPaymentAmount","@type":["rdf:Property","owl:ObjectProperty"],"rdfs:label":"partialPaymentAmount","schema:rangeIncludes":{"@id":"unece:AmountType"},"schema:domainIncludes":{"@id":"unece:PaymentTerms"},"rdfs:comment":""},{"@id":"unece:partialPaymentPercent","@type":["rdf:Property","owl:DatatypeProperty"],"rdfs:label":"partialPaymentPercent","schema:rangeIncludes":{"@id":"schema:Text"},"schema:domainIncludes":{"@id":"unece:PaymentTerms"},"rdfs:comment":"A partial payment, expressed as a percent, in these trade payment terms."},{"@id":"unece:paymentTermsEventTimeReferenceFromEventCode","@type":["rdf:Property","owl:DatatypeProperty"],"rdfs:label":"paymentTermsEventTimeReferenceFromEventCode","schema:rangeIncludes":{"@id":"unece:PaymentTermsEventTimeReferenceCodeList"},"schema:domainIncludes":{"@id":"unece:PaymentTerms"},"rdfs:comment":"The code specifying the event from which these trade payment terms are offered for a length of time."},{"@id":"unece:paymentTermsId","@type":["rdf:Property","owl:DatatypeProperty"],"rdfs:label":"paymentTermsId","schema:rangeIncludes":{"@id":"unece:PaymentTermsId"},"schema:domainIncludes":{"@id":"unece:PaymentTerms"},"rdfs:comment":"The unique identifier of these trade payment terms."},{"@id":"unece:paymentTermsTypeCode","@type":["rdf:Property","owl:DatatypeProperty"],"rdfs:label":"paymentTermsTypeCode","schema:rangeIncludes":{"@id":"unece:PaymentTermsTypeCodeList"},"schema:domainIncludes":{"@id":"unece:PaymentTerms"},"rdfs:comment":"A code specifying the type of trade payment terms."},{"@id":"unece:settlementPeriodMeasure","@type":["rdf:Property","owl:ObjectProperty"],"rdfs:label":"settlementPeriodMeasure","schema:rangeIncludes":{"@id":"unece:MeasureType"},"schema:domainIncludes":{"@id":"unece:PaymentTerms"},"rdfs:comment":""},{"@id":"unece:tradePaymentTermsDirectDebitMandateId","@type":["rdf:Property","owl:DatatypeProperty"],"rdfs:label":"tradePaymentTermsDirectDebitMandateId","schema:rangeIncludes":{"@id":"schema:Text"},"schema:domainIncludes":{"@id":"unece:PaymentTerms"},"rdfs:comment":"An identifier of a direct debit mandate in these trade payment terms."},{"@id":"unece:tradePaymentTermsInstructionTypeCode","@type":["rdf:Property","owl:DatatypeProperty"],"rdfs:label":"tradePaymentTermsInstructionTypeCode","schema:rangeIncludes":{"@id":"schema:Text"},"schema:domainIncludes":{"@id":"unece:PaymentTerms"},"rdfs:comment":"A code specifying a type of instruction for these trade payment terms."},{"@id":"unece:tradePaymentTermsPaymentMeansId","@type":["rdf:Property","owl:DatatypeProperty"],"rdfs:label":"tradePaymentTermsPaymentMeansId","schema:rangeIncludes":{"@id":"schema:Text"},"schema:domainIncludes":{"@id":"unece:PaymentTerms"},"rdfs:comment":"An identifier of a payment means in these trade payment terms."},{"@id":"unece:appliedTaxTypeCode","@type":["rdf:Property","owl:DatatypeProperty"],"rdfs:label":"appliedTaxTypeCode","schema:rangeIncludes":{"@id":"schema:Text"},"schema:domainIncludes":{"@id":"unece:AppliedTax"},"rdfs:comment":"The code specifying the applied tax type such as VAT."},{"@id":"unece:branchName","@type":["rdf:Property","owl:DatatypeProperty"],"rdfs:label":"branchName","schema:rangeIncludes":{"@id":"schema:Text"},"schema:domainIncludes":{"@id":"unece:PaymentFinancialInstitution"},"rdfs:comment":"A branch name, expressed as text, for this payment financial institution."},{"@id":"unece:branchNameId","@type":["rdf:Property","owl:DatatypeProperty"],"rdfs:label":"branchNameId","schema:rangeIncludes":{"@id":"schema:Text"},"schema:domainIncludes":{"@id":"unece:PaymentFinancialInstitution"},"rdfs:comment":"The identifier of the branch name for this payment financial institution."},{"@id":"unece:nameId","@type":["rdf:Property","owl:DatatypeProperty"],"rdfs:label":"nameId","schema:rangeIncludes":{"@id":"schema:Text"},"schema:domainIncludes":{"@id":"unece:PaymentFinancialInstitution"},"rdfs:comment":"The identifier of the name for this payment financial institution."},{"@id":"unece:specifiedCommunication","@type":["rdf:Property","owl:ObjectProperty"],"rdfs:label":"specifiedCommunication","schema:rangeIncludes":{"@id":"unece:Communication"},"schema:domainIncludes":[{"@id":"unece:PaymentFinancialInstitution"},{"@id":"unece:ExperienceFacility"}],"rdfs:comment":"The exchange of thoughts, messages, or information, as universally exchanged by speech, signals, writing, or behaviour between persons and/or organizations."},{"@id":"unece:specifiedPaymentFinancialAccount","@type":["rdf:Property","owl:ObjectProperty"],"rdfs:label":"specifiedPaymentFinancialAccount","schema:rangeIncludes":{"@id":"unece:PaymentFinancialAccount"},"schema:domainIncludes":{"@id":"unece:PaymentFinancialInstitution"},"rdfs:comment":"A payment financial account specified for this payment financial institution."},{"@id":"unece:binaryFile","@type":["rdf:Property","owl:ObjectProperty"],"rdfs:label":"binaryFile","schema:rangeIncludes":{"@id":"unece:BinaryFile"},"schema:domainIncludes":[{"@id":"unece:BreakdownStatement"},{"@id":"unece:BasicWorkItem"},{"@id":"unece:GroupedWorkItem"}],"rdfs:comment":"A specified computer file or program stored in a binary format."},{"@id":"unece:comment","@type":["rdf:Property","owl:DatatypeProperty"],"rdfs:label":"comment","schema:rangeIncludes":{"@id":"schema:Text"},"schema:domainIncludes":[{"@id":"unece:BreakdownStatement"},{"@id":"unece:BasicWorkItem"},{"@id":"unece:GroupedWorkItem"},{"@id":"unece:InspectionReference"},{"@id":"unece:LaboratoryObservationReference"},{"@id":"unece:Illness"},{"@id":"unece:SupplyChainReference"}],"rdfs:comment":"A comment, expressed as text for this MDH illness."},{"@id":"unece:creationBinaryFile","@type":["rdf:Property","owl:ObjectProperty"],"rdfs:label":"creationBinaryFile","schema:rangeIncludes":{"@id":"unece:BinaryFile"},"schema:domainIncludes":{"@id":"unece:BreakdownStatement"},"rdfs:comment":"A specified computer file or program stored in a binary format."},{"@id":"unece:defaultCurrencyCode","@type":["rdf:Property","owl:DatatypeProperty"],"rdfs:label":"defaultCurrencyCode","schema:rangeIncludes":{"@id":"unece:CurrencyCodeList"},"schema:domainIncludes":{"@id":"unece:BreakdownStatement"},"rdfs:comment":"The code specifying the default currency for this valuation breakdown statement."},{"@id":"unece:defaultLanguageCode","@type":["rdf:Property","owl:DatatypeProperty"],"rdfs:label":"defaultLanguageCode","schema:rangeIncludes":{"@id":"schema:Text"},"schema:domainIncludes":{"@id":"unece:BreakdownStatement"},"rdfs:comment":"The code specifying the default language for this valuation breakdown statement."},{"@id":"unece:itemBasicWorkItem","@type":["rdf:Property","owl:ObjectProperty"],"rdfs:label":"itemBasicWorkItem","schema:rangeIncludes":{"@id":"unece:BasicWorkItem"},"schema:domainIncludes":[{"@id":"unece:BreakdownStatement"},{"@id":"unece:BasicWorkItem"},{"@id":"unece:GroupedWorkItem"}],"rdfs:comment":"A basic work item in this basic work item."},{"@id":"unece:itemGroupedWorkItem","@type":["rdf:Property","owl:ObjectProperty"],"rdfs:label":"itemGroupedWorkItem","schema:rangeIncludes":{"@id":"unece:GroupedWorkItem"},"schema:domainIncludes":[{"@id":"unece:BreakdownStatement"},{"@id":"unece:GroupedWorkItem"}],"rdfs:comment":"A grouped work item in this valuation breakdown statement."},{"@id":"unece:measurementMethodId","@type":["rdf:Property","owl:DatatypeProperty"],"rdfs:label":"measurementMethodId","schema:rangeIncludes":{"@id":"schema:Text"},"schema:domainIncludes":{"@id":"unece:BreakdownStatement"},"rdfs:comment":"A unique identifier of a method of measurement for this valuation breakdown statement."},{"@id":"unece:priceListId","@type":["rdf:Property","owl:DatatypeProperty"],"rdfs:label":"priceListId","schema:rangeIncludes":{"@id":"schema:Text"},"schema:domainIncludes":{"@id":"unece:BreakdownStatement"},"rdfs:comment":"The identifier of a price list for this valuation breakdown statement."},{"@id":"unece:readerBinaryFile","@type":["rdf:Property","owl:ObjectProperty"],"rdfs:label":"readerBinaryFile","schema:rangeIncludes":{"@id":"unece:BinaryFile"},"schema:domainIncludes":{"@id":"unece:BreakdownStatement"},"rdfs:comment":"A specified computer file or program stored in a binary format."},{"@id":"unece:totalPrice","@type":["rdf:Property","owl:ObjectProperty"],"rdfs:label":"totalPrice","schema:rangeIncludes":{"@id":"unece:CalculatedPrice"},"schema:domainIncludes":[{"@id":"unece:BreakdownStatement"},{"@id":"unece:BasicWorkItem"},{"@id":"unece:GroupedWorkItem"}],"rdfs:comment":"A total calculated price for this basic work item."},{"@id":"unece:breakdownBalanceOut","@type":["rdf:Property","owl:ObjectProperty"],"rdfs:label":"breakdownBalanceOut","schema:rangeIncludes":{"@id":"unece:HeaderBalanceOut"},"schema:domainIncludes":{"@id":"unece:HeaderBalanceOut"},"rdfs:comment":"A balance out breakdown of this header balance out."},{"@id":"unece:reasonDescription","@type":["rdf:Property","owl:DatatypeProperty"],"rdfs:label":"reasonDescription","schema:rangeIncludes":{"@id":"schema:Text"},"schema:domainIncludes":[{"@id":"unece:HeaderBalanceOut"},{"@id":"unece:PaymentBalanceOut"}],"rdfs:comment":"A textual description of the reason for this header balance out."},{"@id":"unece:financialInstitutionAddressTypeCode","@type":["rdf:Property","owl:DatatypeProperty"],"rdfs:label":"financialInstitutionAddressTypeCode","schema:rangeIncludes":{"@id":"schema:Text"},"schema:domainIncludes":{"@id":"unece:FinancialInstitutionAddress"},"rdfs:comment":"The code specifying the type of financial institution address."},{"@id":"unece:effectiveDelimitedPeriod","@type":["rdf:Property","owl:ObjectProperty"],"rdfs:label":"effectiveDelimitedPeriod","schema:rangeIncludes":{"@id":"unece:DelimitedPeriod"},"schema:domainIncludes":{"@id":"unece:Guarantee"},"rdfs:comment":"A period of time from a start date time onwards up to an end date time."},{"@id":"unece:liabilityAmount","@type":["rdf:Property","owl:ObjectProperty"],"rdfs:label":"liabilityAmount","schema:rangeIncludes":{"@id":"unece:AmountType"},"schema:domainIncludes":{"@id":"unece:Guarantee"},"rdfs:comment":""},{"@id":"unece:exemptionReasonCode","@type":["rdf:Property","owl:DatatypeProperty"],"rdfs:label":"exemptionReasonCode","schema:rangeIncludes":{"@id":"schema:Text"},"schema:domainIncludes":{"@id":"unece:RegisteredTax"},"rdfs:comment":"The code specifying the exemption reason for this registered tax."},{"@id":"unece:registeredTaxTypeCode","@type":["rdf:Property","owl:DatatypeProperty"],"rdfs:label":"registeredTaxTypeCode","schema:rangeIncludes":{"@id":"schema:Text"},"schema:domainIncludes":{"@id":"unece:RegisteredTax"},"rdfs:comment":"The code specifying the type of registered tax."},{"@id":"unece:paidAmount","@type":["rdf:Property","owl:ObjectProperty"],"rdfs:label":"paidAmount","schema:rangeIncludes":{"@id":"unece:AmountType"},"schema:domainIncludes":[{"@id":"unece:InstalmentPayment"},{"@id":"unece:AdvancePayment"}],"rdfs:comment":""},{"@id":"unece:sequenceId","@type":["rdf:Property","owl:DatatypeProperty"],"rdfs:label":"sequenceId","schema:rangeIncludes":{"@id":"schema:Text"},"schema:domainIncludes":{"@id":"unece:InstalmentPayment"},"rdfs:comment":"The sequence identifier for this instalment payment."},{"@id":"unece:specifiedFinancingRequestResultDocument","@type":["rdf:Property","owl:ObjectProperty"],"rdfs:label":"specifiedFinancingRequestResultDocument","schema:rangeIncludes":{"@id":"unece:FinancingRequestResultDocument"},"schema:domainIncludes":{"@id":"unece:InstalmentPayment"},"rdfs:comment":"The financing request result document specified for this instalment payment."},{"@id":"unece:financedRatePercent","@type":["rdf:Property","owl:DatatypeProperty"],"rdfs:label":"financedRatePercent","schema:rangeIncludes":{"@id":"schema:Text"},"schema:domainIncludes":{"@id":"unece:FinancingRequestResultDocument"},"rdfs:comment":"The financed rate, expressed as a percentage, in this financing request result document."},{"@id":"unece:specifiedFinancingStatus","@type":["rdf:Property","owl:ObjectProperty"],"rdfs:label":"specifiedFinancingStatus","schema:rangeIncludes":{"@id":"unece:FinancingStatus"},"schema:domainIncludes":{"@id":"unece:FinancingRequestResultDocument"},"rdfs:comment":"The financing status specified in this financing request result document."},{"@id":"unece:financingStatusConditionCode","@type":["rdf:Property","owl:DatatypeProperty"],"rdfs:label":"financingStatusConditionCode","schema:rangeIncludes":{"@id":"unece:FinancingStatusCodeList"},"schema:domainIncludes":{"@id":"unece:FinancingStatus"},"rdfs:comment":"The code specifying the condition of this financing status."},{"@id":"unece:financingStatusReasonCode","@type":["rdf:Property","owl:DatatypeProperty"],"rdfs:label":"financingStatusReasonCode","schema:rangeIncludes":{"@id":"unece:FinancingStatusReasonCodeList"},"schema:domainIncludes":{"@id":"unece:FinancingStatus"},"rdfs:comment":"The code specifying the reason for this financing status."},{"@id":"unece:includedTax","@type":["rdf:Property","owl:ObjectProperty"],"rdfs:label":"includedTax","schema:rangeIncludes":{"@id":"unece:Tax"},"schema:domainIncludes":[{"@id":"unece:AdvancePayment"},{"@id":"unece:TradePrice"}],"rdfs:comment":"A tax included in this advance payment."},{"@id":"unece:receivedDateTime","@type":["rdf:Property","owl:DatatypeProperty"],"rdfs:label":"receivedDateTime","schema:rangeIncludes":{"@id":"schema:DateTime"},"schema:domainIncludes":[{"@id":"unece:AdvancePayment"},{"@id":"unece:TransportEvent"}],"rdfs:comment":"The date, time, date time, or other date time value when information related to this transport event was received, from the perspective of the receiver."},{"@id":"unece:specifiedInstalmentPayment","@type":["rdf:Property","owl:ObjectProperty"],"rdfs:label":"specifiedInstalmentPayment","schema:rangeIncludes":{"@id":"unece:InstalmentPayment"},"schema:domainIncludes":{"@id":"unece:InstalmentPlan"},"rdfs:comment":"An instalment payment specified for this instalment plan."},{"@id":"unece:accessRightsTypeAccessRightsCode","@type":["rdf:Property","owl:DatatypeProperty"],"rdfs:label":"accessRightsTypeAccessRightsCode","schema:rangeIncludes":{"@id":"unece:AccessRightsTypeCodeList"},"schema:domainIncludes":{"@id":"unece:RequestingParty"},"rdfs:comment":"The code specifying the access rights, such as unlimited, restricted, prohibited, for this requesting party."},{"@id":"unece:languageCode","@type":["rdf:Property","owl:DatatypeProperty"],"rdfs:label":"languageCode","schema:rangeIncludes":{"@id":"schema:Text"},"schema:domainIncludes":{"@id":"unece:RequestingParty"},"rdfs:comment":"A code specifying a language for this requesting party."},{"@id":"unece:actualComplexDescription","@type":["rdf:Property","owl:ObjectProperty"],"rdfs:label":"actualComplexDescription","schema:rangeIncludes":{"@id":"unece:ComplexDescription"},"schema:domainIncludes":[{"@id":"unece:BasicWorkItem"},{"@id":"unece:GroupedWorkItem"}],"rdfs:comment":"An aggregation of descriptive information consisting of different but related characteristics that together constitute a work item complex description."},{"@id":"unece:index","@type":["rdf:Property","owl:DatatypeProperty"],"rdfs:label":"index","schema:rangeIncludes":{"@id":"schema:Text"},"schema:domainIncludes":[{"@id":"unece:BasicWorkItem"},{"@id":"unece:GroupedWorkItem"}],"rdfs:comment":"The index, expressed as text, to be used for this basic work item."},{"@id":"unece:priceListItemId","@type":["rdf:Property","owl:DatatypeProperty"],"rdfs:label":"priceListItemId","schema:rangeIncludes":{"@id":"schema:Text"},"schema:domainIncludes":[{"@id":"unece:BasicWorkItem"},{"@id":"unece:GroupedWorkItem"}],"rdfs:comment":"The identifier of a price list item for this grouped work item."},{"@id":"unece:referenceId","@type":["rdf:Property","owl:DatatypeProperty"],"rdfs:label":"referenceId","schema:rangeIncludes":{"@id":"schema:Text"},"schema:domainIncludes":{"@id":"unece:BasicWorkItem"},"rdfs:comment":"The unique identifier of another work item referenced by this basic work item."},{"@id":"unece:totalQuantity","@type":["rdf:Property","owl:ObjectProperty"],"rdfs:label":"totalQuantity","schema:rangeIncludes":{"@id":"unece:QuantityType"},"schema:domainIncludes":[{"@id":"unece:BasicWorkItem"},{"@id":"unece:GroupedWorkItem"},{"@id":"unece:ProcessWorkItem"}],"rdfs:comment":""},{"@id":"unece:totalQuantityAnalysis","@type":["rdf:Property","owl:ObjectProperty"],"rdfs:label":"totalQuantityAnalysis","schema:rangeIncludes":{"@id":"unece:QuantityAnalysis"},"schema:domainIncludes":{"@id":"unece:BasicWorkItem"},"rdfs:comment":"The quantity analysis for this work item."},{"@id":"unece:totalQuantityClassificationCode","@type":["rdf:Property","owl:DatatypeProperty"],"rdfs:label":"totalQuantityClassificationCode","schema:rangeIncludes":{"@id":"schema:Text"},"schema:domainIncludes":{"@id":"unece:BasicWorkItem"},"rdfs:comment":"The code specifying the classification of the total quantity for this basic work item."},{"@id":"unece:unitPrice","@type":["rdf:Property","owl:ObjectProperty"],"rdfs:label":"unitPrice","schema:rangeIncludes":{"@id":"unece:CalculatedPrice"},"schema:domainIncludes":{"@id":"unece:BasicWorkItem"},"rdfs:comment":"A unit calculated price for this basic work item."},{"@id":"unece:calculatedPriceTypeCode","@type":["rdf:Property","owl:DatatypeProperty"],"rdfs:label":"calculatedPriceTypeCode","schema:rangeIncludes":{"@id":"schema:Text"},"schema:domainIncludes":{"@id":"unece:CalculatedPrice"},"rdfs:comment":"A code specifying the type of calculated price."},{"@id":"unece:chargeAmount","@type":["rdf:Property","owl:ObjectProperty"],"rdfs:label":"chargeAmount","schema:rangeIncludes":{"@id":"unece:AmountType"},"schema:domainIncludes":[{"@id":"unece:CalculatedPrice"},{"@id":"unece:TradePrice"},{"@id":"unece:ReferencePrice"},{"@id":"unece:Service"}],"rdfs:comment":""},{"@id":"unece:relatedAllowanceCharge","@type":["rdf:Property","owl:ObjectProperty"],"rdfs:label":"relatedAllowanceCharge","schema:rangeIncludes":{"@id":"unece:AppliedAllowanceCharge"},"schema:domainIncludes":{"@id":"unece:CalculatedPrice"},"rdfs:comment":"Applied allowance charge information related to this calculated price."},{"@id":"unece:conversionRate","@type":["rdf:Property","owl:DatatypeProperty"],"rdfs:label":"conversionRate","schema:rangeIncludes":{"@id":"schema:Text"},"schema:domainIncludes":{"@id":"unece:CurrencyExchange"},"rdfs:comment":"The rate factor used for conversion from the source currency to the target currency for trade purposes."},{"@id":"unece:conversionRateDateTime","@type":["rdf:Property","owl:DatatypeProperty"],"rdfs:label":"conversionRateDateTime","schema:rangeIncludes":{"@id":"schema:Text"},"schema:domainIncludes":{"@id":"unece:CurrencyExchange"},"rdfs:comment":"The date, time, date time or other date time value of the conversion rate for this trade related currency exchange."},{"@id":"unece:currencySourceCurrencyCode","@type":["rdf:Property","owl:DatatypeProperty"],"rdfs:label":"currencySourceCurrencyCode","schema:rangeIncludes":{"@id":"unece:CurrencyCodeList"},"schema:domainIncludes":{"@id":"unece:CurrencyExchange"},"rdfs:comment":"The code specifying the source currency of a trade related currency conversion."},{"@id":"unece:currencyTargetCurrencyCode","@type":["rdf:Property","owl:DatatypeProperty"],"rdfs:label":"currencyTargetCurrencyCode","schema:rangeIncludes":{"@id":"unece:CurrencyCodeList"},"schema:domainIncludes":{"@id":"unece:CurrencyExchange"},"rdfs:comment":"The code specifying the target currency of a trade related currency conversion."},{"@id":"unece:sourceUnitBasisNumeric","@type":["rdf:Property","owl:DatatypeProperty"],"rdfs:label":"sourceUnitBasisNumeric","schema:rangeIncludes":{"@id":"schema:Text"},"schema:domainIncludes":{"@id":"unece:CurrencyExchange"},"rdfs:comment":"The numeric unit basis of the source currency used in this trade related currency exchange rate calculation."},{"@id":"unece:targetUnitBaseNumeric","@type":["rdf:Property","owl:DatatypeProperty"],"rdfs:label":"targetUnitBaseNumeric","schema:rangeIncludes":{"@id":"schema:Text"},"schema:domainIncludes":{"@id":"unece:CurrencyExchange"},"rdfs:comment":"The numeric unit basis of the target currency used in this trade related currency exchange rate calculation."},{"@id":"unece:tradeCurrencyExchangeMarketId","@type":["rdf:Property","owl:DatatypeProperty"],"rdfs:label":"tradeCurrencyExchangeMarketId","schema:rangeIncludes":{"@id":"schema:Text"},"schema:domainIncludes":{"@id":"unece:CurrencyExchange"},"rdfs:comment":"The unique identifier of the currency exchange market from which the exchange rate is taken for trade purposes."},{"@id":"unece:faceAmount","@type":["rdf:Property","owl:ObjectProperty"],"rdfs:label":"faceAmount","schema:rangeIncludes":{"@id":"unece:AmountType"},"schema:domainIncludes":{"@id":"unece:Voucher"},"rdfs:comment":""},{"@id":"unece:applicablePaymentBalanceOut","@type":["rdf:Property","owl:ObjectProperty"],"rdfs:label":"applicablePaymentBalanceOut","schema:rangeIncludes":{"@id":"unece:PaymentBalanceOut"},"schema:domainIncludes":{"@id":"unece:TradeSettlementPaymentMonetarySummation"},"rdfs:comment":"A balance out applicable to this trade settlement payment monetary summation."},{"@id":"unece:equivalentTransferTotalAmount","@type":["rdf:Property","owl:ObjectProperty"],"rdfs:label":"equivalentTransferTotalAmount","schema:rangeIncludes":{"@id":"unece:AmountType"},"schema:domainIncludes":{"@id":"unece:TradeSettlementPaymentMonetarySummation"},"rdfs:comment":""},{"@id":"unece:actualCurrencyExchange","@type":["rdf:Property","owl:ObjectProperty"],"rdfs:label":"actualCurrencyExchange","schema:rangeIncludes":{"@id":"unece:CurrencyExchange"},"schema:domainIncludes":{"@id":"unece:TradeAllowanceCharge"},"rdfs:comment":"The actual trade currency exchange for this trade allowance charge."},{"@id":"unece:allowanceChargeIdTypeCode","@type":["rdf:Property","owl:DatatypeProperty"],"rdfs:label":"allowanceChargeIdTypeCode","schema:rangeIncludes":{"@id":"unece:AllowanceChargeIdCodeList"},"schema:domainIncludes":{"@id":"unece:TradeAllowanceCharge"},"rdfs:comment":"The code specifying the type of this trade allowance charge."},{"@id":"unece:allowanceChargeReasonCode","@type":["rdf:Property","owl:DatatypeProperty"],"rdfs:label":"allowanceChargeReasonCode","schema:rangeIncludes":{"@id":"unece:AllowanceChargeReasonCodeList"},"schema:domainIncludes":{"@id":"unece:TradeAllowanceCharge"},"rdfs:comment":"The code specifying the reason for this trade allowance charge."},{"@id":"unece:categoryTradeTax","@type":["rdf:Property","owl:ObjectProperty"],"rdfs:label":"categoryTradeTax","schema:rangeIncludes":{"@id":"unece:Tax"},"schema:domainIncludes":{"@id":"unece:TradeAllowanceCharge"},"rdfs:comment":"A tax category of this trade allowance charge."},{"@id":"unece:prepaidIndicator","@type":["rdf:Property","owl:DatatypeProperty"],"rdfs:label":"prepaidIndicator","schema:rangeIncludes":{"@id":"schema:Boolean"},"schema:domainIncludes":{"@id":"unece:TradeAllowanceCharge"},"rdfs:comment":"The indication of whether or not this trade allowance charge is prepaid."},{"@id":"unece:applicableCustomerClass","@type":["rdf:Property","owl:ObjectProperty"],"rdfs:label":"applicableCustomerClass","schema:rangeIncludes":{"@id":"unece:CustomerClass"},"schema:domainIncludes":{"@id":"unece:TradePrice"},"rdfs:comment":"The conditions and requirements of the type of person who may use or purchase a product or service."},{"@id":"unece:applicableSpecifiedNote","@type":["rdf:Property","owl:ObjectProperty"],"rdfs:label":"applicableSpecifiedNote","schema:rangeIncludes":{"@id":"unece:SpecifiedNote"},"schema:domainIncludes":[{"@id":"unece:TradePrice"},{"@id":"unece:GuestPerson"},{"@id":"unece:ExperienceProduct"},{"@id":"unece:ExperienceEvent"}],"rdfs:comment":"A specified textual or coded description, such as a remark or additional information."},{"@id":"unece:appliedAllowanceCharge","@type":["rdf:Property","owl:ObjectProperty"],"rdfs:label":"appliedAllowanceCharge","schema:rangeIncludes":{"@id":"unece:TradeAllowanceCharge"},"schema:domainIncludes":{"@id":"unece:TradePrice"},"rdfs:comment":"An allowance or charge applied to the trade price."},{"@id":"unece:bracketTypeCode","@type":["rdf:Property","owl:DatatypeProperty"],"rdfs:label":"bracketTypeCode","schema:rangeIncludes":{"@id":"schema:Text"},"schema:domainIncludes":{"@id":"unece:TradePrice"},"rdfs:comment":"The code specifying the type of bracket for this trade price."},{"@id":"unece:cancellationPercent","@type":["rdf:Property","owl:DatatypeProperty"],"rdfs:label":"cancellationPercent","schema:rangeIncludes":{"@id":"schema:Text"},"schema:domainIncludes":{"@id":"unece:TradePrice"},"rdfs:comment":"The cancellation percentage for this trade price."},{"@id":"unece:categoryTypeCode","@type":["rdf:Property","owl:DatatypeProperty"],"rdfs:label":"categoryTypeCode","schema:rangeIncludes":{"@id":"schema:Text"},"schema:domainIncludes":{"@id":"unece:TradePrice"},"rdfs:comment":"The code specifying the type of category, such as refund or service charge, for this trade price."},{"@id":"unece:changeReason","@type":["rdf:Property","owl:DatatypeProperty"],"rdfs:label":"changeReason","schema:rangeIncludes":{"@id":"schema:Text"},"schema:domainIncludes":{"@id":"unece:TradePrice"},"rdfs:comment":"A reason, expressed as text, for a change of this trade price."},{"@id":"unece:customerServicePointQuantity","@type":["rdf:Property","owl:ObjectProperty"],"rdfs:label":"customerServicePointQuantity","schema:rangeIncludes":{"@id":"unece:QuantityType"},"schema:domainIncludes":{"@id":"unece:TradePrice"},"rdfs:comment":""},{"@id":"unece:deliveryLocation","@type":["rdf:Property","owl:ObjectProperty"],"rdfs:label":"deliveryLocation","schema:rangeIncludes":{"@id":"unece:Location"},"schema:domainIncludes":{"@id":"unece:TradePrice"},"rdfs:comment":"A reference to a physical location or place."},{"@id":"unece:determinationCode","@type":["rdf:Property","owl:DatatypeProperty"],"rdfs:label":"determinationCode","schema:rangeIncludes":{"@id":"schema:Text"},"schema:domainIncludes":{"@id":"unece:TradePrice"},"rdfs:comment":"The code specifying the determination of this trade price."},{"@id":"unece:grandTotalChargeAmount","@type":["rdf:Property","owl:ObjectProperty"],"rdfs:label":"grandTotalChargeAmount","schema:rangeIncludes":{"@id":"unece:AmountType"},"schema:domainIncludes":{"@id":"unece:TradePrice"},"rdfs:comment":""},{"@id":"unece:maximumQuantity","@type":["rdf:Property","owl:ObjectProperty"],"rdfs:label":"maximumQuantity","schema:rangeIncludes":{"@id":"unece:QuantityType"},"schema:domainIncludes":{"@id":"unece:TradePrice"},"rdfs:comment":""},{"@id":"unece:minimumQuantity","@type":["rdf:Property","owl:ObjectProperty"],"rdfs:label":"minimumQuantity","schema:rangeIncludes":{"@id":"unece:QuantityType"},"schema:domainIncludes":{"@id":"unece:TradePrice"},"rdfs:comment":""},{"@id":"unece:multipleReasonIndicator","@type":["rdf:Property","owl:DatatypeProperty"],"rdfs:label":"multipleReasonIndicator","schema:rangeIncludes":{"@id":"schema:Boolean"},"schema:domainIncludes":{"@id":"unece:TradePrice"},"rdfs:comment":"The indication of whether or not multiple reasons affect this trade price."},{"@id":"unece:netPriceIndicator","@type":["rdf:Property","owl:DatatypeProperty"],"rdfs:label":"netPriceIndicator","schema:rangeIncludes":{"@id":"schema:Boolean"},"schema:domainIncludes":[{"@id":"unece:TradePrice"},{"@id":"unece:ReferencePrice"}],"rdfs:comment":"An indication of whether or not the reference price is a net price."},{"@id":"unece:operationalApplicablePeriod","@type":["rdf:Property","owl:ObjectProperty"],"rdfs:label":"operationalApplicablePeriod","schema:rangeIncludes":{"@id":"unece:SpecifiedPeriod"},"schema:domainIncludes":{"@id":"unece:TradePrice"},"rdfs:comment":"A specified period of time."},{"@id":"unece:orderUnitConversionFactorNumeric","@type":["rdf:Property","owl:DatatypeProperty"],"rdfs:label":"orderUnitConversionFactorNumeric","schema:rangeIncludes":{"@id":"schema:Text"},"schema:domainIncludes":{"@id":"unece:TradePrice"},"rdfs:comment":"The value used as the factor to convert the order unit into the price unit for this trade price."},{"@id":"unece:priceType","@type":["rdf:Property","owl:DatatypeProperty"],"rdfs:label":"priceType","schema:rangeIncludes":{"@id":"schema:Text"},"schema:domainIncludes":{"@id":"unece:TradePrice"},"rdfs:comment":"A type, expressed as text, for this trade price."},{"@id":"unece:priceTypeCode","@type":["rdf:Property","owl:DatatypeProperty"],"rdfs:label":"priceTypeCode","schema:rangeIncludes":{"@id":"unece:PriceTypeCodeList"},"schema:domainIncludes":{"@id":"unece:TradePrice"},"rdfs:comment":"The code specifying the type of trade price."},{"@id":"unece:seasonalApplicablePeriod","@type":["rdf:Property","owl:ObjectProperty"],"rdfs:label":"seasonalApplicablePeriod","schema:rangeIncludes":{"@id":"unece:SpecifiedPeriod"},"schema:domainIncludes":{"@id":"unece:TradePrice"},"rdfs:comment":"A specified period of time."},{"@id":"unece:seasonalRankCode","@type":["rdf:Property","owl:DatatypeProperty"],"rdfs:label":"seasonalRankCode","schema:rangeIncludes":{"@id":"schema:Text"},"schema:domainIncludes":{"@id":"unece:TradePrice"},"rdfs:comment":"The code specifying the seasonal rank of this trade price."},{"@id":"unece:totalChargeAmount","@type":["rdf:Property","owl:ObjectProperty"],"rdfs:label":"totalChargeAmount","schema:rangeIncludes":{"@id":"unece:AmountType"},"schema:domainIncludes":[{"@id":"unece:TradePrice"},{"@id":"unece:RegulatoryProcedure"},{"@id":"unece:Consignment"},{"@id":"unece:ConsignmentItem"}],"rdfs:comment":""},{"@id":"unece:tradeComparisonPrice","@type":["rdf:Property","owl:ObjectProperty"],"rdfs:label":"tradeComparisonPrice","schema:rangeIncludes":{"@id":"unece:ReferencePrice"},"schema:domainIncludes":{"@id":"unece:TradePrice"},"rdfs:comment":"A price that provides a trade comparison with this trade price."},{"@id":"unece:unitAmount","@type":["rdf:Property","owl:ObjectProperty"],"rdfs:label":"unitAmount","schema:rangeIncludes":{"@id":"unece:AmountType"},"schema:domainIncludes":{"@id":"unece:TradePrice"},"rdfs:comment":""},{"@id":"unece:comparisonMethodCode","@type":["rdf:Property","owl:DatatypeProperty"],"rdfs:label":"comparisonMethodCode","schema:rangeIncludes":{"@id":"schema:Text"},"schema:domainIncludes":{"@id":"unece:ReferencePrice"},"rdfs:comment":"The code specifying the comparison method for this reference price."},{"@id":"unece:addedAdjustmentAmount","@type":["rdf:Property","owl:ObjectProperty"],"rdfs:label":"addedAdjustmentAmount","schema:rangeIncludes":{"@id":"unece:AmountType"},"schema:domainIncludes":{"@id":"unece:CustomsValuation"},"rdfs:comment":""},{"@id":"unece:addedAdjustmentPercent","@type":["rdf:Property","owl:DatatypeProperty"],"rdfs:label":"addedAdjustmentPercent","schema:rangeIncludes":{"@id":"schema:Text"},"schema:domainIncludes":{"@id":"unece:CustomsValuation"},"rdfs:comment":"The adjustment added, expressed as a percentage, for this cross-border customs valuation."},{"@id":"unece:applicableCurrencyExchange","@type":["rdf:Property","owl:ObjectProperty"],"rdfs:label":"applicableCurrencyExchange","schema:rangeIncludes":{"@id":"unece:CurrencyExchange"},"schema:domainIncludes":[{"@id":"unece:CustomsValuation"},{"@id":"unece:RegulatoryProcedure"},{"@id":"unece:Consignment"}],"rdfs:comment":"A currency exchange applicable to this supply chain consignment."},{"@id":"unece:buyerSellerRelationshipIndicator","@type":["rdf:Property","owl:DatatypeProperty"],"rdfs:label":"buyerSellerRelationshipIndicator","schema:rangeIncludes":{"@id":"schema:Boolean"},"schema:domainIncludes":{"@id":"unece:CustomsValuation"},"rdfs:comment":"The indication of whether or not there is a relationship between the buyer and the seller, such as a financial relationship, for this cross-border customs valuation."},{"@id":"unece:buyerSellerRelationshipPriceInfluenceIndicator","@type":["rdf:Property","owl:DatatypeProperty"],"rdfs:label":"buyerSellerRelationshipPriceInfluenceIndicator","schema:rangeIncludes":{"@id":"schema:Boolean"},"schema:domainIncludes":{"@id":"unece:CustomsValuation"},"rdfs:comment":"The indication of whether or not the buyer seller relationship influences the price of the goods for this cross-border customs valuation."},{"@id":"unece:chargeApportionMethodCode","@type":["rdf:Property","owl:DatatypeProperty"],"rdfs:label":"chargeApportionMethodCode","schema:rangeIncludes":{"@id":"schema:Text"},"schema:domainIncludes":{"@id":"unece:CustomsValuation"},"rdfs:comment":"The code specifying the method of the apportion of charges for this cross-border customs valuation."},{"@id":"unece:deductedAdjustmentAmount","@type":["rdf:Property","owl:ObjectProperty"],"rdfs:label":"deductedAdjustmentAmount","schema:rangeIncludes":{"@id":"unece:AmountType"},"schema:domainIncludes":{"@id":"unece:CustomsValuation"},"rdfs:comment":""},{"@id":"unece:deductedAdjustmentPercent","@type":["rdf:Property","owl:DatatypeProperty"],"rdfs:label":"deductedAdjustmentPercent","schema:rangeIncludes":{"@id":"schema:Text"},"schema:domainIncludes":{"@id":"unece:CustomsValuation"},"rdfs:comment":"The adjustment deducted, expressed as a percentage, for this cross-border customs valuation."},{"@id":"unece:otherChargeAmount","@type":["rdf:Property","owl:ObjectProperty"],"rdfs:label":"otherChargeAmount","schema:rangeIncludes":{"@id":"unece:AmountType"},"schema:domainIncludes":{"@id":"unece:CustomsValuation"},"rdfs:comment":""},{"@id":"unece:royaltyLicenseFeeIndicator","@type":["rdf:Property","owl:DatatypeProperty"],"rdfs:label":"royaltyLicenseFeeIndicator","schema:rangeIncludes":{"@id":"schema:Boolean"},"schema:domainIncludes":{"@id":"unece:CustomsValuation"},"rdfs:comment":"The indication of whether or not there is a royalty or licence fee related to the goods for this cross-border customs valuation."},{"@id":"unece:salePriceConditionIndicator","@type":["rdf:Property","owl:DatatypeProperty"],"rdfs:label":"salePriceConditionIndicator","schema:rangeIncludes":{"@id":"schema:Boolean"},"schema:domainIncludes":{"@id":"unece:CustomsValuation"},"rdfs:comment":"The indication of whether or not there is a condition imposed on the sale price of the goods for this cross-border customs valuation."},{"@id":"unece:saleRestriction","@type":["rdf:Property","owl:DatatypeProperty"],"rdfs:label":"saleRestriction","schema:rangeIncludes":{"@id":"schema:Text"},"schema:domainIncludes":{"@id":"unece:CustomsValuation"},"rdfs:comment":"A restriction, expressed as text, imposed on the sale of the goods for this cross-border customs valuation."},{"@id":"unece:saleRestrictionIndicator","@type":["rdf:Property","owl:DatatypeProperty"],"rdfs:label":"saleRestrictionIndicator","schema:rangeIncludes":{"@id":"schema:Boolean"},"schema:domainIncludes":{"@id":"unece:CustomsValuation"},"rdfs:comment":"The indication of whether or not there is any restriction imposed on the sale of the goods for this cross-border customs valuation."},{"@id":"unece:wTOAdditionCode","@type":["rdf:Property","owl:DatatypeProperty"],"rdfs:label":"wTOAdditionCode","schema:rangeIncludes":{"@id":"schema:Text"},"schema:domainIncludes":{"@id":"unece:CustomsValuation"},"rdfs:comment":"The code specifying any additions necessary under the World Trade Organization (WTO) Valuation Agreement used for the assessment of this cross-border customs valuation."},{"@id":"unece:abbreviatedName","@type":["rdf:Property","owl:DatatypeProperty"],"rdfs:label":"abbreviatedName","schema:rangeIncludes":{"@id":"schema:Text"},"schema:domainIncludes":{"@id":"unece:AcademicQualification"},"rdfs:comment":"The abbreviated name, expressed as text, of this academic qualification."},{"@id":"unece:abbreviation","@type":["rdf:Property","owl:DatatypeProperty"],"rdfs:label":"abbreviation","schema:rangeIncludes":{"@id":"schema:Text"},"schema:domainIncludes":[{"@id":"unece:InspectionReference"},{"@id":"unece:LaboratoryObservationReference"},{"@id":"unece:SupplyChainReference"}],"rdfs:comment":"An abbreviation, expressed as text, for this supply chain reference."},{"@id":"unece:propertyReferenceCode","@type":["rdf:Property","owl:DatatypeProperty"],"rdfs:label":"propertyReferenceCode","schema:rangeIncludes":{"@id":"schema:Text"},"schema:domainIncludes":[{"@id":"unece:InspectionReference"},{"@id":"unece:LaboratoryObservationReference"},{"@id":"unece:InspectionInstructions"},{"@id":"unece:LaboratoryObservationInstructions"},{"@id":"unece:SupplyChainReference"}],"rdfs:comment":"A code specifying a property reference for this supply chain reference."},{"@id":"unece:acceptedIndicator","@type":["rdf:Property","owl:DatatypeProperty"],"rdfs:label":"acceptedIndicator","schema:rangeIncludes":{"@id":"schema:Boolean"},"schema:domainIncludes":{"@id":"unece:ProtectionMeans"},"rdfs:comment":"The indication of whether or not this disease protection means is accepted."},{"@id":"unece:item","@type":["rdf:Property","owl:DatatypeProperty"],"rdfs:label":"item","schema:rangeIncludes":{"@id":"schema:Text"},"schema:domainIncludes":{"@id":"unece:ProtectionMeans"},"rdfs:comment":"An item, expressed as text, for this disease protection means."},{"@id":"unece:restriction","@type":["rdf:Property","owl:DatatypeProperty"],"rdfs:label":"restriction","schema:rangeIncludes":{"@id":"schema:Text"},"schema:domainIncludes":[{"@id":"unece:ProtectionMeans"},{"@id":"unece:PetAnimal"},{"@id":"unece:Allergy"},{"@id":"unece:CarriedEquipment"},{"@id":"unece:Disability"},{"@id":"unece:FoodChoice"},{"@id":"unece:GuestHealthIndication"}],"rdfs:comment":"A restriction, expressed as text, for this disease protection means."},{"@id":"unece:accreditingBodyName","@type":["rdf:Property","owl:DatatypeProperty"],"rdfs:label":"accreditingBodyName","schema:rangeIncludes":{"@id":"schema:Text"},"schema:domainIncludes":{"@id":"unece:Accreditation"},"rdfs:comment":"The name of the accrediting body, expressed as text, for this certified accreditation."},{"@id":"unece:authenticationMethodCode","@type":["rdf:Property","owl:DatatypeProperty"],"rdfs:label":"authenticationMethodCode","schema:rangeIncludes":{"@id":"schema:Text"},"schema:domainIncludes":{"@id":"unece:Accreditation"},"rdfs:comment":"A code specifying an authentication method for this certified accreditation."},{"@id":"unece:obtainedDateTime","@type":["rdf:Property","owl:DatatypeProperty"],"rdfs:label":"obtainedDateTime","schema:rangeIncludes":{"@id":"schema:DateTime"},"schema:domainIncludes":{"@id":"unece:Accreditation"},"rdfs:comment":"The date, time, date time or other date time value when this certified accreditation was obtained."},{"@id":"unece:amendmentReasonCode","@type":["rdf:Property","owl:DatatypeProperty"],"rdfs:label":"amendmentReasonCode","schema:rangeIncludes":{"@id":"schema:Text"},"schema:domainIncludes":{"@id":"unece:RegulatoryProcedure"},"rdfs:comment":"A code specifying a reason for an amendment to this cross-border regulatory procedure."},{"@id":"unece:annualQuotaQuantity","@type":["rdf:Property","owl:ObjectProperty"],"rdfs:label":"annualQuotaQuantity","schema:rangeIncludes":{"@id":"unece:QuantityType"},"schema:domainIncludes":{"@id":"unece:RegulatoryProcedure"},"rdfs:comment":""},{"@id":"unece:borderClearanceInstructions","@type":["rdf:Property","owl:ObjectProperty"],"rdfs:label":"borderClearanceInstructions","schema:rangeIncludes":{"@id":"unece:TransportInstructions"},"schema:domainIncludes":[{"@id":"unece:RegulatoryProcedure"},{"@id":"unece:ConsignmentItem"}],"rdfs:comment":"Border clearance instructions for this cross-border regulatory procedure."},{"@id":"unece:certificationBasis","@type":["rdf:Property","owl:DatatypeProperty"],"rdfs:label":"certificationBasis","schema:rangeIncludes":{"@id":"schema:Text"},"schema:domainIncludes":{"@id":"unece:RegulatoryProcedure"},"rdfs:comment":"A basis for a certification, expressed as text, for this cross-border regulatory procedure."},{"@id":"unece:consignmentDestinationSpecifiedLocation","@type":["rdf:Property","owl:ObjectProperty"],"rdfs:label":"consignmentDestinationSpecifiedLocation","schema:rangeIncludes":{"@id":"unece:Location"},"schema:domainIncludes":{"@id":"unece:RegulatoryProcedure"},"rdfs:comment":"A reference to a physical location or place."},{"@id":"unece:controlResult","@type":["rdf:Property","owl:DatatypeProperty"],"rdfs:label":"controlResult","schema:rangeIncludes":{"@id":"schema:Text"},"schema:domainIncludes":{"@id":"unece:RegulatoryProcedure"},"rdfs:comment":"A control result, expressed as text, for this cross-border regulatory procedure."},{"@id":"unece:controlStartDateConfirmationIndicator","@type":["rdf:Property","owl:DatatypeProperty"],"rdfs:label":"controlStartDateConfirmationIndicator","schema:rangeIncludes":{"@id":"schema:Boolean"},"schema:domainIncludes":{"@id":"unece:RegulatoryProcedure"},"rdfs:comment":"The indication of whether or not the start date of a control has been confirmed for this cross-border regulatory procedure."},{"@id":"unece:crossBorderRegulatoryProcedurePaymentMethodCode","@type":["rdf:Property","owl:DatatypeProperty"],"rdfs:label":"crossBorderRegulatoryProcedurePaymentMethodCode","schema:rangeIncludes":{"@id":"unece:PaymentMethodCodeList"},"schema:domainIncludes":{"@id":"unece:RegulatoryProcedure"},"rdfs:comment":"The code specifying the payment method for this cross-border regulatory procedure, such as by deferred payment method."},{"@id":"unece:crossBorderRegulatoryProcedureTypeCode","@type":["rdf:Property","owl:DatatypeProperty"],"rdfs:label":"crossBorderRegulatoryProcedureTypeCode","schema:rangeIncludes":{"@id":"schema:Text"},"schema:domainIncludes":{"@id":"unece:RegulatoryProcedure"},"rdfs:comment":"A code specifying a type of cross-border regulatory procedure."},{"@id":"unece:declarantAssignedDeclarationId","@type":["rdf:Property","owl:DatatypeProperty"],"rdfs:label":"declarantAssignedDeclarationId","schema:rangeIncludes":{"@id":"schema:Text"},"schema:domainIncludes":{"@id":"unece:RegulatoryProcedure"},"rdfs:comment":"The declarant assigned identifier of a declaration for this cross-border regulatory procedure."},{"@id":"unece:declarationLodgementLocation","@type":["rdf:Property","owl:ObjectProperty"],"rdfs:label":"declarationLodgementLocation","schema:rangeIncludes":{"@id":"unece:Location"},"schema:domainIncludes":{"@id":"unece:RegulatoryProcedure"},"rdfs:comment":"A reference to a physical location or place."},{"@id":"unece:deferredPayableTotalChargeAmount","@type":["rdf:Property","owl:ObjectProperty"],"rdfs:label":"deferredPayableTotalChargeAmount","schema:rangeIncludes":{"@id":"unece:AmountType"},"schema:domainIncludes":{"@id":"unece:RegulatoryProcedure"},"rdfs:comment":""},{"@id":"unece:deferredPaymentMethodIndicator","@type":["rdf:Property","owl:DatatypeProperty"],"rdfs:label":"deferredPaymentMethodIndicator","schema:rangeIncludes":{"@id":"schema:Boolean"},"schema:domainIncludes":{"@id":"unece:RegulatoryProcedure"},"rdfs:comment":"The indication of whether or not the deferred payment method is applicable to this cross-border regulatory procedure."},{"@id":"unece:document","@type":["rdf:Property","owl:ObjectProperty"],"rdfs:label":"document","schema:rangeIncludes":{"@id":"unece:Document"},"schema:domainIncludes":{"@id":"unece:RegulatoryProcedure"},"rdfs:comment":"Written, printed or electronic matter that is referenced."},{"@id":"unece:entryCustomsOfficeSpecifiedLocation","@type":["rdf:Property","owl:ObjectProperty"],"rdfs:label":"entryCustomsOfficeSpecifiedLocation","schema:rangeIncludes":{"@id":"unece:Location"},"schema:domainIncludes":{"@id":"unece:RegulatoryProcedure"},"rdfs:comment":"A reference to a physical location or place."},{"@id":"unece:examinationEvent","@type":["rdf:Property","owl:ObjectProperty"],"rdfs:label":"examinationEvent","schema:rangeIncludes":{"@id":"unece:Event"},"schema:domainIncludes":[{"@id":"unece:RegulatoryProcedure"},{"@id":"unece:Consignment"},{"@id":"unece:ConsignmentItem"}],"rdfs:comment":"A significant occurrence or happening during transport.,A referenced significant occurrence or happening during transport."},{"@id":"unece:exemptionClaimantParty","@type":["rdf:Property","owl:ObjectProperty"],"rdfs:label":"exemptionClaimantParty","schema:rangeIncludes":{"@id":"unece:Party"},"schema:domainIncludes":{"@id":"unece:RegulatoryProcedure"},"rdfs:comment":""},{"@id":"unece:exitCustomsOfficeSpecifiedLocation","@type":["rdf:Property","owl:ObjectProperty"],"rdfs:label":"exitCustomsOfficeSpecifiedLocation","schema:rangeIncludes":{"@id":"unece:Location"},"schema:domainIncludes":{"@id":"unece:RegulatoryProcedure"},"rdfs:comment":"A reference to a physical location or place."},{"@id":"unece:exportCustomsOfficeSpecifiedLocation","@type":["rdf:Property","owl:ObjectProperty"],"rdfs:label":"exportCustomsOfficeSpecifiedLocation","schema:rangeIncludes":{"@id":"unece:Location"},"schema:domainIncludes":{"@id":"unece:RegulatoryProcedure"},"rdfs:comment":"A reference to a physical location or place."},{"@id":"unece:exportLicenceControlClassificationId","@type":["rdf:Property","owl:DatatypeProperty"],"rdfs:label":"exportLicenceControlClassificationId","schema:rangeIncludes":{"@id":"schema:Text"},"schema:domainIncludes":{"@id":"unece:RegulatoryProcedure"},"rdfs:comment":"The identifier of the export licence classification for control purposes relevant to this cross-border regulatory procedure, such as per the Wassenaar agreement concerning trade in weapons and dual-use goods and technologies."},{"@id":"unece:freeTradeAgreementName","@type":["rdf:Property","owl:DatatypeProperty"],"rdfs:label":"freeTradeAgreementName","schema:rangeIncludes":{"@id":"schema:Text"},"schema:domainIncludes":{"@id":"unece:RegulatoryProcedure"},"rdfs:comment":"The name of a free trade agreement, expressed as text, for this cross-border regulatory procedure."},{"@id":"unece:goodsStatusCode","@type":["rdf:Property","owl:DatatypeProperty"],"rdfs:label":"goodsStatusCode","schema:rangeIncludes":{"@id":"schema:Text"},"schema:domainIncludes":{"@id":"unece:RegulatoryProcedure"},"rdfs:comment":"The code specifying the goods status for this cross-border regulatory procedure."},{"@id":"unece:governmentActionResponsibleAgencyActionCode","@type":["rdf:Property","owl:DatatypeProperty"],"rdfs:label":"governmentActionResponsibleAgencyActionCode","schema:rangeIncludes":{"@id":"unece:GovernmentActionCodeList"},"schema:domainIncludes":{"@id":"unece:RegulatoryProcedure"},"rdfs:comment":"A code specifying an action for a responsible agency in this cross-border regulatory procedure."},{"@id":"unece:immediatePayableTotalChargeAmount","@type":["rdf:Property","owl:ObjectProperty"],"rdfs:label":"immediatePayableTotalChargeAmount","schema:rangeIncludes":{"@id":"unece:AmountType"},"schema:domainIncludes":{"@id":"unece:RegulatoryProcedure"},"rdfs:comment":""},{"@id":"unece:importCustomsOfficeSpecifiedLocation","@type":["rdf:Property","owl:ObjectProperty"],"rdfs:label":"importCustomsOfficeSpecifiedLocation","schema:rangeIncludes":{"@id":"unece:Location"},"schema:domainIncludes":{"@id":"unece:RegulatoryProcedure"},"rdfs:comment":"A reference to a physical location or place."},{"@id":"unece:nonTariffChargeAmount","@type":["rdf:Property","owl:ObjectProperty"],"rdfs:label":"nonTariffChargeAmount","schema:rangeIncludes":{"@id":"unece:AmountType"},"schema:domainIncludes":{"@id":"unece:RegulatoryProcedure"},"rdfs:comment":""},{"@id":"unece:originCriteria","@type":["rdf:Property","owl:DatatypeProperty"],"rdfs:label":"originCriteria","schema:rangeIncludes":{"@id":"schema:Text"},"schema:domainIncludes":{"@id":"unece:RegulatoryProcedure"},"rdfs:comment":"The origin criteria, expressed as text, for this cross-border regulatory procedure."},{"@id":"unece:paymentOfficeLocation","@type":["rdf:Property","owl:ObjectProperty"],"rdfs:label":"paymentOfficeLocation","schema:rangeIncludes":{"@id":"unece:Location"},"schema:domainIncludes":{"@id":"unece:RegulatoryProcedure"},"rdfs:comment":"A reference to a physical location or place."},{"@id":"unece:performanceDateTime","@type":["rdf:Property","owl:DatatypeProperty"],"rdfs:label":"performanceDateTime","schema:rangeIncludes":{"@id":"schema:Text"},"schema:domainIncludes":{"@id":"unece:RegulatoryProcedure"},"rdfs:comment":"A date, time, date time, or other date time value on which this cross-border regulatory procedure was, or will be, performed."},{"@id":"unece:previousProcedureTypeCode","@type":["rdf:Property","owl:DatatypeProperty"],"rdfs:label":"previousProcedureTypeCode","schema:rangeIncludes":{"@id":"schema:Text"},"schema:domainIncludes":{"@id":"unece:RegulatoryProcedure"},"rdfs:comment":"A code specifying a type of previous procedure for this cross-border regulatory procedure."},{"@id":"unece:quotaId","@type":["rdf:Property","owl:DatatypeProperty"],"rdfs:label":"quotaId","schema:rangeIncludes":{"@id":"schema:Text"},"schema:domainIncludes":{"@id":"unece:RegulatoryProcedure"},"rdfs:comment":"A quota identifier for this cross-border regulatory procedure."},{"@id":"unece:registeredDeferredPaymentPayerId","@type":["rdf:Property","owl:DatatypeProperty"],"rdfs:label":"registeredDeferredPaymentPayerId","schema:rangeIncludes":{"@id":"schema:Text"},"schema:domainIncludes":{"@id":"unece:RegulatoryProcedure"},"rdfs:comment":"The identifier of the registered deferred payment payer for this cross-border regulatory procedure."},{"@id":"unece:requestOverrideCode","@type":["rdf:Property","owl:DatatypeProperty"],"rdfs:label":"requestOverrideCode","schema:rangeIncludes":{"@id":"schema:Text"},"schema:domainIncludes":{"@id":"unece:RegulatoryProcedure"},"rdfs:comment":"A code specifying a request, including a reason, to override previously submitted information for this cross-border regulatory procedure, such as due to an error condition."},{"@id":"unece:requiredChemicalTreatment","@type":["rdf:Property","owl:ObjectProperty"],"rdfs:label":"requiredChemicalTreatment","schema:rangeIncludes":{"@id":"unece:AppliedChemicalTreatment"},"schema:domainIncludes":{"@id":"unece:RegulatoryProcedure"},"rdfs:comment":"A chemical treatment applied as required by this cross-border regulatory procedure."},{"@id":"unece:requiredSeal","@type":["rdf:Property","owl:ObjectProperty"],"rdfs:label":"requiredSeal","schema:rangeIncludes":{"@id":"unece:Seal"},"schema:domainIncludes":{"@id":"unece:RegulatoryProcedure"},"rdfs:comment":"A seal required by this cross-border regulatory procedure."},{"@id":"unece:requiredTestSpecificationReport","@type":["rdf:Property","owl:ObjectProperty"],"rdfs:label":"requiredTestSpecificationReport","schema:rangeIncludes":{"@id":"unece:TestSpecificationReport"},"schema:domainIncludes":{"@id":"unece:RegulatoryProcedure"},"rdfs:comment":"A report of a certification test and its attributes that is required for this cross-border regulatory procedure."},{"@id":"unece:responsibleGovernmentAgencyInvolvementResponsibleAgencyInvolvementCode","@type":["rdf:Property","owl:DatatypeProperty"],"rdfs:label":"responsibleGovernmentAgencyInvolvementResponsibleAgencyInvolvementCode","schema:rangeIncludes":{"@id":"unece:ResponsibleGovernmentAgencyInvolvementCodeList"},"schema:domainIncludes":{"@id":"unece:RegulatoryProcedure"},"rdfs:comment":"A code specifying a responsible agency involved in this cross-border regulatory procedure."},{"@id":"unece:responsibleGovernmentAgencyResponsibleAgencyCode","@type":["rdf:Property","owl:DatatypeProperty"],"rdfs:label":"responsibleGovernmentAgencyResponsibleAgencyCode","schema:rangeIncludes":{"@id":"unece:ResponsibleGovernmentAgencyCodeList"},"schema:domainIncludes":{"@id":"unece:RegulatoryProcedure"},"rdfs:comment":"The code specifying the agency responsible for this cross-border regulatory procedure."},{"@id":"unece:specifiedDebtorFinancialAccount","@type":["rdf:Property","owl:ObjectProperty"],"rdfs:label":"specifiedDebtorFinancialAccount","schema:rangeIncludes":{"@id":"unece:DebtorFinancialAccount"},"schema:domainIncludes":{"@id":"unece:RegulatoryProcedure"},"rdfs:comment":"A specific business arrangement whereby debits arising from transactions are recorded."},{"@id":"unece:statementNote","@type":["rdf:Property","owl:ObjectProperty"],"rdfs:label":"statementNote","schema:rangeIncludes":{"@id":"unece:Note"},"schema:domainIncludes":{"@id":"unece:RegulatoryProcedure"},"rdfs:comment":"A textual or coded description, such as a remark or additional information."},{"@id":"unece:tariffAmount","@type":["rdf:Property","owl:ObjectProperty"],"rdfs:label":"tariffAmount","schema:rangeIncludes":{"@id":"unece:AmountType"},"schema:domainIncludes":{"@id":"unece:RegulatoryProcedure"},"rdfs:comment":""},{"@id":"unece:tariffQuantity","@type":["rdf:Property","owl:ObjectProperty"],"rdfs:label":"tariffQuantity","schema:rangeIncludes":{"@id":"unece:QuantityType"},"schema:domainIncludes":[{"@id":"unece:RegulatoryProcedure"},{"@id":"unece:ConsignmentItem"}],"rdfs:comment":""},{"@id":"unece:totalConsignmentValueAmount","@type":["rdf:Property","owl:ObjectProperty"],"rdfs:label":"totalConsignmentValueAmount","schema:rangeIncludes":{"@id":"unece:AmountType"},"schema:domainIncludes":{"@id":"unece:RegulatoryProcedure"},"rdfs:comment":""},{"@id":"unece:transactionNatureCode","@type":["rdf:Property","owl:DatatypeProperty"],"rdfs:label":"transactionNatureCode","schema:rangeIncludes":{"@id":"schema:Text"},"schema:domainIncludes":{"@id":"unece:RegulatoryProcedure"},"rdfs:comment":"A code specifying the nature of a transaction for this cross-border regulatory procedure."},{"@id":"unece:transitCustomsOfficeSpecifiedLocation","@type":["rdf:Property","owl:ObjectProperty"],"rdfs:label":"transitCustomsOfficeSpecifiedLocation","schema:rangeIncludes":{"@id":"unece:Location"},"schema:domainIncludes":{"@id":"unece:RegulatoryProcedure"},"rdfs:comment":"A reference to a physical location or place."},{"@id":"unece:transitReleaseCustomsOfficeSpecifiedLocation","@type":["rdf:Property","owl:ObjectProperty"],"rdfs:label":"transitReleaseCustomsOfficeSpecifiedLocation","schema:rangeIncludes":{"@id":"unece:Location"},"schema:domainIncludes":{"@id":"unece:RegulatoryProcedure"},"rdfs:comment":"A reference to a physical location or place."},{"@id":"unece:transportMovementTypeCode","@type":["rdf:Property","owl:DatatypeProperty"],"rdfs:label":"transportMovementTypeCode","schema:rangeIncludes":{"@id":"unece:TransportMovementTypeCodeList"},"schema:domainIncludes":{"@id":"unece:RegulatoryProcedure"},"rdfs:comment":"A code specifying the transport movement type, such as import, export, transit, for this cross-border regulatory procedure."},{"@id":"unece:treatmentEvent","@type":["rdf:Property","owl:ObjectProperty"],"rdfs:label":"treatmentEvent","schema:rangeIncludes":{"@id":"unece:Event"},"schema:domainIncludes":{"@id":"unece:RegulatoryProcedure"},"rdfs:comment":"A significant occurrence or happening during transport.,A referenced significant occurrence or happening during transport."},{"@id":"unece:usedToDateQuotaQuantity","@type":["rdf:Property","owl:ObjectProperty"],"rdfs:label":"usedToDateQuotaQuantity","schema:rangeIncludes":{"@id":"unece:QuantityType"},"schema:domainIncludes":{"@id":"unece:RegulatoryProcedure"},"rdfs:comment":""},{"@id":"unece:valuationBasisAmount","@type":["rdf:Property","owl:ObjectProperty"],"rdfs:label":"valuationBasisAmount","schema:rangeIncludes":{"@id":"unece:AmountType"},"schema:domainIncludes":{"@id":"unece:RegulatoryProcedure"},"rdfs:comment":""},{"@id":"unece:actualEffectiveDateTime","@type":["rdf:Property","owl:DatatypeProperty"],"rdfs:label":"actualEffectiveDateTime","schema:rangeIncludes":{"@id":"schema:Text"},"schema:domainIncludes":[{"@id":"unece:OrganizationalCertificate"},{"@id":"unece:ProcessCertificate"},{"@id":"unece:ProductBatchCertificate"},{"@id":"unece:ProductCertificate"},{"@id":"unece:SpecifiedCertificate"},{"@id":"unece:AgriculturalCertificate"}],"rdfs:comment":"The actual effective date, time, date time or other date time value for this agricultural certificate."},{"@id":"unece:applicableAssertion","@type":["rdf:Property","owl:ObjectProperty"],"rdfs:label":"applicableAssertion","schema:rangeIncludes":{"@id":"unece:Assertion"},"schema:domainIncludes":[{"@id":"unece:OrganizationalCertificate"},{"@id":"unece:ProcessCertificate"},{"@id":"unece:ProductBatchCertificate"},{"@id":"unece:ProductCertificate"},{"@id":"unece:AgriculturalCertificate"},{"@id":"unece:AnimalCertificate"}],"rdfs:comment":"A sustainability assertion applicable to this agricultural certificate."},{"@id":"unece:applicableObjectCode","@type":["rdf:Property","owl:DatatypeProperty"],"rdfs:label":"applicableObjectCode","schema:rangeIncludes":{"@id":"schema:Text"},"schema:domainIncludes":[{"@id":"unece:OrganizationalCertificate"},{"@id":"unece:ProcessCertificate"},{"@id":"unece:ProductBatchCertificate"},{"@id":"unece:ProductCertificate"},{"@id":"unece:AgriculturalCertificate"}],"rdfs:comment":"A code specifying an applicable object, such as item, animal, person or organization, for this agricultural certificate."},{"@id":"unece:applicableOrganizationCharacteristic","@type":["rdf:Property","owl:ObjectProperty"],"rdfs:label":"applicableOrganizationCharacteristic","schema:rangeIncludes":{"@id":"unece:OrganizationCharacteristic"},"schema:domainIncludes":{"@id":"unece:OrganizationalCertificate"},"rdfs:comment":"A characteristic applicable to this organization certificate."},{"@id":"unece:certificateTypeCode","@type":["rdf:Property","owl:DatatypeProperty"],"rdfs:label":"certificateTypeCode","schema:rangeIncludes":{"@id":"unece:CertificateTypeCodeList"},"schema:domainIncludes":[{"@id":"unece:OrganizationalCertificate"},{"@id":"unece:ProcessCertificate"},{"@id":"unece:ProductBatchCertificate"},{"@id":"unece:ProductCertificate"},{"@id":"unece:SpecifiedCertificate"},{"@id":"unece:ConformanceCertificate"},{"@id":"unece:AgriculturalCertificate"},{"@id":"unece:AnimalCertificate"}],"rdfs:comment":"A code specifying a type of specified certificate."},{"@id":"unece:issueReasonCode","@type":["rdf:Property","owl:DatatypeProperty"],"rdfs:label":"issueReasonCode","schema:rangeIncludes":{"@id":"schema:Text"},"schema:domainIncludes":[{"@id":"unece:OrganizationalCertificate"},{"@id":"unece:ProcessCertificate"},{"@id":"unece:ProductBatchCertificate"},{"@id":"unece:ProductCertificate"},{"@id":"unece:SpecifiedCertificate"},{"@id":"unece:AgriculturalCertificate"}],"rdfs:comment":"The code specifying the reason for the issue of this process certificate."},{"@id":"unece:issuingPartyId","@type":["rdf:Property","owl:DatatypeProperty"],"rdfs:label":"issuingPartyId","schema:rangeIncludes":{"@id":"schema:Text"},"schema:domainIncludes":[{"@id":"unece:OrganizationalCertificate"},{"@id":"unece:ProcessCertificate"},{"@id":"unece:ProductBatchCertificate"},{"@id":"unece:ProductCertificate"},{"@id":"unece:Assertion"},{"@id":"unece:ConformanceCertificate"},{"@id":"unece:AgriculturalCertificate"}],"rdfs:comment":"An identifier of a party issuing this sustainability assertion."},{"@id":"unece:requestedEffectiveDateTime","@type":["rdf:Property","owl:DatatypeProperty"],"rdfs:label":"requestedEffectiveDateTime","schema:rangeIncludes":{"@id":"schema:Text"},"schema:domainIncludes":[{"@id":"unece:OrganizationalCertificate"},{"@id":"unece:ProcessCertificate"},{"@id":"unece:ProductBatchCertificate"},{"@id":"unece:ProductCertificate"},{"@id":"unece:SpecifiedCertificate"},{"@id":"unece:AgriculturalCertificate"}],"rdfs:comment":"The requested effective date, time, date time or other date time value for this agricultural certificate."},{"@id":"unece:applicableProcessCertification","@type":["rdf:Property","owl:ObjectProperty"],"rdfs:label":"applicableProcessCertification","schema:rangeIncludes":{"@id":"unece:ProcessCertification"},"schema:domainIncludes":{"@id":"unece:ProcessCertificate"},"rdfs:comment":"A process certification applicable to this process certificate."},{"@id":"unece:aliasNameCode","@type":["rdf:Property","owl:DatatypeProperty"],"rdfs:label":"aliasNameCode","schema:rangeIncludes":{"@id":"schema:Text"},"schema:domainIncludes":{"@id":"unece:SpecifiedCertificate"},"rdfs:comment":"A code specifying an alias name of this specified certificate."},{"@id":"unece:applicableClause","@type":["rdf:Property","owl:ObjectProperty"],"rdfs:label":"applicableClause","schema:rangeIncludes":{"@id":"unece:Clause"},"schema:domainIncludes":{"@id":"unece:SpecifiedCertificate"},"rdfs:comment":"A distinct article or provision in a document, which requires compliance."},{"@id":"unece:applicableGeographicRegion","@type":["rdf:Property","owl:DatatypeProperty"],"rdfs:label":"applicableGeographicRegion","schema:rangeIncludes":{"@id":"schema:Text"},"schema:domainIncludes":{"@id":"unece:SpecifiedCertificate"},"rdfs:comment":"A geographic region, expressed as text, applicable for this specified certificate."},{"@id":"unece:assuranceLevelCode","@type":["rdf:Property","owl:DatatypeProperty"],"rdfs:label":"assuranceLevelCode","schema:rangeIncludes":{"@id":"schema:Text"},"schema:domainIncludes":[{"@id":"unece:SpecifiedCertificate"},{"@id":"unece:Assessment"},{"@id":"unece:Licence"},{"@id":"unece:SpecifiedDeclaration"}],"rdfs:comment":"A code specifying an assurance level of this specified declaration."},{"@id":"unece:availableLanguageCode","@type":["rdf:Property","owl:DatatypeProperty"],"rdfs:label":"availableLanguageCode","schema:rangeIncludes":{"@id":"unece:LanguageCodeList"},"schema:domainIncludes":{"@id":"unece:SpecifiedCertificate"},"rdfs:comment":"A code specifying an available language for this specified certificate."},{"@id":"unece:capabilityLevel","@type":["rdf:Property","owl:DatatypeProperty"],"rdfs:label":"capabilityLevel","schema:rangeIncludes":{"@id":"schema:Text"},"schema:domainIncludes":[{"@id":"unece:SpecifiedCertificate"},{"@id":"unece:ExperienceItem"}],"rdfs:comment":"A capability level, expressed as text, for this specified experience item."},{"@id":"unece:certifiedObject","@type":["rdf:Property","owl:ObjectProperty"],"rdfs:label":"certifiedObject","schema:rangeIncludes":{"@id":"unece:Object"},"schema:domainIncludes":{"@id":"unece:SpecifiedCertificate"},"rdfs:comment":"Anything that is visible or tangible, such as a product, process, or organization."},{"@id":"unece:certifiedParty","@type":["rdf:Property","owl:ObjectProperty"],"rdfs:label":"certifiedParty","schema:rangeIncludes":{"@id":"unece:Party"},"schema:domainIncludes":{"@id":"unece:SpecifiedCertificate"},"rdfs:comment":""},{"@id":"unece:certifiedPersonQuantity","@type":["rdf:Property","owl:ObjectProperty"],"rdfs:label":"certifiedPersonQuantity","schema:rangeIncludes":{"@id":"unece:QuantityType"},"schema:domainIncludes":{"@id":"unece:SpecifiedCertificate"},"rdfs:comment":""},{"@id":"unece:effectiveFromDateTime","@type":["rdf:Property","owl:DatatypeProperty"],"rdfs:label":"effectiveFromDateTime","schema:rangeIncludes":{"@id":"schema:DateTime"},"schema:domainIncludes":{"@id":"unece:SpecifiedCertificate"},"rdfs:comment":"The date, time, date time, or other date time value from which this specified certificate is effective."},{"@id":"unece:endorsementDateTime","@type":["rdf:Property","owl:DatatypeProperty"],"rdfs:label":"endorsementDateTime","schema:rangeIncludes":{"@id":"schema:DateTime"},"schema:domainIncludes":{"@id":"unece:SpecifiedCertificate"},"rdfs:comment":"An endorsement date, time, date time or other date time value for this specified certificate."},{"@id":"unece:issuanceLocation","@type":["rdf:Property","owl:ObjectProperty"],"rdfs:label":"issuanceLocation","schema:rangeIncludes":{"@id":"unece:Location"},"schema:domainIncludes":{"@id":"unece:SpecifiedCertificate"},"rdfs:comment":"A reference to a physical location or place."},{"@id":"unece:latestEndorsementDateTime","@type":["rdf:Property","owl:DatatypeProperty"],"rdfs:label":"latestEndorsementDateTime","schema:rangeIncludes":{"@id":"schema:DateTime"},"schema:domainIncludes":{"@id":"unece:SpecifiedCertificate"},"rdfs:comment":"A latest endorsement date, time, date time or other date time value for this specified certificate."},{"@id":"unece:partyId","@type":["rdf:Property","owl:DatatypeProperty"],"rdfs:label":"partyId","schema:rangeIncludes":{"@id":"schema:Text"},"schema:domainIncludes":{"@id":"unece:SpecifiedCertificate"},"rdfs:comment":"An identifier of a party for this specified certificate."},{"@id":"unece:providingParty","@type":["rdf:Property","owl:ObjectProperty"],"rdfs:label":"providingParty","schema:rangeIncludes":{"@id":"unece:Party"},"schema:domainIncludes":{"@id":"unece:SpecifiedCertificate"},"rdfs:comment":""},{"@id":"unece:reportedDocumentStatus","@type":["rdf:Property","owl:ObjectProperty"],"rdfs:label":"reportedDocumentStatus","schema:rangeIncludes":{"@id":"unece:DocumentStatus"},"schema:domainIncludes":{"@id":"unece:SpecifiedCertificate"},"rdfs:comment":"The information relevant to a condition related to a document."},{"@id":"unece:requiredIndicator","@type":["rdf:Property","owl:DatatypeProperty"],"rdfs:label":"requiredIndicator","schema:rangeIncludes":{"@id":"schema:Boolean"},"schema:domainIncludes":{"@id":"unece:SpecifiedCertificate"},"rdfs:comment":"The indication of whether or not this specified certificate is required."},{"@id":"unece:subjectTypeCode","@type":["rdf:Property","owl:DatatypeProperty"],"rdfs:label":"subjectTypeCode","schema:rangeIncludes":{"@id":"schema:Text"},"schema:domainIncludes":[{"@id":"unece:SpecifiedCertificate"},{"@id":"unece:Licence"},{"@id":"unece:SpecifiedDeclaration"},{"@id":"unece:SpecifiedCondition"}],"rdfs:comment":"A code specifying a subject type for this licence."},{"@id":"unece:validIndicator","@type":["rdf:Property","owl:DatatypeProperty"],"rdfs:label":"validIndicator","schema:rangeIncludes":{"@id":"schema:Boolean"},"schema:domainIncludes":[{"@id":"unece:SpecifiedCertificate"},{"@id":"unece:Licence"}],"rdfs:comment":"The indication of whether or not this specified certificate is valid."},{"@id":"unece:validityExtendedUntilDateTime","@type":["rdf:Property","owl:DatatypeProperty"],"rdfs:label":"validityExtendedUntilDateTime","schema:rangeIncludes":{"@id":"schema:DateTime"},"schema:domainIncludes":{"@id":"unece:SpecifiedCertificate"},"rdfs:comment":"A date, time, date time or other date time value until which this specified certificate will remain valid under the terms of an approved extension period."},{"@id":"unece:validityTypeCode","@type":["rdf:Property","owl:DatatypeProperty"],"rdfs:label":"validityTypeCode","schema:rangeIncludes":{"@id":"schema:Text"},"schema:domainIncludes":{"@id":"unece:SpecifiedCertificate"},"rdfs:comment":"A code specifying a type of validity for this specified certificate."},{"@id":"unece:actualObservationEndDateTime","@type":["rdf:Property","owl:DatatypeProperty"],"rdfs:label":"actualObservationEndDateTime","schema:rangeIncludes":{"@id":"schema:Text"},"schema:domainIncludes":{"@id":"unece:ObservationResult"},"rdfs:comment":"The date, time, date time, or other date time value for the end of the observation for this sample observation result."},{"@id":"unece:actualObservationStartDateTime","@type":["rdf:Property","owl:DatatypeProperty"],"rdfs:label":"actualObservationStartDateTime","schema:rangeIncludes":{"@id":"schema:Text"},"schema:domainIncludes":{"@id":"unece:ObservationResult"},"rdfs:comment":"The date, time, date time, or other date time value for the start of the observation for this sample observation result."},{"@id":"unece:attachedLaboratoryObservationNote","@type":["rdf:Property","owl:ObjectProperty"],"rdfs:label":"attachedLaboratoryObservationNote","schema:rangeIncludes":{"@id":"unece:LaboratoryObservationNote"},"schema:domainIncludes":{"@id":"unece:ObservationResult"},"rdfs:comment":"A note attached to the laboratory observation results with additional observations and or conclusions."},{"@id":"unece:authorizationParty","@type":["rdf:Property","owl:ObjectProperty"],"rdfs:label":"authorizationParty","schema:rangeIncludes":{"@id":"unece:LaboratoryObservationParty"},"schema:domainIncludes":{"@id":"unece:ObservationResult"},"rdfs:comment":"The laboratory observation party who authorized this sample observation result."},{"@id":"unece:emergencyObservationIndicator","@type":["rdf:Property","owl:DatatypeProperty"],"rdfs:label":"emergencyObservationIndicator","schema:rangeIncludes":{"@id":"schema:Boolean"},"schema:domainIncludes":{"@id":"unece:ObservationResult"},"rdfs:comment":"The indication of whether or not the observation was an emergency observation for this sample observation result."},{"@id":"unece:expectedValueSpecifiedObservationResultCharacteristic","@type":["rdf:Property","owl:ObjectProperty"],"rdfs:label":"expectedValueSpecifiedObservationResultCharacteristic","schema:rangeIncludes":{"@id":"unece:ObservationResultCharacteristic"},"schema:domainIncludes":{"@id":"unece:ObservationResult"},"rdfs:comment":"An expected value for the characteristic, to be observed or measured according to the specified type of observation for this sample observation result."},{"@id":"unece:generalCharacteristic","@type":["rdf:Property","owl:DatatypeProperty"],"rdfs:label":"generalCharacteristic","schema:rangeIncludes":{"@id":"schema:Text"},"schema:domainIncludes":[{"@id":"unece:ObservationResult"},{"@id":"unece:InspectionResult"}],"rdfs:comment":"A general characteristic, such as length, volume, density, sensitivity, conductivity, expressed as text, of this specified inspection result."},{"@id":"unece:interpretationResultApplicableParameter","@type":["rdf:Property","owl:ObjectProperty"],"rdfs:label":"interpretationResultApplicableParameter","schema:rangeIncludes":{"@id":"unece:ObservationObjectiveParameter"},"schema:domainIncludes":[{"@id":"unece:ObservationResult"},{"@id":"unece:InspectionResultCharacteristic"},{"@id":"unece:ObservationResultCharacteristic"}],"rdfs:comment":"An applicable objective observation parameter of the interpretation result for this inspection result characteristic."},{"@id":"unece:laboratoryAnalysisRequestSpecifiedReference","@type":["rdf:Property","owl:ObjectProperty"],"rdfs:label":"laboratoryAnalysisRequestSpecifiedReference","schema:rangeIncludes":{"@id":"unece:LaboratoryObservationReference"},"schema:domainIncludes":{"@id":"unece:ObservationResult"},"rdfs:comment":"A laboratory observation analysis request reference specified for this sample observation result."},{"@id":"unece:materialType","@type":["rdf:Property","owl:DatatypeProperty"],"rdfs:label":"materialType","schema:rangeIncludes":{"@id":"schema:Text"},"schema:domainIncludes":{"@id":"unece:ObservationResult"},"rdfs:comment":"The context material type of the observed sample, expressed as text, such as animal or blood."},{"@id":"unece:materialTypeCode","@type":["rdf:Property","owl:DatatypeProperty"],"rdfs:label":"materialTypeCode","schema:rangeIncludes":{"@id":"schema:Text"},"schema:domainIncludes":{"@id":"unece:ObservationResult"},"rdfs:comment":"The code specifying a material type for this sample observation result."},{"@id":"unece:maximumStandardValueSpecifiedObservationResultCharacteristic","@type":["rdf:Property","owl:ObjectProperty"],"rdfs:label":"maximumStandardValueSpecifiedObservationResultCharacteristic","schema:rangeIncludes":{"@id":"unece:ObservationResultCharacteristic"},"schema:domainIncludes":{"@id":"unece:ObservationResult"},"rdfs:comment":"A maximum standard value of the values for the characteristic observed or measured by using the specified type of observation for this sample observation result."},{"@id":"unece:minimumStandardValueSpecifiedObservationResultCharacteristic","@type":["rdf:Property","owl:ObjectProperty"],"rdfs:label":"minimumStandardValueSpecifiedObservationResultCharacteristic","schema:rangeIncludes":{"@id":"unece:ObservationResultCharacteristic"},"schema:domainIncludes":{"@id":"unece:ObservationResult"},"rdfs:comment":"A minimum standard value of the values for the characteristic observed or measured by using the specified type of observation for this sample observation result."},{"@id":"unece:observationDiscontinuationReason","@type":["rdf:Property","owl:DatatypeProperty"],"rdfs:label":"observationDiscontinuationReason","schema:rangeIncludes":{"@id":"schema:Text"},"schema:domainIncludes":{"@id":"unece:ObservationResult"},"rdfs:comment":"The observation discontinuation reason, expressed as text, for this sample observation result."},{"@id":"unece:observationDiscontinuationReasonCode","@type":["rdf:Property","owl:DatatypeProperty"],"rdfs:label":"observationDiscontinuationReasonCode","schema:rangeIncludes":{"@id":"schema:Text"},"schema:domainIncludes":{"@id":"unece:ObservationResult"},"rdfs:comment":"The code specifying the observation discontinuation reason for this sample observation result."},{"@id":"unece:observationTimeFrame","@type":["rdf:Property","owl:DatatypeProperty"],"rdfs:label":"observationTimeFrame","schema:rangeIncludes":{"@id":"schema:Text"},"schema:domainIncludes":{"@id":"unece:ObservationResult"},"rdfs:comment":"The observation time frame, expressed as text, for this sample observation result."},{"@id":"unece:observedValueSpecifiedObservationResultCharacteristic","@type":["rdf:Property","owl:ObjectProperty"],"rdfs:label":"observedValueSpecifiedObservationResultCharacteristic","schema:rangeIncludes":{"@id":"unece:ObservationResultCharacteristic"},"schema:domainIncludes":{"@id":"unece:ObservationResult"},"rdfs:comment":"An observed value for the characteristic, acquired by observing or measuring according to the specified type of observation for this sample observation result."},{"@id":"unece:outsourcedLaboratoryParty","@type":["rdf:Property","owl:ObjectProperty"],"rdfs:label":"outsourcedLaboratoryParty","schema:rangeIncludes":{"@id":"unece:LaboratoryObservationParty"},"schema:domainIncludes":{"@id":"unece:ObservationResult"},"rdfs:comment":"The outsourced laboratory party who performed this sample observation result."},{"@id":"unece:outsourcedObservationIndicator","@type":["rdf:Property","owl:DatatypeProperty"],"rdfs:label":"outsourcedObservationIndicator","schema:rangeIncludes":{"@id":"schema:Boolean"},"schema:domainIncludes":{"@id":"unece:ObservationResult"},"rdfs:comment":"The indication of whether or not the observation was an outsourced observation (performed by a third party)."},{"@id":"unece:shareableIndicator","@type":["rdf:Property","owl:DatatypeProperty"],"rdfs:label":"shareableIndicator","schema:rangeIncludes":{"@id":"schema:Boolean"},"schema:domainIncludes":[{"@id":"unece:ObservationResult"},{"@id":"unece:InspectionResult"},{"@id":"unece:SustainabilityCharacteristic"},{"@id":"unece:ObservationResultCharacteristic"}],"rdfs:comment":"The indication of whether or not this sample observation result characteristic is shareable."},{"@id":"unece:specifiedLaboratoryObservationInstructions","@type":["rdf:Property","owl:ObjectProperty"],"rdfs:label":"specifiedLaboratoryObservationInstructions","schema:rangeIncludes":{"@id":"unece:LaboratoryObservationInstructions"},"schema:domainIncludes":{"@id":"unece:ObservationResult"},"rdfs:comment":"A set of laboratory observation instructions specified for this sample observation result."},{"@id":"unece:specifiedLaboratoryObservationReference","@type":["rdf:Property","owl:ObjectProperty"],"rdfs:label":"specifiedLaboratoryObservationReference","schema:rangeIncludes":{"@id":"unece:LaboratoryObservationReference"},"schema:domainIncludes":{"@id":"unece:ObservationResult"},"rdfs:comment":"A laboratory observation reference specified for this sample observation result."},{"@id":"unece:usedMethod","@type":["rdf:Property","owl:ObjectProperty"],"rdfs:label":"usedMethod","schema:rangeIncludes":{"@id":"unece:LaboratoryObservationAnalysisMethod"},"schema:domainIncludes":{"@id":"unece:ObservationResult"},"rdfs:comment":"A laboratory observation analysis method used for this sample observation result."},{"@id":"unece:agencyId","@type":["rdf:Property","owl:DatatypeProperty"],"rdfs:label":"agencyId","schema:rangeIncludes":{"@id":"schema:Text"},"schema:domainIncludes":{"@id":"unece:Standard"},"rdfs:comment":"The identifier of the agency for this referenced standard."},{"@id":"unece:applicableCountry","@type":["rdf:Property","owl:ObjectProperty"],"rdfs:label":"applicableCountry","schema:rangeIncludes":{"@id":"unece:Country"},"schema:domainIncludes":[{"@id":"unece:Standard"},{"@id":"unece:ProductCharacteristic"},{"@id":"unece:ProductBatchCharacteristic"}],"rdfs:comment":"The area of land that belongs to a nation together with its properties, such as population, political organization, etc., used or referenced for trade purposes."},{"@id":"unece:applicableMetricCharacteristic","@type":["rdf:Property","owl:ObjectProperty"],"rdfs:label":"applicableMetricCharacteristic","schema:rangeIncludes":{"@id":"unece:MetricCharacteristic"},"schema:domainIncludes":{"@id":"unece:Standard"},"rdfs:comment":"A prominent attribute or aspect of a metric (a standard of measurement)."},{"@id":"unece:elementVersionId","@type":["rdf:Property","owl:DatatypeProperty"],"rdfs:label":"elementVersionId","schema:rangeIncludes":{"@id":"schema:Text"},"schema:domainIncludes":{"@id":"unece:Standard"},"rdfs:comment":"The identifier of the version of a specific element within the referenced standard, such as the version of a data element."},{"@id":"unece:partId","@type":["rdf:Property","owl:DatatypeProperty"],"rdfs:label":"partId","schema:rangeIncludes":{"@id":"schema:Text"},"schema:domainIncludes":{"@id":"unece:Standard"},"rdfs:comment":"The identifier of a part of this referenced standard, such as a section or topic."},{"@id":"unece:applicableCondition","@type":["rdf:Property","owl:ObjectProperty"],"rdfs:label":"applicableCondition","schema:rangeIncludes":{"@id":"unece:ProductCharacteristicCondition"},"schema:domainIncludes":{"@id":"unece:ProductCharacteristic"},"rdfs:comment":"A condition applicable to this product characteristic."},{"@id":"unece:measurementMethodCode","@type":["rdf:Property","owl:DatatypeProperty"],"rdfs:label":"measurementMethodCode","schema:rangeIncludes":{"@id":"schema:Text"},"schema:domainIncludes":[{"@id":"unece:ProductCharacteristic"},{"@id":"unece:SustainabilityCharacteristic"},{"@id":"unece:TechnicalCharacteristic"}],"rdfs:comment":"A code specifying a measurement method for this product characteristic."},{"@id":"unece:productCharacteristicValueCode","@type":["rdf:Property","owl:DatatypeProperty"],"rdfs:label":"productCharacteristicValueCode","schema:rangeIncludes":{"@id":"schema:Text"},"schema:domainIncludes":{"@id":"unece:ProductCharacteristic"},"rdfs:comment":"The code specifying the value of this product characteristic."},{"@id":"unece:targetMarketDescription","@type":["rdf:Property","owl:DatatypeProperty"],"rdfs:label":"targetMarketDescription","schema:rangeIncludes":{"@id":"schema:Text"},"schema:domainIncludes":[{"@id":"unece:ProductCharacteristic"},{"@id":"unece:ProductBatchCharacteristic"}],"rdfs:comment":"A textual description of a target market for this product characteristic."},{"@id":"unece:valueBinaryFile","@type":["rdf:Property","owl:ObjectProperty"],"rdfs:label":"valueBinaryFile","schema:rangeIncludes":{"@id":"unece:BinaryFile"},"schema:domainIncludes":[{"@id":"unece:ProductCharacteristic"},{"@id":"unece:SustainabilityCharacteristic"}],"rdfs:comment":"A specified computer file or program stored in a binary format."},{"@id":"unece:applicableCorrectiveAction","@type":["rdf:Property","owl:ObjectProperty"],"rdfs:label":"applicableCorrectiveAction","schema:rangeIncludes":{"@id":"unece:CorrectiveAction"},"schema:domainIncludes":{"@id":"unece:InspectionResult"},"rdfs:comment":"A corrective action applicable to this specified inspection result."},{"@id":"unece:applicableInspectionResultCharacteristic","@type":["rdf:Property","owl:ObjectProperty"],"rdfs:label":"applicableInspectionResultCharacteristic","schema:rangeIncludes":{"@id":"unece:InspectionResultCharacteristic"},"schema:domainIncludes":{"@id":"unece:InspectionResult"},"rdfs:comment":"A characteristic applicable to this specified inspection result."},{"@id":"unece:applicablePreventiveAction","@type":["rdf:Property","owl:ObjectProperty"],"rdfs:label":"applicablePreventiveAction","schema:rangeIncludes":{"@id":"unece:PreventiveAction"},"schema:domainIncludes":{"@id":"unece:InspectionResult"},"rdfs:comment":"A preventive action applicable to this specified inspection result."},{"@id":"unece:applicableSpecifiedAction","@type":["rdf:Property","owl:ObjectProperty"],"rdfs:label":"applicableSpecifiedAction","schema:rangeIncludes":{"@id":"unece:SpecifiedAction"},"schema:domainIncludes":{"@id":"unece:InspectionResult"},"rdfs:comment":"The process of doing something in order to make something happen or to deal with a situation."},{"@id":"unece:approvalDateTime","@type":["rdf:Property","owl:DatatypeProperty"],"rdfs:label":"approvalDateTime","schema:rangeIncludes":{"@id":"schema:Text"},"schema:domainIncludes":{"@id":"unece:InspectionResult"},"rdfs:comment":"The date, time, date time, or other date time value for the approval of this specified inspection result."},{"@id":"unece:attachedInspectionNote","@type":["rdf:Property","owl:ObjectProperty"],"rdfs:label":"attachedInspectionNote","schema:rangeIncludes":{"@id":"unece:InspectionNote"},"schema:domainIncludes":{"@id":"unece:InspectionResult"},"rdfs:comment":"A note with additional information and or conclusions attached to this specified inspection result."},{"@id":"unece:expectedValueApplicableCharacteristic","@type":["rdf:Property","owl:ObjectProperty"],"rdfs:label":"expectedValueApplicableCharacteristic","schema:rangeIncludes":{"@id":"unece:InspectionResultCharacteristic"},"schema:domainIncludes":{"@id":"unece:InspectionResult"},"rdfs:comment":"An expected value for the inspection characteristic to be acquired by using the type of inspection applicable to this specified inspection result."},{"@id":"unece:inspectionDateTime","@type":["rdf:Property","owl:DatatypeProperty"],"rdfs:label":"inspectionDateTime","schema:rangeIncludes":{"@id":"schema:Text"},"schema:domainIncludes":{"@id":"unece:InspectionResult"},"rdfs:comment":"The date, time, date time, or other date time value of the inspection for this specified inspection result."},{"@id":"unece:inspectionParty","@type":["rdf:Property","owl:ObjectProperty"],"rdfs:label":"inspectionParty","schema:rangeIncludes":{"@id":"unece:Party"},"schema:domainIncludes":[{"@id":"unece:InspectionResult"},{"@id":"unece:TransportMovement"}],"rdfs:comment":""},{"@id":"unece:inspectionStandard","@type":["rdf:Property","owl:ObjectProperty"],"rdfs:label":"inspectionStandard","schema:rangeIncludes":{"@id":"unece:Standard"},"schema:domainIncludes":{"@id":"unece:InspectionResult"},"rdfs:comment":"A referenced inspection standard for this specified inspection result."},{"@id":"unece:laboratoryObservationResult","@type":["rdf:Property","owl:ObjectProperty"],"rdfs:label":"laboratoryObservationResult","schema:rangeIncludes":{"@id":"unece:ObservationResult"},"schema:domainIncludes":{"@id":"unece:InspectionResult"},"rdfs:comment":"A laboratory sample observation result for this specified inspection result."},{"@id":"unece:maximumStandardValueApplicableCharacteristic","@type":["rdf:Property","owl:ObjectProperty"],"rdfs:label":"maximumStandardValueApplicableCharacteristic","schema:rangeIncludes":{"@id":"unece:InspectionResultCharacteristic"},"schema:domainIncludes":{"@id":"unece:InspectionResult"},"rdfs:comment":"A maximum standard value for the inspection characteristic observed or measured by using the type of inspection applicable to this specified inspection result."},{"@id":"unece:minimumStandardValueApplicableCharacteristic","@type":["rdf:Property","owl:ObjectProperty"],"rdfs:label":"minimumStandardValueApplicableCharacteristic","schema:rangeIncludes":{"@id":"unece:InspectionResultCharacteristic"},"schema:domainIncludes":{"@id":"unece:InspectionResult"},"rdfs:comment":"A minimum standard value for the inspection characteristic observed or measured by using the type of inspection applicable to this specified inspection result."},{"@id":"unece:observedValueApplicableCharacteristic","@type":["rdf:Property","owl:ObjectProperty"],"rdfs:label":"observedValueApplicableCharacteristic","schema:rangeIncludes":{"@id":"unece:InspectionResultCharacteristic"},"schema:domainIncludes":{"@id":"unece:InspectionResult"},"rdfs:comment":"An observed value for the inspection characteristic acquired by using the type of inspection applicable to this specified inspection result."},{"@id":"unece:obtainedAssertion","@type":["rdf:Property","owl:ObjectProperty"],"rdfs:label":"obtainedAssertion","schema:rangeIncludes":{"@id":"unece:Assertion"},"schema:domainIncludes":{"@id":"unece:InspectionResult"},"rdfs:comment":"A sustainability assertion obtained by means of this specified inspection result."},{"@id":"unece:obtainedConformanceCertificate","@type":["rdf:Property","owl:ObjectProperty"],"rdfs:label":"obtainedConformanceCertificate","schema:rangeIncludes":{"@id":"unece:ConformanceCertificate"},"schema:domainIncludes":{"@id":"unece:InspectionResult"},"rdfs:comment":"A conformance certificate obtained by means of this specified inspection result."},{"@id":"unece:obtainedOrganizationalCertificate","@type":["rdf:Property","owl:ObjectProperty"],"rdfs:label":"obtainedOrganizationalCertificate","schema:rangeIncludes":{"@id":"unece:OrganizationalCertificate"},"schema:domainIncludes":{"@id":"unece:InspectionResult"},"rdfs:comment":"An organizational certificate obtained by means of this specified inspection result."},{"@id":"unece:obtainedProcessCertificate","@type":["rdf:Property","owl:ObjectProperty"],"rdfs:label":"obtainedProcessCertificate","schema:rangeIncludes":{"@id":"unece:ProcessCertificate"},"schema:domainIncludes":{"@id":"unece:InspectionResult"},"rdfs:comment":"A process certificate obtained by means of this specified inspection result."},{"@id":"unece:obtainedProductCertificate","@type":["rdf:Property","owl:ObjectProperty"],"rdfs:label":"obtainedProductCertificate","schema:rangeIncludes":{"@id":"unece:ProductCertificate"},"schema:domainIncludes":{"@id":"unece:InspectionResult"},"rdfs:comment":"A product certificate obtained by means of this specified inspection result."},{"@id":"unece:obtainedSpecifiedCertificate","@type":["rdf:Property","owl:ObjectProperty"],"rdfs:label":"obtainedSpecifiedCertificate","schema:rangeIncludes":{"@id":"unece:SpecifiedCertificate"},"schema:domainIncludes":{"@id":"unece:InspectionResult"},"rdfs:comment":"A certificate obtained by means of this specified inspection result."},{"@id":"unece:outsourcedInspectionParty","@type":["rdf:Property","owl:ObjectProperty"],"rdfs:label":"outsourcedInspectionParty","schema:rangeIncludes":{"@id":"unece:Party"},"schema:domainIncludes":{"@id":"unece:InspectionResult"},"rdfs:comment":""},{"@id":"unece:relatedAssessment","@type":["rdf:Property","owl:ObjectProperty"],"rdfs:label":"relatedAssessment","schema:rangeIncludes":{"@id":"unece:Assessment"},"schema:domainIncludes":{"@id":"unece:InspectionResult"},"rdfs:comment":"An assessment related to this specified inspection result."},{"@id":"unece:relatedInstructions","@type":["rdf:Property","owl:ObjectProperty"],"rdfs:label":"relatedInstructions","schema:rangeIncludes":{"@id":"unece:InspectionInstructions"},"schema:domainIncludes":{"@id":"unece:InspectionResult"},"rdfs:comment":"Inspection instructions related to this specified inspection result."},{"@id":"unece:relatedMaterialType","@type":["rdf:Property","owl:DatatypeProperty"],"rdfs:label":"relatedMaterialType","schema:rangeIncludes":{"@id":"schema:Text"},"schema:domainIncludes":{"@id":"unece:InspectionResult"},"rdfs:comment":"A material type, expressed as text, related to this specified inspection result."},{"@id":"unece:relatedProductType","@type":["rdf:Property","owl:DatatypeProperty"],"rdfs:label":"relatedProductType","schema:rangeIncludes":{"@id":"schema:Text"},"schema:domainIncludes":{"@id":"unece:InspectionResult"},"rdfs:comment":"A product type, expressed as text, related to this specified inspection result."},{"@id":"unece:specifiedInspectionReference","@type":["rdf:Property","owl:ObjectProperty"],"rdfs:label":"specifiedInspectionReference","schema:rangeIncludes":{"@id":"unece:InspectionReference"},"schema:domainIncludes":{"@id":"unece:InspectionResult"},"rdfs:comment":"An inspection reference specified for this inspection result."},{"@id":"unece:applicableHazardousMaterial","@type":["rdf:Property","owl:ObjectProperty"],"rdfs:label":"applicableHazardousMaterial","schema:rangeIncludes":{"@id":"unece:HazardousMaterial"},"schema:domainIncludes":{"@id":"unece:Chemical"},"rdfs:comment":"An applicable toxicological hazardous material for this distinct chemical."},{"@id":"unece:formulaDescription","@type":["rdf:Property","owl:DatatypeProperty"],"rdfs:label":"formulaDescription","schema:rangeIncludes":{"@id":"schema:Text"},"schema:domainIncludes":{"@id":"unece:Chemical"},"rdfs:comment":"The textual description of the formula for this distinct chemical."},{"@id":"unece:molecularWeightMeasure","@type":["rdf:Property","owl:ObjectProperty"],"rdfs:label":"molecularWeightMeasure","schema:rangeIncludes":{"@id":"unece:MeasureType"},"schema:domainIncludes":{"@id":"unece:Chemical"},"rdfs:comment":""},{"@id":"unece:presenceMeasurement","@type":["rdf:Property","owl:ObjectProperty"],"rdfs:label":"presenceMeasurement","schema:rangeIncludes":{"@id":"unece:IngredientRangeMeasurement"},"schema:domainIncludes":{"@id":"unece:Chemical"},"rdfs:comment":"A measurement of the range of the presence of an ingredient in this distinct chemical."},{"@id":"unece:synonymName","@type":["rdf:Property","owl:DatatypeProperty"],"rdfs:label":"synonymName","schema:rangeIncludes":{"@id":"schema:Text"},"schema:domainIncludes":{"@id":"unece:Chemical"},"rdfs:comment":"A synonym name, expressed as text, for this distinct chemical."},{"@id":"unece:volumeMeasure","@type":["rdf:Property","owl:ObjectProperty"],"rdfs:label":"volumeMeasure","schema:rangeIncludes":{"@id":"unece:MeasureType"},"schema:domainIncludes":[{"@id":"unece:Chemical"},{"@id":"unece:SpecifiedMaterial"},{"@id":"unece:ProductionWasteMaterial"},{"@id":"unece:TransportationWasteMaterial"}],"rdfs:comment":""},{"@id":"unece:volumeRatioMeasure","@type":["rdf:Property","owl:ObjectProperty"],"rdfs:label":"volumeRatioMeasure","schema:rangeIncludes":{"@id":"unece:MeasureType"},"schema:domainIncludes":[{"@id":"unece:Chemical"},{"@id":"unece:SpecifiedMaterial"}],"rdfs:comment":""},{"@id":"unece:applicableInspectionResult","@type":["rdf:Property","owl:ObjectProperty"],"rdfs:label":"applicableInspectionResult","schema:rangeIncludes":{"@id":"unece:InspectionResult"},"schema:domainIncludes":[{"@id":"unece:SustainabilityCharacteristic"},{"@id":"unece:SustainabilityInspection"}],"rdfs:comment":"A specified inspection result applicable to this sustainability characteristic."},{"@id":"unece:subordinateCategoryCode","@type":["rdf:Property","owl:DatatypeProperty"],"rdfs:label":"subordinateCategoryCode","schema:rangeIncludes":{"@id":"schema:Text"},"schema:domainIncludes":{"@id":"unece:SustainabilityCharacteristic"},"rdfs:comment":"The subordinate category for this sustainability characteristic."},{"@id":"unece:valuePeriod","@type":["rdf:Property","owl:ObjectProperty"],"rdfs:label":"valuePeriod","schema:rangeIncludes":{"@id":"unece:SpecifiedPeriod"},"schema:domainIncludes":{"@id":"unece:SustainabilityCharacteristic"},"rdfs:comment":"A specified period of time."},{"@id":"unece:executionParty","@type":["rdf:Property","owl:ObjectProperty"],"rdfs:label":"executionParty","schema:rangeIncludes":{"@id":"unece:Party"},"schema:domainIncludes":[{"@id":"unece:SustainabilityInspection"},{"@id":"unece:SpecifiedInspection"}],"rdfs:comment":""},{"@id":"unece:executionPerson","@type":["rdf:Property","owl:ObjectProperty"],"rdfs:label":"executionPerson","schema:rangeIncludes":{"@id":"unece:InspectionPerson"},"schema:domainIncludes":[{"@id":"unece:SustainabilityInspection"},{"@id":"unece:SpecifiedInspection"}],"rdfs:comment":"The inspector executing this specified inspection."},{"@id":"unece:outsourcedIndicator","@type":["rdf:Property","owl:DatatypeProperty"],"rdfs:label":"outsourcedIndicator","schema:rangeIncludes":{"@id":"schema:Boolean"},"schema:domainIncludes":[{"@id":"unece:SustainabilityInspection"},{"@id":"unece:SpecifiedInspection"}],"rdfs:comment":"The indication of whether or not this specified inspection is outsourced."},{"@id":"unece:specifiedInspectionEvent","@type":["rdf:Property","owl:ObjectProperty"],"rdfs:label":"specifiedInspectionEvent","schema:rangeIncludes":{"@id":"unece:InspectionEvent"},"schema:domainIncludes":[{"@id":"unece:SustainabilityInspection"},{"@id":"unece:SpecifiedInspection"},{"@id":"unece:Consignment"},{"@id":"unece:ConsignmentItem"},{"@id":"unece:LogisticsLocation"}],"rdfs:comment":"A specified inspection event for this sustainability inspection."},{"@id":"unece:specifiedInspectionStatus","@type":["rdf:Property","owl:ObjectProperty"],"rdfs:label":"specifiedInspectionStatus","schema:rangeIncludes":{"@id":"unece:InspectionStatus"},"schema:domainIncludes":[{"@id":"unece:SustainabilityInspection"},{"@id":"unece:SpecifiedInspection"}],"rdfs:comment":"The inspection status specified for this sustainability inspection."},{"@id":"unece:measuredAccuracyMeasure","@type":["rdf:Property","owl:ObjectProperty"],"rdfs:label":"measuredAccuracyMeasure","schema:rangeIncludes":{"@id":"unece:MeasureType"},"schema:domainIncludes":[{"@id":"unece:InspectionResultCharacteristic"},{"@id":"unece:ObservationResultCharacteristic"}],"rdfs:comment":""},{"@id":"unece:measuredValue","@type":["rdf:Property","owl:DatatypeProperty"],"rdfs:label":"measuredValue","schema:rangeIncludes":{"@id":"schema:Text"},"schema:domainIncludes":[{"@id":"unece:InspectionResultCharacteristic"},{"@id":"unece:ObservationResultCharacteristic"}],"rdfs:comment":"The measured value, expressed as text, for this inspection result characteristic."},{"@id":"unece:measuredValueMeasure","@type":["rdf:Property","owl:ObjectProperty"],"rdfs:label":"measuredValueMeasure","schema:rangeIncludes":{"@id":"unece:MeasureType"},"schema:domainIncludes":[{"@id":"unece:InspectionResultCharacteristic"},{"@id":"unece:ObservationResultCharacteristic"}],"rdfs:comment":""},{"@id":"unece:qualityResultCode","@type":["rdf:Property","owl:DatatypeProperty"],"rdfs:label":"qualityResultCode","schema:rangeIncludes":{"@id":"schema:Text"},"schema:domainIncludes":[{"@id":"unece:InspectionResultCharacteristic"},{"@id":"unece:ObservationResultCharacteristic"}],"rdfs:comment":"The code specifying the quality of the result for this inspection result characteristic."},{"@id":"unece:qualityResultDescription","@type":["rdf:Property","owl:DatatypeProperty"],"rdfs:label":"qualityResultDescription","schema:rangeIncludes":{"@id":"schema:Text"},"schema:domainIncludes":[{"@id":"unece:InspectionResultCharacteristic"},{"@id":"unece:ObservationResultCharacteristic"}],"rdfs:comment":"A textual description of the quality of the result for this inspection result characteristic."},{"@id":"unece:qualityResultReferenceLevelDescription","@type":["rdf:Property","owl:DatatypeProperty"],"rdfs:label":"qualityResultReferenceLevelDescription","schema:rangeIncludes":{"@id":"schema:Text"},"schema:domainIncludes":{"@id":"unece:InspectionResultCharacteristic"},"rdfs:comment":"A textual description of the reference level for the quality of the result for this inspection result characteristic."},{"@id":"unece:range","@type":["rdf:Property","owl:DatatypeProperty"],"rdfs:label":"range","schema:rangeIncludes":{"@id":"schema:Text"},"schema:domainIncludes":[{"@id":"unece:InspectionResultCharacteristic"},{"@id":"unece:ObservationResultCharacteristic"}],"rdfs:comment":"The range, expressed as text, of the values of the measurements performed for this inspection result characteristic."},{"@id":"unece:applicableNote","@type":["rdf:Property","owl:ObjectProperty"],"rdfs:label":"applicableNote","schema:rangeIncludes":{"@id":"unece:Note"},"schema:domainIncludes":[{"@id":"unece:Observation"},{"@id":"unece:LogisticsTransportEquipment"},{"@id":"unece:TransportEvent"},{"@id":"unece:ConsignmentItem"}],"rdfs:comment":"A textual or coded description, such as a remark or additional information."},{"@id":"unece:biologicalSeverityDescription","@type":["rdf:Property","owl:DatatypeProperty"],"rdfs:label":"biologicalSeverityDescription","schema:rangeIncludes":{"@id":"schema:Text"},"schema:domainIncludes":{"@id":"unece:HazardousMaterial"},"rdfs:comment":"The textual description of the biological severity of this toxicological hazardous material."},{"@id":"unece:entryRouteDescription","@type":["rdf:Property","owl:DatatypeProperty"],"rdfs:label":"entryRouteDescription","schema:rangeIncludes":{"@id":"schema:Text"},"schema:domainIncludes":{"@id":"unece:HazardousMaterial"},"rdfs:comment":"A textual description of the entry route of this toxicological hazardous material."},{"@id":"unece:reproductiveToxinName","@type":["rdf:Property","owl:DatatypeProperty"],"rdfs:label":"reproductiveToxinName","schema:rangeIncludes":{"@id":"schema:Text"},"schema:domainIncludes":{"@id":"unece:HazardousMaterial"},"rdfs:comment":"The name, expressed as text, of the reproductive toxin in this toxicological hazardous material."},{"@id":"unece:applicableSpecifiedTemperature","@type":["rdf:Property","owl:ObjectProperty"],"rdfs:label":"applicableSpecifiedTemperature","schema:rangeIncludes":{"@id":"unece:SpecifiedTemperature"},"schema:domainIncludes":{"@id":"unece:AppliedChemicalTreatment"},"rdfs:comment":"A specified temperature value or range of values."},{"@id":"unece:appliedPeriod","@type":["rdf:Property","owl:ObjectProperty"],"rdfs:label":"appliedPeriod","schema:rangeIncludes":{"@id":"unece:SpecifiedPeriod"},"schema:domainIncludes":{"@id":"unece:AppliedChemicalTreatment"},"rdfs:comment":"A specified period of time."},{"@id":"unece:chemicalConcentrationMeasure","@type":["rdf:Property","owl:ObjectProperty"],"rdfs:label":"chemicalConcentrationMeasure","schema:rangeIncludes":{"@id":"unece:MeasureType"},"schema:domainIncludes":{"@id":"unece:AppliedChemicalTreatment"},"rdfs:comment":""},{"@id":"unece:methodName","@type":["rdf:Property","owl:DatatypeProperty"],"rdfs:label":"methodName","schema:rangeIncludes":{"@id":"schema:Text"},"schema:domainIncludes":{"@id":"unece:AppliedChemicalTreatment"},"rdfs:comment":"The name, expressed as text, of the method of this applied chemical treatment."},{"@id":"unece:resultAuthentication","@type":["rdf:Property","owl:ObjectProperty"],"rdfs:label":"resultAuthentication","schema:rangeIncludes":{"@id":"unece:Authentication"},"schema:domainIncludes":{"@id":"unece:AppliedChemicalTreatment"},"rdfs:comment":"A proof that a document is genuine."},{"@id":"unece:resultNote","@type":["rdf:Property","owl:ObjectProperty"],"rdfs:label":"resultNote","schema:rangeIncludes":{"@id":"unece:Note"},"schema:domainIncludes":{"@id":"unece:AppliedChemicalTreatment"},"rdfs:comment":"A textual or coded description, such as a remark or additional information."},{"@id":"unece:relatedPolicy","@type":["rdf:Property","owl:ObjectProperty"],"rdfs:label":"relatedPolicy","schema:rangeIncludes":{"@id":"unece:Policy"},"schema:domainIncludes":{"@id":"unece:Assertion"},"rdfs:comment":"A compliance policy related to this sustainability assertion."},{"@id":"unece:assessedObject","@type":["rdf:Property","owl:ObjectProperty"],"rdfs:label":"assessedObject","schema:rangeIncludes":{"@id":"unece:Object"},"schema:domainIncludes":{"@id":"unece:Assessment"},"rdfs:comment":"Anything that is visible or tangible, such as a product, process, or organization."},{"@id":"unece:assessorParty","@type":["rdf:Property","owl:ObjectProperty"],"rdfs:label":"assessorParty","schema:rangeIncludes":{"@id":"unece:Party"},"schema:domainIncludes":{"@id":"unece:Assessment"},"rdfs:comment":""},{"@id":"unece:associatedBinaryFile","@type":["rdf:Property","owl:ObjectProperty"],"rdfs:label":"associatedBinaryFile","schema:rangeIncludes":{"@id":"unece:BinaryFile"},"schema:domainIncludes":{"@id":"unece:Assessment"},"rdfs:comment":"A specified computer file or program stored in a binary format."},{"@id":"unece:reportDateTime","@type":["rdf:Property","owl:DatatypeProperty"],"rdfs:label":"reportDateTime","schema:rangeIncludes":{"@id":"schema:Text"},"schema:domainIncludes":{"@id":"unece:Assessment"},"rdfs:comment":"The date, time, date time or other date time value of the report of this specified assessment."},{"@id":"unece:reportId","@type":["rdf:Property","owl:DatatypeProperty"],"rdfs:label":"reportId","schema:rangeIncludes":{"@id":"schema:Text"},"schema:domainIncludes":{"@id":"unece:Assessment"},"rdfs:comment":"The report identifier for this specified assessment."},{"@id":"unece:selfAssessedIndicator","@type":["rdf:Property","owl:DatatypeProperty"],"rdfs:label":"selfAssessedIndicator","schema:rangeIncludes":{"@id":"schema:Boolean"},"schema:domainIncludes":{"@id":"unece:Assessment"},"rdfs:comment":"The indication of whether or not this specified assessment is self assessed."},{"@id":"unece:verifiedIndicator","@type":["rdf:Property","owl:DatatypeProperty"],"rdfs:label":"verifiedIndicator","schema:rangeIncludes":{"@id":"schema:Boolean"},"schema:domainIncludes":{"@id":"unece:Assessment"},"rdfs:comment":"The indication of whether or not this specified assessment is verified."},{"@id":"unece:verifierParty","@type":["rdf:Property","owl:ObjectProperty"],"rdfs:label":"verifierParty","schema:rangeIncludes":{"@id":"unece:Party"},"schema:domainIncludes":{"@id":"unece:Assessment"},"rdfs:comment":""},{"@id":"unece:assertion","@type":["rdf:Property","owl:DatatypeProperty"],"rdfs:label":"assertion","schema:rangeIncludes":{"@id":"schema:Text"},"schema:domainIncludes":[{"@id":"unece:OrganizationalCertification"},{"@id":"unece:ProcessCertification"},{"@id":"unece:ProductBatchCertification"},{"@id":"unece:SpecifiedCertification"},{"@id":"unece:TradeProductCertification"},{"@id":"unece:AnimalCertification"}],"rdfs:comment":"An assertion, expressed as text, for this animal certification."},{"@id":"unece:assertionCode","@type":["rdf:Property","owl:DatatypeProperty"],"rdfs:label":"assertionCode","schema:rangeIncludes":{"@id":"schema:Text"},"schema:domainIncludes":[{"@id":"unece:OrganizationalCertification"},{"@id":"unece:ProcessCertification"},{"@id":"unece:ProductBatchCertification"},{"@id":"unece:SpecifiedCertification"},{"@id":"unece:TradeProductCertification"},{"@id":"unece:AnimalCertification"}],"rdfs:comment":"A code specifying an assertion for this specified certification, such as a claim that a product is free of hazardous chemicals."},{"@id":"unece:responsibleAgency","@type":["rdf:Property","owl:DatatypeProperty"],"rdfs:label":"responsibleAgency","schema:rangeIncludes":{"@id":"schema:Text"},"schema:domainIncludes":[{"@id":"unece:OrganizationalCertification"},{"@id":"unece:ProcessCertification"},{"@id":"unece:ProductBatchCertification"},{"@id":"unece:SpecifiedCertification"},{"@id":"unece:TradeProductCertification"},{"@id":"unece:AnimalCertification"}],"rdfs:comment":"A responsible agency, expressed as text, for this specified certification."},{"@id":"unece:standard","@type":["rdf:Property","owl:DatatypeProperty"],"rdfs:label":"standard","schema:rangeIncludes":{"@id":"schema:Text"},"schema:domainIncludes":[{"@id":"unece:OrganizationalCertification"},{"@id":"unece:ProcessCertification"},{"@id":"unece:ProductBatchCertification"},{"@id":"unece:SpecifiedCertification"},{"@id":"unece:TradeProductCertification"},{"@id":"unece:AnimalCertification"}],"rdfs:comment":"A standard, expressed as text, for this specified certification."},{"@id":"unece:measuredAttributeTypeCode","@type":["rdf:Property","owl:DatatypeProperty"],"rdfs:label":"measuredAttributeTypeCode","schema:rangeIncludes":{"@id":"unece:MeasuredAttributeCodeList"},"schema:domainIncludes":{"@id":"unece:ProcessCharacteristic"},"rdfs:comment":"The code specifying the type of this process characteristic."},{"@id":"unece:capacityValueMeasure","@type":["rdf:Property","owl:ObjectProperty"],"rdfs:label":"capacityValueMeasure","schema:rangeIncludes":{"@id":"unece:MeasureType"},"schema:domainIncludes":{"@id":"unece:TechnicalCharacteristic"},"rdfs:comment":""},{"@id":"unece:certificationCode","@type":["rdf:Property","owl:DatatypeProperty"],"rdfs:label":"certificationCode","schema:rangeIncludes":{"@id":"schema:Text"},"schema:domainIncludes":{"@id":"unece:TechnicalCharacteristic"},"rdfs:comment":"The code specifying the certification granted to this technical characteristic."},{"@id":"unece:constructionDateTime","@type":["rdf:Property","owl:DatatypeProperty"],"rdfs:label":"constructionDateTime","schema:rangeIncludes":{"@id":"schema:Text"},"schema:domainIncludes":{"@id":"unece:TechnicalCharacteristic"},"rdfs:comment":"The date, time, date time, or other date time value of the construction of this technical characteristic."},{"@id":"unece:latestRenovationDateTime","@type":["rdf:Property","owl:DatatypeProperty"],"rdfs:label":"latestRenovationDateTime","schema:rangeIncludes":{"@id":"schema:Text"},"schema:domainIncludes":[{"@id":"unece:TechnicalCharacteristic"},{"@id":"unece:ExperienceFacility"}],"rdfs:comment":"The date of the latest renovation of this experience facility."},{"@id":"unece:appliedDilutionNumeric","@type":["rdf:Property","owl:DatatypeProperty"],"rdfs:label":"appliedDilutionNumeric","schema:rangeIncludes":{"@id":"schema:Text"},"schema:domainIncludes":{"@id":"unece:ObservationResultCharacteristic"},"rdfs:comment":"The rate of the applied dilution for this sample observation result characteristic."},{"@id":"unece:methodParameterId","@type":["rdf:Property","owl:DatatypeProperty"],"rdfs:label":"methodParameterId","schema:rangeIncludes":{"@id":"schema:Text"},"schema:domainIncludes":{"@id":"unece:ObservationResultCharacteristic"},"rdfs:comment":"The identifier of the method parameter for this sample observation result characteristic."},{"@id":"unece:parameterValue","@type":["rdf:Property","owl:DatatypeProperty"],"rdfs:label":"parameterValue","schema:rangeIncludes":{"@id":"schema:Text"},"schema:domainIncludes":{"@id":"unece:ObservationResultCharacteristic"},"rdfs:comment":"The parameter value, expressed as text, for this sample observation result characteristic."},{"@id":"unece:referenceLevelQualityResultDescription","@type":["rdf:Property","owl:DatatypeProperty"],"rdfs:label":"referenceLevelQualityResultDescription","schema:rangeIncludes":{"@id":"schema:Text"},"schema:domainIncludes":{"@id":"unece:ObservationResultCharacteristic"},"rdfs:comment":"The textual description of the reference level for the quality of the result for this sample observation result characteristic."},{"@id":"unece:auditDateTime","@type":["rdf:Property","owl:DatatypeProperty"],"rdfs:label":"auditDateTime","schema:rangeIncludes":{"@id":"schema:DateTime"},"schema:domainIncludes":{"@id":"unece:SpecifiedCertification"},"rdfs:comment":"An audit date, time, date time or other date time value for this specified certification."},{"@id":"unece:relatedStandard","@type":["rdf:Property","owl:ObjectProperty"],"rdfs:label":"relatedStandard","schema:rangeIncludes":{"@id":"unece:Standard"},"schema:domainIncludes":{"@id":"unece:SpecifiedCertification"},"rdfs:comment":"A referenced standard related to this specified certification."},{"@id":"unece:grantedParty","@type":["rdf:Property","owl:ObjectProperty"],"rdfs:label":"grantedParty","schema:rangeIncludes":{"@id":"unece:Party"},"schema:domainIncludes":{"@id":"unece:Licence"},"rdfs:comment":""},{"@id":"unece:verifiedObject","@type":["rdf:Property","owl:ObjectProperty"],"rdfs:label":"verifiedObject","schema:rangeIncludes":{"@id":"unece:Object"},"schema:domainIncludes":[{"@id":"unece:Licence"},{"@id":"unece:SpecifiedDeclaration"}],"rdfs:comment":"Anything that is visible or tangible, such as a product, process, or organization."},{"@id":"unece:associatedTax","@type":["rdf:Property","owl:ObjectProperty"],"rdfs:label":"associatedTax","schema:rangeIncludes":{"@id":"unece:RegisteredTax"},"schema:domainIncludes":{"@id":"unece:TaxRegistration"},"rdfs:comment":"A registered tax or duty system pertaining to an authority."},{"@id":"unece:iOSSId","@type":["rdf:Property","owl:DatatypeProperty"],"rdfs:label":"iOSSId","schema:rangeIncludes":{"@id":"schema:Text"},"schema:domainIncludes":{"@id":"unece:TaxRegistration"},"rdfs:comment":"The Import One Stop Shop (IOSS) identifier for this tax registration."},{"@id":"unece:reportedInspectionResult","@type":["rdf:Property","owl:ObjectProperty"],"rdfs:label":"reportedInspectionResult","schema:rangeIncludes":{"@id":"unece:InspectionResult"},"schema:domainIncludes":{"@id":"unece:SpecifiedInspection"},"rdfs:comment":"The result reported for this specified inspection."},{"@id":"unece:attainedAcademicQualification","@type":["rdf:Property","owl:ObjectProperty"],"rdfs:label":"attainedAcademicQualification","schema:rangeIncludes":{"@id":"unece:AcademicQualification"},"schema:domainIncludes":[{"@id":"unece:AuthoritativeSignatoryPerson"},{"@id":"unece:TransportPerson"}],"rdfs:comment":"An academic qualification attained by this authoritative signatory person."},{"@id":"unece:attainedSpecifiedQualification","@type":["rdf:Property","owl:ObjectProperty"],"rdfs:label":"attainedSpecifiedQualification","schema:rangeIncludes":{"@id":"unece:SpecifiedQualification"},"schema:domainIncludes":{"@id":"unece:InspectionPerson"},"rdfs:comment":"The specified qualification attained by this inspection person."},{"@id":"unece:inspectionPersonName","@type":["rdf:Property","owl:DatatypeProperty"],"rdfs:label":"inspectionPersonName","schema:rangeIncludes":{"@id":"schema:Text"},"schema:domainIncludes":{"@id":"unece:InspectionPerson"},"rdfs:comment":"The name or set of names, expressed as text, by which this inspection person is known."},{"@id":"unece:bathingProhibitionCaution","@type":["rdf:Property","owl:DatatypeProperty"],"rdfs:label":"bathingProhibitionCaution","schema:rangeIncludes":{"@id":"schema:Text"},"schema:domainIncludes":{"@id":"unece:Source"},"rdfs:comment":"A caution, expressed as text, of a bathing prohibition for this water source."},{"@id":"unece:characteristicCode","@type":["rdf:Property","owl:DatatypeProperty"],"rdfs:label":"characteristicCode","schema:rangeIncludes":{"@id":"schema:Text"},"schema:domainIncludes":{"@id":"unece:Source"},"rdfs:comment":"The code specifying the characteristic of this water source."},{"@id":"unece:drinkingProhibitionCaution","@type":["rdf:Property","owl:DatatypeProperty"],"rdfs:label":"drinkingProhibitionCaution","schema:rangeIncludes":{"@id":"schema:Text"},"schema:domainIncludes":{"@id":"unece:Source"},"rdfs:comment":"A caution, expressed as text, of a drinking prohibition for this water source."},{"@id":"unece:healthBenefit","@type":["rdf:Property","owl:DatatypeProperty"],"rdfs:label":"healthBenefit","schema:rangeIncludes":{"@id":"schema:Text"},"schema:domainIncludes":{"@id":"unece:Source"},"rdfs:comment":"A health benefit, expressed as text, for this water source."},{"@id":"unece:licenceId","@type":["rdf:Property","owl:DatatypeProperty"],"rdfs:label":"licenceId","schema:rangeIncludes":{"@id":"schema:Text"},"schema:domainIncludes":{"@id":"unece:GovernmentRegistration"},"rdfs:comment":"The identifier of a licence for this government registration."},{"@id":"unece:recordedDate","@type":["rdf:Property","owl:DatatypeProperty"],"rdfs:label":"recordedDate","schema:rangeIncludes":{"@id":"schema:Text"},"schema:domainIncludes":{"@id":"unece:GovernmentRegistration"},"rdfs:comment":"The date that this government registration was recorded."},{"@id":"unece:consignmentRiskRelatedCode","@type":["rdf:Property","owl:DatatypeProperty"],"rdfs:label":"consignmentRiskRelatedCode","schema:rangeIncludes":{"@id":"schema:Text"},"schema:domainIncludes":{"@id":"unece:RiskAnalysisResult"},"rdfs:comment":"A code specifying a consignment related risk for this logistics risk analysis result."},{"@id":"unece:levelCode","@type":["rdf:Property","owl:DatatypeProperty"],"rdfs:label":"levelCode","schema:rangeIncludes":{"@id":"schema:Text"},"schema:domainIncludes":[{"@id":"unece:RiskAnalysisResult"},{"@id":"unece:LogisticsPackaging"}],"rdfs:comment":"The code specifying the level for this logistics risk analysis result."},{"@id":"unece:partyRiskRelatedCode","@type":["rdf:Property","owl:DatatypeProperty"],"rdfs:label":"partyRiskRelatedCode","schema:rangeIncludes":{"@id":"schema:Text"},"schema:domainIncludes":{"@id":"unece:RiskAnalysisResult"},"rdfs:comment":"A code specifying a party related risk for this logistics risk analysis result."},{"@id":"unece:screeningMethodCode","@type":["rdf:Property","owl:DatatypeProperty"],"rdfs:label":"screeningMethodCode","schema:rangeIncludes":{"@id":"schema:Text"},"schema:domainIncludes":{"@id":"unece:RiskAnalysisResult"},"rdfs:comment":"A code specifying a method of screening used in this logistics risk analysis result."},{"@id":"unece:securityExemptionCode","@type":["rdf:Property","owl:DatatypeProperty"],"rdfs:label":"securityExemptionCode","schema:rangeIncludes":{"@id":"schema:Text"},"schema:domainIncludes":{"@id":"unece:RiskAnalysisResult"},"rdfs:comment":"A code specifying a security exemption for this logistics risk analysis result."},{"@id":"unece:transportEquipmentRiskRelatedCode","@type":["rdf:Property","owl:DatatypeProperty"],"rdfs:label":"transportEquipmentRiskRelatedCode","schema:rangeIncludes":{"@id":"schema:Text"},"schema:domainIncludes":{"@id":"unece:RiskAnalysisResult"},"rdfs:comment":"A code specifying a transport equipment related risk for this logistics risk analysis result."},{"@id":"unece:transportMovementRiskRelatedCode","@type":["rdf:Property","owl:DatatypeProperty"],"rdfs:label":"transportMovementRiskRelatedCode","schema:rangeIncludes":{"@id":"schema:Text"},"schema:domainIncludes":{"@id":"unece:RiskAnalysisResult"},"rdfs:comment":"A code specifying a transport movement related risk for this logistics risk analysis result."},{"@id":"unece:softwareOperatingSystem","@type":["rdf:Property","owl:DatatypeProperty"],"rdfs:label":"softwareOperatingSystem","schema:rangeIncludes":{"@id":"schema:Text"},"schema:domainIncludes":{"@id":"unece:ConformanceCertificate"},"rdfs:comment":"The software operating system, expressed as text, for which this conformance certificate is produced."},{"@id":"unece:sampledObjectMinimumRequiredObjectSizeMeasure","@type":["rdf:Property","owl:ObjectProperty"],"rdfs:label":"sampledObjectMinimumRequiredObjectSizeMeasure","schema:rangeIncludes":{"@id":"unece:MeasureType"},"schema:domainIncludes":{"@id":"unece:LaboratoryObservationAnalysisMethod"},"rdfs:comment":""},{"@id":"unece:changeableIndicator","@type":["rdf:Property","owl:DatatypeProperty"],"rdfs:label":"changeableIndicator","schema:rangeIncludes":{"@id":"schema:Boolean"},"schema:domainIncludes":[{"@id":"unece:ControlSettingParameter"},{"@id":"unece:OperationalParameter"}],"rdfs:comment":"The indication whether or not this control setting parameter is changeable."},{"@id":"unece:requestedRange","@type":["rdf:Property","owl:ObjectProperty"],"rdfs:label":"requestedRange","schema:rangeIncludes":{"@id":"unece:Range"},"schema:domainIncludes":{"@id":"unece:ControlSettingParameter"},"rdfs:comment":"A row, line or series, commonly used to express the difference between lowest and highest values."},{"@id":"unece:definedRange","@type":["rdf:Property","owl:ObjectProperty"],"rdfs:label":"definedRange","schema:rangeIncludes":{"@id":"unece:Range"},"schema:domainIncludes":{"@id":"unece:OperationalParameter"},"rdfs:comment":"A row, line or series, commonly used to express the difference between lowest and highest values."},{"@id":"unece:conditionCode","@type":["rdf:Property","owl:DatatypeProperty"],"rdfs:label":"conditionCode","schema:rangeIncludes":{"@id":"schema:Text"},"schema:domainIncludes":[{"@id":"unece:InspectionStatus"},{"@id":"unece:LogisticsPackaging"},{"@id":"unece:SupplyChainPackaging"}],"rdfs:comment":"A code specifying a condition of this logistics packaging."},{"@id":"unece:emailCommunication","@type":["rdf:Property","owl:ObjectProperty"],"rdfs:label":"emailCommunication","schema:rangeIncludes":{"@id":"unece:Communication"},"schema:domainIncludes":{"@id":"unece:LaboratoryObservationContact"},"rdfs:comment":"The exchange of thoughts, messages, or information, as universally exchanged by speech, signals, writing, or behaviour between persons and/or organizations."},{"@id":"unece:disposalInstructionsRecyclingDescriptionCode","@type":["rdf:Property","owl:DatatypeProperty"],"rdfs:label":"disposalInstructionsRecyclingDescriptionCode","schema:rangeIncludes":{"@id":"schema:Text"},"schema:domainIncludes":{"@id":"unece:DisposalInstructions"},"rdfs:comment":"A code describing recycling in these disposal instructions."},{"@id":"unece:materialId","@type":["rdf:Property","owl:DatatypeProperty"],"rdfs:label":"materialId","schema:rangeIncludes":{"@id":"schema:Text"},"schema:domainIncludes":[{"@id":"unece:DisposalInstructions"},{"@id":"unece:ReturnableAssetInstructions"}],"rdfs:comment":"An identifier of the material to which these returnable asset instructions apply."},{"@id":"unece:recyclingProcedure","@type":["rdf:Property","owl:DatatypeProperty"],"rdfs:label":"recyclingProcedure","schema:rangeIncludes":{"@id":"schema:Text"},"schema:domainIncludes":{"@id":"unece:DisposalInstructions"},"rdfs:comment":"A recycling procedure, expressed as text, for these disposal instructions."},{"@id":"unece:occurrenceLocation","@type":["rdf:Property","owl:ObjectProperty"],"rdfs:label":"occurrenceLocation","schema:rangeIncludes":{"@id":"unece:Location"},"schema:domainIncludes":[{"@id":"unece:InspectionEvent"},{"@id":"unece:SupplyChainEvent"}],"rdfs:comment":"A reference to a physical location or place."},{"@id":"unece:instructionsType","@type":["rdf:Property","owl:DatatypeProperty"],"rdfs:label":"instructionsType","schema:rangeIncludes":{"@id":"schema:Text"},"schema:domainIncludes":[{"@id":"unece:InspectionInstructions"},{"@id":"unece:LaboratoryObservationInstructions"},{"@id":"unece:PackagingInstructions"}],"rdfs:comment":"A type, expressed as text, of these packaging instructions."},{"@id":"unece:interpretationCode","@type":["rdf:Property","owl:DatatypeProperty"],"rdfs:label":"interpretationCode","schema:rangeIncludes":{"@id":"schema:Text"},"schema:domainIncludes":[{"@id":"unece:InspectionInstructions"},{"@id":"unece:LaboratoryObservationInstructions"}],"rdfs:comment":"The code specifying the interpretation for this laboratory instruction."},{"@id":"unece:latestUpdateDateTime","@type":["rdf:Property","owl:DatatypeProperty"],"rdfs:label":"latestUpdateDateTime","schema:rangeIncludes":{"@id":"schema:Text"},"schema:domainIncludes":[{"@id":"unece:InspectionInstructions"},{"@id":"unece:LaboratoryObservationInstructions"}],"rdfs:comment":"The date, time, date time, or other date time value of the latest update of this set of inspection instructions."},{"@id":"unece:laboratoryObservationInstructionsDescriptionCode","@type":["rdf:Property","owl:DatatypeProperty"],"rdfs:label":"laboratoryObservationInstructionsDescriptionCode","schema:rangeIncludes":{"@id":"schema:Text"},"schema:domainIncludes":{"@id":"unece:LaboratoryObservationInstructions"},"rdfs:comment":"The code specifying a description of a laboratory observation instruction or a set of instructions."},{"@id":"unece:quarantineInstructionsDescriptionCode","@type":["rdf:Property","owl:DatatypeProperty"],"rdfs:label":"quarantineInstructionsDescriptionCode","schema:rangeIncludes":{"@id":"schema:Text"},"schema:domainIncludes":{"@id":"unece:QuarantineInstructions"},"rdfs:comment":"The code specifying the description of these quarantine instructions."},{"@id":"unece:rule","@type":["rdf:Property","owl:DatatypeProperty"],"rdfs:label":"rule","schema:rangeIncludes":{"@id":"schema:Text"},"schema:domainIncludes":{"@id":"unece:Requirement"},"rdfs:comment":"A rule, expressed as text, for this specified requirement."},{"@id":"unece:specifyingParty","@type":["rdf:Property","owl:ObjectProperty"],"rdfs:label":"specifyingParty","schema:rangeIncludes":{"@id":"unece:Party"},"schema:domainIncludes":{"@id":"unece:Requirement"},"rdfs:comment":""},{"@id":"unece:temperatureSettingInstructionsDescriptionCode","@type":["rdf:Property","owl:DatatypeProperty"],"rdfs:label":"temperatureSettingInstructionsDescriptionCode","schema:rangeIncludes":{"@id":"schema:Text"},"schema:domainIncludes":{"@id":"unece:TemperatureSettingInstructions"},"rdfs:comment":"The code specifying a description of these temperature setting instructions."},{"@id":"unece:quantificationTypeCode","@type":["rdf:Property","owl:DatatypeProperty"],"rdfs:label":"quantificationTypeCode","schema:rangeIncludes":{"@id":"schema:Text"},"schema:domainIncludes":{"@id":"unece:CalibratedMeasurement"},"rdfs:comment":"The code specifying a quantification type for this calibrated measurement, such as measured, calculated, or estimated."},{"@id":"unece:tolerancePercent","@type":["rdf:Property","owl:DatatypeProperty"],"rdfs:label":"tolerancePercent","schema:rangeIncludes":{"@id":"schema:Text"},"schema:domainIncludes":{"@id":"unece:CalibratedMeasurement"},"rdfs:comment":"The percent of tolerance of this calibrated measurement."},{"@id":"unece:officeAddress","@type":["rdf:Property","owl:ObjectProperty"],"rdfs:label":"officeAddress","schema:rangeIncludes":{"@id":"unece:Address"},"schema:domainIncludes":{"@id":"unece:LaboratoryObservationParty"},"rdfs:comment":"The location at which a particular trade related organization or person may be found or reached."},{"@id":"unece:personDefinedContact","@type":["rdf:Property","owl:ObjectProperty"],"rdfs:label":"personDefinedContact","schema:rangeIncludes":{"@id":"unece:LaboratoryObservationContact"},"schema:domainIncludes":{"@id":"unece:LaboratoryObservationParty"},"rdfs:comment":"The person defined as the contact for this laboratory observation party."},{"@id":"unece:thirdPartyIssuedId","@type":["rdf:Property","owl:DatatypeProperty"],"rdfs:label":"thirdPartyIssuedId","schema:rangeIncludes":{"@id":"schema:Text"},"schema:domainIncludes":[{"@id":"unece:LaboratoryObservationParty"},{"@id":"unece:Area"}],"rdfs:comment":"An alternate identifier issued by a third party for this laboratory observation party."},{"@id":"unece:thirdPartyIssuedIdentification","@type":["rdf:Property","owl:DatatypeProperty"],"rdfs:label":"thirdPartyIssuedIdentification","schema:rangeIncludes":{"@id":"schema:Text"},"schema:domainIncludes":{"@id":"unece:LaboratoryObservationParty"},"rdfs:comment":"A third party issued identifier, expressed as text, for this laboratory observation party."},{"@id":"unece:result","@type":["rdf:Property","owl:DatatypeProperty"],"rdfs:label":"result","schema:rangeIncludes":{"@id":"schema:Text"},"schema:domainIncludes":{"@id":"unece:TestSpecificationReport"},"rdfs:comment":"A result, expressed as text, reported in this certification test specification report."},{"@id":"unece:standardName","@type":["rdf:Property","owl:DatatypeProperty"],"rdfs:label":"standardName","schema:rangeIncludes":{"@id":"schema:Text"},"schema:domainIncludes":{"@id":"unece:TestSpecificationReport"},"rdfs:comment":"The name, expressed as text, of the standard applicable for this certification test specification report."},{"@id":"unece:testName","@type":["rdf:Property","owl:DatatypeProperty"],"rdfs:label":"testName","schema:rangeIncludes":{"@id":"schema:Text"},"schema:domainIncludes":{"@id":"unece:TestSpecificationReport"},"rdfs:comment":"A test name, expressed as text, for this certification test specification report."},{"@id":"unece:absolutePresenceVolumeMeasure","@type":["rdf:Property","owl:ObjectProperty"],"rdfs:label":"absolutePresenceVolumeMeasure","schema:rangeIncludes":{"@id":"unece:MeasureType"},"schema:domainIncludes":{"@id":"unece:GoodsCharacteristic"},"rdfs:comment":""},{"@id":"unece:absolutePresenceWeightMeasure","@type":["rdf:Property","owl:ObjectProperty"],"rdfs:label":"absolutePresenceWeightMeasure","schema:rangeIncludes":{"@id":"unece:MeasureType"},"schema:domainIncludes":{"@id":"unece:GoodsCharacteristic"},"rdfs:comment":""},{"@id":"unece:proportionalConstituentPercent","@type":["rdf:Property","owl:DatatypeProperty"],"rdfs:label":"proportionalConstituentPercent","schema:rangeIncludes":{"@id":"schema:Text"},"schema:domainIncludes":{"@id":"unece:GoodsCharacteristic"},"rdfs:comment":"The percentage presence of the material within the goods for this material goods characteristic."},{"@id":"unece:applicableQuantity","@type":["rdf:Property","owl:ObjectProperty"],"rdfs:label":"applicableQuantity","schema:rangeIncludes":{"@id":"unece:QuantityType"},"schema:domainIncludes":{"@id":"unece:SpecifiedMaterial"},"rdfs:comment":""},{"@id":"unece:applicableWasteMaterialRecoveryDisposalProcess","@type":["rdf:Property","owl:ObjectProperty"],"rdfs:label":"applicableWasteMaterialRecoveryDisposalProcess","schema:rangeIncludes":{"@id":"unece:WasteMaterialRecoveryDisposalProcess"},"schema:domainIncludes":{"@id":"unece:SpecifiedMaterial"},"rdfs:comment":"A waste material recovery disposal process applicable to this specified material."},{"@id":"unece:classificationId","@type":["rdf:Property","owl:DatatypeProperty"],"rdfs:label":"classificationId","schema:rangeIncludes":{"@id":"schema:Text"},"schema:domainIncludes":{"@id":"unece:SpecifiedMaterial"},"rdfs:comment":"An identifier of the classification of this specified material."},{"@id":"unece:transportInstructionsDescriptionCode","@type":["rdf:Property","owl:DatatypeProperty"],"rdfs:label":"transportInstructionsDescriptionCode","schema:rangeIncludes":{"@id":"schema:Text"},"schema:domainIncludes":{"@id":"unece:TransportInstructions"},"rdfs:comment":"The code specifying a description of these transport instructions."},{"@id":"unece:issuingParty","@type":["rdf:Property","owl:ObjectProperty"],"rdfs:label":"issuingParty","schema:rangeIncludes":{"@id":"unece:Party"},"schema:domainIncludes":{"@id":"unece:Seal"},"rdfs:comment":""},{"@id":"unece:logisticsSealTypeCode","@type":["rdf:Property","owl:DatatypeProperty"],"rdfs:label":"logisticsSealTypeCode","schema:rangeIncludes":{"@id":"schema:Text"},"schema:domainIncludes":{"@id":"unece:Seal"},"rdfs:comment":"The code specifying the type of logistics seal."},{"@id":"unece:logisticsSealingPartyRoleCode","@type":["rdf:Property","owl:DatatypeProperty"],"rdfs:label":"logisticsSealingPartyRoleCode","schema:rangeIncludes":{"@id":"unece:SealingPartyRoleCodeList"},"schema:domainIncludes":{"@id":"unece:Seal"},"rdfs:comment":"The code specifying the role of the party responsible for the sealing of this logistics seal."},{"@id":"unece:maximumId","@type":["rdf:Property","owl:DatatypeProperty"],"rdfs:label":"maximumId","schema:rangeIncludes":{"@id":"schema:Text"},"schema:domainIncludes":{"@id":"unece:Seal"},"rdfs:comment":"The maximum unique identifier used for these logistics seals."},{"@id":"unece:sealConditionCode","@type":["rdf:Property","owl:DatatypeProperty"],"rdfs:label":"sealConditionCode","schema:rangeIncludes":{"@id":"unece:SealConditionCodeList"},"schema:domainIncludes":{"@id":"unece:Seal"},"rdfs:comment":"A code specifying a condition of this logistics seal."},{"@id":"unece:lowerLimitActualMeasure","@type":["rdf:Property","owl:ObjectProperty"],"rdfs:label":"lowerLimitActualMeasure","schema:rangeIncludes":{"@id":"unece:MeasureType"},"schema:domainIncludes":{"@id":"unece:IngredientRangeMeasurement"},"rdfs:comment":""},{"@id":"unece:lowerLimitComparisonOperatorCode","@type":["rdf:Property","owl:DatatypeProperty"],"rdfs:label":"lowerLimitComparisonOperatorCode","schema:rangeIncludes":{"@id":"schema:Text"},"schema:domainIncludes":{"@id":"unece:IngredientRangeMeasurement"},"rdfs:comment":"The code specifying the comparison operator for the lower limit of this ingredient range measurement."},{"@id":"unece:lowerLimitPressureConditionMeasure","@type":["rdf:Property","owl:ObjectProperty"],"rdfs:label":"lowerLimitPressureConditionMeasure","schema:rangeIncludes":{"@id":"unece:MeasureType"},"schema:domainIncludes":{"@id":"unece:IngredientRangeMeasurement"},"rdfs:comment":""},{"@id":"unece:upperLimitActualMeasure","@type":["rdf:Property","owl:ObjectProperty"],"rdfs:label":"upperLimitActualMeasure","schema:rangeIncludes":{"@id":"unece:MeasureType"},"schema:domainIncludes":{"@id":"unece:IngredientRangeMeasurement"},"rdfs:comment":""},{"@id":"unece:upperLimitComparisonOperatorCode","@type":["rdf:Property","owl:DatatypeProperty"],"rdfs:label":"upperLimitComparisonOperatorCode","schema:rangeIncludes":{"@id":"schema:Text"},"schema:domainIncludes":{"@id":"unece:IngredientRangeMeasurement"},"rdfs:comment":"The code specifying the comparison operator for the upper limit of this ingredient range measurement."},{"@id":"unece:upperLimitPressureConditionMeasure","@type":["rdf:Property","owl:ObjectProperty"],"rdfs:label":"upperLimitPressureConditionMeasure","schema:rangeIncludes":{"@id":"unece:MeasureType"},"schema:domainIncludes":{"@id":"unece:IngredientRangeMeasurement"},"rdfs:comment":""},{"@id":"unece:applicableProductionWasteRecoveryDisposalProcess","@type":["rdf:Property","owl:ObjectProperty"],"rdfs:label":"applicableProductionWasteRecoveryDisposalProcess","schema:rangeIncludes":{"@id":"unece:ProductionWasteRecoveryDisposalProcess"},"schema:domainIncludes":{"@id":"unece:ProductionWasteMaterial"},"rdfs:comment":"A production waste recovery disposal process applicable to this production waste material."},{"@id":"unece:includedProductionWasteMaterialComponent","@type":["rdf:Property","owl:ObjectProperty"],"rdfs:label":"includedProductionWasteMaterialComponent","schema:rangeIncludes":{"@id":"unece:ProductionWasteMaterialComponent"},"schema:domainIncludes":{"@id":"unece:ProductionWasteMaterial"},"rdfs:comment":"A production waste material component included in this production waste material."},{"@id":"unece:accompanyingAnimal","@type":["rdf:Property","owl:ObjectProperty"],"rdfs:label":"accompanyingAnimal","schema:rangeIncludes":{"@id":"unece:PetAnimal"},"schema:domainIncludes":{"@id":"unece:GuestPerson"},"rdfs:comment":"A pet animal accompanying this guest person."},{"@id":"unece:carriedCertificate","@type":["rdf:Property","owl:ObjectProperty"],"rdfs:label":"carriedCertificate","schema:rangeIncludes":{"@id":"unece:SpecifiedCertificate"},"schema:domainIncludes":{"@id":"unece:GuestPerson"},"rdfs:comment":"A document issued by a government, public organization or association to certify a property of a person, entity, process or object."},{"@id":"unece:durationUnitAgeMeasure","@type":["rdf:Property","owl:ObjectProperty"],"rdfs:label":"durationUnitAgeMeasure","schema:rangeIncludes":{"@id":"unece:DurationUnitMeasureType"},"schema:domainIncludes":{"@id":"unece:GuestPerson"},"rdfs:comment":""},{"@id":"unece:notifiedAllergy","@type":["rdf:Property","owl:ObjectProperty"],"rdfs:label":"notifiedAllergy","schema:rangeIncludes":{"@id":"unece:Allergy"},"schema:domainIncludes":{"@id":"unece:GuestPerson"},"rdfs:comment":"An allergy notified for this guest person."},{"@id":"unece:notifiedDisability","@type":["rdf:Property","owl:ObjectProperty"],"rdfs:label":"notifiedDisability","schema:rangeIncludes":{"@id":"unece:Disability"},"schema:domainIncludes":{"@id":"unece:GuestPerson"},"rdfs:comment":"A disability notified for this guest person."},{"@id":"unece:notifiedFoodChoice","@type":["rdf:Property","owl:ObjectProperty"],"rdfs:label":"notifiedFoodChoice","schema:rangeIncludes":{"@id":"unece:FoodChoice"},"schema:domainIncludes":{"@id":"unece:GuestPerson"},"rdfs:comment":"A food choice notified for this guest person."},{"@id":"unece:notifiedGuestArrival","@type":["rdf:Property","owl:ObjectProperty"],"rdfs:label":"notifiedGuestArrival","schema:rangeIncludes":{"@id":"unece:GuestArrival"},"schema:domainIncludes":{"@id":"unece:GuestPerson"},"rdfs:comment":"An arrival notified for this guest person."},{"@id":"unece:notifiedHealthIndication","@type":["rdf:Property","owl:ObjectProperty"],"rdfs:label":"notifiedHealthIndication","schema:rangeIncludes":{"@id":"unece:GuestHealthIndication"},"schema:domainIncludes":{"@id":"unece:GuestPerson"},"rdfs:comment":"A health indication notified for this guest person."},{"@id":"unece:notifiedPreference","@type":["rdf:Property","owl:ObjectProperty"],"rdfs:label":"notifiedPreference","schema:rangeIncludes":{"@id":"unece:Preference"},"schema:domainIncludes":{"@id":"unece:GuestPerson"},"rdfs:comment":"An experience item preference notified for this guest person."},{"@id":"unece:notifiedProtectionMeans","@type":["rdf:Property","owl:ObjectProperty"],"rdfs:label":"notifiedProtectionMeans","schema:rangeIncludes":{"@id":"unece:ProtectionMeans"},"schema:domainIncludes":{"@id":"unece:GuestPerson"},"rdfs:comment":"A way to protect something, such as human beings, animals or environment, from getting infected or becoming ill."},{"@id":"unece:raisedQuery","@type":["rdf:Property","owl:ObjectProperty"],"rdfs:label":"raisedQuery","schema:rangeIncludes":{"@id":"unece:SpecialQuery"},"schema:domainIncludes":{"@id":"unece:GuestPerson"},"rdfs:comment":"A special question or request for information."},{"@id":"unece:specifiedCarriedEquipment","@type":["rdf:Property","owl:ObjectProperty"],"rdfs:label":"specifiedCarriedEquipment","schema:rangeIncludes":{"@id":"unece:CarriedEquipment"},"schema:domainIncludes":{"@id":"unece:GuestPerson"},"rdfs:comment":"Carried equipment specified for this guest person."},{"@id":"unece:titleCode","@type":["rdf:Property","owl:DatatypeProperty"],"rdfs:label":"titleCode","schema:rangeIncludes":{"@id":"schema:Text"},"schema:domainIncludes":{"@id":"unece:GuestPerson"},"rdfs:comment":"The code specifying the title of this guest person."},{"@id":"unece:travelInsuranceCertificate","@type":["rdf:Property","owl:ObjectProperty"],"rdfs:label":"travelInsuranceCertificate","schema:rangeIncludes":{"@id":"unece:SpecifiedCertificate"},"schema:domainIncludes":{"@id":"unece:GuestPerson"},"rdfs:comment":"A document issued by a government, public organization or association to certify a property of a person, entity, process or object."},{"@id":"unece:allowedIndicator","@type":["rdf:Property","owl:DatatypeProperty"],"rdfs:label":"allowedIndicator","schema:rangeIncludes":{"@id":"schema:Boolean"},"schema:domainIncludes":{"@id":"unece:PetAnimal"},"rdfs:comment":"The indication of whether or not this pet animal is allowed."},{"@id":"unece:applicableQuantityUnitTypeCode","@type":["rdf:Property","owl:DatatypeProperty"],"rdfs:label":"applicableQuantityUnitTypeCode","schema:rangeIncludes":{"@id":"schema:Text"},"schema:domainIncludes":[{"@id":"unece:ExperienceItem"},{"@id":"unece:ExperienceProduct"}],"rdfs:comment":"The code specifying the type of quantity unit applicable for this experience product."},{"@id":"unece:availablePeriod","@type":["rdf:Property","owl:ObjectProperty"],"rdfs:label":"availablePeriod","schema:rangeIncludes":{"@id":"unece:SpecifiedPeriod"},"schema:domainIncludes":{"@id":"unece:ExperienceItem"},"rdfs:comment":"A specified period of time."},{"@id":"unece:availableProduct","@type":["rdf:Property","owl:ObjectProperty"],"rdfs:label":"availableProduct","schema:rangeIncludes":{"@id":"unece:ExperienceProduct"},"schema:domainIncludes":{"@id":"unece:ExperienceItem"},"rdfs:comment":"An available product for this specified experience item."},{"@id":"unece:availableUnitQuantity","@type":["rdf:Property","owl:ObjectProperty"],"rdfs:label":"availableUnitQuantity","schema:rangeIncludes":{"@id":"unece:QuantityType"},"schema:domainIncludes":{"@id":"unece:ExperienceItem"},"rdfs:comment":""},{"@id":"unece:calculatedPrice","@type":["rdf:Property","owl:ObjectProperty"],"rdfs:label":"calculatedPrice","schema:rangeIncludes":{"@id":"unece:TradePrice"},"schema:domainIncludes":[{"@id":"unece:ExperienceItem"},{"@id":"unece:ExperienceProduct"},{"@id":"unece:ExperienceEvent"}],"rdfs:comment":"A sum of money for which something is or may be bought or sold for trade purposes."},{"@id":"unece:destination","@type":["rdf:Property","owl:DatatypeProperty"],"rdfs:label":"destination","schema:rangeIncludes":{"@id":"schema:Text"},"schema:domainIncludes":{"@id":"unece:ExperienceItem"},"rdfs:comment":"A destination, expressed as text, for this specified experience item."},{"@id":"unece:guestSpecialCareIndicator","@type":["rdf:Property","owl:DatatypeProperty"],"rdfs:label":"guestSpecialCareIndicator","schema:rangeIncludes":{"@id":"schema:Boolean"},"schema:domainIncludes":{"@id":"unece:ExperienceItem"},"rdfs:comment":"The indication of whether or not guest special care is applicable for this specified experience item."},{"@id":"unece:indemnityClause","@type":["rdf:Property","owl:DatatypeProperty"],"rdfs:label":"indemnityClause","schema:rangeIncludes":{"@id":"schema:Text"},"schema:domainIncludes":[{"@id":"unece:ExperienceItem"},{"@id":"unece:ExperienceProduct"},{"@id":"unece:ExperienceEvent"}],"rdfs:comment":"An indemnity clause, expressed as text, for this experience event."},{"@id":"unece:lowerPriceLimitAmount","@type":["rdf:Property","owl:ObjectProperty"],"rdfs:label":"lowerPriceLimitAmount","schema:rangeIncludes":{"@id":"unece:AmountType"},"schema:domainIncludes":{"@id":"unece:ExperienceItem"},"rdfs:comment":""},{"@id":"unece:maximumGuestQuantity","@type":["rdf:Property","owl:ObjectProperty"],"rdfs:label":"maximumGuestQuantity","schema:rangeIncludes":{"@id":"unece:QuantityType"},"schema:domainIncludes":{"@id":"unece:ExperienceItem"},"rdfs:comment":""},{"@id":"unece:minimumGuestQuantity","@type":["rdf:Property","owl:ObjectProperty"],"rdfs:label":"minimumGuestQuantity","schema:rangeIncludes":{"@id":"unece:QuantityType"},"schema:domainIncludes":{"@id":"unece:ExperienceItem"},"rdfs:comment":""},{"@id":"unece:reservationGuarantee","@type":["rdf:Property","owl:DatatypeProperty"],"rdfs:label":"reservationGuarantee","schema:rangeIncludes":{"@id":"schema:Text"},"schema:domainIncludes":[{"@id":"unece:ExperienceItem"},{"@id":"unece:ExperienceProduct"},{"@id":"unece:ExperienceEvent"}],"rdfs:comment":"A reservation guarantee, expressed as text, for this experience event."},{"@id":"unece:theme","@type":["rdf:Property","owl:DatatypeProperty"],"rdfs:label":"theme","schema:rangeIncludes":{"@id":"schema:Text"},"schema:domainIncludes":[{"@id":"unece:ExperienceItem"},{"@id":"unece:ExperienceProduct"}],"rdfs:comment":"A theme, expressed as text, for this experience product."},{"@id":"unece:themeTypeCode","@type":["rdf:Property","owl:DatatypeProperty"],"rdfs:label":"themeTypeCode","schema:rangeIncludes":{"@id":"schema:Text"},"schema:domainIncludes":[{"@id":"unece:ExperienceItem"},{"@id":"unece:ExperienceProduct"}],"rdfs:comment":"The code specifying the type of theme for this experience product."},{"@id":"unece:upperPriceLimitAmount","@type":["rdf:Property","owl:ObjectProperty"],"rdfs:label":"upperPriceLimitAmount","schema:rangeIncludes":{"@id":"unece:AmountType"},"schema:domainIncludes":{"@id":"unece:ExperienceItem"},"rdfs:comment":""},{"@id":"unece:visitingPeriod","@type":["rdf:Property","owl:ObjectProperty"],"rdfs:label":"visitingPeriod","schema:rangeIncludes":{"@id":"unece:SpecifiedPeriod"},"schema:domainIncludes":{"@id":"unece:ExperienceItem"},"rdfs:comment":"A specified period of time."},{"@id":"unece:certifiedPersonArrangementIndicator","@type":["rdf:Property","owl:DatatypeProperty"],"rdfs:label":"certifiedPersonArrangementIndicator","schema:rangeIncludes":{"@id":"schema:Boolean"},"schema:domainIncludes":{"@id":"unece:ExperienceProduct"},"rdfs:comment":"The indication of whether or not a certified person arrangement is made for this experience product."},{"@id":"unece:distinctiveFeature","@type":["rdf:Property","owl:ObjectProperty"],"rdfs:label":"distinctiveFeature","schema:rangeIncludes":{"@id":"unece:SpecifiedFeature"},"schema:domainIncludes":[{"@id":"unece:ExperienceProduct"},{"@id":"unece:ExperienceEvent"}],"rdfs:comment":"A distinctive or characteristic part of something."},{"@id":"unece:includedEvent","@type":["rdf:Property","owl:ObjectProperty"],"rdfs:label":"includedEvent","schema:rangeIncludes":{"@id":"unece:ExperienceEvent"},"schema:domainIncludes":{"@id":"unece:ExperienceProduct"},"rdfs:comment":"An event included within this experience product."},{"@id":"unece:maximumUnitQuantity","@type":["rdf:Property","owl:ObjectProperty"],"rdfs:label":"maximumUnitQuantity","schema:rangeIncludes":{"@id":"unece:QuantityType"},"schema:domainIncludes":{"@id":"unece:ExperienceProduct"},"rdfs:comment":""},{"@id":"unece:minimumUnitQuantity","@type":["rdf:Property","owl:ObjectProperty"],"rdfs:label":"minimumUnitQuantity","schema:rangeIncludes":{"@id":"unece:QuantityType"},"schema:domainIncludes":{"@id":"unece:ExperienceProduct"},"rdfs:comment":""},{"@id":"unece:operationalPeriod","@type":["rdf:Property","owl:ObjectProperty"],"rdfs:label":"operationalPeriod","schema:rangeIncludes":{"@id":"unece:SpecifiedPeriod"},"schema:domainIncludes":[{"@id":"unece:ExperienceProduct"},{"@id":"unece:ExperienceEvent"}],"rdfs:comment":"A specified period of time."},{"@id":"unece:optionalProduct","@type":["rdf:Property","owl:ObjectProperty"],"rdfs:label":"optionalProduct","schema:rangeIncludes":{"@id":"unece:ExperienceProduct"},"schema:domainIncludes":{"@id":"unece:ExperienceProduct"},"rdfs:comment":"An optional product for this experience product."},{"@id":"unece:providedCertificate","@type":["rdf:Property","owl:ObjectProperty"],"rdfs:label":"providedCertificate","schema:rangeIncludes":{"@id":"unece:SpecifiedCertificate"},"schema:domainIncludes":[{"@id":"unece:ExperienceProduct"},{"@id":"unece:ExperienceEvent"}],"rdfs:comment":"A document issued by a government, public organization or association to certify a property of a person, entity, process or object."},{"@id":"unece:providedRequirement","@type":["rdf:Property","owl:ObjectProperty"],"rdfs:label":"providedRequirement","schema:rangeIncludes":{"@id":"unece:Requirement"},"schema:domainIncludes":[{"@id":"unece:ExperienceProduct"},{"@id":"unece:ExperienceEvent"}],"rdfs:comment":"Common conditions contained in a contract or agreement applicable between trading partners."},{"@id":"unece:requiredReservationGuaranteeIndicator","@type":["rdf:Property","owl:DatatypeProperty"],"rdfs:label":"requiredReservationGuaranteeIndicator","schema:rangeIncludes":{"@id":"schema:Boolean"},"schema:domainIncludes":{"@id":"unece:ExperienceProduct"},"rdfs:comment":"The indication of whether or not this experience product requires a reservation guarantee."},{"@id":"unece:requiredUsageCondition","@type":["rdf:Property","owl:ObjectProperty"],"rdfs:label":"requiredUsageCondition","schema:rangeIncludes":{"@id":"unece:UsageCondition"},"schema:domainIncludes":[{"@id":"unece:ExperienceProduct"},{"@id":"unece:ExperienceEvent"}],"rdfs:comment":"The particular state of something, affected by use, that should be respected."},{"@id":"unece:basicObjective","@type":["rdf:Property","owl:DatatypeProperty"],"rdfs:label":"basicObjective","schema:rangeIncludes":{"@id":"schema:Text"},"schema:domainIncludes":{"@id":"unece:ExperienceEvent"},"rdfs:comment":"A basic objective, expressed as text, for this experience event."},{"@id":"unece:breakUpDateTime","@type":["rdf:Property","owl:DatatypeProperty"],"rdfs:label":"breakUpDateTime","schema:rangeIncludes":{"@id":"schema:Text"},"schema:domainIncludes":[{"@id":"unece:ExperienceEvent"},{"@id":"unece:CropProduceBatch"},{"@id":"unece:AnimalBatch"}],"rdfs:comment":"The break up date, time, date time, or other date time value for this experience event."},{"@id":"unece:choiceAllowedIndicator","@type":["rdf:Property","owl:DatatypeProperty"],"rdfs:label":"choiceAllowedIndicator","schema:rangeIncludes":{"@id":"schema:Boolean"},"schema:domainIncludes":{"@id":"unece:ExperienceEvent"},"rdfs:comment":"The indication of whether or not a choice is allowed for this experience event."},{"@id":"unece:dateSequenceNumeric","@type":["rdf:Property","owl:DatatypeProperty"],"rdfs:label":"dateSequenceNumeric","schema:rangeIncludes":{"@id":"schema:Text"},"schema:domainIncludes":{"@id":"unece:ExperienceEvent"},"rdfs:comment":"The date sequence number for this experience event."},{"@id":"unece:meetingDateTime","@type":["rdf:Property","owl:DatatypeProperty"],"rdfs:label":"meetingDateTime","schema:rangeIncludes":{"@id":"schema:DateTime"},"schema:domainIncludes":{"@id":"unece:ExperienceEvent"},"rdfs:comment":"The meeting date, time, date time, or other date time value for this experience event."},{"@id":"unece:reservationRequiredIndicator","@type":["rdf:Property","owl:DatatypeProperty"],"rdfs:label":"reservationRequiredIndicator","schema:rangeIncludes":{"@id":"schema:Boolean"},"schema:domainIncludes":{"@id":"unece:ExperienceEvent"},"rdfs:comment":"The indication of whether or not a reservation is required for this experience event."},{"@id":"unece:architecturalStyle","@type":["rdf:Property","owl:DatatypeProperty"],"rdfs:label":"architecturalStyle","schema:rangeIncludes":{"@id":"schema:Text"},"schema:domainIncludes":{"@id":"unece:ExperienceFacility"},"rdfs:comment":"An architectural style, expressed as text, of this experience facility."},{"@id":"unece:completionDateTime","@type":["rdf:Property","owl:DatatypeProperty"],"rdfs:label":"completionDateTime","schema:rangeIncludes":{"@id":"schema:Text"},"schema:domainIncludes":{"@id":"unece:ExperienceFacility"},"rdfs:comment":"The date of the completion of this experience facility."},{"@id":"unece:facilityType","@type":["rdf:Property","owl:DatatypeProperty"],"rdfs:label":"facilityType","schema:rangeIncludes":{"@id":"schema:Text"},"schema:domainIncludes":{"@id":"unece:ExperienceFacility"},"rdfs:comment":"A type, expressed as text, of this experience facility."},{"@id":"unece:physicalSpecifiedLocation","@type":["rdf:Property","owl:ObjectProperty"],"rdfs:label":"physicalSpecifiedLocation","schema:rangeIncludes":{"@id":"unece:SpecifiedLocation"},"schema:domainIncludes":{"@id":"unece:ExperienceFacility"},"rdfs:comment":"A specified physical location or place."},{"@id":"unece:usedSource","@type":["rdf:Property","owl:ObjectProperty"],"rdfs:label":"usedSource","schema:rangeIncludes":{"@id":"unece:Source"},"schema:domainIncludes":{"@id":"unece:ExperienceFacility"},"rdfs:comment":"A place from which water originates, such as a hot spring or lake that provides water to public drinking water supplies and private wells."},{"@id":"unece:carrierId","@type":["rdf:Property","owl:DatatypeProperty"],"rdfs:label":"carrierId","schema:rangeIncludes":{"@id":"schema:Text"},"schema:domainIncludes":{"@id":"unece:GuestArrival"},"rdfs:comment":"The identifier of the carrier for this specified guest arrival."},{"@id":"unece:carrierName","@type":["rdf:Property","owl:DatatypeProperty"],"rdfs:label":"carrierName","schema:rangeIncludes":{"@id":"schema:Text"},"schema:domainIncludes":{"@id":"unece:GuestArrival"},"rdfs:comment":"A carrier's name, expressed as text, related to this specified guest arrival."},{"@id":"unece:expectedDateTime","@type":["rdf:Property","owl:DatatypeProperty"],"rdfs:label":"expectedDateTime","schema:rangeIncludes":{"@id":"schema:DateTime"},"schema:domainIncludes":{"@id":"unece:GuestArrival"},"rdfs:comment":"The date, time, date time, or other date time value when this specified guest arrival is expected."},{"@id":"unece:transportModeCode","@type":["rdf:Property","owl:DatatypeProperty"],"rdfs:label":"transportModeCode","schema:rangeIncludes":{"@id":"schema:Text"},"schema:domainIncludes":[{"@id":"unece:GuestArrival"},{"@id":"unece:TransportMovement"}],"rdfs:comment":"The code specifying the mode, such as by air, sea, rail, road or inland waterway, for this logistics transport movement."},{"@id":"unece:specificationNote","@type":["rdf:Property","owl:ObjectProperty"],"rdfs:label":"specificationNote","schema:rangeIncludes":{"@id":"unece:SpecifiedNote"},"schema:domainIncludes":{"@id":"unece:CarriedEquipment"},"rdfs:comment":"A specified textual or coded description, such as a remark or additional information."},{"@id":"unece:registeredDateTime","@type":["rdf:Property","owl:DatatypeProperty"],"rdfs:label":"registeredDateTime","schema:rangeIncludes":{"@id":"schema:DateTime"},"schema:domainIncludes":{"@id":"unece:Disability"},"rdfs:comment":"The date, time, date time, or other date time value when this guest disability has been registered."},{"@id":"unece:requiredSupportingDevice","@type":["rdf:Property","owl:DatatypeProperty"],"rdfs:label":"requiredSupportingDevice","schema:rangeIncludes":{"@id":"schema:Text"},"schema:domainIncludes":{"@id":"unece:Disability"},"rdfs:comment":"A supporting device, expressed as text, for this required guest disability."},{"@id":"unece:onboardQuantity","@type":["rdf:Property","owl:ObjectProperty"],"rdfs:label":"onboardQuantity","schema:rangeIncludes":{"@id":"unece:QuantityType"},"schema:domainIncludes":[{"@id":"unece:PersonalEffects"},{"@id":"unece:StoresItemInventory"}],"rdfs:comment":""},{"@id":"unece:dislikedItem","@type":["rdf:Property","owl:DatatypeProperty"],"rdfs:label":"dislikedItem","schema:rangeIncludes":{"@id":"schema:Text"},"schema:domainIncludes":{"@id":"unece:Preference"},"rdfs:comment":"A disliked item, expressed as text, for this experience item preference."},{"@id":"unece:preferredItem","@type":["rdf:Property","owl:DatatypeProperty"],"rdfs:label":"preferredItem","schema:rangeIncludes":{"@id":"schema:Text"},"schema:domainIncludes":{"@id":"unece:Preference"},"rdfs:comment":"A preferred item, expressed as text, for this experience item preference."},{"@id":"unece:priorityRankingNumeric","@type":["rdf:Property","owl:DatatypeProperty"],"rdfs:label":"priorityRankingNumeric","schema:rangeIncludes":{"@id":"schema:Text"},"schema:domainIncludes":{"@id":"unece:Preference"},"rdfs:comment":"The priority ranking number for this experience item preference."},{"@id":"unece:actualEndDateTime","@type":["rdf:Property","owl:DatatypeProperty"],"rdfs:label":"actualEndDateTime","schema:rangeIncludes":{"@id":"schema:Text"},"schema:domainIncludes":{"@id":"unece:AgriculturalProcess"},"rdfs:comment":"The date, time, date time or other date time value of the actual end for the crop production in this agricultural process."},{"@id":"unece:actualStartDateTime","@type":["rdf:Property","owl:DatatypeProperty"],"rdfs:label":"actualStartDateTime","schema:rangeIncludes":{"@id":"schema:Text"},"schema:domainIncludes":{"@id":"unece:AgriculturalProcess"},"rdfs:comment":"The date, time, date time or other date time value for the actual start of the crop production in this agricultural process."},{"@id":"unece:earliestStartDateTime","@type":["rdf:Property","owl:DatatypeProperty"],"rdfs:label":"earliestStartDateTime","schema:rangeIncludes":{"@id":"schema:Text"},"schema:domainIncludes":{"@id":"unece:AgriculturalProcess"},"rdfs:comment":"The date, time, date time or other date time value for the earliest start of the crop production in this agricultural process."},{"@id":"unece:harvestedBatch","@type":["rdf:Property","owl:ObjectProperty"],"rdfs:label":"harvestedBatch","schema:rangeIncludes":{"@id":"unece:CropProduceBatch"},"schema:domainIncludes":{"@id":"unece:AgriculturalProcess"},"rdfs:comment":"A crop produce batch harvested in the crop production for this agricultural process."},{"@id":"unece:latestEndDateTime","@type":["rdf:Property","owl:DatatypeProperty"],"rdfs:label":"latestEndDateTime","schema:rangeIncludes":{"@id":"schema:Text"},"schema:domainIncludes":{"@id":"unece:AgriculturalProcess"},"rdfs:comment":"The date, time, date time or other date time value of the latest end for the crop production in this agricultural process."},{"@id":"unece:specifiedFieldCrop","@type":["rdf:Property","owl:ObjectProperty"],"rdfs:label":"specifiedFieldCrop","schema:rangeIncludes":{"@id":"unece:FieldCrop"},"schema:domainIncludes":{"@id":"unece:AgriculturalProcess"},"rdfs:comment":"A field crop specified for this crop production agricultural process."},{"@id":"unece:applicableAgriculturalCharacteristic","@type":["rdf:Property","owl:ObjectProperty"],"rdfs:label":"applicableAgriculturalCharacteristic","schema:rangeIncludes":{"@id":"unece:AgriculturalCharacteristic"},"schema:domainIncludes":{"@id":"unece:Area"},"rdfs:comment":"An agricultural characteristic applicable to this agricultural zone area."},{"@id":"unece:designatedSection","@type":["rdf:Property","owl:DatatypeProperty"],"rdfs:label":"designatedSection","schema:rangeIncludes":{"@id":"schema:Text"},"schema:domainIncludes":{"@id":"unece:Area"},"rdfs:comment":"The designated section, expressed as text, of this agricultural zone area."},{"@id":"unece:harvestedProduce","@type":["rdf:Property","owl:ObjectProperty"],"rdfs:label":"harvestedProduce","schema:rangeIncludes":{"@id":"unece:Produce"},"schema:domainIncludes":[{"@id":"unece:Area"},{"@id":"unece:FieldCrop"}],"rdfs:comment":"Crop produce harvested from this agricultural zone area."},{"@id":"unece:multiSurfaceTypeCode","@type":["rdf:Property","owl:DatatypeProperty"],"rdfs:label":"multiSurfaceTypeCode","schema:rangeIncludes":{"@id":"schema:Text"},"schema:domainIncludes":{"@id":"unece:Area"},"rdfs:comment":"The code specifying the multi-surface type for this agricultural zone area."},{"@id":"unece:specifiedPlot","@type":["rdf:Property","owl:ObjectProperty"],"rdfs:label":"specifiedPlot","schema:rangeIncludes":{"@id":"unece:Plot"},"schema:domainIncludes":[{"@id":"unece:Area"},{"@id":"unece:AgriculturalApplication"}],"rdfs:comment":"A crop plot specified for this agricultural application."},{"@id":"unece:subordinateArea","@type":["rdf:Property","owl:ObjectProperty"],"rdfs:label":"subordinateArea","schema:rangeIncludes":{"@id":"unece:Area"},"schema:domainIncludes":{"@id":"unece:Area"},"rdfs:comment":"An agricultural zone area subordinate to this agricultural zone area."},{"@id":"unece:applicableAgriculturalProcess","@type":["rdf:Property","owl:ObjectProperty"],"rdfs:label":"applicableAgriculturalProcess","schema:rangeIncludes":{"@id":"unece:AgriculturalProcess"},"schema:domainIncludes":[{"@id":"unece:FieldCrop"},{"@id":"unece:Plot"}],"rdfs:comment":"An agricultural process crop production applicable for this field crop."},{"@id":"unece:cultivationContainerCode","@type":["rdf:Property","owl:DatatypeProperty"],"rdfs:label":"cultivationContainerCode","schema:rangeIncludes":{"@id":"schema:Text"},"schema:domainIncludes":{"@id":"unece:FieldCrop"},"rdfs:comment":"The code specifying the type of cultivation container, such as a pot or an iron cabinet, for this field crop."},{"@id":"unece:cultivationCoverageCode","@type":["rdf:Property","owl:DatatypeProperty"],"rdfs:label":"cultivationCoverageCode","schema:rangeIncludes":{"@id":"schema:Text"},"schema:domainIncludes":{"@id":"unece:FieldCrop"},"rdfs:comment":"A code specifying a type of cultivation coverage, such as glass, for this field crop."},{"@id":"unece:cultivationMediumCode","@type":["rdf:Property","owl:DatatypeProperty"],"rdfs:label":"cultivationMediumCode","schema:rangeIncludes":{"@id":"schema:Text"},"schema:domainIncludes":{"@id":"unece:FieldCrop"},"rdfs:comment":"The code specifying the type of cultivation medium, such as substrate, for this field crop."},{"@id":"unece:cultivationTypeCode","@type":["rdf:Property","owl:DatatypeProperty"],"rdfs:label":"cultivationTypeCode","schema:rangeIncludes":{"@id":"schema:Text"},"schema:domainIncludes":{"@id":"unece:FieldCrop"},"rdfs:comment":"The code specifying the type of cultivation for this field crop."},{"@id":"unece:grownPlot","@type":["rdf:Property","owl:ObjectProperty"],"rdfs:label":"grownPlot","schema:rangeIncludes":{"@id":"unece:Plot"},"schema:domainIncludes":{"@id":"unece:FieldCrop"},"rdfs:comment":"The plot where this field crop is grown."},{"@id":"unece:harvestDateTime","@type":["rdf:Property","owl:DatatypeProperty"],"rdfs:label":"harvestDateTime","schema:rangeIncludes":{"@id":"schema:Text"},"schema:domainIncludes":{"@id":"unece:FieldCrop"},"rdfs:comment":"The date, time, date time, or other date time value for the harvest of this field crop."},{"@id":"unece:plantingReasonCode","@type":["rdf:Property","owl:DatatypeProperty"],"rdfs:label":"plantingReasonCode","schema:rangeIncludes":{"@id":"schema:Text"},"schema:domainIncludes":{"@id":"unece:FieldCrop"},"rdfs:comment":"A code specifying a reason for planting this field crop."},{"@id":"unece:productionEnvironmentCode","@type":["rdf:Property","owl:DatatypeProperty"],"rdfs:label":"productionEnvironmentCode","schema:rangeIncludes":{"@id":"schema:Text"},"schema:domainIncludes":{"@id":"unece:FieldCrop"},"rdfs:comment":"The code specifying the production environment for this field crop."},{"@id":"unece:productionPeriodCode","@type":["rdf:Property","owl:DatatypeProperty"],"rdfs:label":"productionPeriodCode","schema:rangeIncludes":{"@id":"schema:Text"},"schema:domainIncludes":{"@id":"unece:FieldCrop"},"rdfs:comment":"The code specifying the production period for this field crop."},{"@id":"unece:propagationMaterialIndicator","@type":["rdf:Property","owl:DatatypeProperty"],"rdfs:label":"propagationMaterialIndicator","schema:rangeIncludes":{"@id":"schema:Boolean"},"schema:domainIncludes":{"@id":"unece:FieldCrop"},"rdfs:comment":"The indication of whether or not a field crop is to be used as propagation material."},{"@id":"unece:sowingPeriodCode","@type":["rdf:Property","owl:DatatypeProperty"],"rdfs:label":"sowingPeriodCode","schema:rangeIncludes":{"@id":"schema:Text"},"schema:domainIncludes":{"@id":"unece:FieldCrop"},"rdfs:comment":"The code specifying the sowing period for this field crop, such as spring or winter."},{"@id":"unece:specifiedCropMixtureConstituent","@type":["rdf:Property","owl:ObjectProperty"],"rdfs:label":"specifiedCropMixtureConstituent","schema:rangeIncludes":{"@id":"unece:CropMixtureConstituent"},"schema:domainIncludes":{"@id":"unece:FieldCrop"},"rdfs:comment":"A field crop mixture constituent specified for this field crop."},{"@id":"unece:areaMeasure","@type":["rdf:Property","owl:ObjectProperty"],"rdfs:label":"areaMeasure","schema:rangeIncludes":{"@id":"unece:MeasureType"},"schema:domainIncludes":{"@id":"unece:Plot"},"rdfs:comment":""},{"@id":"unece:grownCrop","@type":["rdf:Property","owl:ObjectProperty"],"rdfs:label":"grownCrop","schema:rangeIncludes":{"@id":"unece:FieldCrop"},"schema:domainIncludes":{"@id":"unece:Plot"},"rdfs:comment":"A field crop grown on this crop plot."},{"@id":"unece:regulatoryOrganicIndicator","@type":["rdf:Property","owl:DatatypeProperty"],"rdfs:label":"regulatoryOrganicIndicator","schema:rangeIncludes":{"@id":"schema:Boolean"},"schema:domainIncludes":{"@id":"unece:Plot"},"rdfs:comment":"The indication of whether or not this crop plot is certified as regulatory organic."},{"@id":"unece:regulatorySoilTypeCode","@type":["rdf:Property","owl:DatatypeProperty"],"rdfs:label":"regulatorySoilTypeCode","schema:rangeIncludes":{"@id":"schema:Text"},"schema:domainIncludes":{"@id":"unece:Plot"},"rdfs:comment":"The code specifying the type of regulatory soil for this crop plot."},{"@id":"unece:specifiedArea","@type":["rdf:Property","owl:ObjectProperty"],"rdfs:label":"specifiedArea","schema:rangeIncludes":{"@id":"unece:Area"},"schema:domainIncludes":{"@id":"unece:Plot"},"rdfs:comment":"An agricultural zone area specified for this crop plot."},{"@id":"unece:applicableAnimalCertification","@type":["rdf:Property","owl:ObjectProperty"],"rdfs:label":"applicableAnimalCertification","schema:rangeIncludes":{"@id":"unece:AnimalCertification"},"schema:domainIncludes":{"@id":"unece:AnimalCertificate"},"rdfs:comment":"An animal certification applicable to this animal certificate."},{"@id":"unece:appliedArea","@type":["rdf:Property","owl:ObjectProperty"],"rdfs:label":"appliedArea","schema:rangeIncludes":{"@id":"unece:Area"},"schema:domainIncludes":{"@id":"unece:AgriculturalApplication"},"rdfs:comment":"A specified agricultural application applied to this agricultural zone area."},{"@id":"unece:appliedCertificate","@type":["rdf:Property","owl:ObjectProperty"],"rdfs:label":"appliedCertificate","schema:rangeIncludes":{"@id":"unece:AgriculturalCertificate"},"schema:domainIncludes":{"@id":"unece:AgriculturalApplication"},"rdfs:comment":"An agricultural certificate applied to this specified agricultural application."},{"@id":"unece:appliedMaterial","@type":["rdf:Property","owl:ObjectProperty"],"rdfs:label":"appliedMaterial","schema:rangeIncludes":{"@id":"unece:SpecifiedMaterial"},"schema:domainIncludes":{"@id":"unece:AgriculturalApplication"},"rdfs:comment":"A substance from which something is or could be made."},{"@id":"unece:nominalSizeNumeric","@type":["rdf:Property","owl:DatatypeProperty"],"rdfs:label":"nominalSizeNumeric","schema:rangeIncludes":{"@id":"schema:Text"},"schema:domainIncludes":{"@id":"unece:CropProduceBatch"},"rdfs:comment":"The value of the nominal size for this crop produce batch."},{"@id":"unece:specifiedProduce","@type":["rdf:Property","owl:ObjectProperty"],"rdfs:label":"specifiedProduce","schema:rangeIncludes":{"@id":"unece:Produce"},"schema:domainIncludes":{"@id":"unece:CropProduceBatch"},"rdfs:comment":"A crop produce specified for this crop produce batch."},{"@id":"unece:specifiedQuantity","@type":["rdf:Property","owl:ObjectProperty"],"rdfs:label":"specifiedQuantity","schema:rangeIncludes":{"@id":"unece:QuantityType"},"schema:domainIncludes":{"@id":"unece:CropProduceBatch"},"rdfs:comment":""},{"@id":"unece:deathDateTime","@type":["rdf:Property","owl:DatatypeProperty"],"rdfs:label":"deathDateTime","schema:rangeIncludes":{"@id":"schema:Text"},"schema:domainIncludes":{"@id":"unece:IndividualTTAnimal"},"rdfs:comment":"The death date for this individual TT animal."},{"@id":"unece:botanicalGenusCode","@type":["rdf:Property","owl:DatatypeProperty"],"rdfs:label":"botanicalGenusCode","schema:rangeIncludes":{"@id":"schema:Text"},"schema:domainIncludes":{"@id":"unece:BotanicalCrop"},"rdfs:comment":"The code specifying the genus for this botanical crop."},{"@id":"unece:botanicalIdentificationId","@type":["rdf:Property","owl:DatatypeProperty"],"rdfs:label":"botanicalIdentificationId","schema:rangeIncludes":{"@id":"schema:Text"},"schema:domainIncludes":{"@id":"unece:BotanicalCrop"},"rdfs:comment":"The identifier for this botanical crop."},{"@id":"unece:botanicalName","@type":["rdf:Property","owl:DatatypeProperty"],"rdfs:label":"botanicalName","schema:rangeIncludes":{"@id":"schema:Text"},"schema:domainIncludes":{"@id":"unece:BotanicalCrop"},"rdfs:comment":"The botanical name, expressed as text, for this botanical crop."},{"@id":"unece:botanicalSpeciesCode","@type":["rdf:Property","owl:DatatypeProperty"],"rdfs:label":"botanicalSpeciesCode","schema:rangeIncludes":{"@id":"schema:Text"},"schema:domainIncludes":{"@id":"unece:BotanicalCrop"},"rdfs:comment":"The code specifying the species for this botanical crop."},{"@id":"unece:fLUXId","@type":["rdf:Property","owl:DatatypeProperty"],"rdfs:label":"fLUXId","schema:rangeIncludes":{"@id":"schema:Text"},"schema:domainIncludes":{"@id":"unece:AnimalBatch"},"rdfs:comment":"A Fisheries Language for Universal eXchange (FLUX) identifier for this animal batch."},{"@id":"unece:saleDateTime","@type":["rdf:Property","owl:DatatypeProperty"],"rdfs:label":"saleDateTime","schema:rangeIncludes":{"@id":"schema:Text"},"schema:domainIncludes":{"@id":"unece:AnimalBatch"},"rdfs:comment":"The date, time, date time, or other date time value of the sale for this animal batch."},{"@id":"unece:salesNoteId","@type":["rdf:Property","owl:DatatypeProperty"],"rdfs:label":"salesNoteId","schema:rangeIncludes":{"@id":"schema:Text"},"schema:domainIncludes":{"@id":"unece:AnimalBatch"},"rdfs:comment":"The identifier for the sales note for this animal batch."},{"@id":"unece:calculatedYieldMeasure","@type":["rdf:Property","owl:ObjectProperty"],"rdfs:label":"calculatedYieldMeasure","schema:rangeIncludes":{"@id":"unece:MeasureType"},"schema:domainIncludes":{"@id":"unece:Produce"},"rdfs:comment":""},{"@id":"unece:estimatedYieldMeasure","@type":["rdf:Property","owl:ObjectProperty"],"rdfs:label":"estimatedYieldMeasure","schema:rangeIncludes":{"@id":"unece:MeasureType"},"schema:domainIncludes":{"@id":"unece:Produce"},"rdfs:comment":""},{"@id":"unece:inputSpecifiedBatch","@type":["rdf:Property","owl:ObjectProperty"],"rdfs:label":"inputSpecifiedBatch","schema:rangeIncludes":{"@id":"unece:CropProduceBatch"},"schema:domainIncludes":{"@id":"unece:Produce"},"rdfs:comment":"An input batch crop produce, such as seed or fertilizer, specified for this crop produce."},{"@id":"unece:outputSpecifiedBatch","@type":["rdf:Property","owl:ObjectProperty"],"rdfs:label":"outputSpecifiedBatch","schema:rangeIncludes":{"@id":"unece:CropProduceBatch"},"schema:domainIncludes":{"@id":"unece:Produce"},"rdfs:comment":"An output batch crop produce, such as potatoes, grain, straw, specified for this crop produce."},{"@id":"unece:cropProportionPercent","@type":["rdf:Property","owl:DatatypeProperty"],"rdfs:label":"cropProportionPercent","schema:rangeIncludes":{"@id":"schema:Text"},"schema:domainIncludes":{"@id":"unece:CropMixtureConstituent"},"rdfs:comment":"The percent of the crop proportion of this field crop mixture constituent."},{"@id":"unece:specifiedBotanicalCrop","@type":["rdf:Property","owl:ObjectProperty"],"rdfs:label":"specifiedBotanicalCrop","schema:rangeIncludes":{"@id":"unece:BotanicalCrop"},"schema:domainIncludes":{"@id":"unece:CropMixtureConstituent"},"rdfs:comment":"The botanical crop specified for this field crop mixture constituent."},{"@id":"unece:identifierLengthNumeric","@type":["rdf:Property","owl:DatatypeProperty"],"rdfs:label":"identifierLengthNumeric","schema:rangeIncludes":{"@id":"schema:Text"},"schema:domainIncludes":{"@id":"unece:AnimalIdentity"},"rdfs:comment":"The length, expressed as the number of characters, of the identifier in this animal identity."},{"@id":"unece:issuerPartyName","@type":["rdf:Property","owl:DatatypeProperty"],"rdfs:label":"issuerPartyName","schema:rangeIncludes":{"@id":"schema:Text"},"schema:domainIncludes":{"@id":"unece:AnimalIdentity"},"rdfs:comment":"The name, expressed as text, of the party issuing this animal identity."},{"@id":"unece:legalBasis","@type":["rdf:Property","owl:DatatypeProperty"],"rdfs:label":"legalBasis","schema:rangeIncludes":{"@id":"schema:Text"},"schema:domainIncludes":{"@id":"unece:AnimalIdentity"},"rdfs:comment":"The legal basis, expressed as text, for this animal identity."},{"@id":"unece:locationId","@type":["rdf:Property","owl:DatatypeProperty"],"rdfs:label":"locationId","schema:rangeIncludes":{"@id":"schema:Text"},"schema:domainIncludes":[{"@id":"unece:AnimalHoldingEvent"},{"@id":"unece:MDHHealthIndication"}],"rdfs:comment":"An identifier of a location for this MDH health indication."},{"@id":"unece:regulationSpeciesNameTypeCode","@type":["rdf:Property","owl:DatatypeProperty"],"rdfs:label":"regulationSpeciesNameTypeCode","schema:rangeIncludes":{"@id":"schema:Text"},"schema:domainIncludes":{"@id":"unece:SpeciesTTAnimal"},"rdfs:comment":"A code specifying the type of regulation species name for this TT animal."},{"@id":"unece:scientificSpeciesNameTypeCode","@type":["rdf:Property","owl:DatatypeProperty"],"rdfs:label":"scientificSpeciesNameTypeCode","schema:rangeIncludes":{"@id":"schema:Text"},"schema:domainIncludes":{"@id":"unece:SpeciesTTAnimal"},"rdfs:comment":"A code specifying the type of scientific species name for this TT animal."},{"@id":"unece:tradeSpeciesNameTypeCode","@type":["rdf:Property","owl:DatatypeProperty"],"rdfs:label":"tradeSpeciesNameTypeCode","schema:rangeIncludes":{"@id":"schema:Text"},"schema:domainIncludes":{"@id":"unece:SpeciesTTAnimal"},"rdfs:comment":"A code specifying the type of trade species name for this TT animal."},{"@id":"unece:accompaniedIndicator","@type":["rdf:Property","owl:DatatypeProperty"],"rdfs:label":"accompaniedIndicator","schema:rangeIncludes":{"@id":"schema:Boolean"},"schema:domainIncludes":{"@id":"unece:LogisticsTransportEquipment"},"rdfs:comment":"The indication of whether or not this piece of logistics transport equipment is accompanied, such as by a transport means."},{"@id":"unece:actualRoute","@type":["rdf:Property","owl:ObjectProperty"],"rdfs:label":"actualRoute","schema:rangeIncludes":{"@id":"unece:TransportRoute"},"schema:domainIncludes":{"@id":"unece:LogisticsTransportEquipment"},"rdfs:comment":"An actual route for this piece of logistics transport equipment."},{"@id":"unece:additionalInstructions","@type":["rdf:Property","owl:ObjectProperty"],"rdfs:label":"additionalInstructions","schema:rangeIncludes":{"@id":"unece:TransportInstructions"},"schema:domainIncludes":{"@id":"unece:LogisticsTransportEquipment"},"rdfs:comment":"Transport information of an instructive nature."},{"@id":"unece:affixedSeal","@type":["rdf:Property","owl:ObjectProperty"],"rdfs:label":"affixedSeal","schema:rangeIncludes":{"@id":"unece:Seal"},"schema:domainIncludes":[{"@id":"unece:LogisticsTransportEquipment"},{"@id":"unece:AssociatedTransportEquipment"}],"rdfs:comment":"A device used to secure an object and protect it from unauthorized entry or tampering during transport or other logistics operations."},{"@id":"unece:airFlowUnitAirFlowMeasure","@type":["rdf:Property","owl:ObjectProperty"],"rdfs:label":"airFlowUnitAirFlowMeasure","schema:rangeIncludes":{"@id":"unece:AirFlowUnitMeasureType"},"schema:domainIncludes":{"@id":"unece:LogisticsTransportEquipment"},"rdfs:comment":""},{"@id":"unece:attachedAttachedTransportEquipment","@type":["rdf:Property","owl:ObjectProperty"],"rdfs:label":"attachedAttachedTransportEquipment","schema:rangeIncludes":{"@id":"unece:AttachedTransportEquipment"},"schema:domainIncludes":{"@id":"unece:LogisticsTransportEquipment"},"rdfs:comment":"Transport equipment attached to this piece of logistics transport equipment, such as ropes or refrigeration units."},{"@id":"unece:attachedIOTDevice","@type":["rdf:Property","owl:ObjectProperty"],"rdfs:label":"attachedIOTDevice","schema:rangeIncludes":{"@id":"unece:IOTDevice"},"schema:domainIncludes":[{"@id":"unece:LogisticsTransportEquipment"},{"@id":"unece:LogisticsTransportMeans"}],"rdfs:comment":"An IOT device attached to this logistics transport means."},{"@id":"unece:bondedWarehouseStorageEvent","@type":["rdf:Property","owl:ObjectProperty"],"rdfs:label":"bondedWarehouseStorageEvent","schema:rangeIncludes":{"@id":"unece:TransportEvent"},"schema:domainIncludes":[{"@id":"unece:LogisticsTransportEquipment"},{"@id":"unece:Consignment"}],"rdfs:comment":"A bonded warehouse storage event for this supply chain consignment."},{"@id":"unece:carriedTransportEquipment","@type":["rdf:Property","owl:ObjectProperty"],"rdfs:label":"carriedTransportEquipment","schema:rangeIncludes":{"@id":"unece:AssociatedTransportEquipment"},"schema:domainIncludes":{"@id":"unece:LogisticsTransportEquipment"},"rdfs:comment":"A piece of transport equipment carried on this piece of logistics transport equipment, such as a container placed on a rail wagon."},{"@id":"unece:carrierAssignedBookingId","@type":["rdf:Property","owl:DatatypeProperty"],"rdfs:label":"carrierAssignedBookingId","schema:rangeIncludes":{"@id":"schema:Text"},"schema:domainIncludes":{"@id":"unece:LogisticsTransportEquipment"},"rdfs:comment":"A carrier assigned booking identifier for this piece of logistics transport equipment."},{"@id":"unece:characteristic","@type":["rdf:Property","owl:DatatypeProperty"],"rdfs:label":"characteristic","schema:rangeIncludes":{"@id":"schema:Text"},"schema:domainIncludes":[{"@id":"unece:LogisticsTransportEquipment"},{"@id":"unece:AssociatedTransportEquipment"},{"@id":"unece:AttachedTransportEquipment"}],"rdfs:comment":"The characteristic or characteristics, expressed as text, of a piece of logistics transport equipment, such as its size and type."},{"@id":"unece:consolidationEvent","@type":["rdf:Property","owl:ObjectProperty"],"rdfs:label":"consolidationEvent","schema:rangeIncludes":{"@id":"unece:TransportEvent"},"schema:domainIncludes":{"@id":"unece:LogisticsTransportEquipment"},"rdfs:comment":"A consolidation event specifying when and where this piece of logistics transport equipment will be, or has been, stuffed."},{"@id":"unece:containedConsignment","@type":["rdf:Property","owl:ObjectProperty"],"rdfs:label":"containedConsignment","schema:rangeIncludes":{"@id":"unece:Consignment"},"schema:domainIncludes":[{"@id":"unece:LogisticsTransportEquipment"},{"@id":"unece:AssociatedTransportEquipment"}],"rdfs:comment":"A consignment contained in this piece of logistics transport equipment."},{"@id":"unece:containedConsignmentQuantity","@type":["rdf:Property","owl:ObjectProperty"],"rdfs:label":"containedConsignmentQuantity","schema:rangeIncludes":{"@id":"unece:QuantityType"},"schema:domainIncludes":{"@id":"unece:LogisticsTransportEquipment"},"rdfs:comment":""},{"@id":"unece:containedTransportEquipment","@type":["rdf:Property","owl:ObjectProperty"],"rdfs:label":"containedTransportEquipment","schema:rangeIncludes":{"@id":"unece:AssociatedTransportEquipment"},"schema:domainIncludes":{"@id":"unece:LogisticsTransportEquipment"},"rdfs:comment":"A piece of transport equipment contained within this piece of logistics transport equipment, such as a pallet."},{"@id":"unece:damageRemark","@type":["rdf:Property","owl:DatatypeProperty"],"rdfs:label":"damageRemark","schema:rangeIncludes":{"@id":"schema:Text"},"schema:domainIncludes":{"@id":"unece:LogisticsTransportEquipment"},"rdfs:comment":"A damage remark, expressed as text, for this piece of logistics transport equipment."},{"@id":"unece:deconsolidationEvent","@type":["rdf:Property","owl:ObjectProperty"],"rdfs:label":"deconsolidationEvent","schema:rangeIncludes":{"@id":"unece:TransportEvent"},"schema:domainIncludes":{"@id":"unece:LogisticsTransportEquipment"},"rdfs:comment":"A deconsolidation event for this piece of logistics transport equipment."},{"@id":"unece:deliveryInstructions","@type":["rdf:Property","owl:ObjectProperty"],"rdfs:label":"deliveryInstructions","schema:rangeIncludes":{"@id":"unece:DeliveryInstructions"},"schema:domainIncludes":[{"@id":"unece:LogisticsTransportEquipment"},{"@id":"unece:Consignment"}],"rdfs:comment":"Delivery instructions for this piece of logistics transport equipment."},{"@id":"unece:deliveryTransportEvent","@type":["rdf:Property","owl:ObjectProperty"],"rdfs:label":"deliveryTransportEvent","schema:rangeIncludes":{"@id":"unece:TransportEvent"},"schema:domainIncludes":[{"@id":"unece:LogisticsTransportEquipment"},{"@id":"unece:Consignment"},{"@id":"unece:ConsignmentItem"}],"rdfs:comment":"A delivery event for this piece of logistics transport equipment."},{"@id":"unece:handlingInstructions","@type":["rdf:Property","owl:ObjectProperty"],"rdfs:label":"handlingInstructions","schema:rangeIncludes":{"@id":"unece:HandlingInstructions"},"schema:domainIncludes":[{"@id":"unece:LogisticsTransportEquipment"},{"@id":"unece:DangerousGoods"},{"@id":"unece:Consignment"},{"@id":"unece:ConsignmentItem"}],"rdfs:comment":"Handling instructions for the transported dangerous goods."},{"@id":"unece:humidityPercent","@type":["rdf:Property","owl:DatatypeProperty"],"rdfs:label":"humidityPercent","schema:rangeIncludes":{"@id":"schema:Text"},"schema:domainIncludes":{"@id":"unece:LogisticsTransportEquipment"},"rdfs:comment":"The percent of the humidity (moisture content) within this piece of logistics transport equipment."},{"@id":"unece:linearUnitLoadingLengthMeasure","@type":["rdf:Property","owl:ObjectProperty"],"rdfs:label":"linearUnitLoadingLengthMeasure","schema:rangeIncludes":{"@id":"unece:LinearUnitMeasureType"},"schema:domainIncludes":[{"@id":"unece:LogisticsTransportEquipment"},{"@id":"unece:Consignment"},{"@id":"unece:ConsignmentItem"}],"rdfs:comment":""},{"@id":"unece:linearUnitRequiredLaneLengthMeasure","@type":["rdf:Property","owl:ObjectProperty"],"rdfs:label":"linearUnitRequiredLaneLengthMeasure","schema:rangeIncludes":{"@id":"unece:LinearUnitMeasureType"},"schema:domainIncludes":[{"@id":"unece:LogisticsTransportEquipment"},{"@id":"unece:LogisticsTransportMeans"}],"rdfs:comment":""},{"@id":"unece:loadedConsignmentItem","@type":["rdf:Property","owl:ObjectProperty"],"rdfs:label":"loadedConsignmentItem","schema:rangeIncludes":{"@id":"unece:ConsignmentItem"},"schema:domainIncludes":{"@id":"unece:LogisticsTransportEquipment"},"rdfs:comment":"A consignment item loaded onto, or into, this piece of logistics transport equipment."},{"@id":"unece:loadedDangerousGoods","@type":["rdf:Property","owl:ObjectProperty"],"rdfs:label":"loadedDangerousGoods","schema:rangeIncludes":{"@id":"unece:DangerousGoods"},"schema:domainIncludes":[{"@id":"unece:LogisticsTransportEquipment"},{"@id":"unece:AssociatedTransportEquipment"}],"rdfs:comment":"Dangerous goods loaded into or onto this piece of associated transport equipment."},{"@id":"unece:loadedPackageQuantity","@type":["rdf:Property","owl:ObjectProperty"],"rdfs:label":"loadedPackageQuantity","schema:rangeIncludes":{"@id":"unece:QuantityType"},"schema:domainIncludes":[{"@id":"unece:LogisticsTransportEquipment"},{"@id":"unece:AssociatedTransportEquipment"}],"rdfs:comment":""},{"@id":"unece:loadingEvent","@type":["rdf:Property","owl:ObjectProperty"],"rdfs:label":"loadingEvent","schema:rangeIncludes":{"@id":"unece:TransportEvent"},"schema:domainIncludes":[{"@id":"unece:LogisticsTransportEquipment"},{"@id":"unece:TransportMovement"}],"rdfs:comment":"The loading event during which goods will be or have been loaded into or onto the means of transport used for this logistics transport movement."},{"@id":"unece:loadingInstructions","@type":["rdf:Property","owl:ObjectProperty"],"rdfs:label":"loadingInstructions","schema:rangeIncludes":{"@id":"unece:TransportInstructions"},"schema:domainIncludes":[{"@id":"unece:LogisticsTransportEquipment"},{"@id":"unece:Consignment"}],"rdfs:comment":"Transport information of an instructive nature."},{"@id":"unece:loadingParty","@type":["rdf:Property","owl:ObjectProperty"],"rdfs:label":"loadingParty","schema:rangeIncludes":{"@id":"unece:Party"},"schema:domainIncludes":{"@id":"unece:LogisticsTransportEquipment"},"rdfs:comment":""},{"@id":"unece:loadingRemark","@type":["rdf:Property","owl:DatatypeProperty"],"rdfs:label":"loadingRemark","schema:rangeIncludes":{"@id":"schema:Text"},"schema:domainIncludes":{"@id":"unece:LogisticsTransportEquipment"},"rdfs:comment":"A loading remark, expressed as text, for this piece of logistics transport equipment."},{"@id":"unece:loadingSequenceNumeric","@type":["rdf:Property","owl:DatatypeProperty"],"rdfs:label":"loadingSequenceNumeric","schema:rangeIncludes":{"@id":"schema:Text"},"schema:domainIncludes":[{"@id":"unece:LogisticsTransportEquipment"},{"@id":"unece:Consignment"}],"rdfs:comment":"The loading sequence number for this supply chain consignment."},{"@id":"unece:logisticsTransportEquipmentCharacteristicCode","@type":["rdf:Property","owl:DatatypeProperty"],"rdfs:label":"logisticsTransportEquipmentCharacteristicCode","schema:rangeIncludes":{"@id":"schema:Text"},"schema:domainIncludes":{"@id":"unece:LogisticsTransportEquipment"},"rdfs:comment":"The code specifying the characteristic or characteristics of this piece of logistics transport equipment, such as the ISO 6346 transport equipment size and type code."},{"@id":"unece:manufacturingDateTime","@type":["rdf:Property","owl:DatatypeProperty"],"rdfs:label":"manufacturingDateTime","schema:rangeIncludes":{"@id":"schema:DateTime"},"schema:domainIncludes":[{"@id":"unece:LogisticsTransportEquipment"},{"@id":"unece:LogisticsTransportMeans"}],"rdfs:comment":"The manufacturing date, time, date time, or other date time value for this logistics means of transport."},{"@id":"unece:notifiedParty","@type":["rdf:Property","owl:ObjectProperty"],"rdfs:label":"notifiedParty","schema:rangeIncludes":{"@id":"unece:Party"},"schema:domainIncludes":[{"@id":"unece:LogisticsTransportEquipment"},{"@id":"unece:TransportMovement"},{"@id":"unece:Consignment"}],"rdfs:comment":""},{"@id":"unece:operatingParty","@type":["rdf:Property","owl:ObjectProperty"],"rdfs:label":"operatingParty","schema:rangeIncludes":{"@id":"unece:Party"},"schema:domainIncludes":{"@id":"unece:LogisticsTransportEquipment"},"rdfs:comment":""},{"@id":"unece:ownerParty","@type":["rdf:Property","owl:ObjectProperty"],"rdfs:label":"ownerParty","schema:rangeIncludes":{"@id":"unece:Party"},"schema:domainIncludes":[{"@id":"unece:LogisticsTransportEquipment"},{"@id":"unece:LogisticsTransportMeans"},{"@id":"unece:IOTDevice"},{"@id":"unece:Sensor"}],"rdfs:comment":""},{"@id":"unece:pickUpEvent","@type":["rdf:Property","owl:ObjectProperty"],"rdfs:label":"pickUpEvent","schema:rangeIncludes":{"@id":"unece:TransportEvent"},"schema:domainIncludes":[{"@id":"unece:LogisticsTransportEquipment"},{"@id":"unece:Consignment"},{"@id":"unece:ConsignmentItem"}],"rdfs:comment":"A pick-up event specifying when and where this piece of logistics transport equipment will be, or has been, collected, i.e. picked-up by the carrier."},{"@id":"unece:positioningEvent","@type":["rdf:Property","owl:ObjectProperty"],"rdfs:label":"positioningEvent","schema:rangeIncludes":{"@id":"unece:TransportEvent"},"schema:domainIncludes":{"@id":"unece:LogisticsTransportEquipment"},"rdfs:comment":"A positioning event specifying when and where this piece of logistics transport equipment will be, or has been, positioned, i.e. delivered and available for pick-up."},{"@id":"unece:powerSupplyConnectorQuantity","@type":["rdf:Property","owl:ObjectProperty"],"rdfs:label":"powerSupplyConnectorQuantity","schema:rangeIncludes":{"@id":"unece:QuantityType"},"schema:domainIncludes":{"@id":"unece:LogisticsTransportEquipment"},"rdfs:comment":""},{"@id":"unece:powerSupplyType","@type":["rdf:Property","owl:DatatypeProperty"],"rdfs:label":"powerSupplyType","schema:rangeIncludes":{"@id":"schema:Text"},"schema:domainIncludes":{"@id":"unece:LogisticsTransportEquipment"},"rdfs:comment":"The type of power supply, expressed as text, for this piece of logistics transport equipment, such as diesel fuel or electricity."},{"@id":"unece:powerSupplyTypeCode","@type":["rdf:Property","owl:DatatypeProperty"],"rdfs:label":"powerSupplyTypeCode","schema:rangeIncludes":{"@id":"schema:Text"},"schema:domainIncludes":{"@id":"unece:LogisticsTransportEquipment"},"rdfs:comment":"The code specifying the type of power supply for this piece of logistics transport equipment, such as diesel fuel or electricity."},{"@id":"unece:quarantineInstructions","@type":["rdf:Property","owl:ObjectProperty"],"rdfs:label":"quarantineInstructions","schema:rangeIncludes":{"@id":"unece:QuarantineInstructions"},"schema:domainIncludes":[{"@id":"unece:LogisticsTransportEquipment"},{"@id":"unece:ConsignmentItem"}],"rdfs:comment":"Instructions for a period of imposed isolation or detention."},{"@id":"unece:relatedEvent","@type":["rdf:Property","owl:ObjectProperty"],"rdfs:label":"relatedEvent","schema:rangeIncludes":{"@id":"unece:CommunicationEvent"},"schema:domainIncludes":[{"@id":"unece:LogisticsTransportEquipment"},{"@id":"unece:IOTDevice"}],"rdfs:comment":"A significant occurrence or happening communicated by means of sending or receiving information, such as transmitting digital data by using the internet."},{"@id":"unece:releaseId","@type":["rdf:Property","owl:DatatypeProperty"],"rdfs:label":"releaseId","schema:rangeIncludes":{"@id":"schema:Text"},"schema:domainIncludes":{"@id":"unece:LogisticsTransportEquipment"},"rdfs:comment":"The release identifier for this piece of logistics transport equipment."},{"@id":"unece:releaseRestriction","@type":["rdf:Property","owl:DatatypeProperty"],"rdfs:label":"releaseRestriction","schema:rangeIncludes":{"@id":"schema:Text"},"schema:domainIncludes":{"@id":"unece:LogisticsTransportEquipment"},"rdfs:comment":"The release restriction, expressed as text, for this piece of logistics transport equipment."},{"@id":"unece:reportedLogisticsStatus","@type":["rdf:Property","owl:ObjectProperty"],"rdfs:label":"reportedLogisticsStatus","schema:rangeIncludes":{"@id":"unece:LogisticsStatus"},"schema:domainIncludes":[{"@id":"unece:LogisticsTransportEquipment"},{"@id":"unece:Consignment"},{"@id":"unece:ConsignmentItem"}],"rdfs:comment":"A logistics status reported for this cross-border regulatory procedure."},{"@id":"unece:reportingIOTDevicePairing","@type":["rdf:Property","owl:ObjectProperty"],"rdfs:label":"reportingIOTDevicePairing","schema:rangeIncludes":{"@id":"unece:Pairing"},"schema:domainIncludes":{"@id":"unece:LogisticsTransportEquipment"},"rdfs:comment":"The process by which two potentially communicating entities are linked."},{"@id":"unece:reportingIOTDeviceTransportEvent","@type":["rdf:Property","owl:ObjectProperty"],"rdfs:label":"reportingIOTDeviceTransportEvent","schema:rangeIncludes":{"@id":"unece:TransportEvent"},"schema:domainIncludes":{"@id":"unece:LogisticsTransportEquipment"},"rdfs:comment":"An IOT device reported transport event for this piece of logistics transport equipment."},{"@id":"unece:requestedRoute","@type":["rdf:Property","owl:ObjectProperty"],"rdfs:label":"requestedRoute","schema:rangeIncludes":{"@id":"unece:TransportRoute"},"schema:domainIncludes":{"@id":"unece:LogisticsTransportEquipment"},"rdfs:comment":"A requested route for this piece of logistics transport equipment."},{"@id":"unece:returnableIndicator","@type":["rdf:Property","owl:DatatypeProperty"],"rdfs:label":"returnableIndicator","schema:rangeIncludes":{"@id":"schema:Boolean"},"schema:domainIncludes":[{"@id":"unece:LogisticsTransportEquipment"},{"@id":"unece:Package"},{"@id":"unece:LogisticsPackaging"},{"@id":"unece:SupplyChainPackaging"}],"rdfs:comment":"The indication of whether or not this logistics package is returnable."},{"@id":"unece:scheduledRoute","@type":["rdf:Property","owl:ObjectProperty"],"rdfs:label":"scheduledRoute","schema:rangeIncludes":{"@id":"unece:TransportRoute"},"schema:domainIncludes":{"@id":"unece:LogisticsTransportEquipment"},"rdfs:comment":"A scheduled or planned route for this piece of logistics transport equipment."},{"@id":"unece:sealQuantity","@type":["rdf:Property","owl:ObjectProperty"],"rdfs:label":"sealQuantity","schema:rangeIncludes":{"@id":"unece:QuantityType"},"schema:domainIncludes":[{"@id":"unece:LogisticsTransportEquipment"},{"@id":"unece:AssociatedTransportEquipment"}],"rdfs:comment":""},{"@id":"unece:sealedIndicator","@type":["rdf:Property","owl:DatatypeProperty"],"rdfs:label":"sealedIndicator","schema:rangeIncludes":{"@id":"schema:Boolean"},"schema:domainIncludes":[{"@id":"unece:LogisticsTransportEquipment"},{"@id":"unece:AssociatedTransportEquipment"}],"rdfs:comment":"The indication of whether or not this associated piece of transport equipment is sealed."},{"@id":"unece:settingTemperature","@type":["rdf:Property","owl:ObjectProperty"],"rdfs:label":"settingTemperature","schema:rangeIncludes":{"@id":"unece:TransportSettingTemperature"},"schema:domainIncludes":[{"@id":"unece:LogisticsTransportEquipment"},{"@id":"unece:AssociatedTransportEquipment"}],"rdfs:comment":"A temperature setting for this piece of associated transport equipment, such as storage temperature or operational temperature."},{"@id":"unece:shipperReferenceInformation","@type":["rdf:Property","owl:DatatypeProperty"],"rdfs:label":"shipperReferenceInformation","schema:rangeIncludes":{"@id":"schema:Text"},"schema:domainIncludes":{"@id":"unece:LogisticsTransportEquipment"},"rdfs:comment":"Shipper reference information, expressed as text, for this piece of logistics transport equipment."},{"@id":"unece:specifiedTransportMeans","@type":["rdf:Property","owl:ObjectProperty"],"rdfs:label":"specifiedTransportMeans","schema:rangeIncludes":{"@id":"unece:LogisticsTransportMeans"},"schema:domainIncludes":{"@id":"unece:LogisticsTransportEquipment"},"rdfs:comment":"A transport means specified for this piece of logistics transport equipment."},{"@id":"unece:storageEvent","@type":["rdf:Property","owl:ObjectProperty"],"rdfs:label":"storageEvent","schema:rangeIncludes":{"@id":"unece:TransportEvent"},"schema:domainIncludes":[{"@id":"unece:LogisticsTransportEquipment"},{"@id":"unece:Consignment"}],"rdfs:comment":"A storage event for this supply chain consignment."},{"@id":"unece:stowagePositionId","@type":["rdf:Property","owl:DatatypeProperty"],"rdfs:label":"stowagePositionId","schema:rangeIncludes":{"@id":"schema:Text"},"schema:domainIncludes":{"@id":"unece:LogisticsTransportEquipment"},"rdfs:comment":"The stowage position identifier for this piece of logistics transport equipment."},{"@id":"unece:transportEquipmentCategoryCode","@type":["rdf:Property","owl:DatatypeProperty"],"rdfs:label":"transportEquipmentCategoryCode","schema:rangeIncludes":{"@id":"unece:TransportEquipmentCategoryCodeList"},"schema:domainIncludes":[{"@id":"unece:LogisticsTransportEquipment"},{"@id":"unece:AssociatedTransportEquipment"},{"@id":"unece:AttachedTransportEquipment"}],"rdfs:comment":"A code specifying a category of this piece of associated transport equipment."},{"@id":"unece:transportEquipmentFullnessUsedCapacityCode","@type":["rdf:Property","owl:DatatypeProperty"],"rdfs:label":"transportEquipmentFullnessUsedCapacityCode","schema:rangeIncludes":{"@id":"unece:TransportEquipmentFullnessCodeList"},"schema:domainIncludes":{"@id":"unece:LogisticsTransportEquipment"},"rdfs:comment":"The code specifying the used capacity of this piece of logistics transport equipment, such as full or empty."},{"@id":"unece:transportEquipmentHaulageArrangementsCode","@type":["rdf:Property","owl:DatatypeProperty"],"rdfs:label":"transportEquipmentHaulageArrangementsCode","schema:rangeIncludes":{"@id":"unece:TransportEquipmentHaulageArrangementsCodeList"},"schema:domainIncludes":{"@id":"unece:LogisticsTransportEquipment"},"rdfs:comment":"The code specifying the arrangement for the haulage of this piece of logistics transport equipment."},{"@id":"unece:transportEquipmentLegalStatusLegalStatusCode","@type":["rdf:Property","owl:DatatypeProperty"],"rdfs:label":"transportEquipmentLegalStatusLegalStatusCode","schema:rangeIncludes":{"@id":"unece:TransportEquipmentLegalStatusCodeList"},"schema:domainIncludes":{"@id":"unece:LogisticsTransportEquipment"},"rdfs:comment":"The code specifying the legal status of this piece of logistics transport equipment with respect to a specific law such as the \"Container Convention Code\"."},{"@id":"unece:transportEquipmentMovementStatusTransportMovementStatusCode","@type":["rdf:Property","owl:DatatypeProperty"],"rdfs:label":"transportEquipmentMovementStatusTransportMovementStatusCode","schema:rangeIncludes":{"@id":"unece:TransportEquipmentMovementStatusCodeList"},"schema:domainIncludes":{"@id":"unece:LogisticsTransportEquipment"},"rdfs:comment":"The code specifying the transport movement status for this piece of logistics transport equipment, such as for export, for import, or for transhipment."},{"@id":"unece:transportEquipmentOperationalStatusCode","@type":["rdf:Property","owl:DatatypeProperty"],"rdfs:label":"transportEquipmentOperationalStatusCode","schema:rangeIncludes":{"@id":"unece:TransportEquipmentOperationalStatusCodeList"},"schema:domainIncludes":{"@id":"unece:LogisticsTransportEquipment"},"rdfs:comment":"The code specifying the operational status for this piece of logistics transport equipment, such as to be repaired or to be shifted."},{"@id":"unece:transportEquipmentSizeTypeCharacteristicCode","@type":["rdf:Property","owl:DatatypeProperty"],"rdfs:label":"transportEquipmentSizeTypeCharacteristicCode","schema:rangeIncludes":{"@id":"unece:TransportEquipmentSizeTypeCodeList"},"schema:domainIncludes":[{"@id":"unece:LogisticsTransportEquipment"},{"@id":"unece:AssociatedTransportEquipment"},{"@id":"unece:AttachedTransportEquipment"}],"rdfs:comment":"The code specifying the characteristics, i.e. size and type, of this piece of associated transport equipment."},{"@id":"unece:transportEquipmentSupplierPartyRoleCode","@type":["rdf:Property","owl:DatatypeProperty"],"rdfs:label":"transportEquipmentSupplierPartyRoleCode","schema:rangeIncludes":{"@id":"unece:TransportEquipmentSupplierPartyRoleCodeList"},"schema:domainIncludes":{"@id":"unece:LogisticsTransportEquipment"},"rdfs:comment":"The code specifying the role of the party responsible for supplying this piece of logistics transport equipment, such as the carrier or the buyer."},{"@id":"unece:transportServicesBuyerParty","@type":["rdf:Property","owl:ObjectProperty"],"rdfs:label":"transportServicesBuyerParty","schema:rangeIncludes":{"@id":"unece:Party"},"schema:domainIncludes":[{"@id":"unece:LogisticsTransportEquipment"},{"@id":"unece:Consignment"}],"rdfs:comment":""},{"@id":"unece:unloadingEvent","@type":["rdf:Property","owl:ObjectProperty"],"rdfs:label":"unloadingEvent","schema:rangeIncludes":{"@id":"unece:TransportEvent"},"schema:domainIncludes":[{"@id":"unece:LogisticsTransportEquipment"},{"@id":"unece:TransportMovement"}],"rdfs:comment":"The unloading event during which goods will be or have been unloaded from the means of transport used for this logistics transport movement."},{"@id":"unece:unloadingInstructions","@type":["rdf:Property","owl:ObjectProperty"],"rdfs:label":"unloadingInstructions","schema:rangeIncludes":{"@id":"unece:TransportInstructions"},"schema:domainIncludes":{"@id":"unece:LogisticsTransportEquipment"},"rdfs:comment":"Transport information of an instructive nature."},{"@id":"unece:unloadingSequenceNumeric","@type":["rdf:Property","owl:DatatypeProperty"],"rdfs:label":"unloadingSequenceNumeric","schema:rangeIncludes":{"@id":"schema:Text"},"schema:domainIncludes":[{"@id":"unece:LogisticsTransportEquipment"},{"@id":"unece:Consignment"}],"rdfs:comment":"The sequence number differentiating this piece of logistics transport equipment from others during unloading."},{"@id":"unece:weightUnitTareWeightMeasure","@type":["rdf:Property","owl:ObjectProperty"],"rdfs:label":"weightUnitTareWeightMeasure","schema:rangeIncludes":{"@id":"unece:WeightUnitMeasureType"},"schema:domainIncludes":[{"@id":"unece:LogisticsTransportEquipment"},{"@id":"unece:LogisticsTransportMeans"}],"rdfs:comment":""},{"@id":"unece:actualArrivalRelatedDateTime","@type":["rdf:Property","owl:DatatypeProperty"],"rdfs:label":"actualArrivalRelatedDateTime","schema:rangeIncludes":{"@id":"schema:Text"},"schema:domainIncludes":{"@id":"unece:TransportEvent"},"rdfs:comment":"The date, time, date time or other date time value of the actual arrival related to this transport event."},{"@id":"unece:actualDepartureRelatedDateTime","@type":["rdf:Property","owl:DatatypeProperty"],"rdfs:label":"actualDepartureRelatedDateTime","schema:rangeIncludes":{"@id":"schema:Text"},"schema:domainIncludes":{"@id":"unece:TransportEvent"},"rdfs:comment":"The date, time, date time or other date time value of the actual departure related to this transport event."},{"@id":"unece:additionalSecurityMeasuresApplicableNote","@type":["rdf:Property","owl:ObjectProperty"],"rdfs:label":"additionalSecurityMeasuresApplicableNote","schema:rangeIncludes":{"@id":"unece:Note"},"schema:domainIncludes":{"@id":"unece:TransportEvent"},"rdfs:comment":"A textual or coded description, such as a remark or additional information."},{"@id":"unece:anchorageDescription","@type":["rdf:Property","owl:DatatypeProperty"],"rdfs:label":"anchorageDescription","schema:rangeIncludes":{"@id":"schema:Text"},"schema:domainIncludes":{"@id":"unece:TransportEvent"},"rdfs:comment":"A textual description of an anchorage for this transport event."},{"@id":"unece:anchorageExpectedIndicator","@type":["rdf:Property","owl:DatatypeProperty"],"rdfs:label":"anchorageExpectedIndicator","schema:rangeIncludes":{"@id":"schema:Boolean"},"schema:domainIncludes":{"@id":"unece:TransportEvent"},"rdfs:comment":"The indication of whether or not this anchorage transport event is or was expected."},{"@id":"unece:arrivalRelatedDateTime","@type":["rdf:Property","owl:DatatypeProperty"],"rdfs:label":"arrivalRelatedDateTime","schema:rangeIncludes":{"@id":"schema:Text"},"schema:domainIncludes":{"@id":"unece:TransportEvent"},"rdfs:comment":"An arrival date, time, date time, or other date time value related to this transport event."},{"@id":"unece:cargoFacilityRelatedLocation","@type":["rdf:Property","owl:ObjectProperty"],"rdfs:label":"cargoFacilityRelatedLocation","schema:rangeIncludes":{"@id":"unece:LogisticsLocation"},"schema:domainIncludes":{"@id":"unece:TransportEvent"},"rdfs:comment":"The location of a cargo facility related to this transport event."},{"@id":"unece:certifyingParty","@type":["rdf:Property","owl:ObjectProperty"],"rdfs:label":"certifyingParty","schema:rangeIncludes":{"@id":"unece:Party"},"schema:domainIncludes":{"@id":"unece:TransportEvent"},"rdfs:comment":""},{"@id":"unece:conveyanceFacilityRelatedLocation","@type":["rdf:Property","owl:ObjectProperty"],"rdfs:label":"conveyanceFacilityRelatedLocation","schema:rangeIncludes":{"@id":"unece:LogisticsLocation"},"schema:domainIncludes":{"@id":"unece:TransportEvent"},"rdfs:comment":"A location of a conveyance facility related to this transport event."},{"@id":"unece:delayOccurrencePeriod","@type":["rdf:Property","owl:ObjectProperty"],"rdfs:label":"delayOccurrencePeriod","schema:rangeIncludes":{"@id":"unece:SpecifiedPeriod"},"schema:domainIncludes":{"@id":"unece:TransportEvent"},"rdfs:comment":"A specified period of time."},{"@id":"unece:delaySpecifiedEvent","@type":["rdf:Property","owl:ObjectProperty"],"rdfs:label":"delaySpecifiedEvent","schema:rangeIncludes":{"@id":"unece:TransportEvent"},"schema:domainIncludes":{"@id":"unece:TransportEvent"},"rdfs:comment":"A delay specified for this referenced transport event."},{"@id":"unece:departureRelatedDateTime","@type":["rdf:Property","owl:DatatypeProperty"],"rdfs:label":"departureRelatedDateTime","schema:rangeIncludes":{"@id":"schema:Text"},"schema:domainIncludes":{"@id":"unece:TransportEvent"},"rdfs:comment":"A departure date, time, date time, or other date time value related to this transport event."},{"@id":"unece:estimatedTransportMeansArrivalOccurrenceDateTime","@type":["rdf:Property","owl:DatatypeProperty"],"rdfs:label":"estimatedTransportMeansArrivalOccurrenceDateTime","schema:rangeIncludes":{"@id":"schema:Text"},"schema:domainIncludes":{"@id":"unece:TransportEvent"},"rdfs:comment":"The date, time, date time, or other date time value when the arrival of a means of transport at the location of this transport event is estimated to occur."},{"@id":"unece:expectedIndicator","@type":["rdf:Property","owl:DatatypeProperty"],"rdfs:label":"expectedIndicator","schema:rangeIncludes":{"@id":"schema:Boolean"},"schema:domainIncludes":{"@id":"unece:TransportEvent"},"rdfs:comment":"The indication of whether or not this transport event is or was expected."},{"@id":"unece:laycanOccurrencePeriod","@type":["rdf:Property","owl:ObjectProperty"],"rdfs:label":"laycanOccurrencePeriod","schema:rangeIncludes":{"@id":"unece:SpecifiedPeriod"},"schema:domainIncludes":{"@id":"unece:TransportEvent"},"rdfs:comment":"A specified period of time."},{"@id":"unece:maritimeAnchorageIndicator","@type":["rdf:Property","owl:DatatypeProperty"],"rdfs:label":"maritimeAnchorageIndicator","schema:rangeIncludes":{"@id":"schema:Boolean"},"schema:domainIncludes":{"@id":"unece:TransportEvent"},"rdfs:comment":"The indication of whether or not this transport event is a maritime anchorage."},{"@id":"unece:pilotBoardingPlace","@type":["rdf:Property","owl:DatatypeProperty"],"rdfs:label":"pilotBoardingPlace","schema:rangeIncludes":{"@id":"schema:Text"},"schema:domainIncludes":{"@id":"unece:TransportEvent"},"rdfs:comment":"A pilot boarding place, expressed as text, for this transport event."},{"@id":"unece:previousAssociatedGeographicalFeature","@type":["rdf:Property","owl:ObjectProperty"],"rdfs:label":"previousAssociatedGeographicalFeature","schema:rangeIncludes":{"@id":"unece:GeographicalFeature"},"schema:domainIncludes":[{"@id":"unece:TransportEvent"},{"@id":"unece:LogisticsLocation"}],"rdfs:comment":"Representation of real world phenomenon associated with a location relative to the Earth, such as cities, buildings, roads, rivers, forests and lakes."},{"@id":"unece:reasonTypeCode","@type":["rdf:Property","owl:DatatypeProperty"],"rdfs:label":"reasonTypeCode","schema:rangeIncludes":{"@id":"schema:Text"},"schema:domainIncludes":{"@id":"unece:TransportEvent"},"rdfs:comment":"The code specifying the reason type for this referenced transport event."},{"@id":"unece:relatedObservation","@type":["rdf:Property","owl:ObjectProperty"],"rdfs:label":"relatedObservation","schema:rangeIncludes":{"@id":"unece:Observation"},"schema:domainIncludes":{"@id":"unece:TransportEvent"},"rdfs:comment":"A specified act or instance of viewing or noting a fact or occurrence for some scientific or other special purpose."},{"@id":"unece:relatedRoute","@type":["rdf:Property","owl:ObjectProperty"],"rdfs:label":"relatedRoute","schema:rangeIncludes":{"@id":"unece:TransportRoute"},"schema:domainIncludes":{"@id":"unece:TransportEvent"},"rdfs:comment":"The route related to this transport event."},{"@id":"unece:reportedConditionTypeCode","@type":["rdf:Property","owl:DatatypeProperty"],"rdfs:label":"reportedConditionTypeCode","schema:rangeIncludes":{"@id":"unece:LogisticsStatusCodeList"},"schema:domainIncludes":{"@id":"unece:TransportEvent"},"rdfs:comment":"The code specifying the type of reported condition for this transport event."},{"@id":"unece:reportingIOTDevice","@type":["rdf:Property","owl:ObjectProperty"],"rdfs:label":"reportingIOTDevice","schema:rangeIncludes":{"@id":"unece:IOTDevice"},"schema:domainIncludes":{"@id":"unece:TransportEvent"},"rdfs:comment":"An IOT device for this transport reporting event."},{"@id":"unece:requestedOccurrenceDateTime","@type":["rdf:Property","owl:DatatypeProperty"],"rdfs:label":"requestedOccurrenceDateTime","schema:rangeIncludes":{"@id":"schema:Text"},"schema:domainIncludes":{"@id":"unece:TransportEvent"},"rdfs:comment":"The requested date, time, date time, or other date time value of the occurrence of this transport event."},{"@id":"unece:requestedRelatedService","@type":["rdf:Property","owl:ObjectProperty"],"rdfs:label":"requestedRelatedService","schema:rangeIncludes":{"@id":"unece:Service"},"schema:domainIncludes":{"@id":"unece:TransportEvent"},"rdfs:comment":"A requested service related to this transport event."},{"@id":"unece:scheduledArrivalRelatedDateTime","@type":["rdf:Property","owl:DatatypeProperty"],"rdfs:label":"scheduledArrivalRelatedDateTime","schema:rangeIncludes":{"@id":"schema:Text"},"schema:domainIncludes":{"@id":"unece:TransportEvent"},"rdfs:comment":"The date, time, date time or other date time value of the scheduled arrival related to this referenced transport event."},{"@id":"unece:scheduledDepartureRelatedDateTime","@type":["rdf:Property","owl:DatatypeProperty"],"rdfs:label":"scheduledDepartureRelatedDateTime","schema:rangeIncludes":{"@id":"schema:Text"},"schema:domainIncludes":{"@id":"unece:TransportEvent"},"rdfs:comment":"The date, time, date time or other date time value of the scheduled departure related to this referenced transport event."},{"@id":"unece:securityLevelCode","@type":["rdf:Property","owl:DatatypeProperty"],"rdfs:label":"securityLevelCode","schema:rangeIncludes":{"@id":"schema:Text"},"schema:domainIncludes":[{"@id":"unece:TransportEvent"},{"@id":"unece:SpecifiedRoute"},{"@id":"unece:TransportRoute"}],"rdfs:comment":"A code specifying a security level for this transport route."},{"@id":"unece:specifiedTransportInstructions","@type":["rdf:Property","owl:ObjectProperty"],"rdfs:label":"specifiedTransportInstructions","schema:rangeIncludes":{"@id":"unece:TransportInstructions"},"schema:domainIncludes":{"@id":"unece:TransportEvent"},"rdfs:comment":"Transport information of an instructive nature."},{"@id":"unece:staySpecifiedEvent","@type":["rdf:Property","owl:ObjectProperty"],"rdfs:label":"staySpecifiedEvent","schema:rangeIncludes":{"@id":"unece:TransportEvent"},"schema:domainIncludes":{"@id":"unece:TransportEvent"},"rdfs:comment":"A stay specified for this referenced transport event."},{"@id":"unece:transportMeansStayOccurrencePeriod","@type":["rdf:Property","owl:ObjectProperty"],"rdfs:label":"transportMeansStayOccurrencePeriod","schema:rangeIncludes":{"@id":"unece:SpecifiedPeriod"},"schema:domainIncludes":{"@id":"unece:TransportEvent"},"rdfs:comment":"A specified period of time."},{"@id":"unece:unitValueMeasure","@type":["rdf:Property","owl:ObjectProperty"],"rdfs:label":"unitValueMeasure","schema:rangeIncludes":{"@id":"unece:UnitMeasureType"},"schema:domainIncludes":{"@id":"unece:TransportEvent"},"rdfs:comment":""},{"@id":"unece:actualPerformancePeriod","@type":["rdf:Property","owl:ObjectProperty"],"rdfs:label":"actualPerformancePeriod","schema:rangeIncludes":{"@id":"unece:SpecifiedPeriod"},"schema:domainIncludes":{"@id":"unece:Service"},"rdfs:comment":"A specified period of time."},{"@id":"unece:contractId","@type":["rdf:Property","owl:DatatypeProperty"],"rdfs:label":"contractId","schema:rangeIncludes":{"@id":"schema:Text"},"schema:domainIncludes":[{"@id":"unece:Service"},{"@id":"unece:Consignment"}],"rdfs:comment":"A contract identifier for this supply chain consignment."},{"@id":"unece:deliverySpecifiedLocation","@type":["rdf:Property","owl:ObjectProperty"],"rdfs:label":"deliverySpecifiedLocation","schema:rangeIncludes":{"@id":"unece:LogisticsLocation"},"schema:domainIncludes":{"@id":"unece:Service"},"rdfs:comment":"A logistics location specified for a delivery by this referenced transport service."},{"@id":"unece:estimatedPerformancePeriod","@type":["rdf:Property","owl:ObjectProperty"],"rdfs:label":"estimatedPerformancePeriod","schema:rangeIncludes":{"@id":"unece:SpecifiedPeriod"},"schema:domainIncludes":{"@id":"unece:Service"},"rdfs:comment":"A specified period of time."},{"@id":"unece:itemQuantity","@type":["rdf:Property","owl:ObjectProperty"],"rdfs:label":"itemQuantity","schema:rangeIncludes":{"@id":"unece:QuantityType"},"schema:domainIncludes":[{"@id":"unece:Service"},{"@id":"unece:Package"}],"rdfs:comment":""},{"@id":"unece:plannedPerformancePeriod","@type":["rdf:Property","owl:ObjectProperty"],"rdfs:label":"plannedPerformancePeriod","schema:rangeIncludes":{"@id":"unece:SpecifiedPeriod"},"schema:domainIncludes":{"@id":"unece:Service"},"rdfs:comment":"A specified period of time."},{"@id":"unece:preplannedIndicator","@type":["rdf:Property","owl:DatatypeProperty"],"rdfs:label":"preplannedIndicator","schema:rangeIncludes":{"@id":"schema:Boolean"},"schema:domainIncludes":{"@id":"unece:Service"},"rdfs:comment":"The indication of whether or not this referenced transport service has been planned in advance of its execution."},{"@id":"unece:relatedSpecifiedLocation","@type":["rdf:Property","owl:ObjectProperty"],"rdfs:label":"relatedSpecifiedLocation","schema:rangeIncludes":{"@id":"unece:LogisticsLocation"},"schema:domainIncludes":{"@id":"unece:Service"},"rdfs:comment":"A related logistics location specified for this referenced transport service."},{"@id":"unece:requestedPerformancePeriod","@type":["rdf:Property","owl:ObjectProperty"],"rdfs:label":"requestedPerformancePeriod","schema:rangeIncludes":{"@id":"unece:SpecifiedPeriod"},"schema:domainIncludes":{"@id":"unece:Service"},"rdfs:comment":"A specified period of time."},{"@id":"unece:requesterParty","@type":["rdf:Property","owl:ObjectProperty"],"rdfs:label":"requesterParty","schema:rangeIncludes":{"@id":"unece:Party"},"schema:domainIncludes":{"@id":"unece:Service"},"rdfs:comment":""},{"@id":"unece:specifiedRoute","@type":["rdf:Property","owl:ObjectProperty"],"rdfs:label":"specifiedRoute","schema:rangeIncludes":{"@id":"unece:TransportRoute"},"schema:domainIncludes":{"@id":"unece:Service"},"rdfs:comment":"A transport route specified for this transport service."},{"@id":"unece:transportContractMovementContractMovementTypeCode","@type":["rdf:Property","owl:DatatypeProperty"],"rdfs:label":"transportContractMovementContractMovementTypeCode","schema:rangeIncludes":{"@id":"unece:TransportContractMovementCodeList"},"schema:domainIncludes":{"@id":"unece:Service"},"rdfs:comment":"A code specifying a contract movement type of this transport service."},{"@id":"unece:transportServiceCategoryTypeCode","@type":["rdf:Property","owl:DatatypeProperty"],"rdfs:label":"transportServiceCategoryTypeCode","schema:rangeIncludes":{"@id":"schema:Text"},"schema:domainIncludes":{"@id":"unece:Service"},"rdfs:comment":"A code specifying a type of category for this transport service."},{"@id":"unece:transportServiceConditionTypeCode","@type":["rdf:Property","owl:DatatypeProperty"],"rdfs:label":"transportServiceConditionTypeCode","schema:rangeIncludes":{"@id":"unece:TransportServiceConditionCodeList"},"schema:domainIncludes":{"@id":"unece:Service"},"rdfs:comment":"A code specifying a type of condition for this transport service, such as a contract or carriage condition."},{"@id":"unece:transportServicePaymentArrangementCode","@type":["rdf:Property","owl:DatatypeProperty"],"rdfs:label":"transportServicePaymentArrangementCode","schema:rangeIncludes":{"@id":"unece:TransportServicePaymentArrangementCodeList"},"schema:domainIncludes":[{"@id":"unece:Service"},{"@id":"unece:ServiceCharge"},{"@id":"unece:Consignment"}],"rdfs:comment":"The code specifying the payment arrangement for this logistics service charge [Reference United Nations Code List (UNCL) 4237]."},{"@id":"unece:transportServicePriorityCode","@type":["rdf:Property","owl:DatatypeProperty"],"rdfs:label":"transportServicePriorityCode","schema:rangeIncludes":{"@id":"unece:TransportServicePriorityCodeList"},"schema:domainIncludes":{"@id":"unece:Service"},"rdfs:comment":"The code specifying the priority of this transport service."},{"@id":"unece:transportServiceRequirementCode","@type":["rdf:Property","owl:DatatypeProperty"],"rdfs:label":"transportServiceRequirementCode","schema:rangeIncludes":{"@id":"unece:TransportServiceRequirementCodeList"},"schema:domainIncludes":{"@id":"unece:Service"},"rdfs:comment":"A code specifying a service requirement for this transport service."},{"@id":"unece:additionalHazardClassificationId","@type":["rdf:Property","owl:DatatypeProperty"],"rdfs:label":"additionalHazardClassificationId","schema:rangeIncludes":{"@id":"schema:Text"},"schema:domainIncludes":{"@id":"unece:DangerousGoods"},"rdfs:comment":"The unique identifier of an additional hazard class applicable to these transported dangerous goods."},{"@id":"unece:aircraftLimitationInformation","@type":["rdf:Property","owl:DatatypeProperty"],"rdfs:label":"aircraftLimitationInformation","schema:rangeIncludes":{"@id":"schema:Text"},"schema:domainIncludes":{"@id":"unece:DangerousGoods"},"rdfs:comment":"Aircraft limitation information, expressed as text, for these transported dangerous goods."},{"@id":"unece:allPackedInOneInformation","@type":["rdf:Property","owl:DatatypeProperty"],"rdfs:label":"allPackedInOneInformation","schema:rangeIncludes":{"@id":"schema:Text"},"schema:domainIncludes":{"@id":"unece:DangerousGoods"},"rdfs:comment":"All packed in one information, expressed as text, for these transported dangerous goods."},{"@id":"unece:authorizationInformation","@type":["rdf:Property","owl:DatatypeProperty"],"rdfs:label":"authorizationInformation","schema:rangeIncludes":{"@id":"schema:Text"},"schema:domainIncludes":{"@id":"unece:DangerousGoods"},"rdfs:comment":"Authorization information, expressed as text, for these transported dangerous goods."},{"@id":"unece:complianceDeclarationInformation","@type":["rdf:Property","owl:DatatypeProperty"],"rdfs:label":"complianceDeclarationInformation","schema:rangeIncludes":{"@id":"schema:Text"},"schema:domainIncludes":{"@id":"unece:DangerousGoods"},"rdfs:comment":"Compliance declaration information, expressed as text, for these transported dangerous goods."},{"@id":"unece:controlTemperatureMeasurement","@type":["rdf:Property","owl:ObjectProperty"],"rdfs:label":"controlTemperatureMeasurement","schema:rangeIncludes":{"@id":"unece:Measurement"},"schema:domainIncludes":{"@id":"unece:DangerousGoods"},"rdfs:comment":"An amount, size, or extent as established by measuring."},{"@id":"unece:dangerousGoodsPackagingLevelPackagingDangerLevelCode","@type":["rdf:Property","owl:DatatypeProperty"],"rdfs:label":"dangerousGoodsPackagingLevelPackagingDangerLevelCode","schema:rangeIncludes":{"@id":"unece:DangerousGoodsPackagingLevelCodeList"},"schema:domainIncludes":{"@id":"unece:DangerousGoods"},"rdfs:comment":"The code specifying the level of danger that the packaging of these dangerous goods must cover for transport purposes."},{"@id":"unece:dangerousGoodsRegulationCode","@type":["rdf:Property","owl:DatatypeProperty"],"rdfs:label":"dangerousGoodsRegulationCode","schema:rangeIncludes":{"@id":"unece:DangerousGoodsRegulationCodeList"},"schema:domainIncludes":{"@id":"unece:DangerousGoods"},"rdfs:comment":"The code specifying a regulation applicable to these transported dangerous goods."},{"@id":"unece:densityMeasure","@type":["rdf:Property","owl:ObjectProperty"],"rdfs:label":"densityMeasure","schema:rangeIncludes":{"@id":"unece:MeasureType"},"schema:domainIncludes":{"@id":"unece:DangerousGoods"},"rdfs:comment":""},{"@id":"unece:eMSId","@type":["rdf:Property","owl:DatatypeProperty"],"rdfs:label":"eMSId","schema:rangeIncludes":{"@id":"schema:Text"},"schema:domainIncludes":{"@id":"unece:DangerousGoods"},"rdfs:comment":"The unique transport emergency procedure (EMS) identifier applicable for these transported dangerous goods."},{"@id":"unece:emergencyContact","@type":["rdf:Property","owl:ObjectProperty"],"rdfs:label":"emergencyContact","schema:rangeIncludes":{"@id":"unece:Contact"},"schema:domainIncludes":{"@id":"unece:DangerousGoods"},"rdfs:comment":"An individual human being in a position to give assistance or information."},{"@id":"unece:emergencyTemperatureMeasurement","@type":["rdf:Property","owl:ObjectProperty"],"rdfs:label":"emergencyTemperatureMeasurement","schema:rangeIncludes":{"@id":"unece:Measurement"},"schema:domainIncludes":{"@id":"unece:DangerousGoods"},"rdfs:comment":"An amount, size, or extent as established by measuring."},{"@id":"unece:explosiveCargoNetWeightMeasure","@type":["rdf:Property","owl:ObjectProperty"],"rdfs:label":"explosiveCargoNetWeightMeasure","schema:rangeIncludes":{"@id":"unece:WeightUnitMeasureType"},"schema:domainIncludes":{"@id":"unece:DangerousGoods"},"rdfs:comment":""},{"@id":"unece:explosiveCompatibilityGroupCode","@type":["rdf:Property","owl:DatatypeProperty"],"rdfs:label":"explosiveCompatibilityGroupCode","schema:rangeIncludes":{"@id":"schema:Text"},"schema:domainIncludes":{"@id":"unece:DangerousGoods"},"rdfs:comment":"The code specifying the explosive compatibility group for these transported dangerous goods."},{"@id":"unece:flashpointTemperatureMeasurement","@type":["rdf:Property","owl:ObjectProperty"],"rdfs:label":"flashpointTemperatureMeasurement","schema:rangeIncludes":{"@id":"unece:Measurement"},"schema:domainIncludes":{"@id":"unece:DangerousGoods"},"rdfs:comment":"An amount, size, or extent as established by measuring."},{"@id":"unece:hazardCategoryCode","@type":["rdf:Property","owl:DatatypeProperty"],"rdfs:label":"hazardCategoryCode","schema:rangeIncludes":{"@id":"schema:Text"},"schema:domainIncludes":{"@id":"unece:DangerousGoods"},"rdfs:comment":"The code specifying the hazard category for these transported dangerous goods."},{"@id":"unece:hazardClassVersionId","@type":["rdf:Property","owl:DatatypeProperty"],"rdfs:label":"hazardClassVersionId","schema:rangeIncludes":{"@id":"schema:Text"},"schema:domainIncludes":{"@id":"unece:DangerousGoods"},"rdfs:comment":"The unique identifier of the version of a hazard class for these transported dangerous goods."},{"@id":"unece:hazardClassificationId","@type":["rdf:Property","owl:DatatypeProperty"],"rdfs:label":"hazardClassificationId","schema:rangeIncludes":{"@id":"schema:Text"},"schema:domainIncludes":{"@id":"unece:DangerousGoods"},"rdfs:comment":"The unique identifier of a hazard class applicable to these transported dangerous goods as defined by the relevant governing regulation authority."},{"@id":"unece:hazardTypeCode","@type":["rdf:Property","owl:DatatypeProperty"],"rdfs:label":"hazardTypeCode","schema:rangeIncludes":{"@id":"schema:Text"},"schema:domainIncludes":{"@id":"unece:DangerousGoods"},"rdfs:comment":"A code specifying the type of hazard for these transported dangerous goods."},{"@id":"unece:iMDGSegregationGroupCode","@type":["rdf:Property","owl:DatatypeProperty"],"rdfs:label":"iMDGSegregationGroupCode","schema:rangeIncludes":{"@id":"schema:Text"},"schema:domainIncludes":{"@id":"unece:DangerousGoods"},"rdfs:comment":"The code specifying the IMDG (International Maritime Dangerous Goods regulation) segregation group for these transported dangerous goods."},{"@id":"unece:limitedQuantityCode","@type":["rdf:Property","owl:DatatypeProperty"],"rdfs:label":"limitedQuantityCode","schema:rangeIncludes":{"@id":"schema:Text"},"schema:domainIncludes":{"@id":"unece:DangerousGoods"},"rdfs:comment":"A code specifying facilitations for transport of limited quantities of these transported dangerous goods."},{"@id":"unece:lowerPartOrangeHazardPlacardId","@type":["rdf:Property","owl:DatatypeProperty"],"rdfs:label":"lowerPartOrangeHazardPlacardId","schema:rangeIncludes":{"@id":"schema:Text"},"schema:domainIncludes":{"@id":"unece:DangerousGoods"},"rdfs:comment":"The unique lower part of the orange hazard placard identifier for these transported dangerous goods."},{"@id":"unece:mFAGId","@type":["rdf:Property","owl:DatatypeProperty"],"rdfs:label":"mFAGId","schema:rangeIncludes":{"@id":"schema:Text"},"schema:domainIncludes":{"@id":"unece:DangerousGoods"},"rdfs:comment":"The unique Medical First Aid Guide (MFAG) identifier for these transported dangerous goods."},{"@id":"unece:marinePollutantIndicator","@type":["rdf:Property","owl:DatatypeProperty"],"rdfs:label":"marinePollutantIndicator","schema:rangeIncludes":{"@id":"schema:Boolean"},"schema:domainIncludes":{"@id":"unece:DangerousGoods"},"rdfs:comment":"The indication of whether or not these transported dangerous goods have a marine pollutant content."},{"@id":"unece:maritimePollutantTypeCode","@type":["rdf:Property","owl:DatatypeProperty"],"rdfs:label":"maritimePollutantTypeCode","schema:rangeIncludes":{"@id":"schema:Text"},"schema:domainIncludes":{"@id":"unece:DangerousGoods"},"rdfs:comment":"A code specifying a type of maritime pollutant for the transported dangerous goods."},{"@id":"unece:marking","@type":["rdf:Property","owl:DatatypeProperty"],"rdfs:label":"marking","schema:rangeIncludes":{"@id":"schema:Text"},"schema:domainIncludes":[{"@id":"unece:DangerousGoods"},{"@id":"unece:ShippingMarks"}],"rdfs:comment":"Marking, expressed as text, for these logistics shipping marks."},{"@id":"unece:overpackInformation","@type":["rdf:Property","owl:DatatypeProperty"],"rdfs:label":"overpackInformation","schema:rangeIncludes":{"@id":"schema:Text"},"schema:domainIncludes":{"@id":"unece:DangerousGoods"},"rdfs:comment":"Overpack information, expressed as text, for these transported dangerous goods."},{"@id":"unece:packingInstructionTypeCode","@type":["rdf:Property","owl:DatatypeProperty"],"rdfs:label":"packingInstructionTypeCode","schema:rangeIncludes":{"@id":"schema:Text"},"schema:domainIncludes":{"@id":"unece:DangerousGoods"},"rdfs:comment":"The code specifying a type of packing instruction for these transported dangerous goods."},{"@id":"unece:pollutantIndicator","@type":["rdf:Property","owl:DatatypeProperty"],"rdfs:label":"pollutantIndicator","schema:rangeIncludes":{"@id":"schema:Boolean"},"schema:domainIncludes":{"@id":"unece:DangerousGoods"},"rdfs:comment":"The indication of whether or not these transported dangerous goods have a pollutant content."},{"@id":"unece:pollutantLevelCode","@type":["rdf:Property","owl:DatatypeProperty"],"rdfs:label":"pollutantLevelCode","schema:rangeIncludes":{"@id":"schema:Text"},"schema:domainIncludes":{"@id":"unece:DangerousGoods"},"rdfs:comment":"The code specifying the level of pollution of these transported dangerous goods."},{"@id":"unece:properShippingName","@type":["rdf:Property","owl:DatatypeProperty"],"rdfs:label":"properShippingName","schema:rangeIncludes":{"@id":"schema:Text"},"schema:domainIncludes":{"@id":"unece:DangerousGoods"},"rdfs:comment":"The proper shipping name, expressed as text, for these transported dangerous goods."},{"@id":"unece:qValueNumeric","@type":["rdf:Property","owl:DatatypeProperty"],"rdfs:label":"qValueNumeric","schema:rangeIncludes":{"@id":"schema:Text"},"schema:domainIncludes":{"@id":"unece:DangerousGoods"},"rdfs:comment":"The number of the Q-Value for these transported dangerous goods."},{"@id":"unece:radioactiveIndicator","@type":["rdf:Property","owl:DatatypeProperty"],"rdfs:label":"radioactiveIndicator","schema:rangeIncludes":{"@id":"schema:Boolean"},"schema:domainIncludes":{"@id":"unece:DangerousGoods"},"rdfs:comment":"The indicator of whether or not these transported dangerous goods are radioactive."},{"@id":"unece:radioactiveMaterial","@type":["rdf:Property","owl:ObjectProperty"],"rdfs:label":"radioactiveMaterial","schema:rangeIncludes":{"@id":"unece:RadioactiveMaterial"},"schema:domainIncludes":{"@id":"unece:DangerousGoods"},"rdfs:comment":"Material capable of undergoing spontaneous nuclear decay involving emission of ionizing radiation in the form of particles or gamma rays."},{"@id":"unece:regulationName","@type":["rdf:Property","owl:DatatypeProperty"],"rdfs:label":"regulationName","schema:rangeIncludes":{"@id":"schema:Text"},"schema:domainIncludes":{"@id":"unece:DangerousGoods"},"rdfs:comment":"A name, expressed as text, for a regulation of these transported dangerous goods."},{"@id":"unece:regulatoryAuthorityName","@type":["rdf:Property","owl:DatatypeProperty"],"rdfs:label":"regulatoryAuthorityName","schema:rangeIncludes":{"@id":"schema:Text"},"schema:domainIncludes":{"@id":"unece:DangerousGoods"},"rdfs:comment":"The name, expressed as text, for the regulatory authority for these transported dangerous goods."},{"@id":"unece:relatedDocument","@type":["rdf:Property","owl:ObjectProperty"],"rdfs:label":"relatedDocument","schema:rangeIncludes":{"@id":"unece:Document"},"schema:domainIncludes":{"@id":"unece:DangerousGoods"},"rdfs:comment":"Written, printed or electronic matter that is referenced."},{"@id":"unece:reportableQuantity","@type":["rdf:Property","owl:ObjectProperty"],"rdfs:label":"reportableQuantity","schema:rangeIncludes":{"@id":"unece:QuantityType"},"schema:domainIncludes":{"@id":"unece:DangerousGoods"},"rdfs:comment":""},{"@id":"unece:shipperDeclarationInformation","@type":["rdf:Property","owl:DatatypeProperty"],"rdfs:label":"shipperDeclarationInformation","schema:rangeIncludes":{"@id":"schema:Text"},"schema:domainIncludes":{"@id":"unece:DangerousGoods"},"rdfs:comment":"Shipper declaration information, expressed as text, for these transported dangerous goods."},{"@id":"unece:specialProvisionId","@type":["rdf:Property","owl:DatatypeProperty"],"rdfs:label":"specialProvisionId","schema:rangeIncludes":{"@id":"schema:Text"},"schema:domainIncludes":{"@id":"unece:DangerousGoods"},"rdfs:comment":"The unique identifier of the special provision for these transported dangerous goods."},{"@id":"unece:statedCondition","@type":["rdf:Property","owl:ObjectProperty"],"rdfs:label":"statedCondition","schema:rangeIncludes":{"@id":"unece:SpecifiedCondition"},"schema:domainIncludes":[{"@id":"unece:DangerousGoods"},{"@id":"unece:Package"}],"rdfs:comment":"A stated condition of these transported dangerous goods."},{"@id":"unece:supplementaryInformation","@type":["rdf:Property","owl:DatatypeProperty"],"rdfs:label":"supplementaryInformation","schema:rangeIncludes":{"@id":"schema:Text"},"schema:domainIncludes":{"@id":"unece:DangerousGoods"},"rdfs:comment":"Supplementary information, expressed as text, concerning the transport of these dangerous goods."},{"@id":"unece:tREMId","@type":["rdf:Property","owl:DatatypeProperty"],"rdfs:label":"tREMId","schema:rangeIncludes":{"@id":"schema:Text"},"schema:domainIncludes":{"@id":"unece:DangerousGoods"},"rdfs:comment":"The unique TRansport EMergency (TREM) card identifier for these transported dangerous goods."},{"@id":"unece:technicalName","@type":["rdf:Property","owl:DatatypeProperty"],"rdfs:label":"technicalName","schema:rangeIncludes":{"@id":"schema:Text"},"schema:domainIncludes":{"@id":"unece:DangerousGoods"},"rdfs:comment":"A technical name, expressed as text, for these transported dangerous goods."},{"@id":"unece:temperatureUnitMeltingPointTemperatureMeasure","@type":["rdf:Property","owl:ObjectProperty"],"rdfs:label":"temperatureUnitMeltingPointTemperatureMeasure","schema:rangeIncludes":{"@id":"unece:TemperatureUnitMeasureType"},"schema:domainIncludes":{"@id":"unece:DangerousGoods"},"rdfs:comment":""},{"@id":"unece:transportDangerousGoodsPackageTypeCode","@type":["rdf:Property","owl:DatatypeProperty"],"rdfs:label":"transportDangerousGoodsPackageTypeCode","schema:rangeIncludes":{"@id":"unece:PackageTypeCodeList"},"schema:domainIncludes":{"@id":"unece:DangerousGoods"},"rdfs:comment":"The code specifying the package type for the transported dangerous goods."},{"@id":"unece:transportExpertContact","@type":["rdf:Property","owl:ObjectProperty"],"rdfs:label":"transportExpertContact","schema:rangeIncludes":{"@id":"unece:Contact"},"schema:domainIncludes":{"@id":"unece:DangerousGoods"},"rdfs:comment":"An individual human being in a position to give assistance or information."},{"@id":"unece:tunnelRestrictionCode","@type":["rdf:Property","owl:DatatypeProperty"],"rdfs:label":"tunnelRestrictionCode","schema:rangeIncludes":{"@id":"schema:Text"},"schema:domainIncludes":{"@id":"unece:DangerousGoods"},"rdfs:comment":"The code specifying the tunnel restriction for these transported dangerous goods."},{"@id":"unece:uNDGIdentificationCode","@type":["rdf:Property","owl:DatatypeProperty"],"rdfs:label":"uNDGIdentificationCode","schema:rangeIncludes":{"@id":"schema:Text"},"schema:domainIncludes":{"@id":"unece:DangerousGoods"},"rdfs:comment":"The code specifying the unique United Nations Dangerous Goods (UNDG) number assigned to these transported dangerous goods."},{"@id":"unece:upperPartOrangeHazardPlacardId","@type":["rdf:Property","owl:DatatypeProperty"],"rdfs:label":"upperPartOrangeHazardPlacardId","schema:rangeIncludes":{"@id":"schema:Text"},"schema:domainIncludes":{"@id":"unece:DangerousGoods"},"rdfs:comment":"The unique upper part of the orange hazard placard identifier for these transported dangerous goods."},{"@id":"unece:viscosityMeasure","@type":["rdf:Property","owl:ObjectProperty"],"rdfs:label":"viscosityMeasure","schema:rangeIncludes":{"@id":"unece:MeasureType"},"schema:domainIncludes":{"@id":"unece:DangerousGoods"},"rdfs:comment":""},{"@id":"unece:volumeUnitMarinePollutantVolumeMeasure","@type":["rdf:Property","owl:ObjectProperty"],"rdfs:label":"volumeUnitMarinePollutantVolumeMeasure","schema:rangeIncludes":{"@id":"unece:VolumeUnitMeasureType"},"schema:domainIncludes":{"@id":"unece:DangerousGoods"},"rdfs:comment":""},{"@id":"unece:additionalLevelCode","@type":["rdf:Property","owl:DatatypeProperty"],"rdfs:label":"additionalLevelCode","schema:rangeIncludes":{"@id":"schema:Text"},"schema:domainIncludes":{"@id":"unece:Package"},"rdfs:comment":"The code specifying the additional level of this logistics package."},{"@id":"unece:despatchNoteAssociatedDocument","@type":["rdf:Property","owl:ObjectProperty"],"rdfs:label":"despatchNoteAssociatedDocument","schema:rangeIncludes":{"@id":"unece:Document"},"schema:domainIncludes":{"@id":"unece:Package"},"rdfs:comment":"Written, printed or electronic matter that is referenced."},{"@id":"unece:nominalGrossVolumeMeasure","@type":["rdf:Property","owl:ObjectProperty"],"rdfs:label":"nominalGrossVolumeMeasure","schema:rangeIncludes":{"@id":"unece:VolumeUnitMeasureType"},"schema:domainIncludes":{"@id":"unece:Package"},"rdfs:comment":""},{"@id":"unece:nominalGrossWeightMeasure","@type":["rdf:Property","owl:ObjectProperty"],"rdfs:label":"nominalGrossWeightMeasure","schema:rangeIncludes":{"@id":"unece:WeightUnitMeasureType"},"schema:domainIncludes":{"@id":"unece:Package"},"rdfs:comment":""},{"@id":"unece:packageType","@type":["rdf:Property","owl:DatatypeProperty"],"rdfs:label":"packageType","schema:rangeIncludes":{"@id":"schema:Text"},"schema:domainIncludes":[{"@id":"unece:Package"},{"@id":"unece:Consignment"},{"@id":"unece:ConsignmentItem"}],"rdfs:comment":"A package type, expressed as text, for this supply chain consignment item."},{"@id":"unece:packageTypeCode","@type":["rdf:Property","owl:DatatypeProperty"],"rdfs:label":"packageTypeCode","schema:rangeIncludes":{"@id":"unece:PackageTypeCodeList"},"schema:domainIncludes":[{"@id":"unece:Package"},{"@id":"unece:SupplyChainPackaging"}],"rdfs:comment":"A code specifying the type of logistics package."},{"@id":"unece:packagingLevelCode","@type":["rdf:Property","owl:DatatypeProperty"],"rdfs:label":"packagingLevelCode","schema:rangeIncludes":{"@id":"unece:PackagingLevelCodeList"},"schema:domainIncludes":{"@id":"unece:Package"},"rdfs:comment":"The code specifying the level of this logistics package."},{"@id":"unece:parentId","@type":["rdf:Property","owl:DatatypeProperty"],"rdfs:label":"parentId","schema:rangeIncludes":{"@id":"schema:Text"},"schema:domainIncludes":{"@id":"unece:Package"},"rdfs:comment":"The parent identifier for this referenced logistics package."},{"@id":"unece:physicalShippingMarks","@type":["rdf:Property","owl:ObjectProperty"],"rdfs:label":"physicalShippingMarks","schema:rangeIncludes":{"@id":"unece:ShippingMarks"},"schema:domainIncludes":[{"@id":"unece:Package"},{"@id":"unece:Consignment"},{"@id":"unece:ConsignmentItem"}],"rdfs:comment":"Physical logistics shipping marks and barcode information for this referenced supply chain consignment item."},{"@id":"unece:usedPackaging","@type":["rdf:Property","owl:ObjectProperty"],"rdfs:label":"usedPackaging","schema:rangeIncludes":{"@id":"unece:SupplyChainPackaging"},"schema:domainIncludes":{"@id":"unece:Package"},"rdfs:comment":"Supply chain packaging used for this logistics package."},{"@id":"unece:administrativeMedicalPersonnelOnboardQuantity","@type":["rdf:Property","owl:ObjectProperty"],"rdfs:label":"administrativeMedicalPersonnelOnboardQuantity","schema:rangeIncludes":{"@id":"unece:QuantityType"},"schema:domainIncludes":{"@id":"unece:TransportMovement"},"rdfs:comment":""},{"@id":"unece:arrivalEvent","@type":["rdf:Property","owl:ObjectProperty"],"rdfs:label":"arrivalEvent","schema:rangeIncludes":{"@id":"unece:TransportEvent"},"schema:domainIncludes":{"@id":"unece:TransportMovement"},"rdfs:comment":"An arrival event for this logistics transport movement."},{"@id":"unece:associatedConvoy","@type":["rdf:Property","owl:ObjectProperty"],"rdfs:label":"associatedConvoy","schema:rangeIncludes":{"@id":"unece:Convoy"},"schema:domainIncludes":{"@id":"unece:TransportMovement"},"rdfs:comment":"The convoy associated with this logistics transport movement."},{"@id":"unece:borderCrossingDateTime","@type":["rdf:Property","owl:DatatypeProperty"],"rdfs:label":"borderCrossingDateTime","schema:rangeIncludes":{"@id":"schema:Text"},"schema:domainIncludes":{"@id":"unece:TransportMovement"},"rdfs:comment":"A date, time, date time or other date time value when this logistics transport movement crosses a border."},{"@id":"unece:borderCrossingEvent","@type":["rdf:Property","owl:ObjectProperty"],"rdfs:label":"borderCrossingEvent","schema:rangeIncludes":{"@id":"unece:TransportEvent"},"schema:domainIncludes":{"@id":"unece:TransportMovement"},"rdfs:comment":"A border crossing event for this logistics transport movement."},{"@id":"unece:callEvent","@type":["rdf:Property","owl:ObjectProperty"],"rdfs:label":"callEvent","schema:rangeIncludes":{"@id":"unece:TransportEvent"},"schema:domainIncludes":{"@id":"unece:TransportMovement"},"rdfs:comment":"A call event for this logistics transport movement."},{"@id":"unece:callPurposeCode","@type":["rdf:Property","owl:DatatypeProperty"],"rdfs:label":"callPurposeCode","schema:rangeIncludes":{"@id":"schema:Text"},"schema:domainIncludes":{"@id":"unece:TransportMovement"},"rdfs:comment":"A code specifying a call purpose for this logistics transport movement."},{"@id":"unece:cargoDescription","@type":["rdf:Property","owl:DatatypeProperty"],"rdfs:label":"cargoDescription","schema:rangeIncludes":{"@id":"schema:Text"},"schema:domainIncludes":{"@id":"unece:TransportMovement"},"rdfs:comment":"The textual description of the cargo for this logistics transport movement."},{"@id":"unece:carriedGoodsCharacteristic","@type":["rdf:Property","owl:ObjectProperty"],"rdfs:label":"carriedGoodsCharacteristic","schema:rangeIncludes":{"@id":"unece:GoodsCharacteristic"},"schema:domainIncludes":{"@id":"unece:TransportMovement"},"rdfs:comment":"A distinctive feature of a material contained within physical goods."},{"@id":"unece:carriedInactiveTransportMeans","@type":["rdf:Property","owl:ObjectProperty"],"rdfs:label":"carriedInactiveTransportMeans","schema:rangeIncludes":{"@id":"unece:TransportMeans"},"schema:domainIncludes":{"@id":"unece:TransportMovement"},"rdfs:comment":"Details of transport means inactively carried during the transport movement, such as trucks on a Roll-On/Roll-Off (RORO) ferry."},{"@id":"unece:carrierAgentParty","@type":["rdf:Property","owl:ObjectProperty"],"rdfs:label":"carrierAgentParty","schema:rangeIncludes":{"@id":"unece:Party"},"schema:domainIncludes":[{"@id":"unece:TransportMovement"},{"@id":"unece:Consignment"}],"rdfs:comment":""},{"@id":"unece:closingDateTime","@type":["rdf:Property","owl:DatatypeProperty"],"rdfs:label":"closingDateTime","schema:rangeIncludes":{"@id":"schema:Text"},"schema:domainIncludes":{"@id":"unece:TransportMovement"},"rdfs:comment":"The date, time, date time, or other date time value by which cargo should be loaded onto the means of transport for the departure of this logistics transport movement."},{"@id":"unece:commodityConsolidatorAgentParty","@type":["rdf:Property","owl:ObjectProperty"],"rdfs:label":"commodityConsolidatorAgentParty","schema:rangeIncludes":{"@id":"unece:Party"},"schema:domainIncludes":{"@id":"unece:TransportMovement"},"rdfs:comment":""},{"@id":"unece:commodityConsolidatorParty","@type":["rdf:Property","owl:ObjectProperty"],"rdfs:label":"commodityConsolidatorParty","schema:rangeIncludes":{"@id":"unece:Party"},"schema:domainIncludes":{"@id":"unece:TransportMovement"},"rdfs:comment":""},{"@id":"unece:consignmentQuantity","@type":["rdf:Property","owl:ObjectProperty"],"rdfs:label":"consignmentQuantity","schema:rangeIncludes":{"@id":"unece:QuantityType"},"schema:domainIncludes":{"@id":"unece:TransportMovement"},"rdfs:comment":""},{"@id":"unece:consortiumCarrierParty","@type":["rdf:Property","owl:ObjectProperty"],"rdfs:label":"consortiumCarrierParty","schema:rangeIncludes":{"@id":"unece:Party"},"schema:domainIncludes":{"@id":"unece:TransportMovement"},"rdfs:comment":""},{"@id":"unece:crewListRelatedDocument","@type":["rdf:Property","owl:ObjectProperty"],"rdfs:label":"crewListRelatedDocument","schema:rangeIncludes":{"@id":"unece:Document"},"schema:domainIncludes":{"@id":"unece:TransportMovement"},"rdfs:comment":"Written, printed or electronic matter that is referenced."},{"@id":"unece:crewNationalityCountry","@type":["rdf:Property","owl:ObjectProperty"],"rdfs:label":"crewNationalityCountry","schema:rangeIncludes":{"@id":"unece:Country"},"schema:domainIncludes":{"@id":"unece:TransportMovement"},"rdfs:comment":"The area of land that belongs to a nation together with its properties, such as population, political organization, etc., used or referenced for trade purposes."},{"@id":"unece:crewPerson","@type":["rdf:Property","owl:ObjectProperty"],"rdfs:label":"crewPerson","schema:rangeIncludes":{"@id":"unece:TransportPerson"},"schema:domainIncludes":{"@id":"unece:TransportMovement"},"rdfs:comment":"A person who is a member of the crew of the means of transport used for this logistics transport movement."},{"@id":"unece:crewPersonalEffects","@type":["rdf:Property","owl:ObjectProperty"],"rdfs:label":"crewPersonalEffects","schema:rangeIncludes":{"@id":"unece:PersonalEffects"},"schema:domainIncludes":{"@id":"unece:TransportMovement"},"rdfs:comment":"Specified privately owned articles for personal use by an individual."},{"@id":"unece:crewQuantity","@type":["rdf:Property","owl:ObjectProperty"],"rdfs:label":"crewQuantity","schema:rangeIncludes":{"@id":"unece:QuantityType"},"schema:domainIncludes":{"@id":"unece:TransportMovement"},"rdfs:comment":""},{"@id":"unece:cycle","@type":["rdf:Property","owl:DatatypeProperty"],"rdfs:label":"cycle","schema:rangeIncludes":{"@id":"schema:Text"},"schema:domainIncludes":{"@id":"unece:TransportMovement"},"rdfs:comment":"The cycle, as expressed as text, of this logistics transport movement, such as twice a day."},{"@id":"unece:damageEvent","@type":["rdf:Property","owl:ObjectProperty"],"rdfs:label":"damageEvent","schema:rangeIncludes":{"@id":"unece:TransportEvent"},"schema:domainIncludes":{"@id":"unece:TransportMovement"},"rdfs:comment":"A damage event for this logistics transport movement."},{"@id":"unece:dangerousGoodsIndicator","@type":["rdf:Property","owl:DatatypeProperty"],"rdfs:label":"dangerousGoodsIndicator","schema:rangeIncludes":{"@id":"schema:Boolean"},"schema:domainIncludes":{"@id":"unece:TransportMovement"},"rdfs:comment":"The indication of whether or not dangerous goods are carried for this logistics transport movement."},{"@id":"unece:departureEvent","@type":["rdf:Property","owl:ObjectProperty"],"rdfs:label":"departureEvent","schema:rangeIncludes":{"@id":"unece:TransportEvent"},"schema:domainIncludes":{"@id":"unece:TransportMovement"},"rdfs:comment":"A departure event during this logistics transport movement."},{"@id":"unece:documentaryInstructionsNotifiedParty","@type":["rdf:Property","owl:ObjectProperty"],"rdfs:label":"documentaryInstructionsNotifiedParty","schema:rangeIncludes":{"@id":"unece:Party"},"schema:domainIncludes":{"@id":"unece:TransportMovement"},"rdfs:comment":""},{"@id":"unece:excessTransportService","@type":["rdf:Property","owl:ObjectProperty"],"rdfs:label":"excessTransportService","schema:rangeIncludes":{"@id":"unece:Service"},"schema:domainIncludes":{"@id":"unece:TransportMovement"},"rdfs:comment":"An excess transport service for this logistics transport movement."},{"@id":"unece:firstArrivalEvent","@type":["rdf:Property","owl:ObjectProperty"],"rdfs:label":"firstArrivalEvent","schema:rangeIncludes":{"@id":"unece:TransportEvent"},"schema:domainIncludes":{"@id":"unece:TransportMovement"},"rdfs:comment":"The first arrival event for this logistics transport movement."},{"@id":"unece:iSPSRelatedDocument","@type":["rdf:Property","owl:ObjectProperty"],"rdfs:label":"iSPSRelatedDocument","schema:rangeIncludes":{"@id":"unece:Document"},"schema:domainIncludes":{"@id":"unece:TransportMovement"},"rdfs:comment":"Written, printed or electronic matter that is referenced."},{"@id":"unece:itineraryRoute","@type":["rdf:Property","owl:ObjectProperty"],"rdfs:label":"itineraryRoute","schema:rangeIncludes":{"@id":"unece:TransportRoute"},"schema:domainIncludes":{"@id":"unece:TransportMovement"},"rdfs:comment":"A route in the itinerary of this logistics transport movement."},{"@id":"unece:liftingInstructionsRelatedDocument","@type":["rdf:Property","owl:ObjectProperty"],"rdfs:label":"liftingInstructionsRelatedDocument","schema:rangeIncludes":{"@id":"unece:Document"},"schema:domainIncludes":{"@id":"unece:TransportMovement"},"rdfs:comment":"Written, printed or electronic matter that is referenced."},{"@id":"unece:loadingInspectionParty","@type":["rdf:Property","owl:ObjectProperty"],"rdfs:label":"loadingInspectionParty","schema:rangeIncludes":{"@id":"unece:Party"},"schema:domainIncludes":{"@id":"unece:TransportMovement"},"rdfs:comment":""},{"@id":"unece:loadingInspectionSpecifiedInstructions","@type":["rdf:Property","owl:ObjectProperty"],"rdfs:label":"loadingInspectionSpecifiedInstructions","schema:rangeIncludes":{"@id":"unece:TransportInstructions"},"schema:domainIncludes":{"@id":"unece:TransportMovement"},"rdfs:comment":"Transport information of an instructive nature."},{"@id":"unece:logisticsTransportMovementStatusCode","@type":["rdf:Property","owl:DatatypeProperty"],"rdfs:label":"logisticsTransportMovementStatusCode","schema:rangeIncludes":{"@id":"unece:StatusCodeList"},"schema:domainIncludes":{"@id":"unece:TransportMovement"},"rdfs:comment":"The code specifying a status for the logistics transport movement, such as estimated or final."},{"@id":"unece:manifestOnboardIndicator","@type":["rdf:Property","owl:DatatypeProperty"],"rdfs:label":"manifestOnboardIndicator","schema:rangeIncludes":{"@id":"schema:Boolean"},"schema:domainIncludes":{"@id":"unece:TransportMovement"},"rdfs:comment":"The indication of whether or not the manifest for this logistics transport movement is onboard."},{"@id":"unece:manifestRelatedDocument","@type":["rdf:Property","owl:ObjectProperty"],"rdfs:label":"manifestRelatedDocument","schema:rangeIncludes":{"@id":"unece:Document"},"schema:domainIncludes":{"@id":"unece:TransportMovement"},"rdfs:comment":"Written, printed or electronic matter that is referenced."},{"@id":"unece:masterResponsiblePerson","@type":["rdf:Property","owl:ObjectProperty"],"rdfs:label":"masterResponsiblePerson","schema:rangeIncludes":{"@id":"unece:TransportPerson"},"schema:domainIncludes":{"@id":"unece:TransportMovement"},"rdfs:comment":"The person legally responsible for the operation of the means of transport used for this logistics transport movement."},{"@id":"unece:mode","@type":["rdf:Property","owl:DatatypeProperty"],"rdfs:label":"mode","schema:rangeIncludes":{"@id":"schema:Text"},"schema:domainIncludes":{"@id":"unece:TransportMovement"},"rdfs:comment":"The mode, expressed as text, of this logistics transport movement."},{"@id":"unece:nVOCCCarrierParty","@type":["rdf:Property","owl:ObjectProperty"],"rdfs:label":"nVOCCCarrierParty","schema:rangeIncludes":{"@id":"unece:Party"},"schema:domainIncludes":{"@id":"unece:TransportMovement"},"rdfs:comment":""},{"@id":"unece:onboardInventory","@type":["rdf:Property","owl:ObjectProperty"],"rdfs:label":"onboardInventory","schema:rangeIncludes":{"@id":"unece:StoresItemInventory"},"schema:domainIncludes":{"@id":"unece:TransportMovement"},"rdfs:comment":"A stores inventory item held onboard for this logistics transport movement."},{"@id":"unece:onboardPerson","@type":["rdf:Property","owl:ObjectProperty"],"rdfs:label":"onboardPerson","schema:rangeIncludes":{"@id":"unece:TransportPerson"},"schema:domainIncludes":{"@id":"unece:TransportMovement"},"rdfs:comment":"A person onboard this logistics transport movement."},{"@id":"unece:onboardPersonQuantity","@type":["rdf:Property","owl:ObjectProperty"],"rdfs:label":"onboardPersonQuantity","schema:rangeIncludes":{"@id":"unece:QuantityType"},"schema:domainIncludes":{"@id":"unece:TransportMovement"},"rdfs:comment":""},{"@id":"unece:passengerListRelatedDocument","@type":["rdf:Property","owl:ObjectProperty"],"rdfs:label":"passengerListRelatedDocument","schema:rangeIncludes":{"@id":"unece:Document"},"schema:domainIncludes":{"@id":"unece:TransportMovement"},"rdfs:comment":"Written, printed or electronic matter that is referenced."},{"@id":"unece:passengerNationalityCountry","@type":["rdf:Property","owl:ObjectProperty"],"rdfs:label":"passengerNationalityCountry","schema:rangeIncludes":{"@id":"unece:Country"},"schema:domainIncludes":{"@id":"unece:TransportMovement"},"rdfs:comment":"The area of land that belongs to a nation together with its properties, such as population, political organization, etc., used or referenced for trade purposes."},{"@id":"unece:passengerQuantity","@type":["rdf:Property","owl:ObjectProperty"],"rdfs:label":"passengerQuantity","schema:rangeIncludes":{"@id":"unece:QuantityType"},"schema:domainIncludes":{"@id":"unece:TransportMovement"},"rdfs:comment":""},{"@id":"unece:pilotageExemptionId","@type":["rdf:Property","owl:DatatypeProperty"],"rdfs:label":"pilotageExemptionId","schema:rangeIncludes":{"@id":"schema:Text"},"schema:domainIncludes":{"@id":"unece:TransportMovement"},"rdfs:comment":"The identifier of a pilotage exemption for this logistics transport movement."},{"@id":"unece:professionalMedicalPersonnelOnboardQuantity","@type":["rdf:Property","owl:ObjectProperty"],"rdfs:label":"professionalMedicalPersonnelOnboardQuantity","schema:rangeIncludes":{"@id":"unece:QuantityType"},"schema:domainIncludes":{"@id":"unece:TransportMovement"},"rdfs:comment":""},{"@id":"unece:reportedSecurityInformation","@type":["rdf:Property","owl:DatatypeProperty"],"rdfs:label":"reportedSecurityInformation","schema:rangeIncludes":{"@id":"schema:Text"},"schema:domainIncludes":{"@id":"unece:TransportMovement"},"rdfs:comment":"Reported security information, expressed as text, for this logistics transport movement."},{"@id":"unece:reportedTransportationHealth","@type":["rdf:Property","owl:ObjectProperty"],"rdfs:label":"reportedTransportationHealth","schema:rangeIncludes":{"@id":"unece:TransportationHealth"},"schema:domainIncludes":{"@id":"unece:TransportMovement"},"rdfs:comment":"MDH (Maritime Declaration of Health) transportation health information reported for this logistics transport movement."},{"@id":"unece:reportedTransportationWasteMaterial","@type":["rdf:Property","owl:ObjectProperty"],"rdfs:label":"reportedTransportationWasteMaterial","schema:rangeIncludes":{"@id":"unece:TransportationWasteMaterial"},"schema:domainIncludes":{"@id":"unece:TransportMovement"},"rdfs:comment":"Transportation waste material reported for this logistics transport movement."},{"@id":"unece:sailingAdviceNotificationInformation","@type":["rdf:Property","owl:DatatypeProperty"],"rdfs:label":"sailingAdviceNotificationInformation","schema:rangeIncludes":{"@id":"schema:Text"},"schema:domainIncludes":{"@id":"unece:TransportMovement"},"rdfs:comment":"Sailing advice notification information, expressed as text, for this logistics transport movement."},{"@id":"unece:sailingAdviceNotifiedParty","@type":["rdf:Property","owl:ObjectProperty"],"rdfs:label":"sailingAdviceNotifiedParty","schema:rangeIncludes":{"@id":"unece:Party"},"schema:domainIncludes":{"@id":"unece:TransportMovement"},"rdfs:comment":""},{"@id":"unece:scheduledId","@type":["rdf:Property","owl:DatatypeProperty"],"rdfs:label":"scheduledId","schema:rangeIncludes":{"@id":"schema:Text"},"schema:domainIncludes":{"@id":"unece:TransportMovement"},"rdfs:comment":"A unique identifier for this logistics transport movement, such as a voyage number, flight number, or trip number, as stated in a schedule."},{"@id":"unece:service","@type":["rdf:Property","owl:DatatypeProperty"],"rdfs:label":"service","schema:rangeIncludes":{"@id":"schema:Text"},"schema:domainIncludes":{"@id":"unece:TransportMovement"},"rdfs:comment":"The service, expressed as text, of this logistics transport movement."},{"@id":"unece:serviceCode","@type":["rdf:Property","owl:DatatypeProperty"],"rdfs:label":"serviceCode","schema:rangeIncludes":{"@id":"schema:Text"},"schema:domainIncludes":{"@id":"unece:TransportMovement"},"rdfs:comment":"The code specifying the service of this logistics transport movement, such as regular, milk run or spot service."},{"@id":"unece:shipToShipEvent","@type":["rdf:Property","owl:ObjectProperty"],"rdfs:label":"shipToShipEvent","schema:rangeIncludes":{"@id":"unece:TransportEvent"},"schema:domainIncludes":{"@id":"unece:TransportMovement"},"rdfs:comment":"A ship to ship event for this logistics transport movement."},{"@id":"unece:specialSpecifiedInstructions","@type":["rdf:Property","owl:ObjectProperty"],"rdfs:label":"specialSpecifiedInstructions","schema:rangeIncludes":{"@id":"unece:TransportInstructions"},"schema:domainIncludes":{"@id":"unece:TransportMovement"},"rdfs:comment":"Transport information of an instructive nature."},{"@id":"unece:specifiedEmission","@type":["rdf:Property","owl:ObjectProperty"],"rdfs:label":"specifiedEmission","schema:rangeIncludes":{"@id":"unece:Emission"},"schema:domainIncludes":[{"@id":"unece:TransportMovement"},{"@id":"unece:LogisticsTransportMeans"}],"rdfs:comment":"A calculated emission specified for this logistics transport means."},{"@id":"unece:specifiedLogisticsStatus","@type":["rdf:Property","owl:ObjectProperty"],"rdfs:label":"specifiedLogisticsStatus","schema:rangeIncludes":{"@id":"unece:LogisticsStatus"},"schema:domainIncludes":[{"@id":"unece:TransportMovement"},{"@id":"unece:Consignment"}],"rdfs:comment":"A status specified for this logistics transport movement."},{"@id":"unece:specifiedTransportEvent","@type":["rdf:Property","owl:ObjectProperty"],"rdfs:label":"specifiedTransportEvent","schema:rangeIncludes":{"@id":"unece:TransportEvent"},"schema:domainIncludes":{"@id":"unece:TransportMovement"},"rdfs:comment":"A transport event specified for this logistics transport movement."},{"@id":"unece:stage","@type":["rdf:Property","owl:DatatypeProperty"],"rdfs:label":"stage","schema:rangeIncludes":{"@id":"schema:Text"},"schema:domainIncludes":{"@id":"unece:TransportMovement"},"rdfs:comment":"A stage, expressed as text, of this logistics transport movement."},{"@id":"unece:stayId","@type":["rdf:Property","owl:DatatypeProperty"],"rdfs:label":"stayId","schema:rangeIncludes":{"@id":"schema:Text"},"schema:domainIncludes":{"@id":"unece:TransportMovement"},"rdfs:comment":"The unique identifier of a stay in a port, airport or other place of service for this logistics transport movement."},{"@id":"unece:stevedoreParty","@type":["rdf:Property","owl:ObjectProperty"],"rdfs:label":"stevedoreParty","schema:rangeIncludes":{"@id":"unece:Party"},"schema:domainIncludes":{"@id":"unece:TransportMovement"},"rdfs:comment":""},{"@id":"unece:terminalOperatorAssignedId","@type":["rdf:Property","owl:DatatypeProperty"],"rdfs:label":"terminalOperatorAssignedId","schema:rangeIncludes":{"@id":"schema:Text"},"schema:domainIncludes":{"@id":"unece:TransportMovement"},"rdfs:comment":"A unique identifier for this logistics transport movement as assigned by a terminal operator."},{"@id":"unece:terminalOperatorParty","@type":["rdf:Property","owl:ObjectProperty"],"rdfs:label":"terminalOperatorParty","schema:rangeIncludes":{"@id":"unece:Party"},"schema:domainIncludes":{"@id":"unece:TransportMovement"},"rdfs:comment":""},{"@id":"unece:tradedParcelQuantity","@type":["rdf:Property","owl:ObjectProperty"],"rdfs:label":"tradedParcelQuantity","schema:rangeIncludes":{"@id":"unece:QuantityType"},"schema:domainIncludes":{"@id":"unece:TransportMovement"},"rdfs:comment":""},{"@id":"unece:tradingConsolidatorAssignedId","@type":["rdf:Property","owl:DatatypeProperty"],"rdfs:label":"tradingConsolidatorAssignedId","schema:rangeIncludes":{"@id":"schema:Text"},"schema:domainIncludes":{"@id":"unece:TransportMovement"},"rdfs:comment":"The unique identifier for this logistics transport movement as assigned by the trading consolidator."},{"@id":"unece:trainedMedicalPersonnelOnboardQuantity","@type":["rdf:Property","owl:ObjectProperty"],"rdfs:label":"trainedMedicalPersonnelOnboardQuantity","schema:rangeIncludes":{"@id":"unece:QuantityType"},"schema:domainIncludes":{"@id":"unece:TransportMovement"},"rdfs:comment":""},{"@id":"unece:transportContractRelatedDocument","@type":["rdf:Property","owl:ObjectProperty"],"rdfs:label":"transportContractRelatedDocument","schema:rangeIncludes":{"@id":"unece:Document"},"schema:domainIncludes":{"@id":"unece:TransportMovement"},"rdfs:comment":"Written, printed or electronic matter that is referenced."},{"@id":"unece:transportEquipmentQuantity","@type":["rdf:Property","owl:ObjectProperty"],"rdfs:label":"transportEquipmentQuantity","schema:rangeIncludes":{"@id":"unece:QuantityType"},"schema:domainIncludes":[{"@id":"unece:TransportMovement"},{"@id":"unece:Consignment"}],"rdfs:comment":""},{"@id":"unece:transportMeansDirectionTransitDirectionCode","@type":["rdf:Property","owl:DatatypeProperty"],"rdfs:label":"transportMeansDirectionTransitDirectionCode","schema:rangeIncludes":{"@id":"unece:TransportMeansDirectionCodeList"},"schema:domainIncludes":{"@id":"unece:TransportMovement"},"rdfs:comment":"The code specifying the transit direction of this logistics transport movement."},{"@id":"unece:transportMeansSecurityOfficerPerson","@type":["rdf:Property","owl:ObjectProperty"],"rdfs:label":"transportMeansSecurityOfficerPerson","schema:rangeIncludes":{"@id":"unece:TransportPerson"},"schema:domainIncludes":{"@id":"unece:TransportMovement"},"rdfs:comment":"The officer responsible for the security of the means of transport used for this logistics transport movement."},{"@id":"unece:transportMovementStageCode","@type":["rdf:Property","owl:DatatypeProperty"],"rdfs:label":"transportMovementStageCode","schema:rangeIncludes":{"@id":"unece:TransportMovementStageCodeList"},"schema:domainIncludes":{"@id":"unece:TransportMovement"},"rdfs:comment":"The code specifying the stage of this logistics transport movement."},{"@id":"unece:transportMovementType","@type":["rdf:Property","owl:DatatypeProperty"],"rdfs:label":"transportMovementType","schema:rangeIncludes":{"@id":"schema:Text"},"schema:domainIncludes":{"@id":"unece:TransportMovement"},"rdfs:comment":"The type, as expressed as text, of the logistics transport movement."},{"@id":"unece:transportWasteSpecifiedInstructions","@type":["rdf:Property","owl:ObjectProperty"],"rdfs:label":"transportWasteSpecifiedInstructions","schema:rangeIncludes":{"@id":"unece:DisposalInstructions"},"schema:domainIncludes":{"@id":"unece:TransportMovement"},"rdfs:comment":"A set of instructions detailing how to properly dispose of a material."},{"@id":"unece:transshipmentIntermediateEvent","@type":["rdf:Property","owl:ObjectProperty"],"rdfs:label":"transshipmentIntermediateEvent","schema:rangeIncludes":{"@id":"unece:TransportEvent"},"schema:domainIncludes":{"@id":"unece:TransportMovement"},"rdfs:comment":"A transshipment intermediate event during this logistics transport movement."},{"@id":"unece:unloadingInspectionParty","@type":["rdf:Property","owl:ObjectProperty"],"rdfs:label":"unloadingInspectionParty","schema:rangeIncludes":{"@id":"unece:Party"},"schema:domainIncludes":{"@id":"unece:TransportMovement"},"rdfs:comment":""},{"@id":"unece:unloadingInspectionSpecifiedInstructions","@type":["rdf:Property","owl:ObjectProperty"],"rdfs:label":"unloadingInspectionSpecifiedInstructions","schema:rangeIncludes":{"@id":"unece:TransportInstructions"},"schema:domainIncludes":{"@id":"unece:TransportMovement"},"rdfs:comment":"Transport information of an instructive nature."},{"@id":"unece:usedTransportMeans","@type":["rdf:Property","owl:ObjectProperty"],"rdfs:label":"usedTransportMeans","schema:rangeIncludes":{"@id":"unece:LogisticsTransportMeans"},"schema:domainIncludes":{"@id":"unece:TransportMovement"},"rdfs:comment":"The means of transport used for this logistics transport movement."},{"@id":"unece:affectedDistanceMeasure","@type":["rdf:Property","owl:ObjectProperty"],"rdfs:label":"affectedDistanceMeasure","schema:rangeIncludes":{"@id":"unece:LinearUnitMeasureType"},"schema:domainIncludes":{"@id":"unece:Emission"},"rdfs:comment":""},{"@id":"unece:pollutionMeasure","@type":["rdf:Property","owl:ObjectProperty"],"rdfs:label":"pollutionMeasure","schema:rangeIncludes":{"@id":"unece:MeasureType"},"schema:domainIncludes":{"@id":"unece:Emission"},"rdfs:comment":""},{"@id":"unece:weightUnitWeightMeasure","@type":["rdf:Property","owl:ObjectProperty"],"rdfs:label":"weightUnitWeightMeasure","schema:rangeIncludes":{"@id":"unece:WeightUnitMeasureType"},"schema:domainIncludes":{"@id":"unece:Emission"},"rdfs:comment":""},{"@id":"unece:tareWeightMeasure","@type":["rdf:Property","owl:ObjectProperty"],"rdfs:label":"tareWeightMeasure","schema:rangeIncludes":{"@id":"unece:MeasureType"},"schema:domainIncludes":{"@id":"unece:AssociatedTransportEquipment"},"rdfs:comment":""},{"@id":"unece:usedCapacityCode","@type":["rdf:Property","owl:DatatypeProperty"],"rdfs:label":"usedCapacityCode","schema:rangeIncludes":{"@id":"schema:Text"},"schema:domainIncludes":{"@id":"unece:AssociatedTransportEquipment"},"rdfs:comment":"The code specifying the used capacity, such as full or empty, of this associated piece of transport equipment."},{"@id":"unece:aftDraughtLevelMeasure","@type":["rdf:Property","owl:ObjectProperty"],"rdfs:label":"aftDraughtLevelMeasure","schema:rangeIncludes":{"@id":"unece:MeasureType"},"schema:domainIncludes":{"@id":"unece:LogisticsTransportMeans"},"rdfs:comment":""},{"@id":"unece:airDraughtLevelMeasure","@type":["rdf:Property","owl:ObjectProperty"],"rdfs:label":"airDraughtLevelMeasure","schema:rangeIncludes":{"@id":"unece:LinearUnitMeasureType"},"schema:domainIncludes":{"@id":"unece:LogisticsTransportMeans"},"rdfs:comment":""},{"@id":"unece:approvedSecurityPlanOnboardIndicator","@type":["rdf:Property","owl:DatatypeProperty"],"rdfs:label":"approvedSecurityPlanOnboardIndicator","schema:rangeIncludes":{"@id":"schema:Boolean"},"schema:domainIncludes":{"@id":"unece:LogisticsTransportMeans"},"rdfs:comment":"The indication of whether or not there is an approved security plan onboard this logistics transport means."},{"@id":"unece:attachedLogisticsTransportEquipment","@type":["rdf:Property","owl:ObjectProperty"],"rdfs:label":"attachedLogisticsTransportEquipment","schema:rangeIncludes":{"@id":"unece:LogisticsTransportEquipment"},"schema:domainIncludes":{"@id":"unece:LogisticsTransportMeans"},"rdfs:comment":"A piece of logistics transport equipment attached to this logistics means of transport."},{"@id":"unece:certifiedEmission","@type":["rdf:Property","owl:ObjectProperty"],"rdfs:label":"certifiedEmission","schema:rangeIncludes":{"@id":"unece:Emission"},"schema:domainIncludes":{"@id":"unece:LogisticsTransportMeans"},"rdfs:comment":"A certified level of pollution calculated for an emission from this logistics transport means."},{"@id":"unece:companySecurityOfficerPerson","@type":["rdf:Property","owl:ObjectProperty"],"rdfs:label":"companySecurityOfficerPerson","schema:rangeIncludes":{"@id":"unece:TransportPerson"},"schema:domainIncludes":{"@id":"unece:LogisticsTransportMeans"},"rdfs:comment":"A person who is a company security officer for this logistics transport means."},{"@id":"unece:conferenceCode","@type":["rdf:Property","owl:DatatypeProperty"],"rdfs:label":"conferenceCode","schema:rangeIncludes":{"@id":"schema:Text"},"schema:domainIncludes":{"@id":"unece:LogisticsTransportMeans"},"rdfs:comment":"The code specifying the conference for this logistics means of transport."},{"@id":"unece:draughtLevelMeasure","@type":["rdf:Property","owl:ObjectProperty"],"rdfs:label":"draughtLevelMeasure","schema:rangeIncludes":{"@id":"unece:MeasureType"},"schema:domainIncludes":{"@id":"unece:LogisticsTransportMeans"},"rdfs:comment":""},{"@id":"unece:driverAccompaniedIndicator","@type":["rdf:Property","owl:DatatypeProperty"],"rdfs:label":"driverAccompaniedIndicator","schema:rangeIncludes":{"@id":"schema:Boolean"},"schema:domainIncludes":[{"@id":"unece:LogisticsTransportMeans"},{"@id":"unece:TransportMeans"}],"rdfs:comment":"The indication of whether or not this logistics means of transport is accompanied by a driver."},{"@id":"unece:forwardDraughtLevelMeasure","@type":["rdf:Property","owl:ObjectProperty"],"rdfs:label":"forwardDraughtLevelMeasure","schema:rangeIncludes":{"@id":"unece:MeasureType"},"schema:domainIncludes":{"@id":"unece:LogisticsTransportMeans"},"rdfs:comment":""},{"@id":"unece:helipadIndicator","@type":["rdf:Property","owl:DatatypeProperty"],"rdfs:label":"helipadIndicator","schema:rangeIncludes":{"@id":"schema:Boolean"},"schema:domainIncludes":{"@id":"unece:LogisticsTransportMeans"},"rdfs:comment":"The indication of whether or not there is a helipad on this logistics means of transport."},{"@id":"unece:iSPSSecurityLevelCode","@type":["rdf:Property","owl:DatatypeProperty"],"rdfs:label":"iSPSSecurityLevelCode","schema:rangeIncludes":{"@id":"schema:Text"},"schema:domainIncludes":{"@id":"unece:LogisticsTransportMeans"},"rdfs:comment":"The code specifying the International Ship and Port facility Security (ISPS) level assigned to this logistics means of transport."},{"@id":"unece:iSSCDocument","@type":["rdf:Property","owl:ObjectProperty"],"rdfs:label":"iSSCDocument","schema:rangeIncludes":{"@id":"unece:Document"},"schema:domainIncludes":{"@id":"unece:LogisticsTransportMeans"},"rdfs:comment":"Written, printed or electronic matter that is referenced."},{"@id":"unece:iSSCIssuingAuthorityParty","@type":["rdf:Property","owl:ObjectProperty"],"rdfs:label":"iSSCIssuingAuthorityParty","schema:rangeIncludes":{"@id":"unece:Party"},"schema:domainIncludes":{"@id":"unece:LogisticsTransportMeans"},"rdfs:comment":""},{"@id":"unece:linearUnitLengthMeasure","@type":["rdf:Property","owl:ObjectProperty"],"rdfs:label":"linearUnitLengthMeasure","schema:rangeIncludes":{"@id":"unece:LinearUnitMeasureType"},"schema:domainIncludes":{"@id":"unece:LogisticsTransportMeans"},"rdfs:comment":""},{"@id":"unece:loadedCargoMeasure","@type":["rdf:Property","owl:ObjectProperty"],"rdfs:label":"loadedCargoMeasure","schema:rangeIncludes":{"@id":"unece:MeasureType"},"schema:domainIncludes":{"@id":"unece:LogisticsTransportMeans"},"rdfs:comment":""},{"@id":"unece:manoeuvringSpeedMeasure","@type":["rdf:Property","owl:ObjectProperty"],"rdfs:label":"manoeuvringSpeedMeasure","schema:rangeIncludes":{"@id":"unece:MeasureType"},"schema:domainIncludes":{"@id":"unece:LogisticsTransportMeans"},"rdfs:comment":""},{"@id":"unece:maritimeApplicableCertificate","@type":["rdf:Property","owl:ObjectProperty"],"rdfs:label":"maritimeApplicableCertificate","schema:rangeIncludes":{"@id":"unece:SpecifiedCertificate"},"schema:domainIncludes":{"@id":"unece:LogisticsTransportMeans"},"rdfs:comment":"A document issued by a government, public organization or association to certify a property of a person, entity, process or object."},{"@id":"unece:operatorNationalityCountry","@type":["rdf:Property","owl:ObjectProperty"],"rdfs:label":"operatorNationalityCountry","schema:rangeIncludes":{"@id":"unece:Country"},"schema:domainIncludes":{"@id":"unece:LogisticsTransportMeans"},"rdfs:comment":"The area of land that belongs to a nation together with its properties, such as population, political organization, etc., used or referenced for trade purposes."},{"@id":"unece:ownerAgentParty","@type":["rdf:Property","owl:ObjectProperty"],"rdfs:label":"ownerAgentParty","schema:rangeIncludes":{"@id":"unece:Party"},"schema:domainIncludes":{"@id":"unece:LogisticsTransportMeans"},"rdfs:comment":""},{"@id":"unece:registrationCountry","@type":["rdf:Property","owl:ObjectProperty"],"rdfs:label":"registrationCountry","schema:rangeIncludes":{"@id":"unece:Country"},"schema:domainIncludes":{"@id":"unece:LogisticsTransportMeans"},"rdfs:comment":"The area of land that belongs to a nation together with its properties, such as population, political organization, etc., used or referenced for trade purposes."},{"@id":"unece:registrationEvent","@type":["rdf:Property","owl:ObjectProperty"],"rdfs:label":"registrationEvent","schema:rangeIncludes":{"@id":"unece:TransportEvent"},"schema:domainIncludes":{"@id":"unece:LogisticsTransportMeans"},"rdfs:comment":"A registration event of this logistics transport means."},{"@id":"unece:requiredService","@type":["rdf:Property","owl:ObjectProperty"],"rdfs:label":"requiredService","schema:rangeIncludes":{"@id":"unece:Service"},"schema:domainIncludes":{"@id":"unece:LogisticsTransportMeans"},"rdfs:comment":"A transport service required for this logistics means of transport."},{"@id":"unece:sanitationControlDocument","@type":["rdf:Property","owl:ObjectProperty"],"rdfs:label":"sanitationControlDocument","schema:rangeIncludes":{"@id":"unece:Document"},"schema:domainIncludes":{"@id":"unece:LogisticsTransportMeans"},"rdfs:comment":"Written, printed or electronic matter that is referenced."},{"@id":"unece:sanitationControlReInspectionRequiredIndicator","@type":["rdf:Property","owl:DatatypeProperty"],"rdfs:label":"sanitationControlReInspectionRequiredIndicator","schema:rangeIncludes":{"@id":"schema:Boolean"},"schema:domainIncludes":{"@id":"unece:LogisticsTransportMeans"},"rdfs:comment":"The indication of whether or not a Sanitation Control Exemption or Certificate re-inspection is required for this logistics transport means."},{"@id":"unece:serviceProviderParty","@type":["rdf:Property","owl:ObjectProperty"],"rdfs:label":"serviceProviderParty","schema:rangeIncludes":{"@id":"unece:Party"},"schema:domainIncludes":{"@id":"unece:LogisticsTransportMeans"},"rdfs:comment":""},{"@id":"unece:specifiedDimension","@type":["rdf:Property","owl:ObjectProperty"],"rdfs:label":"specifiedDimension","schema:rangeIncludes":{"@id":"unece:SpatialDimension"},"schema:domainIncludes":{"@id":"unece:LogisticsTransportMeans"},"rdfs:comment":"A measure of spatial extent of an object, such as the length, breadth or height of a shipping container."},{"@id":"unece:specifiedFault","@type":["rdf:Property","owl:ObjectProperty"],"rdfs:label":"specifiedFault","schema:rangeIncludes":{"@id":"unece:IdentifiedFault"},"schema:domainIncludes":{"@id":"unece:LogisticsTransportMeans"},"rdfs:comment":"An identified defect or fault."},{"@id":"unece:transportMeansType","@type":["rdf:Property","owl:DatatypeProperty"],"rdfs:label":"transportMeansType","schema:rangeIncludes":{"@id":"schema:Text"},"schema:domainIncludes":[{"@id":"unece:LogisticsTransportMeans"},{"@id":"unece:TransportMeans"}],"rdfs:comment":"The type, expressed as text, of this logistics means of transport."},{"@id":"unece:transportMeansTypeCode","@type":["rdf:Property","owl:DatatypeProperty"],"rdfs:label":"transportMeansTypeCode","schema:rangeIncludes":{"@id":"unece:TransportMeansTypeCodeList"},"schema:domainIncludes":[{"@id":"unece:LogisticsTransportMeans"},{"@id":"unece:TransportMeans"}],"rdfs:comment":"The code specifying the type of logistics means of transport (Reference UNECE Recommendation 28)."},{"@id":"unece:validSanitationControlIndicator","@type":["rdf:Property","owl:DatatypeProperty"],"rdfs:label":"validSanitationControlIndicator","schema:rangeIncludes":{"@id":"schema:Boolean"},"schema:domainIncludes":{"@id":"unece:LogisticsTransportMeans"},"rdfs:comment":"The indication of whether or not there is a valid Sanitation Control Exemption or Certificate onboard this logistics transport means."},{"@id":"unece:wasteReportingExemptionIndicator","@type":["rdf:Property","owl:DatatypeProperty"],"rdfs:label":"wasteReportingExemptionIndicator","schema:rangeIncludes":{"@id":"schema:Boolean"},"schema:domainIncludes":{"@id":"unece:LogisticsTransportMeans"},"rdfs:comment":"The indication of whether or not there is a waste reporting exemption for this logistics means of transport."},{"@id":"unece:weightUnitCargoGrossWeightMeasure","@type":["rdf:Property","owl:ObjectProperty"],"rdfs:label":"weightUnitCargoGrossWeightMeasure","schema:rangeIncludes":{"@id":"unece:WeightUnitMeasureType"},"schema:domainIncludes":{"@id":"unece:LogisticsTransportMeans"},"rdfs:comment":""},{"@id":"unece:weightUnitDeadweightTonnageMeasure","@type":["rdf:Property","owl:ObjectProperty"],"rdfs:label":"weightUnitDeadweightTonnageMeasure","schema:rangeIncludes":{"@id":"unece:WeightUnitMeasureType"},"schema:domainIncludes":{"@id":"unece:LogisticsTransportMeans"},"rdfs:comment":""},{"@id":"unece:allowanceCharge","@type":["rdf:Property","owl:DatatypeProperty"],"rdfs:label":"allowanceCharge","schema:rangeIncludes":{"@id":"schema:Text"},"schema:domainIncludes":{"@id":"unece:ServiceCharge"},"rdfs:comment":"The allowance or charge, expressed as text, for this logistics service charge."},{"@id":"unece:appliedAmount","@type":["rdf:Property","owl:ObjectProperty"],"rdfs:label":"appliedAmount","schema:rangeIncludes":{"@id":"unece:AmountType"},"schema:domainIncludes":{"@id":"unece:ServiceCharge"},"rdfs:comment":""},{"@id":"unece:appliedFromLocation","@type":["rdf:Property","owl:ObjectProperty"],"rdfs:label":"appliedFromLocation","schema:rangeIncludes":{"@id":"unece:LogisticsLocation"},"schema:domainIncludes":{"@id":"unece:ServiceCharge"},"rdfs:comment":"The start location from which this logistics service charge should be applied."},{"@id":"unece:appliedTax","@type":["rdf:Property","owl:ObjectProperty"],"rdfs:label":"appliedTax","schema:rangeIncludes":{"@id":"unece:Tax"},"schema:domainIncludes":{"@id":"unece:ServiceCharge"},"rdfs:comment":"A trade related fiscal levy or duty."},{"@id":"unece:appliedToLocation","@type":["rdf:Property","owl:ObjectProperty"],"rdfs:label":"appliedToLocation","schema:rangeIncludes":{"@id":"unece:LogisticsLocation"},"schema:domainIncludes":{"@id":"unece:ServiceCharge"},"rdfs:comment":"The end location at which this logistics service charge is no longer to be applied."},{"@id":"unece:calculationBasis","@type":["rdf:Property","owl:DatatypeProperty"],"rdfs:label":"calculationBasis","schema:rangeIncludes":{"@id":"schema:Text"},"schema:domainIncludes":{"@id":"unece:ServiceCharge"},"rdfs:comment":"The basis, expressed as text, on which this logistics service charge is to be calculated, such as by volume or per unit."},{"@id":"unece:calculationBasisPrice","@type":["rdf:Property","owl:ObjectProperty"],"rdfs:label":"calculationBasisPrice","schema:rangeIncludes":{"@id":"unece:TradePrice"},"schema:domainIncludes":{"@id":"unece:ServiceCharge"},"rdfs:comment":"A sum of money for which something is or may be bought or sold for trade purposes."},{"@id":"unece:chargeCategoryCode","@type":["rdf:Property","owl:DatatypeProperty"],"rdfs:label":"chargeCategoryCode","schema:rangeIncludes":{"@id":"schema:Text"},"schema:domainIncludes":{"@id":"unece:ServiceCharge"},"rdfs:comment":"The code specifying the category of charge for this logistics service charge."},{"@id":"unece:chargePayingPartyRoleCode","@type":["rdf:Property","owl:DatatypeProperty"],"rdfs:label":"chargePayingPartyRoleCode","schema:rangeIncludes":{"@id":"unece:ChargePayingPartyRoleCodeList"},"schema:domainIncludes":{"@id":"unece:ServiceCharge"},"rdfs:comment":"The code specifying the role of the party responsible for paying this logistics service charge."},{"@id":"unece:disbursementAmount","@type":["rdf:Property","owl:ObjectProperty"],"rdfs:label":"disbursementAmount","schema:rangeIncludes":{"@id":"unece:AmountType"},"schema:domainIncludes":{"@id":"unece:ServiceCharge"},"rdfs:comment":""},{"@id":"unece:freightChargeTariffClassCode","@type":["rdf:Property","owl:DatatypeProperty"],"rdfs:label":"freightChargeTariffClassCode","schema:rangeIncludes":{"@id":"unece:FreightChargeTariffClassCodeList"},"schema:domainIncludes":{"@id":"unece:ServiceCharge"},"rdfs:comment":"The code specifying the tariff class for this logistics service charge which represents an entry in a table of fixed charges [Reference United Nations Code List (UNCL) 5243]."},{"@id":"unece:freightChargeTypeId","@type":["rdf:Property","owl:DatatypeProperty"],"rdfs:label":"freightChargeTypeId","schema:rangeIncludes":{"@id":"unece:FreightChargeTypeId"},"schema:domainIncludes":{"@id":"unece:ServiceCharge"},"rdfs:comment":"The unique identifier for this logistics service charge."},{"@id":"unece:freightInvoiceTypeCode","@type":["rdf:Property","owl:DatatypeProperty"],"rdfs:label":"freightInvoiceTypeCode","schema:rangeIncludes":{"@id":"schema:Text"},"schema:domainIncludes":{"@id":"unece:ServiceCharge"},"rdfs:comment":"A code specifying a type of freight invoice of this logistics service charge."},{"@id":"unece:logisticsChargeCalculationBasisCalculationBasisCode","@type":["rdf:Property","owl:DatatypeProperty"],"rdfs:label":"logisticsChargeCalculationBasisCalculationBasisCode","schema:rangeIncludes":{"@id":"unece:LogisticsChargeCalculationBasisCodeList"},"schema:domainIncludes":{"@id":"unece:ServiceCharge"},"rdfs:comment":"The code specifying a basis on which this logistics service charge is to be calculated, such as by volume or per unit."},{"@id":"unece:logisticsServiceChargeTransportPaymentMethodCode","@type":["rdf:Property","owl:DatatypeProperty"],"rdfs:label":"logisticsServiceChargeTransportPaymentMethodCode","schema:rangeIncludes":{"@id":"schema:Text"},"schema:domainIncludes":{"@id":"unece:ServiceCharge"},"rdfs:comment":"The code specifying the transport payment method for this logistics service charge."},{"@id":"unece:paymentPlaceLocation","@type":["rdf:Property","owl:ObjectProperty"],"rdfs:label":"paymentPlaceLocation","schema:rangeIncludes":{"@id":"unece:LogisticsLocation"},"schema:domainIncludes":{"@id":"unece:ServiceCharge"},"rdfs:comment":"The location of the place of payment of this logistics service charge."},{"@id":"unece:serviceCategoryCode","@type":["rdf:Property","owl:DatatypeProperty"],"rdfs:label":"serviceCategoryCode","schema:rangeIncludes":{"@id":"schema:Text"},"schema:domainIncludes":{"@id":"unece:ServiceCharge"},"rdfs:comment":"The code specifying the category of service for this logistics service charge."},{"@id":"unece:transportServiceCategoryCode","@type":["rdf:Property","owl:DatatypeProperty"],"rdfs:label":"transportServiceCategoryCode","schema:rangeIncludes":{"@id":"unece:TransportServiceCategoryCodeList"},"schema:domainIncludes":{"@id":"unece:ServiceCharge"},"rdfs:comment":"The code specifying the category of this logistics service charge [Reference United Nations Code List (UNCL) 5237]."},{"@id":"unece:applicableAllowanceCharge","@type":["rdf:Property","owl:ObjectProperty"],"rdfs:label":"applicableAllowanceCharge","schema:rangeIncludes":{"@id":"unece:TradeAllowanceCharge"},"schema:domainIncludes":{"@id":"unece:Consignment"},"rdfs:comment":"A component of pricing, such as an allowance or charge for trade purposes."},{"@id":"unece:applicableCargoInsurance","@type":["rdf:Property","owl:ObjectProperty"],"rdfs:label":"applicableCargoInsurance","schema:rangeIncludes":{"@id":"unece:CargoInsurance"},"schema:domainIncludes":{"@id":"unece:Consignment"},"rdfs:comment":"The cargo insurance applicable to this supply chain consignment."},{"@id":"unece:associatedInvoiceAmount","@type":["rdf:Property","owl:ObjectProperty"],"rdfs:label":"associatedInvoiceAmount","schema:rangeIncludes":{"@id":"unece:AmountType"},"schema:domainIncludes":{"@id":"unece:Consignment"},"rdfs:comment":""},{"@id":"unece:associatedInvoiceDiscountAmount","@type":["rdf:Property","owl:ObjectProperty"],"rdfs:label":"associatedInvoiceDiscountAmount","schema:rangeIncludes":{"@id":"unece:AmountType"},"schema:domainIncludes":{"@id":"unece:Consignment"},"rdfs:comment":""},{"@id":"unece:associatedInvoiceDiscountPercent","@type":["rdf:Property","owl:DatatypeProperty"],"rdfs:label":"associatedInvoiceDiscountPercent","schema:rangeIncludes":{"@id":"schema:Text"},"schema:domainIncludes":{"@id":"unece:Consignment"},"rdfs:comment":"A percent that is a discount on an invoice amount associated with this supply chain consignment."},{"@id":"unece:atArrivalTransportMovement","@type":["rdf:Property","owl:ObjectProperty"],"rdfs:label":"atArrivalTransportMovement","schema:rangeIncludes":{"@id":"unece:TransportMovement"},"schema:domainIncludes":{"@id":"unece:Consignment"},"rdfs:comment":"The logistics transport movement for this supply chain consignment at the point when the means of transport arrives in a country or at a regional border."},{"@id":"unece:atDepartureTransportMovement","@type":["rdf:Property","owl:ObjectProperty"],"rdfs:label":"atDepartureTransportMovement","schema:rangeIncludes":{"@id":"unece:TransportMovement"},"schema:domainIncludes":{"@id":"unece:Consignment"},"rdfs:comment":"The logistics transport movement for this supply chain consignment at the point when the means of transport departs a country or regional border."},{"@id":"unece:availabilityDueDateTime","@type":["rdf:Property","owl:DatatypeProperty"],"rdfs:label":"availabilityDueDateTime","schema:rangeIncludes":{"@id":"schema:Text"},"schema:domainIncludes":{"@id":"unece:Consignment"},"rdfs:comment":"The date, time, date time or other date time value when this supply chain consignment is due to be available."},{"@id":"unece:borderCrossingTransportMovement","@type":["rdf:Property","owl:ObjectProperty"],"rdfs:label":"borderCrossingTransportMovement","schema:rangeIncludes":{"@id":"unece:TransportMovement"},"schema:domainIncludes":{"@id":"unece:Consignment"},"rdfs:comment":"A border crossing logistics transport movement for this supply chain consignment."},{"@id":"unece:cODAmount","@type":["rdf:Property","owl:ObjectProperty"],"rdfs:label":"cODAmount","schema:rangeIncludes":{"@id":"unece:AmountType"},"schema:domainIncludes":{"@id":"unece:Consignment"},"rdfs:comment":""},{"@id":"unece:cargoInsuranceInstructionsInformation","@type":["rdf:Property","owl:DatatypeProperty"],"rdfs:label":"cargoInsuranceInstructionsInformation","schema:rangeIncludes":{"@id":"schema:Text"},"schema:domainIncludes":{"@id":"unece:Consignment"},"rdfs:comment":"Cargo insurance instructions, expressed as text, for this supply chain consignment."},{"@id":"unece:cargoToleranceInformation","@type":["rdf:Property","owl:DatatypeProperty"],"rdfs:label":"cargoToleranceInformation","schema:rangeIncludes":{"@id":"schema:Text"},"schema:domainIncludes":[{"@id":"unece:Consignment"},{"@id":"unece:ConsignmentItem"}],"rdfs:comment":"Cargo tolerance information, expressed as text, for this supply chain consignment item."},{"@id":"unece:carrierAcceptanceDateTime","@type":["rdf:Property","owl:DatatypeProperty"],"rdfs:label":"carrierAcceptanceDateTime","schema:rangeIncludes":{"@id":"schema:Text"},"schema:domainIncludes":{"@id":"unece:Consignment"},"rdfs:comment":"The date, time, date time or other date time value when this referenced supply chain consignment will be, or has been, accepted by the carrier."},{"@id":"unece:carrierAcceptanceLocation","@type":["rdf:Property","owl:ObjectProperty"],"rdfs:label":"carrierAcceptanceLocation","schema:rangeIncludes":{"@id":"unece:LogisticsLocation"},"schema:domainIncludes":{"@id":"unece:Consignment"},"rdfs:comment":"The location where this referenced supply chain consignment will be or has been accepted by the carrier."},{"@id":"unece:carrierAssignedId","@type":["rdf:Property","owl:DatatypeProperty"],"rdfs:label":"carrierAssignedId","schema:rangeIncludes":{"@id":"schema:Text"},"schema:domainIncludes":{"@id":"unece:Consignment"},"rdfs:comment":"The unique identifier assigned by the carrier to this referenced supply chain consignment, such as a booking reference number when cargo space is reserved prior to loading."},{"@id":"unece:carrierProvidedInformation","@type":["rdf:Property","owl:DatatypeProperty"],"rdfs:label":"carrierProvidedInformation","schema:rangeIncludes":{"@id":"schema:Text"},"schema:domainIncludes":{"@id":"unece:Consignment"},"rdfs:comment":"Information, expressed as text, provided by the carrier for this supply chain consignment."},{"@id":"unece:chargeableTransportationStageQuantity","@type":["rdf:Property","owl:ObjectProperty"],"rdfs:label":"chargeableTransportationStageQuantity","schema:rangeIncludes":{"@id":"unece:QuantityType"},"schema:domainIncludes":{"@id":"unece:Consignment"},"rdfs:comment":""},{"@id":"unece:connectingCarrierParty","@type":["rdf:Property","owl:ObjectProperty"],"rdfs:label":"connectingCarrierParty","schema:rangeIncludes":{"@id":"unece:Party"},"schema:domainIncludes":{"@id":"unece:Consignment"},"rdfs:comment":""},{"@id":"unece:consigneeAgentParty","@type":["rdf:Property","owl:ObjectProperty"],"rdfs:label":"consigneeAgentParty","schema:rangeIncludes":{"@id":"unece:Party"},"schema:domainIncludes":{"@id":"unece:Consignment"},"rdfs:comment":""},{"@id":"unece:consigneeAssignedId","@type":["rdf:Property","owl:DatatypeProperty"],"rdfs:label":"consigneeAssignedId","schema:rangeIncludes":{"@id":"schema:Text"},"schema:domainIncludes":{"@id":"unece:Consignment"},"rdfs:comment":"The unique identifier assigned by the consignee to this referenced supply chain consignment."},{"@id":"unece:consigneeParty","@type":["rdf:Property","owl:ObjectProperty"],"rdfs:label":"consigneeParty","schema:rangeIncludes":{"@id":"unece:Party"},"schema:domainIncludes":{"@id":"unece:Consignment"},"rdfs:comment":""},{"@id":"unece:consigneeReceiptLocation","@type":["rdf:Property","owl:ObjectProperty"],"rdfs:label":"consigneeReceiptLocation","schema:rangeIncludes":{"@id":"unece:LogisticsLocation"},"schema:domainIncludes":{"@id":"unece:Consignment"},"rdfs:comment":"The location at which this supply chain consignment will be or has been received by the consignee."},{"@id":"unece:consignmentItemQuantity","@type":["rdf:Property","owl:ObjectProperty"],"rdfs:label":"consignmentItemQuantity","schema:rangeIncludes":{"@id":"unece:QuantityType"},"schema:domainIncludes":{"@id":"unece:Consignment"},"rdfs:comment":""},{"@id":"unece:consignorAgentParty","@type":["rdf:Property","owl:ObjectProperty"],"rdfs:label":"consignorAgentParty","schema:rangeIncludes":{"@id":"unece:Party"},"schema:domainIncludes":{"@id":"unece:Consignment"},"rdfs:comment":""},{"@id":"unece:consignorAssignedId","@type":["rdf:Property","owl:DatatypeProperty"],"rdfs:label":"consignorAssignedId","schema:rangeIncludes":{"@id":"schema:Text"},"schema:domainIncludes":{"@id":"unece:Consignment"},"rdfs:comment":"The unique identifier assigned by the consignor to this referenced supply chain consignment."},{"@id":"unece:consignorParty","@type":["rdf:Property","owl:ObjectProperty"],"rdfs:label":"consignorParty","schema:rangeIncludes":{"@id":"unece:Party"},"schema:domainIncludes":{"@id":"unece:Consignment"},"rdfs:comment":""},{"@id":"unece:consignorProvidedBorderClearanceInstructions","@type":["rdf:Property","owl:ObjectProperty"],"rdfs:label":"consignorProvidedBorderClearanceInstructions","schema:rangeIncludes":{"@id":"unece:TransportInstructions"},"schema:domainIncludes":{"@id":"unece:Consignment"},"rdfs:comment":"Transport information of an instructive nature."},{"@id":"unece:consignorProvidedInformation","@type":["rdf:Property","owl:DatatypeProperty"],"rdfs:label":"consignorProvidedInformation","schema:rangeIncludes":{"@id":"schema:Text"},"schema:domainIncludes":{"@id":"unece:Consignment"},"rdfs:comment":"Information, expressed as text, provided by the consignor for this supply chain consignment."},{"@id":"unece:consolidatorParty","@type":["rdf:Property","owl:ObjectProperty"],"rdfs:label":"consolidatorParty","schema:rangeIncludes":{"@id":"unece:Party"},"schema:domainIncludes":{"@id":"unece:Consignment"},"rdfs:comment":""},{"@id":"unece:containerizationIndicator","@type":["rdf:Property","owl:DatatypeProperty"],"rdfs:label":"containerizationIndicator","schema:rangeIncludes":{"@id":"schema:Boolean"},"schema:domainIncludes":{"@id":"unece:Consignment"},"rdfs:comment":"The indication of whether or not this supply chain consignment is to be transported in a container or containers."},{"@id":"unece:contractTermsInformation","@type":["rdf:Property","owl:DatatypeProperty"],"rdfs:label":"contractTermsInformation","schema:rangeIncludes":{"@id":"schema:Text"},"schema:domainIncludes":{"@id":"unece:Consignment"},"rdfs:comment":"Information related to contract terms and conditions, expressed as text, for this supply chain consignment."},{"@id":"unece:currencyServiceChargeCurrencyCode","@type":["rdf:Property","owl:DatatypeProperty"],"rdfs:label":"currencyServiceChargeCurrencyCode","schema:rangeIncludes":{"@id":"unece:CurrencyCodeList"},"schema:domainIncludes":{"@id":"unece:Consignment"},"rdfs:comment":"A code specifying a service charge currency for this supply chain consignment."},{"@id":"unece:customsExportAgentParty","@type":["rdf:Property","owl:ObjectProperty"],"rdfs:label":"customsExportAgentParty","schema:rangeIncludes":{"@id":"unece:Party"},"schema:domainIncludes":{"@id":"unece:Consignment"},"rdfs:comment":""},{"@id":"unece:customsImportAgentParty","@type":["rdf:Property","owl:ObjectProperty"],"rdfs:label":"customsImportAgentParty","schema:rangeIncludes":{"@id":"unece:Party"},"schema:domainIncludes":{"@id":"unece:Consignment"},"rdfs:comment":""},{"@id":"unece:customsRequiredInvoiceDocument","@type":["rdf:Property","owl:ObjectProperty"],"rdfs:label":"customsRequiredInvoiceDocument","schema:rangeIncludes":{"@id":"unece:Document"},"schema:domainIncludes":{"@id":"unece:Consignment"},"rdfs:comment":"Written, printed or electronic matter that is referenced."},{"@id":"unece:customsTransitAgentParty","@type":["rdf:Property","owl:ObjectProperty"],"rdfs:label":"customsTransitAgentParty","schema:rangeIncludes":{"@id":"unece:Party"},"schema:domainIncludes":{"@id":"unece:Consignment"},"rdfs:comment":""},{"@id":"unece:dangerousGoodsNotifierParty","@type":["rdf:Property","owl:ObjectProperty"],"rdfs:label":"dangerousGoodsNotifierParty","schema:rangeIncludes":{"@id":"unece:Party"},"schema:domainIncludes":{"@id":"unece:Consignment"},"rdfs:comment":""},{"@id":"unece:declaredForCustomsLocation","@type":["rdf:Property","owl:ObjectProperty"],"rdfs:label":"declaredForCustomsLocation","schema:rangeIncludes":{"@id":"unece:LogisticsLocation"},"schema:domainIncludes":[{"@id":"unece:Consignment"},{"@id":"unece:ConsignmentItem"}],"rdfs:comment":"The location of this supply chain consignment as declared for customs."},{"@id":"unece:declaredValueForCarriageAmount","@type":["rdf:Property","owl:ObjectProperty"],"rdfs:label":"declaredValueForCarriageAmount","schema:rangeIncludes":{"@id":"unece:AmountType"},"schema:domainIncludes":[{"@id":"unece:Consignment"},{"@id":"unece:ConsignmentItem"}],"rdfs:comment":""},{"@id":"unece:declaredValueForCustomsAmount","@type":["rdf:Property","owl:ObjectProperty"],"rdfs:label":"declaredValueForCustomsAmount","schema:rangeIncludes":{"@id":"unece:AmountType"},"schema:domainIncludes":[{"@id":"unece:Consignment"},{"@id":"unece:ConsignmentItem"}],"rdfs:comment":""},{"@id":"unece:deconsolidatorParty","@type":["rdf:Property","owl:ObjectProperty"],"rdfs:label":"deconsolidatorParty","schema:rangeIncludes":{"@id":"unece:Party"},"schema:domainIncludes":{"@id":"unece:Consignment"},"rdfs:comment":""},{"@id":"unece:deliveryInformation","@type":["rdf:Property","owl:DatatypeProperty"],"rdfs:label":"deliveryInformation","schema:rangeIncludes":{"@id":"schema:Text"},"schema:domainIncludes":{"@id":"unece:Consignment"},"rdfs:comment":"The delivery information, expressed as text, for this supply chain consignment."},{"@id":"unece:deliveryParty","@type":["rdf:Property","owl:ObjectProperty"],"rdfs:label":"deliveryParty","schema:rangeIncludes":{"@id":"unece:Party"},"schema:domainIncludes":[{"@id":"unece:Consignment"},{"@id":"unece:ConsignmentItem"}],"rdfs:comment":""},{"@id":"unece:demurrageInformation","@type":["rdf:Property","owl:DatatypeProperty"],"rdfs:label":"demurrageInformation","schema:rangeIncludes":{"@id":"schema:Text"},"schema:domainIncludes":{"@id":"unece:Consignment"},"rdfs:comment":"Demurrage information, expressed as text, for this supply chain consignment."},{"@id":"unece:despatchParty","@type":["rdf:Property","owl:ObjectProperty"],"rdfs:label":"despatchParty","schema:rangeIncludes":{"@id":"unece:Party"},"schema:domainIncludes":[{"@id":"unece:Consignment"},{"@id":"unece:ConsignmentItem"}],"rdfs:comment":""},{"@id":"unece:destinationCountry","@type":["rdf:Property","owl:ObjectProperty"],"rdfs:label":"destinationCountry","schema:rangeIncludes":{"@id":"unece:Country"},"schema:domainIncludes":[{"@id":"unece:Consignment"},{"@id":"unece:ConsignmentItem"}],"rdfs:comment":"The area of land that belongs to a nation together with its properties, such as population, political organization, etc., used or referenced for trade purposes."},{"@id":"unece:devanningEvent","@type":["rdf:Property","owl:ObjectProperty"],"rdfs:label":"devanningEvent","schema:rangeIncludes":{"@id":"unece:TransportEvent"},"schema:domainIncludes":{"@id":"unece:Consignment"},"rdfs:comment":"A transport devanning event for this referenced supply chain consignment, i.e. the unloading of this consignment at the place of delivery."},{"@id":"unece:estimatedApplicableServiceCharge","@type":["rdf:Property","owl:ObjectProperty"],"rdfs:label":"estimatedApplicableServiceCharge","schema:rangeIncludes":{"@id":"unece:ServiceCharge"},"schema:domainIncludes":{"@id":"unece:Consignment"},"rdfs:comment":"An estimated logistics service charge applicable to this supply chain consignment, such as freight or insurance charges."},{"@id":"unece:exportCountry","@type":["rdf:Property","owl:ObjectProperty"],"rdfs:label":"exportCountry","schema:rangeIncludes":{"@id":"unece:Country"},"schema:domainIncludes":[{"@id":"unece:Consignment"},{"@id":"unece:ConsignmentItem"}],"rdfs:comment":"The area of land that belongs to a nation together with its properties, such as population, political organization, etc., used or referenced for trade purposes."},{"@id":"unece:exportExitDateTime","@type":["rdf:Property","owl:DatatypeProperty"],"rdfs:label":"exportExitDateTime","schema:rangeIncludes":{"@id":"schema:Text"},"schema:domainIncludes":{"@id":"unece:Consignment"},"rdfs:comment":"The date, time, date time or other date time value when this supply chain consignment will exit, or has exited from the last port, airport, or border post of the country of export."},{"@id":"unece:exportGeopoliticalRegion","@type":["rdf:Property","owl:ObjectProperty"],"rdfs:label":"exportGeopoliticalRegion","schema:rangeIncludes":{"@id":"unece:GeopoliticalRegion"},"schema:domainIncludes":[{"@id":"unece:Consignment"},{"@id":"unece:ConsignmentItem"}],"rdfs:comment":"A collection of countries and/or economies united for trade purposes."},{"@id":"unece:exporterParty","@type":["rdf:Property","owl:ObjectProperty"],"rdfs:label":"exporterParty","schema:rangeIncludes":{"@id":"unece:Party"},"schema:domainIncludes":{"@id":"unece:Consignment"},"rdfs:comment":""},{"@id":"unece:fOBAmount","@type":["rdf:Property","owl:ObjectProperty"],"rdfs:label":"fOBAmount","schema:rangeIncludes":{"@id":"unece:AmountType"},"schema:domainIncludes":[{"@id":"unece:Consignment"},{"@id":"unece:ConsignmentItem"}],"rdfs:comment":""},{"@id":"unece:finalDestinationLocation","@type":["rdf:Property","owl:ObjectProperty"],"rdfs:label":"finalDestinationLocation","schema:rangeIncludes":{"@id":"unece:LogisticsLocation"},"schema:domainIncludes":{"@id":"unece:Consignment"},"rdfs:comment":"The final destination location for this supply chain consignment."},{"@id":"unece:freightForwarderAssignedId","@type":["rdf:Property","owl:DatatypeProperty"],"rdfs:label":"freightForwarderAssignedId","schema:rangeIncludes":{"@id":"schema:Text"},"schema:domainIncludes":{"@id":"unece:Consignment"},"rdfs:comment":"The unique identifier assigned by the freight forwarder to this referenced supply chain consignment."},{"@id":"unece:goodsReleaseRestriction","@type":["rdf:Property","owl:DatatypeProperty"],"rdfs:label":"goodsReleaseRestriction","schema:rangeIncludes":{"@id":"schema:Text"},"schema:domainIncludes":{"@id":"unece:Consignment"},"rdfs:comment":"A goods release restriction, expressed as text, for this supply chain consignment."},{"@id":"unece:groupingCentreParty","@type":["rdf:Property","owl:ObjectProperty"],"rdfs:label":"groupingCentreParty","schema:rangeIncludes":{"@id":"unece:Party"},"schema:domainIncludes":{"@id":"unece:Consignment"},"rdfs:comment":""},{"@id":"unece:haulageInstructions","@type":["rdf:Property","owl:ObjectProperty"],"rdfs:label":"haulageInstructions","schema:rangeIncludes":{"@id":"unece:HaulageInstructions"},"schema:domainIncludes":{"@id":"unece:Consignment"},"rdfs:comment":"Haulage instructions for this supply chain consignment."},{"@id":"unece:importCountry","@type":["rdf:Property","owl:ObjectProperty"],"rdfs:label":"importCountry","schema:rangeIncludes":{"@id":"unece:Country"},"schema:domainIncludes":{"@id":"unece:Consignment"},"rdfs:comment":"The area of land that belongs to a nation together with its properties, such as population, political organization, etc., used or referenced for trade purposes."},{"@id":"unece:importerParty","@type":["rdf:Property","owl:ObjectProperty"],"rdfs:label":"importerParty","schema:rangeIncludes":{"@id":"unece:Party"},"schema:domainIncludes":{"@id":"unece:Consignment"},"rdfs:comment":""},{"@id":"unece:includedConsignment","@type":["rdf:Property","owl:ObjectProperty"],"rdfs:label":"includedConsignment","schema:rangeIncludes":{"@id":"unece:Consignment"},"schema:domainIncludes":{"@id":"unece:Consignment"},"rdfs:comment":"A referenced consignment included in this supply chain consignment."},{"@id":"unece:includedConsignmentItem","@type":["rdf:Property","owl:ObjectProperty"],"rdfs:label":"includedConsignmentItem","schema:rangeIncludes":{"@id":"unece:ConsignmentItem"},"schema:domainIncludes":{"@id":"unece:Consignment"},"rdfs:comment":"A consignment item included in this supply chain consignment."},{"@id":"unece:insuranceApplicableCurrencyExchange","@type":["rdf:Property","owl:ObjectProperty"],"rdfs:label":"insuranceApplicableCurrencyExchange","schema:rangeIncludes":{"@id":"unece:CurrencyExchange"},"schema:domainIncludes":{"@id":"unece:Consignment"},"rdfs:comment":"The conversion of one currency to another for trade purposes."},{"@id":"unece:insurancePremiumAmount","@type":["rdf:Property","owl:ObjectProperty"],"rdfs:label":"insurancePremiumAmount","schema:rangeIncludes":{"@id":"unece:AmountType"},"schema:domainIncludes":{"@id":"unece:Consignment"},"rdfs:comment":""},{"@id":"unece:insuranceValueAmount","@type":["rdf:Property","owl:ObjectProperty"],"rdfs:label":"insuranceValueAmount","schema:rangeIncludes":{"@id":"unece:AmountType"},"schema:domainIncludes":[{"@id":"unece:Consignment"},{"@id":"unece:ConsignmentItem"}],"rdfs:comment":""},{"@id":"unece:intermediateConsigneeParty","@type":["rdf:Property","owl:ObjectProperty"],"rdfs:label":"intermediateConsigneeParty","schema:rangeIncludes":{"@id":"unece:Party"},"schema:domainIncludes":{"@id":"unece:Consignment"},"rdfs:comment":""},{"@id":"unece:invoiceeAssociatedParty","@type":["rdf:Property","owl:ObjectProperty"],"rdfs:label":"invoiceeAssociatedParty","schema:rangeIncludes":{"@id":"unece:Party"},"schema:domainIncludes":{"@id":"unece:Consignment"},"rdfs:comment":""},{"@id":"unece:loadingBaseportLocation","@type":["rdf:Property","owl:ObjectProperty"],"rdfs:label":"loadingBaseportLocation","schema:rangeIncludes":{"@id":"unece:LogisticsLocation"},"schema:domainIncludes":{"@id":"unece:Consignment"},"rdfs:comment":"The baseport location at which this supply chain consignment is to be loaded on a means of transport according to the transport contract."},{"@id":"unece:loadingInformation","@type":["rdf:Property","owl:DatatypeProperty"],"rdfs:label":"loadingInformation","schema:rangeIncludes":{"@id":"schema:Text"},"schema:domainIncludes":{"@id":"unece:Consignment"},"rdfs:comment":"Loading information, expressed as text, for this supply chain consignment, such as advice and instructions."},{"@id":"unece:loadingListQuantity","@type":["rdf:Property","owl:ObjectProperty"],"rdfs:label":"loadingListQuantity","schema:rangeIncludes":{"@id":"unece:QuantityType"},"schema:domainIncludes":{"@id":"unece:Consignment"},"rdfs:comment":""},{"@id":"unece:loadingLocation","@type":["rdf:Property","owl:ObjectProperty"],"rdfs:label":"loadingLocation","schema:rangeIncludes":{"@id":"unece:LogisticsLocation"},"schema:domainIncludes":{"@id":"unece:Consignment"},"rdfs:comment":"The logistics location where the supply chain consignment is loaded."},{"@id":"unece:localConsigneeAgentParty","@type":["rdf:Property","owl:ObjectProperty"],"rdfs:label":"localConsigneeAgentParty","schema:rangeIncludes":{"@id":"unece:Party"},"schema:domainIncludes":{"@id":"unece:Consignment"},"rdfs:comment":""},{"@id":"unece:mainCarriageTransportMovement","@type":["rdf:Property","owl:ObjectProperty"],"rdfs:label":"mainCarriageTransportMovement","schema:rangeIncludes":{"@id":"unece:TransportMovement"},"schema:domainIncludes":{"@id":"unece:Consignment"},"rdfs:comment":"A main carriage logistics transport movement for this supply chain consignment."},{"@id":"unece:manifestAssociatedDocument","@type":["rdf:Property","owl:ObjectProperty"],"rdfs:label":"manifestAssociatedDocument","schema:rangeIncludes":{"@id":"unece:Document"},"schema:domainIncludes":{"@id":"unece:Consignment"},"rdfs:comment":"Written, printed or electronic matter that is referenced."},{"@id":"unece:natureIdentificationCargo","@type":["rdf:Property","owl:ObjectProperty"],"rdfs:label":"natureIdentificationCargo","schema:rangeIncludes":{"@id":"unece:Cargo"},"schema:domainIncludes":[{"@id":"unece:Consignment"},{"@id":"unece:ConsignmentItem"}],"rdfs:comment":"Transport cargo details of this referenced supply chain consignment item sufficient to identify its nature for customs, statistical or transport purposes."},{"@id":"unece:nilCarriageValueIndicator","@type":["rdf:Property","owl:DatatypeProperty"],"rdfs:label":"nilCarriageValueIndicator","schema:rangeIncludes":{"@id":"schema:Boolean"},"schema:domainIncludes":{"@id":"unece:Consignment"},"rdfs:comment":"The indication of whether or not this supply chain consignment has a nil value for carriage."},{"@id":"unece:nilCustomsValueIndicator","@type":["rdf:Property","owl:DatatypeProperty"],"rdfs:label":"nilCustomsValueIndicator","schema:rangeIncludes":{"@id":"schema:Boolean"},"schema:domainIncludes":{"@id":"unece:Consignment"},"rdfs:comment":"The indication of whether or not this supply chain consignment has a nil value for customs."},{"@id":"unece:nilInsuranceValueIndicator","@type":["rdf:Property","owl:DatatypeProperty"],"rdfs:label":"nilInsuranceValueIndicator","schema:rangeIncludes":{"@id":"schema:Boolean"},"schema:domainIncludes":{"@id":"unece:Consignment"},"rdfs:comment":"The indication of whether or not this supply chain consignment has a nil value for insurance."},{"@id":"unece:onCarriageTransportMovement","@type":["rdf:Property","owl:ObjectProperty"],"rdfs:label":"onCarriageTransportMovement","schema:rangeIncludes":{"@id":"unece:TransportMovement"},"schema:domainIncludes":{"@id":"unece:Consignment"},"rdfs:comment":"An on-carriage logistics transport movement for this supply chain consignment."},{"@id":"unece:onwardRoutingLocation","@type":["rdf:Property","owl:ObjectProperty"],"rdfs:label":"onwardRoutingLocation","schema:rangeIncludes":{"@id":"unece:LogisticsLocation"},"schema:domainIncludes":{"@id":"unece:Consignment"},"rdfs:comment":"An onward routing location for this supply chain consignment."},{"@id":"unece:originGeopoliticalRegion","@type":["rdf:Property","owl:ObjectProperty"],"rdfs:label":"originGeopoliticalRegion","schema:rangeIncludes":{"@id":"unece:GeopoliticalRegion"},"schema:domainIncludes":[{"@id":"unece:Consignment"},{"@id":"unece:ConsignmentItem"}],"rdfs:comment":"A collection of countries and/or economies united for trade purposes."},{"@id":"unece:originalDespatchLocation","@type":["rdf:Property","owl:ObjectProperty"],"rdfs:label":"originalDespatchLocation","schema:rangeIncludes":{"@id":"unece:LogisticsLocation"},"schema:domainIncludes":{"@id":"unece:Consignment"},"rdfs:comment":"The location from which this supply chain consignment was originally despatched."},{"@id":"unece:pickUpParty","@type":["rdf:Property","owl:ObjectProperty"],"rdfs:label":"pickUpParty","schema:rangeIncludes":{"@id":"unece:Party"},"schema:domainIncludes":{"@id":"unece:Consignment"},"rdfs:comment":""},{"@id":"unece:preCarriageTransportMovement","@type":["rdf:Property","owl:ObjectProperty"],"rdfs:label":"preCarriageTransportMovement","schema:rangeIncludes":{"@id":"unece:TransportMovement"},"schema:domainIncludes":{"@id":"unece:Consignment"},"rdfs:comment":"A pre-carriage logistics transport movement for this referenced supply chain consignment."},{"@id":"unece:previousAdministrativeDocument","@type":["rdf:Property","owl:ObjectProperty"],"rdfs:label":"previousAdministrativeDocument","schema:rangeIncludes":{"@id":"unece:Document"},"schema:domainIncludes":[{"@id":"unece:Consignment"},{"@id":"unece:ConsignmentItem"}],"rdfs:comment":"Written, printed or electronic matter that is referenced."},{"@id":"unece:reExportCountry","@type":["rdf:Property","owl:ObjectProperty"],"rdfs:label":"reExportCountry","schema:rangeIncludes":{"@id":"unece:Country"},"schema:domainIncludes":{"@id":"unece:Consignment"},"rdfs:comment":"The area of land that belongs to a nation together with its properties, such as population, political organization, etc., used or referenced for trade purposes."},{"@id":"unece:relatedBookingType","@type":["rdf:Property","owl:DatatypeProperty"],"rdfs:label":"relatedBookingType","schema:rangeIncludes":{"@id":"schema:Text"},"schema:domainIncludes":{"@id":"unece:Consignment"},"rdfs:comment":"The type of booking, expressed as text, related to this supply chain consignment."},{"@id":"unece:riskFactorCode","@type":["rdf:Property","owl:DatatypeProperty"],"rdfs:label":"riskFactorCode","schema:rangeIncludes":{"@id":"schema:Text"},"schema:domainIncludes":{"@id":"unece:Consignment"},"rdfs:comment":"The code specifying a risk factor for this supply chain consignment."},{"@id":"unece:serviceChargeApplicableCurrencyExchange","@type":["rdf:Property","owl:ObjectProperty"],"rdfs:label":"serviceChargeApplicableCurrencyExchange","schema:rangeIncludes":{"@id":"unece:CurrencyExchange"},"schema:domainIncludes":{"@id":"unece:Consignment"},"rdfs:comment":"The conversion of one currency to another for trade purposes."},{"@id":"unece:shipStoresIndicator","@type":["rdf:Property","owl:DatatypeProperty"],"rdfs:label":"shipStoresIndicator","schema:rangeIncludes":{"@id":"schema:Boolean"},"schema:domainIncludes":{"@id":"unece:Consignment"},"rdfs:comment":"The indication of whether or not this supply chain consignment is for ship stores, such as for consumption on the means of transport."},{"@id":"unece:shippedOnboardDateTime","@type":["rdf:Property","owl:DatatypeProperty"],"rdfs:label":"shippedOnboardDateTime","schema:rangeIncludes":{"@id":"schema:DateTime"},"schema:domainIncludes":{"@id":"unece:Consignment"},"rdfs:comment":"A date, time, date time, or other date time value when this supply chain consignment is shipped onboard."},{"@id":"unece:specifiedDeliveryTerms","@type":["rdf:Property","owl:ObjectProperty"],"rdfs:label":"specifiedDeliveryTerms","schema:rangeIncludes":{"@id":"unece:DeliveryTerms"},"schema:domainIncludes":{"@id":"unece:Consignment"},"rdfs:comment":"Delivery terms specified for this supply chain consignment."},{"@id":"unece:specifiedSupplyChainReference","@type":["rdf:Property","owl:ObjectProperty"],"rdfs:label":"specifiedSupplyChainReference","schema:rangeIncludes":{"@id":"unece:SupplyChainReference"},"schema:domainIncludes":{"@id":"unece:Consignment"},"rdfs:comment":"A reference specified for this supply chain consignment."},{"@id":"unece:specifiedTransportMovement","@type":["rdf:Property","owl:ObjectProperty"],"rdfs:label":"specifiedTransportMovement","schema:rangeIncludes":{"@id":"unece:TransportMovement"},"schema:domainIncludes":{"@id":"unece:Consignment"},"rdfs:comment":"A logistics transport movement specified for this supply chain consignment."},{"@id":"unece:summaryDescription","@type":["rdf:Property","owl:DatatypeProperty"],"rdfs:label":"summaryDescription","schema:rangeIncludes":{"@id":"schema:Text"},"schema:domainIncludes":{"@id":"unece:Consignment"},"rdfs:comment":"A textual summary description of this supply chain consignment."},{"@id":"unece:totalCollectChargeAmount","@type":["rdf:Property","owl:ObjectProperty"],"rdfs:label":"totalCollectChargeAmount","schema:rangeIncludes":{"@id":"unece:AmountType"},"schema:domainIncludes":{"@id":"unece:Consignment"},"rdfs:comment":""},{"@id":"unece:totalDisbursementAmount","@type":["rdf:Property","owl:ObjectProperty"],"rdfs:label":"totalDisbursementAmount","schema:rangeIncludes":{"@id":"unece:AmountType"},"schema:domainIncludes":{"@id":"unece:Consignment"},"rdfs:comment":""},{"@id":"unece:totalExportExitToImportEntryChargeAmount","@type":["rdf:Property","owl:ObjectProperty"],"rdfs:label":"totalExportExitToImportEntryChargeAmount","schema:rangeIncludes":{"@id":"unece:AmountType"},"schema:domainIncludes":[{"@id":"unece:Consignment"},{"@id":"unece:ConsignmentItem"}],"rdfs:comment":""},{"@id":"unece:totalPrepaidChargeAmount","@type":["rdf:Property","owl:ObjectProperty"],"rdfs:label":"totalPrepaidChargeAmount","schema:rangeIncludes":{"@id":"unece:AmountType"},"schema:domainIncludes":{"@id":"unece:Consignment"},"rdfs:comment":""},{"@id":"unece:tradedParcelId","@type":["rdf:Property","owl:DatatypeProperty"],"rdfs:label":"tradedParcelId","schema:rangeIncludes":{"@id":"schema:Text"},"schema:domainIncludes":{"@id":"unece:Consignment"},"rdfs:comment":"A traded parcel identifier for this supply chain consignment."},{"@id":"unece:transitCountry","@type":["rdf:Property","owl:ObjectProperty"],"rdfs:label":"transitCountry","schema:rangeIncludes":{"@id":"unece:Country"},"schema:domainIncludes":[{"@id":"unece:Consignment"},{"@id":"unece:ConsignmentItem"}],"rdfs:comment":"The area of land that belongs to a nation together with its properties, such as population, political organization, etc., used or referenced for trade purposes."},{"@id":"unece:transitLocation","@type":["rdf:Property","owl:ObjectProperty"],"rdfs:label":"transitLocation","schema:rangeIncludes":{"@id":"unece:LogisticsLocation"},"schema:domainIncludes":{"@id":"unece:Consignment"},"rdfs:comment":"A location of transit for this supply chain consignment."},{"@id":"unece:transportContractDocument","@type":["rdf:Property","owl:ObjectProperty"],"rdfs:label":"transportContractDocument","schema:rangeIncludes":{"@id":"unece:Document"},"schema:domainIncludes":[{"@id":"unece:Consignment"},{"@id":"unece:ConsignmentItem"}],"rdfs:comment":"Written, printed or electronic matter that is referenced."},{"@id":"unece:transportEquipmentSplitGoodsIndicator","@type":["rdf:Property","owl:DatatypeProperty"],"rdfs:label":"transportEquipmentSplitGoodsIndicator","schema:rangeIncludes":{"@id":"schema:Boolean"},"schema:domainIncludes":{"@id":"unece:Consignment"},"rdfs:comment":"The indication of whether or not the goods in this supply chain consignment are split across more than one piece of transport equipment."},{"@id":"unece:transportEvent","@type":["rdf:Property","owl:ObjectProperty"],"rdfs:label":"transportEvent","schema:rangeIncludes":{"@id":"unece:TransportEvent"},"schema:domainIncludes":{"@id":"unece:Consignment"},"rdfs:comment":"An event occurring during the transport of this supply chain consignment."},{"@id":"unece:transportPackage","@type":["rdf:Property","owl:ObjectProperty"],"rdfs:label":"transportPackage","schema:rangeIncludes":{"@id":"unece:Package"},"schema:domainIncludes":[{"@id":"unece:Consignment"},{"@id":"unece:ConsignmentItem"}],"rdfs:comment":"A transport package for this referenced supply chain consignment item."},{"@id":"unece:transportService","@type":["rdf:Property","owl:ObjectProperty"],"rdfs:label":"transportService","schema:rangeIncludes":{"@id":"unece:Service"},"schema:domainIncludes":{"@id":"unece:Consignment"},"rdfs:comment":"A transport service for this supply chain consignment."},{"@id":"unece:transportSplitDescription","@type":["rdf:Property","owl:DatatypeProperty"],"rdfs:label":"transportSplitDescription","schema:rangeIncludes":{"@id":"schema:Text"},"schema:domainIncludes":{"@id":"unece:Consignment"},"rdfs:comment":"The textual description of the transport split of this referenced supply chain consignment across different transport means or transport equipment."},{"@id":"unece:transshipmentLocation","@type":["rdf:Property","owl:ObjectProperty"],"rdfs:label":"transshipmentLocation","schema:rangeIncludes":{"@id":"unece:LogisticsLocation"},"schema:domainIncludes":{"@id":"unece:Consignment"},"rdfs:comment":"A transshipment location for this supply chain consignment."},{"@id":"unece:transshipmentPermissionIndicator","@type":["rdf:Property","owl:DatatypeProperty"],"rdfs:label":"transshipmentPermissionIndicator","schema:rangeIncludes":{"@id":"schema:Boolean"},"schema:domainIncludes":{"@id":"unece:Consignment"},"rdfs:comment":"The indication of whether or not transshipment is permitted for this supply chain consignment."},{"@id":"unece:unloadingBaseportLocation","@type":["rdf:Property","owl:ObjectProperty"],"rdfs:label":"unloadingBaseportLocation","schema:rangeIncludes":{"@id":"unece:LogisticsLocation"},"schema:domainIncludes":{"@id":"unece:Consignment"},"rdfs:comment":"The baseport location at which this supply chain consignment is to be unloaded from a means of transport according to the transport contract."},{"@id":"unece:unloadingLocation","@type":["rdf:Property","owl:ObjectProperty"],"rdfs:label":"unloadingLocation","schema:rangeIncludes":{"@id":"unece:LogisticsLocation"},"schema:domainIncludes":{"@id":"unece:Consignment"},"rdfs:comment":"The logistics location where the supply chain consignment is unloaded."},{"@id":"unece:vanningEvent","@type":["rdf:Property","owl:ObjectProperty"],"rdfs:label":"vanningEvent","schema:rangeIncludes":{"@id":"unece:TransportEvent"},"schema:domainIncludes":[{"@id":"unece:Consignment"},{"@id":"unece:ConsignmentItem"}],"rdfs:comment":"The vanning event (the loading of this consignment at the place of its original despatch) for this referenced supply chain consignment."},{"@id":"unece:warehouseArrivalDateTime","@type":["rdf:Property","owl:DatatypeProperty"],"rdfs:label":"warehouseArrivalDateTime","schema:rangeIncludes":{"@id":"schema:Text"},"schema:domainIncludes":{"@id":"unece:Consignment"},"rdfs:comment":"The date, time, date time or other date time value of the arrival of this supply chain consignment at a warehouse."},{"@id":"unece:warehouseDepositorParty","@type":["rdf:Property","owl:ObjectProperty"],"rdfs:label":"warehouseDepositorParty","schema:rangeIncludes":{"@id":"unece:Party"},"schema:domainIncludes":{"@id":"unece:Consignment"},"rdfs:comment":""},{"@id":"unece:warehouseKeeperParty","@type":["rdf:Property","owl:ObjectProperty"],"rdfs:label":"warehouseKeeperParty","schema:rangeIncludes":{"@id":"unece:Party"},"schema:domainIncludes":{"@id":"unece:Consignment"},"rdfs:comment":""},{"@id":"unece:warehouseOperatorParty","@type":["rdf:Property","owl:ObjectProperty"],"rdfs:label":"warehouseOperatorParty","schema:rangeIncludes":{"@id":"unece:Party"},"schema:domainIncludes":{"@id":"unece:Consignment"},"rdfs:comment":""},{"@id":"unece:warehouseStorageEvent","@type":["rdf:Property","owl:ObjectProperty"],"rdfs:label":"warehouseStorageEvent","schema:rangeIncludes":{"@id":"unece:TransportEvent"},"schema:domainIncludes":{"@id":"unece:Consignment"},"rdfs:comment":"A warehouse storage event for this referenced supply chain consignment."},{"@id":"unece:applicableTransportMeans","@type":["rdf:Property","owl:ObjectProperty"],"rdfs:label":"applicableTransportMeans","schema:rangeIncludes":{"@id":"unece:LogisticsTransportMeans"},"schema:domainIncludes":{"@id":"unece:ConsignmentItem"},"rdfs:comment":"The means of transport applicable to this supply chain consignment item."},{"@id":"unece:damageRemarks","@type":["rdf:Property","owl:DatatypeProperty"],"rdfs:label":"damageRemarks","schema:rangeIncludes":{"@id":"schema:Text"},"schema:domainIncludes":{"@id":"unece:ConsignmentItem"},"rdfs:comment":"Damage remarks, expressed as text, for this supply chain consignment item."},{"@id":"unece:declaredValueForStatisticsAmount","@type":["rdf:Property","owl:ObjectProperty"],"rdfs:label":"declaredValueForStatisticsAmount","schema:rangeIncludes":{"@id":"unece:AmountType"},"schema:domainIncludes":{"@id":"unece:ConsignmentItem"},"rdfs:comment":""},{"@id":"unece:deliveryInstructionsText","@type":["rdf:Property","owl:DatatypeProperty"],"rdfs:label":"deliveryInstructionsText","schema:rangeIncludes":{"@id":"schema:Text"},"schema:domainIncludes":{"@id":"unece:ConsignmentItem"},"rdfs:comment":"Delivery instructions, expressed as text, for this supply chain consignment item."},{"@id":"unece:exportTypeCode","@type":["rdf:Property","owl:DatatypeProperty"],"rdfs:label":"exportTypeCode","schema:rangeIncludes":{"@id":"schema:Text"},"schema:domainIncludes":{"@id":"unece:ConsignmentItem"},"rdfs:comment":"The code specifying the export type of supply chain consignment item."},{"@id":"unece:firstTypeExtensionCode","@type":["rdf:Property","owl:DatatypeProperty"],"rdfs:label":"firstTypeExtensionCode","schema:rangeIncludes":{"@id":"schema:Text"},"schema:domainIncludes":{"@id":"unece:ConsignmentItem"},"rdfs:comment":"The code used as a first extension to the type code for further specifying the type of supply chain consignment item."},{"@id":"unece:goodsTypeCode","@type":["rdf:Property","owl:DatatypeProperty"],"rdfs:label":"goodsTypeCode","schema:rangeIncludes":{"@id":"unece:GoodsTypeCodeList"},"schema:domainIncludes":{"@id":"unece:ConsignmentItem"},"rdfs:comment":"The code specifying the type of referenced supply chain consignment item."},{"@id":"unece:goodsTypeExtensionTypeExtensionCode","@type":["rdf:Property","owl:DatatypeProperty"],"rdfs:label":"goodsTypeExtensionTypeExtensionCode","schema:rangeIncludes":{"@id":"unece:GoodsTypeExtensionCodeList"},"schema:domainIncludes":{"@id":"unece:ConsignmentItem"},"rdfs:comment":"The code used as an extension to the type code for further specifying the type of referenced supply chain consignment item."},{"@id":"unece:importTypeCode","@type":["rdf:Property","owl:DatatypeProperty"],"rdfs:label":"importTypeCode","schema:rangeIncludes":{"@id":"schema:Text"},"schema:domainIncludes":{"@id":"unece:ConsignmentItem"},"rdfs:comment":"The code specifying the import type of supply chain consignment item."},{"@id":"unece:importationCountry","@type":["rdf:Property","owl:ObjectProperty"],"rdfs:label":"importationCountry","schema:rangeIncludes":{"@id":"unece:Country"},"schema:domainIncludes":{"@id":"unece:ConsignmentItem"},"rdfs:comment":"The area of land that belongs to a nation together with its properties, such as population, political organization, etc., used or referenced for trade purposes."},{"@id":"unece:invoiceAmount","@type":["rdf:Property","owl:ObjectProperty"],"rdfs:label":"invoiceAmount","schema:rangeIncludes":{"@id":"unece:AmountType"},"schema:domainIncludes":{"@id":"unece:ConsignmentItem"},"rdfs:comment":""},{"@id":"unece:nationalTypeExtensionCode","@type":["rdf:Property","owl:DatatypeProperty"],"rdfs:label":"nationalTypeExtensionCode","schema:rangeIncludes":{"@id":"schema:Text"},"schema:domainIncludes":{"@id":"unece:ConsignmentItem"},"rdfs:comment":"The code used as a national extension to the type code for further specifying the type of supply chain consignment item."},{"@id":"unece:secondTypeExtensionCode","@type":["rdf:Property","owl:DatatypeProperty"],"rdfs:label":"secondTypeExtensionCode","schema:rangeIncludes":{"@id":"schema:Text"},"schema:domainIncludes":{"@id":"unece:ConsignmentItem"},"rdfs:comment":"The code used as a second extension to the type code for further specifying the type of supply chain consignment item."},{"@id":"unece:specialInstructions","@type":["rdf:Property","owl:DatatypeProperty"],"rdfs:label":"specialInstructions","schema:rangeIncludes":{"@id":"schema:Text"},"schema:domainIncludes":{"@id":"unece:ConsignmentItem"},"rdfs:comment":"Special instructions, expressed as text, for this supply chain consignment item."},{"@id":"unece:tradeLineItemQuantity","@type":["rdf:Property","owl:ObjectProperty"],"rdfs:label":"tradeLineItemQuantity","schema:rangeIncludes":{"@id":"unece:QuantityType"},"schema:domainIncludes":{"@id":"unece:ConsignmentItem"},"rdfs:comment":""},{"@id":"unece:transportTemperature","@type":["rdf:Property","owl:ObjectProperty"],"rdfs:label":"transportTemperature","schema:rangeIncludes":{"@id":"unece:TransportSettingTemperature"},"schema:domainIncludes":{"@id":"unece:ConsignmentItem"},"rdfs:comment":"The transport temperature setting for this supply chain consignment item."},{"@id":"unece:applicablePackagingInstructions","@type":["rdf:Property","owl:ObjectProperty"],"rdfs:label":"applicablePackagingInstructions","schema:rangeIncludes":{"@id":"unece:PackagingInstructions"},"schema:domainIncludes":[{"@id":"unece:LogisticsPackaging"},{"@id":"unece:SupplyChainPackaging"}],"rdfs:comment":"Instructions applicable to this logistics packaging."},{"@id":"unece:certificationIndicator","@type":["rdf:Property","owl:DatatypeProperty"],"rdfs:label":"certificationIndicator","schema:rangeIncludes":{"@id":"schema:Boolean"},"schema:domainIncludes":{"@id":"unece:LogisticsPackaging"},"rdfs:comment":"The indication whether or not this logistics packaging has a certification."},{"@id":"unece:containedPackage","@type":["rdf:Property","owl:ObjectProperty"],"rdfs:label":"containedPackage","schema:rangeIncludes":{"@id":"unece:Package"},"schema:domainIncludes":{"@id":"unece:LogisticsPackaging"},"rdfs:comment":"A package contained in this logistics packaging."},{"@id":"unece:contentLayerQuantity","@type":["rdf:Property","owl:ObjectProperty"],"rdfs:label":"contentLayerQuantity","schema:rangeIncludes":{"@id":"unece:QuantityType"},"schema:domainIncludes":[{"@id":"unece:LogisticsPackaging"},{"@id":"unece:SupplyChainPackaging"}],"rdfs:comment":""},{"@id":"unece:disposalMethodCode","@type":["rdf:Property","owl:DatatypeProperty"],"rdfs:label":"disposalMethodCode","schema:rangeIncludes":{"@id":"schema:Text"},"schema:domainIncludes":[{"@id":"unece:LogisticsPackaging"},{"@id":"unece:SupplyChainPackaging"}],"rdfs:comment":"A code specifying a disposal method for this logistics packaging."},{"@id":"unece:instructionIndicator","@type":["rdf:Property","owl:DatatypeProperty"],"rdfs:label":"instructionIndicator","schema:rangeIncludes":{"@id":"schema:Boolean"},"schema:domainIncludes":{"@id":"unece:LogisticsPackaging"},"rdfs:comment":"The indication of whether or not this logistics packaging has an instruction."},{"@id":"unece:maximumStackabilityQuantity","@type":["rdf:Property","owl:ObjectProperty"],"rdfs:label":"maximumStackabilityQuantity","schema:rangeIncludes":{"@id":"unece:QuantityType"},"schema:domainIncludes":[{"@id":"unece:LogisticsPackaging"},{"@id":"unece:SupplyChainPackaging"}],"rdfs:comment":""},{"@id":"unece:methodDescription","@type":["rdf:Property","owl:DatatypeProperty"],"rdfs:label":"methodDescription","schema:rangeIncludes":{"@id":"schema:Text"},"schema:domainIncludes":{"@id":"unece:LogisticsPackaging"},"rdfs:comment":"The textual description of the method of logistics packaging, such as hermetically sealed."},{"@id":"unece:packagingType","@type":["rdf:Property","owl:DatatypeProperty"],"rdfs:label":"packagingType","schema:rangeIncludes":{"@id":"schema:Text"},"schema:domainIncludes":[{"@id":"unece:LogisticsPackaging"},{"@id":"unece:SupplyChainPackaging"}],"rdfs:comment":"The type, expressed as text, of supply chain packaging."},{"@id":"unece:specifiedMarking","@type":["rdf:Property","owl:ObjectProperty"],"rdfs:label":"specifiedMarking","schema:rangeIncludes":{"@id":"unece:Marking"},"schema:domainIncludes":[{"@id":"unece:LogisticsPackaging"},{"@id":"unece:SupplyChainPackaging"}],"rdfs:comment":"A marking specified for this logistics packaging."},{"@id":"unece:totalUnitQuantity","@type":["rdf:Property","owl:ObjectProperty"],"rdfs:label":"totalUnitQuantity","schema:rangeIncludes":{"@id":"unece:QuantityType"},"schema:domainIncludes":[{"@id":"unece:LogisticsPackaging"},{"@id":"unece:SupplyChainPackaging"}],"rdfs:comment":""},{"@id":"unece:applicableTransportationWasteRecoveryDisposalProcess","@type":["rdf:Property","owl:ObjectProperty"],"rdfs:label":"applicableTransportationWasteRecoveryDisposalProcess","schema:rangeIncludes":{"@id":"unece:TransportationWasteRecoveryDisposalProcess"},"schema:domainIncludes":{"@id":"unece:TransportationWasteMaterial"},"rdfs:comment":"A transportation waste recovery disposal process applicable to this transportation waste material."},{"@id":"unece:completeDeliveryIndicator","@type":["rdf:Property","owl:DatatypeProperty"],"rdfs:label":"completeDeliveryIndicator","schema:rangeIncludes":{"@id":"schema:Boolean"},"schema:domainIncludes":{"@id":"unece:TransportationWasteMaterial"},"rdfs:comment":"The indication of whether or not a transportation waste material delivery is complete."},{"@id":"unece:includedTransportationWasteMaterialComponent","@type":["rdf:Property","owl:ObjectProperty"],"rdfs:label":"includedTransportationWasteMaterialComponent","schema:rangeIncludes":{"@id":"unece:TransportationWasteMaterialComponent"},"schema:domainIncludes":{"@id":"unece:TransportationWasteMaterial"},"rdfs:comment":"A material component included in this transportation waste."},{"@id":"unece:nextDeliveryEvent","@type":["rdf:Property","owl:ObjectProperty"],"rdfs:label":"nextDeliveryEvent","schema:rangeIncludes":{"@id":"unece:TransportEvent"},"schema:domainIncludes":{"@id":"unece:TransportationWasteMaterial"},"rdfs:comment":"A next delivery event for this transportation waste material."},{"@id":"unece:previousDeliveryTransportEvent","@type":["rdf:Property","owl:ObjectProperty"],"rdfs:label":"previousDeliveryTransportEvent","schema:rangeIncludes":{"@id":"unece:TransportEvent"},"schema:domainIncludes":{"@id":"unece:TransportationWasteMaterial"},"rdfs:comment":"A previous delivery event for this transportation waste material."},{"@id":"unece:receptionFacilityContact","@type":["rdf:Property","owl:ObjectProperty"],"rdfs:label":"receptionFacilityContact","schema:rangeIncludes":{"@id":"unece:Contact"},"schema:domainIncludes":{"@id":"unece:TransportationWasteMaterial"},"rdfs:comment":"An individual human being in a position to give assistance or information."},{"@id":"unece:estimatedGeneratedMeasure","@type":["rdf:Property","owl:ObjectProperty"],"rdfs:label":"estimatedGeneratedMeasure","schema:rangeIncludes":{"@id":"unece:VolumeUnitMeasureType"},"schema:domainIncludes":{"@id":"unece:TransportationWasteMaterialComponent"},"rdfs:comment":""},{"@id":"unece:maximumDedicatedStorageCapacityMeasure","@type":["rdf:Property","owl:ObjectProperty"],"rdfs:label":"maximumDedicatedStorageCapacityMeasure","schema:rangeIncludes":{"@id":"unece:VolumeUnitMeasureType"},"schema:domainIncludes":{"@id":"unece:TransportationWasteMaterialComponent"},"rdfs:comment":""},{"@id":"unece:plannedDischargedMeasure","@type":["rdf:Property","owl:ObjectProperty"],"rdfs:label":"plannedDischargedMeasure","schema:rangeIncludes":{"@id":"unece:VolumeUnitMeasureType"},"schema:domainIncludes":{"@id":"unece:TransportationWasteMaterialComponent"},"rdfs:comment":""},{"@id":"unece:remainingDeliveryEvent","@type":["rdf:Property","owl:ObjectProperty"],"rdfs:label":"remainingDeliveryEvent","schema:rangeIncludes":{"@id":"unece:TransportEvent"},"schema:domainIncludes":{"@id":"unece:TransportationWasteMaterialComponent"},"rdfs:comment":"A delivery event for this remaining transportation waste material component."},{"@id":"unece:volumeUnitRetainedMeasure","@type":["rdf:Property","owl:ObjectProperty"],"rdfs:label":"volumeUnitRetainedMeasure","schema:rangeIncludes":{"@id":"unece:VolumeUnitMeasureType"},"schema:domainIncludes":{"@id":"unece:TransportationWasteMaterialComponent"},"rdfs:comment":""},{"@id":"unece:applicableTransportSettingTemperature","@type":["rdf:Property","owl:ObjectProperty"],"rdfs:label":"applicableTransportSettingTemperature","schema:rangeIncludes":{"@id":"unece:TransportSettingTemperature"},"schema:domainIncludes":{"@id":"unece:HandlingInstructions"},"rdfs:comment":"A transport related temperature setting applicable to these handling instructions."},{"@id":"unece:deliveryApplicableTemperature","@type":["rdf:Property","owl:ObjectProperty"],"rdfs:label":"deliveryApplicableTemperature","schema:rangeIncludes":{"@id":"unece:InstructedTemperature"},"schema:domainIncludes":{"@id":"unece:HandlingInstructions"},"rdfs:comment":"The instructed temperature for delivery applicable to these handling instructions."},{"@id":"unece:handlingCode","@type":["rdf:Property","owl:DatatypeProperty"],"rdfs:label":"handlingCode","schema:rangeIncludes":{"@id":"schema:Text"},"schema:domainIncludes":[{"@id":"unece:HandlingInstructions"},{"@id":"unece:PackagingInstructions"},{"@id":"unece:DeliveryInstructions"}],"rdfs:comment":"A code specifying delivery handling instructions."},{"@id":"unece:handlingInstructionsDescriptionCode","@type":["rdf:Property","owl:DatatypeProperty"],"rdfs:label":"handlingInstructionsDescriptionCode","schema:rangeIncludes":{"@id":"schema:Text"},"schema:domainIncludes":{"@id":"unece:HandlingInstructions"},"rdfs:comment":"A code specifying a description of these handling instructions."},{"@id":"unece:marketDeliveryApplicableTemperature","@type":["rdf:Property","owl:ObjectProperty"],"rdfs:label":"marketDeliveryApplicableTemperature","schema:rangeIncludes":{"@id":"unece:InstructedTemperature"},"schema:domainIncludes":{"@id":"unece:HandlingInstructions"},"rdfs:comment":"The instructed temperature for market delivery applicable to these handling instructions."},{"@id":"unece:maximumStackabilityApplicableQuantity","@type":["rdf:Property","owl:ObjectProperty"],"rdfs:label":"maximumStackabilityApplicableQuantity","schema:rangeIncludes":{"@id":"unece:QuantityType"},"schema:domainIncludes":{"@id":"unece:HandlingInstructions"},"rdfs:comment":""},{"@id":"unece:maximumStackabilityWeightApplicableMeasure","@type":["rdf:Property","owl:ObjectProperty"],"rdfs:label":"maximumStackabilityWeightApplicableMeasure","schema:rangeIncludes":{"@id":"unece:WeightUnitMeasureType"},"schema:domainIncludes":{"@id":"unece:HandlingInstructions"},"rdfs:comment":""},{"@id":"unece:maximumStorageHumidityApplicableMeasure","@type":["rdf:Property","owl:ObjectProperty"],"rdfs:label":"maximumStorageHumidityApplicableMeasure","schema:rangeIncludes":{"@id":"unece:MeasureType"},"schema:domainIncludes":{"@id":"unece:HandlingInstructions"},"rdfs:comment":""},{"@id":"unece:minimumStorageHumidityApplicableMeasure","@type":["rdf:Property","owl:ObjectProperty"],"rdfs:label":"minimumStorageHumidityApplicableMeasure","schema:rangeIncludes":{"@id":"unece:MeasureType"},"schema:domainIncludes":{"@id":"unece:HandlingInstructions"},"rdfs:comment":""},{"@id":"unece:storageApplicableTemperature","@type":["rdf:Property","owl:ObjectProperty"],"rdfs:label":"storageApplicableTemperature","schema:rangeIncludes":{"@id":"unece:InstructedTemperature"},"schema:domainIncludes":{"@id":"unece:HandlingInstructions"},"rdfs:comment":"The instructed temperature for storage applicable to these handling instructions."},{"@id":"unece:applicationDateTime","@type":["rdf:Property","owl:DatatypeProperty"],"rdfs:label":"applicationDateTime","schema:rangeIncludes":{"@id":"schema:DateTime"},"schema:domainIncludes":{"@id":"unece:SanitaryMeasure"},"rdfs:comment":"An application date, time, date time or other date time value for this MDH sanitary measure."},{"@id":"unece:appliedSanitaryMeasure","@type":["rdf:Property","owl:ObjectProperty"],"rdfs:label":"appliedSanitaryMeasure","schema:rangeIncludes":{"@id":"unece:SanitaryMeasure"},"schema:domainIncludes":{"@id":"unece:MDHHealthIndication"},"rdfs:comment":"A sanitary measure applied for this MDH health indication."},{"@id":"unece:locationName","@type":["rdf:Property","owl:DatatypeProperty"],"rdfs:label":"locationName","schema:rangeIncludes":{"@id":"schema:Text"},"schema:domainIncludes":{"@id":"unece:MDHHealthIndication"},"rdfs:comment":"A location name, expressed as text, of a location for this MDH health indication."},{"@id":"unece:reportedDateTime","@type":["rdf:Property","owl:DatatypeProperty"],"rdfs:label":"reportedDateTime","schema:rangeIncludes":{"@id":"schema:DateTime"},"schema:domainIncludes":{"@id":"unece:MDHHealthIndication"},"rdfs:comment":"A reported date, time, date time or other date time value for this MDH health indication."},{"@id":"unece:reportedQuantity","@type":["rdf:Property","owl:ObjectProperty"],"rdfs:label":"reportedQuantity","schema:rangeIncludes":{"@id":"unece:QuantityType"},"schema:domainIncludes":{"@id":"unece:MDHHealthIndication"},"rdfs:comment":""},{"@id":"unece:statusIndicator","@type":["rdf:Property","owl:DatatypeProperty"],"rdfs:label":"statusIndicator","schema:rangeIncludes":{"@id":"schema:Boolean"},"schema:domainIncludes":{"@id":"unece:MDHHealthIndication"},"rdfs:comment":"The indication of whether or not the status of this MDH health indication is true or false."},{"@id":"unece:arrivalReportedEvent","@type":["rdf:Property","owl:ObjectProperty"],"rdfs:label":"arrivalReportedEvent","schema:rangeIncludes":{"@id":"unece:TransportEvent"},"schema:domainIncludes":{"@id":"unece:LogisticsStatus"},"rdfs:comment":"A transport arrival event reported for this logistics status."},{"@id":"unece:departureReportedEvent","@type":["rdf:Property","owl:ObjectProperty"],"rdfs:label":"departureReportedEvent","schema:rangeIncludes":{"@id":"unece:TransportEvent"},"schema:domainIncludes":{"@id":"unece:LogisticsStatus"},"rdfs:comment":"A transport departure event reported for this logistics status."},{"@id":"unece:loadingReportedEvent","@type":["rdf:Property","owl:ObjectProperty"],"rdfs:label":"loadingReportedEvent","schema:rangeIncludes":{"@id":"unece:TransportEvent"},"schema:domainIncludes":{"@id":"unece:LogisticsStatus"},"rdfs:comment":"A transport loading event reported for this logistics status."},{"@id":"unece:logisticsStatusConditionCode","@type":["rdf:Property","owl:DatatypeProperty"],"rdfs:label":"logisticsStatusConditionCode","schema:rangeIncludes":{"@id":"unece:LogisticsStatusCodeList"},"schema:domainIncludes":{"@id":"unece:LogisticsStatus"},"rdfs:comment":"The code specifying this logistics status condition [UNECE Recommendation 24]."},{"@id":"unece:logisticsStatusReasonCode","@type":["rdf:Property","owl:DatatypeProperty"],"rdfs:label":"logisticsStatusReasonCode","schema:rangeIncludes":{"@id":"unece:LogisticsStatusCodeList"},"schema:domainIncludes":{"@id":"unece:LogisticsStatus"},"rdfs:comment":"A code specifying a reason for this logistics status [UNECE Recommendation 24]."},{"@id":"unece:reportedSupplyChainEvent","@type":["rdf:Property","owl:ObjectProperty"],"rdfs:label":"reportedSupplyChainEvent","schema:rangeIncludes":{"@id":"unece:SupplyChainEvent"},"schema:domainIncludes":{"@id":"unece:LogisticsStatus"},"rdfs:comment":"A supply chain event reported for this logistics status."},{"@id":"unece:unloadingReportedEvent","@type":["rdf:Property","owl:ObjectProperty"],"rdfs:label":"unloadingReportedEvent","schema:rangeIncludes":{"@id":"unece:TransportEvent"},"schema:domainIncludes":{"@id":"unece:LogisticsStatus"},"rdfs:comment":"A transport unloading event reported for this logistics status."},{"@id":"unece:facilityLocation","@type":["rdf:Property","owl:ObjectProperty"],"rdfs:label":"facilityLocation","schema:rangeIncludes":{"@id":"unece:Location"},"schema:domainIncludes":{"@id":"unece:LogisticsLocation"},"rdfs:comment":"A reference to a physical location or place."},{"@id":"unece:healthAffectedAreaIndicator","@type":["rdf:Property","owl:DatatypeProperty"],"rdfs:label":"healthAffectedAreaIndicator","schema:rangeIncludes":{"@id":"schema:Boolean"},"schema:domainIncludes":{"@id":"unece:LogisticsLocation"},"rdfs:comment":"The indication of whether or not this logistics location is in a health affected area."},{"@id":"unece:logisticsLocationCountryId","@type":["rdf:Property","owl:DatatypeProperty"],"rdfs:label":"logisticsLocationCountryId","schema:rangeIncludes":{"@id":"unece:CountryId"},"schema:domainIncludes":{"@id":"unece:LogisticsLocation"},"rdfs:comment":"The unique identifier of a country for this logistics location."},{"@id":"unece:servicingSpecifiedParty","@type":["rdf:Property","owl:ObjectProperty"],"rdfs:label":"servicingSpecifiedParty","schema:rangeIncludes":{"@id":"unece:LocationParty"},"schema:domainIncludes":{"@id":"unece:LogisticsLocation"},"rdfs:comment":"A servicing party specified for this logistics related location."},{"@id":"unece:stayPeriod","@type":["rdf:Property","owl:ObjectProperty"],"rdfs:label":"stayPeriod","schema:rangeIncludes":{"@id":"unece:SpecifiedPeriod"},"schema:domainIncludes":{"@id":"unece:LogisticsLocation"},"rdfs:comment":"A specified period of time."},{"@id":"unece:subordinateRelatedLocation","@type":["rdf:Property","owl:ObjectProperty"],"rdfs:label":"subordinateRelatedLocation","schema:rangeIncludes":{"@id":"unece:LogisticsLocation"},"schema:domainIncludes":{"@id":"unece:LogisticsLocation"},"rdfs:comment":"A logistics location subordinate to this logistics location."},{"@id":"unece:subordinateSubordinateLocation","@type":["rdf:Property","owl:ObjectProperty"],"rdfs:label":"subordinateSubordinateLocation","schema:rangeIncludes":{"@id":"unece:SubordinateLocation"},"schema:domainIncludes":{"@id":"unece:LogisticsLocation"},"rdfs:comment":"A physical location or place which is a subordinate location of a location."},{"@id":"unece:attachedAssetId","@type":["rdf:Property","owl:DatatypeProperty"],"rdfs:label":"attachedAssetId","schema:rangeIncludes":{"@id":"schema:Text"},"schema:domainIncludes":{"@id":"unece:IOTDevice"},"rdfs:comment":"The identifier for the asset, such as a container, to which this monitoring IOT device is attached."},{"@id":"unece:communicationCapabilityCode","@type":["rdf:Property","owl:DatatypeProperty"],"rdfs:label":"communicationCapabilityCode","schema:rangeIncludes":{"@id":"schema:Text"},"schema:domainIncludes":{"@id":"unece:IOTDevice"},"rdfs:comment":"The code specifying the communication capability of this monitoring IOT device."},{"@id":"unece:embeddedSensor","@type":["rdf:Property","owl:ObjectProperty"],"rdfs:label":"embeddedSensor","schema:rangeIncludes":{"@id":"unece:Sensor"},"schema:domainIncludes":{"@id":"unece:IOTDevice"},"rdfs:comment":"An embedded sensor of this monitoring IOT device."},{"@id":"unece:grantedCertificate","@type":["rdf:Property","owl:ObjectProperty"],"rdfs:label":"grantedCertificate","schema:rangeIncludes":{"@id":"unece:ProductCertificate"},"schema:domainIncludes":[{"@id":"unece:IOTDevice"},{"@id":"unece:Sensor"}],"rdfs:comment":"A collection of data for a piece of written, printed or electronic matter that provides information or evidence about the product."},{"@id":"unece:interfaceEquipment","@type":["rdf:Property","owl:ObjectProperty"],"rdfs:label":"interfaceEquipment","schema:rangeIncludes":{"@id":"unece:Equipment"},"schema:domainIncludes":{"@id":"unece:IOTDevice"},"rdfs:comment":"An interface between an OEM (Original Equipment Manufacturer) equipment and this monitoring IOT device."},{"@id":"unece:latestReceivedGeographicalCoordinate","@type":["rdf:Property","owl:ObjectProperty"],"rdfs:label":"latestReceivedGeographicalCoordinate","schema:rangeIncludes":{"@id":"unece:GeographicalCoordinate"},"schema:domainIncludes":{"@id":"unece:IOTDevice"},"rdfs:comment":"A set of geographical coordinates of a specific point such as the longitude, latitude and altitude."},{"@id":"unece:latestReceivedSignalDateTime","@type":["rdf:Property","owl:DatatypeProperty"],"rdfs:label":"latestReceivedSignalDateTime","schema:rangeIncludes":{"@id":"schema:Text"},"schema:domainIncludes":{"@id":"unece:IOTDevice"},"rdfs:comment":"The date, time, date time or other date time value of the latest received signal for this monitoring IOT device, from the perspective of the receiver."},{"@id":"unece:operationalStatusCode","@type":["rdf:Property","owl:DatatypeProperty"],"rdfs:label":"operationalStatusCode","schema:rangeIncludes":{"@id":"schema:Text"},"schema:domainIncludes":{"@id":"unece:IOTDevice"},"rdfs:comment":"The code specifying the operational status, such as broken, stolen, unpaired, inactive of this monitoring IOT device."},{"@id":"unece:positionCode","@type":["rdf:Property","owl:DatatypeProperty"],"rdfs:label":"positionCode","schema:rangeIncludes":{"@id":"schema:Text"},"schema:domainIncludes":[{"@id":"unece:IOTDevice"},{"@id":"unece:Sensor"}],"rdfs:comment":"The code specifying a position of this monitoring sensor."},{"@id":"unece:powerSourceTypeCode","@type":["rdf:Property","owl:DatatypeProperty"],"rdfs:label":"powerSourceTypeCode","schema:rangeIncludes":{"@id":"schema:Text"},"schema:domainIncludes":{"@id":"unece:IOTDevice"},"rdfs:comment":"The code specifying a type of power source for this monitoring IOT device."},{"@id":"unece:remainingBatteryChargePercent","@type":["rdf:Property","owl:DatatypeProperty"],"rdfs:label":"remainingBatteryChargePercent","schema:rangeIncludes":{"@id":"schema:Text"},"schema:domainIncludes":[{"@id":"unece:IOTDevice"},{"@id":"unece:Sensor"}],"rdfs:comment":"The percentage of the remaining battery charge of this monitoring IOT device."},{"@id":"unece:remoteSensor","@type":["rdf:Property","owl:ObjectProperty"],"rdfs:label":"remoteSensor","schema:rangeIncludes":{"@id":"unece:Sensor"},"schema:domainIncludes":{"@id":"unece:IOTDevice"},"rdfs:comment":"A remote sensor of this monitoring IOT device."},{"@id":"unece:reportedTransportEvent","@type":["rdf:Property","owl:ObjectProperty"],"rdfs:label":"reportedTransportEvent","schema:rangeIncludes":{"@id":"unece:TransportEvent"},"schema:domainIncludes":{"@id":"unece:IOTDevice"},"rdfs:comment":"A transport event reported by this monitoring IOT device."},{"@id":"unece:reportingSensorPairing","@type":["rdf:Property","owl:ObjectProperty"],"rdfs:label":"reportingSensorPairing","schema:rangeIncludes":{"@id":"unece:Pairing"},"schema:domainIncludes":{"@id":"unece:IOTDevice"},"rdfs:comment":"The process by which two potentially communicating entities are linked."},{"@id":"unece:declaredPersonalEffects","@type":["rdf:Property","owl:ObjectProperty"],"rdfs:label":"declaredPersonalEffects","schema:rangeIncludes":{"@id":"unece:PersonalEffects"},"schema:domainIncludes":{"@id":"unece:TransportPerson"},"rdfs:comment":"Specified privately owned articles for personal use by an individual."},{"@id":"unece:disembarkationDateTime","@type":["rdf:Property","owl:DatatypeProperty"],"rdfs:label":"disembarkationDateTime","schema:rangeIncludes":{"@id":"schema:DateTime"},"schema:domainIncludes":{"@id":"unece:TransportPerson"},"rdfs:comment":"A date, time, date time, or other date time value that this person disembarked from a means of transport."},{"@id":"unece:disembarkationLocation","@type":["rdf:Property","owl:ObjectProperty"],"rdfs:label":"disembarkationLocation","schema:rangeIncludes":{"@id":"unece:LogisticsLocation"},"schema:domainIncludes":{"@id":"unece:TransportPerson"},"rdfs:comment":"A disembarkation location for this transport person."},{"@id":"unece:embarkationDateTime","@type":["rdf:Property","owl:DatatypeProperty"],"rdfs:label":"embarkationDateTime","schema:rangeIncludes":{"@id":"schema:DateTime"},"schema:domainIncludes":{"@id":"unece:TransportPerson"},"rdfs:comment":"A date, time, date time, or other date time value that this person embarked upon a means of transport."},{"@id":"unece:embarkationLocation","@type":["rdf:Property","owl:ObjectProperty"],"rdfs:label":"embarkationLocation","schema:rangeIncludes":{"@id":"unece:LogisticsLocation"},"schema:domainIncludes":[{"@id":"unece:TransportPerson"},{"@id":"unece:Stowaway"}],"rdfs:comment":"A logistics location where a found stowaway embarked upon the transport means on which they were discovered."},{"@id":"unece:identifiedStowaway","@type":["rdf:Property","owl:ObjectProperty"],"rdfs:label":"identifiedStowaway","schema:rangeIncludes":{"@id":"unece:Stowaway"},"schema:domainIncludes":{"@id":"unece:TransportPerson"},"rdfs:comment":"A transport person identified as a found stowaway."},{"@id":"unece:inTransitIndicator","@type":["rdf:Property","owl:DatatypeProperty"],"rdfs:label":"inTransitIndicator","schema:rangeIncludes":{"@id":"schema:Boolean"},"schema:domainIncludes":{"@id":"unece:TransportPerson"},"rdfs:comment":"The indication of whether or not this transport person is in transit."},{"@id":"unece:reportedIllness","@type":["rdf:Property","owl:ObjectProperty"],"rdfs:label":"reportedIllness","schema:rangeIncludes":{"@id":"unece:Illness"},"schema:domainIncludes":{"@id":"unece:TransportPerson"},"rdfs:comment":"An MDH (Maritime Declaration of Health) reported illness or disease for this transport person."},{"@id":"unece:specificAccreditation","@type":["rdf:Property","owl:ObjectProperty"],"rdfs:label":"specificAccreditation","schema:rangeIncludes":{"@id":"unece:Accreditation"},"schema:domainIncludes":{"@id":"unece:TransportPerson"},"rdfs:comment":"A certified recognition that provides evidence of a level of competency in a given area, such as certifying a level of skill in a trade."},{"@id":"unece:transportPersonLanguageId","@type":["rdf:Property","owl:DatatypeProperty"],"rdfs:label":"transportPersonLanguageId","schema:rangeIncludes":{"@id":"unece:LanguageId"},"schema:domainIncludes":{"@id":"unece:TransportPerson"},"rdfs:comment":"A unique identifier of a language related to this transport person, such as their spoken or correspondence language."},{"@id":"unece:transportPersonName","@type":["rdf:Property","owl:DatatypeProperty"],"rdfs:label":"transportPersonName","schema:rangeIncludes":{"@id":"schema:Text"},"schema:domainIncludes":{"@id":"unece:TransportPerson"},"rdfs:comment":"The name or set of names, expressed as text, by which this transport person is known."},{"@id":"unece:travelIdentityDocument","@type":["rdf:Property","owl:ObjectProperty"],"rdfs:label":"travelIdentityDocument","schema:rangeIncludes":{"@id":"unece:Document"},"schema:domainIncludes":{"@id":"unece:TransportPerson"},"rdfs:comment":"Written, printed or electronic matter that is referenced."},{"@id":"unece:travelVisaDocument","@type":["rdf:Property","owl:ObjectProperty"],"rdfs:label":"travelVisaDocument","schema:rangeIncludes":{"@id":"unece:Document"},"schema:domainIncludes":{"@id":"unece:TransportPerson"},"rdfs:comment":"Written, printed or electronic matter that is referenced."},{"@id":"unece:automaticDataCaptureMethodTypeCode","@type":["rdf:Property","owl:DatatypeProperty"],"rdfs:label":"automaticDataCaptureMethodTypeCode","schema:rangeIncludes":{"@id":"unece:AutomaticDataCaptureMethodCodeList"},"schema:domainIncludes":{"@id":"unece:Marking"},"rdfs:comment":"A code specifying an automatic data capture method type for this packaging marking."},{"@id":"unece:contentAmount","@type":["rdf:Property","owl:ObjectProperty"],"rdfs:label":"contentAmount","schema:rangeIncludes":{"@id":"unece:AmountType"},"schema:domainIncludes":{"@id":"unece:Marking"},"rdfs:comment":""},{"@id":"unece:contentDateTime","@type":["rdf:Property","owl:DatatypeProperty"],"rdfs:label":"contentDateTime","schema:rangeIncludes":{"@id":"schema:Text"},"schema:domainIncludes":{"@id":"unece:Marking"},"rdfs:comment":"The date, time, date time or other date time value for the content of this packaging marking."},{"@id":"unece:packagingMarkingBarcodeTypeCode","@type":["rdf:Property","owl:DatatypeProperty"],"rdfs:label":"packagingMarkingBarcodeTypeCode","schema:rangeIncludes":{"@id":"schema:Text"},"schema:domainIncludes":{"@id":"unece:Marking"},"rdfs:comment":"A code specifying a type of barcode for this packaging marking."},{"@id":"unece:packagingMarkingTypeCode","@type":["rdf:Property","owl:DatatypeProperty"],"rdfs:label":"packagingMarkingTypeCode","schema:rangeIncludes":{"@id":"unece:PackagingMarkingCodeList"},"schema:domainIncludes":{"@id":"unece:Marking"},"rdfs:comment":"A code specifying a type of packaging marking."},{"@id":"unece:barcodeLabel","@type":["rdf:Property","owl:ObjectProperty"],"rdfs:label":"barcodeLabel","schema:rangeIncludes":{"@id":"unece:LogisticsLabel"},"schema:domainIncludes":{"@id":"unece:ShippingMarks"},"rdfs:comment":"A barcode label that is a part of these logistics shipping marks."},{"@id":"unece:logisticsShippingMarksMarkingInstructionCode","@type":["rdf:Property","owl:DatatypeProperty"],"rdfs:label":"logisticsShippingMarksMarkingInstructionCode","schema:rangeIncludes":{"@id":"unece:MarkingInstructionCodeList"},"schema:domainIncludes":{"@id":"unece:ShippingMarks"},"rdfs:comment":"A code specifying a marking instruction for these logistics shipping marks."},{"@id":"unece:rFIDLabel","@type":["rdf:Property","owl:ObjectProperty"],"rdfs:label":"rFIDLabel","schema:rangeIncludes":{"@id":"unece:LogisticsLabel"},"schema:domainIncludes":{"@id":"unece:ShippingMarks"},"rdfs:comment":"A Radio Frequency Identification (RFID) label that is a part of these logistics shipping marks."},{"@id":"unece:radioactiveLabel","@type":["rdf:Property","owl:ObjectProperty"],"rdfs:label":"radioactiveLabel","schema:rangeIncludes":{"@id":"unece:LogisticsLabel"},"schema:domainIncludes":{"@id":"unece:ShippingMarks"},"rdfs:comment":"Radioactive labelling that is a part of these logistics shipping marks."},{"@id":"unece:vINLabel","@type":["rdf:Property","owl:ObjectProperty"],"rdfs:label":"vINLabel","schema:rangeIncludes":{"@id":"unece:LogisticsLabel"},"schema:domainIncludes":{"@id":"unece:ShippingMarks"},"rdfs:comment":"A Vehicle Identification Number (VIN) label that is a part of these logistics shipping marks."},{"@id":"unece:careProvided","@type":["rdf:Property","owl:DatatypeProperty"],"rdfs:label":"careProvided","schema:rangeIncludes":{"@id":"schema:Text"},"schema:domainIncludes":{"@id":"unece:Stowaway"},"rdfs:comment":"Care, expressed as text, that has been provided to this found stowaway."},{"@id":"unece:countryClaimedNationalityId","@type":["rdf:Property","owl:DatatypeProperty"],"rdfs:label":"countryClaimedNationalityId","schema:rangeIncludes":{"@id":"unece:CountryId"},"schema:domainIncludes":{"@id":"unece:Stowaway"},"rdfs:comment":"An identifier of a nationality claimed by this found stowaway."},{"@id":"unece:discoveredDateTime","@type":["rdf:Property","owl:DatatypeProperty"],"rdfs:label":"discoveredDateTime","schema:rangeIncludes":{"@id":"schema:DateTime"},"schema:domainIncludes":{"@id":"unece:Stowaway"},"rdfs:comment":"A date, time, date time, or other date time value on which this found stowaway is discovered."},{"@id":"unece:homeAddress","@type":["rdf:Property","owl:ObjectProperty"],"rdfs:label":"homeAddress","schema:rangeIncludes":{"@id":"unece:Address"},"schema:domainIncludes":{"@id":"unece:Stowaway"},"rdfs:comment":"The location at which a particular trade related organization or person may be found or reached."},{"@id":"unece:intendedDestinationLocationCode","@type":["rdf:Property","owl:DatatypeProperty"],"rdfs:label":"intendedDestinationLocationCode","schema:rangeIncludes":{"@id":"schema:Text"},"schema:domainIncludes":{"@id":"unece:Stowaway"},"rdfs:comment":"A code specifying a location of an intended destination for this found stowaway."},{"@id":"unece:intendedDestinationName","@type":["rdf:Property","owl:DatatypeProperty"],"rdfs:label":"intendedDestinationName","schema:rangeIncludes":{"@id":"schema:Text"},"schema:domainIncludes":{"@id":"unece:Stowaway"},"rdfs:comment":"A name, expressed as text, of an intended destination for this found stowaway."},{"@id":"unece:interviewDateTime","@type":["rdf:Property","owl:DatatypeProperty"],"rdfs:label":"interviewDateTime","schema:rangeIncludes":{"@id":"schema:DateTime"},"schema:domainIncludes":{"@id":"unece:Stowaway"},"rdfs:comment":"A date, time, date time, or other date time value on which this found stowaway is interviewed."},{"@id":"unece:personalStatement","@type":["rdf:Property","owl:DatatypeProperty"],"rdfs:label":"personalStatement","schema:rangeIncludes":{"@id":"schema:Text"},"schema:domainIncludes":{"@id":"unece:Stowaway"},"rdfs:comment":"A personal statement, expressed as text, made by this found stowaway."},{"@id":"unece:photographicPictureBinaryFile","@type":["rdf:Property","owl:ObjectProperty"],"rdfs:label":"photographicPictureBinaryFile","schema:rangeIncludes":{"@id":"unece:BinaryFile"},"schema:domainIncludes":{"@id":"unece:Stowaway"},"rdfs:comment":"A specified computer file or program stored in a binary format."},{"@id":"unece:physicalDescription","@type":["rdf:Property","owl:DatatypeProperty"],"rdfs:label":"physicalDescription","schema:rangeIncludes":{"@id":"schema:Text"},"schema:domainIncludes":{"@id":"unece:Stowaway"},"rdfs:comment":"The physical description, expressed as text, of this found stowaway."},{"@id":"unece:possessionList","@type":["rdf:Property","owl:DatatypeProperty"],"rdfs:label":"possessionList","schema:rangeIncludes":{"@id":"schema:Text"},"schema:domainIncludes":{"@id":"unece:Stowaway"},"rdfs:comment":"A list of possessions, expressed as text, for this found stowaway."},{"@id":"unece:providedName","@type":["rdf:Property","owl:DatatypeProperty"],"rdfs:label":"providedName","schema:rangeIncludes":{"@id":"schema:Text"},"schema:domainIncludes":{"@id":"unece:Stowaway"},"rdfs:comment":"A name, expressed as text, as provided by this found stowaway."},{"@id":"unece:responsiblePersonStatement","@type":["rdf:Property","owl:DatatypeProperty"],"rdfs:label":"responsiblePersonStatement","schema:rangeIncludes":{"@id":"schema:Text"},"schema:domainIncludes":{"@id":"unece:Stowaway"},"rdfs:comment":"A statement, expressed as text, about the stowaway made by the person responsible for operating the means of transport on which the stowaway was found."},{"@id":"unece:statedEmbarkationMethod","@type":["rdf:Property","owl:DatatypeProperty"],"rdfs:label":"statedEmbarkationMethod","schema:rangeIncludes":{"@id":"schema:Text"},"schema:domainIncludes":{"@id":"unece:Stowaway"},"rdfs:comment":"A method, expressed as text, of embarkation stated by this found stowaway."},{"@id":"unece:statedEmbarkationReason","@type":["rdf:Property","owl:DatatypeProperty"],"rdfs:label":"statedEmbarkationReason","schema:rangeIncludes":{"@id":"schema:Text"},"schema:domainIncludes":{"@id":"unece:Stowaway"},"rdfs:comment":"A reason, expressed as text, for embarkation stated by this found stowaway."},{"@id":"unece:cargoCategoryTypeCode","@type":["rdf:Property","owl:DatatypeProperty"],"rdfs:label":"cargoCategoryTypeCode","schema:rangeIncludes":{"@id":"unece:CargoCategoryCodeList"},"schema:domainIncludes":{"@id":"unece:Cargo"},"rdfs:comment":"The code, such as UNECE Recommendation 21 single digit codes, specifying the type of transported cargo."},{"@id":"unece:cargoCommodityCategoryStatisticalClassificationCode","@type":["rdf:Property","owl:DatatypeProperty"],"rdfs:label":"cargoCommodityCategoryStatisticalClassificationCode","schema:rangeIncludes":{"@id":"unece:CargoCommodityCategoryCodeList"},"schema:domainIncludes":{"@id":"unece:Cargo"},"rdfs:comment":"The code specifying a statistical classification for this transport cargo."},{"@id":"unece:cargoOperationalCategoryCode","@type":["rdf:Property","owl:DatatypeProperty"],"rdfs:label":"cargoOperationalCategoryCode","schema:rangeIncludes":{"@id":"unece:CargoOperationalCategoryCodeList"},"schema:domainIncludes":{"@id":"unece:Cargo"},"rdfs:comment":"The code specifying the operational category for this transport cargo, such as obnoxious or military."},{"@id":"unece:identification","@type":["rdf:Property","owl:DatatypeProperty"],"rdfs:label":"identification","schema:rangeIncludes":{"@id":"schema:Text"},"schema:domainIncludes":{"@id":"unece:Cargo"},"rdfs:comment":"Identification, expressed as text, of this transport cargo that is sufficient to identify it for customs, statistical or transport purposes."},{"@id":"unece:caseDispositionCode","@type":["rdf:Property","owl:DatatypeProperty"],"rdfs:label":"caseDispositionCode","schema:rangeIncludes":{"@id":"schema:Text"},"schema:domainIncludes":{"@id":"unece:Illness"},"rdfs:comment":"A code specifying a case disposition of this MDH illness."},{"@id":"unece:evacuationLocation","@type":["rdf:Property","owl:ObjectProperty"],"rdfs:label":"evacuationLocation","schema:rangeIncludes":{"@id":"unece:LogisticsLocation"},"schema:domainIncludes":{"@id":"unece:Illness"},"rdfs:comment":"A logistics evacuation location for this MDH illness."},{"@id":"unece:healthStatusCode","@type":["rdf:Property","owl:DatatypeProperty"],"rdfs:label":"healthStatusCode","schema:rangeIncludes":{"@id":"schema:Text"},"schema:domainIncludes":{"@id":"unece:Illness"},"rdfs:comment":"A code specifying a health status of this MDH illness."},{"@id":"unece:healthStatusReportedIndicator","@type":["rdf:Property","owl:DatatypeProperty"],"rdfs:label":"healthStatusReportedIndicator","schema:rangeIncludes":{"@id":"schema:Boolean"},"schema:domainIncludes":{"@id":"unece:Illness"},"rdfs:comment":"The indication of whether or not the health status has been reported for this MDH illness."},{"@id":"unece:nature","@type":["rdf:Property","owl:DatatypeProperty"],"rdfs:label":"nature","schema:rangeIncludes":{"@id":"schema:Text"},"schema:domainIncludes":{"@id":"unece:Illness"},"rdfs:comment":"A nature, expressed as text, of this MDH illness."},{"@id":"unece:symptomOnsetDateTime","@type":["rdf:Property","owl:DatatypeProperty"],"rdfs:label":"symptomOnsetDateTime","schema:rangeIncludes":{"@id":"schema:DateTime"},"schema:domainIncludes":{"@id":"unece:Illness"},"rdfs:comment":"A symptom onset date, time, date time or other date time value for this MDH illness."},{"@id":"unece:treatment","@type":["rdf:Property","owl:DatatypeProperty"],"rdfs:label":"treatment","schema:rangeIncludes":{"@id":"schema:Text"},"schema:domainIncludes":{"@id":"unece:Illness"},"rdfs:comment":"A treatment, expressed as text, for this MDH illness."},{"@id":"unece:contractGeneralConditions","@type":["rdf:Property","owl:DatatypeProperty"],"rdfs:label":"contractGeneralConditions","schema:rangeIncludes":{"@id":"schema:Text"},"schema:domainIncludes":{"@id":"unece:CargoInsurance"},"rdfs:comment":"The contract general conditions, expressed as text, for this transport cargo insurance."},{"@id":"unece:coverageCode","@type":["rdf:Property","owl:DatatypeProperty"],"rdfs:label":"coverageCode","schema:rangeIncludes":{"@id":"schema:Text"},"schema:domainIncludes":{"@id":"unece:CargoInsurance"},"rdfs:comment":"The code specifying the coverage of this transport cargo insurance."},{"@id":"unece:coverageDescription","@type":["rdf:Property","owl:DatatypeProperty"],"rdfs:label":"coverageDescription","schema:rangeIncludes":{"@id":"schema:Text"},"schema:domainIncludes":{"@id":"unece:CargoInsurance"},"rdfs:comment":"The textual description of the coverage of this transport cargo insurance."},{"@id":"unece:coverageParty","@type":["rdf:Property","owl:ObjectProperty"],"rdfs:label":"coverageParty","schema:rangeIncludes":{"@id":"unece:Party"},"schema:domainIncludes":{"@id":"unece:CargoInsurance"},"rdfs:comment":""},{"@id":"unece:controlCode","@type":["rdf:Property","owl:DatatypeProperty"],"rdfs:label":"controlCode","schema:rangeIncludes":{"@id":"schema:Text"},"schema:domainIncludes":{"@id":"unece:InstructedTemperature"},"rdfs:comment":"The code specifying the control of this instructed temperature, such as normal or chilled."},{"@id":"unece:departurePoint","@type":["rdf:Property","owl:DatatypeProperty"],"rdfs:label":"departurePoint","schema:rangeIncludes":{"@id":"schema:Text"},"schema:domainIncludes":[{"@id":"unece:SpecifiedRoute"},{"@id":"unece:TransportRoute"}],"rdfs:comment":"A departure point, expressed as text, for this specified route."},{"@id":"unece:linearUnitDistanceMeasure","@type":["rdf:Property","owl:ObjectProperty"],"rdfs:label":"linearUnitDistanceMeasure","schema:rangeIncludes":{"@id":"unece:LinearUnitMeasureType"},"schema:domainIncludes":{"@id":"unece:SpecifiedRoute"},"rdfs:comment":""},{"@id":"unece:routeType","@type":["rdf:Property","owl:DatatypeProperty"],"rdfs:label":"routeType","schema:rangeIncludes":{"@id":"schema:Text"},"schema:domainIncludes":[{"@id":"unece:SpecifiedRoute"},{"@id":"unece:TransportRoute"}],"rdfs:comment":"A type, expressed as text, for this specified route."},{"@id":"unece:transportMeans","@type":["rdf:Property","owl:DatatypeProperty"],"rdfs:label":"transportMeans","schema:rangeIncludes":{"@id":"schema:Text"},"schema:domainIncludes":[{"@id":"unece:SpecifiedRoute"},{"@id":"unece:TransportRoute"}],"rdfs:comment":"A means of transport, expressed as text, for this transport route."},{"@id":"unece:frequencyEffectivePeriod","@type":["rdf:Property","owl:ObjectProperty"],"rdfs:label":"frequencyEffectivePeriod","schema:rangeIncludes":{"@id":"unece:SpecifiedPeriod"},"schema:domainIncludes":{"@id":"unece:TransportRoute"},"rdfs:comment":"A specified period of time."},{"@id":"unece:frequencyTypeCode","@type":["rdf:Property","owl:DatatypeProperty"],"rdfs:label":"frequencyTypeCode","schema:rangeIncludes":{"@id":"schema:Text"},"schema:domainIncludes":{"@id":"unece:TransportRoute"},"rdfs:comment":"The code specifying the type of frequency for this transport route, such as weekly, bi-monthly or daily."},{"@id":"unece:itineraryStopEvent","@type":["rdf:Property","owl:ObjectProperty"],"rdfs:label":"itineraryStopEvent","schema:rangeIncludes":{"@id":"unece:TransportEvent"},"schema:domainIncludes":{"@id":"unece:TransportRoute"},"rdfs:comment":"An itinerary stop event for this transport route, such as a port call in a vessel schedule."},{"@id":"unece:mapBinaryObject","@type":["rdf:Property","owl:DatatypeProperty"],"rdfs:label":"mapBinaryObject","schema:rangeIncludes":{"@id":"schema:Text"},"schema:domainIncludes":{"@id":"unece:TransportRoute"},"rdfs:comment":"Binary object data that is the map of this transport route."},{"@id":"unece:scheduledPeriod","@type":["rdf:Property","owl:ObjectProperty"],"rdfs:label":"scheduledPeriod","schema:rangeIncludes":{"@id":"unece:SpecifiedPeriod"},"schema:domainIncludes":{"@id":"unece:TransportRoute"},"rdfs:comment":"A specified period of time."},{"@id":"unece:transportRouteStatusCode","@type":["rdf:Property","owl:DatatypeProperty"],"rdfs:label":"transportRouteStatusCode","schema:rangeIncludes":{"@id":"unece:StatusCodeList"},"schema:domainIncludes":{"@id":"unece:TransportRoute"},"rdfs:comment":"The code specifying a status for a transport route, such as planned or actual."},{"@id":"unece:depositValueSpecifiedAmount","@type":["rdf:Property","owl:ObjectProperty"],"rdfs:label":"depositValueSpecifiedAmount","schema:rangeIncludes":{"@id":"unece:AmountType"},"schema:domainIncludes":{"@id":"unece:ReturnableAssetInstructions"},"rdfs:comment":""},{"@id":"unece:depositValueValidityPeriod","@type":["rdf:Property","owl:ObjectProperty"],"rdfs:label":"depositValueValidityPeriod","schema:rangeIncludes":{"@id":"unece:SpecifiedPeriod"},"schema:domainIncludes":{"@id":"unece:ReturnableAssetInstructions"},"rdfs:comment":"A specified period of time."},{"@id":"unece:returnableAssetInstructionsTermsAndConditionsDescriptionCode","@type":["rdf:Property","owl:DatatypeProperty"],"rdfs:label":"returnableAssetInstructionsTermsAndConditionsDescriptionCode","schema:rangeIncludes":{"@id":"schema:Text"},"schema:domainIncludes":{"@id":"unece:ReturnableAssetInstructions"},"rdfs:comment":"The code specifying the description of the terms and conditions for these returnable asset instructions."},{"@id":"unece:termsAndConditionsDescription","@type":["rdf:Property","owl:DatatypeProperty"],"rdfs:label":"termsAndConditionsDescription","schema:rangeIncludes":{"@id":"schema:Text"},"schema:domainIncludes":{"@id":"unece:ReturnableAssetInstructions"},"rdfs:comment":"A textual description of the terms and conditions for these returnable asset instructions."},{"@id":"unece:haulageInstructionsDescriptionCode","@type":["rdf:Property","owl:DatatypeProperty"],"rdfs:label":"haulageInstructionsDescriptionCode","schema:rangeIncludes":{"@id":"schema:Text"},"schema:domainIncludes":{"@id":"unece:HaulageInstructions"},"rdfs:comment":"The code specifying the description of these haulage instructions."},{"@id":"unece:handling","@type":["rdf:Property","owl:DatatypeProperty"],"rdfs:label":"handling","schema:rangeIncludes":{"@id":"schema:Text"},"schema:domainIncludes":[{"@id":"unece:PackagingInstructions"},{"@id":"unece:DeliveryInstructions"}],"rdfs:comment":"Delivery handling instructions expressed as text."},{"@id":"unece:itemName","@type":["rdf:Property","owl:DatatypeProperty"],"rdfs:label":"itemName","schema:rangeIncludes":{"@id":"schema:Text"},"schema:domainIncludes":{"@id":"unece:PackagingInstructions"},"rdfs:comment":"A name, expressed as text, of an item included in these packaging instructions."},{"@id":"unece:packagingInstructionsDescriptionCode","@type":["rdf:Property","owl:DatatypeProperty"],"rdfs:label":"packagingInstructionsDescriptionCode","schema:rangeIncludes":{"@id":"schema:Text"},"schema:domainIncludes":{"@id":"unece:PackagingInstructions"},"rdfs:comment":"The code specifying a description of these packaging instructions."},{"@id":"unece:diedOnboardHealthIndication","@type":["rdf:Property","owl:ObjectProperty"],"rdfs:label":"diedOnboardHealthIndication","schema:rangeIncludes":{"@id":"unece:MDHHealthIndication"},"schema:domainIncludes":{"@id":"unece:TransportationHealth"},"rdfs:comment":"A died onboard indication for this MDH transportation health."},{"@id":"unece:diseaseOnboardHealthIndication","@type":["rdf:Property","owl:ObjectProperty"],"rdfs:label":"diseaseOnboardHealthIndication","schema:rangeIncludes":{"@id":"unece:MDHHealthIndication"},"schema:domainIncludes":{"@id":"unece:TransportationHealth"},"rdfs:comment":"A disease onboard indication for this MDH transportation health."},{"@id":"unece:illPersonNowOnboardHealthIndication","@type":["rdf:Property","owl:ObjectProperty"],"rdfs:label":"illPersonNowOnboardHealthIndication","schema:rangeIncludes":{"@id":"unece:MDHHealthIndication"},"schema:domainIncludes":{"@id":"unece:TransportationHealth"},"rdfs:comment":"An ill person or persons now onboard indication for this MDH transportation health."},{"@id":"unece:medicalPractitionerConsultedHealthIndication","@type":["rdf:Property","owl:ObjectProperty"],"rdfs:label":"medicalPractitionerConsultedHealthIndication","schema:rangeIncludes":{"@id":"unece:MDHHealthIndication"},"schema:domainIncludes":{"@id":"unece:TransportationHealth"},"rdfs:comment":"A medical practitioner consulted indication for this MDH transportation health."},{"@id":"unece:moreIllOnboardHealthIndication","@type":["rdf:Property","owl:ObjectProperty"],"rdfs:label":"moreIllOnboardHealthIndication","schema:rangeIncludes":{"@id":"unece:MDHHealthIndication"},"schema:domainIncludes":{"@id":"unece:TransportationHealth"},"rdfs:comment":"A more ill onboard indication for this MDH transportation health."},{"@id":"unece:onboardInfectionConditionHealthIndication","@type":["rdf:Property","owl:ObjectProperty"],"rdfs:label":"onboardInfectionConditionHealthIndication","schema:rangeIncludes":{"@id":"unece:MDHHealthIndication"},"schema:domainIncludes":{"@id":"unece:TransportationHealth"},"rdfs:comment":"An onboard infection condition indication for this MDH transportation health."},{"@id":"unece:sanitaryMeasureAppliedHealthIndication","@type":["rdf:Property","owl:ObjectProperty"],"rdfs:label":"sanitaryMeasureAppliedHealthIndication","schema:rangeIncludes":{"@id":"unece:MDHHealthIndication"},"schema:domainIncludes":{"@id":"unece:TransportationHealth"},"rdfs:comment":"An applied sanitary measure indication for this MDH transportation health."},{"@id":"unece:sickAnimalOnboardHealthIndication","@type":["rdf:Property","owl:ObjectProperty"],"rdfs:label":"sickAnimalOnboardHealthIndication","schema:rangeIncludes":{"@id":"unece:MDHHealthIndication"},"schema:domainIncludes":{"@id":"unece:TransportationHealth"},"rdfs:comment":"A sick animal or animals onboard indication for this MDH transportation health."},{"@id":"unece:stowawayFoundOnboardHealthIndication","@type":["rdf:Property","owl:ObjectProperty"],"rdfs:label":"stowawayFoundOnboardHealthIndication","schema:rangeIncludes":{"@id":"unece:MDHHealthIndication"},"schema:domainIncludes":{"@id":"unece:TransportationHealth"},"rdfs:comment":"A stowaway or stowaways found onboard indication for this MDH transportation health."},{"@id":"unece:includedSection","@type":["rdf:Property","owl:ObjectProperty"],"rdfs:label":"includedSection","schema:rangeIncludes":{"@id":"unece:Section"},"schema:domainIncludes":{"@id":"unece:LogisticsLabel"},"rdfs:comment":"The parts into which a label is or may be divided."},{"@id":"unece:markingIndicator","@type":["rdf:Property","owl:DatatypeProperty"],"rdfs:label":"markingIndicator","schema:rangeIncludes":{"@id":"schema:Boolean"},"schema:domainIncludes":{"@id":"unece:LogisticsLabel"},"rdfs:comment":"The indication of whether or not there is a marking on this logistics label."},{"@id":"unece:informationInstructions","@type":["rdf:Property","owl:ObjectProperty"],"rdfs:label":"informationInstructions","schema:rangeIncludes":{"@id":"unece:TemperatureSettingInstructions"},"schema:domainIncludes":{"@id":"unece:TransportSettingTemperature"},"rdfs:comment":"Temperature setting related information of an instructive nature."},{"@id":"unece:temperatureTypeCode","@type":["rdf:Property","owl:DatatypeProperty"],"rdfs:label":"temperatureTypeCode","schema:rangeIncludes":{"@id":"unece:TemperatureTypeCodeList"},"schema:domainIncludes":{"@id":"unece:TransportSettingTemperature"},"rdfs:comment":"The code specifying the type of transport setting temperature [Reference United Nations Code List (UNCL) 6245]."},{"@id":"unece:maximumWidthMeasure","@type":["rdf:Property","owl:ObjectProperty"],"rdfs:label":"maximumWidthMeasure","schema:rangeIncludes":{"@id":"unece:LinearUnitMeasureType"},"schema:domainIncludes":{"@id":"unece:Convoy"},"rdfs:comment":""},{"@id":"unece:overallLengthMeasure","@type":["rdf:Property","owl:ObjectProperty"],"rdfs:label":"overallLengthMeasure","schema:rangeIncludes":{"@id":"unece:LinearUnitMeasureType"},"schema:domainIncludes":{"@id":"unece:Convoy"},"rdfs:comment":""},{"@id":"unece:powerActiveTransportMeans","@type":["rdf:Property","owl:ObjectProperty"],"rdfs:label":"powerActiveTransportMeans","schema:rangeIncludes":{"@id":"unece:LogisticsTransportMeans"},"schema:domainIncludes":{"@id":"unece:Convoy"},"rdfs:comment":"A means of transport actively powering this logistics convoy."},{"@id":"unece:powerInactiveTransportMeans","@type":["rdf:Property","owl:ObjectProperty"],"rdfs:label":"powerInactiveTransportMeans","schema:rangeIncludes":{"@id":"unece:LogisticsTransportMeans"},"schema:domainIncludes":{"@id":"unece:Convoy"},"rdfs:comment":"A means of transport not actively powering this logistics convoy."},{"@id":"unece:transportMeansQuantity","@type":["rdf:Property","owl:ObjectProperty"],"rdfs:label":"transportMeansQuantity","schema:rangeIncludes":{"@id":"unece:QuantityType"},"schema:domainIncludes":{"@id":"unece:Convoy"},"rdfs:comment":""},{"@id":"unece:actualReportedMeasurement","@type":["rdf:Property","owl:ObjectProperty"],"rdfs:label":"actualReportedMeasurement","schema:rangeIncludes":{"@id":"unece:CalibratedMeasurement"},"schema:domainIncludes":{"@id":"unece:Sensor"},"rdfs:comment":"A measurement established by a device which is tested to a calibration standard of known accuracy."},{"@id":"unece:definedControlSettingParameter","@type":["rdf:Property","owl:ObjectProperty"],"rdfs:label":"definedControlSettingParameter","schema:rangeIncludes":{"@id":"unece:ControlSettingParameter"},"schema:domainIncludes":{"@id":"unece:Sensor"},"rdfs:comment":"A set of measurable factors that specifies the conditions of its operation within a specific context."},{"@id":"unece:definedOperationalParameter","@type":["rdf:Property","owl:ObjectProperty"],"rdfs:label":"definedOperationalParameter","schema:rangeIncludes":{"@id":"unece:OperationalParameter"},"schema:domainIncludes":{"@id":"unece:Sensor"},"rdfs:comment":"A set of measurable factors that specifies the conditions within which an entity operates correctly."},{"@id":"unece:precisionMeasurement","@type":["rdf:Property","owl:ObjectProperty"],"rdfs:label":"precisionMeasurement","schema:rangeIncludes":{"@id":"unece:CalibratedMeasurement"},"schema:domainIncludes":{"@id":"unece:Sensor"},"rdfs:comment":"A measurement established by a device which is tested to a calibration standard of known accuracy."},{"@id":"unece:scheduledReportedMeasurement","@type":["rdf:Property","owl:ObjectProperty"],"rdfs:label":"scheduledReportedMeasurement","schema:rangeIncludes":{"@id":"unece:CalibratedMeasurement"},"schema:domainIncludes":{"@id":"unece:Sensor"},"rdfs:comment":"A measurement established by a device which is tested to a calibration standard of known accuracy."},{"@id":"unece:specifiedMeasurement","@type":["rdf:Property","owl:ObjectProperty"],"rdfs:label":"specifiedMeasurement","schema:rangeIncludes":{"@id":"unece:CalibratedMeasurement"},"schema:domainIncludes":{"@id":"unece:SpecifiedCondition"},"rdfs:comment":"A measurement established by a device which is tested to a calibration standard of known accuracy."},{"@id":"unece:locationPartyRoleCode","@type":["rdf:Property","owl:DatatypeProperty"],"rdfs:label":"locationPartyRoleCode","schema:rangeIncludes":{"@id":"schema:Text"},"schema:domainIncludes":{"@id":"unece:LocationParty"},"rdfs:comment":"A code specifying a role of this location party."},{"@id":"unece:specifiedTransportPerson","@type":["rdf:Property","owl:ObjectProperty"],"rdfs:label":"specifiedTransportPerson","schema:rangeIncludes":{"@id":"unece:TransportPerson"},"schema:domainIncludes":{"@id":"unece:LocationParty"},"rdfs:comment":"A transport related person specified for this location party."},{"@id":"unece:adjustmentReasonCode","@type":["rdf:Property","owl:DatatypeProperty"],"rdfs:label":"adjustmentReasonCode","schema:rangeIncludes":{"@id":"unece:AdjustmentReasonCodeList"},"schema:domainIncludes":{"@id":"unece:DeliveryAdjustment"},"rdfs:comment":"The code specifying a reason for this delivery adjustment."},{"@id":"unece:additionalInstructionCode","@type":["rdf:Property","owl:DatatypeProperty"],"rdfs:label":"additionalInstructionCode","schema:rangeIncludes":{"@id":"schema:Text"},"schema:domainIncludes":{"@id":"unece:SupplyChainPackaging"},"rdfs:comment":"A code specifying an additional instruction for this supply chain packaging."},{"@id":"unece:additionalInstructionIndicator","@type":["rdf:Property","owl:DatatypeProperty"],"rdfs:label":"additionalInstructionIndicator","schema:rangeIncludes":{"@id":"schema:Boolean"},"schema:domainIncludes":{"@id":"unece:SupplyChainPackaging"},"rdfs:comment":"The indication of whether or not there is an additional instruction for this supply chain packaging."},{"@id":"unece:applicableReturnableAssetInstructions","@type":["rdf:Property","owl:ObjectProperty"],"rdfs:label":"applicableReturnableAssetInstructions","schema:rangeIncludes":{"@id":"unece:ReturnableAssetInstructions"},"schema:domainIncludes":{"@id":"unece:SupplyChainPackaging"},"rdfs:comment":"Returnable asset instructions for this supply chain packaging."},{"@id":"unece:customerFacingTotalUnitQuantity","@type":["rdf:Property","owl:ObjectProperty"],"rdfs:label":"customerFacingTotalUnitQuantity","schema:rangeIncludes":{"@id":"unece:QuantityType"},"schema:domainIncludes":{"@id":"unece:SupplyChainPackaging"},"rdfs:comment":""},{"@id":"unece:layerTotalUnitQuantity","@type":["rdf:Property","owl:ObjectProperty"],"rdfs:label":"layerTotalUnitQuantity","schema:rangeIncludes":{"@id":"unece:QuantityType"},"schema:domainIncludes":{"@id":"unece:SupplyChainPackaging"},"rdfs:comment":""},{"@id":"unece:maximumStackabilityWeightMeasure","@type":["rdf:Property","owl:ObjectProperty"],"rdfs:label":"maximumStackabilityWeightMeasure","schema:rangeIncludes":{"@id":"unece:MeasureType"},"schema:domainIncludes":{"@id":"unece:SupplyChainPackaging"},"rdfs:comment":""},{"@id":"unece:associatedReference","@type":["rdf:Property","owl:ObjectProperty"],"rdfs:label":"associatedReference","schema:rangeIncludes":{"@id":"unece:SupplyChainReference"},"schema:domainIncludes":{"@id":"unece:SupplyChainEvent"},"rdfs:comment":"A reference associated with this supply chain event."},{"@id":"unece:descriptionBinaryObject","@type":["rdf:Property","owl:DatatypeProperty"],"rdfs:label":"descriptionBinaryObject","schema:rangeIncludes":{"@id":"schema:Text"},"schema:domainIncludes":{"@id":"unece:SupplyChainEvent"},"rdfs:comment":"Binary object data, such as a photograph, describing this supply chain event."},{"@id":"unece:earliestOccurrenceDateTime","@type":["rdf:Property","owl:DatatypeProperty"],"rdfs:label":"earliestOccurrenceDateTime","schema:rangeIncludes":{"@id":"schema:Text"},"schema:domainIncludes":{"@id":"unece:SupplyChainEvent"},"rdfs:comment":"The date, time, date time, or other date time value of the earliest occurrence of this supply chain event."},{"@id":"unece:frequencyCode","@type":["rdf:Property","owl:DatatypeProperty"],"rdfs:label":"frequencyCode","schema:rangeIncludes":{"@id":"schema:Text"},"schema:domainIncludes":{"@id":"unece:SupplyChainEvent"},"rdfs:comment":"The code specifying a frequency for this supply chain event."},{"@id":"unece:latestOccurrenceDateTime","@type":["rdf:Property","owl:DatatypeProperty"],"rdfs:label":"latestOccurrenceDateTime","schema:rangeIncludes":{"@id":"schema:Text"},"schema:domainIncludes":{"@id":"unece:SupplyChainEvent"},"rdfs:comment":"The date, time, date time, or other date time value of the latest occurrence of this supply chain event."},{"@id":"unece:relatedSustainabilityCharacteristic","@type":["rdf:Property","owl:ObjectProperty"],"rdfs:label":"relatedSustainabilityCharacteristic","schema:rangeIncludes":{"@id":"unece:SustainabilityCharacteristic"},"schema:domainIncludes":{"@id":"unece:SupplyChainEvent"},"rdfs:comment":"A prominent attribute or aspect of an object, such as recyclability of a product, which can meet customer needs without compromising the ability of future generations to meet their own needs."},{"@id":"unece:relatedTechnicalCharacteristic","@type":["rdf:Property","owl:ObjectProperty"],"rdfs:label":"relatedTechnicalCharacteristic","schema:rangeIncludes":{"@id":"unece:TechnicalCharacteristic"},"schema:domainIncludes":{"@id":"unece:SupplyChainEvent"},"rdfs:comment":"A prominent technical attribute or aspect."},{"@id":"unece:timeOccurrenceDateTime","@type":["rdf:Property","owl:DatatypeProperty"],"rdfs:label":"timeOccurrenceDateTime","schema:rangeIncludes":{"@id":"schema:DateTime"},"schema:domainIncludes":{"@id":"unece:SupplyChainEvent"},"rdfs:comment":"A time value of an occurrence of this supply chain event."},{"@id":"unece:deliveryDiscontinuationCode","@type":["rdf:Property","owl:DatatypeProperty"],"rdfs:label":"deliveryDiscontinuationCode","schema:rangeIncludes":{"@id":"schema:Text"},"schema:domainIncludes":{"@id":"unece:DeliveryTerms"},"rdfs:comment":"The code specifying the delivery discontinuation for this trade delivery terms."},{"@id":"unece:deliveryTermsDeliveryTypeCode","@type":["rdf:Property","owl:DatatypeProperty"],"rdfs:label":"deliveryTermsDeliveryTypeCode","schema:rangeIncludes":{"@id":"unece:DeliveryTermsCodeList"},"schema:domainIncludes":{"@id":"unece:DeliveryTerms"},"rdfs:comment":"The code specifying the type of delivery for these trade delivery terms."},{"@id":"unece:deliveryTermsFunctionCode","@type":["rdf:Property","owl:DatatypeProperty"],"rdfs:label":"deliveryTermsFunctionCode","schema:rangeIncludes":{"@id":"unece:DeliveryTermsFunctionCodeList"},"schema:domainIncludes":{"@id":"unece:DeliveryTerms"},"rdfs:comment":"A code specifying a function of these trade delivery terms."},{"@id":"unece:relevantLocation","@type":["rdf:Property","owl:ObjectProperty"],"rdfs:label":"relevantLocation","schema:rangeIncludes":{"@id":"unece:Location"},"schema:domainIncludes":{"@id":"unece:DeliveryTerms"},"rdfs:comment":"A reference to a physical location or place."},{"@id":"unece:deliveryInstructionsDescriptionCode","@type":["rdf:Property","owl:DatatypeProperty"],"rdfs:label":"deliveryInstructionsDescriptionCode","schema:rangeIncludes":{"@id":"schema:Text"},"schema:domainIncludes":{"@id":"unece:DeliveryInstructions"},"rdfs:comment":"The code specifying a description of these delivery instructions."},{"@id":"unece:pollingCapabilityIndicator","@type":["rdf:Property","owl:DatatypeProperty"],"rdfs:label":"pollingCapabilityIndicator","schema:rangeIncludes":{"@id":"schema:Boolean"},"schema:domainIncludes":{"@id":"unece:Equipment"},"rdfs:comment":"The indication of whether or not this OEM equipment has a polling capability."},{"@id":"unece:pollingRateMeasure","@type":["rdf:Property","owl:ObjectProperty"],"rdfs:label":"pollingRateMeasure","schema:rangeIncludes":{"@id":"unece:MeasureType"},"schema:domainIncludes":{"@id":"unece:Equipment"},"rdfs:comment":""}]}